@prefix dc: <http://purl.org/dc/elements/1.1/> .
@prefix dcam: <http://purl.org/dc/dcam/> .
@prefix dcmitype: <http://purl.org/dc/dcmitype/> .
@prefix dcterms: <http://purl.org/dc/terms/> .
@prefix foaf: <http://xmlns.com/foaf/0.1/> .
@prefix linkml: <https://w3id.org/linkml/> .
@prefix okn: <https://purl.org/okn/> .
@prefix okns: <https://purl.org/okn/schema/> .
@prefix owl: <http://www.w3.org/2002/07/owl#> .
@prefix pav: <http://purl.org/pav/> .
@prefix rdf: <http://www.w3.org/1999/02/22-rdf-syntax-ns#> .
@prefix rdfs: <http://www.w3.org/2000/01/rdf-schema#> .
@prefix sc: <http://shapechange.net/resources/ont/base#> .
@prefix schema1: <http://schema.org/> .
@prefix seegrid-basic: <http://def.seegrid.csiro.au/isotc211/iso19103/2005/basic#> .
@prefix seegrid-ci: <http://def.seegrid.csiro.au/isotc211/iso19115/2003/citation#> .
@prefix sh: <http://www.w3.org/ns/shacl#> .
@prefix shex: <http://www.w3.org/ns/shex#> .
@prefix skos: <http://www.w3.org/2004/02/skos/core#> .
@prefix xsd: <http://www.w3.org/2001/XMLSchema#> .

okns:base64binary a linkml:TypeDefinition ;
    skos:definition "Arbitrary Base64-encoded binary data." ;
    skos:inScheme okns:extended_types ;
    skos:note "added by Mahir Morshed <mmorshed@scripps.edu>",
        "used 'string' as base type since no 'binary' base type exists" ;
    linkml:base "string" ;
    linkml:definition_uri linkml:Base64binary ;
    linkml:uri xsd:hexBinary .

okns:curie a linkml:TypeDefinition ;
    dcterms:conformsTo "https://www.w3.org/TR/curie/" ;
    skos:definition "a compact URI" ;
    skos:editorialNote "If you are authoring schemas in LinkML YAML, the type is referenced with the lower case \"curie\"." ;
    skos:inScheme linkml:types ;
    skos:note "in RDF serializations this MUST be expanded to a URI",
        "in non-RDF serializations MAY be serialized as the compact representation" ;
    linkml:base "Curie" ;
    linkml:imported_from "linkml:types" ;
    linkml:repr "str" ;
    linkml:definition_uri linkml:Curie ;
    linkml:uri xsd:string .

okns:date_or_datetime a linkml:TypeDefinition ;
    skos:definition "Either a date or a datetime" ;
    skos:editorialNote "If you are authoring schemas in LinkML YAML, the type is referenced with the lower case \"date_or_datetime\"." ;
    skos:inScheme linkml:types ;
    linkml:base "str" ;
    linkml:imported_from "linkml:types" ;
    linkml:repr "str" ;
    linkml:definition_uri linkml:DateOrDatetime ;
    linkml:uri linkml:DateOrDatetime .

okns:datetime a linkml:TypeDefinition ;
    skos:definition "The combination of a date and time" ;
    skos:editorialNote "If you are authoring schemas in LinkML YAML, the type is referenced with the lower case \"datetime\"." ;
    skos:exactMatch schema1:DateTime ;
    skos:inScheme linkml:types ;
    linkml:base "XSDDateTime" ;
    linkml:imported_from "linkml:types" ;
    linkml:repr "str" ;
    linkml:definition_uri linkml:Datetime ;
    linkml:uri xsd:dateTime .

okns:dct_Box a linkml:TypeDefinition ;
    dcterms:source dcterms: ;
    dcterms:title "DCMI Box" ;
    rdfs:seeAlso <https://www.dublincore.org/specifications/dublin-core/dcmi-box/> ;
    skos:definition "The set of regions in space defined by their geographic coordinates according to the DCMI Box Encoding Scheme." ;
    skos:inScheme okns:dc ;
    linkml:base "str" ;
    linkml:definition_uri okns:DctBox ;
    linkml:typeof okns:string ;
    linkml:uri dcterms:Box .

okns:dct_ISO3166 a linkml:TypeDefinition ;
    dcterms:source dcterms: ;
    dcterms:title "ISO 3166" ;
    rdfs:seeAlso <https://www.iso.org/obp/ui/#search> ;
    skos:definition "The set of codes listed in ISO 3166-1 for the representation of names of countries." ;
    skos:inScheme okns:dc ;
    linkml:base "str" ;
    linkml:definition_uri okns:DctISO3166 ;
    linkml:typeof okns:string ;
    linkml:uri dcterms:ISO3166 .

okns:dct_ISO639_2 a linkml:TypeDefinition ;
    dcterms:source dcterms: ;
    dcterms:title "ISO 639-2" ;
    rdfs:seeAlso <http://lcweb.loc.gov/standards/iso639-2/langhome.html> ;
    skos:definition "The three-letter alphabetic codes listed in ISO639-2 for the representation of names of languages." ;
    skos:inScheme okns:dc ;
    linkml:base "str" ;
    linkml:definition_uri okns:DctISO639-2 ;
    linkml:typeof okns:string ;
    linkml:uri dcterms:ISO639-2 .

okns:dct_ISO639_3 a linkml:TypeDefinition ;
    dcterms:source dcterms: ;
    dcterms:title "ISO 639-3" ;
    rdfs:seeAlso <http://www.sil.org/iso639-3/> ;
    skos:definition "The set of three-letter codes listed in ISO 639-3 for the representation of names of languages." ;
    skos:inScheme okns:dc ;
    linkml:base "str" ;
    linkml:definition_uri okns:DctISO639-3 ;
    linkml:typeof okns:string ;
    linkml:uri dcterms:ISO639-3 .

okns:dct_Period a linkml:TypeDefinition ;
    dcterms:source dcterms: ;
    dcterms:title "DCMI Period" ;
    rdfs:seeAlso <https://www.dublincore.org/specifications/dublin-core/dcmi-period/> ;
    skos:definition "The set of time intervals defined by their limits according to the DCMI Period Encoding Scheme." ;
    skos:inScheme okns:dc ;
    linkml:base "str" ;
    linkml:definition_uri okns:DctPeriod ;
    linkml:typeof okns:string ;
    linkml:uri dcterms:Period .

okns:dct_Point a linkml:TypeDefinition ;
    dcterms:source dcterms: ;
    dcterms:title "DCMI Point" ;
    rdfs:seeAlso <https://www.dublincore.org/specifications/dublin-core/dcmi-point/> ;
    skos:definition "The set of points in space defined by their geographic coordinates according to the DCMI Point Encoding Scheme." ;
    skos:inScheme okns:dc ;
    linkml:base "str" ;
    linkml:definition_uri okns:DctPoint ;
    linkml:typeof okns:string ;
    linkml:uri dcterms:Point .

okns:dct_RFC1766 a linkml:TypeDefinition ;
    dcterms:source dcterms: ;
    dcterms:title "RFC 1766" ;
    rdfs:seeAlso <http://www.ietf.org/rfc/rfc1766.txt> ;
    skos:definition "The set of tags, constructed according to RFC 1766, for the identification of languages." ;
    skos:inScheme okns:dc ;
    linkml:base "str" ;
    linkml:definition_uri okns:DctRFC1766 ;
    linkml:typeof okns:string ;
    linkml:uri dcterms:RFC1766 .

okns:dct_RFC3066 a linkml:TypeDefinition ;
    dcterms:source dcterms: ;
    dcterms:title "RFC 3066" ;
    rdfs:seeAlso <http://www.ietf.org/rfc/rfc3066.txt> ;
    skos:definition "RFC 3066 has been obsoleted by RFC 4646." ;
    skos:inScheme okns:dc ;
    skos:note "description: The set of tags constructed according to RFC 3066 for the identification of languages." ;
    linkml:base "str" ;
    linkml:definition_uri okns:DctRFC3066 ;
    linkml:typeof okns:string ;
    linkml:uri dcterms:RFC3066 .

okns:dct_RFC4646 a linkml:TypeDefinition ;
    dcterms:source dcterms: ;
    dcterms:title "RFC 4646" ;
    rdfs:seeAlso <http://www.ietf.org/rfc/rfc4646.txt> ;
    skos:definition "RFC 4646 obsoletes RFC 3066." ;
    skos:inScheme okns:dc ;
    skos:note "description: The set of tags constructed according to RFC 4646 for the identification of languages." ;
    linkml:base "str" ;
    linkml:definition_uri okns:DctRFC4646 ;
    linkml:typeof okns:string ;
    linkml:uri dcterms:RFC4646 .

okns:dct_RFC5646 a linkml:TypeDefinition ;
    dcterms:source dcterms: ;
    dcterms:title "RFC 5646" ;
    rdfs:seeAlso <http://www.ietf.org/rfc/rfc5646.txt> ;
    skos:definition "RFC 5646 obsoletes RFC 4646." ;
    skos:inScheme okns:dc ;
    skos:note "description: The set of tags constructed according to RFC 5646 for the identification of languages." ;
    linkml:base "str" ;
    linkml:definition_uri okns:DctRFC5646 ;
    linkml:typeof okns:string ;
    linkml:uri dcterms:RFC5646 .

okns:dct_URI a linkml:TypeDefinition ;
    dcterms:source dcterms: ;
    dcterms:title "URI" ;
    rdfs:seeAlso <http://www.ietf.org/rfc/rfc3986.txt> ;
    skos:definition "The set of identifiers constructed according to the generic syntax for Uniform Resource Identifiers as specified by the Internet Engineering Task Force." ;
    skos:inScheme okns:dc ;
    linkml:base "str" ;
    linkml:definition_uri okns:DctURI ;
    linkml:typeof okns:string ;
    linkml:uri dcterms:URI .

okns:dct_W3CDTF a linkml:TypeDefinition ;
    dcterms:source dcterms: ;
    dcterms:title "W3C-DTF" ;
    rdfs:seeAlso <http://www.w3.org/TR/NOTE-datetime> ;
    skos:definition "The set of dates and times constructed according to the W3C Date and Time Formats Specification." ;
    skos:inScheme okns:dc ;
    linkml:base "str" ;
    linkml:definition_uri okns:DctW3CDTF ;
    linkml:typeof okns:string ;
    linkml:uri dcterms:W3CDTF .

okns:float16 a linkml:TypeDefinition ;
    rdfs:seeAlso <https://numpy.org/doc/stable/reference/arrays.scalars.html#numpy.half> ;
    skos:altLabel "e",
        "half" ;
    skos:definition "A 16-bit floating point number" ;
    skos:inScheme okns:extended_types ;
    linkml:base "float" ;
    linkml:definition_uri linkml:Float16 ;
    linkml:typeof okns:float ;
    linkml:uri xsd:float .

okns:float32 a linkml:TypeDefinition ;
    rdfs:seeAlso <https://numpy.org/doc/stable/reference/arrays.scalars.html#numpy.float32> ;
    skos:altLabel "f" ;
    skos:definition "A 32-bit floating point number" ;
    skos:inScheme okns:extended_types ;
    linkml:base "float" ;
    linkml:definition_uri linkml:Float32 ;
    linkml:typeof okns:float ;
    linkml:uri xsd:float .

okns:float64 a linkml:TypeDefinition ;
    rdfs:seeAlso <https://numpy.org/doc/stable/reference/arrays.scalars.html#numpy.float64> ;
    skos:altLabel "d" ;
    skos:definition "A 64-bit floating point number" ;
    skos:inScheme okns:extended_types ;
    linkml:base "float" ;
    linkml:definition_uri linkml:Float64 ;
    linkml:typeof okns:float ;
    linkml:uri xsd:float .

okns:hexbinary a linkml:TypeDefinition ;
    skos:definition "Arbitrary hex-encoded binary data." ;
    skos:inScheme okns:extended_types ;
    skos:note "added by Mahir Morshed <mmorshed@scripps.edu>",
        "used 'string' as base type since no 'binary' base type exists" ;
    linkml:base "string" ;
    linkml:definition_uri linkml:Hexbinary ;
    linkml:uri xsd:hexBinary .

okns:int16 a linkml:TypeDefinition ;
    rdfs:seeAlso <https://numpy.org/doc/stable/reference/arrays.scalars.html#numpy.short> ;
    skos:altLabel "h",
        "short" ;
    skos:definition "A 16-bit signed integer" ;
    skos:inScheme okns:extended_types ;
    skos:note "uri added by Mahir Morshed <mmorshed@scripps.edu>" ;
    linkml:base "int" ;
    linkml:definition_uri linkml:Int16 ;
    linkml:maximum_value "32767"^^<https://purl.org/okn/schema/@id> ;
    linkml:minimum_value "-32768"^^<https://purl.org/okn/schema/@id> ;
    linkml:typeof okns:signedinteger ;
    linkml:uri xsd:short .

okns:int32 a linkml:TypeDefinition ;
    rdfs:seeAlso <https://numpy.org/doc/stable/reference/arrays.scalars.html#numpy.intc> ;
    skos:altLabel "i",
        "intc" ;
    skos:definition "A 32-bit signed integer" ;
    skos:inScheme okns:extended_types ;
    skos:note "uri added by Mahir Morshed <mmorshed@scripps.edu>" ;
    linkml:base "int" ;
    linkml:definition_uri linkml:Int32 ;
    linkml:maximum_value "2147483647"^^<https://purl.org/okn/schema/@id> ;
    linkml:minimum_value "-2147483648"^^<https://purl.org/okn/schema/@id> ;
    linkml:typeof okns:signedinteger ;
    linkml:uri xsd:int .

okns:int64 a linkml:TypeDefinition ;
    rdfs:seeAlso <https://numpy.org/doc/stable/reference/arrays.scalars.html#numpy.int_> ;
    skos:altLabel "int_",
        "l",
        "long" ;
    skos:definition "A 64-bit signed integer" ;
    skos:inScheme okns:extended_types ;
    skos:note "uri added by Mahir Morshed <mmorshed@scripps.edu>" ;
    linkml:base "int" ;
    linkml:definition_uri linkml:Int64 ;
    linkml:maximum_value "9223372036854775807"^^<https://purl.org/okn/schema/@id> ;
    linkml:minimum_value "-9223372036854775808"^^<https://purl.org/okn/schema/@id> ;
    linkml:typeof okns:signedinteger ;
    linkml:uri xsd:long .

okns:int8 a linkml:TypeDefinition ;
    rdfs:seeAlso <https://numpy.org/doc/stable/reference/arrays.scalars.html#numpy.byte> ;
    skos:altLabel "b",
        "byte" ;
    skos:definition "An 8-bit signed integer" ;
    skos:inScheme okns:extended_types ;
    skos:note "uri added by Mahir Morshed <mmorshed@scripps.edu>" ;
    linkml:base "int" ;
    linkml:definition_uri linkml:Int8 ;
    linkml:maximum_value "127"^^<https://purl.org/okn/schema/@id> ;
    linkml:minimum_value "-128"^^<https://purl.org/okn/schema/@id> ;
    linkml:typeof okns:signedinteger ;
    linkml:uri xsd:byte .

okns:jsonpath a linkml:TypeDefinition ;
    dcterms:conformsTo "https://www.ietf.org/archive/id/draft-goessner-dispatch-jsonpath-00.html" ;
    skos:definition "A string encoding a JSON Path. The value of the string MUST conform to JSON Point syntax and SHOULD dereference to zero or more valid objects within the current instance document when encoded in tree form." ;
    skos:editorialNote "If you are authoring schemas in LinkML YAML, the type is referenced with the lower case \"jsonpath\"." ;
    skos:inScheme linkml:types ;
    linkml:base "str" ;
    linkml:imported_from "linkml:types" ;
    linkml:repr "str" ;
    linkml:definition_uri linkml:Jsonpath ;
    linkml:uri xsd:string .

okns:jsonpointer a linkml:TypeDefinition ;
    dcterms:conformsTo "https://datatracker.ietf.org/doc/html/rfc6901" ;
    skos:definition "A string encoding a JSON Pointer. The value of the string MUST conform to JSON Point syntax and SHOULD dereference to a valid object within the current instance document when encoded in tree form." ;
    skos:editorialNote "If you are authoring schemas in LinkML YAML, the type is referenced with the lower case \"jsonpointer\"." ;
    skos:inScheme linkml:types ;
    linkml:base "str" ;
    linkml:imported_from "linkml:types" ;
    linkml:repr "str" ;
    linkml:definition_uri linkml:Jsonpointer ;
    linkml:uri xsd:string .

okns:langrange a linkml:SlotDefinition ;
    skos:definition "Used to refer to a subset of strings containing a particular language tag." ;
    skos:inScheme okns:extended_types ;
    skos:mappingRelation rdf:langRange ;
    skos:note "added by Mahir Morshed <mmorshed@scripps.edu>" ;
    linkml:definition_uri linkml:langrange ;
    linkml:range okns:string ;
    linkml:slot_uri rdf:langRange .

okns:language a linkml:TypeDefinition ;
    skos:definition "Formal natural language identifier, as defined by [BCP 47] (currently represented by [RFC 4646] and [RFC 4647]) or its successor(s)." ;
    skos:inScheme okns:extended_types ;
    skos:note "added by Mahir Morshed <mmorshed@scripps.edu>" ;
    linkml:base "str" ;
    linkml:definition_uri linkml:Language ;
    linkml:typeof okns:token ;
    linkml:uri xsd:language .

okns:length a linkml:SlotDefinition ;
    skos:definition "Number of units of length, where units of length varies depending on the type that is being derived from." ;
    skos:inScheme okns:extended_types ;
    skos:mappingRelation xsd:length ;
    skos:note "added by Mahir Morshed <mmorshed@scripps.edu>" ;
    linkml:definition_uri linkml:length ;
    linkml:range okns:string ;
    linkml:slot_uri xsd:length .

okns:maxexclusive a linkml:SlotDefinition ;
    skos:definition "Exclusive upper bound of the ·value space· for a datatype with the ordered property." ;
    skos:inScheme okns:extended_types ;
    skos:mappingRelation xsd:maxExclusive ;
    skos:note "added by Mahir Morshed <mmorshed@scripps.edu>" ;
    linkml:definition_uri linkml:maxexclusive ;
    linkml:range okns:string ;
    linkml:slot_uri xsd:maxExclusive .

okns:maxlength a linkml:SlotDefinition ;
    skos:definition "Maximum number of units of length, where units of length varies depending on the type that is being derived from." ;
    skos:inScheme okns:extended_types ;
    skos:mappingRelation xsd:maxLength ;
    skos:note "added by Mahir Morshed <mmorshed@scripps.edu>" ;
    linkml:definition_uri linkml:maxlength ;
    linkml:range okns:string ;
    linkml:slot_uri xsd:maxLength .

okns:minexclusive a linkml:SlotDefinition ;
    skos:definition "Exclusive lower bound of the ·value space· for a datatype with the ordered property." ;
    skos:inScheme okns:extended_types ;
    skos:mappingRelation xsd:minExclusive ;
    skos:note "added by Mahir Morshed <mmorshed@scripps.edu>" ;
    linkml:definition_uri linkml:minexclusive ;
    linkml:range okns:string ;
    linkml:slot_uri xsd:minExclusive .

okns:minlength a linkml:SlotDefinition ;
    skos:definition "Minimum number of units of length, where units of length varies depending on the type that is being derived from." ;
    skos:inScheme okns:extended_types ;
    skos:mappingRelation xsd:minLength ;
    skos:note "added by Mahir Morshed <mmorshed@scripps.edu>" ;
    linkml:definition_uri linkml:minlength ;
    linkml:range okns:string ;
    linkml:slot_uri xsd:minLength .

okns:name a linkml:TypeDefinition ;
    skos:definition "XML Name." ;
    skos:inScheme okns:extended_types ;
    skos:note "added by Mahir Morshed <mmorshed@scripps.edu>" ;
    linkml:base "str" ;
    linkml:definition_uri linkml:Name ;
    linkml:typeof okns:token ;
    linkml:uri xsd:Name .

okns:ncname a linkml:TypeDefinition ;
    skos:definition "Prefix part of CURIE" ;
    skos:editorialNote "If you are authoring schemas in LinkML YAML, the type is referenced with the lower case \"ncname\"." ;
    skos:inScheme linkml:types ;
    linkml:base "NCName" ;
    linkml:imported_from "linkml:types" ;
    linkml:repr "str" ;
    linkml:definition_uri linkml:Ncname ;
    linkml:uri xsd:string .

okns:negativeinteger a linkml:TypeDefinition ;
    skos:definition "An integer that is negative" ;
    skos:inScheme okns:extended_types ;
    skos:note "added by Mahir Morshed <mmorshed@scripps.edu>" ;
    linkml:base "int" ;
    linkml:definition_uri linkml:Negativeinteger ;
    linkml:maximum_value "-1"^^<https://purl.org/okn/schema/@id> ;
    linkml:typeof okns:integer ;
    linkml:uri xsd:negativeInteger .

okns:nmtoken a linkml:TypeDefinition ;
    skos:definition "NMTOKEN attribute type from [XML]." ;
    skos:inScheme okns:extended_types ;
    skos:note "added by Mahir Morshed <mmorshed@scripps.edu>" ;
    linkml:base "str" ;
    linkml:definition_uri linkml:Nmtoken ;
    linkml:typeof okns:token ;
    linkml:uri xsd:NMTOKEN .

okns:nodeidentifier a linkml:TypeDefinition ;
    skos:definition "A URI, CURIE or BNODE that represents a node in a model." ;
    skos:editorialNote "If you are authoring schemas in LinkML YAML, the type is referenced with the lower case \"nodeidentifier\"." ;
    skos:inScheme linkml:types ;
    linkml:base "NodeIdentifier" ;
    linkml:imported_from "linkml:types" ;
    linkml:repr "str" ;
    linkml:definition_uri linkml:Nodeidentifier ;
    linkml:uri shex:nonLiteral .

okns:nonpositiveinteger a linkml:TypeDefinition ;
    skos:definition "An integer that is not positive" ;
    skos:inScheme okns:extended_types ;
    skos:note "added by Mahir Morshed <mmorshed@scripps.edu>" ;
    linkml:base "int" ;
    linkml:definition_uri linkml:Nonpositiveinteger ;
    linkml:maximum_value "0"^^<https://purl.org/okn/schema/@id> ;
    linkml:typeof okns:integer ;
    linkml:uri xsd:nonPositiveInteger .

okns:objectidentifier a linkml:TypeDefinition ;
    skos:definition "A URI or CURIE that represents an object in the model." ;
    skos:editorialNote "If you are authoring schemas in LinkML YAML, the type is referenced with the lower case \"objectidentifier\"." ;
    skos:inScheme linkml:types ;
    skos:note "Used for inheritance and type checking" ;
    linkml:base "ElementIdentifier" ;
    linkml:imported_from "linkml:types" ;
    linkml:repr "str" ;
    linkml:definition_uri linkml:Objectidentifier ;
    linkml:uri shex:iri .

okns:rational a linkml:TypeDefinition ;
    skos:definition "Rational number." ;
    skos:inScheme okns:extended_types ;
    skos:note "added by Mahir Morshed <mmorshed@scripps.edu>" ;
    linkml:base "Decimal" ;
    linkml:definition_uri linkml:Rational ;
    linkml:typeof okns:decimal ;
    linkml:uri owl:rational .

okns:rdf_HTML a linkml:TypeDefinition ;
    dcterms:source rdf: ;
    dcterms:title "HTML" ;
    rdfs:seeAlso <http://www.w3.org/TR/rdf11-concepts/#section-html> ;
    skos:definition "The datatype of RDF literals storing fragments of HTML content" ;
    skos:inScheme okns:owl-rdf-rdfs ;
    linkml:base "str" ;
    linkml:definition_uri okns:RdfHTML ;
    linkml:typeof okns:string ;
    linkml:uri rdf:HTML .

okns:rdf_JSON a linkml:TypeDefinition ;
    dcterms:source rdf: ;
    dcterms:title "JSON" ;
    rdfs:seeAlso <https://www.w3.org/TR/json-ld11/#the-rdf-json-datatype> ;
    skos:definition "The datatype of RDF literals storing JSON content." ;
    skos:inScheme okns:owl-rdf-rdfs ;
    linkml:base "str" ;
    linkml:definition_uri okns:RdfJSON ;
    linkml:typeof okns:string ;
    linkml:uri rdf:JSON .

okns:rdf_PlainLiteral a linkml:TypeDefinition ;
    dcterms:source rdf: ;
    dcterms:title "PlainLiteral" ;
    rdfs:seeAlso <http://www.w3.org/TR/rdf-plain-literal/> ;
    skos:definition "The class of plain (i.e. untyped) literal values, as used in RIF and OWL 2" ;
    skos:inScheme okns:owl-rdf-rdfs ;
    linkml:base "str" ;
    linkml:definition_uri okns:RdfPlainLiteral ;
    linkml:typeof okns:string ;
    linkml:uri rdf:PlainLiteral .

okns:rdf_XMLLiteral a linkml:TypeDefinition ;
    dcterms:source rdf: ;
    dcterms:title "XMLLiteral" ;
    skos:definition "The datatype of XML literal values." ;
    skos:inScheme okns:owl-rdf-rdfs ;
    linkml:base "str" ;
    linkml:definition_uri okns:RdfXMLLiteral ;
    linkml:typeof okns:string ;
    linkml:uri rdf:XMLLiteral .

okns:rdf_langString a linkml:TypeDefinition ;
    dcterms:source rdf: ;
    dcterms:title "langString" ;
    rdfs:seeAlso <http://www.w3.org/TR/rdf11-concepts/#section-Graph-Literal> ;
    skos:definition "The datatype of language-tagged string values" ;
    skos:inScheme okns:owl-rdf-rdfs ;
    linkml:base "str" ;
    linkml:definition_uri okns:RdfLangString ;
    linkml:typeof okns:string ;
    linkml:uri rdf:langString .

okns:real a linkml:TypeDefinition ;
    skos:definition "Real number." ;
    skos:inScheme okns:extended_types ;
    skos:note "added by Mahir Morshed <mmorshed@scripps.edu>" ;
    linkml:base "Decimal" ;
    linkml:definition_uri linkml:Real ;
    linkml:typeof okns:decimal ;
    linkml:uri owl:real .

okns:sc_Sign a linkml:TypeDefinition ;
    skos:inScheme okns:sc ;
    linkml:base "str" ;
    linkml:definition_uri okns:ScSign ;
    linkml:typeof okns:string ;
    linkml:uri sc:Sign .

okns:seegrid_basic_Boolean a linkml:TypeDefinition ;
    dcterms:source <http://def.seegrid.csiro.au/isotc211/iso19103/2005/basic> ;
    dcterms:title "boolean" ;
    skos:definition "Truth value. Most valuable in the predicate calculus, where items are either True or False, unless they are ill formed." ;
    skos:inScheme okns:seegrid-iso19115 ;
    linkml:base "str" ;
    linkml:definition_uri okns:Seegrid-basicBoolean ;
    linkml:typeof okns:string ;
    linkml:uri seegrid-basic:Boolean .

okns:seegrid_basic_CharacterString a linkml:TypeDefinition ;
    dcterms:source <http://def.seegrid.csiro.au/isotc211/iso19103/2005/basic> ;
    dcterms:title "characterString" ;
    skos:definition "sequence of characters" ;
    skos:inScheme okns:seegrid-iso19115 ;
    linkml:base "str" ;
    linkml:definition_uri okns:Seegrid-basicCharacterString ;
    linkml:typeof okns:string ;
    linkml:uri seegrid-basic:CharacterString .

okns:seegrid_basic_Date a linkml:TypeDefinition ;
    dcterms:source <http://def.seegrid.csiro.au/isotc211/iso19103/2005/basic> ;
    dcterms:title "date" ;
    skos:definition "Temporal position expressed with precision of days" ;
    skos:inScheme okns:seegrid-iso19115 ;
    linkml:base "str" ;
    linkml:definition_uri okns:Seegrid-basicDate ;
    linkml:typeof okns:string ;
    linkml:uri seegrid-basic:Date .

okns:seegrid_basic_DateTime a linkml:TypeDefinition ;
    dcterms:source <http://def.seegrid.csiro.au/isotc211/iso19103/2005/basic> ;
    dcterms:title "dateTime" ;
    skos:definition "Temporal position expressed as a time and date" ;
    skos:inScheme okns:seegrid-iso19115 ;
    linkml:base "str" ;
    linkml:definition_uri okns:Seegrid-basicDateTime ;
    linkml:typeof okns:string ;
    linkml:uri seegrid-basic:DateTime .

okns:seegrid_basic_Decimal a linkml:TypeDefinition ;
    dcterms:source <http://def.seegrid.csiro.au/isotc211/iso19103/2005/basic> ;
    dcterms:title "decimal" ;
    skos:definition "The usually finite representation of a decimal number. It differs from the common binary Real implementation in that it can represent 1/10 (one-tenth) without error, while binary real representation can only represent powers of 1/2 (one-half) exactly. Since many currencies are decimal, these representations are preferred in dealing with such moneys. This is also true for mile markers, which are often given in decimals.␊␊Can be thought of as an integer part followed by a fractional part given in multiples of powers of 1/10 (tenths)." ;
    skos:inScheme okns:seegrid-iso19115 ;
    linkml:base "str" ;
    linkml:definition_uri okns:Seegrid-basicDecimal ;
    linkml:typeof okns:string ;
    linkml:uri seegrid-basic:Decimal .

okns:seegrid_basic_ISOClassName a linkml:TypeDefinition ;
    skos:inScheme okns:seegrid-iso19115 ;
    linkml:base "str" ;
    linkml:definition_uri okns:Seegrid-basicISOClassName ;
    linkml:typeof okns:string ;
    linkml:uri seegrid-basic:ISOClassName .

okns:seegrid_basic_Integer a linkml:TypeDefinition ;
    dcterms:source <http://def.seegrid.csiro.au/isotc211/iso19103/2005/basic> ;
    dcterms:title "integer" ;
    skos:definition "An exact integer value, with no fractional part." ;
    skos:inScheme okns:seegrid-iso19115 ;
    linkml:base "str" ;
    linkml:definition_uri okns:Seegrid-basicInteger ;
    linkml:typeof okns:string ;
    linkml:uri seegrid-basic:Integer .

okns:seegrid_basic_LocalName a linkml:TypeDefinition ;
    dcterms:source <http://def.seegrid.csiro.au/isotc211/iso19103/2005/basic> ;
    dcterms:title "localName" ;
    skos:definition "Name in some local context" ;
    skos:inScheme okns:seegrid-iso19115 ;
    linkml:base "str" ;
    linkml:definition_uri okns:Seegrid-basicLocalName ;
    linkml:typeof okns:string ;
    linkml:uri seegrid-basic:LocalName .

okns:seegrid_basic_Number a linkml:TypeDefinition ;
    dcterms:source <http://def.seegrid.csiro.au/isotc211/iso19103/2005/basic> ;
    dcterms:title "Number" ;
    skos:definition "Note: integer is a specialization of decimal" ;
    skos:inScheme okns:seegrid-iso19115 ;
    skos:note "description: The set of numbers" ;
    linkml:base "str" ;
    linkml:definition_uri okns:Seegrid-basicNumber ;
    linkml:typeof okns:string ;
    linkml:uri seegrid-basic:Number .

okns:seegrid_basic_Real a linkml:TypeDefinition ;
    dcterms:source <http://def.seegrid.csiro.au/isotc211/iso19103/2005/basic> ;
    dcterms:title "realNumber" ;
    skos:definition "The common binary Real finite implementation using base 2. Since such reals can approximate any measure where absolute accuracy is not possible, this form of numeric is most often used for measures. In cases were absolute accuracy is needed, such as currencies, then a decimal representation may be preferred (assuming the currency is decimal, such as the US dollar, British pound, etc.). Where there are no subunits possible, Integer numbers may be preferred.  ␊␊Can be thought of as an integer part followed by a fractional part given in multiples of powers of 1/2 (halves)." ;
    skos:inScheme okns:seegrid-iso19115 ;
    linkml:base "str" ;
    linkml:definition_uri okns:Seegrid-basicReal ;
    linkml:typeof okns:string ;
    linkml:uri seegrid-basic:Real .

okns:sparqlpath a linkml:TypeDefinition ;
    dcterms:conformsTo "https://www.w3.org/TR/sparql11-query/#propertypaths" ;
    skos:definition "A string encoding a SPARQL Property Path. The value of the string MUST conform to SPARQL syntax and SHOULD dereference to zero or more valid objects within the current instance document when encoded as RDF." ;
    skos:editorialNote "If you are authoring schemas in LinkML YAML, the type is referenced with the lower case \"sparqlpath\"." ;
    skos:inScheme linkml:types ;
    linkml:base "str" ;
    linkml:imported_from "linkml:types" ;
    linkml:repr "str" ;
    linkml:definition_uri linkml:Sparqlpath ;
    linkml:uri xsd:string .

okns:time a linkml:TypeDefinition ;
    skos:definition "A time object represents a (local) time of day, independent of any particular day" ;
    skos:editorialNote "If you are authoring schemas in LinkML YAML, the type is referenced with the lower case \"time\".",
        "URI is dateTime because OWL reasoners do not work with straight date or time" ;
    skos:exactMatch schema1:Time ;
    skos:inScheme linkml:types ;
    linkml:base "XSDTime" ;
    linkml:imported_from "linkml:types" ;
    linkml:repr "str" ;
    linkml:definition_uri linkml:Time ;
    linkml:uri xsd:time .

okns:uint16 a linkml:TypeDefinition ;
    skos:altLabel "H",
        "ushort" ;
    skos:definition "A 16-bit unsigned integer" ;
    skos:inScheme okns:extended_types ;
    skos:note "uri added by Mahir Morshed <mmorshed@scripps.edu>" ;
    linkml:base "int" ;
    linkml:definition_uri linkml:Uint16 ;
    linkml:maximum_value "65535"^^<https://purl.org/okn/schema/@id> ;
    linkml:minimum_value "0"^^<https://purl.org/okn/schema/@id> ;
    linkml:typeof okns:unsignedinteger ;
    linkml:uri xsd:unsignedShort .

okns:uint32 a linkml:TypeDefinition ;
    skos:altLabel "I",
        "uintc" ;
    skos:definition "A 32-bit unsigned integer" ;
    skos:inScheme okns:extended_types ;
    skos:note "uri added by Mahir Morshed <mmorshed@scripps.edu>" ;
    linkml:base "int" ;
    linkml:definition_uri linkml:Uint32 ;
    linkml:maximum_value "4294967295"^^<https://purl.org/okn/schema/@id> ;
    linkml:minimum_value "0"^^<https://purl.org/okn/schema/@id> ;
    linkml:typeof okns:unsignedinteger ;
    linkml:uri xsd:unsignedInt .

okns:uint64 a linkml:TypeDefinition ;
    skos:altLabel "L",
        "uint_",
        "ulong" ;
    skos:definition "A 64-bit unsigned integer" ;
    skos:inScheme okns:extended_types ;
    skos:note "uri added by Mahir Morshed <mmorshed@scripps.edu>" ;
    linkml:base "int" ;
    linkml:definition_uri linkml:Uint64 ;
    linkml:maximum_value "18446744073709551615"^^<https://purl.org/okn/schema/@id> ;
    linkml:minimum_value "0"^^<https://purl.org/okn/schema/@id> ;
    linkml:typeof okns:unsignedinteger ;
    linkml:uri xsd:unsignedLong .

okns:uint8 a linkml:TypeDefinition ;
    rdfs:seeAlso <https://numpy.org/doc/stable/reference/arrays.scalars.html#numpy.uint8> ;
    skos:altLabel "B",
        "ubyte" ;
    skos:definition "An 8-bit unsigned integer" ;
    skos:inScheme okns:extended_types ;
    skos:note "uri added by Mahir Morshed <mmorshed@scripps.edu>" ;
    linkml:base "int" ;
    linkml:definition_uri linkml:Uint8 ;
    linkml:maximum_value "255"^^<https://purl.org/okn/schema/@id> ;
    linkml:minimum_value "0"^^<https://purl.org/okn/schema/@id> ;
    linkml:typeof okns:unsignedinteger ;
    linkml:uri xsd:unsignedByte .

okns:uriorcurie a linkml:TypeDefinition ;
    skos:definition "a URI or a CURIE" ;
    skos:editorialNote "If you are authoring schemas in LinkML YAML, the type is referenced with the lower case \"uriorcurie\"." ;
    skos:inScheme linkml:types ;
    linkml:base "URIorCURIE" ;
    linkml:imported_from "linkml:types" ;
    linkml:repr "str" ;
    linkml:definition_uri linkml:Uriorcurie ;
    linkml:uri xsd:anyURI .

okns:DcmitypeDataset a linkml:ClassDefinition ;
    dcterms:source dcmitype: ;
    dcterms:title "Dataset" ;
    skos:definition "Examples include lists, tables, and databases.  A dataset may be useful for direct machine processing." ;
    skos:inScheme okns:dc ;
    skos:mappingRelation dcmitype:Dataset ;
    skos:note "description: Data encoded in a defined structure." ;
    linkml:class_uri dcmitype:Dataset ;
    linkml:definition_uri okns:DcmitypeDataset ;
    linkml:slot_usage [ ] .

okns:DcmitypeEvent a linkml:ClassDefinition ;
    dcterms:source dcmitype: ;
    dcterms:title "Event" ;
    skos:definition "Metadata for an event provides descriptive information that is the basis for discovery of the purpose, location, duration, and responsible agents associated with an event. Examples include an exhibition, webcast, conference, workshop, open day, performance, battle, trial, wedding, tea party, conflagration." ;
    skos:inScheme okns:dc ;
    skos:mappingRelation dcmitype:Event ;
    skos:note "description: A non-persistent, time-based occurrence." ;
    linkml:class_uri dcmitype:Event ;
    linkml:definition_uri okns:DcmitypeEvent ;
    linkml:slot_usage [ ] .

okns:DcmitypeInteractiveResource a linkml:ClassDefinition ;
    dcterms:source dcmitype: ;
    dcterms:title "Interactive Resource" ;
    skos:definition "Examples include forms on Web pages, applets, multimedia learning objects, chat services, or virtual reality environments." ;
    skos:inScheme okns:dc ;
    skos:mappingRelation dcmitype:InteractiveResource ;
    skos:note "description: A resource requiring interaction from the user to be understood, executed, or experienced." ;
    linkml:class_uri dcmitype:InteractiveResource ;
    linkml:definition_uri okns:DcmitypeInteractiveResource ;
    linkml:slot_usage [ ] .

okns:DcmitypeMovingImage a linkml:ClassDefinition ;
    dcterms:source dcmitype: ;
    dcterms:title "Moving Image" ;
    skos:definition "Examples include animations, movies, television programs, videos, zoetropes, or visual output from a simulation.  Instances of the type Moving Image must also be describable as instances of the broader type Image." ;
    skos:inScheme okns:dc ;
    skos:mappingRelation dcmitype:MovingImage ;
    skos:note "description: A series of visual representations imparting an impression of motion when shown in succession." ;
    linkml:class_uri dcmitype:MovingImage ;
    linkml:definition_uri okns:DcmitypeMovingImage ;
    linkml:is_a okns:DcmitypeImage ;
    linkml:slot_usage [ ] .

okns:DcmitypePhysicalObject a linkml:ClassDefinition ;
    dcterms:source dcmitype: ;
    dcterms:title "Physical Object" ;
    skos:definition "Note that digital representations of, or surrogates for, these objects should use Image, Text or one of the other types." ;
    skos:inScheme okns:dc ;
    skos:mappingRelation dcmitype:PhysicalObject ;
    skos:note "description: An inanimate, three-dimensional object or substance." ;
    linkml:class_uri dcmitype:PhysicalObject ;
    linkml:definition_uri okns:DcmitypePhysicalObject ;
    linkml:slot_usage [ ] .

okns:DcmitypeService a linkml:ClassDefinition ;
    dcterms:source dcmitype: ;
    dcterms:title "Service" ;
    skos:definition "Examples include a photocopying service, a banking service, an authentication service, interlibrary loans, a Z39.50 or Web server." ;
    skos:inScheme okns:dc ;
    skos:mappingRelation dcmitype:Service ;
    skos:note "description: A system that provides one or more functions." ;
    linkml:class_uri dcmitype:Service ;
    linkml:definition_uri okns:DcmitypeService ;
    linkml:slot_usage [ ] .

okns:DcmitypeSoftware a linkml:ClassDefinition ;
    dcterms:source dcmitype: ;
    dcterms:title "Software" ;
    skos:definition "Examples include a C source file, MS-Windows .exe executable, or Perl script." ;
    skos:inScheme okns:dc ;
    skos:mappingRelation dcmitype:Software ;
    skos:note "description: A computer program in source or compiled form." ;
    linkml:class_uri dcmitype:Software ;
    linkml:definition_uri okns:DcmitypeSoftware ;
    linkml:slot_usage [ ] .

okns:DcmitypeSound a linkml:ClassDefinition ;
    dcterms:source dcmitype: ;
    dcterms:title "Sound" ;
    skos:definition "Examples include a music playback file format, an audio compact disc, and recorded speech or sounds." ;
    skos:inScheme okns:dc ;
    skos:mappingRelation dcmitype:Sound ;
    skos:note "description: A resource primarily intended to be heard." ;
    linkml:class_uri dcmitype:Sound ;
    linkml:definition_uri okns:DcmitypeSound ;
    linkml:slot_usage [ ] .

okns:DcmitypeStillImage a linkml:ClassDefinition ;
    dcterms:source dcmitype: ;
    dcterms:title "Still Image" ;
    skos:definition "Examples include paintings, drawings, graphic designs, plans and maps. Recommended best practice is to assign the type Text to images of textual materials. Instances of the type Still Image must also be describable as instances of the broader type Image." ;
    skos:inScheme okns:dc ;
    skos:mappingRelation dcmitype:StillImage ;
    skos:note "description: A static visual representation." ;
    linkml:class_uri dcmitype:StillImage ;
    linkml:definition_uri okns:DcmitypeStillImage ;
    linkml:is_a okns:DcmitypeImage ;
    linkml:slot_usage [ ] .

okns:DcmitypeText a linkml:ClassDefinition ;
    dcterms:source dcmitype: ;
    dcterms:title "Text" ;
    skos:definition "Examples include books, letters, dissertations, poems, newspapers, articles, archives of mailing lists. Note that facsimiles or images of texts are still of the genre Text." ;
    skos:inScheme okns:dc ;
    skos:mappingRelation dcmitype:Text ;
    skos:note "description: A resource consisting primarily of words for reading." ;
    linkml:class_uri dcmitype:Text ;
    linkml:definition_uri okns:DcmitypeText ;
    linkml:slot_usage [ ] .

okns:DctAgent a linkml:ClassDefinition ;
    dcterms:source dcterms: ;
    dcterms:title "Agent" ;
    skos:definition "A resource that acts or has the power to act." ;
    skos:inScheme okns:dc ;
    skos:mappingRelation dcterms:Agent ;
    linkml:class_uri dcterms:Agent ;
    linkml:definition_uri okns:DctAgent ;
    linkml:slot_usage [ ] .

okns:DctBibliographicResource a linkml:ClassDefinition ;
    dcterms:source dcterms: ;
    dcterms:title "Bibliographic Resource" ;
    skos:definition "A book, article, or other documentary resource." ;
    skos:inScheme okns:dc ;
    skos:mappingRelation dcterms:BibliographicResource ;
    linkml:class_uri dcterms:BibliographicResource ;
    linkml:definition_uri okns:DctBibliographicResource ;
    linkml:slot_usage [ ] .

okns:DctFileFormat a linkml:ClassDefinition ;
    dcterms:source dcterms: ;
    dcterms:title "File Format" ;
    skos:definition "A digital resource format." ;
    skos:inScheme okns:dc ;
    skos:mappingRelation dcterms:FileFormat ;
    linkml:class_uri dcterms:FileFormat ;
    linkml:definition_uri okns:DctFileFormat ;
    linkml:is_a okns:DctMediaType ;
    linkml:slot_usage [ ] .

okns:DctFrequency a linkml:ClassDefinition ;
    dcterms:source dcterms: ;
    dcterms:title "Frequency" ;
    skos:definition "A rate at which something recurs." ;
    skos:inScheme okns:dc ;
    skos:mappingRelation dcterms:Frequency ;
    linkml:class_uri dcterms:Frequency ;
    linkml:definition_uri okns:DctFrequency ;
    linkml:slot_usage [ ] .

okns:DctJurisdiction a linkml:ClassDefinition ;
    dcterms:source dcterms: ;
    dcterms:title "Jurisdiction" ;
    skos:definition "The extent or range of judicial, law enforcement, or other authority." ;
    skos:inScheme okns:dc ;
    skos:mappingRelation dcterms:Jurisdiction ;
    linkml:class_uri dcterms:Jurisdiction ;
    linkml:definition_uri okns:DctJurisdiction ;
    linkml:is_a okns:DctLocationPeriodOrJurisdiction ;
    linkml:slot_usage [ ] .

okns:DctLicenseDocument a linkml:ClassDefinition ;
    dcterms:source dcterms: ;
    dcterms:title "License Document" ;
    skos:definition "A legal document giving official permission to do something with a resource." ;
    skos:inScheme okns:dc ;
    skos:mappingRelation dcterms:LicenseDocument ;
    linkml:class_uri dcterms:LicenseDocument ;
    linkml:definition_uri okns:DctLicenseDocument ;
    linkml:is_a okns:DctRightsStatement ;
    linkml:slot_usage [ ] .

okns:DctLinguisticSystem a linkml:ClassDefinition ;
    dcterms:source dcterms: ;
    dcterms:title "Linguistic System" ;
    skos:definition "Written, spoken, sign, and computer languages are linguistic systems." ;
    skos:inScheme okns:dc ;
    skos:mappingRelation dcterms:LinguisticSystem ;
    skos:note "description: A system of signs, symbols, sounds, gestures, or rules used in communication." ;
    linkml:class_uri dcterms:LinguisticSystem ;
    linkml:definition_uri okns:DctLinguisticSystem ;
    linkml:slot_usage [ ] .

okns:DctLocation a linkml:ClassDefinition ;
    dcterms:source dcterms: ;
    dcterms:title "Location" ;
    skos:definition "A spatial region or named place." ;
    skos:inScheme okns:dc ;
    skos:mappingRelation dcterms:Location ;
    linkml:class_uri dcterms:Location ;
    linkml:definition_uri okns:DctLocation ;
    linkml:is_a okns:DctLocationPeriodOrJurisdiction ;
    linkml:slot_usage [ ] .

okns:DctMethodOfAccrual a linkml:ClassDefinition ;
    dcterms:source dcterms: ;
    dcterms:title "Method of Accrual" ;
    skos:definition "A method by which resources are added to a collection." ;
    skos:inScheme okns:dc ;
    skos:mappingRelation dcterms:MethodOfAccrual ;
    linkml:class_uri dcterms:MethodOfAccrual ;
    linkml:definition_uri okns:DctMethodOfAccrual ;
    linkml:slot_usage [ ] .

okns:DctMethodOfInstruction a linkml:ClassDefinition ;
    dcterms:source dcterms: ;
    dcterms:title "Method of Instruction" ;
    skos:definition "A process that is used to engender knowledge, attitudes, and skills." ;
    skos:inScheme okns:dc ;
    skos:mappingRelation dcterms:MethodOfInstruction ;
    linkml:class_uri dcterms:MethodOfInstruction ;
    linkml:definition_uri okns:DctMethodOfInstruction ;
    linkml:slot_usage [ ] .

okns:DctPeriodOfTime a linkml:ClassDefinition ;
    dcterms:source dcterms: ;
    dcterms:title "Period of Time" ;
    skos:definition "An interval of time that is named or defined by its start and end dates." ;
    skos:inScheme okns:dc ;
    skos:mappingRelation dcterms:PeriodOfTime ;
    linkml:class_uri dcterms:PeriodOfTime ;
    linkml:definition_uri okns:DctPeriodOfTime ;
    linkml:is_a okns:DctLocationPeriodOrJurisdiction ;
    linkml:slot_usage [ ] .

okns:DctPhysicalMedium a linkml:ClassDefinition ;
    dcterms:source dcterms: ;
    dcterms:title "Physical Medium" ;
    skos:definition "Examples include paper, canvas, or DVD." ;
    skos:inScheme okns:dc ;
    skos:mappingRelation dcterms:PhysicalMedium ;
    skos:note "description: A physical material or carrier." ;
    linkml:class_uri dcterms:PhysicalMedium ;
    linkml:definition_uri okns:DctPhysicalMedium ;
    linkml:is_a okns:DctMediaType ;
    linkml:slot_usage [ ] .

okns:DctPhysicalResource a linkml:ClassDefinition ;
    dcterms:source dcterms: ;
    dcterms:title "Physical Resource" ;
    skos:definition "A material thing." ;
    skos:inScheme okns:dc ;
    skos:mappingRelation dcterms:PhysicalResource ;
    linkml:class_uri dcterms:PhysicalResource ;
    linkml:definition_uri okns:DctPhysicalResource ;
    linkml:slot_usage [ ] .

okns:DctPolicy a linkml:ClassDefinition ;
    dcterms:source dcterms: ;
    dcterms:title "Policy" ;
    skos:definition "A plan or course of action by an authority, intended to influence and determine decisions, actions, and other matters." ;
    skos:inScheme okns:dc ;
    skos:mappingRelation dcterms:Policy ;
    linkml:class_uri dcterms:Policy ;
    linkml:definition_uri okns:DctPolicy ;
    linkml:slot_usage [ ] .

okns:DctProvenanceStatement a linkml:ClassDefinition ;
    dcterms:source dcterms: ;
    dcterms:title "Provenance Statement" ;
    skos:definition "Any changes in ownership and custody of a resource since its creation that are significant for its authenticity, integrity, and interpretation." ;
    skos:inScheme okns:dc ;
    skos:mappingRelation dcterms:ProvenanceStatement ;
    linkml:class_uri dcterms:ProvenanceStatement ;
    linkml:definition_uri okns:DctProvenanceStatement ;
    linkml:slot_usage [ ] .

okns:DctSizeOrDuration a linkml:ClassDefinition ;
    dcterms:source dcterms: ;
    dcterms:title "Size or Duration" ;
    skos:definition "Examples include a number of pages, a specification of length, width, and breadth, or a period in hours, minutes, and seconds." ;
    skos:inScheme okns:dc ;
    skos:mappingRelation dcterms:SizeOrDuration ;
    skos:note "description: A dimension or extent, or a time taken to play or execute." ;
    linkml:class_uri dcterms:SizeOrDuration ;
    linkml:definition_uri okns:DctSizeOrDuration ;
    linkml:is_a okns:DctMediaTypeOrExtent ;
    linkml:slot_usage [ ] .

okns:DctStandard a linkml:ClassDefinition ;
    dcterms:source dcterms: ;
    dcterms:title "Standard" ;
    skos:definition "A reference point against which other things can be evaluated or compared." ;
    skos:inScheme okns:dc ;
    skos:mappingRelation dcterms:Standard ;
    linkml:class_uri dcterms:Standard ;
    linkml:definition_uri okns:DctStandard ;
    linkml:slot_usage [ ] .

<https://purl.org/okn/schema/HttpDef.seegrid.csiro.auIsotc211Iso191502012Hm2owl#CodeList> a linkml:ClassDefinition ;
    dcterms:title "No class (entity type) name specified -- this class is noted as a superclass of another class in this graph but has not itself been defined." ;
    skos:inScheme okns:seegrid-iso19115 ;
    skos:mappingRelation <http://def.seegrid.csiro.au/isotc211/iso19150/2012/hm2owl#CodeList> ;
    linkml:class_uri <http://def.seegrid.csiro.au/isotc211/iso19150/2012/hm2owl#CodeList> ;
    linkml:definition_uri <https://purl.org/okn/schema/HttpDef.seegrid.csiro.auIsotc211Iso191502012Hm2owl#CodeList> ;
    linkml:slot_usage [ ] .

okns:HyfHYCanal a linkml:ClassDefinition ;
    skos:definition "The HY_Canal feature type defines the existence of body of surface water, participating in a hydrographic network, special due to its artificial origin (man-made)." ;
    skos:inScheme okns:hyf ;
    skos:mappingRelation <hyf:HY_Canal> ;
    linkml:class_uri <https://www.opengis.net/def/schema/hy_features/hyf/HY_Canal> ;
    linkml:definition_uri okns:HyfHYCanal ;
    linkml:is_a okns:HyfHYWaterBody ;
    linkml:slot_usage [ ] .

okns:HyfHYCartographicRealization a linkml:ClassDefinition ;
    skos:definition "The HY_CartographicRealization feature type realizes a catchment as set of separate cartographic layers or maps, displaying a network of hydrologic features which may be connected at the representation level, or not.␊␊Specializing HY_CatchmentRealization, it inherits from generalization the shape attribute and the realizedCatchment association." ;
    skos:inScheme okns:hyf ;
    skos:mappingRelation <hyf:HY_CartographicRealization> ;
    skos:note "description: The HY_CartographicRealization feature type realizes a catchment as set of separate cartographic layers or maps, displaying a network of hydrologic features which may be connected at the representation level, or not.  Specializing HY_CatchmentRealization, it inherits from generalization the shape attribute and the realizedCatchment association." ;
    linkml:class_uri <https://www.opengis.net/def/schema/hy_features/hyf/HY_CartographicRealization> ;
    linkml:definition_uri okns:HyfHYCartographicRealization ;
    linkml:is_a okns:HyfHYCatchmentRealization ;
    linkml:slot_usage [ ] .

okns:HyfHYCatchmentAggregate a linkml:ClassDefinition ;
    skos:definition "The HY_CatchmentAggregate feature type (Figure 30) specializes the HY_Catchment type as a set of non-overlapping dendritic and interior catchments arranged in an encompassing catchment. This can be used to describe multiple inflows into a catchment aggregate through several hydrologically discrete sub-catchments each with a single inflow, and contributing to a joined outflow of the catchment aggregate, including the 'nillable' outflow of interior catchments. Nillable is meant here to signify that the hydro nexus logically exists in the form of flow to the subsurface or atmosphere but is unknown in a given implementation.␊␊Being a special type of the HY_Catchment, the catchment aggregate may be part of a containing catchment at the next higher level of hierarchy, which consists of similar-scale neighboring catchments. The catchment aggregate does not necessarily imply a series of nested containing catchments. It primarily allows navigation to the 'highest' level system (total drainage basin) as typically used for reporting purposes.␊␊HY_CatchmentAggregate inherits through generalization the outflow, inflow, containingCatchment, containedCatchment, conjointCatchment, upperCatchment, lowerCatchment, and catchmentRealization properties, and has exorheicDrainage and endorheicDrainage associations." ;
    skos:inScheme okns:hyf ;
    skos:mappingRelation <hyf:HY_CatchmentAggregate> ;
    skos:note "description: The HY_CatchmentAggregate feature type (Figure 30) specializes the HY_Catchment type as a set of non-overlapping dendritic and interior catchments arranged in an encompassing catchment. This can be used to describe multiple inflows into a catchment aggregate through several hydrologically discrete sub-catchments each with a single inflow, and contributing to a joined outflow of the catchment aggregate, including the 'nillable' outflow of interior catchments. Nillable is meant here to signify that the hydro nexus logically exists in the form of flow to the subsurface or atmosphere but is unknown in a given implementation.  Being a special type of the HY_Catchment, the catchment aggregate may be part of a containing catchment at the next higher level of hierarchy, which consists of similar-scale neighboring catchments. The catchment aggregate does not necessarily imply a series of nested containing catchments. It primarily allows navigation to the 'highest' level system (total drainage basin) as typically used for reporting purposes. HY_CatchmentAggregate inherits through generalization the outflow, inflow, containingCatchment, containedCatchment, conjointCatchment, upperCatchment, lowerCatchment, and catchmentRealization properties, and has exorheicDrainage and endorheicDrainage associations." ;
    linkml:class_uri <https://www.opengis.net/def/schema/hy_features/hyf/HY_CatchmentAggregate> ;
    linkml:definition_uri okns:HyfHYCatchmentAggregate ;
    linkml:is_a okns:HyfHYCatchment ;
    linkml:slot_usage [ ] .

okns:HyfHYChannel a linkml:ClassDefinition ;
    skos:definition "The HY_Channel feature type specializes the HY_Depression class with respect to a natural or man-made, open or closed channel through or along which water may or may not flow. A channel is part of the network of channels and depressions which forms the connecting system for the hydrographic network; a channel may have vertical sections at right angles to the main (average) direction of flow or along its centerline.␊␊HY_Channel has an association indicating the channelNetwork in which it participates. It carries the associations: stream, bedProfileTransversal and bedProfileLongitudinal. HY_Channel inherits from generalization the confinedWaterBody association and the outflow-at-benchmark constraint. An outlet-at-profile constraint emphasizes the recognition of vertical section as the outlet of the catchment that is realized by the channel network." ;
    skos:inScheme okns:hyf ;
    skos:mappingRelation <hyf:HY_Channel> ;
    linkml:class_uri <https://www.opengis.net/def/schema/hy_features/hyf/HY_Channel> ;
    linkml:definition_uri okns:HyfHYChannel ;
    linkml:is_a okns:HyfHYDepression ;
    linkml:slot_usage [ ] .

okns:HyfHYChannelNetwork a linkml:ClassDefinition ;
    skos:definition "The HY_ChannelNetwork feature type specializes the HY_HydroNetwork realization defined in the Hydro Feature core model, specifically as an aggregate of surface depressions and surface channels which continuously or periodically contain water, without imposing a particular drainage pattern. This allows representation of the network, even if logically connected features are not connected at the representation level. If the realized catchment is connected with other catchments via hydro nexuses, the channel network is considered connected to the channel network realizing these catchments.␊␊HY_ChannelNetwork has surfaceDepression and surfaceChannel associations, and carries a drainagePattern attribute; it inherits through generalization the shape attribute, the realizedCatchment association as well as flowpath, catchmentDivide and catchmentArea associations. Depending on the application, the channel network and the related features may be described by suitable attributes. A channel-flowpath constraint is defined to support the recognition of the channel as flowpath realizing the catchment." ;
    skos:inScheme okns:hyf ;
    skos:mappingRelation <hyf:HY_ChannelNetwork> ;
    linkml:class_uri <https://www.opengis.net/def/schema/hy_features/hyf/HY_ChannelNetwork> ;
    linkml:definition_uri okns:HyfHYChannelNetwork ;
    linkml:slot_usage [ ] .

okns:HyfHYCrossSection a linkml:ClassDefinition ;
    skos:definition "The HY_CrossSection feature type conceptualizes the segmentation of a waterbody or a containing channel through vertical sections. Taking into account the conceptual separation of a watercourse, the cross section concept refers to both the cross section of a waterbody orthogonal to the direction of flow, and to the transversal bed profile of a channel.␊␊A cross section associates a crossSectionPoint which should be used to identify a permanent reference location at a vertical section which realizes the conceptual hydro nexus of the catchment realized by the associated channel or waterbody." ;
    skos:inScheme okns:hyf ;
    skos:mappingRelation <hyf:HY_CrossSection> ;
    linkml:class_uri <https://www.opengis.net/def/schema/hy_features/hyf/HY_CrossSection> ;
    linkml:definition_uri okns:HyfHYCrossSection ;
    linkml:slot_usage [ ] .

okns:HyfHYEstuary a linkml:ClassDefinition ;
    skos:definition "The HY_Estuary feature type defines the existence of body of surface water, participating in a hydrographic network, special due to branching and its interaction with the open sea." ;
    skos:inScheme okns:hyf ;
    skos:mappingRelation <hyf:HY_Estuary> ;
    linkml:class_uri <https://www.opengis.net/def/schema/hy_features/hyf/HY_Estuary> ;
    linkml:definition_uri okns:HyfHYEstuary ;
    linkml:is_a okns:HyfHYWaterBody ;
    linkml:slot_usage [ ] .

okns:HyfHYHydroNetwork a linkml:ClassDefinition ;
    skos:definition "The HY_HydroNetwork feature type realizes a catchment as a network of connected hydrologic features. Such a network realizes the hierarchical network of logically connected catchments contained in a larger catchment. It may be a sequence of flowpaths, an aggregate of catchment areas or a mesh of catchment divides.␊␊HY_HydroNetwork feature type specializes HY_CatchmentRealization. Through generalization it inherits the shape and the realizedCatchment properties, and carries the associations flowpath, catchmentDivide and catchmentArea. The optional shape of the is usually given through the individual geometry of the network parts." ;
    skos:inScheme okns:hyf ;
    skos:mappingRelation <hyf:HY_HydroNetwork> ;
    skos:note "description: The HY_HydroNetwork feature type realizes a catchment as a network of connected hydrologic features. Such a network realizes the hierarchical network of logically connected catchments contained in a larger catchment. It may be a sequence of flowpaths, an aggregate of catchment areas or a mesh of catchment divides.  HY_HydroNetwork feature type specializes HY_CatchmentRealization. Through generalization it inherits the shape and the realizedCatchment properties, and carries the associations flowpath, catchmentDivide and catchmentArea. The optional shape of the is usually given through the individual geometry of the network parts." ;
    linkml:class_uri <https://www.opengis.net/def/schema/hy_features/hyf/HY_HydroNetwork> ;
    linkml:definition_uri okns:HyfHYHydroNetwork ;
    linkml:is_a okns:HyfHYCatchmentRealization ;
    linkml:slot_usage [ ] .

okns:HyfHYHydrographicNetwork a linkml:ClassDefinition ;
    skos:definition "The HY_HydrographicNetwork feature type specializes the HY_HydroNetwork realization defined in the Hydro Feature core model, specifically as an aggregate of permanent or temporary bodies standing in depressions or moving in channels. If the realized catchment is connected with other catchments via hydro nexuses, the hydrographic network is considered connected to the network realizing these catchments. This allows representation of the network, even if logically connected features are not connected at the representation level. If required, an application focused on surface-waterbodies contained in channels or depressions may use the defined relationships to describe the realization of a catchment by the hydrographic network, or network parts associated with the channel network.␊␊HY_HydrographicNetwork has a networkWaterBody association. Through generalization, it inherits the shape attribute and the realizedCatchment association as well as flowpath, catchmentDivide and catchmentArea associations, and. A waterbody-flowpath constraint supports the recognition of the waterbody as a flowpath realizing the catchment." ;
    skos:inScheme okns:hyf ;
    skos:mappingRelation <hyf:HY_HydrographicNetwork> ;
    linkml:class_uri <https://www.opengis.net/def/schema/hy_features/hyf/HY_HydrographicNetwork> ;
    linkml:definition_uri okns:HyfHYHydrographicNetwork ;
    linkml:slot_usage [ ] .

okns:HyfHYHydrometricFeature a linkml:ClassDefinition ;
    skos:definition "The HY_HydrometricFeature feature type provides a concept of a monitoring station at which data on water are obtained that realizes the catchment either separately or as part of the hydrometric network (Figure 45).␊␊HY_HydrometricFeature has associations for the hydrometricNetwork in which it participates, and a positionOnRiver. An outlet-at-station constraint emphasizes the recognition of a monitoring station as outlet of the catchment that is realized by the hydrometric network." ;
    skos:inScheme okns:hyf ;
    skos:mappingRelation <hyf:HY_HydrometricFeature> ;
    linkml:class_uri <https://www.opengis.net/def/schema/hy_features/hyf/HY_HydrometricFeature> ;
    linkml:definition_uri okns:HyfHYHydrometricFeature ;
    linkml:slot_usage [ ] .

okns:HyfHYHydrometricNetwork a linkml:ClassDefinition ;
    skos:definition "The HY_HydrometricNetwork feature type specializes the HY_HydroNetwork realization specifically as an aggregate of hydrometric features.␊␊HY_HydrometricNetwork has a networkStation association, and inherits through generalization the shape attribute, the realizedCatchment, flowpath, catchmentDivide and catchmentArea associations." ;
    skos:inScheme okns:hyf ;
    skos:mappingRelation <hyf:HY_HydrometricNetwork> ;
    linkml:class_uri <https://www.opengis.net/def/schema/hy_features/hyf/HY_HydrometricNetwork> ;
    linkml:definition_uri okns:HyfHYHydrometricNetwork ;
    linkml:slot_usage [ ] .

okns:HyfHYImpoundment a linkml:ClassDefinition ;
    skos:definition "The HY_Impoundment feature type defines the existence of body of surface water, participating in a hydrographic network, special due to be formed by collecting water, as by a dam." ;
    skos:inScheme okns:hyf ;
    skos:mappingRelation <hyf:HY_Impoundment> ;
    linkml:class_uri <https://www.opengis.net/def/schema/hy_features/hyf/HY_Impoundment> ;
    linkml:definition_uri okns:HyfHYImpoundment ;
    linkml:is_a okns:HyfHYWaterBody ;
    linkml:slot_usage [ ] .

okns:HyfHYLagoon a linkml:ClassDefinition ;
    skos:definition "The HY_Lagoon feature type defines the existence of body of surface water, participating in a hydrographic network, special due to its shallow depth and interaction with the open sea." ;
    skos:inScheme okns:hyf ;
    skos:mappingRelation <hyf:HY_Lagoon> ;
    linkml:class_uri <https://www.opengis.net/def/schema/hy_features/hyf/HY_Lagoon> ;
    linkml:definition_uri okns:HyfHYLagoon ;
    linkml:is_a okns:HyfHYWaterBody ;
    linkml:slot_usage [ ] .

okns:HyfHYLake a linkml:ClassDefinition ;
    skos:definition "The HY_Lake feature type defines the existence of body of surface water, participating in a hydrographic network, special due to its considerable size." ;
    skos:inScheme okns:hyf ;
    skos:mappingRelation <hyf:HY_Lake> ;
    linkml:class_uri <https://www.opengis.net/def/schema/hy_features/hyf/HY_Lake> ;
    linkml:definition_uri okns:HyfHYLake ;
    linkml:is_a okns:HyfHYWaterBody ;
    linkml:slot_usage [ ] .

okns:HyfHYLongitudinalSection a linkml:ClassDefinition ;
    skos:definition "The HY_LongitudinalSection feature type conceptualizes the segmentation of a waterbody or a containing channel through vertical sections. Taking into account the conceptual separation of a watercourse, the longitudinal section concept refers to both the vertical section of a waterbody along its centerline, and to the longitudinal bed profile of a channel.␊␊A longitudinal section associates a longitudalinalSectionPoint which should be used to identify a permanent reference location at a vertical section which realizes the conceptual hydro nexus of the catchment realized by the associated channel or waterbody." ;
    skos:inScheme okns:hyf ;
    skos:mappingRelation <hyf:HY_LongitudinalSection> ;
    linkml:class_uri <https://www.opengis.net/def/schema/hy_features/hyf/HY_LongitudinalSection> ;
    linkml:definition_uri okns:HyfHYLongitudinalSection ;
    linkml:slot_usage [ ] .

okns:HyfHYReservoir a linkml:ClassDefinition ;
    skos:definition "The HY_Reservoir feature type describes the water body, either natural or man-made, used for storage, regulation and control of water resources. The reservoir concept refers to a volume of water managed in zones between operating levels.␊␊HY_Reservoir associates to a reservoir the storedWaterBody and a reservoirZone." ;
    skos:inScheme okns:hyf ;
    skos:mappingRelation <hyf:HY_Reservoir> ;
    linkml:class_uri <https://www.opengis.net/def/schema/hy_features/hyf/HY_Reservoir> ;
    linkml:definition_uri okns:HyfHYReservoir ;
    linkml:slot_usage [ ] .

okns:HyfHYRiver a linkml:ClassDefinition ;
    dcterms:title "HY_Stream" ;
    skos:definition "The HY_River feature type defines the existence of body of surface water, participating in a hydrographic network, special due to its property to permanently or temporarily flow." ;
    skos:inScheme okns:hyf ;
    skos:mappingRelation <hyf:HY_River> ;
    linkml:class_uri <https://www.opengis.net/def/schema/hy_features/hyf/HY_River> ;
    linkml:definition_uri okns:HyfHYRiver ;
    linkml:is_a okns:HyfHYWaterBody ;
    linkml:slot_usage [ ] .

okns:HyfHYWaterBodyStratum a linkml:ClassDefinition ;
    skos:definition "The HY_WaterBodyStratum feature type describes a horizontal layer in a stratified waterbody determined by differences in thermal or salinity characteristics or by oxygen or nutrient content, or by virtual storage zones of a reservoir.␊␊HY_WaterBodyStratum carries the properties: stratumType and benchmark." ;
    skos:inScheme okns:hyf ;
    skos:mappingRelation <hyf:HY_WaterBodyStratum> ;
    linkml:class_uri <https://www.opengis.net/def/schema/hy_features/hyf/HY_WaterBodyStratum> ;
    linkml:definition_uri okns:HyfHYWaterBodyStratum ;
    linkml:slot_usage [ ] .

okns:HyfHYWaterLiquidPhase a linkml:ClassDefinition ;
    skos:definition "The HY_Water_LiquidPhase feature type provides a simple concept of the accumulation of water in waterbodies. This definition refers to the matter accumulated to a mass of water. In its liquid form water is considered accumulated in waterbodies. The accumulation of water in the atmosphere or below the land surface, e.g. rain, soil moisture or groundwater, is not in scope of this standard, as well as the accumulation of snow and ice in glaciers which is subject of glaciology science.␊␊Contextually related information models may use the HY_Water_LiquidPhase feature type to build relationships to an accumulating waterbody, and ultimately to the catchment realized either by the waterbody or by the network of which the waterbody is part.␊␊HY_Water_LiquidPhase has an association with the accumulatingWaterBody which may be used to identify the waterbody (as part of the hydrographic network) where liquid water is accumulated." ;
    skos:inScheme okns:hyf ;
    skos:mappingRelation <hyf:HY_Water_LiquidPhase> ;
    linkml:class_uri <https://www.opengis.net/def/schema/hy_features/hyf/HY_Water_LiquidPhase> ;
    linkml:definition_uri okns:HyfHYWaterLiquidPhase ;
    linkml:slot_usage [ ] .

okns:HyfHYWaterSolidPhase a linkml:ClassDefinition ;
    skos:definition "The HY_Water_SolidPhase feature type provides a simple concept of the accumulation of water in waterbodies. This definition refers to the matter accumulated to a mass of water. In its solid form water is considered accumulated in water bodies after melting, or as a layer of ice or snow on an open waterbody. The accumulation of water in the atmosphere or below the land surface, e.g. rain, soil moisture or groundwater, is not in scope of this standard, as well as the accumulation of snow and ice in glaciers which is subject of glaciology science.␊␊Contextually related information models may use the HY_Water_LiquidPhase and HY_Water_SolidPhase feature types to build relationships to an accumulating waterbody, and ultimately to the catchment realized either by the waterbody or by the network of which the waterbody is part.␊␊HY_Water_LiquidPhase has an association with the accumulatingWaterBody; HY_Water_SolidPhase has associations with the water from snowmelt and coveredWaterBody. These associations may be used to identify the waterbody (as part of the hydrographic network) where liquid water is accumulated." ;
    skos:inScheme okns:hyf ;
    skos:mappingRelation <hyf:HY_Water_SolidPhase> ;
    linkml:class_uri <https://www.opengis.net/def/schema/hy_features/hyf/HY_Water_SolidPhase> ;
    linkml:definition_uri okns:HyfHYWaterSolidPhase ;
    linkml:slot_usage [ ] .

okns:OwlAllDisjointClasses a linkml:ClassDefinition ;
    dcterms:source owl: ;
    dcterms:title "AllDisjointClasses" ;
    skos:definition "The class of collections of pairwise disjoint classes." ;
    skos:inScheme okns:owl-rdf-rdfs ;
    skos:mappingRelation owl:AllDisjointClasses ;
    linkml:class_uri owl:AllDisjointClasses ;
    linkml:definition_uri okns:OwlAllDisjointClasses ;
    linkml:is_a okns:RdfsResource ;
    linkml:slot_usage [ ] .

okns:OwlAllDisjointProperties a linkml:ClassDefinition ;
    dcterms:source owl: ;
    dcterms:title "AllDisjointProperties" ;
    skos:definition "The class of collections of pairwise disjoint properties." ;
    skos:inScheme okns:owl-rdf-rdfs ;
    skos:mappingRelation owl:AllDisjointProperties ;
    linkml:class_uri owl:AllDisjointProperties ;
    linkml:definition_uri okns:OwlAllDisjointProperties ;
    linkml:is_a okns:RdfsResource ;
    linkml:slot_usage [ ] .

okns:OwlAnnotation a linkml:ClassDefinition ;
    dcterms:source owl: ;
    dcterms:title "Annotation" ;
    skos:definition "The class of annotated annotations for which the RDF serialization consists of an annotated subject, predicate and object." ;
    skos:inScheme okns:owl-rdf-rdfs ;
    skos:mappingRelation owl:Annotation ;
    linkml:class_uri owl:Annotation ;
    linkml:definition_uri okns:OwlAnnotation ;
    linkml:is_a okns:RdfsResource ;
    linkml:slot_usage [ ] .

okns:OwlAnnotationProperty a linkml:ClassDefinition ;
    dcterms:source owl: ;
    dcterms:title "AnnotationProperty" ;
    skos:definition "The class of annotation properties." ;
    skos:inScheme okns:owl-rdf-rdfs ;
    skos:mappingRelation owl:AnnotationProperty ;
    linkml:class_uri owl:AnnotationProperty ;
    linkml:definition_uri okns:OwlAnnotationProperty ;
    linkml:is_a okns:RdfProperty ;
    linkml:slot_usage [ ] .

okns:OwlAsymmetricProperty a linkml:ClassDefinition ;
    dcterms:source owl: ;
    dcterms:title "AsymmetricProperty" ;
    skos:definition "The class of asymmetric properties." ;
    skos:inScheme okns:owl-rdf-rdfs ;
    skos:mappingRelation owl:AsymmetricProperty ;
    linkml:class_uri owl:AsymmetricProperty ;
    linkml:definition_uri okns:OwlAsymmetricProperty ;
    linkml:is_a okns:OwlObjectProperty ;
    linkml:slot_usage [ ] .

okns:OwlAxiom a linkml:ClassDefinition ;
    dcterms:source owl: ;
    dcterms:title "Axiom" ;
    skos:definition "The class of annotated axioms for which the RDF serialization consists of an annotated subject, predicate and object." ;
    skos:inScheme okns:owl-rdf-rdfs ;
    skos:mappingRelation owl:Axiom ;
    linkml:class_uri owl:Axiom ;
    linkml:definition_uri okns:OwlAxiom ;
    linkml:is_a okns:RdfsResource ;
    linkml:slot_usage [ ] .

okns:OwlDataRange a linkml:ClassDefinition ;
    dcterms:source owl: ;
    dcterms:title "DataRange" ;
    skos:definition "The class of OWL data ranges, which are special kinds of datatypes. Note: The use of the IRI owl:DataRange has been deprecated as of OWL 2. The IRI rdfs:Datatype SHOULD be used instead." ;
    skos:inScheme okns:owl-rdf-rdfs ;
    skos:mappingRelation owl:DataRange ;
    linkml:class_uri owl:DataRange ;
    linkml:definition_uri okns:OwlDataRange ;
    linkml:is_a okns:RdfsDatatype ;
    linkml:slot_usage [ ] ;
    linkml:slots okns:rdfs_comment,
        okns:rdfs_isDefinedBy,
        okns:rdfs_label,
        okns:rdfs_seeAlso,
        okns:rdfs_subClassOf .

okns:OwlDatatypeProperty a linkml:ClassDefinition ;
    dcterms:source owl: ;
    dcterms:title "DatatypeProperty" ;
    skos:definition "The class of data properties." ;
    skos:inScheme okns:owl-rdf-rdfs ;
    skos:mappingRelation owl:DatatypeProperty ;
    linkml:class_uri owl:DatatypeProperty ;
    linkml:definition_uri okns:OwlDatatypeProperty ;
    linkml:is_a okns:RdfProperty ;
    linkml:slot_usage [ ] .

okns:OwlDeprecatedClass a linkml:ClassDefinition ;
    dcterms:source owl: ;
    dcterms:title "DeprecatedClass" ;
    skos:definition "The class of deprecated classes." ;
    skos:inScheme okns:owl-rdf-rdfs ;
    skos:mappingRelation owl:DeprecatedClass ;
    linkml:class_uri owl:DeprecatedClass ;
    linkml:definition_uri okns:OwlDeprecatedClass ;
    linkml:is_a okns:RdfsClass ;
    linkml:slot_usage [ ] .

okns:OwlDeprecatedProperty a linkml:ClassDefinition ;
    dcterms:source owl: ;
    dcterms:title "DeprecatedProperty" ;
    skos:definition "The class of deprecated properties." ;
    skos:inScheme okns:owl-rdf-rdfs ;
    skos:mappingRelation owl:DeprecatedProperty ;
    linkml:class_uri owl:DeprecatedProperty ;
    linkml:definition_uri okns:OwlDeprecatedProperty ;
    linkml:is_a okns:RdfProperty ;
    linkml:slot_usage [ ] .

okns:OwlFunctionalProperty a linkml:ClassDefinition ;
    dcterms:source owl: ;
    dcterms:title "FunctionalProperty" ;
    skos:definition "The class of functional properties." ;
    skos:inScheme okns:owl-rdf-rdfs ;
    skos:mappingRelation owl:FunctionalProperty ;
    linkml:class_uri owl:FunctionalProperty ;
    linkml:definition_uri okns:OwlFunctionalProperty ;
    linkml:is_a okns:RdfProperty ;
    linkml:slot_usage [ ] .

okns:OwlInverseFunctionalProperty a linkml:ClassDefinition ;
    dcterms:source owl: ;
    dcterms:title "InverseFunctionalProperty" ;
    skos:definition "The class of inverse-functional properties." ;
    skos:inScheme okns:owl-rdf-rdfs ;
    skos:mappingRelation owl:InverseFunctionalProperty ;
    linkml:class_uri owl:InverseFunctionalProperty ;
    linkml:definition_uri okns:OwlInverseFunctionalProperty ;
    linkml:is_a okns:OwlObjectProperty ;
    linkml:slot_usage [ ] .

okns:OwlIrreflexiveProperty a linkml:ClassDefinition ;
    dcterms:source owl: ;
    dcterms:title "IrreflexiveProperty" ;
    skos:definition "The class of irreflexive properties." ;
    skos:inScheme okns:owl-rdf-rdfs ;
    skos:mappingRelation owl:IrreflexiveProperty ;
    linkml:class_uri owl:IrreflexiveProperty ;
    linkml:definition_uri okns:OwlIrreflexiveProperty ;
    linkml:is_a okns:OwlObjectProperty ;
    linkml:slot_usage [ ] .

okns:OwlNamedIndividual a linkml:ClassDefinition ;
    dcterms:source owl: ;
    dcterms:title "NamedIndividual" ;
    skos:definition "The class of named individuals." ;
    skos:inScheme okns:owl-rdf-rdfs ;
    skos:mappingRelation owl:NamedIndividual ;
    linkml:class_uri owl:NamedIndividual ;
    linkml:definition_uri okns:OwlNamedIndividual ;
    linkml:is_a okns:OwlThing ;
    linkml:slot_usage [ ] .

okns:OwlNothing a linkml:ClassDefinition ;
    dcterms:source owl: ;
    dcterms:title "Nothing" ;
    skos:definition "This is the empty class." ;
    skos:inScheme okns:owl-rdf-rdfs ;
    skos:mappingRelation owl:Nothing ;
    linkml:class_uri owl:Nothing ;
    linkml:definition_uri okns:OwlNothing ;
    linkml:is_a okns:OwlThing ;
    linkml:slot_usage [ ] .

okns:OwlOntologyProperty a linkml:ClassDefinition ;
    dcterms:source owl: ;
    dcterms:title "OntologyProperty" ;
    skos:definition "The class of ontology properties." ;
    skos:inScheme okns:owl-rdf-rdfs ;
    skos:mappingRelation owl:OntologyProperty ;
    linkml:class_uri owl:OntologyProperty ;
    linkml:definition_uri okns:OwlOntologyProperty ;
    linkml:is_a okns:RdfProperty ;
    linkml:slot_usage [ ] .

okns:OwlReflexiveProperty a linkml:ClassDefinition ;
    dcterms:source owl: ;
    dcterms:title "ReflexiveProperty" ;
    skos:definition "The class of reflexive properties." ;
    skos:inScheme okns:owl-rdf-rdfs ;
    skos:mappingRelation owl:ReflexiveProperty ;
    linkml:class_uri owl:ReflexiveProperty ;
    linkml:definition_uri okns:OwlReflexiveProperty ;
    linkml:is_a okns:OwlObjectProperty ;
    linkml:slot_usage [ ] .

okns:OwlSymmetricProperty a linkml:ClassDefinition ;
    dcterms:source owl: ;
    dcterms:title "SymmetricProperty" ;
    skos:definition "The class of symmetric properties." ;
    skos:inScheme okns:owl-rdf-rdfs ;
    skos:mappingRelation owl:SymmetricProperty ;
    linkml:class_uri owl:SymmetricProperty ;
    linkml:definition_uri okns:OwlSymmetricProperty ;
    linkml:is_a okns:OwlObjectProperty ;
    linkml:slot_usage [ ] .

okns:OwlTransitiveProperty a linkml:ClassDefinition ;
    dcterms:source owl: ;
    dcterms:title "TransitiveProperty" ;
    skos:definition "The class of transitive properties." ;
    skos:inScheme okns:owl-rdf-rdfs ;
    skos:mappingRelation owl:TransitiveProperty ;
    linkml:class_uri owl:TransitiveProperty ;
    linkml:definition_uri okns:OwlTransitiveProperty ;
    linkml:is_a okns:OwlObjectProperty ;
    linkml:slot_usage [ ] .

okns:RdfAlt a linkml:ClassDefinition ;
    dcterms:source rdf: ;
    dcterms:title "Alt" ;
    skos:definition "The class of containers of alternatives." ;
    skos:inScheme okns:owl-rdf-rdfs ;
    skos:mappingRelation rdf:Alt ;
    linkml:class_uri rdf:Alt ;
    linkml:definition_uri okns:RdfAlt ;
    linkml:is_a okns:RdfsContainer ;
    linkml:slot_usage [ ] .

okns:RdfBag a linkml:ClassDefinition ;
    dcterms:source rdf: ;
    dcterms:title "Bag" ;
    skos:definition "The class of unordered containers." ;
    skos:inScheme okns:owl-rdf-rdfs ;
    skos:mappingRelation rdf:Bag ;
    linkml:class_uri rdf:Bag ;
    linkml:definition_uri okns:RdfBag ;
    linkml:is_a okns:RdfsContainer ;
    linkml:slot_usage [ ] .

okns:RdfSeq a linkml:ClassDefinition ;
    dcterms:source rdf: ;
    dcterms:title "Seq" ;
    skos:definition "The class of ordered containers." ;
    skos:inScheme okns:owl-rdf-rdfs ;
    skos:mappingRelation rdf:Seq ;
    linkml:class_uri rdf:Seq ;
    linkml:definition_uri okns:RdfSeq ;
    linkml:is_a okns:RdfsContainer ;
    linkml:slot_usage [ ] .

okns:RdfsContainerMembershipProperty a linkml:ClassDefinition ;
    dcterms:source rdfs: ;
    dcterms:title "ContainerMembershipProperty" ;
    skos:definition "The class of container membership properties, rdf:_1, rdf:_2, ..., all of which are sub-properties of 'member'." ;
    skos:inScheme okns:owl-rdf-rdfs ;
    skos:mappingRelation rdfs:ContainerMembershipProperty ;
    linkml:class_uri rdfs:ContainerMembershipProperty ;
    linkml:definition_uri okns:RdfsContainerMembershipProperty ;
    linkml:is_a okns:RdfProperty ;
    linkml:slot_usage [ ] .

okns:Seegrid-basicAcceleration a linkml:ClassDefinition ;
    dcterms:source <http://def.seegrid.csiro.au/isotc211/iso19103/2005/basic> ;
    dcterms:title "Acceleration" ;
    skos:definition "Measure of rate of change of velocity" ;
    skos:inScheme okns:seegrid-iso19115 ;
    skos:mappingRelation seegrid-basic:Acceleration ;
    linkml:class_uri seegrid-basic:Acceleration ;
    linkml:definition_uri okns:Seegrid-basicAcceleration ;
    linkml:is_a okns:Seegrid-basicMeasure ;
    linkml:slot_usage [ ] .

okns:Seegrid-basicAngle a linkml:ClassDefinition ;
    dcterms:source <http://def.seegrid.csiro.au/isotc211/iso19103/2005/basic> ;
    dcterms:title "Angle" ;
    skos:definition "measure of arc length or rotation" ;
    skos:inScheme okns:seegrid-iso19115 ;
    skos:mappingRelation seegrid-basic:Angle ;
    linkml:class_uri seegrid-basic:Angle ;
    linkml:definition_uri okns:Seegrid-basicAngle ;
    linkml:is_a okns:Seegrid-basicMeasure ;
    linkml:slot_usage [ ] .

okns:Seegrid-basicAngularVelocity a linkml:ClassDefinition ;
    dcterms:source <http://def.seegrid.csiro.au/isotc211/iso19103/2005/basic> ;
    dcterms:title "AngularVelocity" ;
    skos:definition "Measure of rate of change of angular position" ;
    skos:inScheme okns:seegrid-iso19115 ;
    skos:mappingRelation seegrid-basic:AngularVelocity ;
    linkml:class_uri seegrid-basic:AngularVelocity ;
    linkml:definition_uri okns:Seegrid-basicAngularVelocity ;
    linkml:is_a okns:Seegrid-basicMeasure ;
    linkml:slot_usage [ ] .

okns:Seegrid-basicArea a linkml:ClassDefinition ;
    dcterms:source <http://def.seegrid.csiro.au/isotc211/iso19103/2005/basic> ;
    dcterms:title "Area" ;
    skos:definition "Measure of 2-D extent" ;
    skos:inScheme okns:seegrid-iso19115 ;
    skos:mappingRelation seegrid-basic:Area ;
    linkml:class_uri seegrid-basic:Area ;
    linkml:definition_uri okns:Seegrid-basicArea ;
    linkml:is_a okns:Seegrid-basicMeasure ;
    linkml:slot_usage [ ] .

okns:Seegrid-basicCurrency a linkml:ClassDefinition ;
    dcterms:source <http://def.seegrid.csiro.au/isotc211/iso19103/2005/basic> ;
    dcterms:title "Currency" ;
    skos:definition "Measure of exchange value" ;
    skos:inScheme okns:seegrid-iso19115 ;
    skos:mappingRelation seegrid-basic:Currency ;
    linkml:class_uri seegrid-basic:Currency ;
    linkml:definition_uri okns:Seegrid-basicCurrency ;
    linkml:is_a okns:Seegrid-basicMeasure ;
    linkml:slot_usage [ ] .

okns:Seegrid-basicDistance a linkml:ClassDefinition ;
    dcterms:source <http://def.seegrid.csiro.au/isotc211/iso19103/2005/basic> ;
    dcterms:title "Distance" ;
    skos:definition "Measure of spatial separation along some 1-D manifold" ;
    skos:inScheme okns:seegrid-iso19115 ;
    skos:mappingRelation seegrid-basic:Distance ;
    linkml:class_uri seegrid-basic:Distance ;
    linkml:definition_uri okns:Seegrid-basicDistance ;
    linkml:is_a okns:Seegrid-basicLength ;
    linkml:slot_usage [ ] .

okns:Seegrid-basicMass a linkml:ClassDefinition ;
    dcterms:source <http://def.seegrid.csiro.au/isotc211/iso19103/2005/basic> ;
    dcterms:title "Mass" ;
    skos:definition "Measure of amount of substance" ;
    skos:inScheme okns:seegrid-iso19115 ;
    skos:mappingRelation seegrid-basic:Mass ;
    linkml:class_uri seegrid-basic:Mass ;
    linkml:definition_uri okns:Seegrid-basicMass ;
    linkml:is_a okns:Seegrid-basicMeasure ;
    linkml:slot_usage [ ] .

okns:Seegrid-basicScale a linkml:ClassDefinition ;
    dcterms:source <http://def.seegrid.csiro.au/isotc211/iso19103/2005/basic> ;
    dcterms:title "Scale" ;
    skos:definition "Factor by which a representation should be magnified to match the geomstric size of the thing it represents." ;
    skos:inScheme okns:seegrid-iso19115 ;
    skos:mappingRelation seegrid-basic:Scale ;
    linkml:class_uri seegrid-basic:Scale ;
    linkml:definition_uri okns:Seegrid-basicScale ;
    linkml:is_a okns:Seegrid-basicMeasure ;
    linkml:slot_usage [ ] .

okns:Seegrid-basicTime a linkml:ClassDefinition ;
    dcterms:source <http://def.seegrid.csiro.au/isotc211/iso19103/2005/basic> ;
    dcterms:title "Time" ;
    skos:definition "Measure of temporal extent" ;
    skos:inScheme okns:seegrid-iso19115 ;
    skos:mappingRelation seegrid-basic:Time ;
    linkml:class_uri seegrid-basic:Time ;
    linkml:definition_uri okns:Seegrid-basicTime ;
    linkml:is_a okns:Seegrid-basicMeasure ;
    linkml:slot_usage [ ] .

okns:Seegrid-basicVelocity a linkml:ClassDefinition ;
    dcterms:source <http://def.seegrid.csiro.au/isotc211/iso19103/2005/basic> ;
    dcterms:title "Velocity" ;
    skos:definition "Measure of rate of change of position" ;
    skos:inScheme okns:seegrid-iso19115 ;
    skos:mappingRelation seegrid-basic:Velocity ;
    linkml:class_uri seegrid-basic:Velocity ;
    linkml:definition_uri okns:Seegrid-basicVelocity ;
    linkml:is_a okns:Seegrid-basicMeasure ;
    linkml:slot_usage [ ] .

okns:Seegrid-basicVolume a linkml:ClassDefinition ;
    dcterms:source <http://def.seegrid.csiro.au/isotc211/iso19103/2005/basic> ;
    dcterms:title "Volume" ;
    skos:definition "Measure of 3-D extent" ;
    skos:inScheme okns:seegrid-iso19115 ;
    skos:mappingRelation seegrid-basic:Volume ;
    linkml:class_uri seegrid-basic:Volume ;
    linkml:definition_uri okns:Seegrid-basicVolume ;
    linkml:is_a okns:Seegrid-basicMeasure ;
    linkml:slot_usage [ ] .

okns:Seegrid-basicWeight a linkml:ClassDefinition ;
    dcterms:source <http://def.seegrid.csiro.au/isotc211/iso19103/2005/basic> ;
    dcterms:title "Weight" ;
    skos:definition "Measure of force due to a mass in a specific gravitational field" ;
    skos:inScheme okns:seegrid-iso19115 ;
    skos:mappingRelation seegrid-basic:Weight ;
    linkml:class_uri seegrid-basic:Weight ;
    linkml:definition_uri okns:Seegrid-basicWeight ;
    linkml:is_a okns:Seegrid-basicMeasure ;
    linkml:slot_usage [ ] .

okns:dc_creator a linkml:SlotDefinition ;
    dcterms:source dc: ;
    dcterms:title "Creator" ;
    skos:definition "Examples of a Creator include a person, an organization, or a service. Typically, the name of a Creator should be used to indicate the entity." ;
    skos:editorialNote "A [second property](/specifications/dublin-core/dcmi-terms/#http://purl.org/dc/terms/creator) with the same name as this property has been declared in the [dcterms: namespace](http://purl.org/dc/terms/).  See the Introduction to the document [DCMI Metadata Terms](/specifications/dublin-core/dcmi-terms/) for an explanation.",
        "No occurrences of this slot in the graph." ;
    skos:inScheme okns:dc ;
    skos:mappingRelation dc:creator ;
    skos:note "description: An entity primarily responsible for making the resource." ;
    linkml:definition_uri okns:dc_creator ;
    linkml:inlined true ;
    linkml:range okns:Any ;
    linkml:slot_uri dc:creator .

okns:dc_source a linkml:SlotDefinition ;
    dcterms:source dc: ;
    dcterms:title "Source" ;
    skos:definition "The described resource may be derived from the related resource in whole or in part. Recommended best practice is to identify the related resource by means of a string conforming to a formal identification system." ;
    skos:editorialNote "A [second property](/specifications/dublin-core/dcmi-terms/#http://purl.org/dc/terms/source) with the same name as this property has been declared in the [dcterms: namespace](http://purl.org/dc/terms/).  See the Introduction to the document [DCMI Metadata Terms](/specifications/dublin-core/dcmi-terms/) for an explanation.",
        "No occurrences of this slot in the graph." ;
    skos:inScheme okns:dc ;
    skos:mappingRelation dc:source ;
    skos:note "description: A related resource from which the described resource is derived." ;
    linkml:definition_uri okns:dc_source ;
    linkml:inlined true ;
    linkml:range okns:Any ;
    linkml:slot_uri dc:source .

okns:dcam_domainIncludes a linkml:SlotDefinition ;
    dcterms:source dcam: ;
    dcterms:title "Domain Includes" ;
    skos:definition "A suggested class for subjects of this property." ;
    skos:editorialNote "No occurrences of this slot in the graph." ;
    skos:inScheme okns:dc ;
    skos:mappingRelation dcam:domainIncludes ;
    linkml:definition_uri okns:dcam_domainIncludes ;
    linkml:inlined true ;
    linkml:range okns:Any ;
    linkml:slot_uri dcam:domainIncludes .

okns:dcam_memberOf a linkml:SlotDefinition ;
    dcterms:source dcam: ;
    dcterms:title "Member Of" ;
    rdfs:seeAlso <https://www.dublincore.org/specifications/dublin-core/2007/06/04/abstract-model/> ;
    skos:definition "A relationship between a resource and a vocabulary encoding scheme which indicates that the resource is a member of a set." ;
    skos:editorialNote "No occurrences of this slot in the graph." ;
    skos:inScheme okns:dc ;
    skos:mappingRelation dcam:memberOf ;
    linkml:definition_uri okns:dcam_memberOf ;
    linkml:inlined true ;
    linkml:range okns:DcamVocabularyEncodingScheme ;
    linkml:slot_uri dcam:memberOf .

okns:dcam_rangeIncludes a linkml:SlotDefinition ;
    dcterms:source dcam: ;
    dcterms:title "Range Includes" ;
    skos:definition "A suggested class for values of this property." ;
    skos:editorialNote "No occurrences of this slot in the graph." ;
    skos:inScheme okns:dc ;
    skos:mappingRelation dcam:rangeIncludes ;
    linkml:definition_uri okns:dcam_rangeIncludes ;
    linkml:inlined true ;
    linkml:range okns:Any ;
    linkml:slot_uri dcam:rangeIncludes .

okns:dct_abstract a linkml:SlotDefinition ;
    dcterms:source dcterms: ;
    dcterms:title "Abstract" ;
    rdfs:subPropertyOf okns:dct_description ;
    skos:definition "A summary of the resource." ;
    skos:editorialNote "No occurrences of this slot in the graph." ;
    skos:inScheme okns:dc ;
    skos:mappingRelation dcterms:abstract ;
    linkml:definition_uri okns:dct_abstract ;
    linkml:inlined true ;
    linkml:range okns:Any ;
    linkml:slot_uri dcterms:abstract .

okns:dct_accessRights a linkml:SlotDefinition ;
    dcterms:source dcterms: ;
    dcterms:title "Access Rights" ;
    rdfs:subPropertyOf okns:dct_rights ;
    skos:definition "Access Rights may include information regarding access or restrictions based on privacy, security, or other policies." ;
    skos:editorialNote "No occurrences of this slot in the graph." ;
    skos:inScheme okns:dc ;
    skos:mappingRelation dcterms:accessRights ;
    skos:note "description: Information about who access the resource or an indication of its security status." ;
    linkml:definition_uri okns:dct_accessRights ;
    linkml:inlined true ;
    linkml:range okns:Any ;
    linkml:slot_uri dcterms:accessRights .

okns:dct_alternative a linkml:SlotDefinition ;
    dcterms:source dcterms: ;
    dcterms:title "Alternative Title" ;
    rdfs:subPropertyOf okns:dct_title ;
    skos:definition "The distinction between titles and alternative titles is application-specific." ;
    skos:editorialNote "No occurrences of this slot in the graph." ;
    skos:inScheme okns:dc ;
    skos:mappingRelation dcterms:alternative ;
    skos:note "description: An alternative name for the resource." ;
    linkml:definition_uri okns:dct_alternative ;
    linkml:inlined true ;
    linkml:range okns:RdfsLiteral ;
    linkml:slot_uri dcterms:alternative .

okns:dct_available a linkml:SlotDefinition ;
    dcterms:source dcterms: ;
    dcterms:title "Date Available" ;
    rdfs:subPropertyOf okns:dct_date ;
    skos:definition "Recommended practice is to describe the date, date/time, or period of time as recommended for the property Date, of which this is a subproperty." ;
    skos:editorialNote "No occurrences of this slot in the graph." ;
    skos:inScheme okns:dc ;
    skos:mappingRelation dcterms:available ;
    skos:note "description: Date that the resource became or will become available." ;
    linkml:definition_uri okns:dct_available ;
    linkml:inlined true ;
    linkml:range okns:RdfsLiteral ;
    linkml:slot_uri dcterms:available .

okns:dct_bibliographicCitation a linkml:SlotDefinition ;
    dcterms:source dcterms: ;
    dcterms:title "Bibliographic Citation" ;
    rdfs:subPropertyOf okns:dct_identifier ;
    skos:definition "Recommended practice is to include sufficient bibliographic detail to identify the resource as unambiguously as possible." ;
    skos:editorialNote "No occurrences of this slot in the graph." ;
    skos:inScheme okns:dc ;
    skos:mappingRelation dcterms:bibliographicCitation ;
    skos:note "description: A bibliographic reference for the resource." ;
    linkml:definition_uri okns:dct_bibliographicCitation ;
    linkml:inlined true ;
    linkml:range okns:RdfsLiteral ;
    linkml:slot_uri dcterms:bibliographicCitation .

okns:dct_conformsTo a linkml:SlotDefinition ;
    dcterms:source dcterms: ;
    dcterms:title "Conforms To" ;
    rdfs:subPropertyOf okns:dct_relation ;
    skos:definition "An established standard to which the described resource conforms." ;
    skos:editorialNote "No occurrences of this slot in the graph." ;
    skos:inScheme okns:dc ;
    skos:mappingRelation dcterms:conformsTo ;
    linkml:definition_uri okns:dct_conformsTo ;
    linkml:inlined true ;
    linkml:range okns:Any ;
    linkml:slot_uri dcterms:conformsTo .

okns:dct_created a linkml:SlotDefinition ;
    dcterms:source dcterms: ;
    dcterms:title "Date Created" ;
    rdfs:subPropertyOf okns:dct_date ;
    skos:definition "Recommended practice is to describe the date, date/time, or period of time as recommended for the property Date, of which this is a subproperty." ;
    skos:editorialNote "No occurrences of this slot in the graph." ;
    skos:inScheme okns:dc ;
    skos:mappingRelation dcterms:created ;
    skos:note "description: Date of creation of the resource." ;
    linkml:definition_uri okns:dct_created ;
    linkml:inlined true ;
    linkml:range okns:RdfsLiteral ;
    linkml:slot_uri dcterms:created .

okns:dct_creator a linkml:SlotDefinition ;
    dcterms:source dcterms: ;
    dcterms:title "Creator" ;
    rdfs:subPropertyOf okns:dct_contributor ;
    skos:definition "Recommended practice is to identify the creator with a URI.  If this is not possible or feasible, a literal value that identifies the creator may be provided." ;
    skos:editorialNote "No occurrences of this slot in the graph." ;
    skos:exactMatch foaf:maker ;
    skos:inScheme okns:dc ;
    skos:mappingRelation dcterms:creator ;
    skos:note "description: An entity responsible for making the resource." ;
    linkml:definition_uri okns:dct_creator ;
    linkml:inlined true ;
    linkml:range okns:Any ;
    linkml:slot_uri dcterms:creator .

okns:dct_dateAccepted a linkml:SlotDefinition ;
    dcterms:source dcterms: ;
    dcterms:title "Date Accepted" ;
    rdfs:subPropertyOf okns:dct_date ;
    skos:definition "Recommended practice is to describe the date, date/time, or period of time as recommended for the property Date, of which this is a subproperty.  Examples of resources to which a date of acceptance may be relevant are a thesis (accepted by a university department) or an article (accepted by a journal)." ;
    skos:editorialNote "No occurrences of this slot in the graph." ;
    skos:inScheme okns:dc ;
    skos:mappingRelation dcterms:dateAccepted ;
    skos:note "description: Date of acceptance of the resource." ;
    linkml:definition_uri okns:dct_dateAccepted ;
    linkml:inlined true ;
    linkml:range okns:RdfsLiteral ;
    linkml:slot_uri dcterms:dateAccepted .

okns:dct_dateCopyrighted a linkml:SlotDefinition ;
    dcterms:source dcterms: ;
    dcterms:title "Date Copyrighted" ;
    rdfs:subPropertyOf okns:dct_date ;
    skos:definition "Typically a year.  Recommended practice is to describe the date, date/time, or period of time as recommended for the property Date, of which this is a subproperty." ;
    skos:editorialNote "No occurrences of this slot in the graph." ;
    skos:inScheme okns:dc ;
    skos:mappingRelation dcterms:dateCopyrighted ;
    skos:note "description: Date of copyright of the resource." ;
    linkml:definition_uri okns:dct_dateCopyrighted ;
    linkml:inlined true ;
    linkml:range okns:RdfsLiteral ;
    linkml:slot_uri dcterms:dateCopyrighted .

okns:dct_dateSubmitted a linkml:SlotDefinition ;
    dcterms:source dcterms: ;
    dcterms:title "Date Submitted" ;
    rdfs:subPropertyOf okns:dct_date ;
    skos:definition "Recommended practice is to describe the date, date/time, or period of time as recommended for the property Date, of which this is a subproperty.  Examples of resources to which a 'Date Submitted' may be relevant include a thesis (submitted to a university department) or an article (submitted to a journal)." ;
    skos:editorialNote "No occurrences of this slot in the graph." ;
    skos:inScheme okns:dc ;
    skos:mappingRelation dcterms:dateSubmitted ;
    skos:note "description: Date of submission of the resource." ;
    linkml:definition_uri okns:dct_dateSubmitted ;
    linkml:inlined true ;
    linkml:range okns:RdfsLiteral ;
    linkml:slot_uri dcterms:dateSubmitted .

okns:dct_educationLevel a linkml:SlotDefinition ;
    dcterms:source dcterms: ;
    dcterms:title "Audience Education Level" ;
    rdfs:subPropertyOf okns:dct_audience ;
    skos:definition "A class of agents, defined in terms of progression through an educational or training context, for which the described resource is intended." ;
    skos:editorialNote "No occurrences of this slot in the graph." ;
    skos:inScheme okns:dc ;
    skos:mappingRelation dcterms:educationLevel ;
    linkml:definition_uri okns:dct_educationLevel ;
    linkml:inlined true ;
    linkml:range okns:Any ;
    linkml:slot_uri dcterms:educationLevel .

okns:dct_extent a linkml:SlotDefinition ;
    dcterms:source dcterms: ;
    dcterms:title "Extent" ;
    rdfs:subPropertyOf okns:dct_format ;
    skos:definition "Recommended practice is to specify the file size in megabytes and duration in ISO 8601 format." ;
    skos:editorialNote "No occurrences of this slot in the graph." ;
    skos:inScheme okns:dc ;
    skos:mappingRelation dcterms:extent ;
    skos:note "description: The size or duration of the resource." ;
    linkml:definition_uri okns:dct_extent ;
    linkml:inlined true ;
    linkml:range okns:Any ;
    linkml:slot_uri dcterms:extent .

okns:dct_hasFormat a linkml:SlotDefinition ;
    dcterms:source dcterms: ;
    dcterms:title "Has Format" ;
    rdfs:subPropertyOf okns:dct_relation ;
    skos:definition "This property is intended to be used with non-literal values. This property is an inverse property of Is Format Of." ;
    skos:editorialNote "No occurrences of this slot in the graph." ;
    skos:inScheme okns:dc ;
    skos:mappingRelation dcterms:hasFormat ;
    skos:note "description: A related resource that is substantially the same as the pre-existing described resource, but in another format." ;
    linkml:definition_uri okns:dct_hasFormat ;
    linkml:inlined true ;
    linkml:range okns:Any ;
    linkml:slot_uri dcterms:hasFormat .

okns:dct_hasPart a linkml:SlotDefinition ;
    dcterms:source dcterms: ;
    dcterms:title "Has Part" ;
    rdfs:subPropertyOf okns:dct_relation ;
    skos:definition "This property is intended to be used with non-literal values. This property is an inverse property of Is Part Of." ;
    skos:editorialNote "No occurrences of this slot in the graph." ;
    skos:inScheme okns:dc ;
    skos:mappingRelation dcterms:hasPart ;
    skos:note "description: A related resource that is included either physically or logically in the described resource." ;
    linkml:definition_uri okns:dct_hasPart ;
    linkml:inlined true ;
    linkml:range okns:Any ;
    linkml:slot_uri dcterms:hasPart .

okns:dct_hasVersion a linkml:SlotDefinition ;
    dcterms:source dcterms: ;
    dcterms:title "Has Version" ;
    rdfs:subPropertyOf okns:dct_relation ;
    skos:definition "Changes in version imply substantive changes in content rather than differences in format. This property is intended to be used with non-literal values. This property is an inverse property of Is Version Of." ;
    skos:editorialNote "No occurrences of this slot in the graph." ;
    skos:inScheme okns:dc ;
    skos:mappingRelation dcterms:hasVersion ;
    skos:note "description: A related resource that is a version, edition, or adaptation of the described resource." ;
    linkml:definition_uri okns:dct_hasVersion ;
    linkml:inlined true ;
    linkml:range okns:Any ;
    linkml:slot_uri dcterms:hasVersion .

okns:dct_instructionalMethod a linkml:SlotDefinition ;
    dcterms:source dcterms: ;
    dcterms:title "Instructional Method" ;
    skos:definition "Instructional Method typically includes ways of presenting instructional materials or conducting instructional activities, patterns of learner-to-learner and learner-to-instructor interactions, and mechanisms by which group and individual levels of learning are measured.  Instructional methods include all aspects of the instruction and learning processes from planning and implementation through evaluation and feedback." ;
    skos:editorialNote "No occurrences of this slot in the graph." ;
    skos:inScheme okns:dc ;
    skos:mappingRelation dcterms:instructionalMethod ;
    skos:note "description: A process, used to engender knowledge, attitudes and skills, that the described resource is designed to support." ;
    linkml:definition_uri okns:dct_instructionalMethod ;
    linkml:inlined true ;
    linkml:range okns:Any ;
    linkml:slot_uri dcterms:instructionalMethod .

okns:dct_isFormatOf a linkml:SlotDefinition ;
    dcterms:source dcterms: ;
    dcterms:title "Is Format Of" ;
    rdfs:subPropertyOf okns:dct_relation ;
    skos:definition "This property is intended to be used with non-literal values. This property is an inverse property of Has Format." ;
    skos:editorialNote "No occurrences of this slot in the graph." ;
    skos:inScheme okns:dc ;
    skos:mappingRelation dcterms:isFormatOf ;
    skos:note "description: A pre-existing related resource that is substantially the same as the described resource, but in another format." ;
    linkml:definition_uri okns:dct_isFormatOf ;
    linkml:inlined true ;
    linkml:range okns:Any ;
    linkml:slot_uri dcterms:isFormatOf .

okns:dct_isPartOf a linkml:SlotDefinition ;
    dcterms:source dcterms: ;
    dcterms:title "Is Part Of" ;
    rdfs:subPropertyOf okns:dct_relation ;
    skos:definition "This property is intended to be used with non-literal values. This property is an inverse property of Has Part." ;
    skos:editorialNote "No occurrences of this slot in the graph." ;
    skos:inScheme okns:dc ;
    skos:mappingRelation dcterms:isPartOf ;
    skos:note "description: A related resource in which the described resource is physically or logically included." ;
    linkml:definition_uri okns:dct_isPartOf ;
    linkml:inlined true ;
    linkml:range okns:Any ;
    linkml:slot_uri dcterms:isPartOf .

okns:dct_isReferencedBy a linkml:SlotDefinition ;
    dcterms:source dcterms: ;
    dcterms:title "Is Referenced By" ;
    rdfs:subPropertyOf okns:dct_relation ;
    skos:definition "This property is intended to be used with non-literal values. This property is an inverse property of References." ;
    skos:editorialNote "No occurrences of this slot in the graph." ;
    skos:inScheme okns:dc ;
    skos:mappingRelation dcterms:isReferencedBy ;
    skos:note "description: A related resource that references, cites, or otherwise points to the described resource." ;
    linkml:definition_uri okns:dct_isReferencedBy ;
    linkml:inlined true ;
    linkml:range okns:Any ;
    linkml:slot_uri dcterms:isReferencedBy .

okns:dct_isReplacedBy a linkml:SlotDefinition ;
    dcterms:source dcterms: ;
    dcterms:title "Is Replaced By" ;
    rdfs:subPropertyOf okns:dct_relation ;
    skos:definition "This property is intended to be used with non-literal values. This property is an inverse property of Replaces." ;
    skos:editorialNote "No occurrences of this slot in the graph." ;
    skos:inScheme okns:dc ;
    skos:mappingRelation dcterms:isReplacedBy ;
    skos:note "description: A related resource that supplants, displaces, or supersedes the described resource." ;
    linkml:definition_uri okns:dct_isReplacedBy ;
    linkml:inlined true ;
    linkml:range okns:Any ;
    linkml:slot_uri dcterms:isReplacedBy .

okns:dct_isRequiredBy a linkml:SlotDefinition ;
    dcterms:source dcterms: ;
    dcterms:title "Is Required By" ;
    rdfs:subPropertyOf okns:dct_relation ;
    skos:definition "This property is intended to be used with non-literal values. This property is an inverse property of Requires." ;
    skos:editorialNote "No occurrences of this slot in the graph." ;
    skos:inScheme okns:dc ;
    skos:mappingRelation dcterms:isRequiredBy ;
    skos:note "description: A related resource that requires the described resource to support its function, delivery, or coherence." ;
    linkml:definition_uri okns:dct_isRequiredBy ;
    linkml:inlined true ;
    linkml:range okns:Any ;
    linkml:slot_uri dcterms:isRequiredBy .

okns:dct_isVersionOf a linkml:SlotDefinition ;
    dcterms:source dcterms: ;
    dcterms:title "Is Version Of" ;
    rdfs:subPropertyOf okns:dct_relation ;
    skos:definition "Changes in version imply substantive changes in content rather than differences in format. This property is intended to be used with non-literal values. This property is an inverse property of Has Version." ;
    skos:editorialNote "No occurrences of this slot in the graph." ;
    skos:inScheme okns:dc ;
    skos:mappingRelation dcterms:isVersionOf ;
    skos:note "description: A related resource of which the described resource is a version, edition, or adaptation." ;
    linkml:definition_uri okns:dct_isVersionOf ;
    linkml:inlined true ;
    linkml:range okns:Any ;
    linkml:slot_uri dcterms:isVersionOf .

okns:dct_language a linkml:SlotDefinition ;
    dcterms:source dcterms: ;
    dcterms:title "Language" ;
    rdfs:subPropertyOf okns:dc_language ;
    skos:definition "Recommended practice is to use either a non-literal value representing a language from a controlled vocabulary such as ISO 639-2 or ISO 639-3, or a literal value consisting of an IETF Best Current Practice 47 [[IETF-BCP47](https://tools.ietf.org/html/bcp47)] language tag." ;
    skos:editorialNote "No occurrences of this slot in the graph." ;
    skos:inScheme okns:dc ;
    skos:mappingRelation dcterms:language ;
    skos:note "description: A language of the resource." ;
    linkml:definition_uri okns:dct_language ;
    linkml:inlined true ;
    linkml:range okns:Any ;
    linkml:slot_uri dcterms:language .

okns:dct_license a linkml:SlotDefinition ;
    dcterms:source dcterms: ;
    dcterms:title "License" ;
    rdfs:subPropertyOf okns:dct_rights ;
    skos:definition "Recommended practice is to identify the license document with a URI. If this is not possible or feasible, a literal value that identifies the license may be provided." ;
    skos:editorialNote "No occurrences of this slot in the graph." ;
    skos:inScheme okns:dc ;
    skos:mappingRelation dcterms:license ;
    skos:note "description: A legal document giving official permission to do something with the resource." ;
    linkml:definition_uri okns:dct_license ;
    linkml:inlined true ;
    linkml:range okns:Any ;
    linkml:slot_uri dcterms:license .

okns:dct_mediator a linkml:SlotDefinition ;
    dcterms:source dcterms: ;
    dcterms:title "Mediator" ;
    rdfs:subPropertyOf okns:dct_audience ;
    skos:definition "In an educational context, a mediator might be a parent, teacher, teaching assistant, or care-giver." ;
    skos:editorialNote "No occurrences of this slot in the graph." ;
    skos:inScheme okns:dc ;
    skos:mappingRelation dcterms:mediator ;
    skos:note "description: An entity that mediates access to the resource." ;
    linkml:definition_uri okns:dct_mediator ;
    linkml:inlined true ;
    linkml:range okns:Any ;
    linkml:slot_uri dcterms:mediator .

okns:dct_medium a linkml:SlotDefinition ;
    dcterms:source dcterms: ;
    dcterms:title "Medium" ;
    rdfs:subPropertyOf okns:dct_format ;
    skos:definition "The material or physical carrier of the resource." ;
    skos:editorialNote "No occurrences of this slot in the graph." ;
    skos:inScheme okns:dc ;
    skos:mappingRelation dcterms:medium ;
    linkml:definition_uri okns:dct_medium ;
    linkml:inlined true ;
    linkml:range okns:Any ;
    linkml:slot_uri dcterms:medium .

okns:dct_modified a linkml:SlotDefinition ;
    dcterms:source dcterms: ;
    dcterms:title "Date Modified" ;
    rdfs:subPropertyOf okns:dct_date ;
    skos:definition "Recommended practice is to describe the date, date/time, or period of time as recommended for the property Date, of which this is a subproperty." ;
    skos:inScheme okns:dc ;
    skos:mappingRelation dcterms:modified ;
    skos:note "description: Date on which the resource was changed." ;
    linkml:any_of [ a okns:AnonymousSlotExpression ;
            linkml:range okns:date ],
        [ a okns:AnonymousSlotExpression ;
            linkml:range okns:RdfsLiteral ] ;
    linkml:definition_uri okns:dct_modified ;
    linkml:inlined true ;
    linkml:range okns:Any ;
    linkml:slot_uri dcterms:modified .

okns:dct_provenance a linkml:SlotDefinition ;
    dcterms:source dcterms: ;
    dcterms:title "Provenance" ;
    skos:definition "The statement may include a description of any changes successive custodians made to the resource." ;
    skos:editorialNote "No occurrences of this slot in the graph." ;
    skos:inScheme okns:dc ;
    skos:mappingRelation dcterms:provenance ;
    skos:note "description: A statement of any changes in ownership and custody of the resource since its creation that are significant for its authenticity, integrity, and interpretation." ;
    linkml:definition_uri okns:dct_provenance ;
    linkml:inlined true ;
    linkml:range okns:Any ;
    linkml:slot_uri dcterms:provenance .

okns:dct_publisher a linkml:SlotDefinition ;
    dcterms:source dcterms: ;
    dcterms:title "Publisher" ;
    rdfs:subPropertyOf okns:dc_publisher ;
    skos:definition "An entity responsible for making the resource available." ;
    skos:inScheme okns:dc ;
    skos:mappingRelation dcterms:publisher ;
    linkml:definition_uri okns:dct_publisher ;
    linkml:range okns:uri ;
    linkml:slot_uri dcterms:publisher .

okns:dct_references a linkml:SlotDefinition ;
    dcterms:source dcterms: ;
    dcterms:title "References" ;
    rdfs:subPropertyOf okns:dct_relation ;
    skos:definition "This property is intended to be used with non-literal values. This property is an inverse property of Is Referenced By." ;
    skos:editorialNote "No occurrences of this slot in the graph." ;
    skos:inScheme okns:dc ;
    skos:mappingRelation dcterms:references ;
    skos:note "description: A related resource that is referenced, cited, or otherwise pointed to by the described resource." ;
    linkml:definition_uri okns:dct_references ;
    linkml:inlined true ;
    linkml:range okns:Any ;
    linkml:slot_uri dcterms:references .

okns:dct_replaces a linkml:SlotDefinition ;
    dcterms:source dcterms: ;
    dcterms:title "Replaces" ;
    rdfs:subPropertyOf okns:dct_relation ;
    skos:definition "This property is intended to be used with non-literal values. This property is an inverse property of Is Replaced By." ;
    skos:editorialNote "No occurrences of this slot in the graph." ;
    skos:inScheme okns:dc ;
    skos:mappingRelation dcterms:replaces ;
    skos:note "description: A related resource that is supplanted, displaced, or superseded by the described resource." ;
    linkml:definition_uri okns:dct_replaces ;
    linkml:inlined true ;
    linkml:range okns:Any ;
    linkml:slot_uri dcterms:replaces .

okns:dct_requires a linkml:SlotDefinition ;
    dcterms:source dcterms: ;
    dcterms:title "Requires" ;
    rdfs:subPropertyOf okns:dct_relation ;
    skos:definition "This property is intended to be used with non-literal values. This property is an inverse property of Is Required By." ;
    skos:editorialNote "No occurrences of this slot in the graph." ;
    skos:inScheme okns:dc ;
    skos:mappingRelation dcterms:requires ;
    skos:note "description: A related resource that is required by the described resource to support its function, delivery, or coherence." ;
    linkml:definition_uri okns:dct_requires ;
    linkml:inlined true ;
    linkml:range okns:Any ;
    linkml:slot_uri dcterms:requires .

okns:dct_rightsHolder a linkml:SlotDefinition ;
    dcterms:source dcterms: ;
    dcterms:title "Rights Holder" ;
    skos:definition "Recommended practice is to refer to the rights holder with a URI. If this is not possible or feasible, a literal value that identifies the rights holder may be provided." ;
    skos:editorialNote "No occurrences of this slot in the graph." ;
    skos:inScheme okns:dc ;
    skos:mappingRelation dcterms:rightsHolder ;
    skos:note "description: A person or organization owning or managing rights over the resource." ;
    linkml:definition_uri okns:dct_rightsHolder ;
    linkml:inlined true ;
    linkml:range okns:Any ;
    linkml:slot_uri dcterms:rightsHolder .

okns:dct_source a linkml:SlotDefinition ;
    dcterms:source dcterms: ;
    dcterms:title "Source" ;
    rdfs:subPropertyOf okns:dct_relation ;
    skos:definition "This property is intended to be used with non-literal values. The described resource may be derived from the related resource in whole or in part. Best practice is to identify the related resource by means of a URI or a string conforming to a formal identification system." ;
    skos:editorialNote "No occurrences of this slot in the graph." ;
    skos:inScheme okns:dc ;
    skos:mappingRelation dcterms:source ;
    skos:note "description: A related resource from which the described resource is derived." ;
    linkml:definition_uri okns:dct_source ;
    linkml:inlined true ;
    linkml:range okns:Any ;
    linkml:slot_uri dcterms:source .

okns:dct_spatial a linkml:SlotDefinition ;
    dcterms:source dcterms: ;
    dcterms:title "Spatial Coverage" ;
    rdfs:subPropertyOf okns:dct_coverage ;
    skos:definition "Spatial characteristics of the resource." ;
    skos:editorialNote "No occurrences of this slot in the graph." ;
    skos:inScheme okns:dc ;
    skos:mappingRelation dcterms:spatial ;
    linkml:definition_uri okns:dct_spatial ;
    linkml:inlined true ;
    linkml:range okns:Any ;
    linkml:slot_uri dcterms:spatial .

okns:dct_subject a linkml:SlotDefinition ;
    dcterms:source dcterms: ;
    dcterms:title "Subject" ;
    rdfs:subPropertyOf okns:dc_subject ;
    skos:definition "Recommended practice is to refer to the subject with a URI. If this is not possible or feasible, a literal value that identifies the subject may be provided. Both should preferably refer to a subject in a controlled vocabulary." ;
    skos:editorialNote "No occurrences of this slot in the graph." ;
    skos:inScheme okns:dc ;
    skos:mappingRelation dcterms:subject ;
    skos:note "description: A topic of the resource." ;
    linkml:definition_uri okns:dct_subject ;
    linkml:inlined true ;
    linkml:range okns:Any ;
    linkml:slot_uri dcterms:subject .

okns:dct_tableOfContents a linkml:SlotDefinition ;
    dcterms:source dcterms: ;
    dcterms:title "Table Of Contents" ;
    rdfs:subPropertyOf okns:dct_description ;
    skos:definition "A list of subunits of the resource." ;
    skos:editorialNote "No occurrences of this slot in the graph." ;
    skos:inScheme okns:dc ;
    skos:mappingRelation dcterms:tableOfContents ;
    linkml:definition_uri okns:dct_tableOfContents ;
    linkml:inlined true ;
    linkml:range okns:Any ;
    linkml:slot_uri dcterms:tableOfContents .

okns:dct_temporal a linkml:SlotDefinition ;
    dcterms:source dcterms: ;
    dcterms:title "Temporal Coverage" ;
    rdfs:subPropertyOf okns:dct_coverage ;
    skos:definition "Temporal characteristics of the resource." ;
    skos:editorialNote "No occurrences of this slot in the graph." ;
    skos:inScheme okns:dc ;
    skos:mappingRelation dcterms:temporal ;
    linkml:definition_uri okns:dct_temporal ;
    linkml:inlined true ;
    linkml:range okns:Any ;
    linkml:slot_uri dcterms:temporal .

okns:dct_type a linkml:SlotDefinition ;
    dcterms:source dcterms: ;
    dcterms:title "Type" ;
    rdfs:subPropertyOf okns:dc_type ;
    skos:definition "Recommended practice is to use a controlled vocabulary such as the DCMI Type Vocabulary [[DCMI-TYPE](http://dublincore.org/documents/dcmi-type-vocabulary/)]. To describe the file format, physical medium, or dimensions of the resource, use the property Format." ;
    skos:editorialNote "No occurrences of this slot in the graph." ;
    skos:inScheme okns:dc ;
    skos:mappingRelation dcterms:type ;
    skos:note "description: The nature or genre of the resource." ;
    linkml:definition_uri okns:dct_type ;
    linkml:inlined true ;
    linkml:range okns:Any ;
    linkml:slot_uri dcterms:type .

okns:dct_valid a linkml:SlotDefinition ;
    dcterms:source dcterms: ;
    dcterms:title "Date Valid" ;
    rdfs:subPropertyOf okns:dct_date ;
    skos:definition "Recommended practice is to describe the date, date/time, or period of time as recommended for the property Date, of which this is a subproperty." ;
    skos:editorialNote "No occurrences of this slot in the graph." ;
    skos:inScheme okns:dc ;
    skos:mappingRelation dcterms:valid ;
    skos:note "description: Date (often a range) of validity of a resource." ;
    linkml:definition_uri okns:dct_valid ;
    linkml:inlined true ;
    linkml:range okns:RdfsLiteral ;
    linkml:slot_uri dcterms:valid .

okns:double a linkml:TypeDefinition ;
    skos:closeMatch schema1:Float ;
    skos:definition "A real number that conforms to the xsd:double specification" ;
    skos:editorialNote "If you are authoring schemas in LinkML YAML, the type is referenced with the lower case \"double\"." ;
    skos:inScheme linkml:types ;
    linkml:base "float" ;
    linkml:imported_from "linkml:types" ;
    linkml:definition_uri linkml:Double ;
    linkml:uri xsd:double .

<https://purl.org/okn/schema/http___def.isotc211.org_iso19150_2_2012_base#isEnumeration> a linkml:SlotDefinition ;
    skos:inScheme okns:sc ;
    skos:mappingRelation <http://def.isotc211.org/iso19150-2/2012/base#isEnumeration> ;
    linkml:definition_uri <https://purl.org/okn/schema/http___def.isotc211.org_iso19150_2_2012_base#isEnumeration> ;
    linkml:range okns:boolean ;
    linkml:slot_uri <http://def.isotc211.org/iso19150-2/2012/base#isEnumeration> .

okns:hyf_absolute a linkml:SlotDefinition ;
    skos:definition "geometric expression of the distance from a located referent. An implementation may use the types described in ISO 19103: Conceptual Schema." ;
    skos:editorialNote "No occurrences of this slot in the graph." ;
    skos:inScheme okns:hyf ;
    skos:mappingRelation <https://www.opengis.net/def/schema/hy_features/hyf/absolute> ;
    linkml:definition_uri okns:hyf_absolute ;
    linkml:range okns:sc_Measure ;
    linkml:slot_uri <https://www.opengis.net/def/schema/hy_features/hyf/absolute> .

okns:hyf_accumulatingWaterBody a linkml:SlotDefinition ;
    skos:definition "water body (stratum) wherein liquid water is accumulated." ;
    skos:editorialNote "No occurrences of this slot in the graph." ;
    skos:inScheme okns:hyf ;
    skos:mappingRelation <https://www.opengis.net/def/schema/hy_features/hyf/accumulatingWaterBody> ;
    linkml:definition_uri okns:hyf_accumulatingWaterBody ;
    linkml:inlined true ;
    linkml:range okns:Any ;
    linkml:slot_uri <https://www.opengis.net/def/schema/hy_features/hyf/accumulatingWaterBody> .

okns:hyf_accuracyStatement a linkml:SlotDefinition ;
    skos:definition "simple statement whether the distance value agrees with the value accepted as being true.  This statement assumes that all known corrections have been applied. An implementation may use the types described in ISO 19103: Conceptual Schema." ;
    skos:editorialNote "No occurrences of this slot in the graph." ;
    skos:inScheme okns:hyf ;
    skos:mappingRelation <https://www.opengis.net/def/schema/hy_features/hyf/accuracyStatement> ;
    linkml:definition_uri okns:hyf_accuracyStatement ;
    linkml:range okns:string ;
    linkml:slot_uri <https://www.opengis.net/def/schema/hy_features/hyf/accuracyStatement> .

okns:hyf_bedProfileLongitudinal a linkml:SlotDefinition ;
    skos:definition "identifies a longitudinal vertical shape of a channel, carrying a permanent reference location which realizes the hydro nexus of the catchment which is realized by the channel." ;
    skos:editorialNote "No occurrences of this slot in the graph." ;
    skos:inScheme okns:hyf ;
    skos:mappingRelation <https://www.opengis.net/def/schema/hy_features/hyf/bedProfileLongitudinal> ;
    linkml:definition_uri okns:hyf_bedProfileLongitudinal ;
    linkml:inlined true ;
    linkml:range okns:Any ;
    linkml:slot_uri <https://www.opengis.net/def/schema/hy_features/hyf/bedProfileLongitudinal> .

okns:hyf_bedProfileTransversal a linkml:SlotDefinition ;
    skos:definition "identifies a transversal vertical shape of a channel, carrying a permanent reference location which realizes the hydro nexus of the catchment which is realized by the channel." ;
    skos:editorialNote "No occurrences of this slot in the graph." ;
    skos:inScheme okns:hyf ;
    skos:mappingRelation <https://www.opengis.net/def/schema/hy_features/hyf/bedProfileTransversal> ;
    linkml:definition_uri okns:hyf_bedProfileTransversal ;
    linkml:inlined true ;
    linkml:range okns:Any ;
    linkml:slot_uri <https://www.opengis.net/def/schema/hy_features/hyf/bedProfileTransversal> .

okns:hyf_catchmentArea a linkml:SlotDefinition ;
    skos:definition "catchment area that participates in the network." ;
    skos:editorialNote "No occurrences of this slot in the graph." ;
    skos:inScheme okns:hyf ;
    skos:mappingRelation <https://www.opengis.net/def/schema/hy_features/hyf/catchmentArea> ;
    linkml:definition_uri okns:hyf_catchmentArea ;
    linkml:inlined true ;
    linkml:range okns:HyfHYCatchmentArea ;
    linkml:slot_uri <https://www.opengis.net/def/schema/hy_features/hyf/catchmentArea> .

okns:hyf_catchmentDivide a linkml:SlotDefinition ;
    skos:definition "catchment boundary that participates in the network." ;
    skos:editorialNote "No occurrences of this slot in the graph." ;
    skos:inScheme okns:hyf ;
    skos:mappingRelation <https://www.opengis.net/def/schema/hy_features/hyf/catchmentDivide> ;
    linkml:definition_uri okns:hyf_catchmentDivide ;
    linkml:inlined true ;
    linkml:range okns:HyfHYCatchmentDivide ;
    linkml:slot_uri <https://www.opengis.net/def/schema/hy_features/hyf/catchmentDivide> .

okns:hyf_catchmentRealization a linkml:SlotDefinition ;
    skos:definition "topological or geographic feature which realizes the logical catchment." ;
    skos:editorialNote "No occurrences of this slot in the graph." ;
    skos:inScheme okns:hyf ;
    skos:mappingRelation <https://www.opengis.net/def/schema/hy_features/hyf/catchmentRealization> ;
    linkml:definition_uri okns:hyf_catchmentRealization ;
    linkml:inlined true ;
    linkml:range okns:HyfHYCatchmentRealization ;
    linkml:slot_uri <https://www.opengis.net/def/schema/hy_features/hyf/catchmentRealization> .

okns:hyf_code a linkml:SlotDefinition ;
    skos:definition "unique identifier to the catchment in given context. The code attribute should be implemented using a controlled classification or coding system. Example: WMO Basin Codes." ;
    skos:editorialNote "No occurrences of this slot in the graph." ;
    skos:inScheme okns:hyf ;
    skos:mappingRelation <https://www.opengis.net/def/schema/hy_features/hyf/code> ;
    linkml:definition_uri okns:hyf_code ;
    linkml:inlined true ;
    linkml:range okns:RdfsResource ;
    linkml:slot_uri <https://www.opengis.net/def/schema/hy_features/hyf/code> .

okns:hyf_confinedWaterBody a linkml:SlotDefinition ;
    skos:definition "identifies a stratum of waterbody contained in the depression." ;
    skos:editorialNote "No occurrences of this slot in the graph." ;
    skos:inScheme okns:hyf ;
    skos:mappingRelation <https://www.opengis.net/def/schema/hy_features/hyf/confinedWaterBody> ;
    linkml:definition_uri okns:hyf_confinedWaterBody ;
    linkml:inlined true ;
    linkml:range okns:Any ;
    linkml:slot_uri <https://www.opengis.net/def/schema/hy_features/hyf/confinedWaterBody> .

okns:hyf_conjointCatchment a linkml:SlotDefinition ;
    skos:definition "catchment that interacts with the catchment across an internal boundary line." ;
    skos:editorialNote "No occurrences of this slot in the graph." ;
    skos:inScheme okns:hyf ;
    skos:mappingRelation <https://www.opengis.net/def/schema/hy_features/hyf/conjointCatchment> ;
    linkml:definition_uri okns:hyf_conjointCatchment ;
    linkml:inlined true ;
    linkml:range okns:HyfHYCatchment ;
    linkml:slot_uri <https://www.opengis.net/def/schema/hy_features/hyf/conjointCatchment> .

okns:hyf_containedCatchment a linkml:SlotDefinition ;
    skos:definition "catchment nested in a containing catchment." ;
    skos:editorialNote "No occurrences of this slot in the graph." ;
    skos:inScheme okns:hyf ;
    skos:mappingRelation <https://www.opengis.net/def/schema/hy_features/hyf/containedCatchment> ;
    linkml:definition_uri okns:hyf_containedCatchment ;
    linkml:inlined true ;
    linkml:range okns:HyfHYCatchment ;
    linkml:slot_uri <https://www.opengis.net/def/schema/hy_features/hyf/containedCatchment> .

okns:hyf_containingCatchment a linkml:SlotDefinition ;
    skos:definition "catchment nesting contained catchments." ;
    skos:editorialNote "No occurrences of this slot in the graph." ;
    skos:inScheme okns:hyf ;
    skos:mappingRelation <https://www.opengis.net/def/schema/hy_features/hyf/containingCatchment> ;
    linkml:definition_uri okns:hyf_containingCatchment ;
    linkml:inlined true ;
    linkml:range okns:HyfHYCatchment ;
    linkml:slot_uri <https://www.opengis.net/def/schema/hy_features/hyf/containingCatchment> .

okns:hyf_contributingCatchment a linkml:SlotDefinition ;
    skos:definition "identifies the catchment that contributes flow to this hydro nexus. This allows connection of a catchment's outflow to an identified inflow and to determine its position through referencing the inflow." ;
    skos:editorialNote "No occurrences of this slot in the graph." ;
    skos:inScheme okns:hyf ;
    skos:mappingRelation <https://www.opengis.net/def/schema/hy_features/hyf/contributingCatchment> ;
    linkml:definition_uri okns:hyf_contributingCatchment ;
    linkml:inlined true ;
    linkml:range okns:HyfHYCatchment ;
    linkml:slot_uri <https://www.opengis.net/def/schema/hy_features/hyf/contributingCatchment> .

okns:hyf_coveredWaterBody a linkml:SlotDefinition ;
    skos:definition "body of open water covered by a layer of ice or snow." ;
    skos:editorialNote "No occurrences of this slot in the graph." ;
    skos:inScheme okns:hyf ;
    skos:mappingRelation <https://www.opengis.net/def/schema/hy_features/hyf/coveredWaterBody> ;
    linkml:definition_uri okns:hyf_coveredWaterBody ;
    linkml:inlined true ;
    linkml:range okns:Any ;
    linkml:slot_uri <https://www.opengis.net/def/schema/hy_features/hyf/coveredWaterBody> .

okns:hyf_distanceDescription a linkml:SlotDefinition ;
    skos:definition "term describing the distance from the feature being used as a reference. An implementation may use the HY_DistanceDescription code list. Alternatively, the types described in ISO 19103: Conceptual Schema may be used." ;
    skos:editorialNote "No occurrences of this slot in the graph." ;
    skos:inScheme okns:hyf ;
    skos:mappingRelation <https://www.opengis.net/def/schema/hy_features/hyf/distanceDescription> ;
    linkml:definition_uri okns:hyf_distanceDescription ;
    linkml:inlined true ;
    linkml:range okns:HyfHYDistanceDescription ;
    linkml:slot_uri <https://www.opengis.net/def/schema/hy_features/hyf/distanceDescription> .

okns:hyf_distanceExpression a linkml:SlotDefinition ;
    skos:definition "absolute or interpolative value of the distance from the feature being used as a reference, including an indication of accuracy and precision of the absolute value. An implementation may use the HY_DistanceFromReferent (data type) referencing basic types. Alternatively, the types described in ISO 19103: Conceptual Schema may be used." ;
    skos:editorialNote "No occurrences of this slot in the graph." ;
    skos:inScheme okns:hyf ;
    skos:mappingRelation <https://www.opengis.net/def/schema/hy_features/hyf/distanceExpression> ;
    linkml:definition_uri okns:hyf_distanceExpression ;
    linkml:inlined true ;
    linkml:range okns:HyfHYDistanceFromReferent ;
    linkml:slot_uri <https://www.opengis.net/def/schema/hy_features/hyf/distanceExpression> .

okns:hyf_downstreamWaterBody a linkml:SlotDefinition ;
    skos:definition "identifies another waterbody immediately downstream, allowing network navigation without knowing an inflow or outflow of the catchment realized by the waterbody." ;
    skos:editorialNote "No occurrences of this slot in the graph." ;
    skos:inScheme okns:hyf ;
    skos:mappingRelation <https://www.opengis.net/def/schema/hy_features/hyf/downstreamWaterBody> ;
    linkml:definition_uri okns:hyf_downstreamWaterBody ;
    linkml:inlined true ;
    linkml:range okns:Any ;
    linkml:slot_uri <https://www.opengis.net/def/schema/hy_features/hyf/downstreamWaterBody> .

okns:hyf_endorheicDrainage a linkml:SlotDefinition ;
    skos:definition "should be used to identify an endorheic-drained catchment, which is not, but may be temporarily connected to the enveloping catchment." ;
    skos:editorialNote "No occurrences of this slot in the graph." ;
    skos:inScheme okns:hyf ;
    skos:mappingRelation <https://www.opengis.net/def/schema/hy_features/hyf/endorheicDrainage> ;
    linkml:definition_uri okns:hyf_endorheicDrainage ;
    linkml:inlined true ;
    linkml:range okns:HyfHYInteriorCatchment ;
    linkml:slot_uri <https://www.opengis.net/def/schema/hy_features/hyf/endorheicDrainage> .

okns:hyf_exorheicDrainage a linkml:SlotDefinition ;
    skos:definition "should be used to identify an exorheic-drained catchment which is permanently connected to the encompassing catchment." ;
    skos:editorialNote "No occurrences of this slot in the graph." ;
    skos:inScheme okns:hyf ;
    skos:mappingRelation <https://www.opengis.net/def/schema/hy_features/hyf/exorheicDrainage> ;
    linkml:definition_uri okns:hyf_exorheicDrainage ;
    linkml:inlined true ;
    linkml:range okns:HyfHYDendriticCatchment ;
    linkml:slot_uri <https://www.opengis.net/def/schema/hy_features/hyf/exorheicDrainage> .

okns:hyf_flowpath a linkml:SlotDefinition ;
    skos:definition "flowpath that participates in the network." ;
    skos:editorialNote "No occurrences of this slot in the graph." ;
    skos:inScheme okns:hyf ;
    skos:mappingRelation <https://www.opengis.net/def/schema/hy_features/hyf/flowpath> ;
    linkml:definition_uri okns:hyf_flowpath ;
    linkml:inlined true ;
    linkml:range okns:HyfHYFlowPath ;
    linkml:slot_uri <https://www.opengis.net/def/schema/hy_features/hyf/flowpath> .

okns:hyf_hydroLocationType a linkml:SlotDefinition ;
    skos:definition "expresses the type of the realized nexus, using a term from the HY_HydroLocationType code list, or a controlled vocabulary. Alternative code lists may be used but should be related to the terms in this code list using an appropriate formalism." ;
    skos:editorialNote "No occurrences of this slot in the graph." ;
    skos:inScheme okns:hyf ;
    skos:mappingRelation <https://www.opengis.net/def/schema/hy_features/hyf/hydroLocationType> ;
    linkml:definition_uri okns:hyf_hydroLocationType ;
    linkml:inlined true ;
    linkml:range okns:HyfHYHydroLocationType ;
    linkml:slot_uri <https://www.opengis.net/def/schema/hy_features/hyf/hydroLocationType> .

okns:hyf_inflow a linkml:SlotDefinition ;
    skos:definition "hydro nexus in terms of an inflow to the receiving catchment. For a dendritic network of catchments, the outflow of a contributing catchment coincides with the inflow to a receiving catchment. This supports description of upstream-downstream relationships between catchments." ;
    skos:editorialNote "No occurrences of this slot in the graph." ;
    skos:inScheme okns:hyf ;
    skos:mappingRelation <https://www.opengis.net/def/schema/hy_features/hyf/inflow> ;
    linkml:definition_uri okns:hyf_inflow ;
    linkml:inlined true ;
    linkml:range okns:HyfHYHydroNexus ;
    linkml:slot_uri <https://www.opengis.net/def/schema/hy_features/hyf/inflow> .

okns:hyf_interpolative a linkml:SlotDefinition ;
    skos:definition "interpolative expression (percentage) of the distance from a located referent. An implementation may use the types described in ISO 19103: Conceptual Schema." ;
    skos:editorialNote "No occurrences of this slot in the graph." ;
    skos:inScheme okns:hyf ;
    skos:mappingRelation <https://www.opengis.net/def/schema/hy_features/hyf/interpolative> ;
    linkml:definition_uri okns:hyf_interpolative ;
    linkml:range okns:double ;
    linkml:slot_uri <https://www.opengis.net/def/schema/hy_features/hyf/interpolative> .

okns:hyf_linearElement a linkml:SlotDefinition ;
    skos:definition "identifies a flowpath used as the linear element along which a position is assigned to a hydro-location, or any feature of interest." ;
    skos:editorialNote "No occurrences of this slot in the graph." ;
    skos:inScheme okns:hyf ;
    skos:mappingRelation <https://www.opengis.net/def/schema/hy_features/hyf/linearElement> ;
    linkml:definition_uri okns:hyf_linearElement ;
    linkml:inlined true ;
    linkml:range okns:HyfHYFlowPath ;
    linkml:slot_uri <https://www.opengis.net/def/schema/hy_features/hyf/linearElement> .

okns:hyf_locatedReferent a linkml:SlotDefinition ;
    skos:definition "identifies an already referenced location such as a catchment outlet relative to which a position may be assigned to a feature of interest." ;
    skos:editorialNote "No occurrences of this slot in the graph." ;
    skos:inScheme okns:hyf ;
    skos:mappingRelation <https://www.opengis.net/def/schema/hy_features/hyf/locatedReferent> ;
    linkml:definition_uri okns:hyf_locatedReferent ;
    linkml:inlined true ;
    linkml:range okns:HyfHYHydroLocation ;
    linkml:slot_uri <https://www.opengis.net/def/schema/hy_features/hyf/locatedReferent> .

okns:hyf_lowerCatchment a linkml:SlotDefinition ;
    skos:definition "catchment located immediately below of the catchment," ;
    skos:editorialNote "No occurrences of this slot in the graph." ;
    skos:inScheme okns:hyf ;
    skos:mappingRelation <https://www.opengis.net/def/schema/hy_features/hyf/lowerCatchment> ;
    linkml:definition_uri okns:hyf_lowerCatchment ;
    linkml:inlined true ;
    linkml:range okns:HyfHYCatchment ;
    linkml:slot_uri <https://www.opengis.net/def/schema/hy_features/hyf/lowerCatchment> .

okns:hyf_namesPart a linkml:SlotDefinition ;
    skos:definition "indicates whether the name applies to a part of feature only or not, using the Boolean value type" ;
    skos:editorialNote "No occurrences of this slot in the graph." ;
    skos:inScheme okns:hyf ;
    skos:mappingRelation <https://www.opengis.net/def/schema/hy_features/hyf/namesPart> ;
    linkml:definition_uri okns:hyf_namesPart ;
    linkml:range okns:boolean ;
    linkml:slot_uri <https://www.opengis.net/def/schema/hy_features/hyf/namesPart> .

okns:hyf_networkStation a linkml:SlotDefinition ;
    skos:definition "hydrometric feature which realizes the catchment either separately, or as part of the hydrometric network." ;
    skos:editorialNote "No occurrences of this slot in the graph." ;
    skos:inScheme okns:hyf ;
    skos:mappingRelation <https://www.opengis.net/def/schema/hy_features/hyf/networkStation> ;
    linkml:definition_uri okns:hyf_networkStation ;
    linkml:inlined true ;
    linkml:range okns:Any ;
    linkml:slot_uri <https://www.opengis.net/def/schema/hy_features/hyf/networkStation> .

okns:hyf_networkWaterBody a linkml:SlotDefinition ;
    skos:definition "waterbody which realizes the catchment either separately, or as part of the hydrographic network." ;
    skos:editorialNote "No occurrences of this slot in the graph." ;
    skos:inScheme okns:hyf ;
    skos:mappingRelation <https://www.opengis.net/def/schema/hy_features/hyf/networkWaterBody> ;
    linkml:definition_uri okns:hyf_networkWaterBody ;
    linkml:inlined true ;
    linkml:range okns:Any ;
    linkml:slot_uri <https://www.opengis.net/def/schema/hy_features/hyf/networkWaterBody> .

okns:hyf_nexusRealization a linkml:SlotDefinition ;
    skos:definition "identifies a hydrologic feature which realizes the hydro nexus. A topological nexus realization is of lower dimension than the realization of the corresponding catchment. Example: an outflow node realizing the nexus would be of lower dimension than the flowpath edge realizing the contributing catchment." ;
    skos:editorialNote "No occurrences of this slot in the graph." ;
    skos:inScheme okns:hyf ;
    skos:mappingRelation <https://www.opengis.net/def/schema/hy_features/hyf/nexusRealization> ;
    linkml:definition_uri okns:hyf_nexusRealization ;
    linkml:inlined true ;
    linkml:range okns:HyfHYHydroLocation ;
    linkml:slot_uri <https://www.opengis.net/def/schema/hy_features/hyf/nexusRealization> .

okns:hyf_outflow a linkml:SlotDefinition ;
    skos:definition "hydro nexus in terms of an outflow of the contributing catchment. For a dendritic network of catchments, the outflow of a contributing catchment coincides with the inflow to a receiving catchment. This supports description of upstream-downstream relationships between catchments." ;
    skos:editorialNote "No occurrences of this slot in the graph." ;
    skos:inScheme okns:hyf ;
    skos:mappingRelation <https://www.opengis.net/def/schema/hy_features/hyf/outflow> ;
    linkml:definition_uri okns:hyf_outflow ;
    linkml:inlined true ;
    linkml:range okns:HyfHYHydroNexus ;
    linkml:slot_uri <https://www.opengis.net/def/schema/hy_features/hyf/outflow> .

okns:hyf_precisionStatement a linkml:SlotDefinition ;
    skos:definition "simple statement on the smallest unit of division on the scale of measurement. An implementation may use the types described in ISO 19103: Conceptual Schema." ;
    skos:editorialNote "No occurrences of this slot in the graph." ;
    skos:inScheme okns:hyf ;
    skos:mappingRelation <https://www.opengis.net/def/schema/hy_features/hyf/precisionStatement> ;
    linkml:definition_uri okns:hyf_precisionStatement ;
    linkml:range okns:sc_Measure ;
    linkml:slot_uri <https://www.opengis.net/def/schema/hy_features/hyf/precisionStatement> .

okns:hyf_preferredBy a linkml:SlotDefinition ;
    skos:definition "specifies that the name is the preferred name according to the named entity. The CI_Responsibility type may be used to further structure the information about the responsible party and their role." ;
    skos:editorialNote "No occurrences of this slot in the graph." ;
    skos:inScheme okns:hyf ;
    skos:mappingRelation <https://www.opengis.net/def/schema/hy_features/hyf/preferredBy> ;
    linkml:definition_uri okns:hyf_preferredBy ;
    linkml:inlined true ;
    linkml:range okns:Seegrid-ciResponsibleParty ;
    linkml:slot_uri <https://www.opengis.net/def/schema/hy_features/hyf/preferredBy> .

okns:hyf_realizedCatchment a linkml:SlotDefinition ;
    skos:definition "identifies the one and only one catchment that is realized by a particular feature. Referencing the hydrologic complex containing the catchment and all of its realizations, supports a catchment's existence to be recognized and linked to multiple realizations without the complexity and full detail of a scientific model. By referencing the catchment topology, topological relationships can be established and common identifiers assigned." ;
    skos:editorialNote "No occurrences of this slot in the graph." ;
    skos:inScheme okns:hyf ;
    skos:mappingRelation <https://www.opengis.net/def/schema/hy_features/hyf/realizedCatchment> ;
    linkml:definition_uri okns:hyf_realizedCatchment ;
    linkml:inlined true ;
    linkml:range okns:HyfHYCatchment ;
    linkml:slot_uri <https://www.opengis.net/def/schema/hy_features/hyf/realizedCatchment> .

okns:hyf_realizedNexus a linkml:SlotDefinition ;
    skos:definition "identifies the one and only one nexus that is realized by a particular feature. Referencing the hydrologic complex containing the hydro nexus and all of its realizations, supports an arbitrary feature of interest to be recognized as outlet of a catchment, and to be placed using the river referencing defined in this standard." ;
    skos:editorialNote "No occurrences of this slot in the graph." ;
    skos:inScheme okns:hyf ;
    skos:mappingRelation <https://www.opengis.net/def/schema/hy_features/hyf/realizedNexus> ;
    linkml:definition_uri okns:hyf_realizedNexus ;
    linkml:inlined true ;
    linkml:range okns:HyfHYHydroNexus ;
    linkml:slot_uri <https://www.opengis.net/def/schema/hy_features/hyf/realizedNexus> .

okns:hyf_receivingCatchment a linkml:SlotDefinition ;
    skos:definition "identifies the catchment that receives flow from this hydro nexus. This allows connection of a catchment's inflow to an identified outflow and to determine its position through referencing the outflow." ;
    skos:editorialNote "No occurrences of this slot in the graph." ;
    skos:inScheme okns:hyf ;
    skos:mappingRelation <https://www.opengis.net/def/schema/hy_features/hyf/receivingCatchment> ;
    linkml:definition_uri okns:hyf_receivingCatchment ;
    linkml:inlined true ;
    linkml:range okns:HyfHYCatchment ;
    linkml:slot_uri <https://www.opengis.net/def/schema/hy_features/hyf/receivingCatchment> .

okns:hyf_referenceLocation a linkml:SlotDefinition ;
    skos:definition "identifies the permanent reference location, usually an existing inflow or outflow hydro nexus relative to which a position is assigned to a hydro location feature of interest." ;
    skos:editorialNote "No occurrences of this slot in the graph." ;
    skos:inScheme okns:hyf ;
    skos:mappingRelation <https://www.opengis.net/def/schema/hy_features/hyf/referenceLocation> ;
    linkml:definition_uri okns:hyf_referenceLocation ;
    linkml:inlined true ;
    linkml:range okns:HyfHYHydroLocation ;
    linkml:slot_uri <https://www.opengis.net/def/schema/hy_features/hyf/referenceLocation> .

okns:hyf_referencedPosition a linkml:SlotDefinition ;
    skos:definition "position expressed as measured or otherwise described distance from a known, already located referent. Commonly, this is used to locate a feature of interest such as a hydrometric station in relation to a catchment's outlet fixed by co-ordinates." ;
    skos:editorialNote "No occurrences of this slot in the graph." ;
    skos:inScheme okns:hyf ;
    skos:mappingRelation <https://www.opengis.net/def/schema/hy_features/hyf/referencedPosition> ;
    linkml:definition_uri okns:hyf_referencedPosition ;
    linkml:inlined true ;
    linkml:range okns:HyfHYIndirectPosition ;
    linkml:slot_uri <https://www.opengis.net/def/schema/hy_features/hyf/referencedPosition> .

okns:hyf_reservoirZone a linkml:SlotDefinition ;
    skos:definition "identifies the waterbody stratum used for storage, for example a management zone, or flood control zone." ;
    skos:editorialNote "No occurrences of this slot in the graph." ;
    skos:inScheme okns:hyf ;
    skos:mappingRelation <https://www.opengis.net/def/schema/hy_features/hyf/reservoirZone> ;
    linkml:definition_uri okns:hyf_reservoirZone ;
    linkml:inlined true ;
    linkml:range okns:Any ;
    linkml:slot_uri <https://www.opengis.net/def/schema/hy_features/hyf/reservoirZone> .

okns:hyf_snowmelt a linkml:SlotDefinition ;
    skos:definition "liquid water from melting of snow." ;
    skos:editorialNote "No occurrences of this slot in the graph." ;
    skos:inScheme okns:hyf ;
    skos:mappingRelation <https://www.opengis.net/def/schema/hy_features/hyf/snowmelt> ;
    linkml:definition_uri okns:hyf_snowmelt ;
    linkml:inlined true ;
    linkml:range okns:Any ;
    linkml:slot_uri <https://www.opengis.net/def/schema/hy_features/hyf/snowmelt> .

okns:hyf_standingWater a linkml:SlotDefinition ;
    skos:definition "identifies the body of stagnant water contained in the depression." ;
    skos:editorialNote "No occurrences of this slot in the graph." ;
    skos:inScheme okns:hyf ;
    skos:mappingRelation <https://www.opengis.net/def/schema/hy_features/hyf/standingWater> ;
    linkml:definition_uri okns:hyf_standingWater ;
    linkml:inlined true ;
    linkml:range okns:Any ;
    linkml:slot_uri <https://www.opengis.net/def/schema/hy_features/hyf/standingWater> .

okns:hyf_storage a linkml:SlotDefinition ;
    skos:definition "identifies a reservoir storing water as a resource for future use. This may be used to describe storage characteristics of the water body participating in the hydrographic network." ;
    skos:editorialNote "No occurrences of this slot in the graph." ;
    skos:inScheme okns:hyf ;
    skos:mappingRelation <https://www.opengis.net/def/schema/hy_features/hyf/storage> ;
    linkml:definition_uri okns:hyf_storage ;
    linkml:inlined true ;
    linkml:range okns:Any ;
    linkml:slot_uri <https://www.opengis.net/def/schema/hy_features/hyf/storage> .

okns:hyf_storedWaterBody a linkml:SlotDefinition ;
    skos:definition "identifies the network waterbody that specifies the connectivity of the storage reservoir in the hydrographic network." ;
    skos:editorialNote "No occurrences of this slot in the graph." ;
    skos:inScheme okns:hyf ;
    skos:mappingRelation <https://www.opengis.net/def/schema/hy_features/hyf/storedWaterBody> ;
    linkml:definition_uri okns:hyf_storedWaterBody ;
    linkml:inlined true ;
    linkml:range okns:Any ;
    linkml:slot_uri <https://www.opengis.net/def/schema/hy_features/hyf/storedWaterBody> .

okns:hyf_stratum a linkml:SlotDefinition ;
    skos:definition "identifies a horizontal layer of consistent characteristics, or a storage zone of a reservoir." ;
    skos:editorialNote "No occurrences of this slot in the graph." ;
    skos:inScheme okns:hyf ;
    skos:mappingRelation <https://www.opengis.net/def/schema/hy_features/hyf/stratum> ;
    linkml:definition_uri okns:hyf_stratum ;
    linkml:inlined true ;
    linkml:range okns:Any ;
    linkml:slot_uri <https://www.opengis.net/def/schema/hy_features/hyf/stratum> .

okns:hyf_stream a linkml:SlotDefinition ;
    skos:definition "identifies the waterbody periodically or continuously flowing in the channel, including subterranean streams." ;
    skos:editorialNote "No occurrences of this slot in the graph." ;
    skos:inScheme okns:hyf ;
    skos:mappingRelation <https://www.opengis.net/def/schema/hy_features/hyf/stream> ;
    linkml:definition_uri okns:hyf_stream ;
    linkml:inlined true ;
    linkml:range okns:Any ;
    linkml:slot_uri <https://www.opengis.net/def/schema/hy_features/hyf/stream> .

okns:hyf_streamCrossSection a linkml:SlotDefinition ;
    skos:definition "identifies a vertical section at right angles to the main (average) direction of flow." ;
    skos:editorialNote "No occurrences of this slot in the graph." ;
    skos:inScheme okns:hyf ;
    skos:mappingRelation <https://www.opengis.net/def/schema/hy_features/hyf/streamCrossSection> ;
    linkml:definition_uri okns:hyf_streamCrossSection ;
    linkml:inlined true ;
    linkml:range okns:Any ;
    linkml:slot_uri <https://www.opengis.net/def/schema/hy_features/hyf/streamCrossSection> .

okns:hyf_streamLongitudinalSection a linkml:SlotDefinition ;
    skos:definition "identifies a vertical section or along a centerline." ;
    skos:editorialNote "No occurrences of this slot in the graph." ;
    skos:inScheme okns:hyf ;
    skos:mappingRelation <https://www.opengis.net/def/schema/hy_features/hyf/streamLongitudinalSection> ;
    linkml:definition_uri okns:hyf_streamLongitudinalSection ;
    linkml:inlined true ;
    linkml:range okns:Any ;
    linkml:slot_uri <https://www.opengis.net/def/schema/hy_features/hyf/streamLongitudinalSection> .

okns:hyf_surfaceChannel a linkml:SlotDefinition ;
    skos:definition "channel on the land surface which realizes the catchment either separately, or as part of the channel network." ;
    skos:editorialNote "No occurrences of this slot in the graph." ;
    skos:inScheme okns:hyf ;
    skos:mappingRelation <https://www.opengis.net/def/schema/hy_features/hyf/surfaceChannel> ;
    linkml:definition_uri okns:hyf_surfaceChannel ;
    linkml:inlined true ;
    linkml:range okns:Any ;
    linkml:slot_uri <https://www.opengis.net/def/schema/hy_features/hyf/surfaceChannel> .

okns:hyf_surfaceDepression a linkml:SlotDefinition ;
    skos:definition "depression on the land surface which realizes the catchment either separately, or as part of the channel network." ;
    skos:editorialNote "No occurrences of this slot in the graph." ;
    skos:inScheme okns:hyf ;
    skos:mappingRelation <https://www.opengis.net/def/schema/hy_features/hyf/surfaceDepression> ;
    linkml:definition_uri okns:hyf_surfaceDepression ;
    linkml:inlined true ;
    linkml:range okns:Any ;
    linkml:slot_uri <https://www.opengis.net/def/schema/hy_features/hyf/surfaceDepression> .

okns:hyf_upperCatchment a linkml:SlotDefinition ;
    skos:definition "catchment located immediately above of the catchment," ;
    skos:editorialNote "No occurrences of this slot in the graph." ;
    skos:inScheme okns:hyf ;
    skos:mappingRelation <https://www.opengis.net/def/schema/hy_features/hyf/upperCatchment> ;
    linkml:definition_uri okns:hyf_upperCatchment ;
    linkml:inlined true ;
    linkml:range okns:HyfHYCatchment ;
    linkml:slot_uri <https://www.opengis.net/def/schema/hy_features/hyf/upperCatchment> .

okns:hyf_upstreamWaterBody a linkml:SlotDefinition ;
    skos:definition "identifies another waterbody immediately upstream, allowing network navigation without knowing an inflow or outflow of the catchment realized by the waterbody." ;
    skos:editorialNote "No occurrences of this slot in the graph." ;
    skos:inScheme okns:hyf ;
    skos:mappingRelation <https://www.opengis.net/def/schema/hy_features/hyf/upstreamWaterBody> ;
    linkml:definition_uri okns:hyf_upstreamWaterBody ;
    linkml:inlined true ;
    linkml:range okns:Any ;
    linkml:slot_uri <https://www.opengis.net/def/schema/hy_features/hyf/upstreamWaterBody> .

okns:hyf_usage a linkml:SlotDefinition ;
    skos:definition "expresses the kind of name usage in a specific community, using a term from the HY_NameUsage code list, or a controlled vocabulary. Alternative code lists may be used but should be related to the terms in the HY_NameUsage codelist using an appropriate formalism." ;
    skos:editorialNote "No occurrences of this slot in the graph." ;
    skos:inScheme okns:hyf ;
    skos:mappingRelation <https://www.opengis.net/def/schema/hy_features/hyf/usage> ;
    linkml:definition_uri okns:hyf_usage ;
    linkml:inlined true ;
    linkml:range okns:HyfHYNameUsage ;
    linkml:slot_uri <https://www.opengis.net/def/schema/hy_features/hyf/usage> .

okns:hyf_variantSpelling a linkml:SlotDefinition ;
    skos:definition "indicates whether the name is a variant spelling or not using the Boolean value type." ;
    skos:editorialNote "No occurrences of this slot in the graph." ;
    skos:inScheme okns:hyf ;
    skos:mappingRelation <https://www.opengis.net/def/schema/hy_features/hyf/variantSpelling> ;
    linkml:definition_uri okns:hyf_variantSpelling ;
    linkml:range okns:boolean ;
    linkml:slot_uri <https://www.opengis.net/def/schema/hy_features/hyf/variantSpelling> .

okns:hyf_watercourse a linkml:SlotDefinition ;
    skos:definition "identifies the natural or man-made channel which continuously or periodically contains moving water, including large interstices in the ground, such as cave, cavern or a group of these." ;
    skos:editorialNote "No occurrences of this slot in the graph." ;
    skos:inScheme okns:hyf ;
    skos:mappingRelation <https://www.opengis.net/def/schema/hy_features/hyf/watercourse> ;
    linkml:definition_uri okns:hyf_watercourse ;
    linkml:inlined true ;
    linkml:range okns:Any ;
    linkml:slot_uri <https://www.opengis.net/def/schema/hy_features/hyf/watercourse> .

okns:hyf_waterpool a linkml:SlotDefinition ;
    skos:definition "identifies the natural or artificial depression which contains standing water, including large interstices in the ground, such as cave, cavern or a group of these." ;
    skos:editorialNote "No occurrences of this slot in the graph." ;
    skos:inScheme okns:hyf ;
    skos:mappingRelation <https://www.opengis.net/def/schema/hy_features/hyf/waterpool> ;
    linkml:definition_uri okns:hyf_waterpool ;
    linkml:inlined true ;
    linkml:range okns:Any ;
    linkml:slot_uri <https://www.opengis.net/def/schema/hy_features/hyf/waterpool> .

okns:normalizedstring a linkml:TypeDefinition ;
    skos:definition "Normalized string, one that does not contain the carriage return (#xD), line feed (#xA) nor tab (#x9) characters." ;
    skos:inScheme okns:extended_types ;
    skos:note "added by Mahir Morshed <mmorshed@scripps.edu>" ;
    linkml:base "str" ;
    linkml:definition_uri linkml:Normalizedstring ;
    linkml:typeof okns:string ;
    linkml:uri xsd:normalizedString .

okns:positiveinteger a linkml:TypeDefinition ;
    skos:definition "An integer that is positive" ;
    skos:inScheme okns:extended_types ;
    skos:note "added by Mahir Morshed <mmorshed@scripps.edu>" ;
    linkml:base "int" ;
    linkml:definition_uri linkml:Positiveinteger ;
    linkml:minimum_value "1"^^<https://purl.org/okn/schema/@id> ;
    linkml:typeof okns:integer ;
    linkml:uri xsd:positiveInteger .

okns:seegrid_basic_measure a linkml:SlotDefinition ;
    dcterms:source <http://def.seegrid.csiro.au/isotc211/iso19103/2005/basic> ;
    dcterms:title "measure" ;
    skos:definition "The value of this property is a scaled number" ;
    skos:editorialNote "No occurrences of this slot in the graph." ;
    skos:inScheme okns:seegrid-iso19115 ;
    skos:mappingRelation seegrid-basic:measure ;
    linkml:definition_uri okns:seegrid_basic_measure ;
    linkml:inlined true ;
    linkml:range okns:Seegrid-basicMeasure ;
    linkml:slot_uri seegrid-basic:measure .

okns:seegrid_basic_uom a linkml:SlotDefinition ;
    dcterms:source <http://def.seegrid.csiro.au/isotc211/iso19103/2005/basic> ;
    dcterms:title "unit of measure" ;
    skos:definition "The value of this property designates the units of measure or scale for the quantity" ;
    skos:editorialNote "No occurrences of this slot in the graph." ;
    skos:inScheme okns:seegrid-iso19115 ;
    skos:mappingRelation seegrid-basic:uom ;
    linkml:definition_uri okns:seegrid_basic_uom ;
    linkml:inlined true ;
    linkml:range okns:Seegrid-basicUnitOfMeasure ;
    linkml:slot_uri seegrid-basic:uom .

okns:seegrid_basic_value a linkml:SlotDefinition ;
    rdfs:subPropertyOf okns:rdf_value ;
    skos:editorialNote "No occurrences of this slot in the graph." ;
    skos:inScheme okns:seegrid-iso19115 ;
    skos:mappingRelation seegrid-basic:value ;
    linkml:definition_uri okns:seegrid_basic_value ;
    linkml:inlined true ;
    linkml:range okns:Any ;
    linkml:slot_uri seegrid-basic:value .

okns:seegrid_ci_name a linkml:SlotDefinition ;
    dcterms:source <http://def.seegrid.csiro.au/isotc211/iso19115/2003/citation> ;
    dcterms:title "name" ;
    skos:editorialNote "No occurrences of this slot in the graph." ;
    skos:inScheme okns:seegrid-iso19115 ;
    skos:mappingRelation seegrid-ci:name ;
    linkml:definition_uri okns:seegrid_ci_name ;
    linkml:range okns:string ;
    linkml:slot_uri seegrid-ci:name .

okns:skos_altLabel a linkml:SlotDefinition ;
    dcterms:source <http://www.w3.org/2004/02/skos/core> ;
    dcterms:title "alternative label" ;
    rdfs:subPropertyOf okns:rdfs_label ;
    skos:definition "An alternative lexical label for a resource." ;
    skos:editorialNote "No occurrences of this slot in the graph." ;
    skos:inScheme okns:skos ;
    skos:mappingRelation skos:altLabel ;
    skos:note "description: The range of skos:altLabel is the class of RDF plain literals.",
        "description: skos:prefLabel, skos:altLabel and skos:hiddenLabel are pairwise disjoint properties." ;
    linkml:definition_uri okns:skos_altLabel ;
    linkml:inlined true ;
    linkml:range okns:Any ;
    linkml:slot_uri skos:altLabel .

okns:skos_changeNote a linkml:SlotDefinition ;
    dcterms:source <http://www.w3.org/2004/02/skos/core> ;
    dcterms:title "change note" ;
    rdfs:subPropertyOf okns:skos_note ;
    skos:definition "A note about a modification to a concept." ;
    skos:editorialNote "No occurrences of this slot in the graph." ;
    skos:inScheme okns:skos ;
    skos:mappingRelation skos:changeNote ;
    linkml:definition_uri okns:skos_changeNote ;
    linkml:inlined true ;
    linkml:range okns:Any ;
    linkml:slot_uri skos:changeNote .

okns:skos_definition a linkml:SlotDefinition ;
    dcterms:source <http://www.w3.org/2004/02/skos/core> ;
    dcterms:title "definition" ;
    rdfs:subPropertyOf okns:skos_note ;
    skos:definition "A statement or formal explanation of the meaning of a concept." ;
    skos:editorialNote "No occurrences of this slot in the graph." ;
    skos:inScheme okns:skos ;
    skos:mappingRelation skos:definition ;
    linkml:definition_uri okns:skos_definition ;
    linkml:inlined true ;
    linkml:range okns:Any ;
    linkml:slot_uri skos:definition .

okns:skos_defnition a linkml:SlotDefinition ;
    skos:inScheme okns:sc ;
    skos:mappingRelation skos:defnition ;
    linkml:definition_uri okns:skos_defnition ;
    linkml:range okns:string ;
    linkml:slot_uri skos:defnition .

okns:skos_editorialNote a linkml:SlotDefinition ;
    dcterms:source <http://www.w3.org/2004/02/skos/core> ;
    dcterms:title "editorial note" ;
    rdfs:subPropertyOf okns:skos_note ;
    skos:definition "A note for an editor, translator or maintainer of the vocabulary." ;
    skos:editorialNote "No occurrences of this slot in the graph." ;
    skos:inScheme okns:skos ;
    skos:mappingRelation skos:editorialNote ;
    linkml:definition_uri okns:skos_editorialNote ;
    linkml:inlined true ;
    linkml:range okns:Any ;
    linkml:slot_uri skos:editorialNote .

okns:skos_exactMatch a linkml:SlotDefinition ;
    dcterms:source <http://www.w3.org/2004/02/skos/core> ;
    dcterms:title "has exact match" ;
    rdfs:subPropertyOf okns:skos_closeMatch ;
    skos:definition "skos:exactMatch is used to link two concepts, indicating a high degree of confidence that the concepts can be used interchangeably across a wide range of information retrieval applications. skos:exactMatch is a transitive property, and is a sub-property of skos:closeMatch." ;
    skos:editorialNote "No occurrences of this slot in the graph." ;
    skos:inScheme okns:skos ;
    skos:mappingRelation skos:exactMatch ;
    skos:note "description: skos:exactMatch is disjoint with each of the properties skos:broadMatch and skos:relatedMatch." ;
    linkml:definition_uri okns:skos_exactMatch ;
    linkml:inlined true ;
    linkml:range okns:Any ;
    linkml:slot_uri skos:exactMatch .

okns:skos_example a linkml:SlotDefinition ;
    dcterms:source <http://www.w3.org/2004/02/skos/core> ;
    dcterms:title "example" ;
    rdfs:subPropertyOf okns:skos_note ;
    skos:definition "An example of the use of a concept." ;
    skos:editorialNote "No occurrences of this slot in the graph." ;
    skos:inScheme okns:skos ;
    skos:mappingRelation skos:example ;
    linkml:definition_uri okns:skos_example ;
    linkml:inlined true ;
    linkml:range okns:Any ;
    linkml:slot_uri skos:example .

okns:skos_hiddenLabel a linkml:SlotDefinition ;
    dcterms:source <http://www.w3.org/2004/02/skos/core> ;
    dcterms:title "hidden label" ;
    rdfs:subPropertyOf okns:rdfs_label ;
    skos:definition "A lexical label for a resource that should be hidden when generating visual displays of the resource, but should still be accessible to free text search operations." ;
    skos:editorialNote "No occurrences of this slot in the graph." ;
    skos:inScheme okns:skos ;
    skos:mappingRelation skos:hiddenLabel ;
    skos:note "description: The range of skos:hiddenLabel is the class of RDF plain literals.",
        "description: skos:prefLabel, skos:altLabel and skos:hiddenLabel are pairwise disjoint properties." ;
    linkml:definition_uri okns:skos_hiddenLabel ;
    linkml:inlined true ;
    linkml:range okns:Any ;
    linkml:slot_uri skos:hiddenLabel .

okns:skos_historyNote a linkml:SlotDefinition ;
    dcterms:source <http://www.w3.org/2004/02/skos/core> ;
    dcterms:title "history note" ;
    rdfs:subPropertyOf okns:skos_note ;
    skos:definition "A note about the past state/use/meaning of a concept." ;
    skos:editorialNote "No occurrences of this slot in the graph." ;
    skos:inScheme okns:skos ;
    skos:mappingRelation skos:historyNote ;
    linkml:definition_uri okns:skos_historyNote ;
    linkml:inlined true ;
    linkml:range okns:Any ;
    linkml:slot_uri skos:historyNote .

okns:skos_notation a linkml:SlotDefinition ;
    dcterms:source <http://www.w3.org/2004/02/skos/core> ;
    dcterms:title "notation" ;
    skos:definition "A notation, also known as classification code, is a string of characters such as \"T58.5\" or \"303.4833\" used to uniquely identify a concept within the scope of a given concept scheme." ;
    skos:editorialNote "By convention, skos:notation is used with a typed literal in the object position of the triple.",
        "No occurrences of this slot in the graph." ;
    skos:inScheme okns:skos ;
    skos:mappingRelation skos:notation ;
    linkml:definition_uri okns:skos_notation ;
    linkml:inlined true ;
    linkml:range okns:Any ;
    linkml:slot_uri skos:notation .

okns:skos_prefLabel a linkml:SlotDefinition ;
    dcterms:source <http://www.w3.org/2004/02/skos/core> ;
    dcterms:title "preferred label" ;
    rdfs:subPropertyOf okns:rdfs_label ;
    skos:definition "The preferred lexical label for a resource, in a given language." ;
    skos:editorialNote "No occurrences of this slot in the graph." ;
    skos:inScheme okns:skos ;
    skos:mappingRelation skos:prefLabel ;
    skos:note "description: A resource has no more than one value of skos:prefLabel per language tag, and no more than one value of skos:prefLabel without language tag.",
        "description: The range of skos:prefLabel is the class of RDF plain literals.",
        """description: skos:prefLabel, skos:altLabel and skos:hiddenLabel are pairwise
      disjoint properties.""" ;
    linkml:definition_uri okns:skos_prefLabel ;
    linkml:inlined true ;
    linkml:range okns:Any ;
    linkml:slot_uri skos:prefLabel .

okns:skos_relatedMatch a linkml:SlotDefinition ;
    dcterms:source <http://www.w3.org/2004/02/skos/core> ;
    dcterms:title "has related match" ;
    rdfs:subPropertyOf okns:skos_related ;
    skos:definition "skos:relatedMatch is used to state an associative mapping link between two conceptual resources in different concept schemes." ;
    skos:editorialNote "No occurrences of this slot in the graph." ;
    skos:inScheme okns:skos ;
    skos:mappingRelation skos:relatedMatch ;
    linkml:definition_uri okns:skos_relatedMatch ;
    linkml:inlined true ;
    linkml:range okns:Any ;
    linkml:slot_uri skos:relatedMatch .

okns:skos_scopeNote a linkml:SlotDefinition ;
    dcterms:source <http://www.w3.org/2004/02/skos/core> ;
    dcterms:title "scope note" ;
    rdfs:subPropertyOf okns:skos_note ;
    skos:definition "A note that helps to clarify the meaning and/or the use of a concept." ;
    skos:editorialNote "No occurrences of this slot in the graph." ;
    skos:inScheme okns:skos ;
    skos:mappingRelation skos:scopeNote ;
    linkml:definition_uri okns:skos_scopeNote ;
    linkml:inlined true ;
    linkml:range okns:Any ;
    linkml:slot_uri skos:scopeNote .

okns:DctRightsStatement a linkml:ClassDefinition ;
    dcterms:source dcterms: ;
    dcterms:title "Rights Statement" ;
    skos:definition "A statement about the intellectual property rights (IPR) held in or over a resource, a legal document giving official permission to do something with a resource, or a statement about access rights." ;
    skos:inScheme okns:dc ;
    skos:mappingRelation dcterms:RightsStatement ;
    linkml:class_uri dcterms:RightsStatement ;
    linkml:definition_uri okns:DctRightsStatement ;
    linkml:slot_usage [ ] .

okns:HyfHYCatchmentArea a linkml:ClassDefinition ;
    skos:definition "The HY_CatchmentArea feature type realizes a catchment specifically as a catchment area connecting the inflow and outflow of the catchment it realizes.␊␊HY_CatchmentArea specializes HY_CatchmentRealization with respect to an implied areal geometric representation. Topologically, the catchment area connecting the inflow and outflow of the catchment is a face bounded inwards by an inflow edge and outwards by an outflow edge. Hydrologically, catchment area refers to the area having a common outlet for its runoff.␊␊Through generalization, HY_CatchmentArea inherits the shape and the realizedCatchment properties. The optional shape of the catchment may be implemented as a surface." ;
    skos:inScheme okns:hyf ;
    skos:mappingRelation <hyf:HY_CatchmentArea> ;
    skos:note "description: The HY_CatchmentArea feature type realizes a catchment specifically as a catchment area connecting the inflow and outflow of the catchment it realizes.  HY_CatchmentArea specializes HY_CatchmentRealization with respect to an implied areal geometric representation. Topologically, the catchment area connecting the inflow and outflow of the catchment is a face bounded inwards by an inflow edge and outwards by an outflow edge. Hydrologically, catchment area refers to the area having a common outlet for its runoff.  Through generalization, HY_CatchmentArea inherits the shape and the realizedCatchment properties. The optional shape of the catchment may be implemented as a surface." ;
    linkml:class_uri <https://www.opengis.net/def/schema/hy_features/hyf/HY_CatchmentArea> ;
    linkml:definition_uri okns:HyfHYCatchmentArea ;
    linkml:is_a okns:HyfHYCatchmentRealization ;
    linkml:slot_usage [ ] .

okns:HyfHYCatchmentDivide a linkml:ClassDefinition ;
    skos:definition "The HY_CatchmentDivide feature type realizes a catchment specifically as catchment boundary connecting the inflow and outflow of the catchment it realizes, whereby inflow and outflow may overlay.␊␊Implying a linear geometric representation, a catchment boundary is topologically understood as an edge bounded by inflow node and outflow nodes, and corresponding to left-bank and right-bank catchment faces inside of the boundary. Hydrologically, the boundary refers to the summit line separating adjacent catchments.␊␊Through generalization, HY_CatchmentDivide inherits the shape and the realizedCatchment properties. The shape of the catchment divide may be implemented as a composition of succeeding curves or a polygon ring." ;
    skos:inScheme okns:hyf ;
    skos:mappingRelation <hyf:HY_CatchmentDivide> ;
    skos:note "description: The HY_CatchmentDivide feature type realizes a catchment specifically as catchment boundary connecting the inflow and outflow of the catchment it realizes, whereby inflow and outflow may overlay. Implying a linear geometric representation, a catchment boundary is topologically understood as an edge bounded by inflow node and outflow nodes, and corresponding to left-bank and right-bank catchment faces inside of the boundary. Hydrologically, the boundary refers to the summit line separating adjacent catchments.  Through generalization, HY_CatchmentDivide inherits the shape and the realizedCatchment properties. The shape of the catchment divide may be implemented as a composition of succeeding curves or a polygon ring." ;
    linkml:class_uri <https://www.opengis.net/def/schema/hy_features/hyf/HY_CatchmentDivide> ;
    linkml:definition_uri okns:HyfHYCatchmentDivide ;
    linkml:is_a okns:HyfHYCatchmentRealization ;
    linkml:slot_usage [ ] .

okns:HyfHYDendriticCatchment a linkml:ClassDefinition ;
    skos:definition "The HY_DendriticCatchment feature type (Figure 31) specializes the general HY_Catchment class as a catchment which is determined by a single common downstream catchment. It represents the catchment as the topological link between an inflow and an outflow. This allows catchments to be connected in a dendritic network by upstream-downstream relationships without knowing the complex hydrology between inflow and outflow. This concept requires a stable identifier purposefully assigned to the catchment and that catchments are delineated as a simple tree hierarchy.␊␊HY_DendriticCatchment inherits from generalization the code, outflow, inflow, containingCatchment, containedCatchment, conjointCatchment, upperCatchment, lowerCatchment, and catchmentRealization properties, and has an encompassingCatchment association. The dendritic nature of this feature is enforced through single-outflow, single-receiving-catchment and single-lower-catchment constraints." ;
    skos:inScheme okns:hyf ;
    skos:mappingRelation <hyf:HY_DendriticCatchment> ;
    skos:note "description: The HY_DendriticCatchment feature type (Figure 31) specializes the general HY_Catchment class as a catchment which is determined by a single common downstream catchment. It represents the catchment as the topological link between an inflow and an outflow. This allows catchments to be connected in a dendritic network by upstream-downstream relationships without knowing the complex hydrology between inflow and outflow. This concept requires a stable identifier purposefully assigned to the catchment and that catchments are delineated as a simple tree hierarchy.  HY_DendriticCatchment inherits from generalization the code, outflow, inflow, containingCatchment, containedCatchment, conjointCatchment, upperCatchment, lowerCatchment, and catchmentRealization properties, and has an encompassingCatchment association. The dendritic nature of this feature is enforced through single-outflow, single-receiving-catchment and single-lower-catchment constraints." ;
    linkml:class_uri <https://www.opengis.net/def/schema/hy_features/hyf/HY_DendriticCatchment> ;
    linkml:definition_uri okns:HyfHYDendriticCatchment ;
    linkml:is_a okns:HyfHYCatchment ;
    linkml:slot_usage [ ] .

okns:HyfHYDepression a linkml:ClassDefinition ;
    dcterms:title "No class (entity type) name specified -- this class is noted as a superclass of another class in this graph but has not itself been defined." ;
    skos:definition "The HY_Depression feature type specializes the general HY_HydroFeature class. It describes land lower than the surrounding land as a container for standing water. A depression is part of the network of channels and depressions forming the connecting system in which waterbodies are contained as parts of hydrographic network.␊␊Through generalization, HY_Depression inherits the name property. It has associations for the surfaceNetwork in which it participates, a body of standingWater and a stratum of a confinedWaterBody. An outlet-at-benchmark constraint emphasizes that a benchmark on the confined waterbody at the outlet of the catchment that is realized by the channel network." ;
    skos:inScheme okns:hyf ;
    skos:mappingRelation <hyf:HY_Depression> ;
    linkml:class_uri <https://www.opengis.net/def/schema/hy_features/hyf/HY_Depression> ;
    linkml:definition_uri okns:HyfHYDepression ;
    linkml:slot_usage [ ] .

okns:HyfHYDistanceDescription a linkml:ClassDefinition ;
    skos:definition "list of general terms commonly used in hydrology to describe a spatial relationship between two locations. If required, an implementation should use terms from this code list, defined specifically to conform to a terminology common in the hydrology domain. Note that alternative code lists may be used but should be related to the terms in but should be related to the terms in this code list using an appropriate formalism." ;
    skos:inScheme okns:hyf ;
    skos:mappingRelation <hyf:HY_DistanceDescription> ;
    linkml:class_uri <https://www.opengis.net/def/schema/hy_features/hyf/HY_DistanceDescription> ;
    linkml:definition_uri okns:HyfHYDistanceDescription ;
    linkml:is_a okns:SkosConcept ;
    linkml:slot_usage [ ] .

okns:HyfHYDistanceFromReferent a linkml:ClassDefinition ;
    skos:definition "The HY_DistanceFromReferent data type provides the distance from a located referent as an absolute or interpolative value, including simple statements on accuracy and precision of the measured position." ;
    skos:inScheme okns:hyf ;
    skos:mappingRelation <hyf:HY_DistanceFromReferent> ;
    linkml:class_uri <https://www.opengis.net/def/schema/hy_features/hyf/HY_DistanceFromReferent> ;
    linkml:definition_uri okns:HyfHYDistanceFromReferent ;
    linkml:slot_usage [ ] .

okns:HyfHYHydroLocationType a linkml:ClassDefinition ;
    skos:definition "terms identifying a Hydro Location determined to realize the conceptual nexus. If required, an implementation should use terms from this code list, defined specifically to conform to a terminology common in the hydrology domain. Note that alternative code lists may be used but should be related to the terms in but should be related to the terms in this code list using an appropriate formalism." ;
    skos:inScheme okns:hyf ;
    skos:mappingRelation <hyf:HY_HydroLocationType> ;
    linkml:class_uri <https://www.opengis.net/def/schema/hy_features/hyf/HY_HydroLocationType> ;
    linkml:definition_uri okns:HyfHYHydroLocationType ;
    linkml:is_a okns:SkosConcept ;
    linkml:slot_usage [ ] .

okns:HyfHYIndirectPosition a linkml:ClassDefinition ;
    skos:definition "The HY_IndirectPosition feature type defines the location referenced along an axis, without the necessity of a geometric realization. Indirect position uses a catchment-specific reference system which defines the flowpath as the required linear element along which the position is determined. The indirect position is then expressed as the distance from the upstream and/or downstream end of the flowpath, or from a referent that is already located on that flowpath.␊␊The (indirect) position of an outflow node referenced along an upstream oriented flowpath can be expressed as the distance from an upstream inflow node located on that flowpath, while the (indirect) position of an inflow node referenced along a downstream oriented flowpath can be expressed as distance from a downstream outflow node located on the flowpath. An ‘intermediate’ position referencing known inflow and outflow nodes bounding a flowpath at both ends can be expressed as part of the distance along the entire flowpath, measured from the upstream end of an upstream flowpath, and/or from the downstream end of a downstream flowpath. A position referencing an already referenced location on the flowpath can be expressed as part of the distance along the entire flowpath, measured from the ‘located referent’.␊␊HY_IndirectPosition carries the distanceExpression, and distanceDescription attributes, and has linearElement, locatedReferent and a referenceLocation associations. A point-referent constraint emphasizes the topological relationship between the linear element and point representation of the reference location; a measure-along-flowpath constraint defines the flowpath as the linear element to be used whenever a position is expressed as a distance from a referent." ;
    skos:inScheme okns:hyf ;
    skos:mappingRelation <hyf:HY_IndirectPosition> ;
    skos:note "description: The HY_IndirectPosition feature type defines the location referenced along an axis, without the necessity of a geometric realization. Indirect position uses a catchment-specific reference system which defines the flowpath as the required linear element along which the position is determined. The indirect position is then expressed as the distance from the upstream and/or downstream end of the flowpath, or from a referent that is already located on that flowpath.  The (indirect) position of an outflow node referenced along an upstream oriented flowpath can be expressed as the distance from an upstream inflow node located on that flowpath, while the (indirect) position of an inflow node referenced along a downstream oriented flowpath can be expressed as distance from a downstream outflow node located on the flowpath. An ‘intermediate’ position referencing known inflow and outflow nodes bounding a flowpath at both ends can be expressed as part of the distance along the entire flowpath, measured from the upstream end of an upstream flowpath, and/or from the downstream end of a downstream flowpath. A position referencing an already referenced location on the flowpath can be expressed as part of the distance along the entire flowpath, measured from the ‘located referent’.   HY_IndirectPosition carries the distanceExpression, and distanceDescription attributes, and has linearElement, locatedReferent and a referenceLocation associations. A point-referent constraint emphasizes the topological relationship between the linear element and point representation of the reference location; a measure-along-flowpath constraint defines the flowpath as the linear element to be used whenever a position is expressed as a distance from a referent." ;
    linkml:class_uri <https://www.opengis.net/def/schema/hy_features/hyf/HY_IndirectPosition> ;
    linkml:definition_uri okns:HyfHYIndirectPosition ;
    linkml:slot_usage [ ] .

okns:HyfHYInteriorCatchment a linkml:ClassDefinition ;
    skos:definition "The HY_InteriorCatchment feature type (Figure 32) specializes the general HY_Catchment class as a catchment which is generally not connected to other catchments. This class describes the interior catchment as a catchment enveloped by other catchments to which it may temporarily contribute. While the interior catchment concept precludes flow to neighboring surface catchments, holistically it is a candidate for establishing connections to groundwater or atmospheric systems." ;
    skos:inScheme okns:hyf ;
    skos:mappingRelation <hyf:HY_InteriorCatchment> ;
    linkml:class_uri <https://www.opengis.net/def/schema/hy_features/hyf/HY_InteriorCatchment> ;
    linkml:definition_uri okns:HyfHYInteriorCatchment ;
    linkml:is_a okns:HyfHYCatchment ;
    linkml:slot_usage [ ] .

okns:HyfHYNameUsage a linkml:ClassDefinition ;
    skos:definition "terms used to indicate the type of name usage. If required, an implementation should use terms from this code list, defined specifically to conform to a terminology common in the hydrology domain. Note that alternative code lists may be used but should be related to the terms in but should be related to the terms in this code list using an appropriate formalism." ;
    skos:inScheme okns:hyf ;
    skos:mappingRelation <hyf:HY_NameUsage> ;
    linkml:class_uri <https://www.opengis.net/def/schema/hy_features/hyf/HY_NameUsage> ;
    linkml:definition_uri okns:HyfHYNameUsage ;
    linkml:is_a okns:SkosConcept ;
    linkml:slot_usage [ ] .

okns:OwlAllDifferent a linkml:ClassDefinition ;
    dcterms:source owl: ;
    dcterms:title "AllDifferent" ;
    skos:definition "The class of collections of pairwise different individuals." ;
    skos:inScheme okns:owl-rdf-rdfs ;
    skos:mappingRelation owl:AllDifferent ;
    linkml:class_uri owl:AllDifferent ;
    linkml:definition_uri okns:OwlAllDifferent ;
    linkml:is_a okns:RdfsResource ;
    linkml:slot_usage [ ] .

okns:Seegrid-basicLength a linkml:ClassDefinition ;
    dcterms:source <http://def.seegrid.csiro.au/isotc211/iso19103/2005/basic> ;
    dcterms:title "Length" ;
    skos:definition "Measure of 1-D extent" ;
    skos:inScheme okns:seegrid-iso19115 ;
    skos:mappingRelation seegrid-basic:Length ;
    linkml:class_uri seegrid-basic:Length ;
    linkml:definition_uri okns:Seegrid-basicLength ;
    linkml:is_a okns:Seegrid-basicMeasure ;
    linkml:slot_usage [ ] .

okns:Seegrid-basicUnitOfMeasure a linkml:ClassDefinition ;
    dcterms:source <http://def.seegrid.csiro.au/isotc211/iso19103/2005/basic> ;
    dcterms:title "Unit of measure" ;
    skos:definition "Scale for a number describing size or extent" ;
    skos:inScheme okns:seegrid-iso19115 ;
    skos:mappingRelation seegrid-basic:UnitOfMeasure ;
    linkml:class_uri seegrid-basic:UnitOfMeasure ;
    linkml:definition_uri okns:Seegrid-basicUnitOfMeasure ;
    linkml:slot_usage [ ] .

okns:Seegrid-ciDateTypeCode a linkml:ClassDefinition ;
    dcterms:source <http://def.seegrid.csiro.au/isotc211/iso19115/2003/citation> ;
    dcterms:title "Date type code" ;
    skos:altLabel "CI_DateTypeCode" ;
    skos:inScheme okns:seegrid-iso19115 ;
    skos:mappingRelation seegrid-ci:DateTypeCode ;
    linkml:class_uri seegrid-ci:DateTypeCode ;
    linkml:definition_uri okns:Seegrid-ciDateTypeCode ;
    linkml:is_a okns:SkosConcept ;
    linkml:slot_usage [ ] .

okns:Seegrid-ciOnLineFunctionCode a linkml:ClassDefinition ;
    dcterms:source <http://def.seegrid.csiro.au/isotc211/iso19115/2003/citation> ;
    dcterms:title "On line function code" ;
    skos:altLabel "CI_OnLineFunctionCode" ;
    skos:inScheme okns:seegrid-iso19115 ;
    skos:mappingRelation seegrid-ci:OnLineFunctionCode ;
    linkml:class_uri seegrid-ci:OnLineFunctionCode ;
    linkml:definition_uri okns:Seegrid-ciOnLineFunctionCode ;
    linkml:is_a okns:SkosConcept ;
    linkml:slot_usage [ ] .

okns:Seegrid-ciPresentationFormCode a linkml:ClassDefinition ;
    dcterms:source <http://def.seegrid.csiro.au/isotc211/iso19115/2003/citation> ;
    dcterms:title "Presentation form code" ;
    skos:altLabel "CI_PresentationFormCode" ;
    skos:inScheme okns:seegrid-iso19115 ;
    skos:mappingRelation seegrid-ci:PresentationFormCode ;
    linkml:class_uri seegrid-ci:PresentationFormCode ;
    linkml:definition_uri okns:Seegrid-ciPresentationFormCode ;
    linkml:is_a okns:SkosConcept ;
    linkml:slot_usage [ ] .

okns:Seegrid-ciRoleCode a linkml:ClassDefinition ;
    dcterms:source <http://def.seegrid.csiro.au/isotc211/iso19115/2003/citation> ;
    dcterms:title "Role code" ;
    skos:altLabel "CI_RoleCode" ;
    skos:inScheme okns:seegrid-iso19115 ;
    skos:mappingRelation seegrid-ci:RoleCode ;
    linkml:class_uri seegrid-ci:RoleCode ;
    linkml:definition_uri okns:Seegrid-ciRoleCode ;
    linkml:is_a okns:SkosConcept ;
    linkml:slot_usage [ ] .

okns:SkosOrderedCollection a linkml:ClassDefinition ;
    dcterms:source <http://www.w3.org/2004/02/skos/core> ;
    dcterms:title "Ordered Collection" ;
    skos:definition "An ordered collection of concepts, where both the grouping and the ordering are meaningful." ;
    skos:editorialNote "Ordered collections can be used where you would like a set of concepts to be displayed in a specific order, and optionally under a 'node label'." ;
    skos:inScheme okns:skos ;
    skos:mappingRelation skos:OrderedCollection ;
    linkml:class_uri skos:OrderedCollection ;
    linkml:definition_uri okns:SkosOrderedCollection ;
    linkml:is_a okns:SkosCollection ;
    linkml:slot_usage [ ] .

okns:dc_contributor a linkml:SlotDefinition ;
    dcterms:source dc: ;
    dcterms:title "Contributor" ;
    skos:definition "The guidelines for using names of persons or organizations as creators also apply to contributors.  Typically, the name of a Contributor should be used to indicate the entity." ;
    skos:editorialNote "A [second property](/specifications/dublin-core/dcmi-terms/#http://purl.org/dc/terms/contributor) with the same name as this property has been declared in the [dcterms: namespace](http://purl.org/dc/terms/).  See the Introduction to the document [DCMI Metadata Terms](/specifications/dublin-core/dcmi-terms/) for an explanation.",
        "No occurrences of this slot in the graph." ;
    skos:inScheme okns:dc ;
    skos:mappingRelation dc:contributor ;
    skos:note "description: An entity responsible for making contributions to the resource." ;
    linkml:definition_uri okns:dc_contributor ;
    linkml:inlined true ;
    linkml:range okns:Any ;
    linkml:slot_uri dc:contributor .

okns:dc_coverage a linkml:SlotDefinition ;
    dcterms:source dc: ;
    dcterms:title "Coverage" ;
    skos:definition "Spatial topic and spatial applicability may be a named place or a location specified by its geographic coordinates. Temporal topic may be a named period, date, or date range. A jurisdiction may be a named administrative entity or a geographic place to which the resource applies. Recommended practice is to use a controlled vocabulary such as the Getty Thesaurus of Geographic Names [[TGN](https://www.getty.edu/research/tools/vocabulary/tgn/index.html)]. Where appropriate, named places or time periods may be used in preference to numeric identifiers such as sets of coordinates or date ranges." ;
    skos:editorialNote "A [second property](/specifications/dublin-core/dcmi-terms/#http://purl.org/dc/terms/coverage) with the same name as this property has been declared in the [dcterms: namespace](http://purl.org/dc/terms/).  See the Introduction to the document [DCMI Metadata Terms](/specifications/dublin-core/dcmi-terms/) for an explanation.",
        "No occurrences of this slot in the graph." ;
    skos:inScheme okns:dc ;
    skos:mappingRelation dc:coverage ;
    skos:note "description: The spatial or temporal topic of the resource, spatial applicability of the resource, or jurisdiction under which the resource is relevant." ;
    linkml:definition_uri okns:dc_coverage ;
    linkml:inlined true ;
    linkml:range okns:Any ;
    linkml:slot_uri dc:coverage .

okns:dc_date a linkml:SlotDefinition ;
    dcterms:source dc: ;
    dcterms:title "Date" ;
    skos:definition "Date may be used to express temporal information at any level of granularity.  Recommended practice is to express the date, date/time, or period of time according to ISO 8601-1 [[ISO 8601-1](https://www.iso.org/iso-8601-date-and-time-format.html)] or a published profile of the ISO standard, such as the W3C Note on Date and Time Formats [[W3CDTF](https://www.w3.org/TR/NOTE-datetime)] or the Extended Date/Time Format Specification [[EDTF](http://www.loc.gov/standards/datetime/)].  If the full date is unknown, month and year (YYYY-MM) or just year (YYYY) may be used. Date ranges may be specified using ISO 8601 period of time specification in which start and end dates are separated by a '/' (slash) character.  Either the start or end date may be missing." ;
    skos:editorialNote "A [second property](/specifications/dublin-core/dcmi-terms/#http://purl.org/dc/terms/date) with the same name as this property has been declared in the [dcterms: namespace](http://purl.org/dc/terms/).  See the Introduction to the document [DCMI Metadata Terms](/specifications/dublin-core/dcmi-terms/) for an explanation.",
        "No occurrences of this slot in the graph." ;
    skos:inScheme okns:dc ;
    skos:mappingRelation dc:date ;
    skos:note "description: A point or period of time associated with an event in the lifecycle of the resource." ;
    linkml:definition_uri okns:dc_date ;
    linkml:inlined true ;
    linkml:range okns:Any ;
    linkml:slot_uri dc:date .

okns:dc_description a linkml:SlotDefinition ;
    dcterms:source dc: ;
    dcterms:title "Description" ;
    skos:definition "Description may include but is not limited to: an abstract, a table of contents, a graphical representation, or a free-text account of the resource." ;
    skos:editorialNote "A [second property](/specifications/dublin-core/dcmi-terms/#http://purl.org/dc/terms/description) with the same name as this property has been declared in the [dcterms: namespace](http://purl.org/dc/terms/).  See the Introduction to the document [DCMI Metadata Terms](/specifications/dublin-core/dcmi-terms/) for an explanation.",
        "No occurrences of this slot in the graph." ;
    skos:inScheme okns:dc ;
    skos:mappingRelation dc:description ;
    skos:note "description: An account of the resource." ;
    linkml:definition_uri okns:dc_description ;
    linkml:inlined true ;
    linkml:range okns:Any ;
    linkml:slot_uri dc:description .

okns:dc_format a linkml:SlotDefinition ;
    dcterms:source dc: ;
    dcterms:title "Format" ;
    skos:definition "Recommended practice is to use a controlled vocabulary where available. For example, for file formats one could use the list of Internet Media Types [[MIME](https://www.iana.org/assignments/media-types/media-types.xhtml)]." ;
    skos:editorialNote "A [second property](/specifications/dublin-core/dcmi-terms/#http://purl.org/dc/terms/format) with the same name as this property has been declared in the [dcterms: namespace](http://purl.org/dc/terms/).  See the Introduction to the document [DCMI Metadata Terms](/specifications/dublin-core/dcmi-terms/) for an explanation.",
        "No occurrences of this slot in the graph." ;
    skos:inScheme okns:dc ;
    skos:mappingRelation dc:format ;
    skos:note "description: The file format, physical medium, or dimensions of the resource." ;
    linkml:definition_uri okns:dc_format ;
    linkml:inlined true ;
    linkml:range okns:Any ;
    linkml:slot_uri dc:format .

okns:dc_identifier a linkml:SlotDefinition ;
    dcterms:source dc: ;
    dcterms:title "Identifier" ;
    skos:definition "Recommended practice is to identify the resource by means of a string conforming to an identification system." ;
    skos:editorialNote "A [second property](/specifications/dublin-core/dcmi-terms/#http://purl.org/dc/terms/identifier) with the same name as this property has been declared in the [dcterms: namespace](http://purl.org/dc/terms/).  See the Introduction to the document [DCMI Metadata Terms](/specifications/dublin-core/dcmi-terms/) for an explanation.",
        "No occurrences of this slot in the graph." ;
    skos:inScheme okns:dc ;
    skos:mappingRelation dc:identifier ;
    skos:note "description: An unambiguous reference to the resource within a given context." ;
    linkml:definition_uri okns:dc_identifier ;
    linkml:inlined true ;
    linkml:range okns:Any ;
    linkml:slot_uri dc:identifier .

okns:dc_language a linkml:SlotDefinition ;
    dcterms:source dc: ;
    dcterms:title "Language" ;
    skos:definition "Recommended practice is to use either a non-literal value representing a language from a controlled vocabulary such as ISO 639-2 or ISO 639-3, or a literal value consisting of an IETF Best Current Practice 47 [[IETF-BCP47](https://tools.ietf.org/html/bcp47)] language tag." ;
    skos:editorialNote "A [second property](/specifications/dublin-core/dcmi-terms/#http://purl.org/dc/terms/language) with the same name as this property has been declared in the [dcterms: namespace](http://purl.org/dc/terms/).  See the Introduction to the document [DCMI Metadata Terms](/specifications/dublin-core/dcmi-terms/) for an explanation.",
        "No occurrences of this slot in the graph." ;
    skos:inScheme okns:dc ;
    skos:mappingRelation dc:language ;
    skos:note "description: A language of the resource." ;
    linkml:definition_uri okns:dc_language ;
    linkml:inlined true ;
    linkml:range okns:Any ;
    linkml:slot_uri dc:language .

okns:dc_publisher a linkml:SlotDefinition ;
    dcterms:source dc: ;
    dcterms:title "Publisher" ;
    skos:definition "Examples of a Publisher include a person, an organization, or a service. Typically, the name of a Publisher should be used to indicate the entity." ;
    skos:editorialNote "A [second property](/specifications/dublin-core/dcmi-terms/#http://purl.org/dc/terms/publisher) with the same name as this property has been declared in the [dcterms: namespace](http://purl.org/dc/terms/).  See the Introduction to the document [DCMI Metadata Terms](/specifications/dublin-core/dcmi-terms/) for an explanation.",
        "No occurrences of this slot in the graph." ;
    skos:inScheme okns:dc ;
    skos:mappingRelation dc:publisher ;
    skos:note "description: An entity responsible for making the resource available." ;
    linkml:definition_uri okns:dc_publisher ;
    linkml:inlined true ;
    linkml:range okns:Any ;
    linkml:slot_uri dc:publisher .

okns:dc_relation a linkml:SlotDefinition ;
    dcterms:source dc: ;
    dcterms:title "Relation" ;
    skos:definition "Recommended practice is to identify the related resource by means of a URI. If this is not possible or feasible, a string conforming to a formal identification system may be provided." ;
    skos:editorialNote "A [second property](/specifications/dublin-core/dcmi-terms/#http://purl.org/dc/terms/relation) with the same name as this property has been declared in the [dcterms: namespace](http://purl.org/dc/terms/).  See the Introduction to the document [DCMI Metadata Terms](/specifications/dublin-core/dcmi-terms/) for an explanation.",
        "No occurrences of this slot in the graph." ;
    skos:inScheme okns:dc ;
    skos:mappingRelation dc:relation ;
    skos:note "description: A related resource." ;
    linkml:definition_uri okns:dc_relation ;
    linkml:inlined true ;
    linkml:range okns:Any ;
    linkml:slot_uri dc:relation .

okns:dc_rights a linkml:SlotDefinition ;
    dcterms:source dc: ;
    dcterms:title "Rights" ;
    skos:definition "Typically, rights information includes a statement about various property rights associated with the resource, including intellectual property rights." ;
    skos:editorialNote "A [second property](/specifications/dublin-core/dcmi-terms/#http://purl.org/dc/terms/rights) with the same name as this property has been declared in the [dcterms: namespace](http://purl.org/dc/terms/).  See the Introduction to the document [DCMI Metadata Terms](/specifications/dublin-core/dcmi-terms/) for an explanation.",
        "No occurrences of this slot in the graph." ;
    skos:inScheme okns:dc ;
    skos:mappingRelation dc:rights ;
    skos:note "description: Information about rights held in and over the resource." ;
    linkml:definition_uri okns:dc_rights ;
    linkml:inlined true ;
    linkml:range okns:Any ;
    linkml:slot_uri dc:rights .

okns:dc_subject a linkml:SlotDefinition ;
    dcterms:source dc: ;
    dcterms:title "Subject" ;
    skos:definition "Typically, the subject will be represented using keywords, key phrases, or classification codes.  Recommended best practice is to use a controlled vocabulary." ;
    skos:editorialNote "A [second property](/specifications/dublin-core/dcmi-terms/#http://purl.org/dc/terms/subject) with the same name as this property has been declared in the [dcterms: namespace](http://purl.org/dc/terms/).  See the Introduction to the document [DCMI Metadata Terms](/specifications/dublin-core/dcmi-terms/) for an explanation.",
        "No occurrences of this slot in the graph." ;
    skos:inScheme okns:dc ;
    skos:mappingRelation dc:subject ;
    skos:note "description: The topic of the resource." ;
    linkml:definition_uri okns:dc_subject ;
    linkml:inlined true ;
    linkml:range okns:Any ;
    linkml:slot_uri dc:subject .

okns:dc_title a linkml:SlotDefinition ;
    dcterms:source dc: ;
    dcterms:title "Title" ;
    skos:definition "A name given to the resource." ;
    skos:editorialNote "A [second property](/specifications/dublin-core/dcmi-terms/#http://purl.org/dc/terms/title) with the same name as this property has been declared in the [dcterms: namespace](http://purl.org/dc/terms/).  See the Introduction to the document [DCMI Metadata Terms](/specifications/dublin-core/dcmi-terms/) for an explanation.",
        "No occurrences of this slot in the graph." ;
    skos:inScheme okns:dc ;
    skos:mappingRelation dc:title ;
    linkml:definition_uri okns:dc_title ;
    linkml:inlined true ;
    linkml:range okns:Any ;
    linkml:slot_uri dc:title .

okns:dc_type a linkml:SlotDefinition ;
    dcterms:source dc: ;
    dcterms:title "Type" ;
    skos:definition "Recommended practice is to use a controlled vocabulary such as the DCMI Type Vocabulary [[DCMI-TYPE](http://dublincore.org/documents/dcmi-type-vocabulary/)]. To describe the file format, physical medium, or dimensions of the resource, use the Format element." ;
    skos:editorialNote "A [second property](/specifications/dublin-core/dcmi-terms/#http://purl.org/dc/terms/type) with the same name as this property has been declared in the [dcterms: namespace](http://purl.org/dc/terms/).  See the Introduction to the document [DCMI Metadata Terms](/specifications/dublin-core/dcmi-terms/) for an explanation.",
        "No occurrences of this slot in the graph." ;
    skos:inScheme okns:dc ;
    skos:mappingRelation dc:type ;
    skos:note "description: The nature or genre of the resource." ;
    linkml:definition_uri okns:dc_type ;
    linkml:inlined true ;
    linkml:range okns:Any ;
    linkml:slot_uri dc:type .

okns:dct_accrualMethod a linkml:SlotDefinition ;
    dcterms:source dcterms: ;
    dcterms:title "Accrual Method" ;
    skos:definition "Recommended practice is to use a value from the Collection Description Accrual Method Vocabulary [[DCMI-ACCRUALMETHOD](https://dublincore.org/groups/collections/accrual-method/)]." ;
    skos:editorialNote "No occurrences of this slot in the graph." ;
    skos:inScheme okns:dc ;
    skos:mappingRelation dcterms:accrualMethod ;
    skos:note "description: The method by which items are added to a collection." ;
    linkml:definition_uri okns:dct_accrualMethod ;
    linkml:domain okns:DcmitypeCollection ;
    linkml:inlined true ;
    linkml:owner okns:dct_accrualMethod ;
    linkml:range okns:Any ;
    linkml:slot_uri dcterms:accrualMethod .

okns:dct_accrualPeriodicity a linkml:SlotDefinition ;
    dcterms:source dcterms: ;
    dcterms:title "Accrual Periodicity" ;
    skos:definition "Recommended practice is to use a value from the Collection Description Frequency Vocabulary [[DCMI-COLLFREQ](https://dublincore.org/groups/collections/frequency/)]." ;
    skos:editorialNote "No occurrences of this slot in the graph." ;
    skos:inScheme okns:dc ;
    skos:mappingRelation dcterms:accrualPeriodicity ;
    skos:note "description: The frequency with which items are added to a collection." ;
    linkml:definition_uri okns:dct_accrualPeriodicity ;
    linkml:domain okns:DcmitypeCollection ;
    linkml:inlined true ;
    linkml:owner okns:dct_accrualPeriodicity ;
    linkml:range okns:Any ;
    linkml:slot_uri dcterms:accrualPeriodicity .

okns:dct_accrualPolicy a linkml:SlotDefinition ;
    dcterms:source dcterms: ;
    dcterms:title "Accrual Policy" ;
    skos:definition "Recommended practice is to use a value from the Collection Description Accrual Policy Vocabulary [[DCMI-ACCRUALPOLICY](https://dublincore.org/groups/collections/accrual-policy/)]." ;
    skos:editorialNote "No occurrences of this slot in the graph." ;
    skos:inScheme okns:dc ;
    skos:mappingRelation dcterms:accrualPolicy ;
    skos:note "description: The policy governing the addition of items to a collection." ;
    linkml:definition_uri okns:dct_accrualPolicy ;
    linkml:domain okns:DcmitypeCollection ;
    linkml:inlined true ;
    linkml:owner okns:dct_accrualPolicy ;
    linkml:range okns:Any ;
    linkml:slot_uri dcterms:accrualPolicy .

okns:dct_contributor a linkml:SlotDefinition ;
    dcterms:source dcterms: ;
    dcterms:title "Contributor" ;
    rdfs:subPropertyOf okns:dc_contributor ;
    skos:definition "The guidelines for using names of persons or organizations as creators apply to contributors." ;
    skos:editorialNote "No occurrences of this slot in the graph." ;
    skos:inScheme okns:dc ;
    skos:mappingRelation dcterms:contributor ;
    skos:note "description: An entity responsible for making contributions to the resource." ;
    linkml:definition_uri okns:dct_contributor ;
    linkml:inlined true ;
    linkml:range okns:Any ;
    linkml:slot_uri dcterms:contributor .

okns:dct_identifier a linkml:SlotDefinition ;
    dcterms:source dcterms: ;
    dcterms:title "Identifier" ;
    rdfs:subPropertyOf okns:dc_identifier ;
    skos:definition "Recommended practice is to identify the resource by means of a string conforming to an identification system. Examples include International Standard Book Number (ISBN), Digital Object Identifier (DOI), and Uniform Resource Name (URN).  Persistent identifiers should be provided as HTTP URIs." ;
    skos:editorialNote "No occurrences of this slot in the graph." ;
    skos:inScheme okns:dc ;
    skos:mappingRelation dcterms:identifier ;
    skos:note "description: An unambiguous reference to the resource within a given context." ;
    linkml:definition_uri okns:dct_identifier ;
    linkml:inlined true ;
    linkml:range okns:RdfsLiteral ;
    linkml:slot_uri dcterms:identifier .

okns:dct_title a linkml:SlotDefinition ;
    dcterms:source dcterms: ;
    dcterms:title "Title" ;
    rdfs:subPropertyOf okns:dc_title ;
    skos:definition "A name given to the resource." ;
    skos:inScheme okns:dc ;
    skos:mappingRelation dcterms:title ;
    linkml:any_of [ a okns:AnonymousSlotExpression ;
            linkml:range okns:RdfsLiteral ],
        [ a okns:AnonymousSlotExpression ;
            linkml:range okns:string ] ;
    linkml:definition_uri okns:dct_title ;
    linkml:inlined true ;
    linkml:range okns:Any ;
    linkml:slot_uri dcterms:title .

okns:decimal a linkml:TypeDefinition ;
    skos:broadMatch schema1:Number ;
    skos:definition "A real number with arbitrary precision that conforms to the xsd:decimal specification" ;
    skos:editorialNote "If you are authoring schemas in LinkML YAML, the type is referenced with the lower case \"decimal\"." ;
    skos:inScheme linkml:types ;
    linkml:base "Decimal" ;
    linkml:imported_from "linkml:types" ;
    linkml:definition_uri linkml:Decimal ;
    linkml:uri xsd:decimal .

okns:hyf_name a linkml:SlotDefinition ;
    skos:definition "name given to the hydrologic feature in cultural, political or historical context." ;
    skos:editorialNote "No occurrences of this slot in the graph." ;
    skos:inScheme okns:hyf ;
    skos:mappingRelation <https://www.opengis.net/def/schema/hy_features/hyf/name> ;
    linkml:definition_uri okns:hyf_name ;
    linkml:domain okns:HyfHYHydroFeature ;
    linkml:inlined true ;
    linkml:owner okns:hyf_name ;
    linkml:range okns:HyfHYHydroFeatureName ;
    linkml:slot_uri <https://www.opengis.net/def/schema/hy_features/hyf/name> .

okns:hyf_name_string a linkml:SlotDefinition ;
    skos:definition "indicates whether the name applies to a part of feature only or not, using the Boolean value type" ;
    skos:editorialNote "No occurrences of this slot in the graph." ;
    skos:inScheme okns:hyf ;
    skos:mappingRelation <https://www.opengis.net/def/schema/hy_features/hyf/name_string> ;
    linkml:definition_uri okns:hyf_name_string ;
    linkml:domain okns:HyfHYHydroFeatureName ;
    linkml:owner okns:hyf_name_string ;
    linkml:range okns:string ;
    linkml:slot_uri <https://www.opengis.net/def/schema/hy_features/hyf/name_string> .

okns:owl_allValuesFrom a linkml:SlotDefinition ;
    dcterms:source owl: ;
    dcterms:title "allValuesFrom" ;
    skos:definition "The property that determines the class that a universal property restriction refers to." ;
    skos:editorialNote "No occurrences of this slot in the graph." ;
    skos:inScheme okns:owl-rdf-rdfs ;
    skos:mappingRelation owl:allValuesFrom ;
    linkml:definition_uri okns:owl_allValuesFrom ;
    linkml:domain okns:OwlRestriction ;
    linkml:inlined true ;
    linkml:owner okns:owl_allValuesFrom ;
    linkml:range okns:RdfsClass ;
    linkml:slot_uri owl:allValuesFrom .

okns:owl_annotatedProperty a linkml:SlotDefinition ;
    dcterms:source owl: ;
    dcterms:title "annotatedProperty" ;
    skos:definition "The property that determines the predicate of an annotated axiom or annotated annotation." ;
    skos:editorialNote "No occurrences of this slot in the graph." ;
    skos:inScheme okns:owl-rdf-rdfs ;
    skos:mappingRelation owl:annotatedProperty ;
    linkml:definition_uri okns:owl_annotatedProperty ;
    linkml:domain okns:RdfsResource ;
    linkml:inlined true ;
    linkml:owner okns:owl_annotatedProperty ;
    linkml:range okns:RdfsResource ;
    linkml:slot_uri owl:annotatedProperty .

okns:owl_annotatedSource a linkml:SlotDefinition ;
    dcterms:source owl: ;
    dcterms:title "annotatedSource" ;
    skos:definition "The property that determines the subject of an annotated axiom or annotated annotation." ;
    skos:editorialNote "No occurrences of this slot in the graph." ;
    skos:inScheme okns:owl-rdf-rdfs ;
    skos:mappingRelation owl:annotatedSource ;
    linkml:definition_uri okns:owl_annotatedSource ;
    linkml:domain okns:RdfsResource ;
    linkml:inlined true ;
    linkml:owner okns:owl_annotatedSource ;
    linkml:range okns:RdfsResource ;
    linkml:slot_uri owl:annotatedSource .

okns:owl_annotatedTarget a linkml:SlotDefinition ;
    dcterms:source owl: ;
    dcterms:title "annotatedTarget" ;
    skos:definition "The property that determines the object of an annotated axiom or annotated annotation." ;
    skos:editorialNote "No occurrences of this slot in the graph." ;
    skos:inScheme okns:owl-rdf-rdfs ;
    skos:mappingRelation owl:annotatedTarget ;
    linkml:definition_uri okns:owl_annotatedTarget ;
    linkml:domain okns:RdfsResource ;
    linkml:inlined true ;
    linkml:owner okns:owl_annotatedTarget ;
    linkml:range okns:RdfsResource ;
    linkml:slot_uri owl:annotatedTarget .

okns:owl_assertionProperty a linkml:SlotDefinition ;
    dcterms:source owl: ;
    dcterms:title "assertionProperty" ;
    skos:definition "The property that determines the predicate of a negative property assertion." ;
    skos:editorialNote "No occurrences of this slot in the graph." ;
    skos:inScheme okns:owl-rdf-rdfs ;
    skos:mappingRelation owl:assertionProperty ;
    linkml:definition_uri okns:owl_assertionProperty ;
    linkml:domain okns:OwlNegativePropertyAssertion ;
    linkml:inlined true ;
    linkml:owner okns:owl_assertionProperty ;
    linkml:range okns:RdfProperty ;
    linkml:slot_uri owl:assertionProperty .

okns:owl_backwardCompatibleWith a linkml:SlotDefinition ;
    dcterms:source owl: ;
    dcterms:title "backwardCompatibleWith" ;
    skos:definition "The annotation property that indicates that a given ontology is backward compatible with another ontology." ;
    skos:editorialNote "No occurrences of this slot in the graph." ;
    skos:inScheme okns:owl-rdf-rdfs ;
    skos:mappingRelation owl:backwardCompatibleWith ;
    linkml:definition_uri okns:owl_backwardCompatibleWith ;
    linkml:domain okns:OwlOntology ;
    linkml:inlined true ;
    linkml:owner okns:owl_backwardCompatibleWith ;
    linkml:range okns:OwlOntology ;
    linkml:slot_uri owl:backwardCompatibleWith .

okns:owl_bottomDataProperty a linkml:SlotDefinition ;
    dcterms:source owl: ;
    dcterms:title "bottomDataProperty" ;
    skos:definition "The data property that does not relate any individual to any data value." ;
    skos:editorialNote "No occurrences of this slot in the graph." ;
    skos:inScheme okns:owl-rdf-rdfs ;
    skos:mappingRelation owl:bottomDataProperty ;
    linkml:definition_uri okns:owl_bottomDataProperty ;
    linkml:domain okns:OwlThing ;
    linkml:inlined true ;
    linkml:owner okns:owl_bottomDataProperty ;
    linkml:range okns:RdfsLiteral ;
    linkml:slot_uri owl:bottomDataProperty .

okns:owl_bottomObjectProperty a linkml:SlotDefinition ;
    dcterms:source owl: ;
    dcterms:title "bottomObjectProperty" ;
    skos:definition "The object property that does not relate any two individuals." ;
    skos:editorialNote "No occurrences of this slot in the graph." ;
    skos:inScheme okns:owl-rdf-rdfs ;
    skos:mappingRelation owl:bottomObjectProperty ;
    linkml:definition_uri okns:owl_bottomObjectProperty ;
    linkml:domain okns:OwlThing ;
    linkml:inlined true ;
    linkml:owner okns:owl_bottomObjectProperty ;
    linkml:range okns:OwlThing ;
    linkml:slot_uri owl:bottomObjectProperty .

okns:owl_cardinality a linkml:SlotDefinition ;
    dcterms:source owl: ;
    dcterms:title "cardinality" ;
    skos:definition "The property that determines the cardinality of an exact cardinality restriction." ;
    skos:editorialNote "No occurrences of this slot in the graph." ;
    skos:inScheme okns:owl-rdf-rdfs ;
    skos:mappingRelation owl:cardinality ;
    linkml:definition_uri okns:owl_cardinality ;
    linkml:domain okns:OwlRestriction ;
    linkml:owner okns:owl_cardinality ;
    linkml:range okns:unsignedinteger ;
    linkml:slot_uri owl:cardinality .

okns:owl_complementOf a linkml:SlotDefinition ;
    dcterms:source owl: ;
    dcterms:title "complementOf" ;
    skos:definition "The property that determines that a given class is the complement of another class." ;
    skos:editorialNote "No occurrences of this slot in the graph." ;
    skos:inScheme okns:owl-rdf-rdfs ;
    skos:mappingRelation owl:complementOf ;
    linkml:definition_uri okns:owl_complementOf ;
    linkml:domain okns:OwlClass ;
    linkml:inlined true ;
    linkml:owner okns:owl_complementOf ;
    linkml:range okns:OwlClass ;
    linkml:slot_uri owl:complementOf .

okns:owl_datatypeComplementOf a linkml:SlotDefinition ;
    dcterms:source owl: ;
    dcterms:title "datatypeComplementOf" ;
    skos:definition "The property that determines that a given data range is the complement of another data range with respect to the data domain." ;
    skos:editorialNote "No occurrences of this slot in the graph." ;
    skos:inScheme okns:owl-rdf-rdfs ;
    skos:mappingRelation owl:datatypeComplementOf ;
    linkml:definition_uri okns:owl_datatypeComplementOf ;
    linkml:domain okns:RdfsDatatype ;
    linkml:inlined true ;
    linkml:owner okns:owl_datatypeComplementOf ;
    linkml:range okns:RdfsDatatype ;
    linkml:slot_uri owl:datatypeComplementOf .

okns:owl_deprecated a linkml:SlotDefinition ;
    dcterms:source owl: ;
    dcterms:title "deprecated" ;
    skos:definition "The annotation property that indicates that a given entity has been deprecated." ;
    skos:editorialNote "No occurrences of this slot in the graph." ;
    skos:inScheme okns:owl-rdf-rdfs ;
    skos:mappingRelation owl:deprecated ;
    linkml:definition_uri okns:owl_deprecated ;
    linkml:domain okns:RdfsResource ;
    linkml:inlined true ;
    linkml:owner okns:owl_deprecated ;
    linkml:range okns:RdfsResource ;
    linkml:slot_uri owl:deprecated .

okns:owl_differentFrom a linkml:SlotDefinition ;
    dcterms:source owl: ;
    dcterms:title "differentFrom" ;
    skos:definition "The property that determines that two given individuals are different." ;
    skos:editorialNote "No occurrences of this slot in the graph." ;
    skos:inScheme okns:owl-rdf-rdfs ;
    skos:mappingRelation owl:differentFrom ;
    linkml:definition_uri okns:owl_differentFrom ;
    linkml:domain okns:OwlThing ;
    linkml:inlined true ;
    linkml:owner okns:owl_differentFrom ;
    linkml:range okns:OwlThing ;
    linkml:slot_uri owl:differentFrom .

okns:owl_disjointUnionOf a linkml:SlotDefinition ;
    dcterms:source owl: ;
    dcterms:title "disjointUnionOf" ;
    skos:definition "The property that determines that a given class is equivalent to the disjoint union of a collection of other classes." ;
    skos:editorialNote "No occurrences of this slot in the graph." ;
    skos:inScheme okns:owl-rdf-rdfs ;
    skos:mappingRelation owl:disjointUnionOf ;
    linkml:definition_uri okns:owl_disjointUnionOf ;
    linkml:domain okns:OwlClass ;
    linkml:inlined true ;
    linkml:owner okns:owl_disjointUnionOf ;
    linkml:range okns:RdfList ;
    linkml:slot_uri owl:disjointUnionOf .

okns:owl_disjointWith a linkml:SlotDefinition ;
    dcterms:source owl: ;
    dcterms:title "disjointWith" ;
    skos:definition "The property that determines that two given classes are disjoint." ;
    skos:editorialNote "No occurrences of this slot in the graph." ;
    skos:inScheme okns:owl-rdf-rdfs ;
    skos:mappingRelation owl:disjointWith ;
    linkml:definition_uri okns:owl_disjointWith ;
    linkml:domain okns:OwlClass ;
    linkml:inlined true ;
    linkml:owner okns:owl_disjointWith ;
    linkml:range okns:OwlClass ;
    linkml:slot_uri owl:disjointWith .

okns:owl_distinctMembers a linkml:SlotDefinition ;
    dcterms:source owl: ;
    dcterms:title "distinctMembers" ;
    skos:definition "The property that determines the collection of pairwise different individuals in a owl:AllDifferent axiom." ;
    skos:editorialNote "No occurrences of this slot in the graph." ;
    skos:inScheme okns:owl-rdf-rdfs ;
    skos:mappingRelation owl:distinctMembers ;
    linkml:definition_uri okns:owl_distinctMembers ;
    linkml:domain okns:OwlAllDifferent ;
    linkml:inlined true ;
    linkml:owner okns:owl_distinctMembers ;
    linkml:range okns:RdfList ;
    linkml:slot_uri owl:distinctMembers .

okns:owl_equivalentClass a linkml:SlotDefinition ;
    dcterms:source owl: ;
    dcterms:title "equivalentClass" ;
    skos:definition "The property that determines that two given classes are equivalent, and that is used to specify datatype definitions." ;
    skos:editorialNote "No occurrences of this slot in the graph." ;
    skos:inScheme okns:owl-rdf-rdfs ;
    skos:mappingRelation owl:equivalentClass ;
    linkml:definition_uri okns:owl_equivalentClass ;
    linkml:domain okns:RdfsClass ;
    linkml:inlined true ;
    linkml:owner okns:owl_equivalentClass ;
    linkml:range okns:RdfsClass ;
    linkml:slot_uri owl:equivalentClass .

okns:owl_equivalentProperty a linkml:SlotDefinition ;
    dcterms:source owl: ;
    dcterms:title "equivalentProperty" ;
    skos:definition "The property that determines that two given properties are equivalent." ;
    skos:editorialNote "No occurrences of this slot in the graph." ;
    skos:inScheme okns:owl-rdf-rdfs ;
    skos:mappingRelation owl:equivalentProperty ;
    linkml:definition_uri okns:owl_equivalentProperty ;
    linkml:domain okns:RdfProperty ;
    linkml:inlined true ;
    linkml:owner okns:owl_equivalentProperty ;
    linkml:range okns:RdfProperty ;
    linkml:slot_uri owl:equivalentProperty .

okns:owl_hasKey a linkml:SlotDefinition ;
    dcterms:source owl: ;
    dcterms:title "hasKey" ;
    skos:definition "The property that determines the collection of properties that jointly build a key." ;
    skos:editorialNote "No occurrences of this slot in the graph." ;
    skos:inScheme okns:owl-rdf-rdfs ;
    skos:mappingRelation owl:hasKey ;
    linkml:definition_uri okns:owl_hasKey ;
    linkml:domain okns:OwlClass ;
    linkml:inlined true ;
    linkml:owner okns:owl_hasKey ;
    linkml:range okns:RdfList ;
    linkml:slot_uri owl:hasKey .

okns:owl_hasSelf a linkml:SlotDefinition ;
    dcterms:source owl: ;
    dcterms:title "hasSelf" ;
    skos:definition "The property that determines the property that a self restriction refers to." ;
    skos:editorialNote "No occurrences of this slot in the graph." ;
    skos:inScheme okns:owl-rdf-rdfs ;
    skos:mappingRelation owl:hasSelf ;
    linkml:definition_uri okns:owl_hasSelf ;
    linkml:domain okns:OwlRestriction ;
    linkml:inlined true ;
    linkml:owner okns:owl_hasSelf ;
    linkml:range okns:RdfsResource ;
    linkml:slot_uri owl:hasSelf .

okns:owl_hasValue a linkml:SlotDefinition ;
    dcterms:source owl: ;
    dcterms:title "hasValue" ;
    skos:definition "The property that determines the individual that a has-value restriction refers to." ;
    skos:editorialNote "No occurrences of this slot in the graph." ;
    skos:inScheme okns:owl-rdf-rdfs ;
    skos:mappingRelation owl:hasValue ;
    linkml:definition_uri okns:owl_hasValue ;
    linkml:domain okns:OwlRestriction ;
    linkml:inlined true ;
    linkml:owner okns:owl_hasValue ;
    linkml:range okns:RdfsResource ;
    linkml:slot_uri owl:hasValue .

okns:owl_imports a linkml:SlotDefinition ;
    dcterms:source owl: ;
    dcterms:title "imports" ;
    skos:definition "The property that is used for importing other ontologies into a given ontology." ;
    skos:editorialNote "No occurrences of this slot in the graph." ;
    skos:inScheme okns:owl-rdf-rdfs ;
    skos:mappingRelation owl:imports ;
    linkml:definition_uri okns:owl_imports ;
    linkml:domain okns:OwlOntology ;
    linkml:inlined true ;
    linkml:owner okns:owl_imports ;
    linkml:range okns:OwlOntology ;
    linkml:slot_uri owl:imports .

okns:owl_incompatibleWith a linkml:SlotDefinition ;
    dcterms:source owl: ;
    dcterms:title "incompatibleWith" ;
    skos:definition "The annotation property that indicates that a given ontology is incompatible with another ontology." ;
    skos:editorialNote "No occurrences of this slot in the graph." ;
    skos:inScheme okns:owl-rdf-rdfs ;
    skos:mappingRelation owl:incompatibleWith ;
    linkml:definition_uri okns:owl_incompatibleWith ;
    linkml:domain okns:OwlOntology ;
    linkml:inlined true ;
    linkml:owner okns:owl_incompatibleWith ;
    linkml:range okns:OwlOntology ;
    linkml:slot_uri owl:incompatibleWith .

okns:owl_intersectionOf a linkml:SlotDefinition ;
    dcterms:source owl: ;
    dcterms:title "intersectionOf" ;
    skos:definition "The property that determines the collection of classes or data ranges that build an intersection." ;
    skos:editorialNote "No occurrences of this slot in the graph." ;
    skos:inScheme okns:owl-rdf-rdfs ;
    skos:mappingRelation owl:intersectionOf ;
    linkml:definition_uri okns:owl_intersectionOf ;
    linkml:domain okns:RdfsClass ;
    linkml:inlined true ;
    linkml:owner okns:owl_intersectionOf ;
    linkml:range okns:RdfList ;
    linkml:slot_uri owl:intersectionOf .

okns:owl_inverseOf a linkml:SlotDefinition ;
    dcterms:source owl: ;
    dcterms:title "inverseOf" ;
    skos:definition "The property that determines that two given properties are inverse." ;
    skos:editorialNote "No occurrences of this slot in the graph." ;
    skos:inScheme okns:owl-rdf-rdfs ;
    skos:mappingRelation owl:inverseOf ;
    linkml:definition_uri okns:owl_inverseOf ;
    linkml:domain okns:OwlObjectProperty ;
    linkml:inlined true ;
    linkml:owner okns:owl_inverseOf ;
    linkml:range okns:OwlObjectProperty ;
    linkml:slot_uri owl:inverseOf .

okns:owl_maxCardinality a linkml:SlotDefinition ;
    dcterms:source owl: ;
    dcterms:title "maxCardinality" ;
    skos:definition "The property that determines the cardinality of a maximum cardinality restriction." ;
    skos:editorialNote "No occurrences of this slot in the graph." ;
    skos:inScheme okns:owl-rdf-rdfs ;
    skos:mappingRelation owl:maxCardinality ;
    linkml:definition_uri okns:owl_maxCardinality ;
    linkml:domain okns:OwlRestriction ;
    linkml:owner okns:owl_maxCardinality ;
    linkml:range okns:unsignedinteger ;
    linkml:slot_uri owl:maxCardinality .

okns:owl_maxQualifiedCardinality a linkml:SlotDefinition ;
    dcterms:source owl: ;
    dcterms:title "maxQualifiedCardinality" ;
    skos:definition "The property that determines the cardinality of a maximum qualified cardinality restriction." ;
    skos:editorialNote "No occurrences of this slot in the graph." ;
    skos:inScheme okns:owl-rdf-rdfs ;
    skos:mappingRelation owl:maxQualifiedCardinality ;
    linkml:definition_uri okns:owl_maxQualifiedCardinality ;
    linkml:domain okns:OwlRestriction ;
    linkml:owner okns:owl_maxQualifiedCardinality ;
    linkml:range okns:unsignedinteger ;
    linkml:slot_uri owl:maxQualifiedCardinality .

okns:owl_members a linkml:SlotDefinition ;
    dcterms:source owl: ;
    dcterms:title "members" ;
    skos:definition "The property that determines the collection of members in either a owl:AllDifferent, owl:AllDisjointClasses or owl:AllDisjointProperties axiom." ;
    skos:editorialNote "No occurrences of this slot in the graph." ;
    skos:inScheme okns:owl-rdf-rdfs ;
    skos:mappingRelation owl:members ;
    linkml:definition_uri okns:owl_members ;
    linkml:domain okns:RdfsResource ;
    linkml:inlined true ;
    linkml:owner okns:owl_members ;
    linkml:range okns:RdfList ;
    linkml:slot_uri owl:members .

okns:owl_minCardinality a linkml:SlotDefinition ;
    dcterms:source owl: ;
    dcterms:title "minCardinality" ;
    skos:definition "The property that determines the cardinality of a minimum cardinality restriction." ;
    skos:editorialNote "No occurrences of this slot in the graph." ;
    skos:inScheme okns:owl-rdf-rdfs ;
    skos:mappingRelation owl:minCardinality ;
    linkml:definition_uri okns:owl_minCardinality ;
    linkml:domain okns:OwlRestriction ;
    linkml:owner okns:owl_minCardinality ;
    linkml:range okns:unsignedinteger ;
    linkml:slot_uri owl:minCardinality .

okns:owl_minQualifiedCardinality a linkml:SlotDefinition ;
    dcterms:source owl: ;
    dcterms:title "minQualifiedCardinality" ;
    skos:definition "The property that determines the cardinality of a minimum qualified cardinality restriction." ;
    skos:editorialNote "No occurrences of this slot in the graph." ;
    skos:inScheme okns:owl-rdf-rdfs ;
    skos:mappingRelation owl:minQualifiedCardinality ;
    linkml:definition_uri okns:owl_minQualifiedCardinality ;
    linkml:domain okns:OwlRestriction ;
    linkml:owner okns:owl_minQualifiedCardinality ;
    linkml:range okns:unsignedinteger ;
    linkml:slot_uri owl:minQualifiedCardinality .

okns:owl_onClass a linkml:SlotDefinition ;
    dcterms:source owl: ;
    dcterms:title "onClass" ;
    skos:definition "The property that determines the class that a qualified object cardinality restriction refers to." ;
    skos:editorialNote "No occurrences of this slot in the graph." ;
    skos:inScheme okns:owl-rdf-rdfs ;
    skos:mappingRelation owl:onClass ;
    linkml:definition_uri okns:owl_onClass ;
    linkml:domain okns:OwlRestriction ;
    linkml:inlined true ;
    linkml:owner okns:owl_onClass ;
    linkml:range okns:OwlClass ;
    linkml:slot_uri owl:onClass .

okns:owl_onDataRange a linkml:SlotDefinition ;
    dcterms:source owl: ;
    dcterms:title "onDataRange" ;
    skos:definition "The property that determines the data range that a qualified data cardinality restriction refers to." ;
    skos:editorialNote "No occurrences of this slot in the graph." ;
    skos:inScheme okns:owl-rdf-rdfs ;
    skos:mappingRelation owl:onDataRange ;
    linkml:definition_uri okns:owl_onDataRange ;
    linkml:domain okns:OwlRestriction ;
    linkml:inlined true ;
    linkml:owner okns:owl_onDataRange ;
    linkml:range okns:RdfsDatatype ;
    linkml:slot_uri owl:onDataRange .

okns:owl_onDatatype a linkml:SlotDefinition ;
    dcterms:source owl: ;
    dcterms:title "onDatatype" ;
    skos:definition "The property that determines the datatype that a datatype restriction refers to." ;
    skos:editorialNote "No occurrences of this slot in the graph." ;
    skos:inScheme okns:owl-rdf-rdfs ;
    skos:mappingRelation owl:onDatatype ;
    linkml:definition_uri okns:owl_onDatatype ;
    linkml:domain okns:RdfsDatatype ;
    linkml:inlined true ;
    linkml:owner okns:owl_onDatatype ;
    linkml:range okns:RdfsDatatype ;
    linkml:slot_uri owl:onDatatype .

okns:owl_onProperties a linkml:SlotDefinition ;
    dcterms:source owl: ;
    dcterms:title "onProperties" ;
    skos:definition "The property that determines the n-tuple of properties that a property restriction on an n-ary data range refers to." ;
    skos:editorialNote "No occurrences of this slot in the graph." ;
    skos:inScheme okns:owl-rdf-rdfs ;
    skos:mappingRelation owl:onProperties ;
    linkml:definition_uri okns:owl_onProperties ;
    linkml:domain okns:OwlRestriction ;
    linkml:inlined true ;
    linkml:owner okns:owl_onProperties ;
    linkml:range okns:RdfList ;
    linkml:slot_uri owl:onProperties .

okns:owl_onProperty a linkml:SlotDefinition ;
    dcterms:source owl: ;
    dcterms:title "onProperty" ;
    skos:definition "The property that determines the property that a property restriction refers to." ;
    skos:editorialNote "No occurrences of this slot in the graph." ;
    skos:inScheme okns:owl-rdf-rdfs ;
    skos:mappingRelation owl:onProperty ;
    linkml:definition_uri okns:owl_onProperty ;
    linkml:domain okns:OwlRestriction ;
    linkml:inlined true ;
    linkml:owner okns:owl_onProperty ;
    linkml:range okns:RdfProperty ;
    linkml:slot_uri owl:onProperty .

okns:owl_oneOf a linkml:SlotDefinition ;
    dcterms:source owl: ;
    dcterms:title "oneOf" ;
    skos:definition "The property that determines the collection of individuals or data values that build an enumeration." ;
    skos:editorialNote "No occurrences of this slot in the graph." ;
    skos:inScheme okns:owl-rdf-rdfs ;
    skos:mappingRelation owl:oneOf ;
    linkml:definition_uri okns:owl_oneOf ;
    linkml:domain okns:RdfsClass ;
    linkml:inlined true ;
    linkml:owner okns:owl_oneOf ;
    linkml:range okns:RdfList ;
    linkml:slot_uri owl:oneOf .

okns:owl_priorVersion a linkml:SlotDefinition ;
    dcterms:source owl: ;
    dcterms:title "priorVersion" ;
    skos:definition "The annotation property that indicates the predecessor ontology of a given ontology." ;
    skos:editorialNote "No occurrences of this slot in the graph." ;
    skos:inScheme okns:owl-rdf-rdfs ;
    skos:mappingRelation owl:priorVersion ;
    linkml:definition_uri okns:owl_priorVersion ;
    linkml:domain okns:OwlOntology ;
    linkml:inlined true ;
    linkml:owner okns:owl_priorVersion ;
    linkml:range okns:OwlOntology ;
    linkml:slot_uri owl:priorVersion .

okns:owl_propertyChainAxiom a linkml:SlotDefinition ;
    dcterms:source owl: ;
    dcterms:title "propertyChainAxiom" ;
    skos:definition "The property that determines the n-tuple of properties that build a sub property chain of a given property." ;
    skos:editorialNote "No occurrences of this slot in the graph." ;
    skos:inScheme okns:owl-rdf-rdfs ;
    skos:mappingRelation owl:propertyChainAxiom ;
    linkml:definition_uri okns:owl_propertyChainAxiom ;
    linkml:domain okns:OwlObjectProperty ;
    linkml:inlined true ;
    linkml:owner okns:owl_propertyChainAxiom ;
    linkml:range okns:RdfList ;
    linkml:slot_uri owl:propertyChainAxiom .

okns:owl_propertyDisjointWith a linkml:SlotDefinition ;
    dcterms:source owl: ;
    dcterms:title "propertyDisjointWith" ;
    skos:definition "The property that determines that two given properties are disjoint." ;
    skos:editorialNote "No occurrences of this slot in the graph." ;
    skos:inScheme okns:owl-rdf-rdfs ;
    skos:mappingRelation owl:propertyDisjointWith ;
    linkml:definition_uri okns:owl_propertyDisjointWith ;
    linkml:domain okns:RdfProperty ;
    linkml:inlined true ;
    linkml:owner okns:owl_propertyDisjointWith ;
    linkml:range okns:RdfProperty ;
    linkml:slot_uri owl:propertyDisjointWith .

okns:owl_qualifiedCardinality a linkml:SlotDefinition ;
    dcterms:source owl: ;
    dcterms:title "qualifiedCardinality" ;
    skos:definition "The property that determines the cardinality of an exact qualified cardinality restriction." ;
    skos:editorialNote "No occurrences of this slot in the graph." ;
    skos:inScheme okns:owl-rdf-rdfs ;
    skos:mappingRelation owl:qualifiedCardinality ;
    linkml:definition_uri okns:owl_qualifiedCardinality ;
    linkml:domain okns:OwlRestriction ;
    linkml:owner okns:owl_qualifiedCardinality ;
    linkml:range okns:unsignedinteger ;
    linkml:slot_uri owl:qualifiedCardinality .

okns:owl_sameAs a linkml:SlotDefinition ;
    dcterms:source owl: ;
    dcterms:title "sameAs" ;
    skos:definition "The property that determines that two given individuals are equal." ;
    skos:editorialNote "No occurrences of this slot in the graph." ;
    skos:inScheme okns:owl-rdf-rdfs ;
    skos:mappingRelation owl:sameAs ;
    linkml:definition_uri okns:owl_sameAs ;
    linkml:domain okns:OwlThing ;
    linkml:inlined true ;
    linkml:owner okns:owl_sameAs ;
    linkml:range okns:OwlThing ;
    linkml:slot_uri owl:sameAs .

okns:owl_someValuesFrom a linkml:SlotDefinition ;
    dcterms:source owl: ;
    dcterms:title "someValuesFrom" ;
    skos:definition "The property that determines the class that an existential property restriction refers to." ;
    skos:editorialNote "No occurrences of this slot in the graph." ;
    skos:inScheme okns:owl-rdf-rdfs ;
    skos:mappingRelation owl:someValuesFrom ;
    linkml:definition_uri okns:owl_someValuesFrom ;
    linkml:domain okns:OwlRestriction ;
    linkml:inlined true ;
    linkml:owner okns:owl_someValuesFrom ;
    linkml:range okns:RdfsClass ;
    linkml:slot_uri owl:someValuesFrom .

okns:owl_sourceIndividual a linkml:SlotDefinition ;
    dcterms:source owl: ;
    dcterms:title "sourceIndividual" ;
    skos:definition "The property that determines the subject of a negative property assertion." ;
    skos:editorialNote "No occurrences of this slot in the graph." ;
    skos:inScheme okns:owl-rdf-rdfs ;
    skos:mappingRelation owl:sourceIndividual ;
    linkml:definition_uri okns:owl_sourceIndividual ;
    linkml:domain okns:OwlNegativePropertyAssertion ;
    linkml:inlined true ;
    linkml:owner okns:owl_sourceIndividual ;
    linkml:range okns:OwlThing ;
    linkml:slot_uri owl:sourceIndividual .

okns:owl_targetIndividual a linkml:SlotDefinition ;
    dcterms:source owl: ;
    dcterms:title "targetIndividual" ;
    skos:definition "The property that determines the object of a negative object property assertion." ;
    skos:editorialNote "No occurrences of this slot in the graph." ;
    skos:inScheme okns:owl-rdf-rdfs ;
    skos:mappingRelation owl:targetIndividual ;
    linkml:definition_uri okns:owl_targetIndividual ;
    linkml:domain okns:OwlNegativePropertyAssertion ;
    linkml:inlined true ;
    linkml:owner okns:owl_targetIndividual ;
    linkml:range okns:OwlThing ;
    linkml:slot_uri owl:targetIndividual .

okns:owl_targetValue a linkml:SlotDefinition ;
    dcterms:source owl: ;
    dcterms:title "targetValue" ;
    skos:definition "The property that determines the value of a negative data property assertion." ;
    skos:editorialNote "No occurrences of this slot in the graph." ;
    skos:inScheme okns:owl-rdf-rdfs ;
    skos:mappingRelation owl:targetValue ;
    linkml:definition_uri okns:owl_targetValue ;
    linkml:domain okns:OwlNegativePropertyAssertion ;
    linkml:inlined true ;
    linkml:owner okns:owl_targetValue ;
    linkml:range okns:RdfsLiteral ;
    linkml:slot_uri owl:targetValue .

okns:owl_topDataProperty a linkml:SlotDefinition ;
    dcterms:source owl: ;
    dcterms:title "topDataProperty" ;
    skos:definition "The data property that relates every individual to every data value." ;
    skos:editorialNote "No occurrences of this slot in the graph." ;
    skos:inScheme okns:owl-rdf-rdfs ;
    skos:mappingRelation owl:topDataProperty ;
    linkml:definition_uri okns:owl_topDataProperty ;
    linkml:domain okns:OwlThing ;
    linkml:inlined true ;
    linkml:owner okns:owl_topDataProperty ;
    linkml:range okns:RdfsLiteral ;
    linkml:slot_uri owl:topDataProperty .

okns:owl_topObjectProperty a linkml:SlotDefinition ;
    dcterms:source owl: ;
    dcterms:title "topObjectProperty" ;
    skos:definition "The object property that relates every two individuals." ;
    skos:editorialNote "No occurrences of this slot in the graph." ;
    skos:inScheme okns:owl-rdf-rdfs ;
    skos:mappingRelation owl:topObjectProperty ;
    linkml:definition_uri okns:owl_topObjectProperty ;
    linkml:domain okns:OwlThing ;
    linkml:inlined true ;
    linkml:owner okns:owl_topObjectProperty ;
    linkml:range okns:OwlThing ;
    linkml:slot_uri owl:topObjectProperty .

okns:owl_unionOf a linkml:SlotDefinition ;
    dcterms:source owl: ;
    dcterms:title "unionOf" ;
    skos:definition "The property that determines the collection of classes or data ranges that build a union." ;
    skos:editorialNote "No occurrences of this slot in the graph." ;
    skos:inScheme okns:owl-rdf-rdfs ;
    skos:mappingRelation owl:unionOf ;
    linkml:definition_uri okns:owl_unionOf ;
    linkml:domain okns:RdfsClass ;
    linkml:inlined true ;
    linkml:owner okns:owl_unionOf ;
    linkml:range okns:RdfList ;
    linkml:slot_uri owl:unionOf .

okns:owl_versionIRI a linkml:SlotDefinition ;
    dcterms:source owl: ;
    dcterms:title "versionIRI" ;
    skos:definition "The property that identifies the version IRI of an ontology." ;
    skos:editorialNote "No occurrences of this slot in the graph." ;
    skos:inScheme okns:owl-rdf-rdfs ;
    skos:mappingRelation owl:versionIRI ;
    linkml:definition_uri okns:owl_versionIRI ;
    linkml:domain okns:OwlOntology ;
    linkml:inlined true ;
    linkml:owner okns:owl_versionIRI ;
    linkml:range okns:OwlOntology ;
    linkml:slot_uri owl:versionIRI .

okns:owl_versionInfo a linkml:SlotDefinition ;
    dcterms:source owl: ;
    dcterms:title "versionInfo" ;
    skos:definition "The annotation property that provides version information for an ontology or another OWL construct." ;
    skos:editorialNote "No occurrences of this slot in the graph." ;
    skos:inScheme okns:owl-rdf-rdfs ;
    skos:mappingRelation owl:versionInfo ;
    linkml:definition_uri okns:owl_versionInfo ;
    linkml:domain okns:RdfsResource ;
    linkml:inlined true ;
    linkml:owner okns:owl_versionInfo ;
    linkml:range okns:RdfsResource ;
    linkml:slot_uri owl:versionInfo .

okns:owl_withRestrictions a linkml:SlotDefinition ;
    dcterms:source owl: ;
    dcterms:title "withRestrictions" ;
    skos:definition "The property that determines the collection of facet-value pairs that define a datatype restriction." ;
    skos:editorialNote "No occurrences of this slot in the graph." ;
    skos:inScheme okns:owl-rdf-rdfs ;
    skos:mappingRelation owl:withRestrictions ;
    linkml:definition_uri okns:owl_withRestrictions ;
    linkml:domain okns:RdfsDatatype ;
    linkml:inlined true ;
    linkml:owner okns:owl_withRestrictions ;
    linkml:range okns:RdfList ;
    linkml:slot_uri owl:withRestrictions .

okns:rdf_direction a linkml:SlotDefinition ;
    dcterms:source rdf: ;
    dcterms:title "direction" ;
    rdfs:seeAlso <https://www.w3.org/TR/json-ld11/#the-rdf-compoundliteral-class-and-the-rdf-language-and-rdf-direction-properties> ;
    skos:definition "The base direction component of a CompoundLiteral." ;
    skos:editorialNote "No occurrences of this slot in the graph." ;
    skos:inScheme okns:owl-rdf-rdfs ;
    skos:mappingRelation rdf:direction ;
    linkml:definition_uri okns:rdf_direction ;
    linkml:domain okns:RdfCompoundLiteral ;
    linkml:inlined true ;
    linkml:owner okns:rdf_direction ;
    linkml:range okns:Any ;
    linkml:slot_uri rdf:direction .

okns:rdf_first a linkml:SlotDefinition ;
    dcterms:source rdf: ;
    dcterms:title "first" ;
    skos:definition "The first item in the subject RDF list." ;
    skos:editorialNote "No occurrences of this slot in the graph." ;
    skos:inScheme okns:owl-rdf-rdfs ;
    skos:mappingRelation rdf:first ;
    linkml:definition_uri okns:rdf_first ;
    linkml:domain okns:RdfList ;
    linkml:inlined true ;
    linkml:owner okns:rdf_first ;
    linkml:range okns:RdfsResource ;
    linkml:slot_uri rdf:first .

okns:rdf_language a linkml:SlotDefinition ;
    dcterms:source rdf: ;
    dcterms:title "language" ;
    rdfs:seeAlso <https://www.w3.org/TR/json-ld11/#the-rdf-compoundliteral-class-and-the-rdf-language-and-rdf-direction-properties> ;
    skos:definition "The language component of a CompoundLiteral." ;
    skos:editorialNote "No occurrences of this slot in the graph." ;
    skos:inScheme okns:owl-rdf-rdfs ;
    skos:mappingRelation rdf:language ;
    linkml:definition_uri okns:rdf_language ;
    linkml:domain okns:RdfCompoundLiteral ;
    linkml:inlined true ;
    linkml:owner okns:rdf_language ;
    linkml:range okns:Any ;
    linkml:slot_uri rdf:language .

okns:rdf_object a linkml:SlotDefinition ;
    dcterms:source rdf: ;
    dcterms:title "object" ;
    skos:definition "The object of the subject RDF statement." ;
    skos:editorialNote "No occurrences of this slot in the graph." ;
    skos:inScheme okns:owl-rdf-rdfs ;
    skos:mappingRelation rdf:object ;
    linkml:definition_uri okns:rdf_object ;
    linkml:domain okns:RdfStatement ;
    linkml:inlined true ;
    linkml:owner okns:rdf_object ;
    linkml:range okns:RdfsResource ;
    linkml:slot_uri rdf:object .

okns:rdf_predicate a linkml:SlotDefinition ;
    dcterms:source rdf: ;
    dcterms:title "predicate" ;
    skos:definition "The predicate of the subject RDF statement." ;
    skos:editorialNote "No occurrences of this slot in the graph." ;
    skos:inScheme okns:owl-rdf-rdfs ;
    skos:mappingRelation rdf:predicate ;
    linkml:definition_uri okns:rdf_predicate ;
    linkml:domain okns:RdfStatement ;
    linkml:inlined true ;
    linkml:owner okns:rdf_predicate ;
    linkml:range okns:RdfsResource ;
    linkml:slot_uri rdf:predicate .

okns:rdf_rest a linkml:SlotDefinition ;
    dcterms:source rdf: ;
    dcterms:title "rest" ;
    skos:definition "The rest of the subject RDF list after the first item." ;
    skos:editorialNote "No occurrences of this slot in the graph." ;
    skos:inScheme okns:owl-rdf-rdfs ;
    skos:mappingRelation rdf:rest ;
    linkml:definition_uri okns:rdf_rest ;
    linkml:domain okns:RdfList ;
    linkml:inlined true ;
    linkml:owner okns:rdf_rest ;
    linkml:range okns:RdfList ;
    linkml:slot_uri rdf:rest .

okns:rdf_subject a linkml:SlotDefinition ;
    dcterms:source rdf: ;
    dcterms:title "subject" ;
    skos:definition "The subject of the subject RDF statement." ;
    skos:editorialNote "No occurrences of this slot in the graph." ;
    skos:inScheme okns:owl-rdf-rdfs ;
    skos:mappingRelation rdf:subject ;
    linkml:definition_uri okns:rdf_subject ;
    linkml:domain okns:RdfStatement ;
    linkml:inlined true ;
    linkml:owner okns:rdf_subject ;
    linkml:range okns:RdfsResource ;
    linkml:slot_uri rdf:subject .

okns:rdf_type a linkml:SlotDefinition ;
    dcterms:source rdf: ;
    dcterms:title "type" ;
    skos:definition "The subject is an instance of a class." ;
    skos:editorialNote "No occurrences of this slot in the graph." ;
    skos:inScheme okns:owl-rdf-rdfs ;
    skos:mappingRelation rdf:type ;
    linkml:definition_uri okns:rdf_type ;
    linkml:domain okns:RdfsResource ;
    linkml:inlined true ;
    linkml:owner okns:rdf_type ;
    linkml:range okns:RdfsClass ;
    linkml:slot_uri rdf:type .

okns:rdfs_domain a linkml:SlotDefinition ;
    dcterms:source rdfs: ;
    dcterms:title "domain" ;
    skos:definition "A domain of the subject property." ;
    skos:editorialNote "No occurrences of this slot in the graph." ;
    skos:inScheme okns:owl-rdf-rdfs ;
    skos:mappingRelation rdfs:domain ;
    linkml:definition_uri okns:rdfs_domain ;
    linkml:domain okns:RdfProperty ;
    linkml:inlined true ;
    linkml:owner okns:rdfs_domain ;
    linkml:range okns:RdfsClass ;
    linkml:slot_uri rdfs:domain .

okns:rdfs_member a linkml:SlotDefinition ;
    dcterms:source rdfs: ;
    dcterms:title "member" ;
    skos:definition "A member of the subject resource." ;
    skos:editorialNote "No occurrences of this slot in the graph." ;
    skos:inScheme okns:owl-rdf-rdfs ;
    skos:mappingRelation rdfs:member ;
    linkml:definition_uri okns:rdfs_member ;
    linkml:domain okns:RdfsResource ;
    linkml:inlined true ;
    linkml:owner okns:rdfs_member ;
    linkml:range okns:RdfsResource ;
    linkml:slot_uri rdfs:member .

okns:rdfs_range a linkml:SlotDefinition ;
    dcterms:source rdfs: ;
    dcterms:title "range" ;
    skos:definition "A range of the subject property." ;
    skos:editorialNote "No occurrences of this slot in the graph." ;
    skos:inScheme okns:owl-rdf-rdfs ;
    skos:mappingRelation rdfs:range ;
    linkml:definition_uri okns:rdfs_range ;
    linkml:domain okns:RdfProperty ;
    linkml:inlined true ;
    linkml:owner okns:rdfs_range ;
    linkml:range okns:RdfsClass ;
    linkml:slot_uri rdfs:range .

okns:rdfs_subPropertyOf a linkml:SlotDefinition ;
    dcterms:source rdfs: ;
    dcterms:title "subPropertyOf" ;
    skos:definition "The subject is a subproperty of a property." ;
    skos:editorialNote "No occurrences of this slot in the graph." ;
    skos:inScheme okns:owl-rdf-rdfs ;
    skos:mappingRelation rdfs:subPropertyOf ;
    linkml:definition_uri okns:rdfs_subPropertyOf ;
    linkml:domain okns:RdfProperty ;
    linkml:inlined true ;
    linkml:owner okns:rdfs_subPropertyOf ;
    linkml:range okns:RdfProperty ;
    linkml:slot_uri rdfs:subPropertyOf .

okns:sc_Measure a linkml:TypeDefinition ;
    skos:inScheme okns:sc ;
    linkml:base "str" ;
    linkml:definition_uri okns:ScMeasure ;
    linkml:typeof okns:string ;
    linkml:uri sc:Measure .

okns:seegrid_basic_dimension a linkml:SlotDefinition ;
    dcterms:source <http://def.seegrid.csiro.au/isotc211/iso19103/2005/basic> ;
    dcterms:title "dimension" ;
    skos:definition "Number of components in the vector" ;
    skos:editorialNote "No occurrences of this slot in the graph." ;
    skos:inScheme okns:seegrid-iso19115 ;
    skos:mappingRelation seegrid-basic:dimension ;
    linkml:definition_uri okns:seegrid_basic_dimension ;
    linkml:domain okns:Seegrid-basicVector ;
    linkml:owner okns:seegrid_basic_dimension ;
    linkml:range okns:positiveinteger ;
    linkml:slot_uri seegrid-basic:dimension .

okns:seegrid_basic_ordinates a linkml:SlotDefinition ;
    dcterms:source <http://def.seegrid.csiro.au/isotc211/iso19103/2005/basic> ;
    dcterms:title "ordinates" ;
    skos:definition "Numerical values of the vector components" ;
    skos:editorialNote "No occurrences of this slot in the graph." ;
    skos:inScheme okns:seegrid-iso19115 ;
    skos:mappingRelation seegrid-basic:ordinates ;
    linkml:definition_uri okns:seegrid_basic_ordinates ;
    linkml:domain okns:Seegrid-basicVector ;
    linkml:inlined true ;
    linkml:owner okns:seegrid_basic_ordinates ;
    linkml:range okns:Any ;
    linkml:slot_uri seegrid-basic:ordinates .

okns:seegrid_ci_Date.date a linkml:SlotDefinition ;
    dcterms:source <http://def.seegrid.csiro.au/isotc211/iso19115/2003/citation> ;
    dcterms:title "Date.date" ;
    skos:editorialNote "No occurrences of this slot in the graph." ;
    skos:inScheme okns:seegrid-iso19115 ;
    skos:mappingRelation seegrid-ci:Date.date ;
    linkml:definition_uri okns:seegrid_ci_Date.date ;
    linkml:domain okns:Seegrid-ciDate ;
    linkml:owner okns:seegrid_ci_Date.date ;
    linkml:range okns:date ;
    linkml:slot_uri seegrid-ci:Date.date .

okns:seegrid_ci_ISBN a linkml:SlotDefinition ;
    dcterms:source <http://def.seegrid.csiro.au/isotc211/iso19115/2003/citation> ;
    dcterms:title "ISBN" ;
    skos:editorialNote "No occurrences of this slot in the graph." ;
    skos:inScheme okns:seegrid-iso19115 ;
    skos:mappingRelation seegrid-ci:ISBN ;
    linkml:definition_uri okns:seegrid_ci_ISBN ;
    linkml:domain okns:Seegrid-ciCitation ;
    linkml:owner okns:seegrid_ci_ISBN ;
    linkml:range okns:string ;
    linkml:slot_uri seegrid-ci:ISBN .

okns:seegrid_ci_ISSN a linkml:SlotDefinition ;
    dcterms:source <http://def.seegrid.csiro.au/isotc211/iso19115/2003/citation> ;
    dcterms:title "ISSN" ;
    skos:editorialNote "No occurrences of this slot in the graph." ;
    skos:inScheme okns:seegrid-iso19115 ;
    skos:mappingRelation seegrid-ci:ISSN ;
    linkml:definition_uri okns:seegrid_ci_ISSN ;
    linkml:domain okns:Seegrid-ciCitation ;
    linkml:owner okns:seegrid_ci_ISSN ;
    linkml:range okns:string ;
    linkml:slot_uri seegrid-ci:ISSN .

okns:seegrid_ci_address a linkml:SlotDefinition ;
    dcterms:source <http://def.seegrid.csiro.au/isotc211/iso19115/2003/citation> ;
    dcterms:title "address" ;
    skos:editorialNote "No occurrences of this slot in the graph." ;
    skos:inScheme okns:seegrid-iso19115 ;
    skos:mappingRelation seegrid-ci:address ;
    linkml:definition_uri okns:seegrid_ci_address ;
    linkml:domain okns:Seegrid-ciContact ;
    linkml:inlined true ;
    linkml:owner okns:seegrid_ci_address ;
    linkml:range okns:Seegrid-ciAddress ;
    linkml:slot_uri seegrid-ci:address .

okns:seegrid_ci_administrativeArea a linkml:SlotDefinition ;
    dcterms:source <http://def.seegrid.csiro.au/isotc211/iso19115/2003/citation> ;
    dcterms:title "administrative area" ;
    skos:editorialNote "No occurrences of this slot in the graph." ;
    skos:inScheme okns:seegrid-iso19115 ;
    skos:mappingRelation seegrid-ci:administrativeArea ;
    linkml:definition_uri okns:seegrid_ci_administrativeArea ;
    linkml:domain okns:Seegrid-ciAddress ;
    linkml:owner okns:seegrid_ci_administrativeArea ;
    linkml:range okns:string ;
    linkml:slot_uri seegrid-ci:administrativeArea .

okns:seegrid_ci_alternateTitle a linkml:SlotDefinition ;
    dcterms:source <http://def.seegrid.csiro.au/isotc211/iso19115/2003/citation> ;
    dcterms:title "alternate title" ;
    skos:editorialNote "No occurrences of this slot in the graph." ;
    skos:inScheme okns:seegrid-iso19115 ;
    skos:mappingRelation seegrid-ci:alternateTitle ;
    linkml:definition_uri okns:seegrid_ci_alternateTitle ;
    linkml:domain okns:Seegrid-ciCitation ;
    linkml:owner okns:seegrid_ci_alternateTitle ;
    linkml:range okns:string ;
    linkml:slot_uri seegrid-ci:alternateTitle .

okns:seegrid_ci_applicationProfile a linkml:SlotDefinition ;
    dcterms:source <http://def.seegrid.csiro.au/isotc211/iso19115/2003/citation> ;
    dcterms:title "application profile" ;
    skos:editorialNote "No occurrences of this slot in the graph." ;
    skos:inScheme okns:seegrid-iso19115 ;
    skos:mappingRelation seegrid-ci:applicationProfile ;
    linkml:definition_uri okns:seegrid_ci_applicationProfile ;
    linkml:domain okns:Seegrid-ciOnlineResource ;
    linkml:owner okns:seegrid_ci_applicationProfile ;
    linkml:range okns:string ;
    linkml:slot_uri seegrid-ci:applicationProfile .

okns:seegrid_ci_citedResponsibleParty a linkml:SlotDefinition ;
    dcterms:source <http://def.seegrid.csiro.au/isotc211/iso19115/2003/citation> ;
    dcterms:title "cited responsible party" ;
    skos:editorialNote "No occurrences of this slot in the graph." ;
    skos:inScheme okns:seegrid-iso19115 ;
    skos:mappingRelation seegrid-ci:citedResponsibleParty ;
    linkml:definition_uri okns:seegrid_ci_citedResponsibleParty ;
    linkml:domain okns:Seegrid-ciCitation ;
    linkml:inlined true ;
    linkml:owner okns:seegrid_ci_citedResponsibleParty ;
    linkml:range okns:Seegrid-ciResponsibleParty ;
    linkml:slot_uri seegrid-ci:citedResponsibleParty .

okns:seegrid_ci_city a linkml:SlotDefinition ;
    dcterms:source <http://def.seegrid.csiro.au/isotc211/iso19115/2003/citation> ;
    dcterms:title "city" ;
    skos:editorialNote "No occurrences of this slot in the graph." ;
    skos:inScheme okns:seegrid-iso19115 ;
    skos:mappingRelation seegrid-ci:city ;
    linkml:definition_uri okns:seegrid_ci_city ;
    linkml:domain okns:Seegrid-ciAddress ;
    linkml:owner okns:seegrid_ci_city ;
    linkml:range okns:string ;
    linkml:slot_uri seegrid-ci:city .

okns:seegrid_ci_collectiveTitle a linkml:SlotDefinition ;
    dcterms:source <http://def.seegrid.csiro.au/isotc211/iso19115/2003/citation> ;
    dcterms:title "collective title" ;
    skos:editorialNote "No occurrences of this slot in the graph." ;
    skos:inScheme okns:seegrid-iso19115 ;
    skos:mappingRelation seegrid-ci:collectiveTitle ;
    linkml:definition_uri okns:seegrid_ci_collectiveTitle ;
    linkml:domain okns:Seegrid-ciCitation ;
    linkml:owner okns:seegrid_ci_collectiveTitle ;
    linkml:range okns:string ;
    linkml:slot_uri seegrid-ci:collectiveTitle .

okns:seegrid_ci_contactInfo a linkml:SlotDefinition ;
    dcterms:source <http://def.seegrid.csiro.au/isotc211/iso19115/2003/citation> ;
    dcterms:title "contact info" ;
    skos:editorialNote "No occurrences of this slot in the graph." ;
    skos:inScheme okns:seegrid-iso19115 ;
    skos:mappingRelation seegrid-ci:contactInfo ;
    linkml:definition_uri okns:seegrid_ci_contactInfo ;
    linkml:domain okns:Seegrid-ciResponsibleParty ;
    linkml:inlined true ;
    linkml:owner okns:seegrid_ci_contactInfo ;
    linkml:range okns:Seegrid-ciContact ;
    linkml:slot_uri seegrid-ci:contactInfo .

okns:seegrid_ci_contactInstructions a linkml:SlotDefinition ;
    dcterms:source <http://def.seegrid.csiro.au/isotc211/iso19115/2003/citation> ;
    dcterms:title "contact instructions" ;
    skos:editorialNote "No occurrences of this slot in the graph." ;
    skos:inScheme okns:seegrid-iso19115 ;
    skos:mappingRelation seegrid-ci:contactInstructions ;
    linkml:definition_uri okns:seegrid_ci_contactInstructions ;
    linkml:domain okns:Seegrid-ciContact ;
    linkml:owner okns:seegrid_ci_contactInstructions ;
    linkml:range okns:string ;
    linkml:slot_uri seegrid-ci:contactInstructions .

okns:seegrid_ci_country a linkml:SlotDefinition ;
    dcterms:source <http://def.seegrid.csiro.au/isotc211/iso19115/2003/citation> ;
    dcterms:title "country" ;
    skos:editorialNote "No occurrences of this slot in the graph." ;
    skos:inScheme okns:seegrid-iso19115 ;
    skos:mappingRelation seegrid-ci:country ;
    linkml:definition_uri okns:seegrid_ci_country ;
    linkml:domain okns:Seegrid-ciAddress ;
    linkml:owner okns:seegrid_ci_country ;
    linkml:range okns:string ;
    linkml:slot_uri seegrid-ci:country .

okns:seegrid_ci_date a linkml:SlotDefinition ;
    dcterms:source <http://def.seegrid.csiro.au/isotc211/iso19115/2003/citation> ;
    dcterms:title "date" ;
    skos:editorialNote "No occurrences of this slot in the graph." ;
    skos:inScheme okns:seegrid-iso19115 ;
    skos:mappingRelation seegrid-ci:date ;
    linkml:definition_uri okns:seegrid_ci_date ;
    linkml:domain okns:Seegrid-ciCitation ;
    linkml:inlined true ;
    linkml:owner okns:seegrid_ci_date ;
    linkml:range okns:Seegrid-ciDate ;
    linkml:slot_uri seegrid-ci:date .

okns:seegrid_ci_dateType a linkml:SlotDefinition ;
    dcterms:source <http://def.seegrid.csiro.au/isotc211/iso19115/2003/citation> ;
    dcterms:title "date type" ;
    skos:editorialNote "No occurrences of this slot in the graph." ;
    skos:inScheme okns:seegrid-iso19115 ;
    skos:mappingRelation seegrid-ci:dateType ;
    linkml:definition_uri okns:seegrid_ci_dateType ;
    linkml:domain okns:Seegrid-ciDate ;
    linkml:inlined true ;
    linkml:owner okns:seegrid_ci_dateType ;
    linkml:range okns:Seegrid-ciDateTypeCode ;
    linkml:slot_uri seegrid-ci:dateType .

okns:seegrid_ci_deliveryPoint a linkml:SlotDefinition ;
    dcterms:source <http://def.seegrid.csiro.au/isotc211/iso19115/2003/citation> ;
    dcterms:title "delivery point" ;
    skos:editorialNote "No occurrences of this slot in the graph." ;
    skos:inScheme okns:seegrid-iso19115 ;
    skos:mappingRelation seegrid-ci:deliveryPoint ;
    linkml:definition_uri okns:seegrid_ci_deliveryPoint ;
    linkml:domain okns:Seegrid-ciAddress ;
    linkml:owner okns:seegrid_ci_deliveryPoint ;
    linkml:range okns:string ;
    linkml:slot_uri seegrid-ci:deliveryPoint .

okns:seegrid_ci_description a linkml:SlotDefinition ;
    dcterms:source <http://def.seegrid.csiro.au/isotc211/iso19115/2003/citation> ;
    dcterms:title "description" ;
    skos:editorialNote "No occurrences of this slot in the graph." ;
    skos:inScheme okns:seegrid-iso19115 ;
    skos:mappingRelation seegrid-ci:description ;
    linkml:definition_uri okns:seegrid_ci_description ;
    linkml:domain okns:Seegrid-ciOnlineResource ;
    linkml:owner okns:seegrid_ci_description ;
    linkml:range okns:string ;
    linkml:slot_uri seegrid-ci:description .

okns:seegrid_ci_edition a linkml:SlotDefinition ;
    dcterms:source <http://def.seegrid.csiro.au/isotc211/iso19115/2003/citation> ;
    dcterms:title "edition" ;
    skos:editorialNote "No occurrences of this slot in the graph." ;
    skos:inScheme okns:seegrid-iso19115 ;
    skos:mappingRelation seegrid-ci:edition ;
    linkml:definition_uri okns:seegrid_ci_edition ;
    linkml:domain okns:Seegrid-ciCitation ;
    linkml:owner okns:seegrid_ci_edition ;
    linkml:range okns:string ;
    linkml:slot_uri seegrid-ci:edition .

okns:seegrid_ci_editionDate a linkml:SlotDefinition ;
    dcterms:source <http://def.seegrid.csiro.au/isotc211/iso19115/2003/citation> ;
    dcterms:title "edition date" ;
    skos:editorialNote "No occurrences of this slot in the graph." ;
    skos:inScheme okns:seegrid-iso19115 ;
    skos:mappingRelation seegrid-ci:editionDate ;
    linkml:definition_uri okns:seegrid_ci_editionDate ;
    linkml:domain okns:Seegrid-ciCitation ;
    linkml:owner okns:seegrid_ci_editionDate ;
    linkml:range okns:date ;
    linkml:slot_uri seegrid-ci:editionDate .

okns:seegrid_ci_electronicMailAddress a linkml:SlotDefinition ;
    dcterms:source <http://def.seegrid.csiro.au/isotc211/iso19115/2003/citation> ;
    dcterms:title "electronic mail address" ;
    skos:editorialNote "No occurrences of this slot in the graph." ;
    skos:inScheme okns:seegrid-iso19115 ;
    skos:mappingRelation seegrid-ci:electronicMailAddress ;
    linkml:definition_uri okns:seegrid_ci_electronicMailAddress ;
    linkml:domain okns:Seegrid-ciAddress ;
    linkml:owner okns:seegrid_ci_electronicMailAddress ;
    linkml:range okns:string ;
    linkml:slot_uri seegrid-ci:electronicMailAddress .

okns:seegrid_ci_facsimile a linkml:SlotDefinition ;
    dcterms:source <http://def.seegrid.csiro.au/isotc211/iso19115/2003/citation> ;
    dcterms:title "facsimile" ;
    skos:editorialNote "No occurrences of this slot in the graph." ;
    skos:inScheme okns:seegrid-iso19115 ;
    skos:mappingRelation seegrid-ci:facsimile ;
    linkml:definition_uri okns:seegrid_ci_facsimile ;
    linkml:domain okns:Seegrid-ciTelephone ;
    linkml:owner okns:seegrid_ci_facsimile ;
    linkml:range okns:string ;
    linkml:slot_uri seegrid-ci:facsimile .

okns:seegrid_ci_function a linkml:SlotDefinition ;
    dcterms:source <http://def.seegrid.csiro.au/isotc211/iso19115/2003/citation> ;
    dcterms:title "function" ;
    skos:editorialNote "No occurrences of this slot in the graph." ;
    skos:inScheme okns:seegrid-iso19115 ;
    skos:mappingRelation seegrid-ci:function ;
    linkml:definition_uri okns:seegrid_ci_function ;
    linkml:domain okns:Seegrid-ciOnlineResource ;
    linkml:inlined true ;
    linkml:owner okns:seegrid_ci_function ;
    linkml:range okns:Seegrid-ciOnLineFunctionCode ;
    linkml:slot_uri seegrid-ci:function .

okns:seegrid_ci_hoursOfService a linkml:SlotDefinition ;
    dcterms:source <http://def.seegrid.csiro.au/isotc211/iso19115/2003/citation> ;
    dcterms:title "hours of service" ;
    skos:editorialNote "No occurrences of this slot in the graph." ;
    skos:inScheme okns:seegrid-iso19115 ;
    skos:mappingRelation seegrid-ci:hoursOfService ;
    linkml:definition_uri okns:seegrid_ci_hoursOfService ;
    linkml:domain okns:Seegrid-ciContact ;
    linkml:owner okns:seegrid_ci_hoursOfService ;
    linkml:range okns:string ;
    linkml:slot_uri seegrid-ci:hoursOfService .

okns:seegrid_ci_identifier a linkml:SlotDefinition ;
    dcterms:source <http://def.seegrid.csiro.au/isotc211/iso19115/2003/citation> ;
    dcterms:title "identifier" ;
    skos:editorialNote "No occurrences of this slot in the graph." ;
    skos:inScheme okns:seegrid-iso19115 ;
    skos:mappingRelation seegrid-ci:identifier ;
    linkml:definition_uri okns:seegrid_ci_identifier ;
    linkml:domain okns:Seegrid-ciCitation ;
    linkml:inlined true ;
    linkml:owner okns:seegrid_ci_identifier ;
    linkml:range okns:Any ;
    linkml:slot_uri seegrid-ci:identifier .

okns:seegrid_ci_individualName a linkml:SlotDefinition ;
    dcterms:source <http://def.seegrid.csiro.au/isotc211/iso19115/2003/citation> ;
    dcterms:title "individual name" ;
    skos:editorialNote "No occurrences of this slot in the graph." ;
    skos:inScheme okns:seegrid-iso19115 ;
    skos:mappingRelation seegrid-ci:individualName ;
    linkml:definition_uri okns:seegrid_ci_individualName ;
    linkml:domain okns:Seegrid-ciResponsibleParty ;
    linkml:owner okns:seegrid_ci_individualName ;
    linkml:range okns:string ;
    linkml:slot_uri seegrid-ci:individualName .

okns:seegrid_ci_issueIdentification a linkml:SlotDefinition ;
    dcterms:source <http://def.seegrid.csiro.au/isotc211/iso19115/2003/citation> ;
    dcterms:title "issue identification" ;
    skos:editorialNote "No occurrences of this slot in the graph." ;
    skos:inScheme okns:seegrid-iso19115 ;
    skos:mappingRelation seegrid-ci:issueIdentification ;
    linkml:definition_uri okns:seegrid_ci_issueIdentification ;
    linkml:domain okns:Seegrid-ciSeries ;
    linkml:inlined true ;
    linkml:owner okns:seegrid_ci_issueIdentification ;
    linkml:range okns:Any ;
    linkml:slot_uri seegrid-ci:issueIdentification .

okns:seegrid_ci_linkage a linkml:SlotDefinition ;
    dcterms:source <http://def.seegrid.csiro.au/isotc211/iso19115/2003/citation> ;
    dcterms:title "linkage" ;
    skos:editorialNote "No occurrences of this slot in the graph." ;
    skos:inScheme okns:seegrid-iso19115 ;
    skos:mappingRelation seegrid-ci:linkage ;
    linkml:definition_uri okns:seegrid_ci_linkage ;
    linkml:domain okns:Seegrid-ciOnlineResource ;
    linkml:inlined true ;
    linkml:owner okns:seegrid_ci_linkage ;
    linkml:range okns:Any ;
    linkml:slot_uri seegrid-ci:linkage .

okns:seegrid_ci_onlineResource a linkml:SlotDefinition ;
    dcterms:source <http://def.seegrid.csiro.au/isotc211/iso19115/2003/citation> ;
    dcterms:title "online resource" ;
    skos:editorialNote "No occurrences of this slot in the graph." ;
    skos:inScheme okns:seegrid-iso19115 ;
    skos:mappingRelation seegrid-ci:onlineResource ;
    linkml:definition_uri okns:seegrid_ci_onlineResource ;
    linkml:domain okns:Seegrid-ciContact ;
    linkml:inlined true ;
    linkml:owner okns:seegrid_ci_onlineResource ;
    linkml:range okns:Seegrid-ciOnlineResource ;
    linkml:slot_uri seegrid-ci:onlineResource .

okns:seegrid_ci_organisationName a linkml:SlotDefinition ;
    dcterms:source <http://def.seegrid.csiro.au/isotc211/iso19115/2003/citation> ;
    dcterms:title "organisation name" ;
    skos:editorialNote "No occurrences of this slot in the graph." ;
    skos:inScheme okns:seegrid-iso19115 ;
    skos:mappingRelation seegrid-ci:organisationName ;
    linkml:definition_uri okns:seegrid_ci_organisationName ;
    linkml:domain okns:Seegrid-ciResponsibleParty ;
    linkml:owner okns:seegrid_ci_organisationName ;
    linkml:range okns:string ;
    linkml:slot_uri seegrid-ci:organisationName .

okns:seegrid_ci_otherCitationDetails a linkml:SlotDefinition ;
    dcterms:source <http://def.seegrid.csiro.au/isotc211/iso19115/2003/citation> ;
    dcterms:title "other citation details" ;
    skos:editorialNote "No occurrences of this slot in the graph." ;
    skos:inScheme okns:seegrid-iso19115 ;
    skos:mappingRelation seegrid-ci:otherCitationDetails ;
    linkml:definition_uri okns:seegrid_ci_otherCitationDetails ;
    linkml:domain okns:Seegrid-ciCitation ;
    linkml:owner okns:seegrid_ci_otherCitationDetails ;
    linkml:range okns:string ;
    linkml:slot_uri seegrid-ci:otherCitationDetails .

okns:seegrid_ci_page a linkml:SlotDefinition ;
    dcterms:source <http://def.seegrid.csiro.au/isotc211/iso19115/2003/citation> ;
    dcterms:title "page" ;
    skos:editorialNote "No occurrences of this slot in the graph." ;
    skos:inScheme okns:seegrid-iso19115 ;
    skos:mappingRelation seegrid-ci:page ;
    linkml:definition_uri okns:seegrid_ci_page ;
    linkml:domain okns:Seegrid-ciSeries ;
    linkml:owner okns:seegrid_ci_page ;
    linkml:range okns:string ;
    linkml:slot_uri seegrid-ci:page .

okns:seegrid_ci_phone a linkml:SlotDefinition ;
    dcterms:source <http://def.seegrid.csiro.au/isotc211/iso19115/2003/citation> ;
    dcterms:title "phone" ;
    skos:editorialNote "No occurrences of this slot in the graph." ;
    skos:inScheme okns:seegrid-iso19115 ;
    skos:mappingRelation seegrid-ci:phone ;
    linkml:definition_uri okns:seegrid_ci_phone ;
    linkml:domain okns:Seegrid-ciContact ;
    linkml:inlined true ;
    linkml:owner okns:seegrid_ci_phone ;
    linkml:range okns:Seegrid-ciTelephone ;
    linkml:slot_uri seegrid-ci:phone .

okns:seegrid_ci_positionName a linkml:SlotDefinition ;
    dcterms:source <http://def.seegrid.csiro.au/isotc211/iso19115/2003/citation> ;
    dcterms:title "position name" ;
    skos:editorialNote "No occurrences of this slot in the graph." ;
    skos:inScheme okns:seegrid-iso19115 ;
    skos:mappingRelation seegrid-ci:positionName ;
    linkml:definition_uri okns:seegrid_ci_positionName ;
    linkml:domain okns:Seegrid-ciResponsibleParty ;
    linkml:owner okns:seegrid_ci_positionName ;
    linkml:range okns:string ;
    linkml:slot_uri seegrid-ci:positionName .

okns:seegrid_ci_postalCode a linkml:SlotDefinition ;
    dcterms:source <http://def.seegrid.csiro.au/isotc211/iso19115/2003/citation> ;
    dcterms:title "postal code" ;
    skos:editorialNote "No occurrences of this slot in the graph." ;
    skos:inScheme okns:seegrid-iso19115 ;
    skos:mappingRelation seegrid-ci:postalCode ;
    linkml:definition_uri okns:seegrid_ci_postalCode ;
    linkml:domain okns:Seegrid-ciAddress ;
    linkml:owner okns:seegrid_ci_postalCode ;
    linkml:range okns:string ;
    linkml:slot_uri seegrid-ci:postalCode .

okns:seegrid_ci_presentationForm a linkml:SlotDefinition ;
    dcterms:source <http://def.seegrid.csiro.au/isotc211/iso19115/2003/citation> ;
    dcterms:title "presentation form" ;
    skos:editorialNote "No occurrences of this slot in the graph." ;
    skos:inScheme okns:seegrid-iso19115 ;
    skos:mappingRelation seegrid-ci:presentationForm ;
    linkml:definition_uri okns:seegrid_ci_presentationForm ;
    linkml:domain okns:Seegrid-ciCitation ;
    linkml:inlined true ;
    linkml:owner okns:seegrid_ci_presentationForm ;
    linkml:range okns:Seegrid-ciPresentationFormCode ;
    linkml:slot_uri seegrid-ci:presentationForm .

okns:seegrid_ci_protocol a linkml:SlotDefinition ;
    dcterms:source <http://def.seegrid.csiro.au/isotc211/iso19115/2003/citation> ;
    dcterms:title "protocol" ;
    skos:editorialNote "No occurrences of this slot in the graph." ;
    skos:inScheme okns:seegrid-iso19115 ;
    skos:mappingRelation seegrid-ci:protocol ;
    linkml:definition_uri okns:seegrid_ci_protocol ;
    linkml:domain okns:Seegrid-ciOnlineResource ;
    linkml:owner okns:seegrid_ci_protocol ;
    linkml:range okns:string ;
    linkml:slot_uri seegrid-ci:protocol .

okns:seegrid_ci_role a linkml:SlotDefinition ;
    dcterms:source <http://def.seegrid.csiro.au/isotc211/iso19115/2003/citation> ;
    dcterms:title "role" ;
    skos:editorialNote "No occurrences of this slot in the graph." ;
    skos:inScheme okns:seegrid-iso19115 ;
    skos:mappingRelation seegrid-ci:role ;
    linkml:definition_uri okns:seegrid_ci_role ;
    linkml:domain okns:Seegrid-ciResponsibleParty ;
    linkml:inlined true ;
    linkml:owner okns:seegrid_ci_role ;
    linkml:range okns:Seegrid-ciRoleCode ;
    linkml:slot_uri seegrid-ci:role .

okns:seegrid_ci_series a linkml:SlotDefinition ;
    dcterms:source <http://def.seegrid.csiro.au/isotc211/iso19115/2003/citation> ;
    dcterms:title "series" ;
    skos:editorialNote "No occurrences of this slot in the graph." ;
    skos:inScheme okns:seegrid-iso19115 ;
    skos:mappingRelation seegrid-ci:series ;
    linkml:definition_uri okns:seegrid_ci_series ;
    linkml:domain okns:Seegrid-ciCitation ;
    linkml:inlined true ;
    linkml:owner okns:seegrid_ci_series ;
    linkml:range okns:Seegrid-ciSeries ;
    linkml:slot_uri seegrid-ci:series .

okns:seegrid_ci_title a linkml:SlotDefinition ;
    dcterms:source <http://def.seegrid.csiro.au/isotc211/iso19115/2003/citation> ;
    dcterms:title "title" ;
    skos:editorialNote "No occurrences of this slot in the graph." ;
    skos:inScheme okns:seegrid-iso19115 ;
    skos:mappingRelation seegrid-ci:title ;
    linkml:definition_uri okns:seegrid_ci_title ;
    linkml:domain okns:Seegrid-ciCitation ;
    linkml:owner okns:seegrid_ci_title ;
    linkml:range okns:string ;
    linkml:slot_uri seegrid-ci:title .

okns:seegrid_ci_voice a linkml:SlotDefinition ;
    dcterms:source <http://def.seegrid.csiro.au/isotc211/iso19115/2003/citation> ;
    dcterms:title "voice" ;
    skos:editorialNote "No occurrences of this slot in the graph." ;
    skos:inScheme okns:seegrid-iso19115 ;
    skos:mappingRelation seegrid-ci:voice ;
    linkml:definition_uri okns:seegrid_ci_voice ;
    linkml:domain okns:Seegrid-ciTelephone ;
    linkml:owner okns:seegrid_ci_voice ;
    linkml:range okns:string ;
    linkml:slot_uri seegrid-ci:voice .

okns:skos_broadMatch a linkml:SlotDefinition ;
    dcterms:source <http://www.w3.org/2004/02/skos/core> ;
    dcterms:title "has broader match" ;
    rdfs:subPropertyOf okns:skos_broader ;
    owl:inverseOf okns:skos_narrowMatch ;
    skos:definition "skos:broadMatch is used to state a hierarchical mapping link between two conceptual resources in different concept schemes." ;
    skos:editorialNote "No occurrences of this slot in the graph." ;
    skos:inScheme okns:skos ;
    skos:mappingRelation skos:broadMatch ;
    linkml:definition_uri okns:skos_broadMatch ;
    linkml:domain okns:Any ;
    linkml:inlined true ;
    linkml:range okns:Any ;
    linkml:slot_uri skos:broadMatch .

okns:skos_closeMatch a linkml:SlotDefinition ;
    dcterms:source <http://www.w3.org/2004/02/skos/core> ;
    dcterms:title "has close match" ;
    rdfs:subPropertyOf okns:skos_mappingRelation ;
    skos:definition "skos:closeMatch is used to link two concepts that are sufficiently similar that they can be used interchangeably in some information retrieval applications. In order to avoid the possibility of \"compound errors\" when combining mappings across more than two concept schemes, skos:closeMatch is not declared to be a transitive property." ;
    skos:editorialNote "No occurrences of this slot in the graph." ;
    skos:inScheme okns:skos ;
    skos:mappingRelation skos:closeMatch ;
    linkml:definition_uri okns:skos_closeMatch ;
    linkml:inlined true ;
    linkml:range okns:Any ;
    linkml:slot_uri skos:closeMatch .

okns:skos_inScheme a linkml:SlotDefinition ;
    dcterms:source <http://www.w3.org/2004/02/skos/core> ;
    dcterms:title "is in scheme" ;
    skos:definition "Relates a resource (for example a concept) to a concept scheme in which it is included." ;
    skos:editorialNote "A concept may be a member of more than one concept scheme.",
        "No occurrences of this slot in the graph." ;
    skos:inScheme okns:skos ;
    skos:mappingRelation skos:inScheme ;
    linkml:definition_uri okns:skos_inScheme ;
    linkml:inlined true ;
    linkml:range okns:SkosConceptScheme ;
    linkml:slot_uri skos:inScheme .

okns:skos_mappingRelation a linkml:SlotDefinition ;
    dcterms:source <http://www.w3.org/2004/02/skos/core> ;
    dcterms:title "is in mapping relation with" ;
    rdfs:subPropertyOf okns:skos_semanticRelation ;
    skos:definition "Relates two concepts coming, by convention, from different schemes, and that have comparable meanings" ;
    skos:editorialNote "No occurrences of this slot in the graph." ;
    skos:inScheme okns:skos ;
    skos:mappingRelation skos:mappingRelation ;
    skos:note "description: These concept mapping relations mirror semantic relations, and the data model defined below is similar (with the exception of skos:exactMatch) to the data model defined for semantic relations. A distinct vocabulary is provided for concept mapping relations, to provide a convenient way to differentiate links within a concept scheme from links between concept schemes. However, this pattern of usage is not a formal requirement of the SKOS data model, and relies on informal definitions of best practice." ;
    linkml:definition_uri okns:skos_mappingRelation ;
    linkml:inlined true ;
    linkml:range okns:Any ;
    linkml:slot_uri skos:mappingRelation .

okns:skos_member a linkml:SlotDefinition ;
    dcterms:source <http://www.w3.org/2004/02/skos/core> ;
    dcterms:title "has member" ;
    skos:definition "Relates a collection to one of its members." ;
    skos:editorialNote "No occurrences of this slot in the graph." ;
    skos:inScheme okns:skos ;
    skos:mappingRelation skos:member ;
    linkml:definition_uri okns:skos_member ;
    linkml:domain okns:SkosCollection ;
    linkml:inlined true ;
    linkml:owner okns:skos_member ;
    linkml:range okns:Any ;
    linkml:slot_uri skos:member .

okns:skos_memberList a linkml:SlotDefinition ;
    dcterms:source <http://www.w3.org/2004/02/skos/core> ;
    dcterms:title "has member list" ;
    skos:definition "Relates an ordered collection to the RDF list containing its members." ;
    skos:editorialNote "No occurrences of this slot in the graph." ;
    skos:inScheme okns:skos ;
    skos:mappingRelation skos:memberList ;
    skos:note """description: For any resource, every item in the list given as the value of the
      skos:memberList property is also a value of the skos:member property.""" ;
    linkml:definition_uri okns:skos_memberList ;
    linkml:domain okns:SkosOrderedCollection ;
    linkml:inlined true ;
    linkml:owner okns:skos_memberList ;
    linkml:range okns:RdfList ;
    linkml:slot_uri skos:memberList .

okns:skos_narrowMatch a linkml:SlotDefinition ;
    dcterms:source <http://www.w3.org/2004/02/skos/core> ;
    dcterms:title "has narrower match" ;
    rdfs:subPropertyOf okns:skos_narrower ;
    owl:inverseOf okns:skos_broadMatch ;
    skos:definition "skos:narrowMatch is used to state a hierarchical mapping link between two conceptual resources in different concept schemes." ;
    skos:editorialNote "No occurrences of this slot in the graph." ;
    skos:inScheme okns:skos ;
    skos:mappingRelation skos:narrowMatch ;
    linkml:definition_uri okns:skos_narrowMatch ;
    linkml:domain okns:Any ;
    linkml:inlined true ;
    linkml:range okns:Any ;
    linkml:slot_uri skos:narrowMatch .

okns:skos_related a linkml:SlotDefinition ;
    dcterms:source <http://www.w3.org/2004/02/skos/core> ;
    dcterms:title "has related" ;
    rdfs:subPropertyOf okns:skos_semanticRelation ;
    skos:definition "Relates a concept to a concept with which there is an associative semantic relationship." ;
    skos:editorialNote "No occurrences of this slot in the graph." ;
    skos:inScheme okns:skos ;
    skos:mappingRelation skos:related ;
    skos:note "description: skos:related is disjoint with skos:broaderTransitive" ;
    linkml:definition_uri okns:skos_related ;
    linkml:inlined true ;
    linkml:range okns:Any ;
    linkml:slot_uri skos:related .

okns:uri a linkml:TypeDefinition ;
    dcterms:conformsTo "https://www.ietf.org/rfc/rfc3987.txt" ;
    skos:closeMatch schema1:URL ;
    skos:definition "a complete URI" ;
    skos:editorialNote "If you are authoring schemas in LinkML YAML, the type is referenced with the lower case \"uri\"." ;
    skos:inScheme linkml:types ;
    skos:note "in RDF serializations a slot with range of uri is treated as a literal or type xsd:anyURI unless it is an identifier or a reference to an identifier, in which case it is translated directly to a node" ;
    linkml:base "URI" ;
    linkml:imported_from "linkml:types" ;
    linkml:repr "str" ;
    linkml:definition_uri linkml:Uri ;
    linkml:uri xsd:anyURI .

okns:DcmitypeImage a linkml:ClassDefinition ;
    dcterms:source dcmitype: ;
    dcterms:title "Image" ;
    skos:definition "Examples include images and photographs of physical objects, paintings, prints, drawings, other images and graphics, animations and moving pictures, film, diagrams, maps, musical notation.  Note that Image may include both electronic and physical representations." ;
    skos:inScheme okns:dc ;
    skos:mappingRelation dcmitype:Image ;
    skos:note "description: A visual representation other than text." ;
    linkml:class_uri dcmitype:Image ;
    linkml:definition_uri okns:DcmitypeImage ;
    linkml:slot_usage [ ] .

okns:DctMediaType a linkml:ClassDefinition ;
    dcterms:source dcterms: ;
    dcterms:title "Media Type" ;
    skos:definition "A file format or physical medium." ;
    skos:inScheme okns:dc ;
    skos:mappingRelation dcterms:MediaType ;
    linkml:class_uri dcterms:MediaType ;
    linkml:definition_uri okns:DctMediaType ;
    linkml:is_a okns:DctMediaTypeOrExtent ;
    linkml:slot_usage [ ] .

okns:DctMediaTypeOrExtent a linkml:ClassDefinition ;
    dcterms:source dcterms: ;
    dcterms:title "Media Type or Extent" ;
    skos:definition "A media type or extent." ;
    skos:inScheme okns:dc ;
    skos:mappingRelation dcterms:MediaTypeOrExtent ;
    linkml:class_uri dcterms:MediaTypeOrExtent ;
    linkml:definition_uri okns:DctMediaTypeOrExtent ;
    linkml:slot_usage [ ] .

okns:HyfHYFlowPath a linkml:ClassDefinition ;
    skos:definition "The HY_Flowpath feature type realizes a catchment specifically as a path connecting the inflow and outflow of the catchment it realizes.␊␊HY_Flowpath specializes HY_CatchmentRealization with respect to an implied linear geometric representation including a straight or curved line. Topologically, the flowpath connects the inflow and outflow of the catchment, and is understood as an edge bounded by an inflow node and an outflow node, and corresponding to left-bank and right-bank catchment faces. Hydrologically, the flowpath is a line describing a moving particle of water.␊␊Through generalization, HY_Flowpath inherits the shape and the realizedCatchment properties. The optional shape of the flowpath is usually a single curve." ;
    skos:inScheme okns:hyf ;
    skos:mappingRelation <hyf:HY_FlowPath> ;
    skos:note "description: The HY_Flowpath feature type realizes a catchment specifically as a path connecting the inflow and outflow of the catchment it realizes. HY_Flowpath specializes HY_CatchmentRealization with respect to an implied linear geometric representation including a straight or curved line. Topologically, the flowpath connects the inflow and outflow of the catchment, and is understood as an edge bounded by an inflow node and an outflow node, and corresponding to left-bank and right-bank catchment faces. Hydrologically, the flowpath is a line describing a moving particle of water.  Through generalization, HY_Flowpath inherits the shape and the realizedCatchment properties. The optional shape of the flowpath is usually a single curve." ;
    linkml:class_uri <https://www.opengis.net/def/schema/hy_features/hyf/HY_FlowPath> ;
    linkml:definition_uri okns:HyfHYFlowPath ;
    linkml:is_a okns:HyfHYCatchmentRealization ;
    linkml:slot_usage [ ] .

okns:HyfHYHydroFeature a linkml:ClassDefinition ;
    skos:definition "basic feature to reflect the properties that all hydrologic features have." ;
    skos:inScheme okns:hyf ;
    skos:mappingRelation <hyf:HY_HydroFeature> ;
    linkml:class_uri <https://www.opengis.net/def/schema/hy_features/hyf/HY_HydroFeature> ;
    linkml:definition_uri okns:HyfHYHydroFeature ;
    linkml:slot_usage [ ] .

okns:HyfHYHydroFeatureName a linkml:ClassDefinition ;
    skos:definition "pattern to handle cultural, political and historical variability of names. This supports the assignment of a referenceable name for all or parts of a hydrologic feature without necessarily having a formal model for the naming." ;
    skos:inScheme okns:hyf ;
    skos:mappingRelation <hyf:HY_HydroFeatureName> ;
    linkml:class_uri <https://www.opengis.net/def/schema/hy_features/hyf/HY_HydroFeatureName> ;
    linkml:definition_uri okns:HyfHYHydroFeatureName ;
    linkml:slot_usage [ ] .

okns:RdfCompoundLiteral a linkml:ClassDefinition ;
    dcterms:source rdf: ;
    dcterms:title "CompoundLiteral" ;
    rdfs:seeAlso <https://www.w3.org/TR/json-ld11/#the-rdf-compoundliteral-class-and-the-rdf-language-and-rdf-direction-properties> ;
    skos:definition "A class representing a compound literal." ;
    skos:inScheme okns:owl-rdf-rdfs ;
    skos:mappingRelation rdf:CompoundLiteral ;
    linkml:class_uri rdf:CompoundLiteral ;
    linkml:definition_uri okns:RdfCompoundLiteral ;
    linkml:is_a okns:RdfsResource ;
    linkml:slot_usage [ ] .

okns:Seegrid-basicVector a linkml:ClassDefinition ;
    dcterms:source <http://def.seegrid.csiro.au/isotc211/iso19103/2005/basic> ;
    dcterms:title "Vector" ;
    skos:definition "A vector is a sequence of a fixed length of Numbers. Normally, the numbers represent some measures, and thus vectors are often used where records of Numbers would be more appropriate. In geometry for example, direct positions are given by undistinguished coordinate vectors, which can be interpreted through the use of coordinate reference systems." ;
    skos:inScheme okns:seegrid-iso19115 ;
    skos:mappingRelation seegrid-basic:Vector ;
    linkml:class_uri seegrid-basic:Vector ;
    linkml:definition_uri okns:Seegrid-basicVector ;
    linkml:slot_usage [ ] .

okns:SkosCollection a linkml:ClassDefinition ;
    dcterms:source <http://www.w3.org/2004/02/skos/core> ;
    dcterms:title "Collection" ;
    skos:definition "A meaningful collection of concepts." ;
    skos:editorialNote "Labelled collections can be used where you would like a set of concepts to be displayed under a 'node label' in the hierarchy." ;
    skos:inScheme okns:skos ;
    skos:mappingRelation skos:Collection ;
    linkml:class_uri skos:Collection ;
    linkml:definition_uri okns:SkosCollection ;
    linkml:slot_usage [ ] .

okns:boolean a linkml:TypeDefinition ;
    skos:definition "A binary (true or false) value" ;
    skos:editorialNote "If you are authoring schemas in LinkML YAML, the type is referenced with the lower case \"boolean\"." ;
    skos:exactMatch schema1:Boolean ;
    skos:inScheme linkml:types ;
    linkml:base "Bool" ;
    linkml:imported_from "linkml:types" ;
    linkml:repr "bool" ;
    linkml:definition_uri linkml:Boolean ;
    linkml:uri xsd:boolean .

okns:dct_audience a linkml:SlotDefinition ;
    dcterms:source dcterms: ;
    dcterms:title "Audience" ;
    skos:definition "Recommended practice is to use this property with non-literal values from a vocabulary of audience types." ;
    skos:editorialNote "No occurrences of this slot in the graph." ;
    skos:inScheme okns:dc ;
    skos:mappingRelation dcterms:audience ;
    skos:note "description: A class of agents for whom the resource is intended or useful." ;
    linkml:definition_uri okns:dct_audience ;
    linkml:inlined true ;
    linkml:range okns:Any ;
    linkml:slot_uri dcterms:audience .

okns:dct_coverage a linkml:SlotDefinition ;
    dcterms:source dcterms: ;
    dcterms:title "Coverage" ;
    rdfs:subPropertyOf okns:dc_coverage ;
    skos:definition "Spatial topic and spatial applicability may be a named place or a location specified by its geographic coordinates. Temporal topic may be a named period, date, or date range. A jurisdiction may be a named administrative entity or a geographic place to which the resource applies. Recommended practice is to use a controlled vocabulary such as the Getty Thesaurus of Geographic Names [[TGN](https://www.getty.edu/research/tools/vocabulary/tgn/index.html)]. Where appropriate, named places or time periods may be used in preference to numeric identifiers such as sets of coordinates or date ranges.  Because coverage is so broadly defined, it is preferable to use the more specific subproperties Temporal Coverage and Spatial Coverage." ;
    skos:editorialNote "No occurrences of this slot in the graph." ;
    skos:inScheme okns:dc ;
    skos:mappingRelation dcterms:coverage ;
    skos:note "description: The spatial or temporal topic of the resource, spatial applicability of the resource, or jurisdiction under which the resource is relevant." ;
    linkml:definition_uri okns:dct_coverage ;
    linkml:inlined true ;
    linkml:range okns:Any ;
    linkml:slot_uri dcterms:coverage .

okns:dct_description a linkml:SlotDefinition ;
    dcterms:source dcterms: ;
    dcterms:title "Description" ;
    rdfs:subPropertyOf okns:dc_description ;
    skos:definition "Description may include but is not limited to: an abstract, a table of contents, a graphical representation, or a free-text account of the resource." ;
    skos:inScheme okns:dc ;
    skos:mappingRelation dcterms:description ;
    skos:note "description: An account of the resource." ;
    linkml:definition_uri okns:dct_description ;
    linkml:range okns:string ;
    linkml:slot_uri dcterms:description .

okns:dct_format a linkml:SlotDefinition ;
    dcterms:source dcterms: ;
    dcterms:title "Format" ;
    rdfs:subPropertyOf okns:dc_format ;
    skos:definition "Recommended practice is to use a controlled vocabulary where available. For example, for file formats one could use the list of Internet Media Types [[MIME](https://www.iana.org/assignments/media-types/media-types.xhtml)].  Examples of dimensions include size and duration." ;
    skos:editorialNote "No occurrences of this slot in the graph." ;
    skos:inScheme okns:dc ;
    skos:mappingRelation dcterms:format ;
    skos:note "description: The file format, physical medium, or dimensions of the resource." ;
    linkml:definition_uri okns:dct_format ;
    linkml:inlined true ;
    linkml:range okns:Any ;
    linkml:slot_uri dcterms:format .

okns:dct_issued a linkml:SlotDefinition ;
    dcterms:source dcterms: ;
    dcterms:title "Date Issued" ;
    rdfs:subPropertyOf okns:dct_date ;
    skos:definition "Recommended practice is to describe the date, date/time, or period of time as recommended for the property Date, of which this is a subproperty." ;
    skos:inScheme okns:dc ;
    skos:mappingRelation dcterms:issued ;
    skos:note "description: Date of formal issuance of the resource." ;
    linkml:any_of [ a okns:AnonymousSlotExpression ;
            linkml:range okns:RdfsLiteral ],
        [ a okns:AnonymousSlotExpression ;
            linkml:range okns:date ] ;
    linkml:definition_uri okns:dct_issued ;
    linkml:domain_of okns:DcamVocabularyEncodingScheme,
        okns:DctAgentClass ;
    linkml:inlined true ;
    linkml:owner okns:DctAgentClass ;
    linkml:range okns:Any ;
    linkml:slot_uri dcterms:issued .

okns:dct_rights a linkml:SlotDefinition ;
    dcterms:source dcterms: ;
    dcterms:title "Rights" ;
    rdfs:subPropertyOf okns:dc_rights ;
    skos:definition "Typically, rights information includes a statement about various property rights associated with the resource, including intellectual property rights.  Recommended practice is to refer to a rights statement with a URI.  If this is not possible or feasible, a literal value (name, label, or short text) may be provided." ;
    skos:editorialNote "No occurrences of this slot in the graph." ;
    skos:inScheme okns:dc ;
    skos:mappingRelation dcterms:rights ;
    skos:note "description: Information about rights held in and over the resource." ;
    linkml:definition_uri okns:dct_rights ;
    linkml:inlined true ;
    linkml:range okns:Any ;
    linkml:slot_uri dcterms:rights .

okns:float a linkml:TypeDefinition ;
    skos:definition "A real number that conforms to the xsd:float specification" ;
    skos:editorialNote "If you are authoring schemas in LinkML YAML, the type is referenced with the lower case \"float\"." ;
    skos:exactMatch schema1:Float ;
    skos:inScheme linkml:types ;
    linkml:base "float" ;
    linkml:imported_from "linkml:types" ;
    linkml:definition_uri linkml:Float ;
    linkml:uri xsd:float .

okns:rdf_value a linkml:SlotDefinition ;
    dcterms:source rdf: ;
    dcterms:title "value" ;
    skos:definition "Idiomatic property used for structured values." ;
    skos:editorialNote "No occurrences of this slot in the graph." ;
    skos:inScheme okns:owl-rdf-rdfs ;
    skos:mappingRelation rdf:value ;
    linkml:definition_uri okns:rdf_value ;
    linkml:domain okns:RdfsResource ;
    linkml:inlined true ;
    linkml:owner okns:rdf_value ;
    linkml:range okns:RdfsResource ;
    linkml:slot_uri rdf:value .

okns:skos_broader a linkml:SlotDefinition ;
    dcterms:source <http://www.w3.org/2004/02/skos/core> ;
    dcterms:title "has broader" ;
    rdfs:subPropertyOf okns:skos_broaderTransitive ;
    owl:inverseOf okns:skos_narrower ;
    skos:definition "Relates a concept to a concept that is more general in meaning." ;
    skos:editorialNote "By convention, skos:broader is only used to assert an immediate (i.e. direct) hierarchical link between two conceptual resources.",
        "No occurrences of this slot in the graph." ;
    skos:inScheme okns:skos ;
    skos:mappingRelation skos:broader ;
    skos:note "description: Broader concepts are typically rendered as parents in a concept hierarchy (tree)." ;
    linkml:definition_uri okns:skos_broader ;
    linkml:domain okns:Any ;
    linkml:inlined true ;
    linkml:range okns:Any ;
    linkml:slot_uri skos:broader .

okns:skos_broaderTransitive a linkml:SlotDefinition ;
    dcterms:source <http://www.w3.org/2004/02/skos/core> ;
    dcterms:title "has broader transitive" ;
    rdfs:subPropertyOf okns:skos_semanticRelation ;
    owl:inverseOf okns:skos_narrowerTransitive ;
    skos:definition "skos:broaderTransitive is a transitive superproperty of skos:broader." ;
    skos:editorialNote "By convention, skos:broaderTransitive is not used to make assertions. Rather, the properties can be used to draw inferences about the transitive closure of the hierarchical relation, which is useful e.g. when implementing a simple query expansion algorithm in a search application.",
        "No occurrences of this slot in the graph." ;
    skos:inScheme okns:skos ;
    skos:mappingRelation skos:broaderTransitive ;
    linkml:definition_uri okns:skos_broaderTransitive ;
    linkml:domain okns:Any ;
    linkml:inlined true ;
    linkml:range okns:Any ;
    linkml:slot_uri skos:broaderTransitive .

okns:skos_hasTopConcept a linkml:SlotDefinition ;
    dcterms:source <http://www.w3.org/2004/02/skos/core> ;
    dcterms:title "has top concept" ;
    owl:inverseOf okns:skos_topConceptOf ;
    skos:definition "Relates, by convention, a concept scheme to a concept which is topmost in the broader/narrower concept hierarchies for that scheme, providing an entry point to these hierarchies." ;
    skos:editorialNote "No occurrences of this slot in the graph." ;
    skos:inScheme okns:skos ;
    skos:mappingRelation skos:hasTopConcept ;
    linkml:definition_uri okns:skos_hasTopConcept ;
    linkml:domain okns:SkosConceptScheme ;
    linkml:inlined true ;
    linkml:owner okns:skos_hasTopConcept ;
    linkml:range okns:SkosConcept ;
    linkml:slot_uri skos:hasTopConcept .

okns:skos_narrower a linkml:SlotDefinition ;
    dcterms:source <http://www.w3.org/2004/02/skos/core> ;
    dcterms:title "has narrower" ;
    rdfs:subPropertyOf okns:skos_narrowerTransitive ;
    owl:inverseOf okns:skos_broader ;
    skos:definition "Relates a concept to a concept that is more specific in meaning." ;
    skos:editorialNote "By convention, skos:broader is only used to assert an immediate (i.e. direct) hierarchical link between two conceptual resources.",
        "No occurrences of this slot in the graph." ;
    skos:inScheme okns:skos ;
    skos:mappingRelation skos:narrower ;
    skos:note "description: Narrower concepts are typically rendered as children in a concept hierarchy (tree)." ;
    linkml:definition_uri okns:skos_narrower ;
    linkml:domain okns:Any ;
    linkml:inlined true ;
    linkml:range okns:Any ;
    linkml:slot_uri skos:narrower .

okns:skos_narrowerTransitive a linkml:SlotDefinition ;
    dcterms:source <http://www.w3.org/2004/02/skos/core> ;
    dcterms:title "has narrower transitive" ;
    rdfs:subPropertyOf okns:skos_semanticRelation ;
    owl:inverseOf okns:skos_broaderTransitive ;
    skos:definition "skos:narrowerTransitive is a transitive superproperty of skos:narrower." ;
    skos:editorialNote "By convention, skos:narrowerTransitive is not used to make assertions. Rather, the properties can be used to draw inferences about the transitive closure of the hierarchical relation, which is useful e.g. when implementing a simple query expansion algorithm in a search application.",
        "No occurrences of this slot in the graph." ;
    skos:inScheme okns:skos ;
    skos:mappingRelation skos:narrowerTransitive ;
    linkml:definition_uri okns:skos_narrowerTransitive ;
    linkml:domain okns:Any ;
    linkml:inlined true ;
    linkml:range okns:Any ;
    linkml:slot_uri skos:narrowerTransitive .

okns:skos_topConceptOf a linkml:SlotDefinition ;
    dcterms:source <http://www.w3.org/2004/02/skos/core> ;
    dcterms:title "is top concept in scheme" ;
    rdfs:subPropertyOf okns:skos_inScheme ;
    owl:inverseOf okns:skos_hasTopConcept ;
    skos:definition "Relates a concept to the concept scheme that it is a top level concept of." ;
    skos:editorialNote "No occurrences of this slot in the graph." ;
    skos:inScheme okns:skos ;
    skos:mappingRelation skos:topConceptOf ;
    linkml:definition_uri okns:skos_topConceptOf ;
    linkml:domain okns:SkosConcept ;
    linkml:inlined true ;
    linkml:owner okns:skos_topConceptOf ;
    linkml:range okns:SkosConceptScheme ;
    linkml:slot_uri skos:topConceptOf .

okns:token a linkml:TypeDefinition ;
    skos:definition "Tokenized string, one that does not contain the carriage return (#xD), line feed (#xA) nor tab (#x9) characters, that has no leading or trailing spaces (#x20) and that has no internal sequences of two or more spaces." ;
    skos:inScheme okns:extended_types ;
    skos:note "added by Mahir Morshed <mmorshed@scripps.edu>" ;
    linkml:base "str" ;
    linkml:definition_uri linkml:Token ;
    linkml:typeof okns:normalizedstring ;
    linkml:uri xsd:token .

okns:DcmitypeCollection a linkml:ClassDefinition ;
    dcterms:source dcmitype: ;
    dcterms:title "Collection" ;
    skos:definition "A collection is described as a group; its parts may also be separately described." ;
    skos:inScheme okns:dc ;
    skos:mappingRelation dcmitype:Collection ;
    skos:note "description: An aggregation of resources." ;
    linkml:class_uri dcmitype:Collection ;
    linkml:definition_uri okns:DcmitypeCollection ;
    linkml:slot_usage [ ] .

okns:DctLocationPeriodOrJurisdiction a linkml:ClassDefinition ;
    dcterms:source dcterms: ;
    dcterms:title "Location, Period, or Jurisdiction" ;
    skos:definition "A location, period of time, or jurisdiction." ;
    skos:inScheme okns:dc ;
    skos:mappingRelation dcterms:LocationPeriodOrJurisdiction ;
    linkml:class_uri dcterms:LocationPeriodOrJurisdiction ;
    linkml:definition_uri okns:DctLocationPeriodOrJurisdiction ;
    linkml:slot_usage [ ] .

okns:HyfHYHydroLocation a linkml:ClassDefinition ;
    dcterms:title "ReferenceLocation" ;
    skos:definition "The HY_HydroLocation feature type (Figure 35) conceptualizes the idea that a hydro nexus can be realized by practically any feature of interest. The hydro nexus concept is used to define the hydrologic determination of a catchment but, like the catchment concept, does not have inherent realization(s). Any hydrologically significant feature that can be identified as (said to be) the outlet of a catchment may realize the hydro nexus. Typically, this will be a permanent, stable location that is fixed and/or referenced by coordinates.␊␊Landmarks such as confluences, points corresponding to vertical sections, or the position of a monitoring station on a river are typical realizations of the hydro nexus. Other kinds of hydro nexus realizations that don't carry normal surface water characteristics as defined in this standard, e.g. a spring where groundwater enters the surface, an arbitrary point projected onto the surface, or a nexus that collects many disjoint locations may use or specialize the general HY_HydroLocation type.␊␊Topologically, the HY_HydroLocation should be understood to be the boundary of the corresponding catchment, and always of lower topological dimension than the catchment. Even though the topological realization of a hydro nexus is typically as a node between catchment edges, a nexus realization may also have any geometric representation, including a single point.␊␊In many cases, HY_HydroLocations are known but corresponding catchments and hydro nexuses are not defined. For example, stream gages that are part of a catchment dataset whose hydro nexus features are realized by confluences. Both the stream gages and confluences are HY_HydroLocations, but the stream gages’ hydro nexus features are not defined. Using this concept, HY_HydroLocation is expected to be used to link between datasets that have catchments delineated for different HY_HydroLocations.␊␊HY_HydroLocation carries two attributes: shape and hydroLocationType. It has referencedPosition and realizedNexus associations implying the hydro-complex feature collection." ;
    skos:inScheme okns:hyf ;
    skos:mappingRelation <hyf:HY_HydroLocation> ;
    skos:note "description: The HY_HydroLocation feature type (Figure 35) conceptualizes the idea that a hydro nexus can be realized by practically any feature of interest. The hydro nexus concept is used to define the hydrologic determination of a catchment but, like the catchment concept, does not have inherent realization(s). Any hydrologically significant feature that can be identified as (said to be) the outlet of a catchment may realize the hydro nexus. Typically, this will be a permanent, stable location that is fixed and/or referenced by coordinates.  Landmarks such as confluences, points corresponding to vertical sections, or the position of a monitoring station on a river are typical realizations of the hydro nexus. Other kinds of hydro nexus realizations that don't carry normal surface water characteristics as defined in this standard, e.g. a spring where groundwater enters the surface, an arbitrary point projected onto the surface, or a nexus that collects many disjoint locations may use or specialize the general HY_HydroLocation type.  Topologically, the HY_HydroLocation should be understood to be the boundary of the corresponding catchment, and always of lower topological dimension than the catchment. Even though the topological realization of a hydro nexus is typically as a node between catchment edges, a nexus realization may also have any geometric representation, including a single point. In many cases, HY_HydroLocations are known but corresponding catchments and hydro nexuses are not defined. For example, stream gages that are part of a catchment dataset whose hydro nexus features are realized by confluences. Both the stream gages and confluences are HY_HydroLocations, but the stream gages’ hydro nexus features are not defined. Using this concept, HY_HydroLocation is expected to be used to link between datasets that have catchments delineated for different HY_HydroLocations. HY_HydroLocation carries two attributes: shape and hydroLocationType. It has referencedPosition and realizedNexus associations implying the hydro-complex feature collection." ;
    linkml:class_uri <https://www.opengis.net/def/schema/hy_features/hyf/HY_HydroLocation> ;
    linkml:definition_uri okns:HyfHYHydroLocation ;
    linkml:slot_usage [ ] .

okns:HyfHYHydroNexus a linkml:ClassDefinition ;
    skos:definition "The HY_HydroNexus feature type (Figure 33) conceptualizes a hydrologically determined nexus of a corresponding catchment (Figure 26). The hydro nexus represents the place where a catchment interacts with another catchment, i.e. where the outflow of a contributing catchment becomes inflow into a receiving catchment. A catchment may receive flow from several upstream catchments or contribute flow to several downstream catchments through a single hydro nexus. Through shared identity, each hydro nexus feature may be associated with different realizations within a hydrologic complex given that each realization has the same hydrologic function or characteristics. This includes the topological realization as a node on the one-dimensional flowpath (edge) in terms of a topological 'boundary'.␊␊Placed topologically relative to a catchment which links inflow and outflow, a hydro nexus has a position relative to another hydro nexus that is 'fixed' in the network by the catchments it is associated with. Additionally, the union of catchment and hydro nexus(es) can be used to define a linear river reference system, where an inflow or outflow node is the origin and the flowpath realizing the catchment is the linear element along which a position can be determined." ;
    skos:inScheme okns:hyf ;
    skos:mappingRelation <hyf:HY_HydroNexus> ;
    skos:note "description: The HY_HydroNexus feature type (Figure 33) conceptualizes a hydrologically determined nexus of a corresponding catchment (Figure 26). The hydro nexus represents the place where a catchment interacts with another catchment, i.e. where the outflow of a contributing catchment becomes inflow into a receiving catchment. A catchment may receive flow from several upstream catchments or contribute flow to several downstream catchments through a single hydro nexus. Through shared identity, each hydro nexus feature may be associated with different realizations within a hydrologic complex given that each realization has the same hydrologic function or characteristics. This includes the topological realization as a node on the one-dimensional flowpath (edge) in terms of a topological 'boundary'.  Placed topologically relative to a catchment which links inflow and outflow, a hydro nexus has a position relative to another hydro nexus that is 'fixed' in the network by the catchments it is associated with. Additionally, the union of catchment and hydro nexus(es) can be used to define a linear river reference system, where an inflow or outflow node is the origin and the flowpath realizing the catchment is the linear element along which a position can be determined." ;
    linkml:class_uri <https://www.opengis.net/def/schema/hy_features/hyf/HY_HydroNexus> ;
    linkml:definition_uri okns:HyfHYHydroNexus ;
    linkml:slot_usage [ ] .

okns:RdfStatement a linkml:ClassDefinition ;
    dcterms:source rdf: ;
    dcterms:title "Statement" ;
    skos:definition "The class of RDF statements." ;
    skos:inScheme okns:owl-rdf-rdfs ;
    skos:mappingRelation rdf:Statement ;
    linkml:class_uri rdf:Statement ;
    linkml:definition_uri okns:RdfStatement ;
    linkml:is_a okns:RdfsResource ;
    linkml:slot_usage [ ] .

okns:RdfsContainer a linkml:ClassDefinition ;
    dcterms:source rdfs: ;
    dcterms:title "Container" ;
    skos:definition "The class of RDF containers." ;
    skos:inScheme okns:owl-rdf-rdfs ;
    skos:mappingRelation rdfs:Container ;
    linkml:class_uri rdfs:Container ;
    linkml:definition_uri okns:RdfsContainer ;
    linkml:is_a okns:RdfsResource ;
    linkml:slot_usage [ ] .

okns:Seegrid-ciDate a linkml:ClassDefinition ;
    dcterms:source <http://def.seegrid.csiro.au/isotc211/iso19115/2003/citation> ;
    dcterms:title "Date" ;
    skos:altLabel "CI_Date" ;
    skos:inScheme okns:seegrid-iso19115 ;
    skos:mappingRelation seegrid-ci:Date ;
    linkml:class_uri seegrid-ci:Date ;
    linkml:definition_uri okns:Seegrid-ciDate ;
    linkml:is_a <https://purl.org/okn/schema/HttpDef.seegrid.csiro.auIsotc211Iso191502012Hm2owl#DataType> ;
    linkml:slot_usage [ ] .

okns:Seegrid-ciSeries a linkml:ClassDefinition ;
    dcterms:source <http://def.seegrid.csiro.au/isotc211/iso19115/2003/citation> ;
    dcterms:title "Series" ;
    skos:altLabel "CI_Series" ;
    skos:inScheme okns:seegrid-iso19115 ;
    skos:mappingRelation seegrid-ci:Series ;
    linkml:class_uri seegrid-ci:Series ;
    linkml:definition_uri okns:Seegrid-ciSeries ;
    linkml:is_a <https://purl.org/okn/schema/HttpDef.seegrid.csiro.auIsotc211Iso191502012Hm2owl#DataType> ;
    linkml:slot_usage [ ] .

okns:Seegrid-ciTelephone a linkml:ClassDefinition ;
    dcterms:source <http://def.seegrid.csiro.au/isotc211/iso19115/2003/citation> ;
    dcterms:title "Telephone" ;
    skos:altLabel "CI_Telephone" ;
    skos:inScheme okns:seegrid-iso19115 ;
    skos:mappingRelation seegrid-ci:Telephone ;
    linkml:class_uri seegrid-ci:Telephone ;
    linkml:definition_uri okns:Seegrid-ciTelephone ;
    linkml:is_a <https://purl.org/okn/schema/HttpDef.seegrid.csiro.auIsotc211Iso191502012Hm2owl#DataType> ;
    linkml:slot_usage [ ] .

okns:SkosConceptScheme a linkml:ClassDefinition ;
    dcterms:source <http://www.w3.org/2004/02/skos/core> ;
    dcterms:title "Concept Scheme" ;
    skos:definition "A set of concepts, optionally including statements about semantic relationships between those concepts." ;
    skos:editorialNote "A concept scheme may be defined to include concepts from different sources." ;
    skos:inScheme okns:skos ;
    skos:mappingRelation skos:ConceptScheme ;
    linkml:class_uri skos:ConceptScheme ;
    linkml:definition_uri okns:SkosConceptScheme ;
    linkml:slot_usage [ ] .

okns:date a linkml:TypeDefinition ;
    skos:definition "a date (year, month and day) in an idealized calendar" ;
    skos:editorialNote "If you are authoring schemas in LinkML YAML, the type is referenced with the lower case \"date\".",
        "URI is dateTime because OWL reasoners don't work with straight date or time" ;
    skos:exactMatch schema1:Date ;
    skos:inScheme linkml:types ;
    linkml:base "XSDDate" ;
    linkml:imported_from "linkml:types" ;
    linkml:repr "str" ;
    linkml:definition_uri linkml:Date ;
    linkml:uri xsd:date .

okns:rdfs_subClassOf a linkml:SlotDefinition ;
    dcterms:source rdfs: ;
    dcterms:title "subClassOf" ;
    skos:definition "The subject is a subclass of a class." ;
    skos:inScheme okns:owl-rdf-rdfs ;
    skos:mappingRelation rdfs:subClassOf ;
    linkml:definition_uri okns:rdfs_subClassOf ;
    linkml:domain okns:RdfsClass ;
    linkml:domain_of okns:RdfsDatatype ;
    linkml:inlined true ;
    linkml:owner okns:rdfs_subClassOf ;
    linkml:range okns:RdfsClass ;
    linkml:slot_uri rdfs:subClassOf .

okns:signedinteger a linkml:TypeDefinition ;
    rdfs:seeAlso <https://numpy.org/doc/stable/reference/arrays.scalars.html#numpy.signedinteger> ;
    skos:definition "An integer that may be negative" ;
    skos:inScheme okns:extended_types ;
    linkml:base "int" ;
    linkml:definition_uri linkml:Signedinteger ;
    linkml:typeof okns:integer ;
    linkml:uri xsd:integer .

okns:OwlNegativePropertyAssertion a linkml:ClassDefinition ;
    dcterms:source owl: ;
    dcterms:title "NegativePropertyAssertion" ;
    skos:definition "The class of negative property assertions." ;
    skos:inScheme okns:owl-rdf-rdfs ;
    skos:mappingRelation owl:NegativePropertyAssertion ;
    linkml:class_uri owl:NegativePropertyAssertion ;
    linkml:definition_uri okns:OwlNegativePropertyAssertion ;
    linkml:is_a okns:RdfsResource ;
    linkml:slot_usage [ ] .

okns:integer a linkml:TypeDefinition ;
    skos:definition "An integer" ;
    skos:editorialNote "If you are authoring schemas in LinkML YAML, the type is referenced with the lower case \"integer\"." ;
    skos:exactMatch schema1:Integer ;
    skos:inScheme linkml:types ;
    linkml:base "int" ;
    linkml:imported_from "linkml:types" ;
    linkml:definition_uri linkml:Integer ;
    linkml:uri xsd:integer .

okns:DctAgentClass a linkml:ClassDefinition ;
    dcterms:source dcterms: ;
    dcterms:title "Agent Class" ;
    skos:definition "A group of agents." ;
    skos:inScheme okns:dc ;
    skos:mappingRelation dcterms:AgentClass ;
    linkml:class_uri dcterms:AgentClass ;
    linkml:definition_uri okns:DctAgentClass ;
    linkml:is_a okns:RdfsClass ;
    linkml:slot_usage [ ] ;
    linkml:slots okns:dct_issued,
        okns:rdfs_comment,
        okns:rdfs_isDefinedBy,
        okns:rdfs_label .

okns:rdfs_seeAlso a linkml:SlotDefinition ;
    dcterms:source rdfs: ;
    dcterms:title "seeAlso" ;
    skos:definition "Further information about the subject resource." ;
    skos:inScheme okns:owl-rdf-rdfs ;
    skos:mappingRelation rdfs:seeAlso ;
    linkml:any_of [ a okns:AnonymousSlotExpression ;
            linkml:range okns:RdfsResource ],
        [ a okns:AnonymousSlotExpression ;
            linkml:range okns:uri ] ;
    linkml:definition_uri okns:rdfs_seeAlso ;
    linkml:domain okns:RdfsResource ;
    linkml:domain_of okns:DcamVocabularyEncodingScheme,
        okns:RdfsDatatype ;
    linkml:inlined true ;
    linkml:owner okns:rdfs_seeAlso ;
    linkml:range okns:Any ;
    linkml:slot_uri rdfs:seeAlso .

okns:skos_semanticRelation a linkml:SlotDefinition ;
    dcterms:source <http://www.w3.org/2004/02/skos/core> ;
    dcterms:title "is in semantic relation with" ;
    skos:definition "Links a concept to a concept related by meaning." ;
    skos:editorialNote "No occurrences of this slot in the graph.",
        "This property should not be used directly, but as a super-property for all properties denoting a relationship of meaning between concepts." ;
    skos:inScheme okns:skos ;
    skos:mappingRelation skos:semanticRelation ;
    linkml:definition_uri okns:skos_semanticRelation ;
    linkml:domain okns:SkosConcept ;
    linkml:inlined true ;
    linkml:owner okns:skos_semanticRelation ;
    linkml:range okns:SkosConcept ;
    linkml:slot_uri skos:semanticRelation .

okns:DcamVocabularyEncodingScheme a linkml:ClassDefinition ;
    dcterms:source dcam: ;
    dcterms:title "Vocabulary Encoding Scheme" ;
    rdfs:seeAlso <https://www.dublincore.org/specifications/dublin-core/2007/06/04/abstract-model/> ;
    skos:definition "An enumerated set of resources." ;
    skos:inScheme okns:dc ;
    skos:mappingRelation dcam:VocabularyEncodingScheme ;
    linkml:class_uri dcam:VocabularyEncodingScheme ;
    linkml:definition_uri okns:DcamVocabularyEncodingScheme ;
    linkml:slot_usage [ ] ;
    linkml:slots okns:dct_issued,
        okns:rdfs_comment,
        okns:rdfs_isDefinedBy,
        okns:rdfs_label,
        okns:rdfs_seeAlso .

okns:HyfHYCatchmentRealization a linkml:ClassDefinition ;
    dcterms:title "No class (entity type) name specified -- this class is noted as a superclass of another class in this graph but has not itself been defined." ;
    skos:definition "The HY_CatchmentRealization feature type (Figure 34) is based on the idea that there are multiple hydrology-specific perspectives of the holistic catchment concept that are used to describe a catchment as a unit of study shared across sub-domains and studies.␊␊A given catchment realization exists within a hydrologic complex in that, if a catchment realization exists, it exists in the same hydrologic complex as the catchment it realizes. In this way, any realization of a catchment has the same hydrologic determination of the catchment it realizes. If a catchment is connected with other catchments via inflow and/or outflow hydro nexuses, its realizations are also connected. A realization of the logical catchment is always of higher topological dimension than the realization of the corresponding hydro nexus topological boundary. For example, a linear flowpath realizing a catchment may be understood as an edge between inflow and outflow nodes; the areal realization of a catchment as a face bounded by linear inflow and outflow.␊␊The catchment realization features defined in this standard refer to objects on the land surface for the purpose of surface water hydrology. In other contexts, other types of catchment realization may exist. Catchment realizations that do not conform to those defined in this standard, for instance realizations in 3- or 4-dimensional perspectives, may be implemented using the general HY_CatchmentRealization type. HY_CatchmentRealization carries a shape attribute and as a realizedCatchment association." ;
    skos:inScheme okns:hyf ;
    skos:mappingRelation <hyf:HY_CatchmentRealization> ;
    skos:note "description: The HY_CatchmentRealization feature type (Figure 34) is based on the idea that there are multiple hydrology-specific perspectives of the holistic catchment concept that are used to describe a catchment as a unit of study shared across sub-domains and studies.  A given catchment realization exists within a hydrologic complex in that, if a catchment realization exists, it exists in the same hydrologic complex as the catchment it realizes. In this way, any realization of a catchment has the same hydrologic determination of the catchment it realizes. If a catchment is connected with other catchments via inflow and/or outflow hydro nexuses, its realizations are also connected. A realization of the logical catchment is always of higher topological dimension than the realization of the corresponding hydro nexus topological boundary. For example, a linear flowpath realizing a catchment may be understood as an edge between inflow and outflow nodes; the areal realization of a catchment as a face bounded by linear inflow and outflow. The catchment realization features defined in this standard refer to objects on the land surface for the purpose of surface water hydrology. In other contexts, other types of catchment realization may exist. Catchment realizations that do not conform to those defined in this standard, for instance realizations in 3- or 4-dimensional perspectives, may be implemented using the general HY_CatchmentRealization type. HY_CatchmentRealization carries a shape attribute and as a realizedCatchment association." ;
    linkml:class_uri <https://www.opengis.net/def/schema/hy_features/hyf/HY_CatchmentRealization> ;
    linkml:definition_uri okns:HyfHYCatchmentRealization ;
    linkml:slot_usage [ ] .

okns:HyfHYWaterBody a linkml:ClassDefinition ;
    dcterms:title "No class (entity type) name specified -- this class is noted as a superclass of another class in this graph but has not itself been defined." ;
    skos:definition "The HY_WaterBody feature type specializes the general HY_HydroFeature class. A waterbody is part of the hydrographic network and is either standing in a depression or flowing in a channel, which are parts of the channel network. A waterbody may be segmented in vertical sections at right angles to the main (average) direction of flow or along its centerline, and horizontal strata. Conceptually, each waterbody, or a stratum, could be thought of as a reservoir used for storage, regulation or control of water recourses.␊␊Through generalization, HY_WaterBody inherits the name property. It has associations for the hydrographicNetwork in which it participates, the containing waterpool and watercourse, the vertical streamCrossSection, streamLongitudinalSection, a horizontal stratum, and a reservoir for storage of water. Outlet-at-section and outlet-at-landmark constraints emphasize the recognition of a fixed landmark as outlet of the catchment realized by hydrographic network." ;
    skos:inScheme okns:hyf ;
    skos:mappingRelation <hyf:HY_WaterBody> ;
    linkml:class_uri <https://www.opengis.net/def/schema/hy_features/hyf/HY_WaterBody> ;
    linkml:definition_uri okns:HyfHYWaterBody ;
    linkml:slot_usage [ ] .

okns:Seegrid-ciContact a linkml:ClassDefinition ;
    dcterms:source <http://def.seegrid.csiro.au/isotc211/iso19115/2003/citation> ;
    dcterms:title "Contact" ;
    skos:altLabel "CI_Contact" ;
    skos:inScheme okns:seegrid-iso19115 ;
    skos:mappingRelation seegrid-ci:Contact ;
    linkml:class_uri seegrid-ci:Contact ;
    linkml:definition_uri okns:Seegrid-ciContact ;
    linkml:is_a <https://purl.org/okn/schema/HttpDef.seegrid.csiro.auIsotc211Iso191502012Hm2owl#DataType> ;
    linkml:slot_usage [ ] .

okns:Seegrid-ciOnlineResource a linkml:ClassDefinition ;
    dcterms:source <http://def.seegrid.csiro.au/isotc211/iso19115/2003/citation> ;
    dcterms:title "Online resource" ;
    skos:altLabel "CI_OnlineResource" ;
    skos:inScheme okns:seegrid-iso19115 ;
    skos:mappingRelation seegrid-ci:OnlineResource ;
    linkml:class_uri seegrid-ci:OnlineResource ;
    linkml:definition_uri okns:Seegrid-ciOnlineResource ;
    linkml:is_a <https://purl.org/okn/schema/HttpDef.seegrid.csiro.auIsotc211Iso191502012Hm2owl#DataType> ;
    linkml:slot_usage [ ] .

okns:rdfs_comment a linkml:SlotDefinition ;
    dcterms:source rdfs: ;
    dcterms:title "comment" ;
    skos:definition "A description of the subject resource." ;
    skos:inScheme okns:owl-rdf-rdfs ;
    skos:mappingRelation rdfs:comment ;
    linkml:any_of [ a okns:AnonymousSlotExpression ;
            linkml:range okns:RdfsLiteral ],
        [ a okns:AnonymousSlotExpression ;
            linkml:range okns:string ] ;
    linkml:definition_uri okns:rdfs_comment ;
    linkml:domain okns:RdfsResource ;
    linkml:domain_of okns:DcamVocabularyEncodingScheme,
        okns:DctAgentClass,
        okns:RdfList,
        okns:RdfsDatatype ;
    linkml:inlined true ;
    linkml:owner okns:rdfs_comment ;
    linkml:range okns:Any ;
    linkml:slot_uri rdfs:comment .

okns:rdfs_isDefinedBy a linkml:SlotDefinition ;
    dcterms:source rdfs: ;
    dcterms:title "isDefinedBy" ;
    rdfs:subPropertyOf okns:rdfs_seeAlso ;
    skos:definition "The definition of the subject resource." ;
    skos:inScheme okns:owl-rdf-rdfs ;
    skos:mappingRelation rdfs:isDefinedBy ;
    linkml:any_of [ a okns:AnonymousSlotExpression ;
            linkml:range okns:RdfsResource ],
        [ a okns:AnonymousSlotExpression ;
            linkml:range okns:OwlOntology ] ;
    linkml:definition_uri okns:rdfs_isDefinedBy ;
    linkml:domain okns:RdfsResource ;
    linkml:domain_of okns:DcamVocabularyEncodingScheme,
        okns:DctAgentClass,
        okns:RdfList,
        okns:RdfsDatatype ;
    linkml:inlined true ;
    linkml:owner okns:rdfs_isDefinedBy ;
    linkml:range okns:Any ;
    linkml:slot_uri rdfs:isDefinedBy .

okns:skos_note a linkml:SlotDefinition ;
    dcterms:source <http://www.w3.org/2004/02/skos/core> ;
    dcterms:title "note" ;
    skos:definition "A general note, for any purpose." ;
    skos:editorialNote "No occurrences of this slot in the graph.",
        "This property may be used directly, or as a super-property for more specific note types." ;
    skos:inScheme okns:skos ;
    skos:mappingRelation skos:note ;
    linkml:definition_uri okns:skos_note ;
    linkml:inlined true ;
    linkml:range okns:Any ;
    linkml:slot_uri skos:note .

okns:Seegrid-ciAddress a linkml:ClassDefinition ;
    dcterms:source <http://def.seegrid.csiro.au/isotc211/iso19115/2003/citation> ;
    dcterms:title "Address" ;
    skos:altLabel "CI_Address" ;
    skos:inScheme okns:seegrid-iso19115 ;
    skos:mappingRelation seegrid-ci:Address ;
    linkml:class_uri seegrid-ci:Address ;
    linkml:definition_uri okns:Seegrid-ciAddress ;
    linkml:is_a <https://purl.org/okn/schema/HttpDef.seegrid.csiro.auIsotc211Iso191502012Hm2owl#DataType> ;
    linkml:slot_usage [ ] .

okns:Seegrid-ciResponsibleParty a linkml:ClassDefinition ;
    dcterms:source <http://def.seegrid.csiro.au/isotc211/iso19115/2003/citation> ;
    dcterms:title "Responsible party" ;
    skos:altLabel "CI_ResponsibleParty" ;
    skos:inScheme okns:seegrid-iso19115 ;
    skos:mappingRelation seegrid-ci:ResponsibleParty ;
    linkml:class_uri seegrid-ci:ResponsibleParty ;
    linkml:definition_uri okns:Seegrid-ciResponsibleParty ;
    linkml:is_a <https://purl.org/okn/schema/HttpDef.seegrid.csiro.auIsotc211Iso191502012Hm2owl#DataType> ;
    linkml:slot_usage [ ] .

<https://purl.org/okn/schema/HttpDef.seegrid.csiro.auIsotc211Iso191502012Hm2owl#DataType> a linkml:ClassDefinition ;
    dcterms:title "No class (entity type) name specified -- this class is noted as a superclass of another class in this graph but has not itself been defined." ;
    skos:inScheme okns:seegrid-iso19115 ;
    skos:mappingRelation <http://def.seegrid.csiro.au/isotc211/iso19150/2012/hm2owl#DataType> ;
    linkml:class_uri <http://def.seegrid.csiro.au/isotc211/iso19150/2012/hm2owl#DataType> ;
    linkml:definition_uri <https://purl.org/okn/schema/HttpDef.seegrid.csiro.auIsotc211Iso191502012Hm2owl#DataType> ;
    linkml:slot_usage [ ] .

okns:OwlClass a linkml:ClassDefinition ;
    dcterms:source owl: ;
    dcterms:title "Class" ;
    skos:definition "The class of OWL classes." ;
    skos:inScheme okns:owl-rdf-rdfs ;
    skos:mappingRelation owl:Class ;
    linkml:class_uri owl:Class ;
    linkml:definition_uri okns:OwlClass ;
    linkml:is_a okns:RdfsClass ;
    linkml:slot_usage [ ] .

okns:dct_date a linkml:SlotDefinition ;
    dcterms:source dcterms: ;
    dcterms:title "Date" ;
    rdfs:subPropertyOf okns:dc_date ;
    skos:definition "Date may be used to express temporal information at any level of granularity.  Recommended practice is to express the date, date/time, or period of time according to ISO 8601-1 [[ISO 8601-1](https://www.iso.org/iso-8601-date-and-time-format.html)] or a published profile of the ISO standard, such as the W3C Note on Date and Time Formats [[W3CDTF](https://www.w3.org/TR/NOTE-datetime)] or the Extended Date/Time Format Specification [[EDTF](http://www.loc.gov/standards/datetime/)].  If the full date is unknown, month and year (YYYY-MM) or just year (YYYY) may be used. Date ranges may be specified using ISO 8601 period of time specification in which start and end dates are separated by a '/' (slash) character.  Either the start or end date may be missing." ;
    skos:editorialNote "No occurrences of this slot in the graph." ;
    skos:inScheme okns:dc ;
    skos:mappingRelation dcterms:date ;
    skos:note "description: A point or period of time associated with an event in the lifecycle of the resource." ;
    linkml:definition_uri okns:dct_date ;
    linkml:inlined true ;
    linkml:range okns:RdfsLiteral ;
    linkml:slot_uri dcterms:date .

okns:OwlObjectProperty a linkml:ClassDefinition ;
    dcterms:source owl: ;
    dcterms:title "ObjectProperty" ;
    skos:definition "The class of object properties." ;
    skos:inScheme okns:owl-rdf-rdfs ;
    skos:mappingRelation owl:ObjectProperty ;
    linkml:class_uri owl:ObjectProperty ;
    linkml:definition_uri okns:OwlObjectProperty ;
    linkml:is_a okns:RdfProperty ;
    linkml:slot_usage [ ] .

okns:rdfs_label a linkml:SlotDefinition ;
    dcterms:source rdfs: ;
    dcterms:title "label" ;
    skos:definition "A human-readable name for the subject." ;
    skos:inScheme okns:owl-rdf-rdfs ;
    skos:mappingRelation rdfs:label ;
    linkml:any_of [ a okns:AnonymousSlotExpression ;
            linkml:range okns:RdfsLiteral ],
        [ a okns:AnonymousSlotExpression ;
            linkml:range okns:string ] ;
    linkml:definition_uri okns:rdfs_label ;
    linkml:domain okns:RdfsResource ;
    linkml:domain_of okns:DcamVocabularyEncodingScheme,
        okns:DctAgentClass,
        okns:RdfList,
        okns:RdfsDatatype ;
    linkml:inlined true ;
    linkml:owner okns:rdfs_label ;
    linkml:range okns:Any ;
    linkml:slot_uri rdfs:label .

okns:unsignedinteger a linkml:TypeDefinition ;
    rdfs:seeAlso <https://numpy.org/doc/stable/reference/arrays.scalars.html#numpy.unsignedinteger>,
        <https://www.w3.org/TR/xmlschema-2/#nonNegativeInteger> ;
    skos:definition "An integer that is non-negative" ;
    skos:inScheme okns:extended_types ;
    linkml:base "int" ;
    linkml:definition_uri linkml:Unsignedinteger ;
    linkml:minimum_value "0"^^<https://purl.org/okn/schema/@id> ;
    linkml:typeof okns:integer ;
    linkml:uri xsd:unsignedInt .

okns:HyfHYCatchment a linkml:ClassDefinition ;
    dcterms:title "No class (entity type) name specified -- this class is noted as a superclass of another class in this graph but has not itself been defined." ;
    skos:definition "The Catchment model conceptualizes the hydrologic determination of a catchment through inflow and outflow hydro nexus features with the role of getting flow from a contributing catchment, or providing inflow to a receiving catchment (Figure 25 and Figure 26). Conceptually, each catchment has an outflow hydro nexus, and any hydro nexus has a corresponding catchment, even if catchment and/or hydro nexus may not be present in a particular application. A catchment interacts with upper and lower catchments via associated hydro nexuses, and ultimately contributes flow to the hydro nexus of a containing catchment. The catchment should be understood as the logical link between two hydro nexuses.␊␊The HY_Catchment feature type captures the union of catchment and hydro nexus, and the multiple realizations of the holistic catchment concept. These realizations include both topological realizations, as well as their geometric representation. HY_Catchment may be further specialized with respect to catchment interaction.␊␊The HY_Catchment feature type (Figure 26) specializes the general HY_HydroFeature type. Through generalization, HY_Catchment inherits the name property. It carries a code attribute and the associations: outflow, inflow, containingCatchment, containedCatchment, conjointCatchment, upperCatchment, lowerCatchment, catchmentRealization." ;
    skos:inScheme okns:hyf ;
    skos:mappingRelation <hyf:HY_Catchment> ;
    skos:note "description: The Catchment model conceptualizes the hydrologic determination of a catchment through inflow and outflow hydro nexus features with the role of getting flow from a contributing catchment, or providing inflow to a receiving catchment (Figure 25 and Figure 26). Conceptually, each catchment has an outflow hydro nexus, and any hydro nexus has a corresponding catchment, even if catchment and/or hydro nexus may not be present in a particular application. A catchment interacts with upper and lower catchments via associated hydro nexuses, and ultimately contributes flow to the hydro nexus of a containing catchment. The catchment should be understood as the logical link between two hydro nexuses. The HY_Catchment feature type captures the union of catchment and hydro nexus, and the multiple realizations of the holistic catchment concept. These realizations include both topological realizations, as well as their geometric representation. HY_Catchment may be further specialized with respect to catchment interaction.  The HY_Catchment feature type (Figure 26) specializes the general HY_HydroFeature type. Through generalization, HY_Catchment inherits the name property. It carries a code attribute and the associations: outflow, inflow, containingCatchment, containedCatchment, conjointCatchment, upperCatchment, lowerCatchment, catchmentRealization." ;
    linkml:class_uri <https://www.opengis.net/def/schema/hy_features/hyf/HY_Catchment> ;
    linkml:definition_uri okns:HyfHYCatchment ;
    linkml:is_a okns:HyfHYHydroFeature ;
    linkml:slot_usage [ ] .

okns:OwlOntology a linkml:ClassDefinition ;
    dcterms:source owl: ;
    dcterms:title "Ontology" ;
    skos:definition "The class of ontologies." ;
    skos:inScheme okns:owl-rdf-rdfs ;
    skos:mappingRelation owl:Ontology ;
    linkml:class_uri owl:Ontology ;
    linkml:definition_uri okns:OwlOntology ;
    linkml:is_a okns:RdfsResource ;
    linkml:slot_usage [ ] .

okns:SkosConcept a linkml:ClassDefinition ;
    dcterms:source <http://www.w3.org/2004/02/skos/core> ;
    dcterms:title "Concept" ;
    skos:definition "An idea or notion; a unit of thought." ;
    skos:inScheme okns:skos ;
    skos:mappingRelation skos:Concept ;
    linkml:class_uri skos:Concept ;
    linkml:definition_uri okns:SkosConcept ;
    linkml:slot_usage [ ] .

okns:RdfsDatatype a linkml:ClassDefinition ;
    dcterms:source rdfs: ;
    dcterms:title "Datatype" ;
    skos:definition "The class of RDF datatypes." ;
    skos:inScheme okns:owl-rdf-rdfs ;
    skos:mappingRelation rdfs:Datatype ;
    linkml:class_uri rdfs:Datatype ;
    linkml:definition_uri okns:RdfsDatatype ;
    linkml:is_a okns:RdfsClass ;
    linkml:slot_usage [ ] ;
    linkml:slots okns:rdfs_comment,
        okns:rdfs_isDefinedBy,
        okns:rdfs_label,
        okns:rdfs_seeAlso,
        okns:rdfs_subClassOf .

okns:Seegrid-basicMeasure a linkml:ClassDefinition ;
    dcterms:source <http://def.seegrid.csiro.au/isotc211/iso19103/2005/basic> ;
    dcterms:title "Measure" ;
    skos:definition "Scaled number" ;
    skos:inScheme okns:seegrid-iso19115 ;
    skos:mappingRelation seegrid-basic:Measure ;
    skos:note "title: Mesure" ;
    linkml:class_uri seegrid-basic:Measure ;
    linkml:definition_uri okns:Seegrid-basicMeasure ;
    linkml:slot_usage [ ] .

okns:Seegrid-ciCitation a linkml:ClassDefinition ;
    dcterms:source <http://def.seegrid.csiro.au/isotc211/iso19115/2003/citation> ;
    dcterms:title "Citation" ;
    skos:altLabel "CI_Citation" ;
    skos:inScheme okns:seegrid-iso19115 ;
    skos:mappingRelation seegrid-ci:Citation ;
    linkml:class_uri seegrid-ci:Citation ;
    linkml:definition_uri okns:Seegrid-ciCitation ;
    linkml:is_a <https://purl.org/okn/schema/HttpDef.seegrid.csiro.auIsotc211Iso191502012Hm2owl#DataType> ;
    linkml:slot_usage [ ] .

okns:OwlRestriction a linkml:ClassDefinition ;
    dcterms:source owl: ;
    dcterms:title "Restriction" ;
    skos:definition "The class of property restrictions." ;
    skos:inScheme okns:owl-rdf-rdfs ;
    skos:mappingRelation owl:Restriction ;
    linkml:class_uri owl:Restriction ;
    linkml:definition_uri okns:OwlRestriction ;
    linkml:is_a okns:OwlClass ;
    linkml:slot_usage [ ] .

okns:OwlThing a linkml:ClassDefinition ;
    dcterms:source owl: ;
    dcterms:title "Thing" ;
    skos:definition "The class of OWL individuals." ;
    skos:inScheme okns:owl-rdf-rdfs ;
    skos:mappingRelation owl:Thing ;
    linkml:class_uri owl:Thing ;
    linkml:definition_uri okns:OwlThing ;
    linkml:slot_usage [ ] .

okns:dct_relation a linkml:SlotDefinition ;
    dcterms:source dcterms: ;
    dcterms:title "Relation" ;
    rdfs:subPropertyOf okns:dc_relation ;
    skos:definition "Recommended practice is to identify the related resource by means of a URI.  If this is not possible or feasible, a string conforming to a formal identification system may be provided." ;
    skos:editorialNote "No occurrences of this slot in the graph." ;
    skos:inScheme okns:dc ;
    skos:mappingRelation dcterms:relation ;
    skos:note "description: A related resource." ;
    linkml:definition_uri okns:dct_relation ;
    linkml:inlined true ;
    linkml:range okns:Any ;
    linkml:slot_uri dcterms:relation .

okns:RdfsClass a linkml:ClassDefinition ;
    dcterms:source rdfs: ;
    dcterms:title "Class" ;
    skos:definition "The class of classes." ;
    skos:inScheme okns:owl-rdf-rdfs ;
    skos:mappingRelation rdfs:Class ;
    linkml:class_uri rdfs:Class ;
    linkml:definition_uri okns:RdfsClass ;
    linkml:is_a okns:RdfsResource ;
    linkml:slot_usage [ ] .

okns:RdfList a linkml:ClassDefinition ;
    dcterms:source rdf: ;
    dcterms:title "List" ;
    skos:definition "The class of RDF Lists." ;
    skos:inScheme okns:owl-rdf-rdfs ;
    skos:mappingRelation rdf:List ;
    linkml:class_uri rdf:List ;
    linkml:definition_uri okns:RdfList ;
    linkml:is_a okns:RdfsResource ;
    linkml:slot_usage [ ] ;
    linkml:slots okns:rdfs_comment,
        okns:rdfs_isDefinedBy,
        okns:rdfs_label .

okns:RdfProperty a linkml:ClassDefinition ;
    dcterms:source rdf: ;
    dcterms:title "Property" ;
    skos:definition "The class of RDF properties." ;
    skos:inScheme okns:owl-rdf-rdfs ;
    skos:mappingRelation rdf:Property ;
    linkml:class_uri rdf:Property ;
    linkml:definition_uri okns:RdfProperty ;
    linkml:is_a okns:RdfsResource ;
    linkml:slot_usage [ ] .

okns:RdfsLiteral a linkml:ClassDefinition ;
    dcterms:source rdfs: ;
    dcterms:title "No (data)type name specified -- this type is noted as a supertype of another type in this graph but has not itself been defined." ;
    skos:definition "The class of literal values, eg. textual strings and integers." ;
    skos:inScheme okns:owl-rdf-rdfs ;
    skos:mappingRelation rdfs:Literal ;
    linkml:class_uri rdfs:Literal ;
    linkml:definition_uri okns:RdfsLiteral ;
    linkml:is_a okns:RdfsResource ;
    linkml:slot_usage [ ] .

okns:RdfsResource a linkml:ClassDefinition ;
    dcterms:source rdfs: ;
    dcterms:title "Resource" ;
    skos:definition "The class resource, everything." ;
    skos:inScheme okns:owl-rdf-rdfs ;
    skos:mappingRelation rdfs:Resource ;
    linkml:class_uri rdfs:Resource ;
    linkml:definition_uri okns:RdfsResource ;
    linkml:slot_usage [ ] .

okns:string a linkml:TypeDefinition ;
    skos:definition "A character string" ;
    skos:editorialNote "In RDF serializations, a slot with range of string is treated as a literal or type xsd:string.   If you are authoring schemas in LinkML YAML, the type is referenced with the lower case \"string\"." ;
    skos:exactMatch schema1:Text ;
    skos:inScheme linkml:types ;
    linkml:base "str" ;
    linkml:imported_from "linkml:types" ;
    linkml:definition_uri linkml:String ;
    linkml:uri xsd:string .

okns:hyf a linkml:SchemaDefinition ;
    dcterms:license "https://creativecommons.org/publicdomain/zero/1.0/" ;
    pav:createdOn "2025-09-03T12:58:33.676520"^^xsd:dateTime ;
    pav:lastUpdatedOn "2025-09-03T12:58:33.676520"^^xsd:dateTime ;
    skos:definition "The HydroFeature module (Figure 21) provides the core concepts of a named hydrologic feature in the Named Feature, of a hydrologic complex in which the union of catchment and its common outlet is realized in several ways by a collection of hydrologic features, and of a river referencing system which allows placement of an arbitrary feature ‘along a river’ using linear referencing along a one-dimensional topological, flowpath realization.  The HY_HydroFeature feature type is defined as hydrology-specific instance of the General Feature metaclass (as defined in the OGC General Feature Model, GFM), whose identity needs to be maintained and tracked through a processing chain from measurement to distribution of hydrologic information.␊As an instance of the General Feature metaclass a feature type is identified by a unique identifier and typical properties. Typically, a hydrologic feature is additionally identified through names in common usage and through hydrologically significant characteristics.  The HY_HydroFeature feature type is specialized into more specific feature types (Figure 23), which specify additional properties and represent particular hydrologic phenomena.Providing a standard terminology for the typical relationships between hydrologic features allows the hydrosphere to be expressed in a consistent way across multiple data products, regardless of various spatial or temporal representations. The definitions of HydroFeature feature types are rooted in the definitions documented in the WMO/UNESCO Glossary of Hydrology. They are applied regardless of their application context in respect to the Earth's surface. For the purpose of testing the applicability of the HY_Features conceptual model in the context of surface water hydrology, the definitions in this standard refer to surface water hydrology. A conceptual model capturing the specifics of features associated with the groundwater domain is developed with reference to the OGC WaterML 2: Part 4 – GroundwaterML2 standard." ;
    skos:note "description: The HydroFeature module (Figure 21) provides the core concepts of a named hydrologic feature in the Named Feature, of a hydrologic complex in which the union of catchment and its common outlet is realized in several ways by a collection of hydrologic features, and of a river referencing system which allows placement of an arbitrary feature ‘along a river’ using linear referencing along a one-dimensional topological, flowpath realization.␊␊The HY_HydroFeature feature type is defined as hydrology-specific instance of the General Feature metaclass (as defined in the OGC General Feature Model, GFM), whose identity needs to be maintained and tracked through a processing chain from measurement to distribution of hydrologic information.␊As an instance of the General Feature metaclass a feature type is identified by a unique identifier and typical properties. Typically, a hydrologic feature is additionally identified through names in common usage and through hydrologically significant characteristics.␊␊The HY_HydroFeature feature type is specialized into more specific feature types (Figure 23), which specify additional properties and represent particular hydrologic phenomena.Providing a standard terminology for the typical relationships between hydrologic features allows the hydrosphere to be expressed in a consistent way across multiple data products, regardless of various spatial or temporal representations.␊␊The definitions of HydroFeature feature types are rooted in the definitions documented in the WMO/UNESCO Glossary of Hydrology. They are applied regardless of their application context in respect to the Earth's surface. For the purpose of testing the applicability of the HY_Features conceptual model in the context of surface water hydrology, the definitions in this standard refer to surface water hydrology. A conceptual model capturing the specifics of features associated with the groundwater domain is developed with reference to the OGC WaterML 2: Part 4 – GroundwaterML2 standard.",
        "description: The Hydrometric Network application schema (Figure 45) defines a logical model to take into account a network of hydrometric stations as a specific realization of the catchment in the perspective of hydrologic observation, without the detail of an observation strategy.␊␊The Hydrometric Network model specifies the concepts defined in the Hydro Feature core model.. The general concept is that of a network of logically connected hydrometric stations realizing as a whole the catchment. This enables contextually related information models to relate monitoring stations and observing posts to hydrologic features, as is often required for environmental reporting or when interpreting, analyzing and processing observation results.",
        "description: The Surface Hydro Feature application schema provides common concepts of hydrologic features occurring on the land surface and specifies the core concepts defined in the abstract Hydro Feature application schema. This will enable contextually linked information models to build relationships between multiple realizations of the same catchments. Typical realizations of the catchment concept and hydro nexuses can be described in a consistent way using standard terminology for the relationships between surface water features defined in this application schema.␊␊The Surface Hydro Feature model (Figure 37) conceptualizes the accumulation of water on the land surface in waterbodies, each made unique by its origin, size, or movement. With respect to the management and storage of water resources, a concept of water storage is provided and allows any waterbody type to be considered a managed reservoir.␊␊Relying on a conceptual separation of waterbody and container, the Surface Hydro Feature schema defines a network of potentially connected depressions and channels on the land surface which periodically or continuously contain water. Separate from the hydrographic network of permanent or temporary waterbodies, the channel network can be used as the connecting system.␊␊The definitions in this schema are rooted in the definitions given in the WMO/UNESCO Glossary of Hydrology which defines a network of watercourse regardless of the location in respect to the Earth's surface. The conceptual model defined here has been vetted in the context of surface water hydrology. In other words, in this standard, 'channel network' and 'hydrographic network' refer to surface channels or other containers for surface-waterbodies.␊␊The Surface Hydro Feature application schema contains the leaf packages: Channel Network, Hydrographic Network, Water Body Types and Storage.",
        "title: HY_Features HydroFeature package" ;
    sh:declare [ sh:namespace sc: ;
            sh:prefix "sc" ],
        [ sh:namespace owl: ;
            sh:prefix "owl" ],
        [ sh:namespace linkml: ;
            sh:prefix "linkml" ],
        [ sh:namespace <https://www.opengis.net/def/schema/hy_features/hyf/> ;
            sh:prefix "hyf" ],
        [ sh:namespace rdfs: ;
            sh:prefix "rdfs" ],
        [ sh:namespace seegrid-ci: ;
            sh:prefix "seegrid-ci" ],
        [ sh:namespace okns: ;
            sh:prefix "okns" ],
        [ sh:namespace skos: ;
            sh:prefix "skos" ],
        [ sh:namespace okn: ;
            sh:prefix "okn" ],
        [ sh:namespace xsd: ;
            sh:prefix "xsd" ] ;
    linkml:default_prefix "okns" ;
    linkml:metamodel_version "1.7.0" ;
    linkml:source_file "hyf.yaml" ;
    linkml:annotations [ skos:example [ okns:pairs [ skos:example [ ] ;
                            linkml:tag okns:pairs ] ;
                    linkml:classes [ skos:example [ ] ;
                            linkml:tag okns:classes ] ] ;
            linkml:tag okns:examples ],
        [ skos:example [ okns:pairs [ skos:example [ ] ;
                            linkml:tag okns:pairs ] ;
                    linkml:classes [ skos:example [ ] ;
                            linkml:tag okns:classes ] ;
                    linkml:slots [ skos:example [ ] ;
                            linkml:tag okns:slots ] ] ;
            linkml:tag okns:counts ] ;
    linkml:classes okns:Any,
        okns:DcamVocabularyEncodingScheme,
        okns:DcmitypeCollection,
        okns:DcmitypeDataset,
        okns:DcmitypeEvent,
        okns:DcmitypeImage,
        okns:DcmitypeInteractiveResource,
        okns:DcmitypeMovingImage,
        okns:DcmitypePhysicalObject,
        okns:DcmitypeService,
        okns:DcmitypeSoftware,
        okns:DcmitypeSound,
        okns:DcmitypeStillImage,
        okns:DcmitypeText,
        okns:DctAgent,
        okns:DctAgentClass,
        okns:DctBibliographicResource,
        okns:DctFileFormat,
        okns:DctFrequency,
        okns:DctJurisdiction,
        okns:DctLicenseDocument,
        okns:DctLinguisticSystem,
        okns:DctLocation,
        okns:DctLocationPeriodOrJurisdiction,
        okns:DctMediaType,
        okns:DctMediaTypeOrExtent,
        okns:DctMethodOfAccrual,
        okns:DctMethodOfInstruction,
        okns:DctPeriodOfTime,
        okns:DctPhysicalMedium,
        okns:DctPhysicalResource,
        okns:DctPolicy,
        okns:DctProvenanceStatement,
        okns:DctRightsStatement,
        okns:DctSizeOrDuration,
        okns:DctStandard,
        <https://purl.org/okn/schema/HttpDef.seegrid.csiro.auIsotc211Iso191502012Hm2owl#CodeList>,
        <https://purl.org/okn/schema/HttpDef.seegrid.csiro.auIsotc211Iso191502012Hm2owl#DataType>,
        okns:HyfHYCanal,
        okns:HyfHYCartographicRealization,
        okns:HyfHYCatchment,
        okns:HyfHYCatchmentAggregate,
        okns:HyfHYCatchmentArea,
        okns:HyfHYCatchmentDivide,
        okns:HyfHYCatchmentRealization,
        okns:HyfHYChannel,
        okns:HyfHYChannelNetwork,
        okns:HyfHYCrossSection,
        okns:HyfHYDendriticCatchment,
        okns:HyfHYDepression,
        okns:HyfHYDistanceDescription,
        okns:HyfHYDistanceFromReferent,
        okns:HyfHYEstuary,
        okns:HyfHYFlowPath,
        okns:HyfHYHydroFeature,
        okns:HyfHYHydroFeatureName,
        okns:HyfHYHydroLocation,
        okns:HyfHYHydroLocationType,
        okns:HyfHYHydroNetwork,
        okns:HyfHYHydroNexus,
        okns:HyfHYHydrographicNetwork,
        okns:HyfHYHydrometricFeature,
        okns:HyfHYHydrometricNetwork,
        okns:HyfHYImpoundment,
        okns:HyfHYIndirectPosition,
        okns:HyfHYInteriorCatchment,
        okns:HyfHYLagoon,
        okns:HyfHYLake,
        okns:HyfHYLongitudinalSection,
        okns:HyfHYNameUsage,
        okns:HyfHYReservoir,
        okns:HyfHYRiver,
        okns:HyfHYWaterBody,
        okns:HyfHYWaterBodyStratum,
        okns:HyfHYWaterLiquidPhase,
        okns:HyfHYWaterSolidPhase,
        okns:OwlAllDifferent,
        okns:OwlAllDisjointClasses,
        okns:OwlAllDisjointProperties,
        okns:OwlAnnotation,
        okns:OwlAnnotationProperty,
        okns:OwlAsymmetricProperty,
        okns:OwlAxiom,
        okns:OwlClass,
        okns:OwlDataRange,
        okns:OwlDatatypeProperty,
        okns:OwlDeprecatedClass,
        okns:OwlDeprecatedProperty,
        okns:OwlFunctionalProperty,
        okns:OwlInverseFunctionalProperty,
        okns:OwlIrreflexiveProperty,
        okns:OwlNamedIndividual,
        okns:OwlNegativePropertyAssertion,
        okns:OwlNothing,
        okns:OwlObjectProperty,
        okns:OwlOntology,
        okns:OwlOntologyProperty,
        okns:OwlReflexiveProperty,
        okns:OwlRestriction,
        okns:OwlSymmetricProperty,
        okns:OwlThing,
        okns:OwlTransitiveProperty,
        okns:RdfAlt,
        okns:RdfBag,
        okns:RdfCompoundLiteral,
        okns:RdfList,
        okns:RdfProperty,
        okns:RdfSeq,
        okns:RdfStatement,
        okns:RdfsClass,
        okns:RdfsContainer,
        okns:RdfsContainerMembershipProperty,
        okns:RdfsDatatype,
        okns:RdfsLiteral,
        okns:RdfsResource,
        okns:Seegrid-basicAcceleration,
        okns:Seegrid-basicAngle,
        okns:Seegrid-basicAngularVelocity,
        okns:Seegrid-basicArea,
        okns:Seegrid-basicCurrency,
        okns:Seegrid-basicDistance,
        okns:Seegrid-basicLength,
        okns:Seegrid-basicMass,
        okns:Seegrid-basicMeasure,
        okns:Seegrid-basicScale,
        okns:Seegrid-basicTime,
        okns:Seegrid-basicUnitOfMeasure,
        okns:Seegrid-basicVector,
        okns:Seegrid-basicVelocity,
        okns:Seegrid-basicVolume,
        okns:Seegrid-basicWeight,
        okns:Seegrid-ciAddress,
        okns:Seegrid-ciCitation,
        okns:Seegrid-ciContact,
        okns:Seegrid-ciDate,
        okns:Seegrid-ciDateTypeCode,
        okns:Seegrid-ciOnLineFunctionCode,
        okns:Seegrid-ciOnlineResource,
        okns:Seegrid-ciPresentationFormCode,
        okns:Seegrid-ciResponsibleParty,
        okns:Seegrid-ciRoleCode,
        okns:Seegrid-ciSeries,
        okns:Seegrid-ciTelephone,
        okns:SkosCollection,
        okns:SkosConcept,
        okns:SkosConceptScheme,
        okns:SkosOrderedCollection ;
    linkml:default_range okns:string ;
    linkml:generation_date "2025-09-04T07:58:08"^^xsd:dateTime ;
    linkml:id okns:hyf ;
    linkml:imports okns:dc,
        okns:extended_types,
        okns:owl-rdf-rdfs,
        okns:sc,
        okns:seegrid-iso19115,
        okns:skos,
        linkml:types ;
    linkml:slots okns:dc_contributor,
        okns:dc_coverage,
        okns:dc_creator,
        okns:dc_date,
        okns:dc_description,
        okns:dc_format,
        okns:dc_identifier,
        okns:dc_language,
        okns:dc_publisher,
        okns:dc_relation,
        okns:dc_rights,
        okns:dc_source,
        okns:dc_subject,
        okns:dc_title,
        okns:dc_type,
        okns:dcam_domainIncludes,
        okns:dcam_memberOf,
        okns:dcam_rangeIncludes,
        okns:dct_abstract,
        okns:dct_accessRights,
        okns:dct_accrualMethod,
        okns:dct_accrualPeriodicity,
        okns:dct_accrualPolicy,
        okns:dct_alternative,
        okns:dct_audience,
        okns:dct_available,
        okns:dct_bibliographicCitation,
        okns:dct_conformsTo,
        okns:dct_contributor,
        okns:dct_coverage,
        okns:dct_created,
        okns:dct_creator,
        okns:dct_date,
        okns:dct_dateAccepted,
        okns:dct_dateCopyrighted,
        okns:dct_dateSubmitted,
        okns:dct_description,
        okns:dct_educationLevel,
        okns:dct_extent,
        okns:dct_format,
        okns:dct_hasFormat,
        okns:dct_hasPart,
        okns:dct_hasVersion,
        okns:dct_identifier,
        okns:dct_instructionalMethod,
        okns:dct_isFormatOf,
        okns:dct_isPartOf,
        okns:dct_isReferencedBy,
        okns:dct_isReplacedBy,
        okns:dct_isRequiredBy,
        okns:dct_isVersionOf,
        okns:dct_issued,
        okns:dct_language,
        okns:dct_license,
        okns:dct_mediator,
        okns:dct_medium,
        okns:dct_modified,
        okns:dct_provenance,
        okns:dct_publisher,
        okns:dct_references,
        okns:dct_relation,
        okns:dct_replaces,
        okns:dct_requires,
        okns:dct_rights,
        okns:dct_rightsHolder,
        okns:dct_source,
        okns:dct_spatial,
        okns:dct_subject,
        okns:dct_tableOfContents,
        okns:dct_temporal,
        okns:dct_title,
        okns:dct_type,
        okns:dct_valid,
        <https://purl.org/okn/schema/http___def.isotc211.org_iso19150_2_2012_base#isEnumeration>,
        okns:hyf_absolute,
        okns:hyf_accumulatingWaterBody,
        okns:hyf_accuracyStatement,
        okns:hyf_bedProfileLongitudinal,
        okns:hyf_bedProfileTransversal,
        okns:hyf_catchmentArea,
        okns:hyf_catchmentDivide,
        okns:hyf_catchmentRealization,
        okns:hyf_code,
        okns:hyf_confinedWaterBody,
        okns:hyf_conjointCatchment,
        okns:hyf_containedCatchment,
        okns:hyf_containingCatchment,
        okns:hyf_contributingCatchment,
        okns:hyf_coveredWaterBody,
        okns:hyf_distanceDescription,
        okns:hyf_distanceExpression,
        okns:hyf_downstreamWaterBody,
        okns:hyf_endorheicDrainage,
        okns:hyf_exorheicDrainage,
        okns:hyf_flowpath,
        okns:hyf_hydroLocationType,
        okns:hyf_inflow,
        okns:hyf_interpolative,
        okns:hyf_linearElement,
        okns:hyf_locatedReferent,
        okns:hyf_lowerCatchment,
        okns:hyf_name,
        okns:hyf_name_string,
        okns:hyf_namesPart,
        okns:hyf_networkStation,
        okns:hyf_networkWaterBody,
        okns:hyf_nexusRealization,
        okns:hyf_outflow,
        okns:hyf_precisionStatement,
        okns:hyf_preferredBy,
        okns:hyf_realizedCatchment,
        okns:hyf_realizedNexus,
        okns:hyf_receivingCatchment,
        okns:hyf_referenceLocation,
        okns:hyf_referencedPosition,
        okns:hyf_reservoirZone,
        okns:hyf_snowmelt,
        okns:hyf_standingWater,
        okns:hyf_storage,
        okns:hyf_storedWaterBody,
        okns:hyf_stratum,
        okns:hyf_stream,
        okns:hyf_streamCrossSection,
        okns:hyf_streamLongitudinalSection,
        okns:hyf_surfaceChannel,
        okns:hyf_surfaceDepression,
        okns:hyf_upperCatchment,
        okns:hyf_upstreamWaterBody,
        okns:hyf_usage,
        okns:hyf_variantSpelling,
        okns:hyf_watercourse,
        okns:hyf_waterpool,
        okns:langrange,
        okns:length,
        okns:maxexclusive,
        okns:maxlength,
        okns:minexclusive,
        okns:minlength,
        okns:owl_allValuesFrom,
        okns:owl_annotatedProperty,
        okns:owl_annotatedSource,
        okns:owl_annotatedTarget,
        okns:owl_assertionProperty,
        okns:owl_backwardCompatibleWith,
        okns:owl_bottomDataProperty,
        okns:owl_bottomObjectProperty,
        okns:owl_cardinality,
        okns:owl_complementOf,
        okns:owl_datatypeComplementOf,
        okns:owl_deprecated,
        okns:owl_differentFrom,
        okns:owl_disjointUnionOf,
        okns:owl_disjointWith,
        okns:owl_distinctMembers,
        okns:owl_equivalentClass,
        okns:owl_equivalentProperty,
        okns:owl_hasKey,
        okns:owl_hasSelf,
        okns:owl_hasValue,
        okns:owl_imports,
        okns:owl_incompatibleWith,
        okns:owl_intersectionOf,
        okns:owl_inverseOf,
        okns:owl_maxCardinality,
        okns:owl_maxQualifiedCardinality,
        okns:owl_members,
        okns:owl_minCardinality,
        okns:owl_minQualifiedCardinality,
        okns:owl_onClass,
        okns:owl_onDataRange,
        okns:owl_onDatatype,
        okns:owl_onProperties,
        okns:owl_onProperty,
        okns:owl_oneOf,
        okns:owl_priorVersion,
        okns:owl_propertyChainAxiom,
        okns:owl_propertyDisjointWith,
        okns:owl_qualifiedCardinality,
        okns:owl_sameAs,
        okns:owl_someValuesFrom,
        okns:owl_sourceIndividual,
        okns:owl_targetIndividual,
        okns:owl_targetValue,
        okns:owl_topDataProperty,
        okns:owl_topObjectProperty,
        okns:owl_unionOf,
        okns:owl_versionIRI,
        okns:owl_versionInfo,
        okns:owl_withRestrictions,
        okns:rdf_direction,
        okns:rdf_first,
        okns:rdf_language,
        okns:rdf_object,
        okns:rdf_predicate,
        okns:rdf_rest,
        okns:rdf_subject,
        okns:rdf_type,
        okns:rdf_value,
        okns:rdfs_comment,
        okns:rdfs_domain,
        okns:rdfs_isDefinedBy,
        okns:rdfs_label,
        okns:rdfs_member,
        okns:rdfs_range,
        okns:rdfs_seeAlso,
        okns:rdfs_subClassOf,
        okns:rdfs_subPropertyOf,
        okns:seegrid_basic_dimension,
        okns:seegrid_basic_measure,
        okns:seegrid_basic_ordinates,
        okns:seegrid_basic_uom,
        okns:seegrid_basic_value,
        okns:seegrid_ci_Date.date,
        okns:seegrid_ci_ISBN,
        okns:seegrid_ci_ISSN,
        okns:seegrid_ci_address,
        okns:seegrid_ci_administrativeArea,
        okns:seegrid_ci_alternateTitle,
        okns:seegrid_ci_applicationProfile,
        okns:seegrid_ci_citedResponsibleParty,
        okns:seegrid_ci_city,
        okns:seegrid_ci_collectiveTitle,
        okns:seegrid_ci_contactInfo,
        okns:seegrid_ci_contactInstructions,
        okns:seegrid_ci_country,
        okns:seegrid_ci_date,
        okns:seegrid_ci_dateType,
        okns:seegrid_ci_deliveryPoint,
        okns:seegrid_ci_description,
        okns:seegrid_ci_edition,
        okns:seegrid_ci_editionDate,
        okns:seegrid_ci_electronicMailAddress,
        okns:seegrid_ci_facsimile,
        okns:seegrid_ci_function,
        okns:seegrid_ci_hoursOfService,
        okns:seegrid_ci_identifier,
        okns:seegrid_ci_individualName,
        okns:seegrid_ci_issueIdentification,
        okns:seegrid_ci_linkage,
        okns:seegrid_ci_name,
        okns:seegrid_ci_onlineResource,
        okns:seegrid_ci_organisationName,
        okns:seegrid_ci_otherCitationDetails,
        okns:seegrid_ci_page,
        okns:seegrid_ci_phone,
        okns:seegrid_ci_positionName,
        okns:seegrid_ci_postalCode,
        okns:seegrid_ci_presentationForm,
        okns:seegrid_ci_protocol,
        okns:seegrid_ci_role,
        okns:seegrid_ci_series,
        okns:seegrid_ci_title,
        okns:seegrid_ci_voice,
        okns:skos_altLabel,
        okns:skos_broadMatch,
        okns:skos_broader,
        okns:skos_broaderTransitive,
        okns:skos_changeNote,
        okns:skos_closeMatch,
        okns:skos_definition,
        okns:skos_defnition,
        okns:skos_editorialNote,
        okns:skos_exactMatch,
        okns:skos_example,
        okns:skos_hasTopConcept,
        okns:skos_hiddenLabel,
        okns:skos_historyNote,
        okns:skos_inScheme,
        okns:skos_mappingRelation,
        okns:skos_member,
        okns:skos_memberList,
        okns:skos_narrowMatch,
        okns:skos_narrower,
        okns:skos_narrowerTransitive,
        okns:skos_notation,
        okns:skos_note,
        okns:skos_prefLabel,
        okns:skos_related,
        okns:skos_relatedMatch,
        okns:skos_scopeNote,
        okns:skos_semanticRelation,
        okns:skos_topConceptOf ;
    linkml:source_file_date "2025-09-03T12:58:33"^^xsd:dateTime ;
    linkml:source_file_size 77744 ;
    linkml:types okns:base64binary,
        okns:boolean,
        okns:curie,
        okns:date,
        okns:date_or_datetime,
        okns:datetime,
        okns:dct_Box,
        okns:dct_ISO3166,
        okns:dct_ISO639_2,
        okns:dct_ISO639_3,
        okns:dct_Period,
        okns:dct_Point,
        okns:dct_RFC1766,
        okns:dct_RFC3066,
        okns:dct_RFC4646,
        okns:dct_RFC5646,
        okns:dct_URI,
        okns:dct_W3CDTF,
        okns:decimal,
        okns:double,
        okns:float,
        okns:float16,
        okns:float32,
        okns:float64,
        okns:hexbinary,
        okns:int16,
        okns:int32,
        okns:int64,
        okns:int8,
        okns:integer,
        okns:jsonpath,
        okns:jsonpointer,
        okns:language,
        okns:name,
        okns:ncname,
        okns:negativeinteger,
        okns:nmtoken,
        okns:nodeidentifier,
        okns:nonpositiveinteger,
        okns:normalizedstring,
        okns:objectidentifier,
        okns:positiveinteger,
        okns:rational,
        okns:rdf_HTML,
        okns:rdf_JSON,
        okns:rdf_PlainLiteral,
        okns:rdf_XMLLiteral,
        okns:rdf_langString,
        okns:real,
        okns:sc_Measure,
        okns:sc_Sign,
        okns:seegrid_basic_Boolean,
        okns:seegrid_basic_CharacterString,
        okns:seegrid_basic_Date,
        okns:seegrid_basic_DateTime,
        okns:seegrid_basic_Decimal,
        okns:seegrid_basic_ISOClassName,
        okns:seegrid_basic_Integer,
        okns:seegrid_basic_LocalName,
        okns:seegrid_basic_Number,
        okns:seegrid_basic_Real,
        okns:signedinteger,
        okns:sparqlpath,
        okns:string,
        okns:time,
        okns:token,
        okns:uint16,
        okns:uint32,
        okns:uint64,
        okns:uint8,
        okns:unsignedinteger,
        okns:uri,
        okns:uriorcurie .

okns:Any a linkml:ClassDefinition ;
    skos:definition "An unconstrained type or object" ;
    skos:inScheme okns:extended_types ;
    skos:mappingRelation linkml:Any ;
    linkml:class_uri linkml:Any ;
    linkml:definition_uri linkml:Any ;
    linkml:slot_usage [ ] .


