@prefix ao: <http://purl.org/ontology/ao/core#> .
@prefix cc: <http://web.resource.org/cc/> .
@prefix daml: <http://www.daml.org/2000/10/daml-ont#> .
@prefix daml-2001: <http://www.daml.org/2001/03/> .
@prefix daml-city: <http://www.daml.ri.cmu.edu/ont/City.daml#> .
@prefix daml-country: <http://www.daml.ri.cmu.edu/ont/Country.daml#> .
@prefix daml-country-ont: <http://www.daml.org/2001/09/countries/country-ont#> .
@prefix daml-iso3166: <http://www.daml.org/2001/09/countries/iso-3166-ont#> .
@prefix daml-oil: <http://www.daml.org/2001/03/daml+oil#> .
@prefix daml-ont: <http://www.daml.ri.cmu.edu/ont/> .
@prefix daml-profile: <http://www.daml.org/services/daml-s/2001/10/Profile.daml#> .
@prefix daml-state: <http://www.daml.ri.cmu.edu/ont/State.daml#> .
@prefix daml-usregionstate: <http://www.daml.ri.cmu.edu/ont/USRegionState.daml#> .
@prefix dc: <http://purl.org/dc/elements/1.1/> .
@prefix dcam: <http://purl.org/dc/dcam/> .
@prefix dcmitype: <http://purl.org/dc/dcmitype/> .
@prefix dcterms: <http://purl.org/dc/terms/> .
@prefix event: <http://purl.org/NET/c4dm/event.owl#> .
@prefix foaf: <http://xmlns.com/foaf/0.1/> .
@prefix frbr: <http://purl.org/vocab/frbr/core#> .
@prefix ical: <http://www.w3.org/2002/12/cal/ical#> .
@prefix icalspec: <http://www.w3.org/2002/12/cal/icalSpec#> .
@prefix linkml: <https://w3id.org/linkml/> .
@prefix ns1: <mo:> .
@prefix okn: <https://purl.org/okn/> .
@prefix okns: <https://purl.org/okn/schema/> .
@prefix owl: <http://www.w3.org/2002/07/owl#> .
@prefix pav: <http://purl.org/pav/> .
@prefix rdf: <http://www.w3.org/1999/02/22-rdf-syntax-ns#> .
@prefix rdfs: <http://www.w3.org/2000/01/rdf-schema#> .
@prefix rev: <http://purl.org/stuff/rev#> .
@prefix schema1: <http://schema.org/> .
@prefix sh: <http://www.w3.org/ns/shacl#> .
@prefix shex: <http://www.w3.org/ns/shex#> .
@prefix sim: <http://purl.org/ontology/similarity/> .
@prefix skos: <http://www.w3.org/2004/02/skos/core#> .
@prefix swvs: <http://www.w3.org/2003/06/sw-vocab-status/ns#> .
@prefix time: <http://www.w3.org/2006/time#> .
@prefix time-entry: <http://www.isi.edu/~pan/damltime/time-entry.owl#> .
@prefix tzont: <http://www.isi.edu/~pan/damltime/timezone-ont.owl#> .
@prefix vann: <http://purl.org/vocab/vann/> .
@prefix wfb: <http://ontolingua.stanford.edu/doc/chimaera/ontologies/world-fact-book.daml#> .
@prefix wgs1: <http://www.w3.org/2003/01/geo/wgs84_pos#> .
@prefix wn16: <http://xmlns.com/wordnet/1.6/> .
@prefix wot: <http://xmlns.com/wot/0.1/> .
@prefix xsd: <http://www.w3.org/2001/XMLSchema#> .
@prefix xsd2000: <http://www.w3.org/2000/10/XMLSchema#> .

okns:base64binary a linkml:TypeDefinition ;
    skos:definition "Arbitrary Base64-encoded binary data." ;
    skos:inScheme okns:extended_types ;
    skos:note "added by Mahir Morshed <mmorshed@scripps.edu>",
        "used 'string' as base type since no 'binary' base type exists" ;
    linkml:base "string" ;
    linkml:definition_uri linkml:Base64binary ;
    linkml:uri xsd:hexBinary .

okns:curie a linkml:TypeDefinition ;
    dcterms:conformsTo "https://www.w3.org/TR/curie/" ;
    skos:definition "a compact URI" ;
    skos:editorialNote "If you are authoring schemas in LinkML YAML, the type is referenced with the lower case \"curie\"." ;
    skos:inScheme linkml:types ;
    skos:note "in RDF serializations this MUST be expanded to a URI",
        "in non-RDF serializations MAY be serialized as the compact representation" ;
    linkml:base "Curie" ;
    linkml:imported_from "linkml:types" ;
    linkml:repr "str" ;
    linkml:definition_uri linkml:Curie ;
    linkml:uri xsd:string .

okns:date_or_datetime a linkml:TypeDefinition ;
    skos:definition "Either a date or a datetime" ;
    skos:editorialNote "If you are authoring schemas in LinkML YAML, the type is referenced with the lower case \"date_or_datetime\"." ;
    skos:inScheme linkml:types ;
    linkml:base "str" ;
    linkml:imported_from "linkml:types" ;
    linkml:repr "str" ;
    linkml:definition_uri linkml:DateOrDatetime ;
    linkml:uri linkml:DateOrDatetime .

okns:dct_Box a linkml:TypeDefinition ;
    dcterms:source dcterms: ;
    dcterms:title "DCMI Box" ;
    rdfs:seeAlso <https://www.dublincore.org/specifications/dublin-core/dcmi-box/> ;
    skos:definition "The set of regions in space defined by their geographic coordinates according to the DCMI Box Encoding Scheme." ;
    skos:inScheme okns:dc ;
    linkml:base "str" ;
    linkml:definition_uri okns:DctBox ;
    linkml:typeof okns:string ;
    linkml:uri dcterms:Box .

okns:dct_ISO3166 a linkml:TypeDefinition ;
    dcterms:source dcterms: ;
    dcterms:title "ISO 3166" ;
    rdfs:seeAlso <https://www.iso.org/obp/ui/#search> ;
    skos:definition "The set of codes listed in ISO 3166-1 for the representation of names of countries." ;
    skos:inScheme okns:dc ;
    linkml:base "str" ;
    linkml:definition_uri okns:DctISO3166 ;
    linkml:typeof okns:string ;
    linkml:uri dcterms:ISO3166 .

okns:dct_ISO639_2 a linkml:TypeDefinition ;
    dcterms:source dcterms: ;
    dcterms:title "ISO 639-2" ;
    rdfs:seeAlso <http://lcweb.loc.gov/standards/iso639-2/langhome.html> ;
    skos:definition "The three-letter alphabetic codes listed in ISO639-2 for the representation of names of languages." ;
    skos:inScheme okns:dc ;
    linkml:base "str" ;
    linkml:definition_uri okns:DctISO639-2 ;
    linkml:typeof okns:string ;
    linkml:uri dcterms:ISO639-2 .

okns:dct_ISO639_3 a linkml:TypeDefinition ;
    dcterms:source dcterms: ;
    dcterms:title "ISO 639-3" ;
    rdfs:seeAlso <http://www.sil.org/iso639-3/> ;
    skos:definition "The set of three-letter codes listed in ISO 639-3 for the representation of names of languages." ;
    skos:inScheme okns:dc ;
    linkml:base "str" ;
    linkml:definition_uri okns:DctISO639-3 ;
    linkml:typeof okns:string ;
    linkml:uri dcterms:ISO639-3 .

okns:dct_Period a linkml:TypeDefinition ;
    dcterms:source dcterms: ;
    dcterms:title "DCMI Period" ;
    rdfs:seeAlso <https://www.dublincore.org/specifications/dublin-core/dcmi-period/> ;
    skos:definition "The set of time intervals defined by their limits according to the DCMI Period Encoding Scheme." ;
    skos:inScheme okns:dc ;
    linkml:base "str" ;
    linkml:definition_uri okns:DctPeriod ;
    linkml:typeof okns:string ;
    linkml:uri dcterms:Period .

okns:dct_Point a linkml:TypeDefinition ;
    dcterms:source dcterms: ;
    dcterms:title "DCMI Point" ;
    rdfs:seeAlso <https://www.dublincore.org/specifications/dublin-core/dcmi-point/> ;
    skos:definition "The set of points in space defined by their geographic coordinates according to the DCMI Point Encoding Scheme." ;
    skos:inScheme okns:dc ;
    linkml:base "str" ;
    linkml:definition_uri okns:DctPoint ;
    linkml:typeof okns:string ;
    linkml:uri dcterms:Point .

okns:dct_RFC1766 a linkml:TypeDefinition ;
    dcterms:source dcterms: ;
    dcterms:title "RFC 1766" ;
    rdfs:seeAlso <http://www.ietf.org/rfc/rfc1766.txt> ;
    skos:definition "The set of tags, constructed according to RFC 1766, for the identification of languages." ;
    skos:inScheme okns:dc ;
    linkml:base "str" ;
    linkml:definition_uri okns:DctRFC1766 ;
    linkml:typeof okns:string ;
    linkml:uri dcterms:RFC1766 .

okns:dct_RFC3066 a linkml:TypeDefinition ;
    dcterms:source dcterms: ;
    dcterms:title "RFC 3066" ;
    rdfs:seeAlso <http://www.ietf.org/rfc/rfc3066.txt> ;
    skos:definition "RFC 3066 has been obsoleted by RFC 4646." ;
    skos:inScheme okns:dc ;
    skos:note "description: The set of tags constructed according to RFC 3066 for the identification of languages." ;
    linkml:base "str" ;
    linkml:definition_uri okns:DctRFC3066 ;
    linkml:typeof okns:string ;
    linkml:uri dcterms:RFC3066 .

okns:dct_RFC4646 a linkml:TypeDefinition ;
    dcterms:source dcterms: ;
    dcterms:title "RFC 4646" ;
    rdfs:seeAlso <http://www.ietf.org/rfc/rfc4646.txt> ;
    skos:definition "RFC 4646 obsoletes RFC 3066." ;
    skos:inScheme okns:dc ;
    skos:note "description: The set of tags constructed according to RFC 4646 for the identification of languages." ;
    linkml:base "str" ;
    linkml:definition_uri okns:DctRFC4646 ;
    linkml:typeof okns:string ;
    linkml:uri dcterms:RFC4646 .

okns:dct_RFC5646 a linkml:TypeDefinition ;
    dcterms:source dcterms: ;
    dcterms:title "RFC 5646" ;
    rdfs:seeAlso <http://www.ietf.org/rfc/rfc5646.txt> ;
    skos:definition "RFC 5646 obsoletes RFC 4646." ;
    skos:inScheme okns:dc ;
    skos:note "description: The set of tags constructed according to RFC 5646 for the identification of languages." ;
    linkml:base "str" ;
    linkml:definition_uri okns:DctRFC5646 ;
    linkml:typeof okns:string ;
    linkml:uri dcterms:RFC5646 .

okns:dct_URI a linkml:TypeDefinition ;
    dcterms:source dcterms: ;
    dcterms:title "URI" ;
    rdfs:seeAlso <http://www.ietf.org/rfc/rfc3986.txt> ;
    skos:definition "The set of identifiers constructed according to the generic syntax for Uniform Resource Identifiers as specified by the Internet Engineering Task Force." ;
    skos:inScheme okns:dc ;
    linkml:base "str" ;
    linkml:definition_uri okns:DctURI ;
    linkml:typeof okns:string ;
    linkml:uri dcterms:URI .

okns:dct_W3CDTF a linkml:TypeDefinition ;
    dcterms:source dcterms: ;
    dcterms:title "W3C-DTF" ;
    rdfs:seeAlso <http://www.w3.org/TR/NOTE-datetime> ;
    skos:definition "The set of dates and times constructed according to the W3C Date and Time Formats Specification." ;
    skos:inScheme okns:dc ;
    linkml:base "str" ;
    linkml:definition_uri okns:DctW3CDTF ;
    linkml:typeof okns:string ;
    linkml:uri dcterms:W3CDTF .

okns:double a linkml:TypeDefinition ;
    skos:closeMatch schema1:Float ;
    skos:definition "A real number that conforms to the xsd:double specification" ;
    skos:editorialNote "If you are authoring schemas in LinkML YAML, the type is referenced with the lower case \"double\"." ;
    skos:inScheme linkml:types ;
    linkml:base "float" ;
    linkml:imported_from "linkml:types" ;
    linkml:definition_uri linkml:Double ;
    linkml:uri xsd:double .

okns:float16 a linkml:TypeDefinition ;
    rdfs:seeAlso <https://numpy.org/doc/stable/reference/arrays.scalars.html#numpy.half> ;
    skos:altLabel "e",
        "half" ;
    skos:definition "A 16-bit floating point number" ;
    skos:inScheme okns:extended_types ;
    linkml:base "float" ;
    linkml:definition_uri linkml:Float16 ;
    linkml:typeof okns:float ;
    linkml:uri xsd:float .

okns:float32 a linkml:TypeDefinition ;
    rdfs:seeAlso <https://numpy.org/doc/stable/reference/arrays.scalars.html#numpy.float32> ;
    skos:altLabel "f" ;
    skos:definition "A 32-bit floating point number" ;
    skos:inScheme okns:extended_types ;
    linkml:base "float" ;
    linkml:definition_uri linkml:Float32 ;
    linkml:typeof okns:float ;
    linkml:uri xsd:float .

okns:float64 a linkml:TypeDefinition ;
    rdfs:seeAlso <https://numpy.org/doc/stable/reference/arrays.scalars.html#numpy.float64> ;
    skos:altLabel "d" ;
    skos:definition "A 64-bit floating point number" ;
    skos:inScheme okns:extended_types ;
    linkml:base "float" ;
    linkml:definition_uri linkml:Float64 ;
    linkml:typeof okns:float ;
    linkml:uri xsd:float .

okns:hexbinary a linkml:TypeDefinition ;
    skos:definition "Arbitrary hex-encoded binary data." ;
    skos:inScheme okns:extended_types ;
    skos:note "added by Mahir Morshed <mmorshed@scripps.edu>",
        "used 'string' as base type since no 'binary' base type exists" ;
    linkml:base "string" ;
    linkml:definition_uri linkml:Hexbinary ;
    linkml:uri xsd:hexBinary .

okns:int16 a linkml:TypeDefinition ;
    rdfs:seeAlso <https://numpy.org/doc/stable/reference/arrays.scalars.html#numpy.short> ;
    skos:altLabel "h",
        "short" ;
    skos:definition "A 16-bit signed integer" ;
    skos:inScheme okns:extended_types ;
    skos:note "uri added by Mahir Morshed <mmorshed@scripps.edu>" ;
    linkml:base "int" ;
    linkml:definition_uri linkml:Int16 ;
    linkml:maximum_value "32767"^^<https://purl.org/okn/schema/@id> ;
    linkml:minimum_value "-32768"^^<https://purl.org/okn/schema/@id> ;
    linkml:typeof okns:signedinteger ;
    linkml:uri xsd:short .

okns:int64 a linkml:TypeDefinition ;
    rdfs:seeAlso <https://numpy.org/doc/stable/reference/arrays.scalars.html#numpy.int_> ;
    skos:altLabel "int_",
        "l",
        "long" ;
    skos:definition "A 64-bit signed integer" ;
    skos:inScheme okns:extended_types ;
    skos:note "uri added by Mahir Morshed <mmorshed@scripps.edu>" ;
    linkml:base "int" ;
    linkml:definition_uri linkml:Int64 ;
    linkml:maximum_value "9223372036854775807"^^<https://purl.org/okn/schema/@id> ;
    linkml:minimum_value "-9223372036854775808"^^<https://purl.org/okn/schema/@id> ;
    linkml:typeof okns:signedinteger ;
    linkml:uri xsd:long .

okns:int8 a linkml:TypeDefinition ;
    rdfs:seeAlso <https://numpy.org/doc/stable/reference/arrays.scalars.html#numpy.byte> ;
    skos:altLabel "b",
        "byte" ;
    skos:definition "An 8-bit signed integer" ;
    skos:inScheme okns:extended_types ;
    skos:note "uri added by Mahir Morshed <mmorshed@scripps.edu>" ;
    linkml:base "int" ;
    linkml:definition_uri linkml:Int8 ;
    linkml:maximum_value "127"^^<https://purl.org/okn/schema/@id> ;
    linkml:minimum_value "-128"^^<https://purl.org/okn/schema/@id> ;
    linkml:typeof okns:signedinteger ;
    linkml:uri xsd:byte .

okns:jsonpath a linkml:TypeDefinition ;
    dcterms:conformsTo "https://www.ietf.org/archive/id/draft-goessner-dispatch-jsonpath-00.html" ;
    skos:definition "A string encoding a JSON Path. The value of the string MUST conform to JSON Point syntax and SHOULD dereference to zero or more valid objects within the current instance document when encoded in tree form." ;
    skos:editorialNote "If you are authoring schemas in LinkML YAML, the type is referenced with the lower case \"jsonpath\"." ;
    skos:inScheme linkml:types ;
    linkml:base "str" ;
    linkml:imported_from "linkml:types" ;
    linkml:repr "str" ;
    linkml:definition_uri linkml:Jsonpath ;
    linkml:uri xsd:string .

okns:jsonpointer a linkml:TypeDefinition ;
    dcterms:conformsTo "https://datatracker.ietf.org/doc/html/rfc6901" ;
    skos:definition "A string encoding a JSON Pointer. The value of the string MUST conform to JSON Point syntax and SHOULD dereference to a valid object within the current instance document when encoded in tree form." ;
    skos:editorialNote "If you are authoring schemas in LinkML YAML, the type is referenced with the lower case \"jsonpointer\"." ;
    skos:inScheme linkml:types ;
    linkml:base "str" ;
    linkml:imported_from "linkml:types" ;
    linkml:repr "str" ;
    linkml:definition_uri linkml:Jsonpointer ;
    linkml:uri xsd:string .

okns:langrange a linkml:SlotDefinition ;
    skos:definition "Used to refer to a subset of strings containing a particular language tag." ;
    skos:inScheme okns:extended_types ;
    skos:mappingRelation rdf:langRange ;
    skos:note "added by Mahir Morshed <mmorshed@scripps.edu>" ;
    linkml:definition_uri linkml:langrange ;
    linkml:range okns:string ;
    linkml:slot_uri rdf:langRange .

okns:language a linkml:TypeDefinition ;
    skos:definition "Formal natural language identifier, as defined by [BCP 47] (currently represented by [RFC 4646] and [RFC 4647]) or its successor(s)." ;
    skos:inScheme okns:extended_types ;
    skos:note "added by Mahir Morshed <mmorshed@scripps.edu>" ;
    linkml:base "str" ;
    linkml:definition_uri linkml:Language ;
    linkml:typeof okns:token ;
    linkml:uri xsd:language .

okns:length a linkml:SlotDefinition ;
    skos:definition "Number of units of length, where units of length varies depending on the type that is being derived from." ;
    skos:inScheme okns:extended_types ;
    skos:mappingRelation xsd:length ;
    skos:note "added by Mahir Morshed <mmorshed@scripps.edu>" ;
    linkml:definition_uri linkml:length ;
    linkml:range okns:string ;
    linkml:slot_uri xsd:length .

okns:maxexclusive a linkml:SlotDefinition ;
    skos:definition "Exclusive upper bound of the ·value space· for a datatype with the ordered property." ;
    skos:inScheme okns:extended_types ;
    skos:mappingRelation xsd:maxExclusive ;
    skos:note "added by Mahir Morshed <mmorshed@scripps.edu>" ;
    linkml:definition_uri linkml:maxexclusive ;
    linkml:range okns:string ;
    linkml:slot_uri xsd:maxExclusive .

okns:maxlength a linkml:SlotDefinition ;
    skos:definition "Maximum number of units of length, where units of length varies depending on the type that is being derived from." ;
    skos:inScheme okns:extended_types ;
    skos:mappingRelation xsd:maxLength ;
    skos:note "added by Mahir Morshed <mmorshed@scripps.edu>" ;
    linkml:definition_uri linkml:maxlength ;
    linkml:range okns:string ;
    linkml:slot_uri xsd:maxLength .

okns:minexclusive a linkml:SlotDefinition ;
    skos:definition "Exclusive lower bound of the ·value space· for a datatype with the ordered property." ;
    skos:inScheme okns:extended_types ;
    skos:mappingRelation xsd:minExclusive ;
    skos:note "added by Mahir Morshed <mmorshed@scripps.edu>" ;
    linkml:definition_uri linkml:minexclusive ;
    linkml:range okns:string ;
    linkml:slot_uri xsd:minExclusive .

okns:minlength a linkml:SlotDefinition ;
    skos:definition "Minimum number of units of length, where units of length varies depending on the type that is being derived from." ;
    skos:inScheme okns:extended_types ;
    skos:mappingRelation xsd:minLength ;
    skos:note "added by Mahir Morshed <mmorshed@scripps.edu>" ;
    linkml:definition_uri linkml:minlength ;
    linkml:range okns:string ;
    linkml:slot_uri xsd:minLength .

okns:name a linkml:TypeDefinition ;
    skos:definition "XML Name." ;
    skos:inScheme okns:extended_types ;
    skos:note "added by Mahir Morshed <mmorshed@scripps.edu>" ;
    linkml:base "str" ;
    linkml:definition_uri linkml:Name ;
    linkml:typeof okns:token ;
    linkml:uri xsd:Name .

okns:ncname a linkml:TypeDefinition ;
    skos:definition "Prefix part of CURIE" ;
    skos:editorialNote "If you are authoring schemas in LinkML YAML, the type is referenced with the lower case \"ncname\"." ;
    skos:inScheme linkml:types ;
    linkml:base "NCName" ;
    linkml:imported_from "linkml:types" ;
    linkml:repr "str" ;
    linkml:definition_uri linkml:Ncname ;
    linkml:uri xsd:string .

okns:negativeinteger a linkml:TypeDefinition ;
    skos:definition "An integer that is negative" ;
    skos:inScheme okns:extended_types ;
    skos:note "added by Mahir Morshed <mmorshed@scripps.edu>" ;
    linkml:base "int" ;
    linkml:definition_uri linkml:Negativeinteger ;
    linkml:maximum_value "-1"^^<https://purl.org/okn/schema/@id> ;
    linkml:typeof okns:integer ;
    linkml:uri xsd:negativeInteger .

okns:nmtoken a linkml:TypeDefinition ;
    skos:definition "NMTOKEN attribute type from [XML]." ;
    skos:inScheme okns:extended_types ;
    skos:note "added by Mahir Morshed <mmorshed@scripps.edu>" ;
    linkml:base "str" ;
    linkml:definition_uri linkml:Nmtoken ;
    linkml:typeof okns:token ;
    linkml:uri xsd:NMTOKEN .

okns:nodeidentifier a linkml:TypeDefinition ;
    skos:definition "A URI, CURIE or BNODE that represents a node in a model." ;
    skos:editorialNote "If you are authoring schemas in LinkML YAML, the type is referenced with the lower case \"nodeidentifier\"." ;
    skos:inScheme linkml:types ;
    linkml:base "NodeIdentifier" ;
    linkml:imported_from "linkml:types" ;
    linkml:repr "str" ;
    linkml:definition_uri linkml:Nodeidentifier ;
    linkml:uri shex:nonLiteral .

okns:nonpositiveinteger a linkml:TypeDefinition ;
    skos:definition "An integer that is not positive" ;
    skos:inScheme okns:extended_types ;
    skos:note "added by Mahir Morshed <mmorshed@scripps.edu>" ;
    linkml:base "int" ;
    linkml:definition_uri linkml:Nonpositiveinteger ;
    linkml:maximum_value "0"^^<https://purl.org/okn/schema/@id> ;
    linkml:typeof okns:integer ;
    linkml:uri xsd:nonPositiveInteger .

okns:objectidentifier a linkml:TypeDefinition ;
    skos:definition "A URI or CURIE that represents an object in the model." ;
    skos:editorialNote "If you are authoring schemas in LinkML YAML, the type is referenced with the lower case \"objectidentifier\"." ;
    skos:inScheme linkml:types ;
    skos:note "Used for inheritance and type checking" ;
    linkml:base "ElementIdentifier" ;
    linkml:imported_from "linkml:types" ;
    linkml:repr "str" ;
    linkml:definition_uri linkml:Objectidentifier ;
    linkml:uri shex:iri .

okns:positiveinteger a linkml:TypeDefinition ;
    skos:definition "An integer that is positive" ;
    skos:inScheme okns:extended_types ;
    skos:note "added by Mahir Morshed <mmorshed@scripps.edu>" ;
    linkml:base "int" ;
    linkml:definition_uri linkml:Positiveinteger ;
    linkml:minimum_value "1"^^<https://purl.org/okn/schema/@id> ;
    linkml:typeof okns:integer ;
    linkml:uri xsd:positiveInteger .

okns:rational a linkml:TypeDefinition ;
    skos:definition "Rational number." ;
    skos:inScheme okns:extended_types ;
    skos:note "added by Mahir Morshed <mmorshed@scripps.edu>" ;
    linkml:base "Decimal" ;
    linkml:definition_uri linkml:Rational ;
    linkml:typeof okns:decimal ;
    linkml:uri owl:rational .

okns:rdf_HTML a linkml:TypeDefinition ;
    dcterms:source rdf: ;
    dcterms:title "HTML" ;
    rdfs:seeAlso <http://www.w3.org/TR/rdf11-concepts/#section-html> ;
    skos:definition "The datatype of RDF literals storing fragments of HTML content" ;
    skos:inScheme okns:owl-rdf-rdfs ;
    linkml:base "str" ;
    linkml:definition_uri okns:RdfHTML ;
    linkml:typeof okns:string ;
    linkml:uri rdf:HTML .

okns:rdf_JSON a linkml:TypeDefinition ;
    dcterms:source rdf: ;
    dcterms:title "JSON" ;
    rdfs:seeAlso <https://www.w3.org/TR/json-ld11/#the-rdf-json-datatype> ;
    skos:definition "The datatype of RDF literals storing JSON content." ;
    skos:inScheme okns:owl-rdf-rdfs ;
    linkml:base "str" ;
    linkml:definition_uri okns:RdfJSON ;
    linkml:typeof okns:string ;
    linkml:uri rdf:JSON .

okns:rdf_PlainLiteral a linkml:TypeDefinition ;
    dcterms:source rdf: ;
    dcterms:title "PlainLiteral" ;
    rdfs:seeAlso <http://www.w3.org/TR/rdf-plain-literal/> ;
    skos:definition "The class of plain (i.e. untyped) literal values, as used in RIF and OWL 2" ;
    skos:inScheme okns:owl-rdf-rdfs ;
    linkml:base "str" ;
    linkml:definition_uri okns:RdfPlainLiteral ;
    linkml:typeof okns:string ;
    linkml:uri rdf:PlainLiteral .

okns:rdf_langString a linkml:TypeDefinition ;
    dcterms:source rdf: ;
    dcterms:title "langString" ;
    rdfs:seeAlso <http://www.w3.org/TR/rdf11-concepts/#section-Graph-Literal> ;
    skos:definition "The datatype of language-tagged string values" ;
    skos:inScheme okns:owl-rdf-rdfs ;
    linkml:base "str" ;
    linkml:definition_uri okns:RdfLangString ;
    linkml:typeof okns:string ;
    linkml:uri rdf:langString .

okns:real a linkml:TypeDefinition ;
    skos:definition "Real number." ;
    skos:inScheme okns:extended_types ;
    skos:note "added by Mahir Morshed <mmorshed@scripps.edu>" ;
    linkml:base "Decimal" ;
    linkml:definition_uri linkml:Real ;
    linkml:typeof okns:decimal ;
    linkml:uri owl:real .

okns:sparqlpath a linkml:TypeDefinition ;
    dcterms:conformsTo "https://www.w3.org/TR/sparql11-query/#propertypaths" ;
    skos:definition "A string encoding a SPARQL Property Path. The value of the string MUST conform to SPARQL syntax and SHOULD dereference to zero or more valid objects within the current instance document when encoded as RDF." ;
    skos:editorialNote "If you are authoring schemas in LinkML YAML, the type is referenced with the lower case \"sparqlpath\"." ;
    skos:inScheme linkml:types ;
    linkml:base "str" ;
    linkml:imported_from "linkml:types" ;
    linkml:repr "str" ;
    linkml:definition_uri linkml:Sparqlpath ;
    linkml:uri xsd:string .

okns:time_generalDay a linkml:TypeDefinition ;
    dcterms:title "Generalized day" ;
    skos:definition "Day of month - formulated as a text string with a pattern constraint to reproduce the same lexical form as gDay, except that values up to 99 are permitted, in order to support calendars with more than 31 days in a month. ␊Note that the value-space is not defined, so a generic OWL2 processor cannot compute ordering relationships of values of this type." ;
    skos:inScheme okns:time ;
    skos:note """description: Day of month - formulated as a text string with a pattern constraint to reproduce the same lexical form as gDay, except that values up to 99 are permitted, in order to support calendars with more than 31 days in a month. 
Note that the value-space is not defined, so a generic OWL2 processor cannot compute ordering relationships of values of this type.""",
        """description: Día del mes - formulado como una cadena de texto con una restricción patrón para reproducir la misma forma léxica que gDay, excepto que se permiten valores hasta el 99, con el propósito de proporcionar soporte a calendarios con meses con más de 31 días.
            Nótese que el espacio de valores no está definido, por tanto, un procesador genérico de OWL2 no puede computar relaciones de orden de valores de este tipo.""",
        "title: Día generalizado" ;
    linkml:base "str" ;
    linkml:definition_uri okns:TimeGeneralDay ;
    linkml:typeof okns:string ;
    linkml:uri time:generalDay .

okns:time_generalMonth a linkml:TypeDefinition ;
    dcterms:title "Generalized month" ;
    skos:definition "Month of year - formulated as a text string with a pattern constraint to reproduce the same lexical form as gMonth, except that values up to 20 are permitted, in order to support calendars with more than 12 months in the year. ␊Note that the value-space is not defined, so a generic OWL2 processor cannot compute ordering relationships of values of this type." ;
    skos:inScheme okns:time ;
    skos:note """description: Mes del año - formulado como una cadena de texto con una restricción patrón para reproducir la misma forma léxica que gMonth, excepto que se permiten valores hasta el 20, con el propósito de proporcionar soporte a calendarios con años con más de 12 meses.
            Nótese que el espacio de valores no está definido, por tanto, un procesador genérico de OWL2 no puede computar relaciones de orden de valores de este tipo.""",
        """description: Month of year - formulated as a text string with a pattern constraint to reproduce the same lexical form as gMonth, except that values up to 20 are permitted, in order to support calendars with more than 12 months in the year. 
Note that the value-space is not defined, so a generic OWL2 processor cannot compute ordering relationships of values of this type.""",
        "title: Mes generalizado" ;
    linkml:base "str" ;
    linkml:definition_uri okns:TimeGeneralMonth ;
    linkml:typeof okns:string ;
    linkml:uri time:generalMonth .

okns:time_generalYear a linkml:TypeDefinition ;
    dcterms:title "Generalized year" ;
    skos:definition "Year number - formulated as a text string with a pattern constraint to reproduce the same lexical form as gYear, but not restricted to values from the Gregorian calendar. ␊Note that the value-space is not defined, so a generic OWL2 processor cannot compute ordering relationships of values of this type." ;
    skos:inScheme okns:time ;
    skos:note """description: Número de año - formulado como una cadena de texto con una restricción patrón para reproducir la misma forma léxica que gYear, aunque no está restringido a valores del calendario gregoriano.
            Nótese que el espacio de valores no está definido, por tanto, un procesador genérico de OWL2 no puede computar relaciones de orden de valores de este tipo.""",
        """description: Year number - formulated as a text string with a pattern constraint to reproduce the same lexical form as gYear, but not restricted to values from the Gregorian calendar. 
Note that the value-space is not defined, so a generic OWL2 processor cannot compute ordering relationships of values of this type.""",
        "title: Año generalizado" ;
    linkml:base "str" ;
    linkml:definition_uri okns:TimeGeneralYear ;
    linkml:typeof okns:string ;
    linkml:uri time:generalYear .

okns:uint16 a linkml:TypeDefinition ;
    skos:altLabel "H",
        "ushort" ;
    skos:definition "A 16-bit unsigned integer" ;
    skos:inScheme okns:extended_types ;
    skos:note "uri added by Mahir Morshed <mmorshed@scripps.edu>" ;
    linkml:base "int" ;
    linkml:definition_uri linkml:Uint16 ;
    linkml:maximum_value "65535"^^<https://purl.org/okn/schema/@id> ;
    linkml:minimum_value "0"^^<https://purl.org/okn/schema/@id> ;
    linkml:typeof okns:unsignedinteger ;
    linkml:uri xsd:unsignedShort .

okns:uint32 a linkml:TypeDefinition ;
    skos:altLabel "I",
        "uintc" ;
    skos:definition "A 32-bit unsigned integer" ;
    skos:inScheme okns:extended_types ;
    skos:note "uri added by Mahir Morshed <mmorshed@scripps.edu>" ;
    linkml:base "int" ;
    linkml:definition_uri linkml:Uint32 ;
    linkml:maximum_value "4294967295"^^<https://purl.org/okn/schema/@id> ;
    linkml:minimum_value "0"^^<https://purl.org/okn/schema/@id> ;
    linkml:typeof okns:unsignedinteger ;
    linkml:uri xsd:unsignedInt .

okns:uint64 a linkml:TypeDefinition ;
    skos:altLabel "L",
        "uint_",
        "ulong" ;
    skos:definition "A 64-bit unsigned integer" ;
    skos:inScheme okns:extended_types ;
    skos:note "uri added by Mahir Morshed <mmorshed@scripps.edu>" ;
    linkml:base "int" ;
    linkml:definition_uri linkml:Uint64 ;
    linkml:maximum_value "18446744073709551615"^^<https://purl.org/okn/schema/@id> ;
    linkml:minimum_value "0"^^<https://purl.org/okn/schema/@id> ;
    linkml:typeof okns:unsignedinteger ;
    linkml:uri xsd:unsignedLong .

okns:uint8 a linkml:TypeDefinition ;
    rdfs:seeAlso <https://numpy.org/doc/stable/reference/arrays.scalars.html#numpy.uint8> ;
    skos:altLabel "B",
        "ubyte" ;
    skos:definition "An 8-bit unsigned integer" ;
    skos:inScheme okns:extended_types ;
    skos:note "uri added by Mahir Morshed <mmorshed@scripps.edu>" ;
    linkml:base "int" ;
    linkml:definition_uri linkml:Uint8 ;
    linkml:maximum_value "255"^^<https://purl.org/okn/schema/@id> ;
    linkml:minimum_value "0"^^<https://purl.org/okn/schema/@id> ;
    linkml:typeof okns:unsignedinteger ;
    linkml:uri xsd:unsignedByte .

okns:uriorcurie a linkml:TypeDefinition ;
    skos:definition "a URI or a CURIE" ;
    skos:editorialNote "If you are authoring schemas in LinkML YAML, the type is referenced with the lower case \"uriorcurie\"." ;
    skos:inScheme linkml:types ;
    linkml:base "URIorCURIE" ;
    linkml:imported_from "linkml:types" ;
    linkml:repr "str" ;
    linkml:definition_uri linkml:Uriorcurie ;
    linkml:uri xsd:anyURI .

okns:AoLikeableAssociation a linkml:ClassDefinition ;
    dcterms:source ao: ;
    dcterms:title "Likeable Association" ;
    skos:definition "A likeable association. That means this association type is intended to be used for voting (ao:likeminded), feedbacking (rev:Feedback), reviewing (e.g. rev:rating) an association statement (related by ao:included_association) in the context of something." ;
    skos:inScheme okns:ao ;
    skos:mappingRelation ao:LikeableAssociation ;
    linkml:class_uri ao:LikeableAssociation ;
    linkml:definition_uri okns:AoLikeableAssociation ;
    linkml:is_a okns:RevReview ;
    linkml:slot_usage [ ] .

okns:CcAgent a linkml:ClassDefinition ;
    dcterms:title "agent" ;
    skos:definition "something (e.g. a person, corporation or computer) capable of creating things" ;
    skos:inScheme okns:cc ;
    skos:mappingRelation cc:Agent ;
    linkml:class_uri cc:Agent ;
    linkml:definition_uri okns:CcAgent ;
    linkml:slot_usage [ ] .

okns:Daml-oilDatatype a linkml:ClassDefinition ;
    dcterms:title "Datatype" ;
    skos:definition "The class of all datatype classes" ;
    skos:inScheme okns:daml ;
    skos:mappingRelation daml-oil:Datatype ;
    linkml:class_uri daml-oil:Datatype ;
    linkml:definition_uri okns:Daml-oilDatatype ;
    linkml:is_a okns:RdfsClass ;
    linkml:slot_usage [ ] .

okns:Daml-oilLiteral a linkml:ClassDefinition ;
    skos:inScheme okns:daml ;
    skos:mappingRelation daml-oil:Literal ;
    linkml:class_uri daml-oil:Literal ;
    linkml:definition_uri okns:Daml-oilLiteral ;
    linkml:slot_usage [ ] .

okns:Daml-oilTransitiveProperty a linkml:ClassDefinition ;
    dcterms:title "TransitiveProperty" ;
    skos:definition "if P is a TransitiveProperty, then if P(x, y) and P(y, z) then P(x, z). cf OIL TransitiveProperty." ;
    skos:inScheme okns:daml ;
    skos:mappingRelation daml-oil:TransitiveProperty ;
    linkml:class_uri daml-oil:TransitiveProperty ;
    linkml:definition_uri okns:Daml-oilTransitiveProperty ;
    linkml:is_a okns:Daml-oilObjectProperty ;
    linkml:slot_usage [ ] ;
    linkml:slots okns:daml_oil_domain,
        okns:daml_oil_range,
        okns:daml_oil_subPropertyOf .

okns:Daml-oilUnambiguousProperty a linkml:ClassDefinition ;
    dcterms:title "UnambiguousProperty" ;
    skos:definition "if P is an UnambiguousProperty, then if P(x, y) and P(z, y) then x=z. aka injective. e.g. if firstBorne(m, Susan) and firstBorne(n, Susan) then m and n are the same." ;
    skos:inScheme okns:daml ;
    skos:mappingRelation daml-oil:UnambiguousProperty ;
    linkml:class_uri daml-oil:UnambiguousProperty ;
    linkml:definition_uri okns:Daml-oilUnambiguousProperty ;
    linkml:is_a okns:Daml-oilObjectProperty ;
    linkml:slot_usage [ ] ;
    linkml:slots okns:daml_oil_domain,
        okns:daml_oil_range,
        okns:daml_oil_subPropertyOf .

okns:DcmitypeDataset a linkml:ClassDefinition ;
    dcterms:source dcmitype: ;
    dcterms:title "Dataset" ;
    skos:definition "Examples include lists, tables, and databases.  A dataset may be useful for direct machine processing." ;
    skos:inScheme okns:dc ;
    skos:mappingRelation dcmitype:Dataset ;
    skos:note "description: Data encoded in a defined structure." ;
    linkml:class_uri dcmitype:Dataset ;
    linkml:definition_uri okns:DcmitypeDataset ;
    linkml:slot_usage [ ] .

okns:DcmitypeEvent a linkml:ClassDefinition ;
    dcterms:source dcmitype: ;
    dcterms:title "Event" ;
    skos:definition "Metadata for an event provides descriptive information that is the basis for discovery of the purpose, location, duration, and responsible agents associated with an event. Examples include an exhibition, webcast, conference, workshop, open day, performance, battle, trial, wedding, tea party, conflagration." ;
    skos:inScheme okns:dc ;
    skos:mappingRelation dcmitype:Event ;
    skos:note "description: A non-persistent, time-based occurrence." ;
    linkml:class_uri dcmitype:Event ;
    linkml:definition_uri okns:DcmitypeEvent ;
    linkml:slot_usage [ ] .

okns:DcmitypeInteractiveResource a linkml:ClassDefinition ;
    dcterms:source dcmitype: ;
    dcterms:title "Interactive Resource" ;
    skos:definition "Examples include forms on Web pages, applets, multimedia learning objects, chat services, or virtual reality environments." ;
    skos:inScheme okns:dc ;
    skos:mappingRelation dcmitype:InteractiveResource ;
    skos:note "description: A resource requiring interaction from the user to be understood, executed, or experienced." ;
    linkml:class_uri dcmitype:InteractiveResource ;
    linkml:definition_uri okns:DcmitypeInteractiveResource ;
    linkml:slot_usage [ ] .

okns:DcmitypeMovingImage a linkml:ClassDefinition ;
    dcterms:source dcmitype: ;
    dcterms:title "Moving Image" ;
    skos:definition "Examples include animations, movies, television programs, videos, zoetropes, or visual output from a simulation.  Instances of the type Moving Image must also be describable as instances of the broader type Image." ;
    skos:inScheme okns:dc ;
    skos:mappingRelation dcmitype:MovingImage ;
    skos:note "description: A series of visual representations imparting an impression of motion when shown in succession." ;
    linkml:class_uri dcmitype:MovingImage ;
    linkml:definition_uri okns:DcmitypeMovingImage ;
    linkml:is_a okns:DcmitypeImage ;
    linkml:slot_usage [ ] .

okns:DcmitypePhysicalObject a linkml:ClassDefinition ;
    dcterms:source dcmitype: ;
    dcterms:title "Physical Object" ;
    skos:definition "Note that digital representations of, or surrogates for, these objects should use Image, Text or one of the other types." ;
    skos:inScheme okns:dc ;
    skos:mappingRelation dcmitype:PhysicalObject ;
    skos:note "description: An inanimate, three-dimensional object or substance." ;
    linkml:class_uri dcmitype:PhysicalObject ;
    linkml:definition_uri okns:DcmitypePhysicalObject ;
    linkml:slot_usage [ ] .

okns:DcmitypeService a linkml:ClassDefinition ;
    dcterms:source dcmitype: ;
    dcterms:title "Service" ;
    skos:definition "Examples include a photocopying service, a banking service, an authentication service, interlibrary loans, a Z39.50 or Web server." ;
    skos:inScheme okns:dc ;
    skos:mappingRelation dcmitype:Service ;
    skos:note "description: A system that provides one or more functions." ;
    linkml:class_uri dcmitype:Service ;
    linkml:definition_uri okns:DcmitypeService ;
    linkml:slot_usage [ ] .

okns:DcmitypeSoftware a linkml:ClassDefinition ;
    dcterms:source dcmitype: ;
    dcterms:title "Software" ;
    skos:definition "Examples include a C source file, MS-Windows .exe executable, or Perl script." ;
    skos:inScheme okns:dc ;
    skos:mappingRelation dcmitype:Software ;
    skos:note "description: A computer program in source or compiled form." ;
    linkml:class_uri dcmitype:Software ;
    linkml:definition_uri okns:DcmitypeSoftware ;
    linkml:slot_usage [ ] .

okns:DcmitypeSound a linkml:ClassDefinition ;
    dcterms:source dcmitype: ;
    dcterms:title "Sound" ;
    skos:definition "Examples include a music playback file format, an audio compact disc, and recorded speech or sounds." ;
    skos:inScheme okns:dc ;
    skos:mappingRelation dcmitype:Sound ;
    skos:note "description: A resource primarily intended to be heard." ;
    linkml:class_uri dcmitype:Sound ;
    linkml:definition_uri okns:DcmitypeSound ;
    linkml:slot_usage [ ] .

okns:DcmitypeStillImage a linkml:ClassDefinition ;
    dcterms:source dcmitype: ;
    dcterms:title "Still Image" ;
    skos:definition "Examples include paintings, drawings, graphic designs, plans and maps. Recommended best practice is to assign the type Text to images of textual materials. Instances of the type Still Image must also be describable as instances of the broader type Image." ;
    skos:inScheme okns:dc ;
    skos:mappingRelation dcmitype:StillImage ;
    skos:note "description: A static visual representation." ;
    linkml:class_uri dcmitype:StillImage ;
    linkml:definition_uri okns:DcmitypeStillImage ;
    linkml:is_a okns:DcmitypeImage ;
    linkml:slot_usage [ ] .

okns:DcmitypeText a linkml:ClassDefinition ;
    dcterms:source dcmitype: ;
    dcterms:title "Text" ;
    skos:definition "Examples include books, letters, dissertations, poems, newspapers, articles, archives of mailing lists. Note that facsimiles or images of texts are still of the genre Text." ;
    skos:inScheme okns:dc ;
    skos:mappingRelation dcmitype:Text ;
    skos:note "description: A resource consisting primarily of words for reading." ;
    linkml:class_uri dcmitype:Text ;
    linkml:definition_uri okns:DcmitypeText ;
    linkml:slot_usage [ ] .

okns:DctAgent a linkml:ClassDefinition ;
    dcterms:source dcterms: ;
    dcterms:title "Agent" ;
    skos:definition "A resource that acts or has the power to act." ;
    skos:inScheme okns:dc ;
    skos:mappingRelation dcterms:Agent ;
    linkml:class_uri dcterms:Agent ;
    linkml:definition_uri okns:DctAgent ;
    linkml:slot_usage [ ] .

okns:DctBibliographicResource a linkml:ClassDefinition ;
    dcterms:source dcterms: ;
    dcterms:title "Bibliographic Resource" ;
    skos:definition "A book, article, or other documentary resource." ;
    skos:inScheme okns:dc ;
    skos:mappingRelation dcterms:BibliographicResource ;
    linkml:class_uri dcterms:BibliographicResource ;
    linkml:definition_uri okns:DctBibliographicResource ;
    linkml:slot_usage [ ] .

okns:DctFileFormat a linkml:ClassDefinition ;
    dcterms:source dcterms: ;
    dcterms:title "File Format" ;
    skos:definition "A digital resource format." ;
    skos:inScheme okns:dc ;
    skos:mappingRelation dcterms:FileFormat ;
    linkml:class_uri dcterms:FileFormat ;
    linkml:definition_uri okns:DctFileFormat ;
    linkml:is_a okns:DctMediaType ;
    linkml:slot_usage [ ] .

okns:DctFrequency a linkml:ClassDefinition ;
    dcterms:source dcterms: ;
    dcterms:title "Frequency" ;
    skos:definition "A rate at which something recurs." ;
    skos:inScheme okns:dc ;
    skos:mappingRelation dcterms:Frequency ;
    linkml:class_uri dcterms:Frequency ;
    linkml:definition_uri okns:DctFrequency ;
    linkml:slot_usage [ ] .

okns:DctJurisdiction a linkml:ClassDefinition ;
    dcterms:source dcterms: ;
    dcterms:title "Jurisdiction" ;
    skos:definition "The extent or range of judicial, law enforcement, or other authority." ;
    skos:inScheme okns:dc ;
    skos:mappingRelation dcterms:Jurisdiction ;
    linkml:class_uri dcterms:Jurisdiction ;
    linkml:definition_uri okns:DctJurisdiction ;
    linkml:is_a okns:DctLocationPeriodOrJurisdiction ;
    linkml:slot_usage [ ] .

okns:DctLicenseDocument a linkml:ClassDefinition ;
    dcterms:source dcterms: ;
    dcterms:title "License Document" ;
    skos:definition "A legal document giving official permission to do something with a resource." ;
    skos:inScheme okns:dc ;
    skos:mappingRelation dcterms:LicenseDocument ;
    linkml:class_uri dcterms:LicenseDocument ;
    linkml:definition_uri okns:DctLicenseDocument ;
    linkml:is_a okns:DctRightsStatement ;
    linkml:slot_usage [ ] .

okns:DctLinguisticSystem a linkml:ClassDefinition ;
    dcterms:source dcterms: ;
    dcterms:title "Linguistic System" ;
    skos:definition "Written, spoken, sign, and computer languages are linguistic systems." ;
    skos:inScheme okns:dc ;
    skos:mappingRelation dcterms:LinguisticSystem ;
    skos:note "description: A system of signs, symbols, sounds, gestures, or rules used in communication." ;
    linkml:class_uri dcterms:LinguisticSystem ;
    linkml:definition_uri okns:DctLinguisticSystem ;
    linkml:slot_usage [ ] .

okns:DctLocation a linkml:ClassDefinition ;
    dcterms:source dcterms: ;
    dcterms:title "Location" ;
    skos:definition "A spatial region or named place." ;
    skos:inScheme okns:dc ;
    skos:mappingRelation dcterms:Location ;
    linkml:class_uri dcterms:Location ;
    linkml:definition_uri okns:DctLocation ;
    linkml:is_a okns:DctLocationPeriodOrJurisdiction ;
    linkml:slot_usage [ ] .

okns:DctMethodOfAccrual a linkml:ClassDefinition ;
    dcterms:source dcterms: ;
    dcterms:title "Method of Accrual" ;
    skos:definition "A method by which resources are added to a collection." ;
    skos:inScheme okns:dc ;
    skos:mappingRelation dcterms:MethodOfAccrual ;
    linkml:class_uri dcterms:MethodOfAccrual ;
    linkml:definition_uri okns:DctMethodOfAccrual ;
    linkml:slot_usage [ ] .

okns:DctMethodOfInstruction a linkml:ClassDefinition ;
    dcterms:source dcterms: ;
    dcterms:title "Method of Instruction" ;
    skos:definition "A process that is used to engender knowledge, attitudes, and skills." ;
    skos:inScheme okns:dc ;
    skos:mappingRelation dcterms:MethodOfInstruction ;
    linkml:class_uri dcterms:MethodOfInstruction ;
    linkml:definition_uri okns:DctMethodOfInstruction ;
    linkml:slot_usage [ ] .

okns:DctPeriodOfTime a linkml:ClassDefinition ;
    dcterms:source dcterms: ;
    dcterms:title "Period of Time" ;
    skos:definition "An interval of time that is named or defined by its start and end dates." ;
    skos:inScheme okns:dc ;
    skos:mappingRelation dcterms:PeriodOfTime ;
    linkml:class_uri dcterms:PeriodOfTime ;
    linkml:definition_uri okns:DctPeriodOfTime ;
    linkml:is_a okns:DctLocationPeriodOrJurisdiction ;
    linkml:slot_usage [ ] .

okns:DctPhysicalMedium a linkml:ClassDefinition ;
    dcterms:source dcterms: ;
    dcterms:title "Physical Medium" ;
    skos:definition "Examples include paper, canvas, or DVD." ;
    skos:inScheme okns:dc ;
    skos:mappingRelation dcterms:PhysicalMedium ;
    skos:note "description: A physical material or carrier." ;
    linkml:class_uri dcterms:PhysicalMedium ;
    linkml:definition_uri okns:DctPhysicalMedium ;
    linkml:is_a okns:DctMediaType ;
    linkml:slot_usage [ ] .

okns:DctPhysicalResource a linkml:ClassDefinition ;
    dcterms:source dcterms: ;
    dcterms:title "Physical Resource" ;
    skos:definition "A material thing." ;
    skos:inScheme okns:dc ;
    skos:mappingRelation dcterms:PhysicalResource ;
    linkml:class_uri dcterms:PhysicalResource ;
    linkml:definition_uri okns:DctPhysicalResource ;
    linkml:slot_usage [ ] .

okns:DctPolicy a linkml:ClassDefinition ;
    dcterms:source dcterms: ;
    dcterms:title "Policy" ;
    skos:definition "A plan or course of action by an authority, intended to influence and determine decisions, actions, and other matters." ;
    skos:inScheme okns:dc ;
    skos:mappingRelation dcterms:Policy ;
    linkml:class_uri dcterms:Policy ;
    linkml:definition_uri okns:DctPolicy ;
    linkml:slot_usage [ ] .

okns:DctProvenanceStatement a linkml:ClassDefinition ;
    dcterms:source dcterms: ;
    dcterms:title "Provenance Statement" ;
    skos:definition "Any changes in ownership and custody of a resource since its creation that are significant for its authenticity, integrity, and interpretation." ;
    skos:inScheme okns:dc ;
    skos:mappingRelation dcterms:ProvenanceStatement ;
    linkml:class_uri dcterms:ProvenanceStatement ;
    linkml:definition_uri okns:DctProvenanceStatement ;
    linkml:slot_usage [ ] .

okns:DctSizeOrDuration a linkml:ClassDefinition ;
    dcterms:source dcterms: ;
    dcterms:title "Size or Duration" ;
    skos:definition "Examples include a number of pages, a specification of length, width, and breadth, or a period in hours, minutes, and seconds." ;
    skos:inScheme okns:dc ;
    skos:mappingRelation dcterms:SizeOrDuration ;
    skos:note "description: A dimension or extent, or a time taken to play or execute." ;
    linkml:class_uri dcterms:SizeOrDuration ;
    linkml:definition_uri okns:DctSizeOrDuration ;
    linkml:is_a okns:DctMediaTypeOrExtent ;
    linkml:slot_usage [ ] .

okns:DctStandard a linkml:ClassDefinition ;
    dcterms:source dcterms: ;
    dcterms:title "Standard" ;
    skos:definition "A reference point against which other things can be evaluated or compared." ;
    skos:inScheme okns:dc ;
    skos:mappingRelation dcterms:Standard ;
    linkml:class_uri dcterms:Standard ;
    linkml:definition_uri okns:DctStandard ;
    linkml:slot_usage [ ] .

okns:EventFactor a linkml:ClassDefinition ;
    dcterms:title "Factor" ;
    skos:definition "Everything used as a factor in an event" ;
    skos:inScheme okns:event ;
    skos:mappingRelation event:Factor ;
    linkml:class_uri event:Factor ;
    linkml:definition_uri okns:EventFactor ;
    linkml:slot_usage [ ] .

okns:EventProduct a linkml:ClassDefinition ;
    dcterms:title "Product" ;
    skos:definition "Everything produced by an event" ;
    skos:inScheme okns:event ;
    skos:mappingRelation event:Product ;
    linkml:class_uri event:Product ;
    linkml:definition_uri okns:EventProduct ;
    linkml:slot_usage [ ] .

okns:FoafLabelProperty a linkml:ClassDefinition ;
    dcterms:source foaf: ;
    dcterms:title "Label Property" ;
    skos:definition "A foaf:LabelProperty is any RDF property with texual values that serve as labels." ;
    skos:inScheme okns:foaf ;
    skos:mappingRelation foaf:LabelProperty ;
    linkml:class_uri foaf:LabelProperty ;
    linkml:definition_uri okns:FoafLabelProperty ;
    linkml:slot_usage [ ] .

okns:FoafOnlineChatAccount a linkml:ClassDefinition ;
    dcterms:source foaf: ;
    dcterms:title "Online Chat Account" ;
    skos:definition "An online chat account." ;
    skos:inScheme okns:foaf ;
    skos:mappingRelation foaf:OnlineChatAccount ;
    linkml:class_uri foaf:OnlineChatAccount ;
    linkml:definition_uri okns:FoafOnlineChatAccount ;
    linkml:is_a okns:FoafOnlineAccount ;
    linkml:slot_usage [ ] .

okns:FoafOnlineEcommerceAccount a linkml:ClassDefinition ;
    dcterms:source foaf: ;
    dcterms:title "Online E-commerce Account" ;
    skos:definition "An online e-commerce account." ;
    skos:inScheme okns:foaf ;
    skos:mappingRelation foaf:OnlineEcommerceAccount ;
    linkml:class_uri foaf:OnlineEcommerceAccount ;
    linkml:definition_uri okns:FoafOnlineEcommerceAccount ;
    linkml:is_a okns:FoafOnlineAccount ;
    linkml:slot_usage [ ] .

okns:FoafOnlineGamingAccount a linkml:ClassDefinition ;
    dcterms:source foaf: ;
    dcterms:title "Online Gaming Account" ;
    skos:definition "An online gaming account." ;
    skos:inScheme okns:foaf ;
    skos:mappingRelation foaf:OnlineGamingAccount ;
    linkml:class_uri foaf:OnlineGamingAccount ;
    linkml:definition_uri okns:FoafOnlineGamingAccount ;
    linkml:is_a okns:FoafOnlineAccount ;
    linkml:slot_usage [ ] .

okns:FoafPersonalProfileDocument a linkml:ClassDefinition ;
    dcterms:title "PersonalProfileDocument" ;
    skos:definition "A personal profile RDF document." ;
    skos:inScheme okns:foaf ;
    skos:mappingRelation foaf:PersonalProfileDocument ;
    linkml:class_uri foaf:PersonalProfileDocument ;
    linkml:definition_uri okns:FoafPersonalProfileDocument ;
    linkml:is_a okns:FoafDocument ;
    linkml:slot_usage [ ] .

okns:FoafProject a linkml:ClassDefinition ;
    dcterms:source foaf: ;
    dcterms:title "Project" ;
    skos:definition "A project (a collective endeavour of some kind)." ;
    skos:inScheme okns:foaf ;
    skos:mappingRelation foaf:Project ;
    linkml:class_uri foaf:Project ;
    linkml:definition_uri okns:FoafProject ;
    linkml:slot_usage [ ] .

okns:FrbrConcept a linkml:ClassDefinition ;
    dcterms:source frbr: ;
    dcterms:title "concept" ;
    skos:definition "An abstract idea or notion." ;
    skos:editorialNote "N0700dd006c204902af73cf16bc783f0e",
        "N6a66620bbb5b4f14bdd478d690ccb827",
        "Neb3e310a3aca4c30b4ab0dd6e27b06ed",
        "Nefc66e4078bd4e058f1410d55d0d814d" ;
    skos:inScheme okns:frbr ;
    skos:mappingRelation frbr:Concept ;
    skos:note "description: This class corresponds to the FRBR group three entity 'Concept'." ;
    linkml:class_uri frbr:Concept ;
    linkml:definition_uri okns:FrbrConcept ;
    linkml:is_a okns:SkosConcept ;
    linkml:slot_usage [ ] .

okns:FrbrCorporateBody a linkml:ClassDefinition ;
    dcterms:source frbr: ;
    dcterms:title "corporate body" ;
    skos:definition "An organization or group of individuals and/or other organizations." ;
    skos:editorialNote "N7844fc43281c4c0b94fb3de4092b55bd",
        "Nd637f86269e44eda9faa4e535b3e2dd7",
        "Nef1629fb0380414b9b619c305e9b54f2" ;
    skos:inScheme okns:frbr ;
    skos:mappingRelation frbr:CorporateBody ;
    skos:note "description: This class corresponds to the FRBR group two entity 'Corporate Body'." ;
    linkml:class_uri frbr:CorporateBody ;
    linkml:definition_uri okns:FrbrCorporateBody ;
    linkml:is_a okns:FrbrResponsibleEntity ;
    linkml:slot_usage [ ] .

okns:FrbrEvent a linkml:ClassDefinition ;
    dcterms:source frbr: ;
    dcterms:title "event" ;
    skos:definition "An action or occurrence." ;
    skos:editorialNote "N7ae9bcee39154d4c8edb1c71231aa4bb",
        "Nae890efc55e94163b9dd6f42be868904",
        "Nf192cef2e52c43ea985654628f2df832" ;
    skos:inScheme okns:frbr ;
    skos:mappingRelation frbr:Event ;
    skos:note "description: This class corresponds to the FRBR group three entity 'Event'." ;
    linkml:class_uri frbr:Event ;
    linkml:definition_uri okns:FrbrEvent ;
    linkml:is_a okns:Time-entryEvent ;
    linkml:slot_usage [ ] .

okns:FrbrObject a linkml:ClassDefinition ;
    dcterms:source frbr: ;
    dcterms:title "object" ;
    skos:definition "A tangible or material thing." ;
    skos:editorialNote "N12a9782a0bea4e15981509b9e1994fc4",
        "N79db2676181e4c54946ff0aeb4db7eae",
        "N91d2223903464c18bab8f5512ec69cc4",
        "Nc5a35175cb5e4d6796bd865ce3616634" ;
    skos:inScheme okns:frbr ;
    skos:mappingRelation frbr:Object ;
    skos:note "description: This class corresponds to the FRBR group three entity 'Object'." ;
    linkml:class_uri frbr:Object ;
    linkml:definition_uri okns:FrbrObject ;
    linkml:is_a okns:WgsSpatialThing ;
    linkml:slot_usage [ ] .

okns:FrbrPerson a linkml:ClassDefinition ;
    dcterms:source frbr: ;
    dcterms:title "person" ;
    skos:definition "A living or dead individual." ;
    skos:editorialNote "N2a2cf99698ba4492a74e6828348b9ec5",
        "N6a8e567782d7409ea059943d2c8f7c0c",
        "N7d4a4e9ac98c4c1b98adf5f82190733c" ;
    skos:inScheme okns:frbr ;
    skos:mappingRelation frbr:Person ;
    skos:note "description: This class corresponds to the FRBR group two entity 'Person'." ;
    linkml:class_uri frbr:Person ;
    linkml:definition_uri okns:FrbrPerson ;
    linkml:slot_usage [ ] .

okns:FrbrPlace a linkml:ClassDefinition ;
    dcterms:source frbr: ;
    dcterms:title "place" ;
    skos:definition "A location." ;
    skos:editorialNote "N12e2c56320dc4fe893a172c83ae9e740",
        "N3b417383d3c3435fb4f1f7dd74e24080",
        "Nc12693d9241744efa3bf3a4069e56306",
        "Nee958ddd3d9840799b14b1e985c478e7" ;
    skos:inScheme okns:frbr ;
    skos:mappingRelation frbr:Place ;
    skos:note "description: This class corresponds to the FRBR group three entity 'Place'." ;
    linkml:class_uri frbr:Place ;
    linkml:definition_uri okns:FrbrPlace ;
    linkml:is_a okns:WgsSpatialThing ;
    linkml:slot_usage [ ] .

okns:FrbrSubject a linkml:ClassDefinition ;
    dcterms:source frbr: ;
    dcterms:title "subject" ;
    skos:definition "Something that may serve as the subject of a work." ;
    skos:editorialNote "N2ee373921f494d389d178bfc65afb1a8",
        "N3d89dfcc4b8444e2a90d4927e75cd031",
        "N8e57c30ecf7b42669a8fb31d7eded226" ;
    skos:inScheme okns:frbr ;
    skos:mappingRelation frbr:Subject ;
    skos:note "description: This class represents any of the FRBR group three entities." ;
    linkml:class_uri frbr:Subject ;
    linkml:definition_uri okns:FrbrSubject ;
    linkml:slot_usage [ ] .

okns:IcalValueDATE a linkml:ClassDefinition ;
    skos:inScheme okns:ical ;
    skos:mappingRelation ical:Value_DATE ;
    linkml:class_uri ical:Value_DATE ;
    linkml:definition_uri okns:IcalValueDATE ;
    linkml:slot_usage [ ] .

okns:IcalVfreebusy a linkml:ClassDefinition ;
    dcterms:title "VFREEBUSY" ;
    skos:definition "Provide a grouping of component properties that describe either a request for free/busy time, describe a response to a request for free/busy time or describe a published set of busy time." ;
    skos:inScheme okns:ical ;
    skos:mappingRelation ical:Vfreebusy ;
    linkml:class_uri ical:Vfreebusy ;
    linkml:definition_uri okns:IcalVfreebusy ;
    linkml:slot_usage [ ] .

okns:IcalVjournal a linkml:ClassDefinition ;
    dcterms:title "VJOURNAL" ;
    skos:definition "Provide a grouping of component properties that describe a journal entry." ;
    skos:inScheme okns:ical ;
    skos:mappingRelation ical:Vjournal ;
    linkml:class_uri ical:Vjournal ;
    linkml:definition_uri okns:IcalVjournal ;
    linkml:slot_usage [ ] .

okns:MoArranger a linkml:ClassDefinition ;
    dcterms:title "arranger" ;
    skos:inScheme okns:mo ;
    skos:mappingRelation ns1:Arranger ;
    linkml:class_uri <http://purl.org/ontology/mo/Arranger> ;
    linkml:definition_uri okns:MoArranger ;
    linkml:is_a okns:FoafAgent ;
    linkml:slot_usage [ ] .

okns:MoCD a linkml:ClassDefinition ;
    dcterms:source <http://purl.org/ontology/mo/> ;
    dcterms:title "CD" ;
    skos:definition "Compact Disc used as medium to record a musical manifestation." ;
    skos:inScheme okns:mo ;
    skos:mappingRelation ns1:CD ;
    linkml:class_uri <http://purl.org/ontology/mo/CD> ;
    linkml:definition_uri okns:MoCD ;
    linkml:is_a okns:MoMedium ;
    linkml:slot_usage [ ] .

okns:MoComposer a linkml:ClassDefinition ;
    dcterms:title "composer" ;
    skos:inScheme okns:mo ;
    skos:mappingRelation ns1:Composer ;
    linkml:class_uri <http://purl.org/ontology/mo/Composer> ;
    linkml:definition_uri okns:MoComposer ;
    linkml:is_a okns:FoafAgent ;
    linkml:slot_usage [ ] .

okns:MoConductor a linkml:ClassDefinition ;
    dcterms:title "conductor" ;
    skos:inScheme okns:mo ;
    skos:mappingRelation ns1:Conductor ;
    linkml:class_uri <http://purl.org/ontology/mo/Conductor> ;
    linkml:definition_uri okns:MoConductor ;
    linkml:is_a okns:FoafAgent ;
    linkml:slot_usage [ ] .

okns:MoDAT a linkml:ClassDefinition ;
    dcterms:source <http://purl.org/ontology/mo/> ;
    dcterms:title "DAT" ;
    skos:definition "Digital Audio Tape used as medium to record a musical manifestation." ;
    skos:inScheme okns:mo ;
    skos:mappingRelation ns1:DAT ;
    linkml:class_uri <http://purl.org/ontology/mo/DAT> ;
    linkml:definition_uri okns:MoDAT ;
    linkml:is_a okns:MoMedium ;
    linkml:slot_usage [ ] .

okns:MoDCC a linkml:ClassDefinition ;
    dcterms:source <http://purl.org/ontology/mo/> ;
    dcterms:title "DCC" ;
    skos:definition "Digital Compact Cassette used as medium to record a musical manifestation." ;
    skos:inScheme okns:mo ;
    skos:mappingRelation ns1:DCC ;
    linkml:class_uri <http://purl.org/ontology/mo/DCC> ;
    linkml:definition_uri okns:MoDCC ;
    linkml:is_a okns:MoMedium ;
    linkml:slot_usage [ ] .

okns:MoDVDA a linkml:ClassDefinition ;
    dcterms:source <http://purl.org/ontology/mo/> ;
    dcterms:title "DVDA" ;
    skos:definition "DVD-Audio used as medium to record a musical manifestation." ;
    skos:inScheme okns:mo ;
    skos:mappingRelation ns1:DVDA ;
    linkml:class_uri <http://purl.org/ontology/mo/DVDA> ;
    linkml:definition_uri okns:MoDVDA ;
    linkml:is_a okns:MoMedium ;
    linkml:slot_usage [ ] .

okns:MoED2K a linkml:ClassDefinition ;
    dcterms:source <http://purl.org/ontology/mo/> ;
    dcterms:title "ED2K" ;
    skos:definition "Something available on the E-Donkey peer-2-peer filesharing network" ;
    skos:inScheme okns:mo ;
    skos:mappingRelation ns1:ED2K ;
    linkml:class_uri <http://purl.org/ontology/mo/ED2K> ;
    linkml:definition_uri okns:MoED2K ;
    linkml:is_a okns:MoMedium ;
    linkml:slot_usage [ ] .

okns:MoFestival a linkml:ClassDefinition ;
    dcterms:source <http://purl.org/ontology/mo/> ;
    dcterms:title "Festival" ;
    skos:definition "A festival - musical/artistic event lasting several days, like Glastonbury, Rock Am Ring...␊        We migth decompose this event (which is in fact just a classification of the space/time region related to ␊        a particular festival) using hasSubEvent in several performances at different space/time." ;
    skos:inScheme okns:mo ;
    skos:mappingRelation ns1:Festival ;
    linkml:class_uri <http://purl.org/ontology/mo/Festival> ;
    linkml:definition_uri okns:MoFestival ;
    linkml:is_a okns:EventEvent ;
    linkml:slot_usage [ ] .

okns:MoInstrumentation a linkml:ClassDefinition ;
    dcterms:source <http://purl.org/ontology/mo/> ;
    dcterms:title "instrumentation" ;
    skos:definition "Instrumentation deals with the techniques of writing music for a specific instrument, ␊        including the limitations of the instrument, playing techniques and idiomatic handling of the instrument." ;
    skos:inScheme okns:mo ;
    skos:mappingRelation ns1:Instrumentation ;
    linkml:class_uri <http://purl.org/ontology/mo/Instrumentation> ;
    linkml:definition_uri okns:MoInstrumentation ;
    linkml:is_a okns:MoArrangement ;
    linkml:slot_usage [ ] .

okns:MoLibretto a linkml:ClassDefinition ;
    dcterms:source <http://purl.org/ontology/mo/> ;
    dcterms:title "libretto" ;
    skos:definition "Libretto" ;
    skos:inScheme okns:mo ;
    skos:mappingRelation ns1:Libretto ;
    linkml:class_uri <http://purl.org/ontology/mo/Libretto> ;
    linkml:definition_uri okns:MoLibretto ;
    linkml:is_a okns:MoMusicalExpression ;
    linkml:slot_usage [ ] .

okns:MoListener a linkml:ClassDefinition ;
    dcterms:title "listened" ;
    skos:inScheme okns:mo ;
    skos:mappingRelation ns1:Listener ;
    linkml:class_uri <http://purl.org/ontology/mo/Listener> ;
    linkml:definition_uri okns:MoListener ;
    linkml:is_a okns:FoafAgent ;
    linkml:slot_usage [ ] .

okns:MoMD a linkml:ClassDefinition ;
    dcterms:source <http://purl.org/ontology/mo/> ;
    dcterms:title "MD" ;
    skos:definition "Mini Disc used as medium to record a musical manifestation." ;
    skos:inScheme okns:mo ;
    skos:mappingRelation ns1:MD ;
    linkml:class_uri <http://purl.org/ontology/mo/MD> ;
    linkml:definition_uri okns:MoMD ;
    linkml:is_a okns:MoMedium ;
    linkml:slot_usage [ ] .

okns:MoMagneticTape a linkml:ClassDefinition ;
    dcterms:source <http://purl.org/ontology/mo/> ;
    dcterms:title "MagneticTape" ;
    skos:definition "Magnetic analogue tape used as medium to record a musical manifestation." ;
    skos:inScheme okns:mo ;
    skos:mappingRelation ns1:MagneticTape ;
    linkml:class_uri <http://purl.org/ontology/mo/MagneticTape> ;
    linkml:definition_uri okns:MoMagneticTape ;
    linkml:is_a okns:MoMedium ;
    linkml:slot_usage [ ] .

okns:MoOrchestration a linkml:ClassDefinition ;
    dcterms:source <http://purl.org/ontology/mo/> ;
    dcterms:title "orchestration" ;
    skos:definition "Orchestration includes, in addition to instrumentation, the handling of groups of instruments and their balance and interaction." ;
    skos:inScheme okns:mo ;
    skos:mappingRelation ns1:Orchestration ;
    linkml:class_uri <http://purl.org/ontology/mo/Orchestration> ;
    linkml:definition_uri okns:MoOrchestration ;
    linkml:is_a okns:MoArrangement ;
    linkml:slot_usage [ ] .

okns:MoPerformer a linkml:ClassDefinition ;
    dcterms:title "performer" ;
    skos:inScheme okns:mo ;
    skos:mappingRelation ns1:Performer ;
    linkml:class_uri <http://purl.org/ontology/mo/Performer> ;
    linkml:definition_uri okns:MoPerformer ;
    linkml:is_a okns:FoafAgent ;
    linkml:slot_usage [ ] .

okns:MoPublishedLibretto a linkml:ClassDefinition ;
    dcterms:source <http://purl.org/ontology/mo/> ;
    dcterms:title "published libretto" ;
    skos:definition "A published libretto" ;
    skos:inScheme okns:mo ;
    skos:mappingRelation ns1:PublishedLibretto ;
    linkml:class_uri <http://purl.org/ontology/mo/PublishedLibretto> ;
    linkml:definition_uri okns:MoPublishedLibretto ;
    linkml:is_a okns:MoMusicalManifestation ;
    linkml:slot_usage [ ] .

okns:MoPublishedLyrics a linkml:ClassDefinition ;
    dcterms:source <http://purl.org/ontology/mo/> ;
    dcterms:title "published lyrics" ;
    skos:definition "Published lyrics, as a book or as a text file, for example" ;
    skos:inScheme okns:mo ;
    skos:mappingRelation ns1:PublishedLyrics ;
    linkml:class_uri <http://purl.org/ontology/mo/PublishedLyrics> ;
    linkml:definition_uri okns:MoPublishedLyrics ;
    linkml:is_a okns:MoMusicalManifestation ;
    linkml:slot_usage [ ] .

okns:MoPublishedScore a linkml:ClassDefinition ;
    dcterms:source <http://purl.org/ontology/mo/> ;
    dcterms:title "published score" ;
    skos:definition "A published score (subclass of MusicalManifestation)" ;
    skos:inScheme okns:mo ;
    skos:mappingRelation ns1:PublishedScore ;
    linkml:class_uri <http://purl.org/ontology/mo/PublishedScore> ;
    linkml:definition_uri okns:MoPublishedScore ;
    linkml:is_a okns:MoMusicalManifestation ;
    linkml:slot_usage [ ] .

okns:MoSACD a linkml:ClassDefinition ;
    dcterms:source <http://purl.org/ontology/mo/> ;
    dcterms:title "SACD" ;
    skos:definition "Super Audio Compact Disc used as medium to record a musical manifestation." ;
    skos:inScheme okns:mo ;
    skos:mappingRelation ns1:SACD ;
    linkml:class_uri <http://purl.org/ontology/mo/SACD> ;
    linkml:definition_uri okns:MoSACD ;
    linkml:is_a okns:MoMedium ;
    linkml:slot_usage [ ] .

okns:MoShow a linkml:ClassDefinition ;
    dcterms:source <http://purl.org/ontology/mo/> ;
    dcterms:title "Show" ;
    skos:definition "A show - a musical event lasting several days, in a particular venue. Examples can be␊        \"The Magic Flute\" at the Opera Bastille, August 2005, or a musical in the west end..." ;
    skos:inScheme okns:mo ;
    skos:mappingRelation ns1:Show ;
    linkml:class_uri <http://purl.org/ontology/mo/Show> ;
    linkml:definition_uri okns:MoShow ;
    linkml:is_a okns:EventEvent ;
    linkml:slot_usage [ ] .

okns:MoSoloMusicArtist a linkml:ClassDefinition ;
    dcterms:source <http://purl.org/ontology/mo/> ;
    dcterms:title "solo music artist" ;
    skos:definition "Single person whose musical creative work shows sensitivity and imagination." ;
    skos:inScheme okns:mo ;
    skos:mappingRelation ns1:SoloMusicArtist ;
    linkml:class_uri <http://purl.org/ontology/mo/SoloMusicArtist> ;
    linkml:definition_uri okns:MoSoloMusicArtist ;
    linkml:is_a okns:MoMusicArtist ;
    linkml:slot_usage [ ] .

okns:MoSoundEngineer a linkml:ClassDefinition ;
    dcterms:title "sound engineer" ;
    skos:inScheme okns:mo ;
    skos:mappingRelation ns1:SoundEngineer ;
    linkml:class_uri <http://purl.org/ontology/mo/SoundEngineer> ;
    linkml:definition_uri okns:MoSoundEngineer ;
    linkml:is_a okns:FoafAgent ;
    linkml:slot_usage [ ] .

okns:MoStream a linkml:ClassDefinition ;
    dcterms:source <http://purl.org/ontology/mo/> ;
    dcterms:title "Stream" ;
    skos:definition "Transmission over a network  used as medium to broadcast a musical manifestation" ;
    skos:inScheme okns:mo ;
    skos:mappingRelation ns1:Stream ;
    linkml:class_uri <http://purl.org/ontology/mo/Stream> ;
    linkml:definition_uri okns:MoStream ;
    linkml:is_a okns:MoMedium ;
    linkml:slot_usage [ ] .

okns:MoTorrent a linkml:ClassDefinition ;
    dcterms:source <http://purl.org/ontology/mo/> ;
    dcterms:title "Torrent" ;
    skos:definition "Something available on the Bittorrent peer-2-peer filesharing network" ;
    skos:inScheme okns:mo ;
    skos:mappingRelation ns1:Torrent ;
    linkml:class_uri <http://purl.org/ontology/mo/Torrent> ;
    linkml:definition_uri okns:MoTorrent ;
    linkml:is_a okns:MoMedium ;
    linkml:slot_usage [ ] .

okns:MoTranscription a linkml:ClassDefinition ;
    dcterms:source <http://purl.org/ontology/mo/> ;
    dcterms:title "transcription" ;
    skos:definition "Transcription event" ;
    skos:inScheme okns:mo ;
    skos:mappingRelation ns1:Transcription ;
    linkml:class_uri <http://purl.org/ontology/mo/Transcription> ;
    linkml:definition_uri okns:MoTranscription ;
    linkml:is_a okns:EventEvent ;
    linkml:slot_usage [ ] .

okns:MoVinyl a linkml:ClassDefinition ;
    dcterms:source <http://purl.org/ontology/mo/> ;
    dcterms:title "Vinyl" ;
    skos:definition "Vinyl used as medium to record a musical manifestation" ;
    skos:inScheme okns:mo ;
    skos:mappingRelation ns1:Vinyl ;
    linkml:class_uri <http://purl.org/ontology/mo/Vinyl> ;
    linkml:definition_uri okns:MoVinyl ;
    linkml:is_a okns:MoMedium ;
    linkml:slot_usage [ ] .

okns:OwlAllDisjointClasses a linkml:ClassDefinition ;
    dcterms:source owl: ;
    dcterms:title "AllDisjointClasses" ;
    skos:definition "The class of collections of pairwise disjoint classes." ;
    skos:inScheme okns:owl-rdf-rdfs ;
    skos:mappingRelation owl:AllDisjointClasses ;
    linkml:class_uri owl:AllDisjointClasses ;
    linkml:definition_uri okns:OwlAllDisjointClasses ;
    linkml:is_a okns:RdfsResource ;
    linkml:slot_usage [ ] .

okns:OwlAllDisjointProperties a linkml:ClassDefinition ;
    dcterms:source owl: ;
    dcterms:title "AllDisjointProperties" ;
    skos:definition "The class of collections of pairwise disjoint properties." ;
    skos:inScheme okns:owl-rdf-rdfs ;
    skos:mappingRelation owl:AllDisjointProperties ;
    linkml:class_uri owl:AllDisjointProperties ;
    linkml:definition_uri okns:OwlAllDisjointProperties ;
    linkml:is_a okns:RdfsResource ;
    linkml:slot_usage [ ] .

okns:OwlAnnotation a linkml:ClassDefinition ;
    dcterms:source owl: ;
    dcterms:title "Annotation" ;
    skos:definition "The class of annotated annotations for which the RDF serialization consists of an annotated subject, predicate and object." ;
    skos:inScheme okns:owl-rdf-rdfs ;
    skos:mappingRelation owl:Annotation ;
    linkml:class_uri owl:Annotation ;
    linkml:definition_uri okns:OwlAnnotation ;
    linkml:is_a okns:RdfsResource ;
    linkml:slot_usage [ ] .

okns:OwlAnnotationProperty a linkml:ClassDefinition ;
    dcterms:source owl: ;
    dcterms:title "AnnotationProperty" ;
    skos:definition "The class of annotation properties." ;
    skos:inScheme okns:owl-rdf-rdfs ;
    skos:mappingRelation owl:AnnotationProperty ;
    linkml:class_uri owl:AnnotationProperty ;
    linkml:definition_uri okns:OwlAnnotationProperty ;
    linkml:is_a okns:RdfProperty ;
    linkml:slot_usage [ ] .

okns:OwlAsymmetricProperty a linkml:ClassDefinition ;
    dcterms:source owl: ;
    dcterms:title "AsymmetricProperty" ;
    skos:definition "The class of asymmetric properties." ;
    skos:inScheme okns:owl-rdf-rdfs ;
    skos:mappingRelation owl:AsymmetricProperty ;
    linkml:class_uri owl:AsymmetricProperty ;
    linkml:definition_uri okns:OwlAsymmetricProperty ;
    linkml:is_a okns:OwlObjectProperty ;
    linkml:slot_usage [ ] .

okns:OwlAxiom a linkml:ClassDefinition ;
    dcterms:source owl: ;
    dcterms:title "Axiom" ;
    skos:definition "The class of annotated axioms for which the RDF serialization consists of an annotated subject, predicate and object." ;
    skos:inScheme okns:owl-rdf-rdfs ;
    skos:mappingRelation owl:Axiom ;
    linkml:class_uri owl:Axiom ;
    linkml:definition_uri okns:OwlAxiom ;
    linkml:is_a okns:RdfsResource ;
    linkml:slot_usage [ ] .

okns:OwlDataRange a linkml:ClassDefinition ;
    dcterms:source owl: ;
    dcterms:title "DataRange" ;
    skos:definition "The class of OWL data ranges, which are special kinds of datatypes. Note: The use of the IRI owl:DataRange has been deprecated as of OWL 2. The IRI rdfs:Datatype SHOULD be used instead." ;
    skos:inScheme okns:owl-rdf-rdfs ;
    skos:mappingRelation owl:DataRange ;
    linkml:class_uri owl:DataRange ;
    linkml:definition_uri okns:OwlDataRange ;
    linkml:is_a okns:RdfsDatatype ;
    linkml:slot_usage [ ] ;
    linkml:slots okns:rdfs_comment,
        okns:rdfs_isDefinedBy,
        okns:rdfs_label,
        okns:rdfs_seeAlso,
        okns:rdfs_subClassOf .

okns:OwlDatatypeProperty a linkml:ClassDefinition ;
    dcterms:source owl: ;
    dcterms:title "DatatypeProperty" ;
    skos:definition "The class of data properties." ;
    skos:inScheme okns:owl-rdf-rdfs ;
    skos:mappingRelation owl:DatatypeProperty ;
    linkml:class_uri owl:DatatypeProperty ;
    linkml:definition_uri okns:OwlDatatypeProperty ;
    linkml:is_a okns:RdfProperty ;
    linkml:slot_usage [ ] .

okns:OwlDeprecatedClass a linkml:ClassDefinition ;
    dcterms:source owl: ;
    dcterms:title "DeprecatedClass" ;
    skos:definition "The class of deprecated classes." ;
    skos:inScheme okns:owl-rdf-rdfs ;
    skos:mappingRelation owl:DeprecatedClass ;
    linkml:class_uri owl:DeprecatedClass ;
    linkml:definition_uri okns:OwlDeprecatedClass ;
    linkml:is_a okns:RdfsClass ;
    linkml:slot_usage [ ] .

okns:OwlDeprecatedProperty a linkml:ClassDefinition ;
    dcterms:source owl: ;
    dcterms:title "DeprecatedProperty" ;
    skos:definition "The class of deprecated properties." ;
    skos:inScheme okns:owl-rdf-rdfs ;
    skos:mappingRelation owl:DeprecatedProperty ;
    linkml:class_uri owl:DeprecatedProperty ;
    linkml:definition_uri okns:OwlDeprecatedProperty ;
    linkml:is_a okns:RdfProperty ;
    linkml:slot_usage [ ] .

okns:OwlFunctionalProperty a linkml:ClassDefinition ;
    dcterms:source owl: ;
    dcterms:title "FunctionalProperty" ;
    skos:definition "The class of functional properties." ;
    skos:inScheme okns:owl-rdf-rdfs ;
    skos:mappingRelation owl:FunctionalProperty ;
    linkml:class_uri owl:FunctionalProperty ;
    linkml:definition_uri okns:OwlFunctionalProperty ;
    linkml:is_a okns:RdfProperty ;
    linkml:slot_usage [ ] .

okns:OwlInverseFunctionalProperty a linkml:ClassDefinition ;
    dcterms:source owl: ;
    dcterms:title "InverseFunctionalProperty" ;
    skos:definition "The class of inverse-functional properties." ;
    skos:inScheme okns:owl-rdf-rdfs ;
    skos:mappingRelation owl:InverseFunctionalProperty ;
    linkml:class_uri owl:InverseFunctionalProperty ;
    linkml:definition_uri okns:OwlInverseFunctionalProperty ;
    linkml:is_a okns:OwlObjectProperty ;
    linkml:slot_usage [ ] .

okns:OwlIrreflexiveProperty a linkml:ClassDefinition ;
    dcterms:source owl: ;
    dcterms:title "IrreflexiveProperty" ;
    skos:definition "The class of irreflexive properties." ;
    skos:inScheme okns:owl-rdf-rdfs ;
    skos:mappingRelation owl:IrreflexiveProperty ;
    linkml:class_uri owl:IrreflexiveProperty ;
    linkml:definition_uri okns:OwlIrreflexiveProperty ;
    linkml:is_a okns:OwlObjectProperty ;
    linkml:slot_usage [ ] .

okns:OwlNamedIndividual a linkml:ClassDefinition ;
    dcterms:source owl: ;
    dcterms:title "NamedIndividual" ;
    skos:definition "The class of named individuals." ;
    skos:inScheme okns:owl-rdf-rdfs ;
    skos:mappingRelation owl:NamedIndividual ;
    linkml:class_uri owl:NamedIndividual ;
    linkml:definition_uri okns:OwlNamedIndividual ;
    linkml:is_a okns:OwlThing ;
    linkml:slot_usage [ ] .

okns:OwlNothing a linkml:ClassDefinition ;
    dcterms:source owl: ;
    dcterms:title "Nothing" ;
    skos:definition "This is the empty class." ;
    skos:inScheme okns:owl-rdf-rdfs ;
    skos:mappingRelation owl:Nothing ;
    linkml:class_uri owl:Nothing ;
    linkml:definition_uri okns:OwlNothing ;
    linkml:is_a okns:OwlThing ;
    linkml:slot_usage [ ] .

okns:OwlOntologyProperty a linkml:ClassDefinition ;
    dcterms:source owl: ;
    dcterms:title "OntologyProperty" ;
    skos:definition "The class of ontology properties." ;
    skos:inScheme okns:owl-rdf-rdfs ;
    skos:mappingRelation owl:OntologyProperty ;
    linkml:class_uri owl:OntologyProperty ;
    linkml:definition_uri okns:OwlOntologyProperty ;
    linkml:is_a okns:RdfProperty ;
    linkml:slot_usage [ ] .

okns:OwlReflexiveProperty a linkml:ClassDefinition ;
    dcterms:source owl: ;
    dcterms:title "ReflexiveProperty" ;
    skos:definition "The class of reflexive properties." ;
    skos:inScheme okns:owl-rdf-rdfs ;
    skos:mappingRelation owl:ReflexiveProperty ;
    linkml:class_uri owl:ReflexiveProperty ;
    linkml:definition_uri okns:OwlReflexiveProperty ;
    linkml:is_a okns:OwlObjectProperty ;
    linkml:slot_usage [ ] .

okns:OwlSymmetricProperty a linkml:ClassDefinition ;
    dcterms:source owl: ;
    dcterms:title "SymmetricProperty" ;
    skos:definition "The class of symmetric properties." ;
    skos:inScheme okns:owl-rdf-rdfs ;
    skos:mappingRelation owl:SymmetricProperty ;
    linkml:class_uri owl:SymmetricProperty ;
    linkml:definition_uri okns:OwlSymmetricProperty ;
    linkml:is_a okns:OwlObjectProperty ;
    linkml:slot_usage [ ] .

okns:OwlTransitiveProperty a linkml:ClassDefinition ;
    dcterms:source owl: ;
    dcterms:title "TransitiveProperty" ;
    skos:definition "The class of transitive properties." ;
    skos:inScheme okns:owl-rdf-rdfs ;
    skos:mappingRelation owl:TransitiveProperty ;
    linkml:class_uri owl:TransitiveProperty ;
    linkml:definition_uri okns:OwlTransitiveProperty ;
    linkml:is_a okns:OwlObjectProperty ;
    linkml:slot_usage [ ] .

okns:RdfAlt a linkml:ClassDefinition ;
    dcterms:source rdf: ;
    dcterms:title "Alt" ;
    skos:definition "The class of containers of alternatives." ;
    skos:inScheme okns:owl-rdf-rdfs ;
    skos:mappingRelation rdf:Alt ;
    linkml:class_uri rdf:Alt ;
    linkml:definition_uri okns:RdfAlt ;
    linkml:is_a okns:RdfsContainer ;
    linkml:slot_usage [ ] .

okns:RdfBag a linkml:ClassDefinition ;
    dcterms:source rdf: ;
    dcterms:title "Bag" ;
    skos:definition "The class of unordered containers." ;
    skos:inScheme okns:owl-rdf-rdfs ;
    skos:mappingRelation rdf:Bag ;
    linkml:class_uri rdf:Bag ;
    linkml:definition_uri okns:RdfBag ;
    linkml:is_a okns:RdfsContainer ;
    linkml:slot_usage [ ] .

okns:RdfsContainerMembershipProperty a linkml:ClassDefinition ;
    dcterms:source rdfs: ;
    dcterms:title "ContainerMembershipProperty" ;
    skos:definition "The class of container membership properties, rdf:_1, rdf:_2, ..., all of which are sub-properties of 'member'." ;
    skos:inScheme okns:owl-rdf-rdfs ;
    skos:mappingRelation rdfs:ContainerMembershipProperty ;
    linkml:class_uri rdfs:ContainerMembershipProperty ;
    linkml:definition_uri okns:RdfsContainerMembershipProperty ;
    linkml:is_a okns:RdfProperty ;
    linkml:slot_usage [ ] .

okns:SimInfluence a linkml:ClassDefinition ;
    dcterms:source sim: ;
    dcterms:title "Influence" ;
    skos:definition "An abstract class indicating a directed association of influence where the subject entity has influenced the object entity." ;
    skos:inScheme okns:sim ;
    skos:mappingRelation sim:Influence ;
    linkml:class_uri sim:Influence ;
    linkml:definition_uri okns:SimInfluence ;
    linkml:is_a okns:SimAssociation ;
    linkml:slot_usage [ ] .

okns:SimSimilarity a linkml:ClassDefinition ;
    dcterms:source sim: ;
    dcterms:title "Similarity" ;
    skos:definition "An abstract class to define similarity between two or more things.  Entities share a similarity if they share some common characteristics of interest.  A similarity is a special type of association." ;
    skos:inScheme okns:sim ;
    skos:mappingRelation sim:Similarity ;
    linkml:class_uri sim:Similarity ;
    linkml:definition_uri okns:SimSimilarity ;
    linkml:is_a okns:SimAssociation ;
    linkml:slot_usage [ ] .

okns:Time-entryInstant a linkml:ClassDefinition ;
    skos:inScheme okns:daml ;
    skos:mappingRelation time-entry:Instant ;
    linkml:class_uri time-entry:Instant ;
    linkml:definition_uri okns:Time-entryInstant ;
    linkml:is_a okns:Time-entryInstantThing ;
    linkml:slot_usage [ ] .

okns:Time-entryInstantEvent a linkml:ClassDefinition ;
    skos:inScheme okns:daml ;
    skos:mappingRelation time-entry:InstantEvent ;
    linkml:class_uri time-entry:InstantEvent ;
    linkml:definition_uri okns:Time-entryInstantEvent ;
    linkml:is_a okns:Time-entryEvent ;
    linkml:slot_usage [ ] .

okns:Time-entryInterval a linkml:ClassDefinition ;
    skos:inScheme okns:daml ;
    skos:mappingRelation time-entry:Interval ;
    linkml:class_uri time-entry:Interval ;
    linkml:definition_uri okns:Time-entryInterval ;
    linkml:is_a okns:Time-entryIntervalThing ;
    linkml:slot_usage [ ] .

okns:Time-entryIntervalEvent a linkml:ClassDefinition ;
    skos:inScheme okns:daml ;
    skos:mappingRelation time-entry:IntervalEvent ;
    linkml:class_uri time-entry:IntervalEvent ;
    linkml:definition_uri okns:Time-entryIntervalEvent ;
    linkml:is_a okns:Time-entryEvent ;
    linkml:slot_usage [ ] .

okns:Time-entryTemporalEntity a linkml:ClassDefinition ;
    dcterms:title "No class (entity type) name specified -- this class is noted as a superclass of another class in this graph but has not itself been defined." ;
    skos:inScheme okns:daml ;
    skos:mappingRelation time-entry:TemporalEntity ;
    linkml:class_uri time-entry:TemporalEntity ;
    linkml:definition_uri okns:Time-entryTemporalEntity ;
    linkml:is_a okns:Time-entryTemporalThing ;
    linkml:slot_usage [ ] .

okns:TimeJanuary a linkml:ClassDefinition ;
    dcterms:title "January" ;
    skos:editorialNote "This class was present in the 2006 version of OWL-Time. It was presented as an example of how DateTimeDescription could be specialized, but does not belong in the revised ontology." ;
    skos:inScheme okns:time ;
    skos:mappingRelation time:January ;
    linkml:deprecated "true" ;
    linkml:class_uri time:January ;
    linkml:definition_uri okns:TimeJanuary ;
    linkml:is_a okns:TimeDateTimeDescription ;
    linkml:slot_usage [ ] .

okns:TimeYear a linkml:ClassDefinition ;
    dcterms:title "Year" ;
    skos:definition "Year duration" ;
    skos:editorialNote """Year was proposed in the 2006 version of OWL-Time as an example of how DurationDescription could be specialized to allow for a duration to be restricted to a number of years. 

It is deprecated in this edition of OWL-Time.""" ;
    skos:inScheme okns:time ;
    skos:mappingRelation time:Year ;
    skos:note "description: Year duration" ;
    linkml:deprecated "true" ;
    linkml:class_uri time:Year ;
    linkml:definition_uri okns:TimeYear ;
    linkml:is_a okns:TimeDurationDescription ;
    linkml:slot_usage [ ] .

okns:TzontCity a linkml:ClassDefinition ;
    skos:inScheme okns:daml ;
    skos:mappingRelation tzont:City ;
    linkml:class_uri tzont:City ;
    linkml:definition_uri okns:TzontCity ;
    linkml:is_a okns:TzontPoliticalRegion ;
    linkml:slot_usage [ ] .

okns:TzontCounty a linkml:ClassDefinition ;
    skos:inScheme okns:daml ;
    skos:mappingRelation tzont:County ;
    linkml:class_uri tzont:County ;
    linkml:definition_uri okns:TzontCounty ;
    linkml:is_a okns:TzontPoliticalRegion ;
    linkml:slot_usage [ ] .

okns:TzontEnumeratedDaylightSavingsPolicy a linkml:ClassDefinition ;
    skos:inScheme okns:daml ;
    skos:mappingRelation tzont:EnumeratedDaylightSavingsPolicy ;
    linkml:class_uri tzont:EnumeratedDaylightSavingsPolicy ;
    linkml:definition_uri okns:TzontEnumeratedDaylightSavingsPolicy ;
    linkml:is_a okns:TzontDaylightSavingsPolicy ;
    linkml:slot_usage [ ] .

okns:TzontReservation a linkml:ClassDefinition ;
    skos:inScheme okns:daml ;
    skos:mappingRelation tzont:Reservation ;
    linkml:class_uri tzont:Reservation ;
    linkml:definition_uri okns:TzontReservation ;
    linkml:is_a okns:TzontPoliticalRegion ;
    linkml:slot_usage [ ] .

okns:WgsPoint a linkml:ClassDefinition ;
    dcterms:title "point" ;
    skos:definition "A point, typically described using a coordinate system relative to Earth, such as WGS84." ;
    skos:inScheme okns:wgs ;
    skos:mappingRelation wgs1:Point ;
    skos:note """description: Uniquely identified by lat/long/alt. i.e.

spaciallyIntersects(P1, P2) :- lat(P1, LAT), long(P1, LONG), alt(P1, ALT),
  lat(P2, LAT), long(P2, LONG), alt(P2, ALT).

sameThing(P1, P2) :- type(P1, Point), type(P2, Point), spaciallyIntersects(P1, P2).""" ;
    linkml:class_uri wgs1:Point ;
    linkml:definition_uri okns:WgsPoint ;
    linkml:is_a okns:WgsSpatialThing ;
    linkml:slot_usage [ ] .

okns:ao_activity a linkml:SlotDefinition ;
    dcterms:source ao: ;
    dcterms:title "has activity" ;
    rdfs:subPropertyOf okns:ao_context ;
    skos:definition "An activity, which is associated to an individual, e.g. dancing, sleeping, driving." ;
    skos:editorialNote "No occurrences of this slot in the graph." ;
    skos:inScheme okns:ao ;
    skos:mappingRelation ao:activity ;
    linkml:definition_uri okns:ao_activity ;
    linkml:inlined true ;
    linkml:range okns:Any ;
    linkml:slot_uri ao:activity .

okns:ao_location a linkml:SlotDefinition ;
    dcterms:source ao: ;
    dcterms:title "has location" ;
    rdfs:subPropertyOf okns:ao_context ;
    skos:definition "A location, which is associated to an individual, e.g. my house, my country, my current whereabouts." ;
    skos:editorialNote "No occurrences of this slot in the graph." ;
    skos:inScheme okns:ao ;
    skos:mappingRelation ao:location ;
    linkml:definition_uri okns:ao_location ;
    linkml:inlined true ;
    linkml:range okns:Any ;
    linkml:slot_uri ao:location .

okns:ao_time a linkml:SlotDefinition ;
    dcterms:source ao: ;
    dcterms:title "has time" ;
    rdfs:subPropertyOf okns:ao_context ;
    skos:definition "A time, which is associated to an individual, e.g. morning, afternoon, evening." ;
    skos:editorialNote "No occurrences of this slot in the graph." ;
    skos:exactMatch dc:date ;
    skos:inScheme okns:ao ;
    skos:mappingRelation ao:time ;
    linkml:definition_uri okns:ao_time ;
    linkml:inlined true ;
    linkml:range okns:Any ;
    linkml:slot_uri ao:time .

okns:ao_used_application a linkml:SlotDefinition ;
    dcterms:source ao: ;
    dcterms:title "has used application" ;
    rdfs:subPropertyOf okns:ao_application ;
    skos:definition "An application that is related to an event, e.g. a iTunes to a play back event of a music track." ;
    skos:editorialNote "No occurrences of this slot in the graph." ;
    skos:inScheme okns:ao ;
    skos:mappingRelation ao:used_application ;
    linkml:definition_uri okns:ao_used_application ;
    linkml:inlined true ;
    linkml:range okns:Any ;
    linkml:slot_uri ao:used_application .

okns:ao_used_device a linkml:SlotDefinition ;
    dcterms:source ao: ;
    dcterms:title "has used device" ;
    rdfs:subPropertyOf okns:ao_device ;
    skos:definition "A device that is related to an event, e.g. a MP3 player to a play back event of a music track." ;
    skos:editorialNote "No occurrences of this slot in the graph." ;
    skos:inScheme okns:ao ;
    skos:mappingRelation ao:used_device ;
    linkml:definition_uri okns:ao_used_device ;
    linkml:inlined true ;
    linkml:range okns:Any ;
    linkml:slot_uri ao:used_device .

okns:boolean a linkml:TypeDefinition ;
    skos:definition "A binary (true or false) value" ;
    skos:editorialNote "If you are authoring schemas in LinkML YAML, the type is referenced with the lower case \"boolean\"." ;
    skos:exactMatch schema1:Boolean ;
    skos:inScheme linkml:types ;
    linkml:base "Bool" ;
    linkml:imported_from "linkml:types" ;
    linkml:repr "bool" ;
    linkml:definition_uri linkml:Boolean ;
    linkml:uri xsd:boolean .

okns:daml_oil_isDefinedBy a linkml:SlotDefinition ;
    rdfs:subPropertyOf okns:daml_oil_seeAlso ;
    skos:editorialNote "No occurrences of this slot in the graph." ;
    skos:inScheme okns:daml ;
    skos:mappingRelation daml-oil:isDefinedBy ;
    linkml:definition_uri okns:daml_oil_isDefinedBy ;
    linkml:inlined true ;
    linkml:range okns:Any ;
    linkml:slot_uri daml-oil:isDefinedBy .

okns:daml_oil_type a linkml:SlotDefinition ;
    skos:editorialNote "No occurrences of this slot in the graph." ;
    skos:inScheme okns:daml ;
    skos:mappingRelation daml-oil:type ;
    linkml:definition_uri okns:daml_oil_type ;
    linkml:inlined true ;
    linkml:range okns:Any ;
    linkml:slot_uri daml-oil:type .

okns:daml_oil_value a linkml:SlotDefinition ;
    skos:editorialNote "No occurrences of this slot in the graph." ;
    skos:inScheme okns:daml ;
    skos:mappingRelation daml-oil:value ;
    linkml:definition_uri okns:daml_oil_value ;
    linkml:inlined true ;
    linkml:range okns:Any ;
    linkml:slot_uri daml-oil:value .

okns:dc_creator a linkml:SlotDefinition ;
    dcterms:source dc: ;
    dcterms:title "Creator" ;
    skos:definition "Examples of a Creator include a person, an organization, or a service. Typically, the name of a Creator should be used to indicate the entity." ;
    skos:editorialNote "A [second property](/specifications/dublin-core/dcmi-terms/#http://purl.org/dc/terms/creator) with the same name as this property has been declared in the [dcterms: namespace](http://purl.org/dc/terms/).  See the Introduction to the document [DCMI Metadata Terms](/specifications/dublin-core/dcmi-terms/) for an explanation.",
        "No occurrences of this slot in the graph." ;
    skos:inScheme okns:dc ;
    skos:mappingRelation dc:creator ;
    skos:note "description: An entity primarily responsible for making the resource." ;
    linkml:definition_uri okns:dc_creator ;
    linkml:inlined true ;
    linkml:range okns:Any ;
    linkml:slot_uri dc:creator .

okns:dc_source a linkml:SlotDefinition ;
    dcterms:source dc: ;
    dcterms:title "Source" ;
    skos:definition "The described resource may be derived from the related resource in whole or in part. Recommended best practice is to identify the related resource by means of a string conforming to a formal identification system." ;
    skos:editorialNote "A [second property](/specifications/dublin-core/dcmi-terms/#http://purl.org/dc/terms/source) with the same name as this property has been declared in the [dcterms: namespace](http://purl.org/dc/terms/).  See the Introduction to the document [DCMI Metadata Terms](/specifications/dublin-core/dcmi-terms/) for an explanation.",
        "No occurrences of this slot in the graph." ;
    skos:inScheme okns:dc ;
    skos:mappingRelation dc:source ;
    skos:note "description: A related resource from which the described resource is derived." ;
    linkml:definition_uri okns:dc_source ;
    linkml:inlined true ;
    linkml:range okns:Any ;
    linkml:slot_uri dc:source .

okns:dcam_domainIncludes a linkml:SlotDefinition ;
    dcterms:source dcam: ;
    dcterms:title "Domain Includes" ;
    skos:definition "A suggested class for subjects of this property." ;
    skos:editorialNote "No occurrences of this slot in the graph." ;
    skos:inScheme okns:dc ;
    skos:mappingRelation dcam:domainIncludes ;
    linkml:definition_uri okns:dcam_domainIncludes ;
    linkml:inlined true ;
    linkml:range okns:Any ;
    linkml:slot_uri dcam:domainIncludes .

okns:dcam_memberOf a linkml:SlotDefinition ;
    dcterms:source dcam: ;
    dcterms:title "Member Of" ;
    rdfs:seeAlso <https://www.dublincore.org/specifications/dublin-core/2007/06/04/abstract-model/> ;
    skos:definition "A relationship between a resource and a vocabulary encoding scheme which indicates that the resource is a member of a set." ;
    skos:editorialNote "No occurrences of this slot in the graph." ;
    skos:inScheme okns:dc ;
    skos:mappingRelation dcam:memberOf ;
    linkml:definition_uri okns:dcam_memberOf ;
    linkml:inlined true ;
    linkml:range okns:DcamVocabularyEncodingScheme ;
    linkml:slot_uri dcam:memberOf .

okns:dcam_rangeIncludes a linkml:SlotDefinition ;
    dcterms:source dcam: ;
    dcterms:title "Range Includes" ;
    skos:definition "A suggested class for values of this property." ;
    skos:editorialNote "No occurrences of this slot in the graph." ;
    skos:inScheme okns:dc ;
    skos:mappingRelation dcam:rangeIncludes ;
    linkml:definition_uri okns:dcam_rangeIncludes ;
    linkml:inlined true ;
    linkml:range okns:Any ;
    linkml:slot_uri dcam:rangeIncludes .

okns:dct_abstract a linkml:SlotDefinition ;
    dcterms:source dcterms: ;
    dcterms:title "Abstract" ;
    rdfs:subPropertyOf okns:dct_description ;
    skos:definition "A summary of the resource." ;
    skos:editorialNote "No occurrences of this slot in the graph." ;
    skos:inScheme okns:dc ;
    skos:mappingRelation dcterms:abstract ;
    linkml:definition_uri okns:dct_abstract ;
    linkml:inlined true ;
    linkml:range okns:Any ;
    linkml:slot_uri dcterms:abstract .

okns:dct_accessRights a linkml:SlotDefinition ;
    dcterms:source dcterms: ;
    dcterms:title "Access Rights" ;
    rdfs:subPropertyOf okns:dct_rights ;
    skos:definition "Access Rights may include information regarding access or restrictions based on privacy, security, or other policies." ;
    skos:editorialNote "No occurrences of this slot in the graph." ;
    skos:inScheme okns:dc ;
    skos:mappingRelation dcterms:accessRights ;
    skos:note "description: Information about who access the resource or an indication of its security status." ;
    linkml:definition_uri okns:dct_accessRights ;
    linkml:inlined true ;
    linkml:range okns:Any ;
    linkml:slot_uri dcterms:accessRights .

okns:dct_alternative a linkml:SlotDefinition ;
    dcterms:source dcterms: ;
    dcterms:title "Alternative Title" ;
    rdfs:subPropertyOf okns:dct_title ;
    skos:definition "The distinction between titles and alternative titles is application-specific." ;
    skos:editorialNote "No occurrences of this slot in the graph." ;
    skos:inScheme okns:dc ;
    skos:mappingRelation dcterms:alternative ;
    skos:note "description: An alternative name for the resource." ;
    linkml:definition_uri okns:dct_alternative ;
    linkml:inlined true ;
    linkml:range okns:RdfsLiteral ;
    linkml:slot_uri dcterms:alternative .

okns:dct_available a linkml:SlotDefinition ;
    dcterms:source dcterms: ;
    dcterms:title "Date Available" ;
    rdfs:subPropertyOf okns:dct_date ;
    skos:definition "Recommended practice is to describe the date, date/time, or period of time as recommended for the property Date, of which this is a subproperty." ;
    skos:editorialNote "No occurrences of this slot in the graph." ;
    skos:inScheme okns:dc ;
    skos:mappingRelation dcterms:available ;
    skos:note "description: Date that the resource became or will become available." ;
    linkml:definition_uri okns:dct_available ;
    linkml:inlined true ;
    linkml:range okns:RdfsLiteral ;
    linkml:slot_uri dcterms:available .

okns:dct_bibliographicCitation a linkml:SlotDefinition ;
    dcterms:source dcterms: ;
    dcterms:title "Bibliographic Citation" ;
    rdfs:subPropertyOf okns:dct_identifier ;
    skos:definition "Recommended practice is to include sufficient bibliographic detail to identify the resource as unambiguously as possible." ;
    skos:editorialNote "No occurrences of this slot in the graph." ;
    skos:inScheme okns:dc ;
    skos:mappingRelation dcterms:bibliographicCitation ;
    skos:note "description: A bibliographic reference for the resource." ;
    linkml:definition_uri okns:dct_bibliographicCitation ;
    linkml:inlined true ;
    linkml:range okns:RdfsLiteral ;
    linkml:slot_uri dcterms:bibliographicCitation .

okns:dct_conformsTo a linkml:SlotDefinition ;
    dcterms:source dcterms: ;
    dcterms:title "Conforms To" ;
    rdfs:subPropertyOf okns:dct_relation ;
    skos:definition "An established standard to which the described resource conforms." ;
    skos:editorialNote "No occurrences of this slot in the graph." ;
    skos:inScheme okns:dc ;
    skos:mappingRelation dcterms:conformsTo ;
    linkml:definition_uri okns:dct_conformsTo ;
    linkml:inlined true ;
    linkml:range okns:Any ;
    linkml:slot_uri dcterms:conformsTo .

okns:dct_created a linkml:SlotDefinition ;
    dcterms:source dcterms: ;
    dcterms:title "Date Created" ;
    rdfs:subPropertyOf okns:dct_date ;
    skos:definition "Recommended practice is to describe the date, date/time, or period of time as recommended for the property Date, of which this is a subproperty." ;
    skos:editorialNote "No occurrences of this slot in the graph." ;
    skos:inScheme okns:dc ;
    skos:mappingRelation dcterms:created ;
    skos:note "description: Date of creation of the resource." ;
    linkml:definition_uri okns:dct_created ;
    linkml:inlined true ;
    linkml:range okns:RdfsLiteral ;
    linkml:slot_uri dcterms:created .

okns:dct_creator a linkml:SlotDefinition ;
    dcterms:source dcterms: ;
    dcterms:title "Creator" ;
    rdfs:subPropertyOf okns:dct_contributor ;
    skos:definition "Recommended practice is to identify the creator with a URI.  If this is not possible or feasible, a literal value that identifies the creator may be provided." ;
    skos:editorialNote "No occurrences of this slot in the graph." ;
    skos:exactMatch foaf:maker ;
    skos:inScheme okns:dc ;
    skos:mappingRelation dcterms:creator ;
    skos:note "description: An entity responsible for making the resource." ;
    linkml:definition_uri okns:dct_creator ;
    linkml:inlined true ;
    linkml:range okns:Any ;
    linkml:slot_uri dcterms:creator .

okns:dct_dateAccepted a linkml:SlotDefinition ;
    dcterms:source dcterms: ;
    dcterms:title "Date Accepted" ;
    rdfs:subPropertyOf okns:dct_date ;
    skos:definition "Recommended practice is to describe the date, date/time, or period of time as recommended for the property Date, of which this is a subproperty.  Examples of resources to which a date of acceptance may be relevant are a thesis (accepted by a university department) or an article (accepted by a journal)." ;
    skos:editorialNote "No occurrences of this slot in the graph." ;
    skos:inScheme okns:dc ;
    skos:mappingRelation dcterms:dateAccepted ;
    skos:note "description: Date of acceptance of the resource." ;
    linkml:definition_uri okns:dct_dateAccepted ;
    linkml:inlined true ;
    linkml:range okns:RdfsLiteral ;
    linkml:slot_uri dcterms:dateAccepted .

okns:dct_dateCopyrighted a linkml:SlotDefinition ;
    dcterms:source dcterms: ;
    dcterms:title "Date Copyrighted" ;
    rdfs:subPropertyOf okns:dct_date ;
    skos:definition "Typically a year.  Recommended practice is to describe the date, date/time, or period of time as recommended for the property Date, of which this is a subproperty." ;
    skos:editorialNote "No occurrences of this slot in the graph." ;
    skos:inScheme okns:dc ;
    skos:mappingRelation dcterms:dateCopyrighted ;
    skos:note "description: Date of copyright of the resource." ;
    linkml:definition_uri okns:dct_dateCopyrighted ;
    linkml:inlined true ;
    linkml:range okns:RdfsLiteral ;
    linkml:slot_uri dcterms:dateCopyrighted .

okns:dct_dateSubmitted a linkml:SlotDefinition ;
    dcterms:source dcterms: ;
    dcterms:title "Date Submitted" ;
    rdfs:subPropertyOf okns:dct_date ;
    skos:definition "Recommended practice is to describe the date, date/time, or period of time as recommended for the property Date, of which this is a subproperty.  Examples of resources to which a 'Date Submitted' may be relevant include a thesis (submitted to a university department) or an article (submitted to a journal)." ;
    skos:editorialNote "No occurrences of this slot in the graph." ;
    skos:inScheme okns:dc ;
    skos:mappingRelation dcterms:dateSubmitted ;
    skos:note "description: Date of submission of the resource." ;
    linkml:definition_uri okns:dct_dateSubmitted ;
    linkml:inlined true ;
    linkml:range okns:RdfsLiteral ;
    linkml:slot_uri dcterms:dateSubmitted .

okns:dct_educationLevel a linkml:SlotDefinition ;
    dcterms:source dcterms: ;
    dcterms:title "Audience Education Level" ;
    rdfs:subPropertyOf okns:dct_audience ;
    skos:definition "A class of agents, defined in terms of progression through an educational or training context, for which the described resource is intended." ;
    skos:editorialNote "No occurrences of this slot in the graph." ;
    skos:inScheme okns:dc ;
    skos:mappingRelation dcterms:educationLevel ;
    linkml:definition_uri okns:dct_educationLevel ;
    linkml:inlined true ;
    linkml:range okns:Any ;
    linkml:slot_uri dcterms:educationLevel .

okns:dct_extent a linkml:SlotDefinition ;
    dcterms:source dcterms: ;
    dcterms:title "Extent" ;
    rdfs:subPropertyOf okns:dct_format ;
    skos:definition "Recommended practice is to specify the file size in megabytes and duration in ISO 8601 format." ;
    skos:editorialNote "No occurrences of this slot in the graph." ;
    skos:inScheme okns:dc ;
    skos:mappingRelation dcterms:extent ;
    skos:note "description: The size or duration of the resource." ;
    linkml:definition_uri okns:dct_extent ;
    linkml:inlined true ;
    linkml:range okns:Any ;
    linkml:slot_uri dcterms:extent .

okns:dct_hasFormat a linkml:SlotDefinition ;
    dcterms:source dcterms: ;
    dcterms:title "Has Format" ;
    rdfs:subPropertyOf okns:dct_relation ;
    skos:definition "This property is intended to be used with non-literal values. This property is an inverse property of Is Format Of." ;
    skos:editorialNote "No occurrences of this slot in the graph." ;
    skos:inScheme okns:dc ;
    skos:mappingRelation dcterms:hasFormat ;
    skos:note "description: A related resource that is substantially the same as the pre-existing described resource, but in another format." ;
    linkml:definition_uri okns:dct_hasFormat ;
    linkml:inlined true ;
    linkml:range okns:Any ;
    linkml:slot_uri dcterms:hasFormat .

okns:dct_hasPart a linkml:SlotDefinition ;
    dcterms:source dcterms: ;
    dcterms:title "Has Part" ;
    rdfs:subPropertyOf okns:dct_relation ;
    skos:definition "This property is intended to be used with non-literal values. This property is an inverse property of Is Part Of." ;
    skos:editorialNote "No occurrences of this slot in the graph." ;
    skos:inScheme okns:dc ;
    skos:mappingRelation dcterms:hasPart ;
    skos:note "description: A related resource that is included either physically or logically in the described resource." ;
    linkml:definition_uri okns:dct_hasPart ;
    linkml:inlined true ;
    linkml:range okns:Any ;
    linkml:slot_uri dcterms:hasPart .

okns:dct_hasVersion a linkml:SlotDefinition ;
    dcterms:source dcterms: ;
    dcterms:title "Has Version" ;
    rdfs:subPropertyOf okns:dct_relation ;
    skos:definition "Changes in version imply substantive changes in content rather than differences in format. This property is intended to be used with non-literal values. This property is an inverse property of Is Version Of." ;
    skos:editorialNote "No occurrences of this slot in the graph." ;
    skos:inScheme okns:dc ;
    skos:mappingRelation dcterms:hasVersion ;
    skos:note "description: A related resource that is a version, edition, or adaptation of the described resource." ;
    linkml:definition_uri okns:dct_hasVersion ;
    linkml:inlined true ;
    linkml:range okns:Any ;
    linkml:slot_uri dcterms:hasVersion .

okns:dct_instructionalMethod a linkml:SlotDefinition ;
    dcterms:source dcterms: ;
    dcterms:title "Instructional Method" ;
    skos:definition "Instructional Method typically includes ways of presenting instructional materials or conducting instructional activities, patterns of learner-to-learner and learner-to-instructor interactions, and mechanisms by which group and individual levels of learning are measured.  Instructional methods include all aspects of the instruction and learning processes from planning and implementation through evaluation and feedback." ;
    skos:editorialNote "No occurrences of this slot in the graph." ;
    skos:inScheme okns:dc ;
    skos:mappingRelation dcterms:instructionalMethod ;
    skos:note "description: A process, used to engender knowledge, attitudes and skills, that the described resource is designed to support." ;
    linkml:definition_uri okns:dct_instructionalMethod ;
    linkml:inlined true ;
    linkml:range okns:Any ;
    linkml:slot_uri dcterms:instructionalMethod .

okns:dct_isFormatOf a linkml:SlotDefinition ;
    dcterms:source dcterms: ;
    dcterms:title "Is Format Of" ;
    rdfs:subPropertyOf okns:dct_relation ;
    skos:definition "This property is intended to be used with non-literal values. This property is an inverse property of Has Format." ;
    skos:editorialNote "No occurrences of this slot in the graph." ;
    skos:inScheme okns:dc ;
    skos:mappingRelation dcterms:isFormatOf ;
    skos:note "description: A pre-existing related resource that is substantially the same as the described resource, but in another format." ;
    linkml:definition_uri okns:dct_isFormatOf ;
    linkml:inlined true ;
    linkml:range okns:Any ;
    linkml:slot_uri dcterms:isFormatOf .

okns:dct_isPartOf a linkml:SlotDefinition ;
    dcterms:source dcterms: ;
    dcterms:title "Is Part Of" ;
    rdfs:subPropertyOf okns:dct_relation ;
    skos:definition "This property is intended to be used with non-literal values. This property is an inverse property of Has Part." ;
    skos:editorialNote "No occurrences of this slot in the graph." ;
    skos:inScheme okns:dc ;
    skos:mappingRelation dcterms:isPartOf ;
    skos:note "description: A related resource in which the described resource is physically or logically included." ;
    linkml:definition_uri okns:dct_isPartOf ;
    linkml:inlined true ;
    linkml:range okns:Any ;
    linkml:slot_uri dcterms:isPartOf .

okns:dct_isReferencedBy a linkml:SlotDefinition ;
    dcterms:source dcterms: ;
    dcterms:title "Is Referenced By" ;
    rdfs:subPropertyOf okns:dct_relation ;
    skos:definition "This property is intended to be used with non-literal values. This property is an inverse property of References." ;
    skos:editorialNote "No occurrences of this slot in the graph." ;
    skos:inScheme okns:dc ;
    skos:mappingRelation dcterms:isReferencedBy ;
    skos:note "description: A related resource that references, cites, or otherwise points to the described resource." ;
    linkml:definition_uri okns:dct_isReferencedBy ;
    linkml:inlined true ;
    linkml:range okns:Any ;
    linkml:slot_uri dcterms:isReferencedBy .

okns:dct_isReplacedBy a linkml:SlotDefinition ;
    dcterms:source dcterms: ;
    dcterms:title "Is Replaced By" ;
    rdfs:subPropertyOf okns:dct_relation ;
    skos:definition "This property is intended to be used with non-literal values. This property is an inverse property of Replaces." ;
    skos:editorialNote "No occurrences of this slot in the graph." ;
    skos:inScheme okns:dc ;
    skos:mappingRelation dcterms:isReplacedBy ;
    skos:note "description: A related resource that supplants, displaces, or supersedes the described resource." ;
    linkml:definition_uri okns:dct_isReplacedBy ;
    linkml:inlined true ;
    linkml:range okns:Any ;
    linkml:slot_uri dcterms:isReplacedBy .

okns:dct_isRequiredBy a linkml:SlotDefinition ;
    dcterms:source dcterms: ;
    dcterms:title "Is Required By" ;
    rdfs:subPropertyOf okns:dct_relation ;
    skos:definition "This property is intended to be used with non-literal values. This property is an inverse property of Requires." ;
    skos:editorialNote "No occurrences of this slot in the graph." ;
    skos:inScheme okns:dc ;
    skos:mappingRelation dcterms:isRequiredBy ;
    skos:note "description: A related resource that requires the described resource to support its function, delivery, or coherence." ;
    linkml:definition_uri okns:dct_isRequiredBy ;
    linkml:inlined true ;
    linkml:range okns:Any ;
    linkml:slot_uri dcterms:isRequiredBy .

okns:dct_isVersionOf a linkml:SlotDefinition ;
    dcterms:source dcterms: ;
    dcterms:title "Is Version Of" ;
    rdfs:subPropertyOf okns:dct_relation ;
    skos:definition "Changes in version imply substantive changes in content rather than differences in format. This property is intended to be used with non-literal values. This property is an inverse property of Has Version." ;
    skos:editorialNote "No occurrences of this slot in the graph." ;
    skos:inScheme okns:dc ;
    skos:mappingRelation dcterms:isVersionOf ;
    skos:note "description: A related resource of which the described resource is a version, edition, or adaptation." ;
    linkml:definition_uri okns:dct_isVersionOf ;
    linkml:inlined true ;
    linkml:range okns:Any ;
    linkml:slot_uri dcterms:isVersionOf .

okns:dct_language a linkml:SlotDefinition ;
    dcterms:source dcterms: ;
    dcterms:title "Language" ;
    rdfs:subPropertyOf okns:dc_language ;
    skos:definition "Recommended practice is to use either a non-literal value representing a language from a controlled vocabulary such as ISO 639-2 or ISO 639-3, or a literal value consisting of an IETF Best Current Practice 47 [[IETF-BCP47](https://tools.ietf.org/html/bcp47)] language tag." ;
    skos:editorialNote "No occurrences of this slot in the graph." ;
    skos:inScheme okns:dc ;
    skos:mappingRelation dcterms:language ;
    skos:note "description: A language of the resource." ;
    linkml:definition_uri okns:dct_language ;
    linkml:inlined true ;
    linkml:range okns:Any ;
    linkml:slot_uri dcterms:language .

okns:dct_mediator a linkml:SlotDefinition ;
    dcterms:source dcterms: ;
    dcterms:title "Mediator" ;
    rdfs:subPropertyOf okns:dct_audience ;
    skos:definition "In an educational context, a mediator might be a parent, teacher, teaching assistant, or care-giver." ;
    skos:editorialNote "No occurrences of this slot in the graph." ;
    skos:inScheme okns:dc ;
    skos:mappingRelation dcterms:mediator ;
    skos:note "description: An entity that mediates access to the resource." ;
    linkml:definition_uri okns:dct_mediator ;
    linkml:inlined true ;
    linkml:range okns:Any ;
    linkml:slot_uri dcterms:mediator .

okns:dct_medium a linkml:SlotDefinition ;
    dcterms:source dcterms: ;
    dcterms:title "Medium" ;
    rdfs:subPropertyOf okns:dct_format ;
    skos:definition "The material or physical carrier of the resource." ;
    skos:editorialNote "No occurrences of this slot in the graph." ;
    skos:inScheme okns:dc ;
    skos:mappingRelation dcterms:medium ;
    linkml:definition_uri okns:dct_medium ;
    linkml:inlined true ;
    linkml:range okns:Any ;
    linkml:slot_uri dcterms:medium .

okns:dct_modified a linkml:SlotDefinition ;
    dcterms:source dcterms: ;
    dcterms:title "Date Modified" ;
    rdfs:subPropertyOf okns:dct_date ;
    skos:definition "Recommended practice is to describe the date, date/time, or period of time as recommended for the property Date, of which this is a subproperty." ;
    skos:inScheme okns:dc ;
    skos:mappingRelation dcterms:modified ;
    skos:note "description: Date on which the resource was changed." ;
    linkml:any_of [ a okns:AnonymousSlotExpression ;
            linkml:range okns:RdfsLiteral ],
        [ a okns:AnonymousSlotExpression ;
            linkml:range okns:date ] ;
    linkml:definition_uri okns:dct_modified ;
    linkml:inlined true ;
    linkml:range okns:Any ;
    linkml:slot_uri dcterms:modified .

okns:dct_provenance a linkml:SlotDefinition ;
    dcterms:source dcterms: ;
    dcterms:title "Provenance" ;
    skos:definition "The statement may include a description of any changes successive custodians made to the resource." ;
    skos:editorialNote "No occurrences of this slot in the graph." ;
    skos:inScheme okns:dc ;
    skos:mappingRelation dcterms:provenance ;
    skos:note "description: A statement of any changes in ownership and custody of the resource since its creation that are significant for its authenticity, integrity, and interpretation." ;
    linkml:definition_uri okns:dct_provenance ;
    linkml:inlined true ;
    linkml:range okns:Any ;
    linkml:slot_uri dcterms:provenance .

okns:dct_publisher a linkml:SlotDefinition ;
    dcterms:source dcterms: ;
    dcterms:title "Publisher" ;
    rdfs:subPropertyOf okns:dc_publisher ;
    skos:definition "An entity responsible for making the resource available." ;
    skos:inScheme okns:dc ;
    skos:mappingRelation dcterms:publisher ;
    linkml:definition_uri okns:dct_publisher ;
    linkml:range okns:uri ;
    linkml:slot_uri dcterms:publisher .

okns:dct_references a linkml:SlotDefinition ;
    dcterms:source dcterms: ;
    dcterms:title "References" ;
    rdfs:subPropertyOf okns:dct_relation ;
    skos:definition "This property is intended to be used with non-literal values. This property is an inverse property of Is Referenced By." ;
    skos:editorialNote "No occurrences of this slot in the graph." ;
    skos:inScheme okns:dc ;
    skos:mappingRelation dcterms:references ;
    skos:note "description: A related resource that is referenced, cited, or otherwise pointed to by the described resource." ;
    linkml:definition_uri okns:dct_references ;
    linkml:inlined true ;
    linkml:range okns:Any ;
    linkml:slot_uri dcterms:references .

okns:dct_replaces a linkml:SlotDefinition ;
    dcterms:source dcterms: ;
    dcterms:title "Replaces" ;
    rdfs:subPropertyOf okns:dct_relation ;
    skos:definition "This property is intended to be used with non-literal values. This property is an inverse property of Is Replaced By." ;
    skos:editorialNote "No occurrences of this slot in the graph." ;
    skos:inScheme okns:dc ;
    skos:mappingRelation dcterms:replaces ;
    skos:note "description: A related resource that is supplanted, displaced, or superseded by the described resource." ;
    linkml:definition_uri okns:dct_replaces ;
    linkml:inlined true ;
    linkml:range okns:Any ;
    linkml:slot_uri dcterms:replaces .

okns:dct_requires a linkml:SlotDefinition ;
    dcterms:source dcterms: ;
    dcterms:title "Requires" ;
    rdfs:subPropertyOf okns:dct_relation ;
    skos:definition "This property is intended to be used with non-literal values. This property is an inverse property of Is Required By." ;
    skos:editorialNote "No occurrences of this slot in the graph." ;
    skos:inScheme okns:dc ;
    skos:mappingRelation dcterms:requires ;
    skos:note "description: A related resource that is required by the described resource to support its function, delivery, or coherence." ;
    linkml:definition_uri okns:dct_requires ;
    linkml:inlined true ;
    linkml:range okns:Any ;
    linkml:slot_uri dcterms:requires .

okns:dct_rightsHolder a linkml:SlotDefinition ;
    dcterms:source dcterms: ;
    dcterms:title "Rights Holder" ;
    skos:definition "Recommended practice is to refer to the rights holder with a URI. If this is not possible or feasible, a literal value that identifies the rights holder may be provided." ;
    skos:editorialNote "No occurrences of this slot in the graph." ;
    skos:inScheme okns:dc ;
    skos:mappingRelation dcterms:rightsHolder ;
    skos:note "description: A person or organization owning or managing rights over the resource." ;
    linkml:definition_uri okns:dct_rightsHolder ;
    linkml:inlined true ;
    linkml:range okns:Any ;
    linkml:slot_uri dcterms:rightsHolder .

okns:dct_spatial a linkml:SlotDefinition ;
    dcterms:source dcterms: ;
    dcterms:title "Spatial Coverage" ;
    rdfs:subPropertyOf okns:dct_coverage ;
    skos:definition "Spatial characteristics of the resource." ;
    skos:editorialNote "No occurrences of this slot in the graph." ;
    skos:inScheme okns:dc ;
    skos:mappingRelation dcterms:spatial ;
    linkml:definition_uri okns:dct_spatial ;
    linkml:inlined true ;
    linkml:range okns:Any ;
    linkml:slot_uri dcterms:spatial .

okns:dct_tableOfContents a linkml:SlotDefinition ;
    dcterms:source dcterms: ;
    dcterms:title "Table Of Contents" ;
    rdfs:subPropertyOf okns:dct_description ;
    skos:definition "A list of subunits of the resource." ;
    skos:editorialNote "No occurrences of this slot in the graph." ;
    skos:inScheme okns:dc ;
    skos:mappingRelation dcterms:tableOfContents ;
    linkml:definition_uri okns:dct_tableOfContents ;
    linkml:inlined true ;
    linkml:range okns:Any ;
    linkml:slot_uri dcterms:tableOfContents .

okns:dct_temporal a linkml:SlotDefinition ;
    dcterms:source dcterms: ;
    dcterms:title "Temporal Coverage" ;
    rdfs:subPropertyOf okns:dct_coverage ;
    skos:definition "Temporal characteristics of the resource." ;
    skos:editorialNote "No occurrences of this slot in the graph." ;
    skos:inScheme okns:dc ;
    skos:mappingRelation dcterms:temporal ;
    linkml:definition_uri okns:dct_temporal ;
    linkml:inlined true ;
    linkml:range okns:Any ;
    linkml:slot_uri dcterms:temporal .

okns:dct_type a linkml:SlotDefinition ;
    dcterms:source dcterms: ;
    dcterms:title "Type" ;
    rdfs:subPropertyOf okns:dc_type ;
    skos:definition "Recommended practice is to use a controlled vocabulary such as the DCMI Type Vocabulary [[DCMI-TYPE](http://dublincore.org/documents/dcmi-type-vocabulary/)]. To describe the file format, physical medium, or dimensions of the resource, use the property Format." ;
    skos:editorialNote "No occurrences of this slot in the graph." ;
    skos:inScheme okns:dc ;
    skos:mappingRelation dcterms:type ;
    skos:note "description: The nature or genre of the resource." ;
    linkml:definition_uri okns:dct_type ;
    linkml:inlined true ;
    linkml:range okns:Any ;
    linkml:slot_uri dcterms:type .

okns:dct_valid a linkml:SlotDefinition ;
    dcterms:source dcterms: ;
    dcterms:title "Date Valid" ;
    rdfs:subPropertyOf okns:dct_date ;
    skos:definition "Recommended practice is to describe the date, date/time, or period of time as recommended for the property Date, of which this is a subproperty." ;
    skos:editorialNote "No occurrences of this slot in the graph." ;
    skos:inScheme okns:dc ;
    skos:mappingRelation dcterms:valid ;
    skos:note "description: Date (often a range) of validity of a resource." ;
    linkml:definition_uri okns:dct_valid ;
    linkml:inlined true ;
    linkml:range okns:RdfsLiteral ;
    linkml:slot_uri dcterms:valid .

okns:event_hasAgent a linkml:SlotDefinition ;
    skos:editorialNote "No occurrences of this slot in the graph." ;
    skos:inScheme okns:event ;
    skos:mappingRelation event:hasAgent ;
    linkml:definition_uri okns:event_hasAgent ;
    linkml:inlined true ;
    linkml:range okns:Any ;
    linkml:slot_uri event:hasAgent .

okns:event_hasFactor a linkml:SlotDefinition ;
    skos:editorialNote "No occurrences of this slot in the graph." ;
    skos:inScheme okns:event ;
    skos:mappingRelation event:hasFactor ;
    linkml:definition_uri okns:event_hasFactor ;
    linkml:inlined true ;
    linkml:range okns:Any ;
    linkml:slot_uri event:hasFactor .

okns:event_hasLiteralFactor a linkml:SlotDefinition ;
    skos:editorialNote "No occurrences of this slot in the graph." ;
    skos:inScheme okns:event ;
    skos:mappingRelation event:hasLiteralFactor ;
    linkml:definition_uri okns:event_hasLiteralFactor ;
    linkml:inlined true ;
    linkml:range okns:Any ;
    linkml:slot_uri event:hasLiteralFactor .

okns:event_hasProduct a linkml:SlotDefinition ;
    skos:editorialNote "No occurrences of this slot in the graph." ;
    skos:inScheme okns:event ;
    skos:mappingRelation event:hasProduct ;
    linkml:definition_uri okns:event_hasProduct ;
    linkml:inlined true ;
    linkml:range okns:Any ;
    linkml:slot_uri event:hasProduct .

okns:event_hasSubEvent a linkml:SlotDefinition ;
    skos:editorialNote "No occurrences of this slot in the graph." ;
    skos:inScheme okns:event ;
    skos:mappingRelation event:hasSubEvent ;
    linkml:definition_uri okns:event_hasSubEvent ;
    linkml:inlined true ;
    linkml:range okns:Any ;
    linkml:slot_uri event:hasSubEvent .

okns:foaf_dnaChecksum a linkml:SlotDefinition ;
    dcterms:source foaf: ;
    dcterms:title "DNA checksum" ;
    skos:definition "A checksum for the DNA of some thing. Joke." ;
    skos:editorialNote "No occurrences of this slot in the graph." ;
    skos:inScheme okns:foaf ;
    skos:mappingRelation foaf:dnaChecksum ;
    linkml:definition_uri okns:foaf_dnaChecksum ;
    linkml:inlined true ;
    linkml:range okns:RdfsLiteral ;
    linkml:slot_uri foaf:dnaChecksum .

okns:foaf_givenName a linkml:SlotDefinition ;
    dcterms:source foaf: ;
    dcterms:title "Given name" ;
    skos:definition "The given name of some person." ;
    skos:editorialNote "No occurrences of this slot in the graph." ;
    skos:inScheme okns:foaf ;
    skos:mappingRelation foaf:givenName ;
    linkml:definition_uri okns:foaf_givenName ;
    linkml:inlined true ;
    linkml:range okns:Any ;
    linkml:slot_uri foaf:givenName .

okns:foaf_givenname a linkml:SlotDefinition ;
    dcterms:source foaf: ;
    dcterms:title "Given name" ;
    skos:definition "The given name of some person." ;
    skos:editorialNote "No occurrences of this slot in the graph." ;
    skos:inScheme okns:foaf ;
    skos:mappingRelation foaf:givenname ;
    linkml:definition_uri okns:foaf_givenname ;
    linkml:inlined true ;
    linkml:range okns:Any ;
    linkml:slot_uri foaf:givenname .

okns:foaf_membershipClass a linkml:SlotDefinition ;
    dcterms:source foaf: ;
    dcterms:title "membershipClass" ;
    skos:definition "Indicates the class of individuals that are a member of a Group" ;
    skos:editorialNote "No occurrences of this slot in the graph." ;
    skos:inScheme okns:foaf ;
    skos:mappingRelation foaf:membershipClass ;
    linkml:definition_uri okns:foaf_membershipClass ;
    linkml:inlined true ;
    linkml:range okns:Any ;
    linkml:slot_uri foaf:membershipClass .

okns:foaf_phone a linkml:SlotDefinition ;
    dcterms:source foaf: ;
    dcterms:title "phone" ;
    skos:definition "A phone,  specified using fully qualified tel: URI scheme (refs: http://www.w3.org/Addressing/schemes.html#tel)." ;
    skos:editorialNote "No occurrences of this slot in the graph." ;
    skos:inScheme okns:foaf ;
    skos:mappingRelation foaf:phone ;
    linkml:definition_uri okns:foaf_phone ;
    linkml:inlined true ;
    linkml:range okns:Any ;
    linkml:slot_uri foaf:phone .

okns:foaf_title a linkml:SlotDefinition ;
    dcterms:source foaf: ;
    dcterms:title "title" ;
    skos:definition "Title (Mr, Mrs, Ms, Dr. etc)" ;
    skos:editorialNote "No occurrences of this slot in the graph." ;
    skos:inScheme okns:foaf ;
    skos:mappingRelation foaf:title ;
    linkml:definition_uri okns:foaf_title ;
    linkml:inlined true ;
    linkml:range okns:Any ;
    linkml:slot_uri foaf:title .

okns:http___purl.org_vocab_bio_0.1_event a linkml:SlotDefinition ;
    dcterms:title "No slot (predicate) name specified -- this slot is noted as a subproperty of another slot in this graph but has not itself been defined." ;
    skos:editorialNote "No occurrences of this slot in the graph." ;
    skos:inScheme okns:mo ;
    skos:mappingRelation <http://purl.org/vocab/bio/0.1/event> ;
    linkml:definition_uri okns:http___purl.org_vocab_bio_0.1_event ;
    linkml:inlined true ;
    linkml:range okns:Any ;
    linkml:slot_uri <http://purl.org/vocab/bio/0.1/event> .

okns:ical_X_ a linkml:SlotDefinition ;
    dcterms:title "Any property name with a \"X-\" prefix" ;
    skos:definition "This class of property provides a framework for defining non-standard properties." ;
    skos:editorialNote "No occurrences of this slot in the graph." ;
    skos:inScheme okns:ical ;
    skos:mappingRelation ical:X- ;
    skos:note "description: value type: TEXT" ;
    linkml:definition_uri okns:ical_X_ ;
    linkml:range okns:string ;
    linkml:slot_uri ical:X- .

okns:ical_action a linkml:SlotDefinition ;
    dcterms:title "ACTION" ;
    skos:definition "This property defines the action to be invoked when an alarm is triggered." ;
    skos:editorialNote "No occurrences of this slot in the graph." ;
    skos:inScheme okns:ical ;
    skos:mappingRelation ical:action ;
    skos:note "description: value type: TEXT" ;
    linkml:definition_uri okns:ical_action ;
    linkml:range okns:string ;
    linkml:slot_uri ical:action .

okns:ical_attach a linkml:SlotDefinition ;
    dcterms:title "ATTACH" ;
    skos:definition "The property provides the capability to associate a document object with a calendar component." ;
    skos:editorialNote "No occurrences of this slot in the graph." ;
    skos:inScheme okns:ical ;
    skos:mappingRelation ical:attach ;
    skos:note "description: default value type: URI" ;
    linkml:definition_uri okns:ical_attach ;
    linkml:inlined true ;
    linkml:range okns:Any ;
    linkml:slot_uri ical:attach .

okns:ical_attendee a linkml:SlotDefinition ;
    dcterms:title "ATTENDEE" ;
    skos:definition "The property defines an \"Attendee\" within a calendar component." ;
    skos:editorialNote "No occurrences of this slot in the graph." ;
    skos:inScheme okns:ical ;
    skos:mappingRelation ical:attendee ;
    skos:note "description: value type: CAL-ADDRESS" ;
    linkml:definition_uri okns:ical_attendee ;
    linkml:inlined true ;
    linkml:range okns:IcalValueCAL-ADDRESS ;
    linkml:slot_uri ical:attendee .

okns:ical_calscale a linkml:SlotDefinition ;
    dcterms:title "CALSCALE" ;
    skos:definition "This property defines the calendar scale used for the calendar information specified in the iCalendar object." ;
    skos:editorialNote "No occurrences of this slot in the graph." ;
    skos:inScheme okns:ical ;
    skos:mappingRelation ical:calscale ;
    skos:note "description: value type: TEXT" ;
    linkml:definition_uri okns:ical_calscale ;
    linkml:range okns:string ;
    linkml:slot_uri ical:calscale .

okns:ical_categories a linkml:SlotDefinition ;
    dcterms:title "CATEGORIES" ;
    skos:definition "This property defines the categories for a calendar component." ;
    skos:editorialNote "No occurrences of this slot in the graph." ;
    skos:inScheme okns:ical ;
    skos:mappingRelation ical:categories ;
    skos:note "description: value type: TEXT" ;
    linkml:definition_uri okns:ical_categories ;
    linkml:range okns:string ;
    linkml:slot_uri ical:categories .

okns:ical_class a linkml:SlotDefinition ;
    dcterms:title "CLASS" ;
    skos:definition "This property defines the access classification for a calendar component." ;
    skos:editorialNote "No occurrences of this slot in the graph." ;
    skos:inScheme okns:ical ;
    skos:mappingRelation ical:class ;
    skos:note "description: value type: TEXT" ;
    linkml:definition_uri okns:ical_class ;
    linkml:range okns:string ;
    linkml:slot_uri ical:class .

okns:ical_comment a linkml:SlotDefinition ;
    dcterms:title "COMMENT" ;
    skos:definition "This property specifies non-processing information intended to provide a comment to the calendar user." ;
    skos:editorialNote "No occurrences of this slot in the graph." ;
    skos:inScheme okns:ical ;
    skos:mappingRelation ical:comment ;
    skos:note "description: value type: TEXT" ;
    linkml:definition_uri okns:ical_comment ;
    linkml:range okns:string ;
    linkml:slot_uri ical:comment .

okns:ical_contact a linkml:SlotDefinition ;
    dcterms:title "CONTACT" ;
    skos:definition "The property is used to represent contact information or alternately a reference to contact information associated with the calendar component." ;
    skos:editorialNote "No occurrences of this slot in the graph." ;
    skos:inScheme okns:ical ;
    skos:mappingRelation ical:contact ;
    skos:note "description: value type: TEXT" ;
    linkml:definition_uri okns:ical_contact ;
    linkml:range okns:string ;
    linkml:slot_uri ical:contact .

okns:ical_created a linkml:SlotDefinition ;
    dcterms:title "CREATED" ;
    skos:definition "This property specifies the date and time that the calendar information was created by the calendar user agent in the calendar store. Note: This is analogous to the creation date and time for a file in the file system." ;
    skos:editorialNote "No occurrences of this slot in the graph." ;
    skos:inScheme okns:ical ;
    skos:mappingRelation ical:created ;
    skos:note "description: value type: DATE-TIME" ;
    linkml:definition_uri okns:ical_created ;
    linkml:inlined true ;
    linkml:range okns:IcalValueDATE-TIME ;
    linkml:slot_uri ical:created .

okns:ical_description a linkml:SlotDefinition ;
    dcterms:title "DESCRIPTION" ;
    skos:definition "This property provides a more complete description of the calendar component, than that provided by the \"SUMMARY\" property." ;
    skos:editorialNote "No occurrences of this slot in the graph." ;
    skos:inScheme okns:ical ;
    skos:mappingRelation ical:description ;
    skos:note "description: value type: TEXT" ;
    linkml:definition_uri okns:ical_description ;
    linkml:range okns:string ;
    linkml:slot_uri ical:description .

okns:ical_dtend a linkml:SlotDefinition ;
    dcterms:title "DTEND" ;
    skos:definition "This property specifies the date and time that a calendar component ends." ;
    skos:editorialNote "No occurrences of this slot in the graph." ;
    skos:inScheme okns:ical ;
    skos:mappingRelation ical:dtend ;
    skos:note "description: default value type: DATE-TIME" ;
    linkml:definition_uri okns:ical_dtend ;
    linkml:inlined true ;
    linkml:range okns:Any ;
    linkml:slot_uri ical:dtend .

okns:ical_dtstamp a linkml:SlotDefinition ;
    dcterms:title "DTSTAMP" ;
    skos:definition "The property indicates the date/time that the instance of the iCalendar object was created." ;
    skos:editorialNote "No occurrences of this slot in the graph." ;
    skos:inScheme okns:ical ;
    skos:mappingRelation ical:dtstamp ;
    skos:note "description: value type: DATE-TIME" ;
    linkml:definition_uri okns:ical_dtstamp ;
    linkml:inlined true ;
    linkml:range okns:IcalValueDATE-TIME ;
    linkml:slot_uri ical:dtstamp .

okns:ical_dtstart a linkml:SlotDefinition ;
    dcterms:title "DTSTART" ;
    skos:definition "This property specifies when the calendar component begins." ;
    skos:editorialNote "No occurrences of this slot in the graph." ;
    skos:inScheme okns:ical ;
    skos:mappingRelation ical:dtstart ;
    skos:note "description: default value type: DATE-TIME" ;
    linkml:definition_uri okns:ical_dtstart ;
    linkml:inlined true ;
    linkml:range okns:Any ;
    linkml:slot_uri ical:dtstart .

okns:ical_duration a linkml:SlotDefinition ;
    dcterms:title "DURATION" ;
    skos:definition "The property specifies a positive duration of time." ;
    skos:editorialNote "No occurrences of this slot in the graph." ;
    skos:inScheme okns:ical ;
    skos:mappingRelation ical:duration ;
    skos:note "description: value type: DURATION" ;
    linkml:definition_uri okns:ical_duration ;
    linkml:inlined true ;
    linkml:range okns:IcalValueDURATION ;
    linkml:slot_uri ical:duration .

okns:ical_exrule a linkml:SlotDefinition ;
    dcterms:title "EXRULE" ;
    skos:definition "This property defines a rule or repeating pattern for an exception to a recurrence set." ;
    skos:editorialNote "No occurrences of this slot in the graph." ;
    skos:inScheme okns:ical ;
    skos:mappingRelation ical:exrule ;
    skos:note "description: value type: RECUR" ;
    linkml:definition_uri okns:ical_exrule ;
    linkml:inlined true ;
    linkml:range okns:IcalValueRECUR ;
    linkml:slot_uri ical:exrule .

okns:ical_freebusy a linkml:SlotDefinition ;
    dcterms:title "FREEBUSY" ;
    skos:definition "The property defines one or more free or busy time intervals." ;
    skos:editorialNote "No occurrences of this slot in the graph." ;
    skos:inScheme okns:ical ;
    skos:mappingRelation ical:freebusy ;
    skos:note "description: value type: PERIOD" ;
    linkml:definition_uri okns:ical_freebusy ;
    linkml:inlined true ;
    linkml:range okns:IcalValuePERIOD ;
    linkml:slot_uri ical:freebusy .

okns:ical_geo a linkml:SlotDefinition ;
    dcterms:title "GEO" ;
    skos:definition "This property specifies information related to the global position for the activity specified by a calendar component." ;
    skos:editorialNote "No occurrences of this slot in the graph." ;
    skos:inScheme okns:ical ;
    skos:mappingRelation ical:geo ;
    skos:note "description: value type: list of FLOAT" ;
    linkml:definition_uri okns:ical_geo ;
    linkml:inlined true ;
    linkml:range okns:IcalListOfFloat ;
    linkml:slot_uri ical:geo .

okns:ical_lastModified a linkml:SlotDefinition ;
    dcterms:title "LAST-MODIFIED" ;
    skos:definition "The property specifies the date and time that the information associated with the calendar component was last revised in the calendar store. Note: This is analogous to the modification date and time for a file in the file system." ;
    skos:editorialNote "No occurrences of this slot in the graph." ;
    skos:inScheme okns:ical ;
    skos:mappingRelation ical:lastModified ;
    skos:note "description: value type: DATE-TIME" ;
    linkml:definition_uri okns:ical_lastModified ;
    linkml:inlined true ;
    linkml:range okns:IcalValueDATE-TIME ;
    linkml:slot_uri ical:lastModified .

okns:ical_location a linkml:SlotDefinition ;
    dcterms:title "LOCATION" ;
    skos:definition "The property defines the intended venue for the activity defined by a calendar component." ;
    skos:editorialNote "No occurrences of this slot in the graph." ;
    skos:inScheme okns:ical ;
    skos:mappingRelation ical:location ;
    skos:note "description: value type: TEXT" ;
    linkml:definition_uri okns:ical_location ;
    linkml:range okns:string ;
    linkml:slot_uri ical:location .

okns:ical_method a linkml:SlotDefinition ;
    dcterms:title "METHOD" ;
    skos:definition "This property defines the iCalendar object method associated with the calendar object." ;
    skos:editorialNote "No occurrences of this slot in the graph." ;
    skos:inScheme okns:ical ;
    skos:mappingRelation ical:method ;
    skos:note "description: value type: TEXT" ;
    linkml:definition_uri okns:ical_method ;
    linkml:range okns:string ;
    linkml:slot_uri ical:method .

okns:ical_organizer a linkml:SlotDefinition ;
    dcterms:title "ORGANIZER" ;
    skos:definition "The property defines the organizer for a calendar component." ;
    skos:editorialNote "No occurrences of this slot in the graph." ;
    skos:inScheme okns:ical ;
    skos:mappingRelation ical:organizer ;
    skos:note "description: value type: CAL-ADDRESS" ;
    linkml:definition_uri okns:ical_organizer ;
    linkml:inlined true ;
    linkml:range okns:IcalValueCAL-ADDRESS ;
    linkml:slot_uri ical:organizer .

okns:ical_priority a linkml:SlotDefinition ;
    dcterms:title "PRIORITY" ;
    skos:definition "The property defines the relative priority for a calendar component." ;
    skos:editorialNote "No occurrences of this slot in the graph." ;
    skos:inScheme okns:ical ;
    skos:mappingRelation ical:priority ;
    skos:note "description: value type: INTEGER" ;
    linkml:definition_uri okns:ical_priority ;
    linkml:range okns:integer ;
    linkml:slot_uri ical:priority .

okns:ical_prodid a linkml:SlotDefinition ;
    dcterms:title "PRODID" ;
    skos:definition "This property specifies the identifier for the product that created the iCalendar object." ;
    skos:editorialNote "No occurrences of this slot in the graph." ;
    skos:inScheme okns:ical ;
    skos:mappingRelation ical:prodid ;
    skos:note "description: value type: TEXT" ;
    linkml:definition_uri okns:ical_prodid ;
    linkml:range okns:string ;
    linkml:slot_uri ical:prodid .

okns:ical_rdate a linkml:SlotDefinition ;
    dcterms:title "RDATE" ;
    skos:definition "This property defines the list of date/times for a recurrence set." ;
    skos:editorialNote "No occurrences of this slot in the graph." ;
    skos:inScheme okns:ical ;
    skos:mappingRelation ical:rdate ;
    skos:note "description: default value type: DATE-TIME" ;
    linkml:definition_uri okns:ical_rdate ;
    linkml:inlined true ;
    linkml:range okns:Any ;
    linkml:slot_uri ical:rdate .

okns:ical_relatedTo a linkml:SlotDefinition ;
    dcterms:title "RELATED-TO" ;
    skos:definition "The property is used to represent a relationship or reference between one calendar component and another." ;
    skos:editorialNote "No occurrences of this slot in the graph." ;
    skos:inScheme okns:ical ;
    skos:mappingRelation ical:relatedTo ;
    skos:note "description: value type: TEXT" ;
    linkml:definition_uri okns:ical_relatedTo ;
    linkml:range okns:string ;
    linkml:slot_uri ical:relatedTo .

okns:ical_requestStatus a linkml:SlotDefinition ;
    dcterms:title "REQUEST-STATUS" ;
    skos:definition "This property defines the status code returned for a scheduling request." ;
    skos:editorialNote "No occurrences of this slot in the graph." ;
    skos:inScheme okns:ical ;
    skos:mappingRelation ical:requestStatus ;
    skos:note "description: value type: TEXT" ;
    linkml:definition_uri okns:ical_requestStatus ;
    linkml:range okns:string ;
    linkml:slot_uri ical:requestStatus .

okns:ical_resources a linkml:SlotDefinition ;
    dcterms:title "RESOURCES" ;
    skos:definition "This property defines the equipment or resources anticipated for an activity specified by a calendar entity.." ;
    skos:editorialNote "No occurrences of this slot in the graph." ;
    skos:inScheme okns:ical ;
    skos:mappingRelation ical:resources ;
    skos:note "description: value type: TEXT" ;
    linkml:definition_uri okns:ical_resources ;
    linkml:range okns:string ;
    linkml:slot_uri ical:resources .

okns:ical_rrule a linkml:SlotDefinition ;
    dcterms:title "RRULE" ;
    skos:definition "This property defines a rule or repeating pattern for recurring events, to-dos, or time zone definitions." ;
    skos:editorialNote "No occurrences of this slot in the graph." ;
    skos:inScheme okns:ical ;
    skos:mappingRelation ical:rrule ;
    skos:note "description: value type: RECUR" ;
    linkml:definition_uri okns:ical_rrule ;
    linkml:inlined true ;
    linkml:range okns:IcalValueRECUR ;
    linkml:slot_uri ical:rrule .

okns:ical_sequence a linkml:SlotDefinition ;
    dcterms:title "SEQUENCE" ;
    skos:definition "This property defines the revision sequence number of the calendar component within a sequence of revisions." ;
    skos:editorialNote "No occurrences of this slot in the graph." ;
    skos:inScheme okns:ical ;
    skos:mappingRelation ical:sequence ;
    skos:note "description: value type: integer" ;
    linkml:definition_uri okns:ical_sequence ;
    linkml:range okns:integer ;
    linkml:slot_uri ical:sequence .

okns:ical_status a linkml:SlotDefinition ;
    dcterms:title "STATUS" ;
    skos:definition "This property defines the overall status or confirmation for the calendar component." ;
    skos:editorialNote "No occurrences of this slot in the graph." ;
    skos:inScheme okns:ical ;
    skos:mappingRelation ical:status ;
    skos:note "description: value type: TEXT" ;
    linkml:definition_uri okns:ical_status ;
    linkml:range okns:string ;
    linkml:slot_uri ical:status .

okns:ical_summary a linkml:SlotDefinition ;
    dcterms:title "SUMMARY" ;
    skos:definition "This property defines a short summary or subject for the calendar component." ;
    skos:editorialNote "No occurrences of this slot in the graph." ;
    skos:inScheme okns:ical ;
    skos:mappingRelation ical:summary ;
    skos:note "description: value type: TEXT" ;
    linkml:definition_uri okns:ical_summary ;
    linkml:range okns:string ;
    linkml:slot_uri ical:summary .

okns:ical_trigger a linkml:SlotDefinition ;
    dcterms:title "TRIGGER" ;
    skos:definition "This property specifies when an alarm will trigger." ;
    skos:editorialNote "No occurrences of this slot in the graph." ;
    skos:inScheme okns:ical ;
    skos:mappingRelation ical:trigger ;
    skos:note "description: default value type: DURATION" ;
    linkml:definition_uri okns:ical_trigger ;
    linkml:inlined true ;
    linkml:range okns:Any ;
    linkml:slot_uri ical:trigger .

okns:ical_tzoffsetfrom a linkml:SlotDefinition ;
    dcterms:title "TZOFFSETFROM" ;
    skos:definition "This property specifies the offset which is in use prior to this time zone observance." ;
    skos:editorialNote "No occurrences of this slot in the graph." ;
    skos:inScheme okns:ical ;
    skos:mappingRelation ical:tzoffsetfrom ;
    skos:note "description: value type: UTC-OFFSET" ;
    linkml:definition_uri okns:ical_tzoffsetfrom ;
    linkml:range okns:string ;
    linkml:slot_uri ical:tzoffsetfrom .

okns:ical_tzurl a linkml:SlotDefinition ;
    dcterms:title "TZURL" ;
    skos:definition "The TZURL provides a means for a VTIMEZONE component to point to a network location that can be used to retrieve an up-to- date version of itself." ;
    skos:editorialNote "No occurrences of this slot in the graph." ;
    skos:inScheme okns:ical ;
    skos:mappingRelation ical:tzurl ;
    skos:note "description: value type: URI" ;
    linkml:definition_uri okns:ical_tzurl ;
    linkml:inlined true ;
    linkml:range okns:Any ;
    linkml:slot_uri ical:tzurl .

okns:ical_uid a linkml:SlotDefinition ;
    dcterms:title "UID" ;
    skos:definition "This property defines the persistent, globally unique identifier for the calendar component." ;
    skos:editorialNote "No occurrences of this slot in the graph." ;
    skos:inScheme okns:ical ;
    skos:mappingRelation ical:uid ;
    skos:note "description: value type: TEXT" ;
    linkml:definition_uri okns:ical_uid ;
    linkml:range okns:string ;
    linkml:slot_uri ical:uid .

okns:ical_url a linkml:SlotDefinition ;
    dcterms:title "URL" ;
    skos:definition "This property defines a Uniform Resource Locator (URL) associated with the iCalendar object." ;
    skos:editorialNote "No occurrences of this slot in the graph." ;
    skos:inScheme okns:ical ;
    skos:mappingRelation ical:url ;
    skos:note "description: value type: URI" ;
    linkml:definition_uri okns:ical_url ;
    linkml:inlined true ;
    linkml:range okns:Any ;
    linkml:slot_uri ical:url .

okns:ical_version a linkml:SlotDefinition ;
    dcterms:title "VERSION" ;
    skos:definition "This property specifies the identifier corresponding to the highest version number or the minimum and maximum range of the iCalendar specification that is required in order to interpret the iCalendar object." ;
    skos:editorialNote "No occurrences of this slot in the graph." ;
    skos:inScheme okns:ical ;
    skos:mappingRelation ical:version ;
    skos:note "description: value type: TEXT" ;
    linkml:definition_uri okns:ical_version ;
    linkml:range okns:string ;
    linkml:slot_uri ical:version .

okns:icalspec_valueListType a linkml:SlotDefinition ;
    skos:editorialNote "No occurrences of this slot in the graph." ;
    skos:inScheme okns:ical ;
    skos:mappingRelation icalspec:valueListType ;
    linkml:definition_uri okns:icalspec_valueListType ;
    linkml:inlined true ;
    linkml:range okns:Any ;
    linkml:slot_uri icalspec:valueListType .

okns:icalspec_valueType a linkml:SlotDefinition ;
    skos:editorialNote "No occurrences of this slot in the graph." ;
    skos:inScheme okns:ical ;
    skos:mappingRelation icalspec:valueType ;
    linkml:definition_uri okns:icalspec_valueType ;
    linkml:inlined true ;
    linkml:range okns:Any ;
    linkml:slot_uri icalspec:valueType .

okns:mo_amazon_asin a linkml:SlotDefinition ;
    dcterms:source <http://purl.org/ontology/mo/> ;
    dcterms:title "amazon_asin" ;
    rdfs:subPropertyOf okns:foaf_isPrimaryTopicOf ;
    skos:definition "Used to link a work or the expression of a work to its corresponding Amazon ASINs page." ;
    skos:editorialNote "No occurrences of this slot in the graph." ;
    skos:inScheme okns:mo ;
    skos:mappingRelation <http://purl.org/ontology/mo/amazon_asin> ;
    linkml:definition_uri okns:mo_amazon_asin ;
    linkml:inlined true ;
    linkml:range okns:FoafDocument ;
    linkml:slot_uri <http://purl.org/ontology/mo/amazon_asin> .

okns:mo_availableAs a linkml:SlotDefinition ;
    skos:editorialNote "No occurrences of this slot in the graph." ;
    skos:exactMatch <http://purl.org/ontology/mo/available_as> ;
    skos:inScheme okns:mo ;
    skos:mappingRelation <http://purl.org/ontology/mo/availableAs> ;
    linkml:definition_uri okns:mo_availableAs ;
    linkml:inlined true ;
    linkml:range okns:Any ;
    linkml:slot_uri <http://purl.org/ontology/mo/availableAs> .

okns:mo_bpm a linkml:SlotDefinition ;
    dcterms:source <http://purl.org/ontology/mo/> ;
    dcterms:title "bpm" ;
    skos:definition "Indicates the BPM of a MusicalWork or a particular Performance ␊        Beats per minute: the pace of music measured by the number of beats occurring in 60 seconds." ;
    skos:editorialNote "No occurrences of this slot in the graph." ;
    skos:inScheme okns:mo ;
    skos:mappingRelation <http://purl.org/ontology/mo/bpm> ;
    linkml:definition_uri okns:mo_bpm ;
    linkml:range okns:float ;
    linkml:slot_uri <http://purl.org/ontology/mo/bpm> .

okns:mo_contains_sample_from a linkml:SlotDefinition ;
    dcterms:source <http://purl.org/ontology/mo/> ;
    dcterms:title "contains_sample_from" ;
    rdfs:subPropertyOf okns:mo_derived_from ;
    skos:definition "Relates a signal to another signal, which has been sampled." ;
    skos:editorialNote "No occurrences of this slot in the graph." ;
    skos:inScheme okns:mo ;
    skos:mappingRelation <http://purl.org/ontology/mo/contains_sample_from> ;
    linkml:definition_uri okns:mo_contains_sample_from ;
    linkml:inlined true ;
    linkml:range okns:Any ;
    linkml:slot_uri <http://purl.org/ontology/mo/contains_sample_from> .

okns:mo_discogs a linkml:SlotDefinition ;
    dcterms:source <http://purl.org/ontology/mo/> ;
    dcterms:title "discogs" ;
    rdfs:subPropertyOf okns:foaf_isPrimaryTopicOf ;
    skos:definition "Used to link a musical work or the expression of a musical work, an artist or a corporate body to to its corresponding Discogs page." ;
    skos:editorialNote "No occurrences of this slot in the graph." ;
    skos:inScheme okns:mo ;
    skos:mappingRelation <http://purl.org/ontology/mo/discogs> ;
    linkml:definition_uri okns:mo_discogs ;
    linkml:inlined true ;
    linkml:range okns:FoafDocument ;
    linkml:slot_uri <http://purl.org/ontology/mo/discogs> .

okns:mo_djmix_of a linkml:SlotDefinition ;
    dcterms:source <http://purl.org/ontology/mo/> ;
    dcterms:title "djmix_of" ;
    rdfs:subPropertyOf okns:mo_derived_from ;
    skos:definition "Indicates that all (or most of) the tracks of a musical work or the expression of a musical work were mixed together from all (or most of) the tracks from another musical work or the expression of a musical work to form a so called DJ-Mix. ␊    ␊The tracks might have been altered by pitching (so that the tempo of one track matches the tempo of the following track) and fading (so that one track blends in smoothly with the other). If the tracks have been more substantially altered, the \"mo:remix\" relationship type is more appropriate." ;
    skos:editorialNote "No occurrences of this slot in the graph." ;
    skos:inScheme okns:mo ;
    skos:mappingRelation <http://purl.org/ontology/mo/djmix_of> ;
    linkml:definition_uri okns:mo_djmix_of ;
    linkml:inlined true ;
    linkml:range okns:Any ;
    linkml:slot_uri <http://purl.org/ontology/mo/djmix_of> .

okns:mo_duration a linkml:SlotDefinition ;
    dcterms:source <http://purl.org/ontology/mo/> ;
    skos:definition "The duration of a track or a signal in ms" ;
    skos:editorialNote "No occurrences of this slot in the graph." ;
    skos:inScheme okns:mo ;
    skos:mappingRelation <http://purl.org/ontology/mo/duration> ;
    linkml:definition_uri okns:mo_duration ;
    linkml:range okns:float ;
    linkml:slot_uri <http://purl.org/ontology/mo/duration> .

okns:mo_eventHomePage a linkml:SlotDefinition ;
    skos:editorialNote "No occurrences of this slot in the graph." ;
    skos:exactMatch <http://purl.org/ontology/mo/event_homepage> ;
    skos:inScheme okns:mo ;
    skos:mappingRelation <http://purl.org/ontology/mo/eventHomePage> ;
    linkml:definition_uri okns:mo_eventHomePage ;
    linkml:inlined true ;
    linkml:range okns:Any ;
    linkml:slot_uri <http://purl.org/ontology/mo/eventHomePage> .

okns:mo_free_download a linkml:SlotDefinition ;
    dcterms:source <http://purl.org/ontology/mo/> ;
    dcterms:title "free download" ;
    rdfs:subPropertyOf okns:foaf_isPrimaryTopicOf ;
    skos:definition "This property can be used to link from a person to the website where they make their works available, or from␊        a manifestation (a track or an album, for example) to a web page where it is available for free ␊        download.␊␊        This property MUST be used only if the content is just available through a web page (holding, for example␊        a Flash application) - it is better to link to actual content directly through the use of mo:available_as and ␊        mo:Stream, mo:Torrent or mo:ED2K, etc. Therefore, Semantic Web user agents that don't know how to read HTML and even␊        less to rip streams from Flash applications can still access the audio content." ;
    skos:editorialNote "No occurrences of this slot in the graph." ;
    skos:inScheme okns:mo ;
    skos:mappingRelation <http://purl.org/ontology/mo/free_download> ;
    linkml:definition_uri okns:mo_free_download ;
    linkml:inlined true ;
    linkml:range okns:FoafDocument ;
    linkml:slot_uri <http://purl.org/ontology/mo/free_download> .

okns:mo_freedownload a linkml:SlotDefinition ;
    dcterms:source <http://purl.org/ontology/mo/> ;
    skos:editorialNote "No occurrences of this slot in the graph." ;
    skos:exactMatch <http://purl.org/ontology/mo/free_download> ;
    skos:inScheme okns:mo ;
    skos:mappingRelation <http://purl.org/ontology/mo/freedownload> ;
    linkml:definition_uri okns:mo_freedownload ;
    linkml:inlined true ;
    linkml:range okns:Any ;
    linkml:slot_uri <http://purl.org/ontology/mo/freedownload> .

okns:mo_genre a linkml:SlotDefinition ;
    dcterms:source <http://purl.org/ontology/mo/> ;
    dcterms:title "genre" ;
    rdfs:subPropertyOf okns:ao_genre ;
    skos:definition "Associates an event (like a performance or a recording) to a particular musical genre.␊        Further version of this property may also include works and scores in the domain." ;
    skos:editorialNote "No occurrences of this slot in the graph." ;
    skos:inScheme okns:mo ;
    skos:mappingRelation <http://purl.org/ontology/mo/genre> ;
    linkml:definition_uri okns:mo_genre ;
    linkml:inlined true ;
    linkml:range okns:MoGenre ;
    linkml:slot_uri <http://purl.org/ontology/mo/genre> .

okns:mo_has_track a linkml:SlotDefinition ;
    dcterms:source <http://purl.org/ontology/mo/> ;
    skos:editorialNote "No occurrences of this slot in the graph." ;
    skos:exactMatch <http://purl.org/ontology/mo/track> ;
    skos:inScheme okns:mo ;
    skos:mappingRelation <http://purl.org/ontology/mo/has_track> ;
    linkml:definition_uri okns:mo_has_track ;
    linkml:inlined true ;
    linkml:range okns:Any ;
    linkml:slot_uri <http://purl.org/ontology/mo/has_track> .

okns:mo_headliner a linkml:SlotDefinition ;
    dcterms:source <http://purl.org/ontology/mo/> ;
    dcterms:title "headliner" ;
    rdfs:subPropertyOf okns:mo_performer ;
    skos:definition "Relates a performance to the headliner(s) involved" ;
    skos:editorialNote "No occurrences of this slot in the graph." ;
    skos:inScheme okns:mo ;
    skos:mappingRelation <http://purl.org/ontology/mo/headliner> ;
    linkml:definition_uri okns:mo_headliner ;
    linkml:inlined true ;
    linkml:range okns:Any ;
    linkml:slot_uri <http://purl.org/ontology/mo/headliner> .

okns:mo_homepage a linkml:SlotDefinition ;
    dcterms:source <http://purl.org/ontology/mo/> ;
    dcterms:title "homepage" ;
    rdfs:subPropertyOf okns:foaf_isPrimaryTopicOf ;
    skos:definition "Links an artist, a record, etc. to a corresponding web page" ;
    skos:editorialNote "No occurrences of this slot in the graph." ;
    skos:inScheme okns:mo ;
    skos:mappingRelation <http://purl.org/ontology/mo/homepage> ;
    linkml:definition_uri okns:mo_homepage ;
    linkml:inlined true ;
    linkml:range okns:FoafDocument ;
    linkml:slot_uri <http://purl.org/ontology/mo/homepage> .

okns:mo_image a linkml:SlotDefinition ;
    dcterms:source <http://purl.org/ontology/mo/> ;
    dcterms:title "image" ;
    rdfs:subPropertyOf okns:foaf_depiction ;
    skos:definition "Indicates a pictorial image (JPEG, GIF, PNG, Etc.) of a musical work, the expression of a musical work, the manifestation of a work or the examplar of a manifestation." ;
    skos:editorialNote "No occurrences of this slot in the graph." ;
    skos:inScheme okns:mo ;
    skos:mappingRelation <http://purl.org/ontology/mo/image> ;
    linkml:definition_uri okns:mo_image ;
    linkml:inlined true ;
    linkml:range okns:FoafImage ;
    linkml:slot_uri <http://purl.org/ontology/mo/image> .

okns:mo_imdb a linkml:SlotDefinition ;
    dcterms:source <http://purl.org/ontology/mo/> ;
    dcterms:title "imdb" ;
    rdfs:subPropertyOf okns:foaf_isPrimaryTopicOf ;
    skos:definition "Used to link an artist, a musical work or the expression of a musical work to their equivalent page on IMDb, the InternetMovieDatabase." ;
    skos:editorialNote "No occurrences of this slot in the graph." ;
    skos:inScheme okns:mo ;
    skos:mappingRelation <http://purl.org/ontology/mo/imdb> ;
    linkml:definition_uri okns:mo_imdb ;
    linkml:inlined true ;
    linkml:range okns:FoafDocument ;
    linkml:slot_uri <http://purl.org/ontology/mo/imdb> .

okns:mo_ismn a linkml:SlotDefinition ;
    dcterms:source <http://purl.org/ontology/mo/> ;
    dcterms:title "ismn" ;
    rdfs:subPropertyOf okns:mo_uuid ;
    skos:definition "The International Standard Music Number (ISMN) is an ISO standard similar to ISBNs for identifying printed music publications" ;
    skos:editorialNote "No occurrences of this slot in the graph." ;
    skos:inScheme okns:mo ;
    skos:mappingRelation <http://purl.org/ontology/mo/ismn> ;
    linkml:definition_uri okns:mo_ismn ;
    linkml:range okns:string ;
    linkml:slot_uri <http://purl.org/ontology/mo/ismn> .

okns:mo_key a linkml:SlotDefinition ;
    dcterms:source <http://purl.org/ontology/mo/> ;
    dcterms:title "key" ;
    skos:definition "Indicated the key used by the musicians during a performance, or the key of a MusicalWork.␊        Any of 24 major or minor diatonic scales that provide the tonal framework for a piece of music." ;
    skos:editorialNote "No occurrences of this slot in the graph." ;
    skos:inScheme okns:mo ;
    skos:mappingRelation <http://purl.org/ontology/mo/key> ;
    linkml:definition_uri okns:mo_key ;
    linkml:inlined true ;
    linkml:range <https://purl.org/okn/schema/HttpPurl.orgNETC4dmKeys.owl#Key> ;
    linkml:slot_uri <http://purl.org/ontology/mo/key> .

okns:mo_label a linkml:SlotDefinition ;
    dcterms:source <http://purl.org/ontology/mo/> ;
    dcterms:title "label" ;
    skos:definition "Associates a release event with the label releasing the record" ;
    skos:editorialNote "No occurrences of this slot in the graph." ;
    skos:inScheme okns:mo ;
    skos:mappingRelation <http://purl.org/ontology/mo/label> ;
    linkml:definition_uri okns:mo_label ;
    linkml:inlined true ;
    linkml:range okns:MoLabel ;
    linkml:slot_uri <http://purl.org/ontology/mo/label> .

okns:mo_licence a linkml:SlotDefinition ;
    dcterms:source <http://purl.org/ontology/mo/> ;
    dcterms:title "licence" ;
    skos:definition "Used to link a work or the expression of a work to the license under which they can be manipulated (downloaded, modified, etc). ␊    ␊This is usually used to link to a Creative Commons licence." ;
    skos:editorialNote "No occurrences of this slot in the graph." ;
    skos:inScheme okns:mo ;
    skos:mappingRelation <http://purl.org/ontology/mo/licence> ;
    linkml:definition_uri okns:mo_licence ;
    linkml:inlined true ;
    linkml:range okns:CcLicense ;
    linkml:slot_uri <http://purl.org/ontology/mo/licence> .

okns:mo_mailorder a linkml:SlotDefinition ;
    dcterms:source <http://purl.org/ontology/mo/> ;
    dcterms:title "mailorder" ;
    rdfs:subPropertyOf okns:foaf_isPrimaryTopicOf ;
    skos:definition "Used to link a musical work or the expression of a musical work to a website where people can buy a copy of the musical manifestation." ;
    skos:editorialNote "No occurrences of this slot in the graph." ;
    skos:inScheme okns:mo ;
    skos:mappingRelation <http://purl.org/ontology/mo/mailorder> ;
    linkml:definition_uri okns:mo_mailorder ;
    linkml:inlined true ;
    linkml:range okns:FoafDocument ;
    linkml:slot_uri <http://purl.org/ontology/mo/mailorder> .

okns:mo_mashup_of a linkml:SlotDefinition ;
    dcterms:source <http://purl.org/ontology/mo/> ;
    dcterms:title "mashup_of" ;
    rdfs:subPropertyOf okns:mo_derived_from ;
    skos:definition "Indicates that musical works or the expressions of a musical work were mashed up on this album or track. ␊    ␊This means that two musical works or the expressions of a musical work by different artists are mixed together, over each other, or otherwise combined into a single musical work (usually by a third artist, the remixer)." ;
    skos:editorialNote "No occurrences of this slot in the graph." ;
    skos:inScheme okns:mo ;
    skos:mappingRelation <http://purl.org/ontology/mo/mashup_of> ;
    linkml:definition_uri okns:mo_mashup_of ;
    linkml:inlined true ;
    linkml:range okns:Any ;
    linkml:slot_uri <http://purl.org/ontology/mo/mashup_of> .

okns:mo_medley_of a linkml:SlotDefinition ;
    dcterms:source <http://purl.org/ontology/mo/> ;
    dcterms:title "medley_of" ;
    rdfs:subPropertyOf okns:mo_derived_from ;
    skos:definition "Indicates that a musical expression is a medley of several other musical expressions. ␊    ␊This means that the orignial musical expression were rearranged to create a new musical expression in the form of a medley." ;
    skos:editorialNote "No occurrences of this slot in the graph." ;
    skos:inScheme okns:mo ;
    skos:mappingRelation <http://purl.org/ontology/mo/medley_of> ;
    linkml:definition_uri okns:mo_medley_of ;
    linkml:inlined true ;
    linkml:range okns:Any ;
    linkml:slot_uri <http://purl.org/ontology/mo/medley_of> .

okns:mo_meter a linkml:SlotDefinition ;
    dcterms:source <http://purl.org/ontology/mo/> ;
    dcterms:title "meter" ;
    skos:definition "Associates a musical work or a score with its meter" ;
    skos:editorialNote "No occurrences of this slot in the graph." ;
    skos:inScheme okns:mo ;
    skos:mappingRelation <http://purl.org/ontology/mo/meter> ;
    linkml:definition_uri okns:mo_meter ;
    linkml:inlined true ;
    linkml:range okns:Any ;
    linkml:slot_uri <http://purl.org/ontology/mo/meter> .

okns:mo_movementNum a linkml:SlotDefinition ;
    skos:editorialNote "No occurrences of this slot in the graph." ;
    skos:exactMatch <http://purl.org/ontology/mo/movement_number> ;
    skos:inScheme okns:mo ;
    skos:mappingRelation <http://purl.org/ontology/mo/movementNum> ;
    linkml:definition_uri okns:mo_movementNum ;
    linkml:inlined true ;
    linkml:range okns:Any ;
    linkml:slot_uri <http://purl.org/ontology/mo/movementNum> .

okns:mo_musicbrainz a linkml:SlotDefinition ;
    dcterms:source <http://purl.org/ontology/mo/> ;
    dcterms:title "musicbrainz" ;
    rdfs:subPropertyOf okns:foaf_isPrimaryTopicOf ;
    skos:definition "Linking an agent, a track or a record to its corresponding Musicbrainz page." ;
    skos:editorialNote "No occurrences of this slot in the graph." ;
    skos:inScheme okns:mo ;
    skos:mappingRelation <http://purl.org/ontology/mo/musicbrainz> ;
    linkml:definition_uri okns:mo_musicbrainz ;
    linkml:inlined true ;
    linkml:range okns:FoafDocument ;
    linkml:slot_uri <http://purl.org/ontology/mo/musicbrainz> .

okns:mo_musicbrainz_guid a linkml:SlotDefinition ;
    dcterms:source <http://purl.org/ontology/mo/> ;
    dcterms:title "Musicbrainz GUID" ;
    rdfs:subPropertyOf okns:mo_uuid ;
    skos:definition "Links an object to the corresponding Musicbrainz identifier" ;
    skos:editorialNote "No occurrences of this slot in the graph." ;
    skos:inScheme okns:mo ;
    skos:mappingRelation <http://purl.org/ontology/mo/musicbrainz_guid> ;
    linkml:definition_uri okns:mo_musicbrainz_guid ;
    linkml:inlined true ;
    linkml:range okns:Any ;
    linkml:slot_uri <http://purl.org/ontology/mo/musicbrainz_guid> .

okns:mo_musicmoz a linkml:SlotDefinition ;
    dcterms:source <http://purl.org/ontology/mo/> ;
    dcterms:title "musicmoz" ;
    rdfs:subPropertyOf okns:foaf_isPrimaryTopicOf ;
    skos:definition "Used to link an artist, a musical work or the expression of a musical work to its corresponding MusicMoz page." ;
    skos:editorialNote "No occurrences of this slot in the graph." ;
    skos:inScheme okns:mo ;
    skos:mappingRelation <http://purl.org/ontology/mo/musicmoz> ;
    linkml:definition_uri okns:mo_musicmoz ;
    linkml:inlined true ;
    linkml:range okns:FoafDocument ;
    linkml:slot_uri <http://purl.org/ontology/mo/musicmoz> .

okns:mo_paid_download a linkml:SlotDefinition ;
    dcterms:source <http://purl.org/ontology/mo/> ;
    dcterms:title "paid download" ;
    rdfs:subPropertyOf okns:foaf_isPrimaryTopicOf ;
    skos:definition "Provide a link from an artist to a web page where all of that artist's musical work is available for some money,␊                or a link from a manifestation (record/track, for example) to a web page providing a paid access to this manifestation." ;
    skos:editorialNote "No occurrences of this slot in the graph." ;
    skos:inScheme okns:mo ;
    skos:mappingRelation <http://purl.org/ontology/mo/paid_download> ;
    linkml:definition_uri okns:mo_paid_download ;
    linkml:inlined true ;
    linkml:range okns:FoafDocument ;
    linkml:slot_uri <http://purl.org/ontology/mo/paid_download> .

okns:mo_paiddownload a linkml:SlotDefinition ;
    dcterms:source <http://purl.org/ontology/mo/> ;
    skos:editorialNote "No occurrences of this slot in the graph." ;
    skos:exactMatch <http://purl.org/ontology/mo/paid_download> ;
    skos:inScheme okns:mo ;
    skos:mappingRelation <http://purl.org/ontology/mo/paiddownload> ;
    linkml:definition_uri okns:mo_paiddownload ;
    linkml:inlined true ;
    linkml:range okns:Any ;
    linkml:slot_uri <http://purl.org/ontology/mo/paiddownload> .

okns:mo_preview_download a linkml:SlotDefinition ;
    dcterms:source <http://purl.org/ontology/mo/> ;
    dcterms:title "preview download" ;
    rdfs:subPropertyOf okns:mo_download ;
    skos:definition "This property can be used to link from a person to the website where they make previews of their works available, or from␊                a manifestation (a track or an album, for example) to a web page where a preview download is available.␊␊                This property MUST be used only if the content is just available through a web page (holding, for example␊                a Flash application) - it is better to link to actual content directly through the use of mo:available_as and␊                mo:Stream, mo:Torrent or mo:ED2K, etc. Therefore, Semantic Web user agents that don't know how to read HTML and even␊                less to rip streams from Flash applications can still access the audio content." ;
    skos:editorialNote "No occurrences of this slot in the graph." ;
    skos:inScheme okns:mo ;
    skos:mappingRelation <http://purl.org/ontology/mo/preview_download> ;
    linkml:definition_uri okns:mo_preview_download ;
    linkml:inlined true ;
    linkml:range okns:FoafDocument ;
    linkml:slot_uri <http://purl.org/ontology/mo/preview_download> .

okns:mo_primary_instrument a linkml:SlotDefinition ;
    dcterms:source <http://purl.org/ontology/mo/> ;
    dcterms:title "primary instrument" ;
    skos:definition "Indicates that an artist primarily plays an instrument, or that a member was primarily playing a particular instrument during his membership" ;
    skos:editorialNote "No occurrences of this slot in the graph." ;
    skos:inScheme okns:mo ;
    skos:mappingRelation <http://purl.org/ontology/mo/primary_instrument> ;
    linkml:definition_uri okns:mo_primary_instrument ;
    linkml:inlined true ;
    linkml:range okns:MoInstrument ;
    linkml:slot_uri <http://purl.org/ontology/mo/primary_instrument> .

okns:mo_produced_score a linkml:SlotDefinition ;
    dcterms:source <http://purl.org/ontology/mo/> ;
    dcterms:title "produced score" ;
    rdfs:subPropertyOf okns:event_product ;
    skos:definition "Associates an arrangement or a composition event to a score product (score here does not refer to a published score, but more␊        an abstract arrangement of a particular work)." ;
    skos:editorialNote "No occurrences of this slot in the graph." ;
    skos:inScheme okns:mo ;
    skos:mappingRelation <http://purl.org/ontology/mo/produced_score> ;
    linkml:definition_uri okns:mo_produced_score ;
    linkml:inlined true ;
    linkml:range okns:MoScore ;
    linkml:slot_uri <http://purl.org/ontology/mo/produced_score> .

okns:mo_producesSignal a linkml:SlotDefinition ;
    dcterms:source <http://purl.org/ontology/mo/> ;
    skos:editorialNote "No occurrences of this slot in the graph." ;
    skos:exactMatch <http://purl.org/ontology/mo/produced_signal> ;
    skos:inScheme okns:mo ;
    skos:mappingRelation <http://purl.org/ontology/mo/producesSignal> ;
    linkml:definition_uri okns:mo_producesSignal ;
    linkml:inlined true ;
    linkml:range okns:Any ;
    linkml:slot_uri <http://purl.org/ontology/mo/producesSignal> .

okns:mo_producesSound a linkml:SlotDefinition ;
    dcterms:source <http://purl.org/ontology/mo/> ;
    skos:editorialNote "No occurrences of this slot in the graph." ;
    skos:exactMatch <http://purl.org/ontology/mo/produced_sound> ;
    skos:inScheme okns:mo ;
    skos:mappingRelation <http://purl.org/ontology/mo/producesSound> ;
    linkml:definition_uri okns:mo_producesSound ;
    linkml:inlined true ;
    linkml:range okns:Any ;
    linkml:slot_uri <http://purl.org/ontology/mo/producesSound> .

okns:mo_producesWork a linkml:SlotDefinition ;
    skos:editorialNote "No occurrences of this slot in the graph." ;
    skos:exactMatch <http://purl.org/ontology/mo/produced_work> ;
    skos:inScheme okns:mo ;
    skos:mappingRelation <http://purl.org/ontology/mo/producesWork> ;
    linkml:definition_uri okns:mo_producesWork ;
    linkml:inlined true ;
    linkml:range okns:Any ;
    linkml:slot_uri <http://purl.org/ontology/mo/producesWork> .

okns:mo_productOfComposition a linkml:SlotDefinition ;
    dcterms:source <http://purl.org/ontology/mo/> ;
    skos:editorialNote "No occurrences of this slot in the graph." ;
    skos:exactMatch <http://purl.org/ontology/mo/composed_in> ;
    skos:inScheme okns:mo ;
    skos:mappingRelation <http://purl.org/ontology/mo/productOfComposition> ;
    linkml:definition_uri okns:mo_productOfComposition ;
    linkml:inlined true ;
    linkml:range okns:Any ;
    linkml:slot_uri <http://purl.org/ontology/mo/productOfComposition> .

okns:mo_publicationOf a linkml:SlotDefinition ;
    skos:editorialNote "No occurrences of this slot in the graph." ;
    skos:exactMatch <http://purl.org/ontology/mo/publication_of> ;
    skos:inScheme okns:mo ;
    skos:mappingRelation <http://purl.org/ontology/mo/publicationOf> ;
    linkml:definition_uri okns:mo_publicationOf ;
    linkml:inlined true ;
    linkml:range okns:Any ;
    linkml:slot_uri <http://purl.org/ontology/mo/publicationOf> .

okns:mo_publishedAs a linkml:SlotDefinition ;
    skos:editorialNote "No occurrences of this slot in the graph." ;
    skos:exactMatch <http://purl.org/ontology/mo/published_as> ;
    skos:inScheme okns:mo ;
    skos:mappingRelation <http://purl.org/ontology/mo/publishedAs> ;
    linkml:definition_uri okns:mo_publishedAs ;
    linkml:inlined true ;
    linkml:range okns:Any ;
    linkml:slot_uri <http://purl.org/ontology/mo/publishedAs> .

okns:mo_publishingLocation a linkml:SlotDefinition ;
    skos:editorialNote "No occurrences of this slot in the graph." ;
    skos:exactMatch <http://purl.org/ontology/mo/publishing_location> ;
    skos:inScheme okns:mo ;
    skos:mappingRelation <http://purl.org/ontology/mo/publishingLocation> ;
    linkml:definition_uri okns:mo_publishingLocation ;
    linkml:inlined true ;
    linkml:range okns:Any ;
    linkml:slot_uri <http://purl.org/ontology/mo/publishingLocation> .

okns:mo_releaseStatus a linkml:SlotDefinition ;
    skos:editorialNote "No occurrences of this slot in the graph." ;
    skos:exactMatch <http://purl.org/ontology/mo/release_status> ;
    skos:inScheme okns:mo ;
    skos:mappingRelation <http://purl.org/ontology/mo/releaseStatus> ;
    linkml:definition_uri okns:mo_releaseStatus ;
    linkml:inlined true ;
    linkml:range okns:Any ;
    linkml:slot_uri <http://purl.org/ontology/mo/releaseStatus> .

okns:mo_releaseType a linkml:SlotDefinition ;
    skos:editorialNote "No occurrences of this slot in the graph." ;
    skos:exactMatch <http://purl.org/ontology/mo/release_type> ;
    skos:inScheme okns:mo ;
    skos:mappingRelation <http://purl.org/ontology/mo/releaseType> ;
    linkml:definition_uri okns:mo_releaseType ;
    linkml:inlined true ;
    linkml:range okns:Any ;
    linkml:slot_uri <http://purl.org/ontology/mo/releaseType> .

okns:mo_remaster_of a linkml:SlotDefinition ;
    dcterms:source <http://purl.org/ontology/mo/> ;
    dcterms:title "remaster_of" ;
    rdfs:subPropertyOf okns:mo_derived_from ;
    skos:definition "This relates two musical work or the expression of a musical work, where one is a remaster of the other. ␊    ␊A remaster is a new version made for release from source recordings that were earlier released separately. This is usually done to improve the audio quality or adjust for more modern playback equipment. The process generally doesn't involve changing the music in any artistically important way. It may, however, result in tracks that are a few seconds longer or shorter." ;
    skos:editorialNote "No occurrences of this slot in the graph." ;
    skos:inScheme okns:mo ;
    skos:mappingRelation <http://purl.org/ontology/mo/remaster_of> ;
    linkml:definition_uri okns:mo_remaster_of ;
    linkml:inlined true ;
    linkml:range okns:Any ;
    linkml:slot_uri <http://purl.org/ontology/mo/remaster_of> .

okns:mo_remix_of a linkml:SlotDefinition ;
    dcterms:source <http://purl.org/ontology/mo/> ;
    dcterms:title "remix_of" ;
    rdfs:subPropertyOf okns:mo_derived_from ;
    skos:definition "Used to relate the remix of a musical work in a substantially altered version produced by mixing together individual tracks or segments of an original musical source work." ;
    skos:editorialNote "No occurrences of this slot in the graph." ;
    skos:inScheme okns:mo ;
    skos:mappingRelation <http://purl.org/ontology/mo/remix_of> ;
    linkml:definition_uri okns:mo_remix_of ;
    linkml:inlined true ;
    linkml:range okns:Any ;
    linkml:slot_uri <http://purl.org/ontology/mo/remix_of> .

okns:mo_review a linkml:SlotDefinition ;
    dcterms:source <http://purl.org/ontology/mo/> ;
    dcterms:title "review" ;
    rdfs:subPropertyOf okns:foaf_isPrimaryTopicOf ;
    skos:definition "Used to link a work or the expression of a work to a review. ␊    ␊The review does not have to be open content, as long as it is accessible to the general internet population." ;
    skos:editorialNote "No occurrences of this slot in the graph." ;
    skos:inScheme okns:mo ;
    skos:mappingRelation <http://purl.org/ontology/mo/review> ;
    linkml:definition_uri okns:mo_review ;
    linkml:inlined true ;
    linkml:range okns:FoafDocument ;
    linkml:slot_uri <http://purl.org/ontology/mo/review> .

okns:mo_sampleRate a linkml:SlotDefinition ;
    skos:editorialNote "No occurrences of this slot in the graph." ;
    skos:exactMatch <http://purl.org/ontology/mo/sample_rate> ;
    skos:inScheme okns:mo ;
    skos:mappingRelation <http://purl.org/ontology/mo/sampleRate> ;
    linkml:definition_uri okns:mo_sampleRate ;
    linkml:inlined true ;
    linkml:range okns:Any ;
    linkml:slot_uri <http://purl.org/ontology/mo/sampleRate> .

okns:mo_sampledVersionOf a linkml:SlotDefinition ;
    dcterms:source <http://purl.org/ontology/mo/> ;
    skos:editorialNote "No occurrences of this slot in the graph." ;
    skos:exactMatch <http://purl.org/ontology/mo/sampled_version_of> ;
    skos:inScheme okns:mo ;
    skos:mappingRelation <http://purl.org/ontology/mo/sampledVersionOf> ;
    linkml:definition_uri okns:mo_sampledVersionOf ;
    linkml:inlined true ;
    linkml:range okns:Any ;
    linkml:slot_uri <http://purl.org/ontology/mo/sampledVersionOf> .

okns:mo_signalTime a linkml:SlotDefinition ;
    dcterms:source <http://purl.org/ontology/mo/> ;
    skos:editorialNote "No occurrences of this slot in the graph." ;
    skos:exactMatch <http://purl.org/ontology/mo/time> ;
    skos:inScheme okns:mo ;
    skos:mappingRelation <http://purl.org/ontology/mo/signalTime> ;
    linkml:definition_uri okns:mo_signalTime ;
    linkml:inlined true ;
    linkml:range okns:Any ;
    linkml:slot_uri <http://purl.org/ontology/mo/signalTime> .

okns:mo_similar_to a linkml:SlotDefinition ;
    dcterms:source <http://purl.org/ontology/mo/> ;
    dcterms:title "similar_to" ;
    skos:definition "A similarity relationships between two objects (so far, either an agent, a signal or a genre, but␊        this could grow).␊        This relationship is pretty general and doesn't make any assumptions on how the similarity claim␊        was derived.␊        Such similarity statements can come from a range of different sources (Musicbrainz similarities between␊        artists, or coming from some automatic content analysis).␊        However, the origin of such statements should be kept using a named graph approach - and ultimately, the ␊        documents providing such statements should attach some metadata to themselves (confidence of the claim, etc.)." ;
    skos:editorialNote "No occurrences of this slot in the graph." ;
    skos:inScheme okns:mo ;
    skos:mappingRelation <http://purl.org/ontology/mo/similar_to> ;
    linkml:definition_uri okns:mo_similar_to ;
    linkml:inlined true ;
    linkml:range okns:Any ;
    linkml:slot_uri <http://purl.org/ontology/mo/similar_to> .

okns:mo_tempo a linkml:SlotDefinition ;
    dcterms:source <http://purl.org/ontology/mo/> ;
    dcterms:title "tempo" ;
    skos:definition "Rate of speed or pace of music. Tempo markings are traditionally given in Italian; ␊        common markings include: grave (solemn; very, very slow); largo (broad; very slow); ␊        adagio (quite slow); andante (a walking pace); moderato (moderate); allegro (fast; cheerful); ␊        vivace (lively); presto (very fast); accelerando (getting faster); ritardando (getting slower); ␊        and a tempo (in time; returning to the original pace)." ;
    skos:editorialNote "No occurrences of this slot in the graph." ;
    skos:inScheme okns:mo ;
    skos:mappingRelation <http://purl.org/ontology/mo/tempo> ;
    linkml:definition_uri okns:mo_tempo ;
    linkml:range okns:string ;
    linkml:slot_uri <http://purl.org/ontology/mo/tempo> .

okns:mo_trackNum a linkml:SlotDefinition ;
    dcterms:source <http://purl.org/ontology/mo/> ;
    skos:editorialNote "No occurrences of this slot in the graph." ;
    skos:exactMatch <http://purl.org/ontology/mo/track_number> ;
    skos:inScheme okns:mo ;
    skos:mappingRelation <http://purl.org/ontology/mo/trackNum> ;
    linkml:definition_uri okns:mo_trackNum ;
    linkml:inlined true ;
    linkml:range okns:Any ;
    linkml:slot_uri <http://purl.org/ontology/mo/trackNum> .

okns:mo_usedInPerformance a linkml:SlotDefinition ;
    dcterms:source <http://purl.org/ontology/mo/> ;
    skos:editorialNote "No occurrences of this slot in the graph." ;
    skos:exactMatch <http://purl.org/ontology/mo/performed_in> ;
    skos:inScheme okns:mo ;
    skos:mappingRelation <http://purl.org/ontology/mo/usedInPerformance> ;
    linkml:definition_uri okns:mo_usedInPerformance ;
    linkml:inlined true ;
    linkml:range okns:Any ;
    linkml:slot_uri <http://purl.org/ontology/mo/usedInPerformance> .

okns:mo_usedInRecording a linkml:SlotDefinition ;
    dcterms:source <http://purl.org/ontology/mo/> ;
    skos:editorialNote "No occurrences of this slot in the graph." ;
    skos:exactMatch <http://purl.org/ontology/mo/recorded_in> ;
    skos:inScheme okns:mo ;
    skos:mappingRelation <http://purl.org/ontology/mo/usedInRecording> ;
    linkml:definition_uri okns:mo_usedInRecording ;
    linkml:inlined true ;
    linkml:range okns:Any ;
    linkml:slot_uri <http://purl.org/ontology/mo/usedInRecording> .

okns:mo_usesSound a linkml:SlotDefinition ;
    dcterms:source <http://purl.org/ontology/mo/> ;
    skos:editorialNote "No occurrences of this slot in the graph." ;
    skos:exactMatch <http://purl.org/ontology/mo/recording_of> ;
    skos:inScheme okns:mo ;
    skos:mappingRelation <http://purl.org/ontology/mo/usesSound> ;
    linkml:definition_uri okns:mo_usesSound ;
    linkml:inlined true ;
    linkml:range okns:Any ;
    linkml:slot_uri <http://purl.org/ontology/mo/usesSound> .

okns:mo_usesWork a linkml:SlotDefinition ;
    dcterms:source <http://purl.org/ontology/mo/> ;
    skos:editorialNote "No occurrences of this slot in the graph." ;
    skos:exactMatch <http://purl.org/ontology/mo/performance_of> ;
    skos:inScheme okns:mo ;
    skos:mappingRelation <http://purl.org/ontology/mo/usesWork> ;
    linkml:definition_uri okns:mo_usesWork ;
    linkml:inlined true ;
    linkml:range okns:Any ;
    linkml:slot_uri <http://purl.org/ontology/mo/usesWork> .

okns:mo_wikipedia a linkml:SlotDefinition ;
    dcterms:source <http://purl.org/ontology/mo/> ;
    dcterms:title "wikipedia" ;
    rdfs:subPropertyOf okns:foaf_isPrimaryTopicOf ;
    skos:definition "Used to link an work, an expression of a work, a manifestation of a work, ␊        a person, an instrument or a musical genre to its corresponding WikiPedia page. ␊        The full URL should be used, not just the WikiName." ;
    skos:editorialNote "No occurrences of this slot in the graph." ;
    skos:inScheme okns:mo ;
    skos:mappingRelation <http://purl.org/ontology/mo/wikipedia> ;
    linkml:definition_uri okns:mo_wikipedia ;
    linkml:inlined true ;
    linkml:range okns:FoafDocument ;
    linkml:slot_uri <http://purl.org/ontology/mo/wikipedia> .

okns:normalizedstring a linkml:TypeDefinition ;
    skos:definition "Normalized string, one that does not contain the carriage return (#xD), line feed (#xA) nor tab (#x9) characters." ;
    skos:inScheme okns:extended_types ;
    skos:note "added by Mahir Morshed <mmorshed@scripps.edu>" ;
    linkml:base "str" ;
    linkml:definition_uri linkml:Normalizedstring ;
    linkml:typeof okns:string ;
    linkml:uri xsd:normalizedString .

okns:rdf_XMLLiteral a linkml:TypeDefinition ;
    dcterms:source rdf: ;
    dcterms:title "XMLLiteral" ;
    skos:definition "The datatype of XML literal values." ;
    skos:inScheme okns:owl-rdf-rdfs ;
    linkml:base "str" ;
    linkml:definition_uri okns:RdfXMLLiteral ;
    linkml:typeof okns:string ;
    linkml:uri rdf:XMLLiteral .

okns:rev_commenter a linkml:SlotDefinition ;
    dcterms:source rev: ;
    dcterms:title "commenter" ;
    skos:definition "The commenter on the review" ;
    skos:editorialNote "No occurrences of this slot in the graph." ;
    skos:inScheme okns:rev ;
    skos:mappingRelation rev:commenter ;
    linkml:definition_uri okns:rev_commenter ;
    linkml:inlined true ;
    linkml:range okns:FoafAgent ;
    linkml:slot_uri rev:commenter ;
    linkml:union_of okns:rev_Comment,
        okns:rev_Feedback .

okns:rev_maxRating a linkml:SlotDefinition ;
    dcterms:source rev: ;
    dcterms:title "max Rating" ;
    skos:definition "A numeric value" ;
    skos:editorialNote "No occurrences of this slot in the graph." ;
    skos:inScheme okns:rev ;
    skos:mappingRelation rev:maxRating ;
    skos:note "description: Maximum value for rating property" ;
    linkml:definition_uri okns:rev_maxRating ;
    linkml:inlined true ;
    linkml:range okns:Any ;
    linkml:slot_uri rev:maxRating .

okns:rev_minRating a linkml:SlotDefinition ;
    dcterms:source rev: ;
    dcterms:title "min Rating" ;
    skos:definition "A numeric value" ;
    skos:editorialNote "No occurrences of this slot in the graph." ;
    skos:inScheme okns:rev ;
    skos:mappingRelation rev:minRating ;
    skos:note "description: Minimum value for rating property" ;
    linkml:definition_uri okns:rev_minRating ;
    linkml:inlined true ;
    linkml:range okns:Any ;
    linkml:slot_uri rev:minRating .

okns:rev_rating a linkml:SlotDefinition ;
    dcterms:source rev: ;
    dcterms:title "rating" ;
    skos:definition "A numeric value" ;
    skos:editorialNote "No occurrences of this slot in the graph." ;
    skos:inScheme okns:rev ;
    skos:mappingRelation rev:rating ;
    linkml:definition_uri okns:rev_rating ;
    linkml:inlined true ;
    linkml:range okns:Any ;
    linkml:slot_uri rev:rating .

okns:rev_text a linkml:SlotDefinition ;
    dcterms:source rev: ;
    dcterms:title "text" ;
    skos:definition "The text of the review" ;
    skos:editorialNote "No occurrences of this slot in the graph." ;
    skos:inScheme okns:rev ;
    skos:mappingRelation rev:text ;
    linkml:definition_uri okns:rev_text ;
    linkml:inlined true ;
    linkml:range okns:Any ;
    linkml:slot_uri rev:text .

okns:rev_type a linkml:SlotDefinition ;
    dcterms:source rev: ;
    dcterms:title "type" ;
    skos:definition "The type of media of a work under review" ;
    skos:editorialNote "No occurrences of this slot in the graph." ;
    skos:inScheme okns:rev ;
    skos:mappingRelation rev:type ;
    linkml:definition_uri okns:rev_type ;
    linkml:inlined true ;
    linkml:range okns:Any ;
    linkml:slot_uri rev:type .

okns:skos_altLabel a linkml:SlotDefinition ;
    dcterms:source <http://www.w3.org/2004/02/skos/core> ;
    dcterms:title "alternative label" ;
    rdfs:subPropertyOf okns:rdfs_label ;
    skos:definition "An alternative lexical label for a resource." ;
    skos:editorialNote "No occurrences of this slot in the graph." ;
    skos:inScheme okns:skos ;
    skos:mappingRelation skos:altLabel ;
    skos:note "description: The range of skos:altLabel is the class of RDF plain literals.",
        "description: skos:prefLabel, skos:altLabel and skos:hiddenLabel are pairwise disjoint properties." ;
    linkml:definition_uri okns:skos_altLabel ;
    linkml:inlined true ;
    linkml:range okns:Any ;
    linkml:slot_uri skos:altLabel .

okns:skos_changeNote a linkml:SlotDefinition ;
    dcterms:source <http://www.w3.org/2004/02/skos/core> ;
    dcterms:title "change note" ;
    rdfs:subPropertyOf okns:skos_note ;
    skos:definition "A note about a modification to a concept." ;
    skos:editorialNote "No occurrences of this slot in the graph." ;
    skos:inScheme okns:skos ;
    skos:mappingRelation skos:changeNote ;
    linkml:definition_uri okns:skos_changeNote ;
    linkml:inlined true ;
    linkml:range okns:Any ;
    linkml:slot_uri skos:changeNote .

okns:skos_definition a linkml:SlotDefinition ;
    dcterms:source <http://www.w3.org/2004/02/skos/core> ;
    dcterms:title "definition" ;
    rdfs:subPropertyOf okns:skos_note ;
    skos:definition "A statement or formal explanation of the meaning of a concept." ;
    skos:editorialNote "No occurrences of this slot in the graph." ;
    skos:inScheme okns:skos ;
    skos:mappingRelation skos:definition ;
    linkml:definition_uri okns:skos_definition ;
    linkml:inlined true ;
    linkml:range okns:Any ;
    linkml:slot_uri skos:definition .

okns:skos_editorialNote a linkml:SlotDefinition ;
    dcterms:source <http://www.w3.org/2004/02/skos/core> ;
    dcterms:title "editorial note" ;
    rdfs:subPropertyOf okns:skos_note ;
    skos:definition "A note for an editor, translator or maintainer of the vocabulary." ;
    skos:editorialNote "No occurrences of this slot in the graph." ;
    skos:inScheme okns:skos ;
    skos:mappingRelation skos:editorialNote ;
    linkml:definition_uri okns:skos_editorialNote ;
    linkml:inlined true ;
    linkml:range okns:Any ;
    linkml:slot_uri skos:editorialNote .

okns:skos_exactMatch a linkml:SlotDefinition ;
    dcterms:source <http://www.w3.org/2004/02/skos/core> ;
    dcterms:title "has exact match" ;
    rdfs:subPropertyOf okns:skos_closeMatch ;
    skos:definition "skos:exactMatch is used to link two concepts, indicating a high degree of confidence that the concepts can be used interchangeably across a wide range of information retrieval applications. skos:exactMatch is a transitive property, and is a sub-property of skos:closeMatch." ;
    skos:editorialNote "No occurrences of this slot in the graph." ;
    skos:inScheme okns:skos ;
    skos:mappingRelation skos:exactMatch ;
    skos:note "description: skos:exactMatch is disjoint with each of the properties skos:broadMatch and skos:relatedMatch." ;
    linkml:definition_uri okns:skos_exactMatch ;
    linkml:inlined true ;
    linkml:range okns:Any ;
    linkml:slot_uri skos:exactMatch .

okns:skos_example a linkml:SlotDefinition ;
    dcterms:source <http://www.w3.org/2004/02/skos/core> ;
    dcterms:title "example" ;
    rdfs:subPropertyOf okns:skos_note ;
    skos:definition "An example of the use of a concept." ;
    skos:editorialNote "No occurrences of this slot in the graph." ;
    skos:inScheme okns:skos ;
    skos:mappingRelation skos:example ;
    linkml:definition_uri okns:skos_example ;
    linkml:inlined true ;
    linkml:range okns:Any ;
    linkml:slot_uri skos:example .

okns:skos_hiddenLabel a linkml:SlotDefinition ;
    dcterms:source <http://www.w3.org/2004/02/skos/core> ;
    dcterms:title "hidden label" ;
    rdfs:subPropertyOf okns:rdfs_label ;
    skos:definition "A lexical label for a resource that should be hidden when generating visual displays of the resource, but should still be accessible to free text search operations." ;
    skos:editorialNote "No occurrences of this slot in the graph." ;
    skos:inScheme okns:skos ;
    skos:mappingRelation skos:hiddenLabel ;
    skos:note "description: The range of skos:hiddenLabel is the class of RDF plain literals.",
        "description: skos:prefLabel, skos:altLabel and skos:hiddenLabel are pairwise disjoint properties." ;
    linkml:definition_uri okns:skos_hiddenLabel ;
    linkml:inlined true ;
    linkml:range okns:Any ;
    linkml:slot_uri skos:hiddenLabel .

okns:skos_historyNote a linkml:SlotDefinition ;
    dcterms:source <http://www.w3.org/2004/02/skos/core> ;
    dcterms:title "history note" ;
    rdfs:subPropertyOf okns:skos_note ;
    skos:definition "A note about the past state/use/meaning of a concept." ;
    skos:editorialNote "No occurrences of this slot in the graph." ;
    skos:inScheme okns:skos ;
    skos:mappingRelation skos:historyNote ;
    linkml:definition_uri okns:skos_historyNote ;
    linkml:inlined true ;
    linkml:range okns:Any ;
    linkml:slot_uri skos:historyNote .

okns:skos_notation a linkml:SlotDefinition ;
    dcterms:source <http://www.w3.org/2004/02/skos/core> ;
    dcterms:title "notation" ;
    skos:definition "A notation, also known as classification code, is a string of characters such as \"T58.5\" or \"303.4833\" used to uniquely identify a concept within the scope of a given concept scheme." ;
    skos:editorialNote "By convention, skos:notation is used with a typed literal in the object position of the triple.",
        "No occurrences of this slot in the graph." ;
    skos:inScheme okns:skos ;
    skos:mappingRelation skos:notation ;
    linkml:definition_uri okns:skos_notation ;
    linkml:inlined true ;
    linkml:range okns:Any ;
    linkml:slot_uri skos:notation .

okns:skos_relatedMatch a linkml:SlotDefinition ;
    dcterms:source <http://www.w3.org/2004/02/skos/core> ;
    dcterms:title "has related match" ;
    rdfs:subPropertyOf okns:skos_related ;
    skos:definition "skos:relatedMatch is used to state an associative mapping link between two conceptual resources in different concept schemes." ;
    skos:editorialNote "No occurrences of this slot in the graph." ;
    skos:inScheme okns:skos ;
    skos:mappingRelation skos:relatedMatch ;
    linkml:definition_uri okns:skos_relatedMatch ;
    linkml:inlined true ;
    linkml:range okns:Any ;
    linkml:slot_uri skos:relatedMatch .

okns:skos_scopeNote a linkml:SlotDefinition ;
    dcterms:source <http://www.w3.org/2004/02/skos/core> ;
    dcterms:title "scope note" ;
    rdfs:subPropertyOf okns:skos_note ;
    skos:definition "A note that helps to clarify the meaning and/or the use of a concept." ;
    skos:editorialNote "No occurrences of this slot in the graph." ;
    skos:inScheme okns:skos ;
    skos:mappingRelation skos:scopeNote ;
    linkml:definition_uri okns:skos_scopeNote ;
    linkml:inlined true ;
    linkml:range okns:Any ;
    linkml:slot_uri skos:scopeNote .

okns:time_hasDuration a linkml:SlotDefinition ;
    dcterms:title "has duration" ;
    rdfs:subPropertyOf okns:time_hasTemporalDuration ;
    skos:definition "Duration of a temporal entity, expressed as a scaled value or nominal value" ;
    skos:editorialNote "No occurrences of this slot in the graph." ;
    skos:inScheme okns:time ;
    skos:mappingRelation time:hasDuration ;
    skos:note "description: Duración de una entidad temporal, evento o actividad, o cosa, expresada como un valor escalado.",
        "description: Duración de una entidad temporal, expresada como un valor escalado o un valor nominal.",
        "description: Duration of a temporal entity, event or activity, or thing, expressed as a scaled value",
        "title: tiene duración" ;
    linkml:definition_uri okns:time_hasDuration ;
    linkml:inlined true ;
    linkml:range okns:TimeDuration ;
    linkml:slot_uri time:hasDuration .

okns:time_hasDurationDescription a linkml:SlotDefinition ;
    dcterms:title "has duration description" ;
    rdfs:subPropertyOf okns:time_hasTemporalDuration ;
    skos:definition "Duration of a temporal entity, expressed using a structured description" ;
    skos:editorialNote "No occurrences of this slot in the graph." ;
    skos:inScheme okns:time ;
    skos:mappingRelation time:hasDurationDescription ;
    skos:note "description: Duración de una entidad temporal, expresada utilizando una descripción estructurada.",
        "description: Duration of a temporal entity, expressed using a structured description",
        "title: tiene descripción de duración" ;
    linkml:definition_uri okns:time_hasDurationDescription ;
    linkml:inlined true ;
    linkml:range okns:TimeGeneralDurationDescription ;
    linkml:slot_uri time:hasDurationDescription .

okns:time_hasTRS a linkml:SlotDefinition ;
    dcterms:title "Temporal reference system used" ;
    skos:definition "The temporal reference system used by a temporal position or extent description." ;
    skos:editorialNote "No occurrences of this slot in the graph." ;
    skos:inScheme okns:time ;
    skos:mappingRelation time:hasTRS ;
    skos:note "description: El sistema de referencia temporal utilizado por una posición temporal o descripción de extensión.",
        "description: The temporal reference system used by a temporal position or extent description.",
        "title: sistema de referencia temporal utilizado" ;
    linkml:definition_uri okns:time_hasTRS ;
    linkml:inlined true ;
    linkml:range okns:TimeTRS ;
    linkml:slot_uri time:hasTRS .

okns:time_unitType a linkml:SlotDefinition ;
    dcterms:title "temporal unit type" ;
    skos:definition "The temporal unit which provides the precision of a date-time value or scale of a temporal extent" ;
    skos:editorialNote "No occurrences of this slot in the graph." ;
    skos:inScheme okns:time ;
    skos:mappingRelation time:unitType ;
    skos:note "description: La unidad de tiempo que proporciona la precisión de un valor fecha-hora o la escala de una extensión temporal.",
        "title: tipo de unidad temporal" ;
    linkml:definition_uri okns:time_unitType ;
    linkml:inlined true ;
    linkml:range okns:TimeTemporalUnit ;
    linkml:slot_uri time:unitType .

okns:tzont_DLSendDate a linkml:SlotDefinition ;
    skos:editorialNote "No occurrences of this slot in the graph." ;
    skos:inScheme okns:daml ;
    skos:mappingRelation tzont:DLSendDate ;
    linkml:definition_uri okns:tzont_DLSendDate ;
    linkml:range okns:date ;
    linkml:slot_uri tzont:DLSendDate .

okns:tzont_DLSstartDate a linkml:SlotDefinition ;
    skos:editorialNote "No occurrences of this slot in the graph." ;
    skos:inScheme okns:daml ;
    skos:mappingRelation tzont:DLSstartDate ;
    linkml:definition_uri okns:tzont_DLSstartDate ;
    linkml:range okns:date ;
    linkml:slot_uri tzont:DLSstartDate .

okns:tzont_countryOf a linkml:SlotDefinition ;
    rdfs:subPropertyOf okns:tzont_hasParentRegion ;
    skos:editorialNote "No occurrences of this slot in the graph." ;
    skos:inScheme okns:daml ;
    skos:mappingRelation tzont:countryOf ;
    linkml:definition_uri okns:tzont_countryOf ;
    linkml:inlined true ;
    linkml:range okns:TzontCountry ;
    linkml:slot_uri tzont:countryOf .

okns:tzont_name a linkml:SlotDefinition ;
    skos:editorialNote "No occurrences of this slot in the graph." ;
    skos:exactMatch daml-iso3166:name ;
    skos:inScheme okns:daml ;
    skos:mappingRelation tzont:name ;
    linkml:definition_uri okns:tzont_name ;
    linkml:inlined true ;
    linkml:range okns:Any ;
    linkml:slot_uri tzont:name .

okns:tzont_stateOf a linkml:SlotDefinition ;
    rdfs:subPropertyOf okns:tzont_hasParentRegion ;
    skos:editorialNote "No occurrences of this slot in the graph." ;
    skos:inScheme okns:daml ;
    skos:mappingRelation tzont:stateOf ;
    linkml:definition_uri okns:tzont_stateOf ;
    linkml:inlined true ;
    linkml:range okns:TzontState ;
    linkml:slot_uri tzont:stateOf .

okns:vann_changes a linkml:SlotDefinition ;
    skos:editorialNote "No occurrences of this slot in the graph." ;
    skos:inScheme okns:frbr ;
    skos:mappingRelation vann:changes ;
    linkml:definition_uri okns:vann_changes ;
    linkml:inlined true ;
    linkml:range okns:Any ;
    linkml:slot_uri vann:changes .

okns:vann_preferredNamespacePrefix a linkml:SlotDefinition ;
    skos:editorialNote "No occurrences of this slot in the graph." ;
    skos:inScheme okns:frbr ;
    skos:mappingRelation vann:preferredNamespacePrefix ;
    linkml:definition_uri okns:vann_preferredNamespacePrefix ;
    linkml:inlined true ;
    linkml:range okns:Any ;
    linkml:slot_uri vann:preferredNamespacePrefix .

okns:vann_preferredNamespaceUri a linkml:SlotDefinition ;
    skos:editorialNote "No occurrences of this slot in the graph." ;
    skos:inScheme okns:frbr ;
    skos:mappingRelation vann:preferredNamespaceUri ;
    linkml:definition_uri okns:vann_preferredNamespaceUri ;
    linkml:inlined true ;
    linkml:range okns:Any ;
    linkml:slot_uri vann:preferredNamespaceUri .

okns:wgs_lat_long a linkml:SlotDefinition ;
    dcterms:title "lat/long" ;
    skos:definition "A comma-separated representation of a latitude, longitude coordinate." ;
    skos:editorialNote "No occurrences of this slot in the graph." ;
    skos:inScheme okns:wgs ;
    skos:mappingRelation wgs1:lat_long ;
    linkml:definition_uri okns:wgs_lat_long ;
    linkml:inlined true ;
    linkml:range okns:Any ;
    linkml:slot_uri wgs1:lat_long .

okns:wgs_location a linkml:SlotDefinition ;
    dcterms:title "location" ;
    rdfs:subPropertyOf okns:foaf_based_near ;
    skos:definition "The relation between something and the point, ␊ or other geometrical thing in space, where it is.  For example, the realtionship between␊ a radio tower and a Point with a given lat and long.␊ Or a relationship between a park and its outline as a closed arc of points, or a road and␊ its location as a arc (a sequence of points).␊ Clearly in practice there will be limit to the accuracy of any such statement, but one would expect␊ an accuracy appropriate for the size of the object and uses such as mapping ." ;
    skos:editorialNote "No occurrences of this slot in the graph." ;
    skos:inScheme okns:wgs ;
    skos:mappingRelation wgs1:location ;
    linkml:definition_uri okns:wgs_location ;
    linkml:inlined true ;
    linkml:range okns:WgsSpatialThing ;
    linkml:slot_uri wgs1:location .

okns:wot_src_assurance a linkml:SlotDefinition ;
    skos:editorialNote "No occurrences of this slot in the graph." ;
    skos:inScheme okns:foaf ;
    skos:mappingRelation wot:src_assurance ;
    linkml:definition_uri okns:wot_src_assurance ;
    linkml:inlined true ;
    linkml:range okns:Any ;
    linkml:slot_uri wot:src_assurance .

okns:xsd_pattern a linkml:SlotDefinition ;
    skos:inScheme okns:time ;
    skos:mappingRelation xsd:pattern ;
    linkml:definition_uri okns:xsd_pattern ;
    linkml:range okns:string ;
    linkml:slot_uri xsd:pattern .

okns:Daml-2001List a linkml:ClassDefinition ;
    skos:inScheme okns:daml ;
    skos:mappingRelation daml-2001:List ;
    linkml:class_uri daml-2001:List ;
    linkml:definition_uri okns:Daml-2001List ;
    linkml:slot_usage [ ] ;
    linkml:slots okns:rdfs_comment .

okns:Daml-country-ontCountry a linkml:ClassDefinition ;
    skos:inScheme okns:daml ;
    skos:mappingRelation daml-country-ont:Country ;
    linkml:class_uri daml-country-ont:Country ;
    linkml:definition_uri okns:Daml-country-ontCountry ;
    linkml:slot_usage [ ] .

okns:Daml-countryUNITED-STATES a linkml:ClassDefinition ;
    dcterms:title "No class (entity type) name specified -- this class is noted as being in the domain or range of a slot in this graph but has not itself been defined." ;
    skos:inScheme okns:daml ;
    skos:mappingRelation daml-country:UNITED-STATES ;
    linkml:class_uri daml-country:UNITED-STATES ;
    linkml:definition_uri okns:Daml-countryUNITED-STATES ;
    linkml:slot_usage [ ] .

okns:Daml-profileLocation a linkml:ClassDefinition ;
    dcterms:title "No class (entity type) name specified -- this class is noted as a superclass of another class in this graph but has not itself been defined." ;
    skos:inScheme okns:daml ;
    skos:mappingRelation daml-profile:Location ;
    linkml:class_uri daml-profile:Location ;
    linkml:definition_uri okns:Daml-profileLocation ;
    linkml:slot_usage [ ] .

okns:DctRightsStatement a linkml:ClassDefinition ;
    dcterms:source dcterms: ;
    dcterms:title "Rights Statement" ;
    skos:definition "A statement about the intellectual property rights (IPR) held in or over a resource, a legal document giving official permission to do something with a resource, or a statement about access rights." ;
    skos:inScheme okns:dc ;
    skos:mappingRelation dcterms:RightsStatement ;
    linkml:class_uri dcterms:RightsStatement ;
    linkml:definition_uri okns:DctRightsStatement ;
    linkml:slot_usage [ ] .

okns:FoafOrganization a linkml:ClassDefinition ;
    dcterms:source foaf: ;
    dcterms:title "Organization" ;
    skos:definition "An organization." ;
    skos:inScheme okns:foaf ;
    skos:mappingRelation foaf:Organization ;
    linkml:class_uri foaf:Organization ;
    linkml:definition_uri okns:FoafOrganization ;
    linkml:is_a okns:FoafAgent ;
    linkml:slot_usage [ ] .

<https://purl.org/okn/schema/HttpPurl.orgNETC4dmKeys.owl#Key> a linkml:ClassDefinition ;
    dcterms:title "No class (entity type) name specified -- this class is noted as being in the domain or range of a slot in this graph but has not itself been defined." ;
    skos:inScheme okns:mo ;
    skos:mappingRelation <http://purl.org/NET/c4dm/keys.owl#Key> ;
    linkml:class_uri <http://purl.org/NET/c4dm/keys.owl#Key> ;
    linkml:definition_uri <https://purl.org/okn/schema/HttpPurl.orgNETC4dmKeys.owl#Key> ;
    linkml:slot_usage [ ] .

okns:IcalListOfFloat a linkml:ClassDefinition ;
    skos:inScheme okns:ical ;
    skos:mappingRelation ical:List_of_Float ;
    linkml:class_uri ical:List_of_Float ;
    linkml:definition_uri okns:IcalListOfFloat ;
    linkml:slot_usage [ ] .

okns:IcalValarm a linkml:ClassDefinition ;
    dcterms:title "VALARM" ;
    skos:definition "Provide a grouping of component properties that define an alarm." ;
    skos:inScheme okns:ical ;
    skos:mappingRelation ical:Valarm ;
    linkml:class_uri ical:Valarm ;
    linkml:definition_uri okns:IcalValarm ;
    linkml:slot_usage [ ] .

okns:IcalValueDURATION a linkml:ClassDefinition ;
    skos:inScheme okns:ical ;
    skos:mappingRelation ical:Value_DURATION ;
    linkml:class_uri ical:Value_DURATION ;
    linkml:definition_uri okns:IcalValueDURATION ;
    linkml:slot_usage [ ] .

okns:IcalValuePERIOD a linkml:ClassDefinition ;
    skos:inScheme okns:ical ;
    skos:mappingRelation ical:Value_PERIOD ;
    linkml:class_uri ical:Value_PERIOD ;
    linkml:definition_uri okns:IcalValuePERIOD ;
    linkml:slot_usage [ ] .

okns:IcalVevent a linkml:ClassDefinition ;
    dcterms:title "VEVENT" ;
    skos:definition "Provide a grouping of component properties that describe an event." ;
    skos:inScheme okns:ical ;
    skos:mappingRelation ical:Vevent ;
    linkml:class_uri ical:Vevent ;
    linkml:definition_uri okns:IcalVevent ;
    linkml:slot_usage [ ] .

okns:MoActivity a linkml:ClassDefinition ;
    dcterms:source <http://purl.org/ontology/mo/> ;
    dcterms:title "activity" ;
    skos:definition "An activity period, defining when an artist was musically active." ;
    skos:inScheme okns:mo ;
    skos:mappingRelation ns1:Activity ;
    linkml:class_uri <http://purl.org/ontology/mo/Activity> ;
    linkml:definition_uri okns:MoActivity ;
    linkml:is_a okns:EventEvent ;
    linkml:slot_usage [ ] .

okns:MoAudioFile a linkml:ClassDefinition ;
    dcterms:source <http://purl.org/ontology/mo/> ;
    dcterms:title "audio file" ;
    skos:definition "An audio file, which may be available on a local file system or through http, ftp, etc." ;
    skos:inScheme okns:mo ;
    skos:mappingRelation ns1:AudioFile ;
    linkml:class_uri <http://purl.org/ontology/mo/AudioFile> ;
    linkml:definition_uri okns:MoAudioFile ;
    linkml:is_a okns:FoafDocument ;
    linkml:slot_usage [ ] .

okns:MoCorporateBody a linkml:ClassDefinition ;
    dcterms:source <http://purl.org/ontology/mo/> ;
    dcterms:title "corporate body" ;
    skos:definition "Organization or group of individuals and/or other organizations involved in the music market." ;
    skos:inScheme okns:mo ;
    skos:mappingRelation ns1:CorporateBody ;
    linkml:class_uri <http://purl.org/ontology/mo/CorporateBody> ;
    linkml:definition_uri okns:MoCorporateBody ;
    linkml:is_a okns:FoafOrganization ;
    linkml:slot_usage [ ] .

okns:MoGenre a linkml:ClassDefinition ;
    dcterms:source <http://purl.org/ontology/mo/> ;
    dcterms:title "Genre" ;
    skos:definition "An expressive style of music.␊        ␊        Any taxonomy can be plug-in here. You can either define a genre by yourself, like this:␊␊        :mygenre a mo:Genre; dc:title \"electro rock\".␊␊        Or you can refer to a DBPedia genre (such as http://dbpedia.org/resource/Baroque_music), allowing semantic web␊        clients to access easily really detailed structured information about the genre you are refering to." ;
    skos:inScheme okns:mo ;
    skos:mappingRelation ns1:Genre ;
    linkml:class_uri <http://purl.org/ontology/mo/Genre> ;
    linkml:definition_uri okns:MoGenre ;
    linkml:slot_usage [ ] .

okns:MoMusicGroup a linkml:ClassDefinition ;
    dcterms:source <http://purl.org/ontology/mo/> ;
    dcterms:title "music group" ;
    skos:definition "Group of musicians, or musical ensemble, usually popular or folk, playing parts of or improvising off of a musical arrangement." ;
    skos:inScheme okns:mo ;
    skos:mappingRelation ns1:MusicGroup ;
    linkml:class_uri <http://purl.org/ontology/mo/MusicGroup> ;
    linkml:definition_uri okns:MoMusicGroup ;
    linkml:is_a okns:MoMusicArtist ;
    linkml:slot_usage [ ] .

okns:MoRecordingSession a linkml:ClassDefinition ;
    dcterms:source <http://purl.org/ontology/mo/> ;
    dcterms:title "recording session" ;
    skos:definition "A set of performances/recordings/mastering events. This event can be decomposed in its constituent events using event:sub_event" ;
    skos:inScheme okns:mo ;
    skos:mappingRelation ns1:RecordingSession ;
    linkml:class_uri <http://purl.org/ontology/mo/RecordingSession> ;
    linkml:definition_uri okns:MoRecordingSession ;
    linkml:is_a okns:EventEvent ;
    linkml:slot_usage [ ] .

okns:MoReleaseEvent a linkml:ClassDefinition ;
    dcterms:source <http://purl.org/ontology/mo/> ;
    dcterms:title "release event" ;
    skos:definition "A release event, in a particular place (e.g. a country) at a particular time. Other factors of this event might include cover art, liner notes, box, etc. or a release grouping all these." ;
    skos:inScheme okns:mo ;
    skos:mappingRelation ns1:ReleaseEvent ;
    linkml:class_uri <http://purl.org/ontology/mo/ReleaseEvent> ;
    linkml:definition_uri okns:MoReleaseEvent ;
    linkml:is_a okns:EventEvent ;
    linkml:slot_usage [ ] .

okns:MoScore a linkml:ClassDefinition ;
    dcterms:source <http://purl.org/ontology/mo/> ;
    dcterms:title "score" ;
    skos:definition "Here, we are dealing with the informational object (the MusicalExpression), not the actually \"published\" score.␊        This may be, for example, the product of an arrangement process." ;
    skos:inScheme okns:mo ;
    skos:mappingRelation ns1:Score ;
    linkml:class_uri <http://purl.org/ontology/mo/Score> ;
    linkml:definition_uri okns:MoScore ;
    linkml:is_a okns:MoMusicalExpression ;
    linkml:slot_usage [ ] .

okns:OwlAllDifferent a linkml:ClassDefinition ;
    dcterms:source owl: ;
    dcterms:title "AllDifferent" ;
    skos:definition "The class of collections of pairwise different individuals." ;
    skos:inScheme okns:owl-rdf-rdfs ;
    skos:mappingRelation owl:AllDifferent ;
    linkml:class_uri owl:AllDifferent ;
    linkml:definition_uri okns:OwlAllDifferent ;
    linkml:is_a okns:RdfsResource ;
    linkml:slot_usage [ ] .

okns:RdfSeq a linkml:ClassDefinition ;
    dcterms:source rdf: ;
    dcterms:title "Seq" ;
    skos:definition "The class of ordered containers." ;
    skos:inScheme okns:owl-rdf-rdfs ;
    skos:mappingRelation rdf:Seq ;
    linkml:class_uri rdf:Seq ;
    linkml:definition_uri okns:RdfSeq ;
    linkml:is_a okns:RdfsContainer ;
    linkml:slot_usage [ ] .

okns:RevComment a linkml:ClassDefinition ;
    dcterms:source rev: ;
    dcterms:title "Comment" ;
    skos:definition "A comment on a review" ;
    skos:inScheme okns:rev ;
    skos:mappingRelation rev:Comment ;
    linkml:class_uri rev:Comment ;
    linkml:definition_uri okns:RevComment ;
    linkml:slot_usage [ ] .

okns:RevFeedback a linkml:ClassDefinition ;
    dcterms:source rev: ;
    dcterms:title "Feedback" ;
    skos:definition "Feedback on the review. Expresses whether the review was useful or not" ;
    skos:inScheme okns:rev ;
    skos:mappingRelation rev:Feedback ;
    linkml:class_uri rev:Feedback ;
    linkml:definition_uri okns:RevFeedback ;
    linkml:slot_usage [ ] .

okns:SimNetwork a linkml:ClassDefinition ;
    dcterms:source sim: ;
    dcterms:title "Network" ;
    skos:definition "A network is a grouping of <code>sim:Association</code>s.  The associations that comprise a network are specified using a series of <code>sim:edge</code> predicates." ;
    skos:inScheme okns:sim ;
    skos:mappingRelation sim:Network ;
    linkml:class_uri sim:Network ;
    linkml:definition_uri okns:SimNetwork ;
    linkml:is_a okns:OwlThing ;
    linkml:slot_usage [ ] .

okns:SkosOrderedCollection a linkml:ClassDefinition ;
    dcterms:source <http://www.w3.org/2004/02/skos/core> ;
    dcterms:title "Ordered Collection" ;
    skos:definition "An ordered collection of concepts, where both the grouping and the ordering are meaningful." ;
    skos:editorialNote "Ordered collections can be used where you would like a set of concepts to be displayed in a specific order, and optionally under a 'node label'." ;
    skos:inScheme okns:skos ;
    skos:mappingRelation skos:OrderedCollection ;
    linkml:class_uri skos:OrderedCollection ;
    linkml:definition_uri okns:SkosOrderedCollection ;
    linkml:is_a okns:SkosCollection ;
    linkml:slot_usage [ ] .

okns:Time-entryProperInterval a linkml:ClassDefinition ;
    skos:inScheme okns:daml ;
    skos:mappingRelation time-entry:ProperInterval ;
    linkml:class_uri time-entry:ProperInterval ;
    linkml:definition_uri okns:Time-entryProperInterval ;
    linkml:is_a okns:Time-entryProperIntervalThing ;
    linkml:slot_usage [ ] .

okns:Time-entryTemporalUnit a linkml:ClassDefinition ;
    skos:inScheme okns:daml ;
    skos:mappingRelation time-entry:TemporalUnit ;
    linkml:class_uri time-entry:TemporalUnit ;
    linkml:definition_uri okns:Time-entryTemporalUnit ;
    linkml:slot_usage [ ] .

okns:TimeDurationDescription a linkml:ClassDefinition ;
    dcterms:title "Duration description" ;
    skos:definition "Description of temporal extent structured with separate values for the various elements of a calendar-clock system. The temporal reference system is fixed to Gregorian Calendar, and the range of each of the numeric properties is restricted to xsd:decimal" ;
    skos:editorialNote "En el calendario gregoriano la longitud de los meses no es fija. Por lo tanto, un valor como \"2,5 meses\" no se puede comparar exactamente con una duración similar expresada en términos de semanas o días.",
        "In the Gregorian calendar the length of the month is not fixed. Therefore, a value like \"2.5 months\" cannot be exactly compared with a similar duration expressed in terms of weeks or days." ;
    skos:inScheme okns:time ;
    skos:mappingRelation time:DurationDescription ;
    skos:note "description: Descripción de extensión temporal estructurada con valores separados para los distintos elementos de un sistema de horario-calendario. El sistema de referencia temporal se fija al calendario gregoriano, y el intervalo de cada una de las propiedades numéricas se restringe a xsd:decimal.",
        "description: Description of temporal extent structured with separate values for the various elements of a calendar-clock system. The temporal reference system is fixed to Gregorian Calendar, and the range of each of the numeric properties is restricted to xsd:decimal",
        "title: descripción de duración" ;
    linkml:class_uri time:DurationDescription ;
    linkml:definition_uri okns:TimeDurationDescription ;
    linkml:is_a okns:TimeGeneralDurationDescription ;
    linkml:slot_usage [ ] .

okns:TimeMonthOfYear a linkml:ClassDefinition ;
    dcterms:title "Month of year" ;
    skos:definition "The month of the year" ;
    skos:editorialNote "Característica en riesgo - añadida en la revisión de 2017, y no utilizada todavía de forma amplia.",
        "Feature at risk - added in 2017 revision, and not yet widely used.",
        "La pertenencia a la clase 'mes del año' está abierta, a permitir calendarios anuales alternativos y diferentes nombres de meses.",
        "Membership of the class :MonthOfYear is open, to allow for alternative annual calendars and different month names." ;
    skos:inScheme okns:time ;
    skos:mappingRelation time:MonthOfYear ;
    skos:note "description: El mes del año.",
        "description: The month of the year",
        "title: mes del año" ;
    linkml:class_uri time:MonthOfYear ;
    linkml:definition_uri okns:TimeMonthOfYear ;
    linkml:is_a okns:TimeDateTimeDescription ;
    linkml:slot_usage [ ] .

okns:TimeTRS a linkml:ClassDefinition ;
    dcterms:title "Temporal Reference System" ;
    skos:definition "A temporal reference system, such as a temporal coordinate system (with an origin, direction, and scale), a calendar-clock combination, or a (possibly hierarchical) ordinal system. ␊␊This is a stub class, representing the set of all temporal reference systems." ;
    skos:editorialNote "A taxonomy of temporal reference systems is provided in ISO 19108:2002 [ISO19108], including (a) calendar + clock systems; (b) temporal coordinate systems (i.e. numeric offset from an epoch); (c) temporal ordinal reference systems (i.e. ordered sequence of named intervals, not necessarily of equal duration).",
        "En el ISO 19108:2002 [ISO19108] se proporciona una taxonomía de sistemas de referencia temporal, incluyendo (a) sistemas de calendario + reloj; (b) sistemas de coordenadas temporales (es decir, desplazamiento numérico a partir de una época); (c) sistemas de referencia ordinales temporales (es decir, secuencia ordenada de intervalos nombrados, no necesariamente de igual duración)." ;
    skos:inScheme okns:time ;
    skos:mappingRelation time:TRS ;
    skos:note """description: A temporal reference system, such as a temporal coordinate system (with an origin, direction, and scale), a calendar-clock combination, or a (possibly hierarchical) ordinal system. 

This is a stub class, representing the set of all temporal reference systems.""",
        """description: Un sistema de referencia temporal, tal como un sistema de coordenadas temporales (con un origen, una dirección y una escala), una combinación calendario-reloj, o un sistema ordinal (posiblemente jerárquico).
        Esta clase comodín representa el conjunto de todos los sistemas de referencia temporal.""",
        """description: Un sistema de referencia temporal, tal como un sistema de coordenadas temporales (con un origen, una dirección y una escala), una combinación calendario-reloj, o un sistema ordinal (posiblemente jerárquico).
    Esta clase comodín representa el conjunto de todos los sistemas de referencia temporal.""",
        "title: sistema de referencia temporal" ;
    linkml:class_uri time:TRS ;
    linkml:definition_uri okns:TimeTRS ;
    linkml:slot_usage [ ] .

okns:TimeTimeZone a linkml:ClassDefinition ;
    dcterms:title "Time Zone" ;
    skos:definition "A Time Zone specifies the amount by which the local time is offset from UTC. ␊	A time zone is usually denoted geographically (e.g. Australian Eastern Daylight Time), with a constant value in a given region. ␊The region where it applies and the offset from UTC are specified by a locally recognised governing authority." ;
    skos:editorialNote """A designated timezone is associated with a geographic region. However, for a particular region the offset from UTC often varies seasonally, and the dates of the changes may vary from year to year. The timezone designation usually changes for the different seasons (e.g. Australian Eastern Standard Time vs. Australian Eastern Daylight Time). Furthermore, the offset for a timezone may change over longer timescales, though its designation might not.  

Detailed guidance about working with time zones is given in http://www.w3.org/TR/timezone/ .""",
        "An ontology for time zone descriptions was described in [owl-time-20060927] and provided as RDF in a separate namespace tzont:. However, that ontology was incomplete in scope, and the example datasets were selective. Furthermore, since the use of a class from an external ontology as the range of an ObjectProperty in OWL-Time creates a dependency, reference to the time zone class has been replaced with the 'stub' class in the normative part of this version of OWL-Time.",
        "En esta implementación 'huso horario' no tiene definidas propiedades. Se debería pensar como una superclase \"abstracta\" de todas las implementaciones de huso horario específicas.",
        """En la versión original de OWL-Time de 2006, se definió, en un espacio de nombres diferente "http://www.w3.org/2006/timezone#", la clase 'huso horario', con varias propiedades específicas correspondientes a un modelo específico de huso horario.
    En la versión actual hay una clase con el mismo nombre local en el espacio de nombres de OWL-Time, eliminando la dependencia del espacio de nombres externo.
    Un axioma de alineación permite que los datos codificados de acuerdo con la versión anterior sean consistentes con la ontología actualizada.""",
        """In the original 2006 version of OWL-Time, the TimeZone class, with several properties corresponding to a specific model of time-zones, was defined in a separate namespace "http://www.w3.org/2006/timezone#". 

In the current version a class with same local name is put into the main OWL-Time namespace, removing the dependency on the external namespace. 

An alignment axiom 
	tzont:TimeZone rdfs:subClassOf time:TimeZone . 
allows data encoded according to the previous version to be consistent with the updated ontology.""",
        "In this implementation TimeZone has no properties defined. It should be thought of as an 'abstract' superclass of all specific timezone implementations.",
        """Un huso horario designado está asociado con una región geográfica. Sin embargo, para una región particular el desplazamiento desde UTC a menudo varía según las estaciones, y las fechas de los cambios pueden variar de un año a otro. La designación de huso horario  normalmente cambia de una estación a otra (por ejemplo, el horario estándar frente al horario de verano ambos del este de Australia). Además, del desplazamiento para un huso horario puede cambiar sobre escalas de tiempo mayores, aunque su designación no lo haga.
    Se puede encontrar una guía detallada sobre el funcionamiento de husos horarios en http://www.w3.org/TR/timezone/."@es , "En [owl-time-20060927] se describió una ontología para descripciones de husos horarios, y se proporcionó en un espacio de nombres separado tzont:. Sin embargo, dicha ontología estaba incompleta en su alcance, y el ejemplo de conjuntos de datos (datasets) era selectivo. Además, puesto que el uso de una clase de una ontología externa como el rango de una propiedad de objeto en OWL-Time crea una dependencia, la referencia a la clase huso horario se ha reemplazado por una clase que viene a ser un "cajón de sastre" en la en la parte normativa de esta versión de OWL-Time.""" ;
    skos:inScheme okns:time ;
    skos:mappingRelation time:TimeZone ;
    skos:note """description: A Time Zone specifies the amount by which the local time is offset from UTC. 
	A time zone is usually denoted geographically (e.g. Australian Eastern Daylight Time), with a constant value in a given region. 
The region where it applies and the offset from UTC are specified by a locally recognised governing authority.""",
        """description: Un huso horario especifica la cantidad en que la hora local está desplazada con respecto a UTC.
        Un huso horario normalmente se denota geográficamente (p.ej. el horario de verano del este de Australia), con un valor constante en una región dada.
        La región donde aplica y el desplazamiento desde UTC las especifica una autoridad gubernamental localmente reconocida.""",
        """description: Un huso horario especifica la cantidad en que la hora local está desplazada con respecto a UTC.
    Un huso horario normalmente se denota geográficamente (p.ej. el horario de verano del este de Australia), con un valor constante en una región dada.
    La región donde aplica y el desplazamiento desde UTC las especifica una autoridad gubernamental localmente reconocida.""",
        "title: huso horario" ;
    linkml:class_uri time:TimeZone ;
    linkml:definition_uri okns:TimeTimeZone ;
    linkml:slot_usage [ ] .

okns:TzontCountry a linkml:ClassDefinition ;
    skos:inScheme okns:daml ;
    skos:mappingRelation tzont:Country ;
    linkml:class_uri tzont:Country ;
    linkml:definition_uri okns:TzontCountry ;
    linkml:is_a okns:TzontPoliticalRegion ;
    linkml:slot_usage [ ] .

okns:TzontState a linkml:ClassDefinition ;
    skos:inScheme okns:daml ;
    skos:mappingRelation tzont:State ;
    linkml:class_uri tzont:State ;
    linkml:definition_uri okns:TzontState ;
    linkml:is_a okns:TzontPoliticalRegion ;
    linkml:slot_usage [ ] .

okns:WfbGEOREF a linkml:ClassDefinition ;
    dcterms:title "No class (entity type) name specified -- this class is noted as being in the domain or range of a slot in this graph but has not itself been defined." ;
    skos:inScheme okns:daml ;
    skos:mappingRelation wfb:GEOREF ;
    linkml:class_uri wfb:GEOREF ;
    linkml:definition_uri okns:WfbGEOREF ;
    linkml:slot_usage [ ] .

okns:Wn16Credential a linkml:ClassDefinition ;
    dcterms:title "No class (entity type) name specified -- this class is noted as a superclass of another class in this graph but has not itself been defined." ;
    skos:inScheme okns:wot ;
    skos:mappingRelation wn16:Credential ;
    linkml:class_uri wn16:Credential ;
    linkml:definition_uri okns:Wn16Credential ;
    linkml:slot_usage [ ] .

okns:Wn16Event a linkml:ClassDefinition ;
    dcterms:title "No class (entity type) name specified -- this class is noted as a superclass of another class in this graph but has not itself been defined." ;
    skos:inScheme okns:wot ;
    skos:mappingRelation wn16:Event ;
    linkml:class_uri wn16:Event ;
    linkml:definition_uri okns:Wn16Event ;
    linkml:slot_usage [ ] .

<https://purl.org/okn/schema/Wn16Work~2> a linkml:ClassDefinition ;
    skos:inScheme okns:frbr ;
    skos:mappingRelation <http://xmlns.com/wordnet/1.6/Work~2> ;
    linkml:class_uri <http://xmlns.com/wordnet/1.6/Work~2> ;
    linkml:definition_uri <https://purl.org/okn/schema/Wn16Work~2> ;
    linkml:slot_usage [ ] .

okns:WotEndorsement a linkml:ClassDefinition ;
    dcterms:source wot: ;
    dcterms:title "Endorsement" ;
    skos:definition "An endorsement resource containing a detached ascii signature." ;
    skos:inScheme okns:wot ;
    skos:mappingRelation wot:Endorsement ;
    linkml:class_uri wot:Endorsement ;
    linkml:definition_uri okns:WotEndorsement ;
    linkml:is_a okns:Wn16Endorsement-4 ;
    linkml:slot_usage [ ] .

okns:XsdDateTimeStamp a linkml:ClassDefinition ;
    dcterms:title "No class (entity type) name specified -- this class is noted as being in the domain or range of a slot in this graph but has not itself been defined." ;
    skos:inScheme okns:time ;
    skos:mappingRelation xsd:dateTimeStamp ;
    linkml:class_uri xsd:dateTimeStamp ;
    linkml:definition_uri okns:XsdDateTimeStamp ;
    linkml:slot_usage [ ] .

okns:XsdGDay a linkml:ClassDefinition ;
    dcterms:title "No class (entity type) name specified -- this class is noted as being in the domain or range of a slot in this graph but has not itself been defined." ;
    skos:inScheme okns:daml ;
    skos:mappingRelation xsd:gDay ;
    linkml:class_uri xsd:gDay ;
    linkml:definition_uri okns:XsdGDay ;
    linkml:slot_usage [ ] .

okns:XsdGMonth a linkml:ClassDefinition ;
    dcterms:title "No class (entity type) name specified -- this class is noted as being in the domain or range of a slot in this graph but has not itself been defined." ;
    skos:inScheme okns:daml ;
    skos:mappingRelation xsd:gMonth ;
    linkml:class_uri xsd:gMonth ;
    linkml:definition_uri okns:XsdGMonth ;
    linkml:slot_usage [ ] .

okns:XsdGYearMonth a linkml:ClassDefinition ;
    dcterms:title "No class (entity type) name specified -- this class is noted as being in the domain or range of a slot in this graph but has not itself been defined." ;
    skos:inScheme okns:time ;
    skos:mappingRelation xsd:gYearMonth ;
    linkml:class_uri xsd:gYearMonth ;
    linkml:definition_uri okns:XsdGYearMonth ;
    linkml:slot_usage [ ] .

okns:ao_application a linkml:SlotDefinition ;
    dcterms:source ao: ;
    dcterms:title "has application" ;
    rdfs:subPropertyOf okns:ao_context ;
    skos:definition "An application, which is associated to an individual, e.g. a music player to a music track it's currently playing back." ;
    skos:editorialNote "No occurrences of this slot in the graph." ;
    skos:inScheme okns:ao ;
    skos:mappingRelation ao:application ;
    linkml:definition_uri okns:ao_application ;
    linkml:inlined true ;
    linkml:range okns:Any ;
    linkml:slot_uri ao:application .

okns:ao_device a linkml:SlotDefinition ;
    dcterms:source ao: ;
    dcterms:title "has device" ;
    rdfs:subPropertyOf okns:ao_context ;
    skos:definition "A device, which is associated with an individual, e.g. a CD player with a CD it's currently playing back." ;
    skos:editorialNote "No occurrences of this slot in the graph." ;
    skos:inScheme okns:ao ;
    skos:mappingRelation ao:device ;
    linkml:definition_uri okns:ao_device ;
    linkml:inlined true ;
    linkml:range okns:Any ;
    linkml:slot_uri ao:device .

okns:ao_included_association a linkml:SlotDefinition ;
    dcterms:source ao: ;
    dcterms:title "has included association" ;
    skos:definition "This property could be used to compose association statements or to reuse them, e.g. to make them likeable in a specific context." ;
    skos:editorialNote "No occurrences of this slot in the graph." ;
    skos:inScheme okns:ao ;
    skos:mappingRelation ao:included_association ;
    linkml:definition_uri okns:ao_included_association ;
    linkml:domain okns:SimAssociation ;
    linkml:inlined true ;
    linkml:owner okns:ao_included_association ;
    linkml:range okns:SimAssociation ;
    linkml:slot_uri ao:included_association .

okns:ao_likeminded a linkml:SlotDefinition ;
    dcterms:source ao: ;
    dcterms:title "has likeminded" ;
    skos:definition "Associates likeminded people to an association, which they like/ agree with." ;
    skos:editorialNote "No occurrences of this slot in the graph." ;
    skos:inScheme okns:ao ;
    skos:mappingRelation ao:likeminded ;
    linkml:definition_uri okns:ao_likeminded ;
    linkml:domain okns:SimAssociation ;
    linkml:inlined true ;
    linkml:owner okns:ao_likeminded ;
    linkml:range okns:FoafAgent ;
    linkml:slot_uri ao:likeminded .

okns:ao_mood a linkml:SlotDefinition ;
    dcterms:source ao: ;
    dcterms:title "has mood" ;
    rdfs:subPropertyOf okns:dct_subject ;
    skos:definition "A mood that should be created by something." ;
    skos:editorialNote "No occurrences of this slot in the graph." ;
    skos:inScheme okns:ao ;
    skos:mappingRelation ao:mood ;
    linkml:definition_uri okns:ao_mood ;
    linkml:domain okns:OwlThing ;
    linkml:inlined true ;
    linkml:owner okns:ao_mood ;
    linkml:range okns:Any ;
    linkml:slot_uri ao:mood .

okns:ao_occasion a linkml:SlotDefinition ;
    dcterms:source ao: ;
    dcterms:title "has occassion" ;
    rdfs:subPropertyOf okns:dct_subject ;
    skos:definition "An occasion for which something was created." ;
    skos:editorialNote "No occurrences of this slot in the graph." ;
    skos:inScheme okns:ao ;
    skos:mappingRelation ao:occasion ;
    linkml:definition_uri okns:ao_occasion ;
    linkml:domain okns:OwlThing ;
    linkml:inlined true ;
    linkml:owner okns:ao_occasion ;
    linkml:range okns:Any ;
    linkml:slot_uri ao:occasion .

okns:cc_derivativeWork a linkml:SlotDefinition ;
    dcterms:title "has a derivative work" ;
    rdfs:seeAlso dc:source ;
    skos:editorialNote "No occurrences of this slot in the graph." ;
    skos:inScheme okns:cc ;
    skos:mappingRelation cc:derivativeWork ;
    linkml:definition_uri okns:cc_derivativeWork ;
    linkml:domain okns:CcWork ;
    linkml:inlined true ;
    linkml:owner okns:cc_derivativeWork ;
    linkml:range okns:CcWork ;
    linkml:slot_uri cc:derivativeWork .

okns:cc_license a linkml:SlotDefinition ;
    dcterms:title "has license" ;
    rdfs:seeAlso <http://www.w3.org/2000/10/swap/pim/doc#ipr> ;
    rdfs:subPropertyOf okns:dct_license ;
    skos:editorialNote "No occurrences of this slot in the graph." ;
    skos:inScheme okns:cc ;
    skos:mappingRelation cc:license ;
    linkml:definition_uri okns:cc_license ;
    linkml:domain okns:CcWork ;
    linkml:inlined true ;
    linkml:owner okns:cc_license ;
    linkml:range okns:CcLicense ;
    linkml:slot_uri cc:license .

okns:cc_permits a linkml:SlotDefinition ;
    dcterms:title "permits" ;
    skos:editorialNote "No occurrences of this slot in the graph." ;
    skos:inScheme okns:cc ;
    skos:mappingRelation cc:permits ;
    linkml:definition_uri okns:cc_permits ;
    linkml:domain okns:CcLicense ;
    linkml:inlined true ;
    linkml:owner okns:cc_permits ;
    linkml:range okns:CcPermission ;
    linkml:slot_uri cc:permits .

okns:cc_prohibits a linkml:SlotDefinition ;
    dcterms:title "prohibits" ;
    skos:editorialNote "No occurrences of this slot in the graph." ;
    skos:inScheme okns:cc ;
    skos:mappingRelation cc:prohibits ;
    linkml:definition_uri okns:cc_prohibits ;
    linkml:domain okns:CcLicense ;
    linkml:inlined true ;
    linkml:owner okns:cc_prohibits ;
    linkml:range okns:CcProhibition ;
    linkml:slot_uri cc:prohibits .

okns:cc_requires a linkml:SlotDefinition ;
    dcterms:title "requires" ;
    skos:editorialNote "No occurrences of this slot in the graph." ;
    skos:inScheme okns:cc ;
    skos:mappingRelation cc:requires ;
    linkml:definition_uri okns:cc_requires ;
    linkml:domain okns:CcLicense ;
    linkml:inlined true ;
    linkml:owner okns:cc_requires ;
    linkml:range okns:CcRequirement ;
    linkml:slot_uri cc:requires .

okns:daml_2001_comment a linkml:SlotDefinition ;
    skos:inScheme okns:daml ;
    skos:mappingRelation daml-2001:comment ;
    linkml:definition_uri okns:daml_2001_comment ;
    linkml:domain_of okns:Daml-2001Property ;
    linkml:owner okns:Daml-2001Property ;
    linkml:range okns:string ;
    linkml:slot_uri daml-2001:comment .

okns:daml_2001_complementOf a linkml:SlotDefinition ;
    skos:inScheme okns:daml ;
    skos:mappingRelation daml-2001:complementOf ;
    linkml:definition_uri okns:daml_2001_complementOf ;
    linkml:domain_of okns:Daml-2001Class ;
    linkml:inlined true ;
    linkml:owner okns:Daml-2001Class ;
    linkml:range okns:Daml-2001Class ;
    linkml:slot_uri daml-2001:complementOf .

okns:daml_2001_imports a linkml:SlotDefinition ;
    skos:inScheme okns:daml ;
    skos:mappingRelation daml-2001:imports ;
    linkml:definition_uri okns:daml_2001_imports ;
    linkml:domain_of okns:Daml-2001Ontology ;
    linkml:owner okns:Daml-2001Ontology ;
    linkml:range okns:uri ;
    linkml:slot_uri daml-2001:imports .

okns:daml_2001_unionOf a linkml:SlotDefinition ;
    skos:inScheme okns:daml ;
    skos:mappingRelation daml-2001:unionOf ;
    linkml:definition_uri okns:daml_2001_unionOf ;
    linkml:domain_of okns:Daml-2001Class ;
    linkml:owner okns:Daml-2001Class ;
    linkml:range okns:rdf_XMLLiteral ;
    linkml:slot_uri daml-2001:unionOf .

okns:daml_2001_versionInfo a linkml:SlotDefinition ;
    skos:inScheme okns:daml ;
    skos:mappingRelation daml-2001:versionInfo ;
    linkml:definition_uri okns:daml_2001_versionInfo ;
    linkml:domain_of okns:Daml-2001Ontology ;
    linkml:owner okns:Daml-2001Ontology ;
    linkml:range okns:string ;
    linkml:slot_uri daml-2001:versionInfo .

okns:daml_asClass a linkml:SlotDefinition ;
    skos:inScheme okns:daml ;
    skos:mappingRelation daml:asClass ;
    linkml:definition_uri okns:daml_asClass ;
    linkml:domain_of okns:DamlClass ;
    linkml:inlined true ;
    linkml:owner okns:DamlClass ;
    linkml:range okns:DamlClass ;
    linkml:slot_uri daml:asClass .

okns:daml_city_country a linkml:SlotDefinition ;
    skos:editorialNote "No occurrences of this slot in the graph." ;
    skos:inScheme okns:daml ;
    skos:mappingRelation daml-city:country ;
    linkml:definition_uri okns:daml_city_country ;
    linkml:domain okns:Daml-cityCity ;
    linkml:inlined true ;
    linkml:owner okns:daml_city_country ;
    linkml:range okns:Daml-countryCountry ;
    linkml:slot_uri daml-city:country .

okns:daml_city_name a linkml:SlotDefinition ;
    skos:editorialNote "No occurrences of this slot in the graph." ;
    skos:inScheme okns:daml ;
    skos:mappingRelation daml-city:name ;
    linkml:definition_uri okns:daml_city_name ;
    linkml:domain okns:Daml-cityCity ;
    linkml:inlined true ;
    linkml:owner okns:daml_city_name ;
    linkml:range okns:RdfsLiteral ;
    linkml:slot_uri daml-city:name .

okns:daml_complementOf a linkml:SlotDefinition ;
    skos:inScheme okns:daml ;
    skos:mappingRelation daml:complementOf ;
    linkml:definition_uri okns:daml_complementOf ;
    linkml:domain_of okns:DamlClass ;
    linkml:inlined true ;
    linkml:owner okns:DamlClass ;
    linkml:range okns:DamlClass ;
    linkml:slot_uri daml:complementOf .

okns:daml_country_cia a linkml:SlotDefinition ;
    skos:editorialNote "No occurrences of this slot in the graph." ;
    skos:inScheme okns:daml ;
    skos:mappingRelation daml-country:cia ;
    linkml:definition_uri okns:daml_country_cia ;
    linkml:domain okns:Daml-countryCountry ;
    linkml:inlined true ;
    linkml:owner okns:daml_country_cia ;
    linkml:range okns:WfbGEOREF ;
    linkml:slot_uri daml-country:cia .

okns:daml_country_name a linkml:SlotDefinition ;
    skos:editorialNote "No occurrences of this slot in the graph." ;
    skos:inScheme okns:daml ;
    skos:mappingRelation daml-country:name ;
    linkml:definition_uri okns:daml_country_name ;
    linkml:domain okns:Daml-countryCountry ;
    linkml:inlined true ;
    linkml:owner okns:daml_country_name ;
    linkml:range okns:RdfsLiteral ;
    linkml:slot_uri daml-country:name .

okns:daml_domain a linkml:SlotDefinition ;
    skos:inScheme okns:daml ;
    skos:mappingRelation daml:domain ;
    linkml:definition_uri okns:daml_domain ;
    linkml:domain_of okns:DamlProperty ;
    linkml:inlined true ;
    linkml:owner okns:DamlProperty ;
    linkml:range okns:DamlClass ;
    linkml:slot_uri daml:domain .

okns:daml_imports a linkml:SlotDefinition ;
    skos:inScheme okns:daml ;
    skos:mappingRelation daml:imports ;
    linkml:any_of [ a okns:AnonymousSlotExpression ;
            linkml:range okns:uri ],
        [ a okns:AnonymousSlotExpression ;
            linkml:range okns:Daml-2001Ontology ],
        [ a okns:AnonymousSlotExpression ;
            linkml:range okns:DamlOntology ] ;
    linkml:definition_uri okns:daml_imports ;
    linkml:domain_of okns:DamlOntology ;
    linkml:inlined true ;
    linkml:owner okns:DamlOntology ;
    linkml:range okns:Any ;
    linkml:slot_uri daml:imports .

okns:daml_iso3166_code a linkml:SlotDefinition ;
    skos:inScheme okns:daml ;
    skos:mappingRelation daml-iso3166:code ;
    linkml:definition_uri okns:daml_iso3166_code ;
    linkml:domain_of okns:Daml-iso3166Country ;
    linkml:owner okns:Daml-iso3166Country ;
    linkml:range okns:string ;
    linkml:slot_uri daml-iso3166:code .

okns:daml_iso3166_name a linkml:SlotDefinition ;
    skos:inScheme okns:daml ;
    skos:mappingRelation daml-iso3166:name ;
    linkml:definition_uri okns:daml_iso3166_name ;
    linkml:domain_of okns:Daml-iso3166Country ;
    linkml:owner okns:Daml-iso3166Country ;
    linkml:range okns:string ;
    linkml:slot_uri daml-iso3166:name .

okns:daml_oil_cardinality a linkml:SlotDefinition ;
    dcterms:title "cardinality" ;
    skos:definition "for onProperty(R, P) and cardinality(R, n), read: i is in class R if and only if there are exactly n distinct j with P(i, j). cf OIL Cardinality" ;
    skos:editorialNote "No occurrences of this slot in the graph." ;
    skos:inScheme okns:daml ;
    skos:mappingRelation daml-oil:cardinality ;
    linkml:definition_uri okns:daml_oil_cardinality ;
    linkml:domain okns:Daml-oilRestriction ;
    linkml:inlined true ;
    linkml:owner okns:daml_oil_cardinality ;
    linkml:range okns:Xsd2000NonNegativeInteger ;
    linkml:slot_uri daml-oil:cardinality .

okns:daml_oil_cardinalityQ a linkml:SlotDefinition ;
    dcterms:title "cardinality" ;
    skos:definition "for onProperty(R, P), cardinalityQ(R, n) and hasClassQ(R, X), read: i is in class R if and only if there are exactly n distinct j with P(i, j) and type(j, X). cf OIL Cardinality" ;
    skos:editorialNote "No occurrences of this slot in the graph." ;
    skos:inScheme okns:daml ;
    skos:mappingRelation daml-oil:cardinalityQ ;
    linkml:definition_uri okns:daml_oil_cardinalityQ ;
    linkml:domain okns:Daml-oilRestriction ;
    linkml:inlined true ;
    linkml:owner okns:daml_oil_cardinalityQ ;
    linkml:range okns:Xsd2000NonNegativeInteger ;
    linkml:slot_uri daml-oil:cardinalityQ .

okns:daml_oil_complementOf a linkml:SlotDefinition ;
    dcterms:title "complementOf" ;
    skos:definition "for complementOf(X, Y) read: X is the complement of Y; if something is in Y, then it's not in X, and vice versa. cf OIL NOT" ;
    skos:editorialNote "No occurrences of this slot in the graph." ;
    skos:inScheme okns:daml ;
    skos:mappingRelation daml-oil:complementOf ;
    linkml:definition_uri okns:daml_oil_complementOf ;
    linkml:domain okns:Daml-oilClass ;
    linkml:inlined true ;
    linkml:owner okns:daml_oil_complementOf ;
    linkml:range okns:Daml-oilClass ;
    linkml:slot_uri daml-oil:complementOf .

okns:daml_oil_disjointUnionOf a linkml:SlotDefinition ;
    dcterms:title "disjointUnionOf" ;
    skos:definition "for disjointUnionOf(X, Y) read: X is the disjoint union of the classes in the list Y: (a) for any c1 and c2 in Y, disjointWith(c1, c2), and (b) unionOf(X, Y). i.e. if something is in any of the classes in Y, it's in X, and vice versa. cf OIL disjoint-covered" ;
    skos:editorialNote "No occurrences of this slot in the graph." ;
    skos:inScheme okns:daml ;
    skos:mappingRelation daml-oil:disjointUnionOf ;
    linkml:definition_uri okns:daml_oil_disjointUnionOf ;
    linkml:domain okns:Daml-oilClass ;
    linkml:inlined true ;
    linkml:owner okns:daml_oil_disjointUnionOf ;
    linkml:range okns:Daml-oilList ;
    linkml:slot_uri daml-oil:disjointUnionOf .

okns:daml_oil_disjointWith a linkml:SlotDefinition ;
    dcterms:title "disjointWith" ;
    skos:definition "for disjointWith(X, Y) read: X and Y have no members in common. cf OIL Disjoint" ;
    skos:editorialNote "No occurrences of this slot in the graph." ;
    skos:inScheme okns:daml ;
    skos:mappingRelation daml-oil:disjointWith ;
    linkml:definition_uri okns:daml_oil_disjointWith ;
    linkml:domain okns:Daml-oilClass ;
    linkml:inlined true ;
    linkml:owner okns:daml_oil_disjointWith ;
    linkml:range okns:Daml-oilClass ;
    linkml:slot_uri daml-oil:disjointWith .

okns:daml_oil_first a linkml:SlotDefinition ;
    skos:editorialNote "No occurrences of this slot in the graph." ;
    skos:inScheme okns:daml ;
    skos:mappingRelation daml-oil:first ;
    linkml:definition_uri okns:daml_oil_first ;
    linkml:domain okns:Daml-oilList ;
    linkml:inlined true ;
    linkml:owner okns:daml_oil_first ;
    linkml:range okns:Any ;
    linkml:slot_uri daml-oil:first .

okns:daml_oil_hasClass a linkml:SlotDefinition ;
    dcterms:title "hasClass" ;
    skos:definition "for onProperty(R, P) and hasClass(R, X), read: i is in class R if and only if for some j, P(i, j) and type(j, X). cf OIL HasValue" ;
    skos:editorialNote "No occurrences of this slot in the graph." ;
    skos:inScheme okns:daml ;
    skos:mappingRelation daml-oil:hasClass ;
    linkml:definition_uri okns:daml_oil_hasClass ;
    linkml:domain okns:Daml-oilRestriction ;
    linkml:inlined true ;
    linkml:owner okns:daml_oil_hasClass ;
    linkml:range okns:RdfsClass ;
    linkml:slot_uri daml-oil:hasClass .

okns:daml_oil_hasClassQ a linkml:SlotDefinition ;
    dcterms:title "hasClassQ" ;
    skos:definition "property for specifying class restriction with cardinalityQ constraints" ;
    skos:editorialNote "No occurrences of this slot in the graph." ;
    skos:inScheme okns:daml ;
    skos:mappingRelation daml-oil:hasClassQ ;
    linkml:definition_uri okns:daml_oil_hasClassQ ;
    linkml:domain okns:Daml-oilRestriction ;
    linkml:inlined true ;
    linkml:owner okns:daml_oil_hasClassQ ;
    linkml:range okns:RdfsClass ;
    linkml:slot_uri daml-oil:hasClassQ .

okns:daml_oil_hasValue a linkml:SlotDefinition ;
    dcterms:title "hasValue" ;
    skos:definition "for onProperty(R, P) and hasValue(R, V), read: i is in class R if and only if P(i, V). cf OIL HasFiller" ;
    skos:editorialNote "No occurrences of this slot in the graph." ;
    skos:inScheme okns:daml ;
    skos:mappingRelation daml-oil:hasValue ;
    linkml:definition_uri okns:daml_oil_hasValue ;
    linkml:domain okns:Daml-oilRestriction ;
    linkml:inlined true ;
    linkml:owner okns:daml_oil_hasValue ;
    linkml:range okns:Any ;
    linkml:slot_uri daml-oil:hasValue .

okns:daml_oil_imports a linkml:SlotDefinition ;
    dcterms:title "imports" ;
    skos:definition "for imports(X, Y) read: X imports Y; i.e. X asserts the* contents of Y by reference; i.e. if imports(X, Y) and you believe X and Y says something, then you should believe it. Note: \"the contents\" is, in the general case, an il-formed definite description. Different interactions with a resource may expose contents that vary with time, data format, preferred language, requestor credentials, etc. So for \"the contents\", read \"any contents\"." ;
    skos:inScheme okns:daml ;
    skos:mappingRelation daml-oil:imports ;
    linkml:any_of [ a okns:AnonymousSlotExpression ;
            linkml:range okns:uri ],
        [ a okns:AnonymousSlotExpression ;
            linkml:range okns:Daml-2001Ontology ] ;
    linkml:definition_uri okns:daml_oil_imports ;
    linkml:domain_of okns:Daml-oilOntology ;
    linkml:inlined true ;
    linkml:owner okns:Daml-oilOntology ;
    linkml:range okns:Any ;
    linkml:slot_uri daml-oil:imports .

okns:daml_oil_intersectionOf a linkml:SlotDefinition ;
    dcterms:title "intersectionOf" ;
    skos:definition "for intersectionOf(X, Y) read: X is the intersection of the classes in the list Y; i.e. if something is in all the classes in Y, then it's in X, and vice versa. cf OIL AND" ;
    skos:editorialNote "No occurrences of this slot in the graph." ;
    skos:inScheme okns:daml ;
    skos:mappingRelation daml-oil:intersectionOf ;
    linkml:definition_uri okns:daml_oil_intersectionOf ;
    linkml:domain okns:Daml-oilClass ;
    linkml:inlined true ;
    linkml:owner okns:daml_oil_intersectionOf ;
    linkml:range okns:Daml-oilList ;
    linkml:slot_uri daml-oil:intersectionOf .

okns:daml_oil_inverseOf a linkml:SlotDefinition ;
    dcterms:title "inverseOf" ;
    skos:definition "for inverseOf(R, S) read: R is the inverse of S; i.e. if R(x, y) then S(y, x) and vice versa. cf OIL inverseRelationOf" ;
    skos:editorialNote "No occurrences of this slot in the graph." ;
    skos:inScheme okns:daml ;
    skos:mappingRelation daml-oil:inverseOf ;
    linkml:definition_uri okns:daml_oil_inverseOf ;
    linkml:domain okns:Daml-oilObjectProperty ;
    linkml:inlined true ;
    linkml:owner okns:daml_oil_inverseOf ;
    linkml:range okns:Daml-oilObjectProperty ;
    linkml:slot_uri daml-oil:inverseOf .

okns:daml_oil_item a linkml:SlotDefinition ;
    skos:definition "for item(L, I) read: I is an item in L; either first(L, I) or item(R, I) where rest(L, R)." ;
    skos:editorialNote "No occurrences of this slot in the graph." ;
    skos:inScheme okns:daml ;
    skos:mappingRelation daml-oil:item ;
    linkml:definition_uri okns:daml_oil_item ;
    linkml:domain okns:Daml-oilList ;
    linkml:inlined true ;
    linkml:owner okns:daml_oil_item ;
    linkml:range okns:Any ;
    linkml:slot_uri daml-oil:item .

okns:daml_oil_maxCardinality a linkml:SlotDefinition ;
    dcterms:title "maxCardinality" ;
    skos:definition "for onProperty(R, P) and maxCardinality(R, n), read: i is in class R if and only if there are at most n distinct j with P(i, j). cf OIL MaxCardinality" ;
    skos:editorialNote "No occurrences of this slot in the graph." ;
    skos:inScheme okns:daml ;
    skos:mappingRelation daml-oil:maxCardinality ;
    linkml:definition_uri okns:daml_oil_maxCardinality ;
    linkml:domain okns:Daml-oilRestriction ;
    linkml:inlined true ;
    linkml:owner okns:daml_oil_maxCardinality ;
    linkml:range okns:Xsd2000NonNegativeInteger ;
    linkml:slot_uri daml-oil:maxCardinality .

okns:daml_oil_maxCardinalityQ a linkml:SlotDefinition ;
    dcterms:title "maxCardinality" ;
    skos:definition "for onProperty(R, P), maxCardinalityQ(R, n) and hasClassQ(R, X), read: i is in class R if and only if there are at most n distinct j with P(i, j) and type(j, X). cf OIL MaxCardinality" ;
    skos:editorialNote "No occurrences of this slot in the graph." ;
    skos:inScheme okns:daml ;
    skos:mappingRelation daml-oil:maxCardinalityQ ;
    linkml:definition_uri okns:daml_oil_maxCardinalityQ ;
    linkml:domain okns:Daml-oilRestriction ;
    linkml:inlined true ;
    linkml:owner okns:daml_oil_maxCardinalityQ ;
    linkml:range okns:Xsd2000NonNegativeInteger ;
    linkml:slot_uri daml-oil:maxCardinalityQ .

okns:daml_oil_minCardinality a linkml:SlotDefinition ;
    dcterms:title "minCardinality" ;
    skos:definition "for onProperty(R, P) and minCardinality(R, n), read: i is in class R if and only if there are at least n distinct j with P(i, j). cf OIL MinCardinality" ;
    skos:editorialNote "No occurrences of this slot in the graph." ;
    skos:inScheme okns:daml ;
    skos:mappingRelation daml-oil:minCardinality ;
    linkml:definition_uri okns:daml_oil_minCardinality ;
    linkml:domain okns:Daml-oilRestriction ;
    linkml:inlined true ;
    linkml:owner okns:daml_oil_minCardinality ;
    linkml:range okns:Xsd2000NonNegativeInteger ;
    linkml:slot_uri daml-oil:minCardinality .

okns:daml_oil_minCardinalityQ a linkml:SlotDefinition ;
    dcterms:title "minCardinality" ;
    skos:definition "for onProperty(R, P), minCardinalityQ(R, n) and hasClassQ(R, X), read: i is in class R if and only if there are at least n distinct j with P(i, j) and type(j, X). cf OIL MinCardinality" ;
    skos:editorialNote "No occurrences of this slot in the graph." ;
    skos:inScheme okns:daml ;
    skos:mappingRelation daml-oil:minCardinalityQ ;
    linkml:definition_uri okns:daml_oil_minCardinalityQ ;
    linkml:domain okns:Daml-oilRestriction ;
    linkml:inlined true ;
    linkml:owner okns:daml_oil_minCardinalityQ ;
    linkml:range okns:Xsd2000NonNegativeInteger ;
    linkml:slot_uri daml-oil:minCardinalityQ .

okns:daml_oil_onProperty a linkml:SlotDefinition ;
    dcterms:title "onProperty" ;
    skos:definition "for onProperty(R, P), read: R is a restricted with respect to property P." ;
    skos:editorialNote "No occurrences of this slot in the graph." ;
    skos:inScheme okns:daml ;
    skos:mappingRelation daml-oil:onProperty ;
    linkml:definition_uri okns:daml_oil_onProperty ;
    linkml:domain okns:Daml-oilRestriction ;
    linkml:inlined true ;
    linkml:owner okns:daml_oil_onProperty ;
    linkml:range okns:RdfProperty ;
    linkml:slot_uri daml-oil:onProperty .

okns:daml_oil_oneOf a linkml:SlotDefinition ;
    dcterms:title "oneOf" ;
    skos:definition "for oneOf(C, L) read everything in C is one of the things in L; This lets us define classes by enumerating the members. cf OIL OneOf" ;
    skos:editorialNote "No occurrences of this slot in the graph." ;
    skos:inScheme okns:daml ;
    skos:mappingRelation daml-oil:oneOf ;
    linkml:definition_uri okns:daml_oil_oneOf ;
    linkml:domain okns:Daml-oilClass ;
    linkml:inlined true ;
    linkml:owner okns:daml_oil_oneOf ;
    linkml:range okns:Daml-oilList ;
    linkml:slot_uri daml-oil:oneOf .

okns:daml_oil_rest a linkml:SlotDefinition ;
    skos:editorialNote "No occurrences of this slot in the graph." ;
    skos:inScheme okns:daml ;
    skos:mappingRelation daml-oil:rest ;
    linkml:definition_uri okns:daml_oil_rest ;
    linkml:domain okns:Daml-oilList ;
    linkml:inlined true ;
    linkml:owner okns:daml_oil_rest ;
    linkml:range okns:Daml-oilList ;
    linkml:slot_uri daml-oil:rest .

okns:daml_oil_seeAlso a linkml:SlotDefinition ;
    skos:editorialNote "No occurrences of this slot in the graph." ;
    skos:inScheme okns:daml ;
    skos:mappingRelation daml-oil:seeAlso ;
    linkml:definition_uri okns:daml_oil_seeAlso ;
    linkml:inlined true ;
    linkml:range okns:Any ;
    linkml:slot_uri daml-oil:seeAlso .

okns:daml_oil_toClass a linkml:SlotDefinition ;
    dcterms:title "toClass" ;
    skos:definition "for onProperty(R, P) and toClass(R, X), read: i is in class R if and only if for all j, P(i, j) implies type(j, X). cf OIL ValueType" ;
    skos:editorialNote "No occurrences of this slot in the graph." ;
    skos:inScheme okns:daml ;
    skos:mappingRelation daml-oil:toClass ;
    linkml:definition_uri okns:daml_oil_toClass ;
    linkml:domain okns:Daml-oilRestriction ;
    linkml:inlined true ;
    linkml:owner okns:daml_oil_toClass ;
    linkml:range okns:RdfsClass ;
    linkml:slot_uri daml-oil:toClass .

okns:daml_oil_unionOf a linkml:SlotDefinition ;
    dcterms:title "unionOf" ;
    skos:definition "for unionOf(X, Y) read: X is the union of the classes in the list Y; i.e. if something is in any of the classes in Y, it's in X, and vice versa. cf OIL OR" ;
    skos:editorialNote "No occurrences of this slot in the graph." ;
    skos:inScheme okns:daml ;
    skos:mappingRelation daml-oil:unionOf ;
    linkml:definition_uri okns:daml_oil_unionOf ;
    linkml:domain okns:Daml-oilClass ;
    linkml:inlined true ;
    linkml:owner okns:daml_oil_unionOf ;
    linkml:range okns:Daml-oilList ;
    linkml:slot_uri daml-oil:unionOf .

okns:daml_oil_versionInfo a linkml:SlotDefinition ;
    dcterms:title "versionInfo" ;
    skos:definition "generally, a string giving information about this version; e.g. RCS/CVS keywords" ;
    skos:inScheme okns:daml ;
    skos:mappingRelation daml-oil:versionInfo ;
    linkml:definition_uri okns:daml_oil_versionInfo ;
    linkml:domain_of okns:Daml-oilOntology ;
    linkml:owner okns:Daml-oilOntology ;
    linkml:range okns:string ;
    linkml:slot_uri daml-oil:versionInfo .

okns:daml_ont_borderstate a linkml:SlotDefinition ;
    skos:inScheme okns:daml ;
    skos:mappingRelation daml-ont:borderstate ;
    linkml:definition_uri okns:daml_ont_borderstate ;
    linkml:domain_of okns:Daml-ontUSState ;
    linkml:inlined true ;
    linkml:owner okns:Daml-ontUSState ;
    linkml:range okns:Daml-ontUSState ;
    linkml:slot_uri daml-ont:borderstate .

okns:daml_ont_capital a linkml:SlotDefinition ;
    skos:inScheme okns:daml ;
    skos:mappingRelation daml-ont:capital ;
    linkml:definition_uri okns:daml_ont_capital ;
    linkml:domain_of okns:Daml-ontUSState ;
    linkml:owner okns:Daml-ontUSState ;
    linkml:range okns:uri ;
    linkml:slot_uri daml-ont:capital .

okns:daml_ont_cia a linkml:SlotDefinition ;
    skos:inScheme okns:daml ;
    skos:mappingRelation daml-ont:cia ;
    linkml:definition_uri okns:daml_ont_cia ;
    linkml:domain_of okns:Daml-ontCountry ;
    linkml:owner okns:Daml-ontCountry ;
    linkml:range okns:uri ;
    linkml:slot_uri daml-ont:cia .

okns:daml_ont_code a linkml:SlotDefinition ;
    skos:inScheme okns:daml ;
    skos:mappingRelation daml-ont:code ;
    linkml:definition_uri okns:daml_ont_code ;
    linkml:domain_of okns:Daml-ontUSState ;
    linkml:owner okns:Daml-ontUSState ;
    linkml:range okns:string ;
    linkml:slot_uri daml-ont:code .

okns:daml_ont_memberstate a linkml:SlotDefinition ;
    skos:inScheme okns:daml ;
    skos:mappingRelation daml-ont:memberstate ;
    linkml:definition_uri okns:daml_ont_memberstate ;
    linkml:domain_of okns:Daml-ontUSRegion ;
    linkml:inlined true ;
    linkml:owner okns:Daml-ontUSRegion ;
    linkml:range okns:Daml-ontUSState ;
    linkml:slot_uri daml-ont:memberstate .

okns:daml_ont_region a linkml:SlotDefinition ;
    skos:inScheme okns:daml ;
    skos:mappingRelation daml-ont:region ;
    linkml:definition_uri okns:daml_ont_region ;
    linkml:domain_of okns:Daml-ontUSState ;
    linkml:inlined true ;
    linkml:owner okns:Daml-ontUSState ;
    linkml:range okns:Daml-ontUSRegion ;
    linkml:slot_uri daml-ont:region .

okns:daml_range a linkml:SlotDefinition ;
    skos:inScheme okns:daml ;
    skos:mappingRelation daml:range ;
    linkml:definition_uri okns:daml_range ;
    linkml:domain_of okns:DamlProperty ;
    linkml:inlined true ;
    linkml:owner okns:DamlProperty ;
    linkml:range okns:DamlClass ;
    linkml:slot_uri daml:range .

okns:daml_samePropertyAs a linkml:SlotDefinition ;
    skos:inScheme okns:daml ;
    skos:mappingRelation daml:samePropertyAs ;
    linkml:definition_uri okns:daml_samePropertyAs ;
    linkml:domain_of okns:DamlProperty ;
    linkml:owner okns:DamlProperty ;
    linkml:range okns:uri ;
    linkml:slot_uri daml:samePropertyAs .

okns:daml_state_borderstate a linkml:SlotDefinition ;
    skos:editorialNote "No occurrences of this slot in the graph." ;
    skos:inScheme okns:daml ;
    skos:mappingRelation daml-state:borderstate ;
    linkml:definition_uri okns:daml_state_borderstate ;
    linkml:domain okns:Daml-stateState ;
    linkml:inlined true ;
    linkml:owner okns:daml_state_borderstate ;
    linkml:range okns:Daml-stateState ;
    linkml:slot_uri daml-state:borderstate .

okns:daml_state_capital a linkml:SlotDefinition ;
    skos:editorialNote "No occurrences of this slot in the graph." ;
    skos:inScheme okns:daml ;
    skos:mappingRelation daml-state:capital ;
    linkml:definition_uri okns:daml_state_capital ;
    linkml:domain okns:Daml-stateState ;
    linkml:inlined true ;
    linkml:owner okns:daml_state_capital ;
    linkml:range okns:Daml-cityCity ;
    linkml:slot_uri daml-state:capital .

okns:daml_state_code a linkml:SlotDefinition ;
    skos:editorialNote "No occurrences of this slot in the graph." ;
    skos:inScheme okns:daml ;
    skos:mappingRelation daml-state:code ;
    linkml:definition_uri okns:daml_state_code ;
    linkml:domain okns:Daml-stateState ;
    linkml:inlined true ;
    linkml:owner okns:daml_state_code ;
    linkml:range okns:RdfsLiteral ;
    linkml:slot_uri daml-state:code .

okns:daml_state_country a linkml:SlotDefinition ;
    skos:editorialNote "No occurrences of this slot in the graph." ;
    skos:inScheme okns:daml ;
    skos:mappingRelation daml-state:country ;
    linkml:any_of [ a okns:AnonymousSlotExpression ;
            linkml:range okns:Daml-countryCountry ],
        [ a okns:AnonymousSlotExpression ;
            linkml:range okns:Daml-countryUNITED-STATES ] ;
    linkml:definition_uri okns:daml_state_country ;
    linkml:domain okns:Daml-stateState ;
    linkml:inlined true ;
    linkml:owner okns:daml_state_country ;
    linkml:range okns:Any ;
    linkml:slot_uri daml-state:country .

okns:daml_state_name a linkml:SlotDefinition ;
    skos:editorialNote "No occurrences of this slot in the graph." ;
    skos:inScheme okns:daml ;
    skos:mappingRelation daml-state:name ;
    linkml:definition_uri okns:daml_state_name ;
    linkml:domain okns:Daml-stateState ;
    linkml:inlined true ;
    linkml:owner okns:daml_state_name ;
    linkml:range okns:RdfsLiteral ;
    linkml:slot_uri daml-state:name .

okns:daml_subClassOf a linkml:SlotDefinition ;
    skos:inScheme okns:daml ;
    skos:mappingRelation daml:subClassOf ;
    linkml:any_of [ a okns:AnonymousSlotExpression ;
            linkml:range okns:DamlClass ],
        [ a okns:AnonymousSlotExpression ;
            linkml:range okns:uri ] ;
    linkml:definition_uri okns:daml_subClassOf ;
    linkml:domain_of okns:DamlClass ;
    linkml:inlined true ;
    linkml:owner okns:DamlClass ;
    linkml:range okns:Any ;
    linkml:slot_uri daml:subClassOf .

okns:daml_subPropertyOf a linkml:SlotDefinition ;
    skos:inScheme okns:daml ;
    skos:mappingRelation daml:subPropertyOf ;
    linkml:any_of [ a okns:AnonymousSlotExpression ;
            linkml:range okns:DamlProperty ],
        [ a okns:AnonymousSlotExpression ;
            linkml:range okns:uri ] ;
    linkml:definition_uri okns:daml_subPropertyOf ;
    linkml:domain_of okns:DamlProperty ;
    linkml:inlined true ;
    linkml:owner okns:DamlProperty ;
    linkml:range okns:Any ;
    linkml:slot_uri daml:subPropertyOf .

okns:daml_usregionstate_memberstate a linkml:SlotDefinition ;
    skos:editorialNote "No occurrences of this slot in the graph." ;
    skos:inScheme okns:daml ;
    skos:mappingRelation daml-usregionstate:memberstate ;
    linkml:definition_uri okns:daml_usregionstate_memberstate ;
    linkml:domain okns:Daml-usregionstateUSRegion ;
    linkml:inlined true ;
    linkml:owner okns:daml_usregionstate_memberstate ;
    linkml:range okns:Daml-usregionstateUSState ;
    linkml:slot_uri daml-usregionstate:memberstate .

okns:daml_usregionstate_region a linkml:SlotDefinition ;
    skos:editorialNote "No occurrences of this slot in the graph." ;
    skos:inScheme okns:daml ;
    skos:mappingRelation daml-usregionstate:region ;
    linkml:definition_uri okns:daml_usregionstate_region ;
    linkml:domain okns:Daml-usregionstateUSState ;
    linkml:inlined true ;
    linkml:owner okns:daml_usregionstate_region ;
    linkml:range okns:Daml-usregionstateUSRegion ;
    linkml:slot_uri daml-usregionstate:region .

okns:daml_versionInfo a linkml:SlotDefinition ;
    skos:inScheme okns:daml ;
    skos:mappingRelation daml:versionInfo ;
    linkml:definition_uri okns:daml_versionInfo ;
    linkml:domain_of okns:DamlOntology ;
    linkml:owner okns:DamlOntology ;
    linkml:range okns:string ;
    linkml:slot_uri daml:versionInfo .

okns:dc_contributor a linkml:SlotDefinition ;
    dcterms:source dc: ;
    dcterms:title "Contributor" ;
    skos:definition "The guidelines for using names of persons or organizations as creators also apply to contributors.  Typically, the name of a Contributor should be used to indicate the entity." ;
    skos:editorialNote "A [second property](/specifications/dublin-core/dcmi-terms/#http://purl.org/dc/terms/contributor) with the same name as this property has been declared in the [dcterms: namespace](http://purl.org/dc/terms/).  See the Introduction to the document [DCMI Metadata Terms](/specifications/dublin-core/dcmi-terms/) for an explanation.",
        "No occurrences of this slot in the graph." ;
    skos:inScheme okns:dc ;
    skos:mappingRelation dc:contributor ;
    skos:note "description: An entity responsible for making contributions to the resource." ;
    linkml:definition_uri okns:dc_contributor ;
    linkml:inlined true ;
    linkml:range okns:Any ;
    linkml:slot_uri dc:contributor .

okns:dc_coverage a linkml:SlotDefinition ;
    dcterms:source dc: ;
    dcterms:title "Coverage" ;
    skos:definition "Spatial topic and spatial applicability may be a named place or a location specified by its geographic coordinates. Temporal topic may be a named period, date, or date range. A jurisdiction may be a named administrative entity or a geographic place to which the resource applies. Recommended practice is to use a controlled vocabulary such as the Getty Thesaurus of Geographic Names [[TGN](https://www.getty.edu/research/tools/vocabulary/tgn/index.html)]. Where appropriate, named places or time periods may be used in preference to numeric identifiers such as sets of coordinates or date ranges." ;
    skos:editorialNote "A [second property](/specifications/dublin-core/dcmi-terms/#http://purl.org/dc/terms/coverage) with the same name as this property has been declared in the [dcterms: namespace](http://purl.org/dc/terms/).  See the Introduction to the document [DCMI Metadata Terms](/specifications/dublin-core/dcmi-terms/) for an explanation.",
        "No occurrences of this slot in the graph." ;
    skos:inScheme okns:dc ;
    skos:mappingRelation dc:coverage ;
    skos:note "description: The spatial or temporal topic of the resource, spatial applicability of the resource, or jurisdiction under which the resource is relevant." ;
    linkml:definition_uri okns:dc_coverage ;
    linkml:inlined true ;
    linkml:range okns:Any ;
    linkml:slot_uri dc:coverage .

okns:dc_date a linkml:SlotDefinition ;
    dcterms:source dc: ;
    dcterms:title "Date" ;
    skos:definition "Date may be used to express temporal information at any level of granularity.  Recommended practice is to express the date, date/time, or period of time according to ISO 8601-1 [[ISO 8601-1](https://www.iso.org/iso-8601-date-and-time-format.html)] or a published profile of the ISO standard, such as the W3C Note on Date and Time Formats [[W3CDTF](https://www.w3.org/TR/NOTE-datetime)] or the Extended Date/Time Format Specification [[EDTF](http://www.loc.gov/standards/datetime/)].  If the full date is unknown, month and year (YYYY-MM) or just year (YYYY) may be used. Date ranges may be specified using ISO 8601 period of time specification in which start and end dates are separated by a '/' (slash) character.  Either the start or end date may be missing." ;
    skos:editorialNote "A [second property](/specifications/dublin-core/dcmi-terms/#http://purl.org/dc/terms/date) with the same name as this property has been declared in the [dcterms: namespace](http://purl.org/dc/terms/).  See the Introduction to the document [DCMI Metadata Terms](/specifications/dublin-core/dcmi-terms/) for an explanation.",
        "No occurrences of this slot in the graph." ;
    skos:inScheme okns:dc ;
    skos:mappingRelation dc:date ;
    skos:note "description: A point or period of time associated with an event in the lifecycle of the resource." ;
    linkml:definition_uri okns:dc_date ;
    linkml:inlined true ;
    linkml:range okns:Any ;
    linkml:slot_uri dc:date .

okns:dc_format a linkml:SlotDefinition ;
    dcterms:source dc: ;
    dcterms:title "Format" ;
    skos:definition "Recommended practice is to use a controlled vocabulary where available. For example, for file formats one could use the list of Internet Media Types [[MIME](https://www.iana.org/assignments/media-types/media-types.xhtml)]." ;
    skos:editorialNote "A [second property](/specifications/dublin-core/dcmi-terms/#http://purl.org/dc/terms/format) with the same name as this property has been declared in the [dcterms: namespace](http://purl.org/dc/terms/).  See the Introduction to the document [DCMI Metadata Terms](/specifications/dublin-core/dcmi-terms/) for an explanation.",
        "No occurrences of this slot in the graph." ;
    skos:inScheme okns:dc ;
    skos:mappingRelation dc:format ;
    skos:note "description: The file format, physical medium, or dimensions of the resource." ;
    linkml:definition_uri okns:dc_format ;
    linkml:inlined true ;
    linkml:range okns:Any ;
    linkml:slot_uri dc:format .

okns:dc_identifier a linkml:SlotDefinition ;
    dcterms:source dc: ;
    dcterms:title "Identifier" ;
    skos:definition "Recommended practice is to identify the resource by means of a string conforming to an identification system." ;
    skos:editorialNote "A [second property](/specifications/dublin-core/dcmi-terms/#http://purl.org/dc/terms/identifier) with the same name as this property has been declared in the [dcterms: namespace](http://purl.org/dc/terms/).  See the Introduction to the document [DCMI Metadata Terms](/specifications/dublin-core/dcmi-terms/) for an explanation.",
        "No occurrences of this slot in the graph." ;
    skos:inScheme okns:dc ;
    skos:mappingRelation dc:identifier ;
    skos:note "description: An unambiguous reference to the resource within a given context." ;
    linkml:definition_uri okns:dc_identifier ;
    linkml:inlined true ;
    linkml:range okns:Any ;
    linkml:slot_uri dc:identifier .

okns:dc_language a linkml:SlotDefinition ;
    dcterms:source dc: ;
    dcterms:title "Language" ;
    skos:definition "Recommended practice is to use either a non-literal value representing a language from a controlled vocabulary such as ISO 639-2 or ISO 639-3, or a literal value consisting of an IETF Best Current Practice 47 [[IETF-BCP47](https://tools.ietf.org/html/bcp47)] language tag." ;
    skos:editorialNote "A [second property](/specifications/dublin-core/dcmi-terms/#http://purl.org/dc/terms/language) with the same name as this property has been declared in the [dcterms: namespace](http://purl.org/dc/terms/).  See the Introduction to the document [DCMI Metadata Terms](/specifications/dublin-core/dcmi-terms/) for an explanation.",
        "No occurrences of this slot in the graph." ;
    skos:inScheme okns:dc ;
    skos:mappingRelation dc:language ;
    skos:note "description: A language of the resource." ;
    linkml:definition_uri okns:dc_language ;
    linkml:inlined true ;
    linkml:range okns:Any ;
    linkml:slot_uri dc:language .

okns:dc_publisher a linkml:SlotDefinition ;
    dcterms:source dc: ;
    dcterms:title "Publisher" ;
    skos:definition "Examples of a Publisher include a person, an organization, or a service. Typically, the name of a Publisher should be used to indicate the entity." ;
    skos:editorialNote "A [second property](/specifications/dublin-core/dcmi-terms/#http://purl.org/dc/terms/publisher) with the same name as this property has been declared in the [dcterms: namespace](http://purl.org/dc/terms/).  See the Introduction to the document [DCMI Metadata Terms](/specifications/dublin-core/dcmi-terms/) for an explanation.",
        "No occurrences of this slot in the graph." ;
    skos:inScheme okns:dc ;
    skos:mappingRelation dc:publisher ;
    skos:note "description: An entity responsible for making the resource available." ;
    linkml:definition_uri okns:dc_publisher ;
    linkml:inlined true ;
    linkml:range okns:Any ;
    linkml:slot_uri dc:publisher .

okns:dc_relation a linkml:SlotDefinition ;
    dcterms:source dc: ;
    dcterms:title "Relation" ;
    skos:definition "Recommended practice is to identify the related resource by means of a URI. If this is not possible or feasible, a string conforming to a formal identification system may be provided." ;
    skos:editorialNote "A [second property](/specifications/dublin-core/dcmi-terms/#http://purl.org/dc/terms/relation) with the same name as this property has been declared in the [dcterms: namespace](http://purl.org/dc/terms/).  See the Introduction to the document [DCMI Metadata Terms](/specifications/dublin-core/dcmi-terms/) for an explanation.",
        "No occurrences of this slot in the graph." ;
    skos:inScheme okns:dc ;
    skos:mappingRelation dc:relation ;
    skos:note "description: A related resource." ;
    linkml:definition_uri okns:dc_relation ;
    linkml:inlined true ;
    linkml:range okns:Any ;
    linkml:slot_uri dc:relation .

okns:dc_rights a linkml:SlotDefinition ;
    dcterms:source dc: ;
    dcterms:title "Rights" ;
    skos:definition "Typically, rights information includes a statement about various property rights associated with the resource, including intellectual property rights." ;
    skos:editorialNote "A [second property](/specifications/dublin-core/dcmi-terms/#http://purl.org/dc/terms/rights) with the same name as this property has been declared in the [dcterms: namespace](http://purl.org/dc/terms/).  See the Introduction to the document [DCMI Metadata Terms](/specifications/dublin-core/dcmi-terms/) for an explanation.",
        "No occurrences of this slot in the graph." ;
    skos:inScheme okns:dc ;
    skos:mappingRelation dc:rights ;
    skos:note "description: Information about rights held in and over the resource." ;
    linkml:definition_uri okns:dc_rights ;
    linkml:inlined true ;
    linkml:range okns:Any ;
    linkml:slot_uri dc:rights .

okns:dc_subject a linkml:SlotDefinition ;
    dcterms:source dc: ;
    dcterms:title "Subject" ;
    skos:definition "Typically, the subject will be represented using keywords, key phrases, or classification codes.  Recommended best practice is to use a controlled vocabulary." ;
    skos:editorialNote "A [second property](/specifications/dublin-core/dcmi-terms/#http://purl.org/dc/terms/subject) with the same name as this property has been declared in the [dcterms: namespace](http://purl.org/dc/terms/).  See the Introduction to the document [DCMI Metadata Terms](/specifications/dublin-core/dcmi-terms/) for an explanation.",
        "No occurrences of this slot in the graph." ;
    skos:inScheme okns:dc ;
    skos:mappingRelation dc:subject ;
    skos:note "description: The topic of the resource." ;
    linkml:definition_uri okns:dc_subject ;
    linkml:inlined true ;
    linkml:range okns:Any ;
    linkml:slot_uri dc:subject .

okns:dc_type a linkml:SlotDefinition ;
    dcterms:source dc: ;
    dcterms:title "Type" ;
    skos:definition "Recommended practice is to use a controlled vocabulary such as the DCMI Type Vocabulary [[DCMI-TYPE](http://dublincore.org/documents/dcmi-type-vocabulary/)]. To describe the file format, physical medium, or dimensions of the resource, use the Format element." ;
    skos:editorialNote "A [second property](/specifications/dublin-core/dcmi-terms/#http://purl.org/dc/terms/type) with the same name as this property has been declared in the [dcterms: namespace](http://purl.org/dc/terms/).  See the Introduction to the document [DCMI Metadata Terms](/specifications/dublin-core/dcmi-terms/) for an explanation.",
        "No occurrences of this slot in the graph." ;
    skos:inScheme okns:dc ;
    skos:mappingRelation dc:type ;
    skos:note "description: The nature or genre of the resource." ;
    linkml:definition_uri okns:dc_type ;
    linkml:inlined true ;
    linkml:range okns:Any ;
    linkml:slot_uri dc:type .

okns:dct_accrualMethod a linkml:SlotDefinition ;
    dcterms:source dcterms: ;
    dcterms:title "Accrual Method" ;
    skos:definition "Recommended practice is to use a value from the Collection Description Accrual Method Vocabulary [[DCMI-ACCRUALMETHOD](https://dublincore.org/groups/collections/accrual-method/)]." ;
    skos:editorialNote "No occurrences of this slot in the graph." ;
    skos:inScheme okns:dc ;
    skos:mappingRelation dcterms:accrualMethod ;
    skos:note "description: The method by which items are added to a collection." ;
    linkml:definition_uri okns:dct_accrualMethod ;
    linkml:domain okns:DcmitypeCollection ;
    linkml:inlined true ;
    linkml:owner okns:dct_accrualMethod ;
    linkml:range okns:Any ;
    linkml:slot_uri dcterms:accrualMethod .

okns:dct_accrualPeriodicity a linkml:SlotDefinition ;
    dcterms:source dcterms: ;
    dcterms:title "Accrual Periodicity" ;
    skos:definition "Recommended practice is to use a value from the Collection Description Frequency Vocabulary [[DCMI-COLLFREQ](https://dublincore.org/groups/collections/frequency/)]." ;
    skos:editorialNote "No occurrences of this slot in the graph." ;
    skos:inScheme okns:dc ;
    skos:mappingRelation dcterms:accrualPeriodicity ;
    skos:note "description: The frequency with which items are added to a collection." ;
    linkml:definition_uri okns:dct_accrualPeriodicity ;
    linkml:domain okns:DcmitypeCollection ;
    linkml:inlined true ;
    linkml:owner okns:dct_accrualPeriodicity ;
    linkml:range okns:Any ;
    linkml:slot_uri dcterms:accrualPeriodicity .

okns:dct_accrualPolicy a linkml:SlotDefinition ;
    dcterms:source dcterms: ;
    dcterms:title "Accrual Policy" ;
    skos:definition "Recommended practice is to use a value from the Collection Description Accrual Policy Vocabulary [[DCMI-ACCRUALPOLICY](https://dublincore.org/groups/collections/accrual-policy/)]." ;
    skos:editorialNote "No occurrences of this slot in the graph." ;
    skos:inScheme okns:dc ;
    skos:mappingRelation dcterms:accrualPolicy ;
    skos:note "description: The policy governing the addition of items to a collection." ;
    linkml:definition_uri okns:dct_accrualPolicy ;
    linkml:domain okns:DcmitypeCollection ;
    linkml:inlined true ;
    linkml:owner okns:dct_accrualPolicy ;
    linkml:range okns:Any ;
    linkml:slot_uri dcterms:accrualPolicy .

okns:dct_contributor a linkml:SlotDefinition ;
    dcterms:source dcterms: ;
    dcterms:title "Contributor" ;
    rdfs:subPropertyOf okns:dc_contributor ;
    skos:definition "The guidelines for using names of persons or organizations as creators apply to contributors." ;
    skos:editorialNote "No occurrences of this slot in the graph." ;
    skos:inScheme okns:dc ;
    skos:mappingRelation dcterms:contributor ;
    skos:note "description: An entity responsible for making contributions to the resource." ;
    linkml:definition_uri okns:dct_contributor ;
    linkml:inlined true ;
    linkml:range okns:Any ;
    linkml:slot_uri dcterms:contributor .

okns:dct_license a linkml:SlotDefinition ;
    dcterms:source dcterms: ;
    dcterms:title "License" ;
    rdfs:subPropertyOf okns:dct_rights ;
    skos:definition "Recommended practice is to identify the license document with a URI. If this is not possible or feasible, a literal value that identifies the license may be provided." ;
    skos:editorialNote "No occurrences of this slot in the graph." ;
    skos:inScheme okns:dc ;
    skos:mappingRelation dcterms:license ;
    skos:note "description: A legal document giving official permission to do something with the resource." ;
    linkml:definition_uri okns:dct_license ;
    linkml:inlined true ;
    linkml:range okns:Any ;
    linkml:slot_uri dcterms:license .

okns:dct_source a linkml:SlotDefinition ;
    dcterms:source dcterms: ;
    dcterms:title "Source" ;
    rdfs:subPropertyOf okns:dct_relation ;
    skos:definition "This property is intended to be used with non-literal values. The described resource may be derived from the related resource in whole or in part. Best practice is to identify the related resource by means of a URI or a string conforming to a formal identification system." ;
    skos:editorialNote "No occurrences of this slot in the graph." ;
    skos:inScheme okns:dc ;
    skos:mappingRelation dcterms:source ;
    skos:note "description: A related resource from which the described resource is derived." ;
    linkml:definition_uri okns:dct_source ;
    linkml:inlined true ;
    linkml:range okns:Any ;
    linkml:slot_uri dcterms:source .

okns:dct_title a linkml:SlotDefinition ;
    dcterms:source dcterms: ;
    dcterms:title "Title" ;
    rdfs:subPropertyOf okns:dc_title ;
    skos:definition "A name given to the resource." ;
    skos:inScheme okns:dc ;
    skos:mappingRelation dcterms:title ;
    linkml:any_of [ a okns:AnonymousSlotExpression ;
            linkml:range okns:RdfsLiteral ],
        [ a okns:AnonymousSlotExpression ;
            linkml:range okns:string ] ;
    linkml:definition_uri okns:dct_title ;
    linkml:inlined true ;
    linkml:range okns:Any ;
    linkml:slot_uri dcterms:title .

okns:event_agent_in a linkml:SlotDefinition ;
    owl:inverseOf okns:event_agent ;
    skos:editorialNote "No occurrences of this slot in the graph." ;
    skos:inScheme okns:event ;
    skos:mappingRelation event:agent_in ;
    linkml:definition_uri okns:event_agent_in ;
    linkml:domain okns:FoafAgent ;
    linkml:inlined true ;
    linkml:range okns:Any ;
    linkml:slot_uri event:agent_in .

okns:event_factor_of a linkml:SlotDefinition ;
    owl:inverseOf okns:event_factor ;
    skos:editorialNote "No occurrences of this slot in the graph." ;
    skos:inScheme okns:event ;
    skos:mappingRelation event:factor_of ;
    linkml:definition_uri okns:event_factor_of ;
    linkml:domain okns:Any ;
    linkml:inlined true ;
    linkml:range okns:Any ;
    linkml:slot_uri event:factor_of .

okns:event_literal_factor a linkml:SlotDefinition ;
    dcterms:title "literal factor" ;
    skos:definition "Relates an event to a factor which can be described as a literal. This property␊		should not be used as-is, but should be subsumed by other, more specific, properties␊		(like an hypothetic :weatherCelsius, linking an event to a temperature)." ;
    skos:editorialNote "No occurrences of this slot in the graph." ;
    skos:exactMatch event:hasLiteralFactor ;
    skos:inScheme okns:event ;
    skos:mappingRelation event:literal_factor ;
    linkml:definition_uri okns:event_literal_factor ;
    linkml:domain okns:EventEvent ;
    linkml:inlined true ;
    linkml:owner okns:event_literal_factor ;
    linkml:range okns:Any ;
    linkml:slot_uri event:literal_factor .

okns:event_place a linkml:SlotDefinition ;
    dcterms:title "place" ;
    skos:definition "Relates an event to a spatial object." ;
    skos:editorialNote "No occurrences of this slot in the graph." ;
    skos:inScheme okns:event ;
    skos:mappingRelation event:place ;
    linkml:definition_uri okns:event_place ;
    linkml:domain okns:EventEvent ;
    linkml:inlined true ;
    linkml:owner okns:event_place ;
    linkml:range okns:WgsSpatialThing ;
    linkml:slot_uri event:place .

okns:event_producedIn a linkml:SlotDefinition ;
    dcterms:title "produced in" ;
    skos:editorialNote "No occurrences of this slot in the graph." ;
    skos:exactMatch event:produced_in ;
    skos:inScheme okns:event ;
    skos:mappingRelation event:producedIn ;
    linkml:definition_uri okns:event_producedIn ;
    linkml:inlined true ;
    linkml:range okns:Any ;
    linkml:slot_uri event:producedIn .

okns:event_produced_in a linkml:SlotDefinition ;
    owl:inverseOf okns:event_product ;
    skos:editorialNote "No occurrences of this slot in the graph." ;
    skos:inScheme okns:event ;
    skos:mappingRelation event:produced_in ;
    linkml:definition_uri okns:event_produced_in ;
    linkml:domain okns:Any ;
    linkml:inlined true ;
    linkml:range okns:Any ;
    linkml:slot_uri event:produced_in .

okns:event_sub_event a linkml:SlotDefinition ;
    dcterms:title "sub-event" ;
    skos:definition "This property provides a way to split a complex event (for example, a performance involving several ␊		musicians) into simpler ones (one event per musician)." ;
    skos:editorialNote "No occurrences of this slot in the graph." ;
    skos:exactMatch event:hasSubEvent ;
    skos:inScheme okns:event ;
    skos:mappingRelation event:sub_event ;
    linkml:definition_uri okns:event_sub_event ;
    linkml:domain okns:EventEvent ;
    linkml:inlined true ;
    linkml:owner okns:event_sub_event ;
    linkml:range okns:EventEvent ;
    linkml:slot_uri event:sub_event .

okns:event_time a linkml:SlotDefinition ;
    dcterms:title "time" ;
    skos:definition "Relates an event to a time object, classifying a time region (either instantaneous or having an extent).␊		By using the Timeline ontology here, you can define event happening on a recorded track or on any ␊		media with a temporal extent." ;
    skos:editorialNote "No occurrences of this slot in the graph." ;
    skos:inScheme okns:event ;
    skos:mappingRelation event:time ;
    linkml:definition_uri okns:event_time ;
    linkml:domain okns:EventEvent ;
    linkml:inlined true ;
    linkml:owner okns:event_time ;
    linkml:range okns:TimeTemporalEntity ;
    linkml:slot_uri event:time .

okns:foaf_account a linkml:SlotDefinition ;
    dcterms:source foaf: ;
    dcterms:title "account" ;
    skos:definition "Indicates an account held by this agent." ;
    skos:editorialNote "No occurrences of this slot in the graph." ;
    skos:inScheme okns:foaf ;
    skos:mappingRelation foaf:account ;
    linkml:definition_uri okns:foaf_account ;
    linkml:domain okns:FoafAgent ;
    linkml:inlined true ;
    linkml:owner okns:foaf_account ;
    linkml:range okns:FoafOnlineAccount ;
    linkml:slot_uri foaf:account .

okns:foaf_accountName a linkml:SlotDefinition ;
    dcterms:source foaf: ;
    dcterms:title "account name" ;
    skos:definition "Indicates the name (identifier) associated with this online account." ;
    skos:editorialNote "No occurrences of this slot in the graph." ;
    skos:inScheme okns:foaf ;
    skos:mappingRelation foaf:accountName ;
    linkml:definition_uri okns:foaf_accountName ;
    linkml:domain okns:FoafOnlineAccount ;
    linkml:inlined true ;
    linkml:owner okns:foaf_accountName ;
    linkml:range okns:RdfsLiteral ;
    linkml:slot_uri foaf:accountName .

okns:foaf_accountServiceHomepage a linkml:SlotDefinition ;
    dcterms:source foaf: ;
    dcterms:title "account service homepage" ;
    skos:definition "Indicates a homepage of the service provide for this online account." ;
    skos:editorialNote "No occurrences of this slot in the graph." ;
    skos:inScheme okns:foaf ;
    skos:mappingRelation foaf:accountServiceHomepage ;
    linkml:definition_uri okns:foaf_accountServiceHomepage ;
    linkml:domain okns:FoafOnlineAccount ;
    linkml:inlined true ;
    linkml:owner okns:foaf_accountServiceHomepage ;
    linkml:range okns:FoafDocument ;
    linkml:slot_uri foaf:accountServiceHomepage .

okns:foaf_age a linkml:SlotDefinition ;
    dcterms:source foaf: ;
    dcterms:title "age" ;
    skos:definition "The age in years of some agent." ;
    skos:editorialNote "No occurrences of this slot in the graph." ;
    skos:inScheme okns:foaf ;
    skos:mappingRelation foaf:age ;
    linkml:definition_uri okns:foaf_age ;
    linkml:domain okns:FoafAgent ;
    linkml:inlined true ;
    linkml:owner okns:foaf_age ;
    linkml:range okns:RdfsLiteral ;
    linkml:slot_uri foaf:age .

okns:foaf_aimChatID a linkml:SlotDefinition ;
    dcterms:source foaf: ;
    dcterms:title "AIM chat ID" ;
    rdfs:subPropertyOf okns:foaf_nick ;
    skos:definition "An AIM chat ID" ;
    skos:editorialNote "No occurrences of this slot in the graph." ;
    skos:inScheme okns:foaf ;
    skos:mappingRelation foaf:aimChatID ;
    linkml:definition_uri okns:foaf_aimChatID ;
    linkml:domain okns:FoafAgent ;
    linkml:inlined true ;
    linkml:owner okns:foaf_aimChatID ;
    linkml:range okns:RdfsLiteral ;
    linkml:slot_uri foaf:aimChatID .

okns:foaf_based_near a linkml:SlotDefinition ;
    dcterms:title "No slot (predicate) name specified -- this slot is noted as a subproperty of another slot in this graph but has not itself been defined." ;
    skos:editorialNote "No occurrences of this slot in the graph." ;
    skos:inScheme okns:wgs ;
    skos:mappingRelation foaf:based_near ;
    linkml:definition_uri okns:foaf_based_near ;
    linkml:inlined true ;
    linkml:range okns:Any ;
    linkml:slot_uri foaf:based_near .

okns:foaf_birthday a linkml:SlotDefinition ;
    dcterms:source foaf: ;
    dcterms:title "birthday" ;
    skos:definition "The birthday of this Agent, represented in mm-dd string form, eg. '12-31'." ;
    skos:editorialNote "No occurrences of this slot in the graph." ;
    skos:inScheme okns:foaf ;
    skos:mappingRelation foaf:birthday ;
    linkml:definition_uri okns:foaf_birthday ;
    linkml:domain okns:FoafAgent ;
    linkml:inlined true ;
    linkml:owner okns:foaf_birthday ;
    linkml:range okns:RdfsLiteral ;
    linkml:slot_uri foaf:birthday .

okns:foaf_currentProject a linkml:SlotDefinition ;
    dcterms:source foaf: ;
    dcterms:title "current project" ;
    skos:definition "A current project this person works on." ;
    skos:editorialNote "No occurrences of this slot in the graph." ;
    skos:inScheme okns:foaf ;
    skos:mappingRelation foaf:currentProject ;
    linkml:definition_uri okns:foaf_currentProject ;
    linkml:domain okns:FoafPerson ;
    linkml:inlined true ;
    linkml:owner okns:foaf_currentProject ;
    linkml:range okns:OwlThing ;
    linkml:slot_uri foaf:currentProject .

okns:foaf_familyName a linkml:SlotDefinition ;
    dcterms:source foaf: ;
    dcterms:title "familyName" ;
    skos:definition "The family name of some person." ;
    skos:editorialNote "No occurrences of this slot in the graph." ;
    skos:inScheme okns:foaf ;
    skos:mappingRelation foaf:familyName ;
    linkml:definition_uri okns:foaf_familyName ;
    linkml:domain okns:FoafPerson ;
    linkml:inlined true ;
    linkml:owner okns:foaf_familyName ;
    linkml:range okns:RdfsLiteral ;
    linkml:slot_uri foaf:familyName .

okns:foaf_family_name a linkml:SlotDefinition ;
    dcterms:source foaf: ;
    dcterms:title "family_name" ;
    skos:definition "The family name of some person." ;
    skos:editorialNote "No occurrences of this slot in the graph." ;
    skos:inScheme okns:foaf ;
    skos:mappingRelation foaf:family_name ;
    linkml:definition_uri okns:foaf_family_name ;
    linkml:domain okns:FoafPerson ;
    linkml:inlined true ;
    linkml:owner okns:foaf_family_name ;
    linkml:range okns:RdfsLiteral ;
    linkml:slot_uri foaf:family_name .

okns:foaf_firstName a linkml:SlotDefinition ;
    dcterms:source foaf: ;
    dcterms:title "firstName" ;
    skos:definition "The first name of a person." ;
    skos:editorialNote "No occurrences of this slot in the graph." ;
    skos:inScheme okns:foaf ;
    skos:mappingRelation foaf:firstName ;
    linkml:definition_uri okns:foaf_firstName ;
    linkml:domain okns:FoafPerson ;
    linkml:inlined true ;
    linkml:owner okns:foaf_firstName ;
    linkml:range okns:RdfsLiteral ;
    linkml:slot_uri foaf:firstName .

okns:foaf_focus a linkml:SlotDefinition ;
    dcterms:source foaf: ;
    dcterms:title "focus" ;
    skos:definition "The underlying or 'focal' entity associated with some SKOS-described concept." ;
    skos:editorialNote "No occurrences of this slot in the graph." ;
    skos:inScheme okns:foaf ;
    skos:mappingRelation foaf:focus ;
    linkml:definition_uri okns:foaf_focus ;
    linkml:domain okns:SkosConcept ;
    linkml:inlined true ;
    linkml:owner okns:foaf_focus ;
    linkml:range okns:OwlThing ;
    linkml:slot_uri foaf:focus .

okns:foaf_fundedBy a linkml:SlotDefinition ;
    dcterms:source foaf: ;
    dcterms:title "funded by" ;
    skos:definition "An organization funding a project or person." ;
    skos:editorialNote "No occurrences of this slot in the graph." ;
    skos:inScheme okns:foaf ;
    skos:mappingRelation foaf:fundedBy ;
    linkml:definition_uri okns:foaf_fundedBy ;
    linkml:domain okns:OwlThing ;
    linkml:inlined true ;
    linkml:owner okns:foaf_fundedBy ;
    linkml:range okns:OwlThing ;
    linkml:slot_uri foaf:fundedBy .

okns:foaf_geekcode a linkml:SlotDefinition ;
    dcterms:source foaf: ;
    dcterms:title "geekcode" ;
    skos:definition "A textual geekcode for this person, see http://www.geekcode.com/geek.html" ;
    skos:editorialNote "No occurrences of this slot in the graph." ;
    skos:inScheme okns:foaf ;
    skos:mappingRelation foaf:geekcode ;
    linkml:definition_uri okns:foaf_geekcode ;
    linkml:domain okns:FoafPerson ;
    linkml:inlined true ;
    linkml:owner okns:foaf_geekcode ;
    linkml:range okns:RdfsLiteral ;
    linkml:slot_uri foaf:geekcode .

okns:foaf_gender a linkml:SlotDefinition ;
    dcterms:source foaf: ;
    dcterms:title "gender" ;
    skos:definition "The gender of this Agent (typically but not necessarily 'male' or 'female')." ;
    skos:editorialNote "No occurrences of this slot in the graph." ;
    skos:inScheme okns:foaf ;
    skos:mappingRelation foaf:gender ;
    linkml:definition_uri okns:foaf_gender ;
    linkml:domain okns:FoafAgent ;
    linkml:inlined true ;
    linkml:owner okns:foaf_gender ;
    linkml:range okns:RdfsLiteral ;
    linkml:slot_uri foaf:gender .

okns:foaf_holdsAccount a linkml:SlotDefinition ;
    dcterms:source foaf: ;
    dcterms:title "account" ;
    skos:definition "Indicates an account held by this agent." ;
    skos:editorialNote "No occurrences of this slot in the graph." ;
    skos:inScheme okns:foaf ;
    skos:mappingRelation foaf:holdsAccount ;
    linkml:definition_uri okns:foaf_holdsAccount ;
    linkml:domain okns:FoafAgent ;
    linkml:inlined true ;
    linkml:owner okns:foaf_holdsAccount ;
    linkml:range okns:FoafOnlineAccount ;
    linkml:slot_uri foaf:holdsAccount .

okns:foaf_homepage a linkml:SlotDefinition ;
    dcterms:source foaf: ;
    dcterms:title "homepage" ;
    rdfs:subPropertyOf okns:foaf_isPrimaryTopicOf ;
    skos:definition "A homepage for some thing." ;
    skos:editorialNote "No occurrences of this slot in the graph." ;
    skos:inScheme okns:foaf ;
    skos:mappingRelation foaf:homepage ;
    linkml:definition_uri okns:foaf_homepage ;
    linkml:domain okns:OwlThing ;
    linkml:inlined true ;
    linkml:owner okns:foaf_homepage ;
    linkml:range okns:FoafDocument ;
    linkml:slot_uri foaf:homepage .

okns:foaf_icqChatID a linkml:SlotDefinition ;
    dcterms:source foaf: ;
    dcterms:title "ICQ chat ID" ;
    rdfs:subPropertyOf okns:foaf_nick ;
    skos:definition "An ICQ chat ID" ;
    skos:editorialNote "No occurrences of this slot in the graph." ;
    skos:inScheme okns:foaf ;
    skos:mappingRelation foaf:icqChatID ;
    linkml:definition_uri okns:foaf_icqChatID ;
    linkml:domain okns:FoafAgent ;
    linkml:inlined true ;
    linkml:owner okns:foaf_icqChatID ;
    linkml:range okns:RdfsLiteral ;
    linkml:slot_uri foaf:icqChatID .

okns:foaf_img a linkml:SlotDefinition ;
    dcterms:source foaf: ;
    dcterms:title "image" ;
    rdfs:subPropertyOf okns:foaf_depiction ;
    skos:definition "An image that can be used to represent some thing (ie. those depictions which are particularly representative of something, eg. one's photo on a homepage)." ;
    skos:editorialNote "No occurrences of this slot in the graph." ;
    skos:inScheme okns:foaf ;
    skos:mappingRelation foaf:img ;
    linkml:definition_uri okns:foaf_img ;
    linkml:domain okns:FoafPerson ;
    linkml:inlined true ;
    linkml:owner okns:foaf_img ;
    linkml:range okns:FoafImage ;
    linkml:slot_uri foaf:img .

okns:foaf_interest a linkml:SlotDefinition ;
    dcterms:source foaf: ;
    dcterms:title "interest" ;
    skos:definition "A page about a topic of interest to this person." ;
    skos:editorialNote "No occurrences of this slot in the graph." ;
    skos:inScheme okns:foaf ;
    skos:mappingRelation foaf:interest ;
    linkml:definition_uri okns:foaf_interest ;
    linkml:domain okns:FoafAgent ;
    linkml:inlined true ;
    linkml:owner okns:foaf_interest ;
    linkml:range okns:FoafDocument ;
    linkml:slot_uri foaf:interest .

okns:foaf_jabberID a linkml:SlotDefinition ;
    dcterms:source foaf: ;
    dcterms:title "jabber ID" ;
    skos:definition "A jabber ID for something." ;
    skos:editorialNote "No occurrences of this slot in the graph." ;
    skos:inScheme okns:foaf ;
    skos:mappingRelation foaf:jabberID ;
    linkml:definition_uri okns:foaf_jabberID ;
    linkml:domain okns:FoafAgent ;
    linkml:inlined true ;
    linkml:owner okns:foaf_jabberID ;
    linkml:range okns:RdfsLiteral ;
    linkml:slot_uri foaf:jabberID .

okns:foaf_knows a linkml:SlotDefinition ;
    dcterms:source foaf: ;
    dcterms:title "knows" ;
    skos:definition "A person known by this person (indicating some level of reciprocated interaction between the parties)." ;
    skos:editorialNote "No occurrences of this slot in the graph." ;
    skos:inScheme okns:foaf ;
    skos:mappingRelation foaf:knows ;
    linkml:definition_uri okns:foaf_knows ;
    linkml:domain okns:FoafPerson ;
    linkml:inlined true ;
    linkml:owner okns:foaf_knows ;
    linkml:range okns:FoafPerson ;
    linkml:slot_uri foaf:knows .

okns:foaf_lastName a linkml:SlotDefinition ;
    dcterms:source foaf: ;
    dcterms:title "lastName" ;
    skos:definition "The last name of a person." ;
    skos:editorialNote "No occurrences of this slot in the graph." ;
    skos:inScheme okns:foaf ;
    skos:mappingRelation foaf:lastName ;
    linkml:definition_uri okns:foaf_lastName ;
    linkml:domain okns:FoafPerson ;
    linkml:inlined true ;
    linkml:owner okns:foaf_lastName ;
    linkml:range okns:RdfsLiteral ;
    linkml:slot_uri foaf:lastName .

okns:foaf_logo a linkml:SlotDefinition ;
    dcterms:source foaf: ;
    dcterms:title "logo" ;
    skos:definition "A logo representing some thing." ;
    skos:editorialNote "No occurrences of this slot in the graph." ;
    skos:inScheme okns:foaf ;
    skos:mappingRelation foaf:logo ;
    linkml:definition_uri okns:foaf_logo ;
    linkml:domain okns:OwlThing ;
    linkml:inlined true ;
    linkml:owner okns:foaf_logo ;
    linkml:range okns:OwlThing ;
    linkml:slot_uri foaf:logo .

okns:foaf_mbox a linkml:SlotDefinition ;
    dcterms:source foaf: ;
    dcterms:title "personal mailbox" ;
    skos:definition "A  personal mailbox, ie. an Internet mailbox associated with exactly one owner, the first owner of this mailbox. This is a 'static inverse functional property', in that  there is (across time and change) at most one individual that ever has any particular value for foaf:mbox." ;
    skos:editorialNote "No occurrences of this slot in the graph." ;
    skos:inScheme okns:foaf ;
    skos:mappingRelation foaf:mbox ;
    linkml:definition_uri okns:foaf_mbox ;
    linkml:domain okns:FoafAgent ;
    linkml:inlined true ;
    linkml:owner okns:foaf_mbox ;
    linkml:range okns:OwlThing ;
    linkml:slot_uri foaf:mbox .

okns:foaf_mbox_sha1sum a linkml:SlotDefinition ;
    dcterms:source foaf: ;
    dcterms:title "sha1sum of a personal mailbox URI name" ;
    skos:definition "The sha1sum of the URI of an Internet mailbox associated with exactly one owner, the  first owner of the mailbox." ;
    skos:editorialNote "No occurrences of this slot in the graph." ;
    skos:inScheme okns:foaf ;
    skos:mappingRelation foaf:mbox_sha1sum ;
    linkml:definition_uri okns:foaf_mbox_sha1sum ;
    linkml:domain okns:FoafAgent ;
    linkml:inlined true ;
    linkml:owner okns:foaf_mbox_sha1sum ;
    linkml:range okns:RdfsLiteral ;
    linkml:slot_uri foaf:mbox_sha1sum .

okns:foaf_msnChatID a linkml:SlotDefinition ;
    dcterms:source foaf: ;
    dcterms:title "MSN chat ID" ;
    rdfs:subPropertyOf okns:foaf_nick ;
    skos:definition "An MSN chat ID" ;
    skos:editorialNote "No occurrences of this slot in the graph." ;
    skos:inScheme okns:foaf ;
    skos:mappingRelation foaf:msnChatID ;
    linkml:definition_uri okns:foaf_msnChatID ;
    linkml:domain okns:FoafAgent ;
    linkml:inlined true ;
    linkml:owner okns:foaf_msnChatID ;
    linkml:range okns:RdfsLiteral ;
    linkml:slot_uri foaf:msnChatID .

okns:foaf_myersBriggs a linkml:SlotDefinition ;
    dcterms:source foaf: ;
    dcterms:title "myersBriggs" ;
    skos:definition "A Myers Briggs (MBTI) personality classification." ;
    skos:editorialNote "No occurrences of this slot in the graph." ;
    skos:inScheme okns:foaf ;
    skos:mappingRelation foaf:myersBriggs ;
    linkml:definition_uri okns:foaf_myersBriggs ;
    linkml:domain okns:FoafPerson ;
    linkml:inlined true ;
    linkml:owner okns:foaf_myersBriggs ;
    linkml:range okns:RdfsLiteral ;
    linkml:slot_uri foaf:myersBriggs .

okns:foaf_name a linkml:SlotDefinition ;
    dcterms:source foaf: ;
    dcterms:title "name" ;
    rdfs:subPropertyOf okns:rdfs_label ;
    skos:definition "A name for some thing." ;
    skos:editorialNote "No occurrences of this slot in the graph." ;
    skos:inScheme okns:foaf ;
    skos:mappingRelation foaf:name ;
    linkml:definition_uri okns:foaf_name ;
    linkml:domain okns:OwlThing ;
    linkml:inlined true ;
    linkml:owner okns:foaf_name ;
    linkml:range okns:RdfsLiteral ;
    linkml:slot_uri foaf:name .

okns:foaf_openid a linkml:SlotDefinition ;
    dcterms:source foaf: ;
    dcterms:title "openid" ;
    rdfs:subPropertyOf okns:foaf_isPrimaryTopicOf ;
    skos:definition "An OpenID for an Agent." ;
    skos:editorialNote "No occurrences of this slot in the graph." ;
    skos:inScheme okns:foaf ;
    skos:mappingRelation foaf:openid ;
    linkml:definition_uri okns:foaf_openid ;
    linkml:domain okns:FoafAgent ;
    linkml:inlined true ;
    linkml:owner okns:foaf_openid ;
    linkml:range okns:FoafDocument ;
    linkml:slot_uri foaf:openid .

okns:foaf_pastProject a linkml:SlotDefinition ;
    dcterms:source foaf: ;
    dcterms:title "past project" ;
    skos:definition "A project this person has previously worked on." ;
    skos:editorialNote "No occurrences of this slot in the graph." ;
    skos:inScheme okns:foaf ;
    skos:mappingRelation foaf:pastProject ;
    linkml:definition_uri okns:foaf_pastProject ;
    linkml:domain okns:FoafPerson ;
    linkml:inlined true ;
    linkml:owner okns:foaf_pastProject ;
    linkml:range okns:OwlThing ;
    linkml:slot_uri foaf:pastProject .

okns:foaf_plan a linkml:SlotDefinition ;
    dcterms:source foaf: ;
    dcterms:title "plan" ;
    skos:definition "A .plan comment, in the tradition of finger and '.plan' files." ;
    skos:editorialNote "No occurrences of this slot in the graph." ;
    skos:inScheme okns:foaf ;
    skos:mappingRelation foaf:plan ;
    linkml:definition_uri okns:foaf_plan ;
    linkml:domain okns:FoafPerson ;
    linkml:inlined true ;
    linkml:owner okns:foaf_plan ;
    linkml:range okns:RdfsLiteral ;
    linkml:slot_uri foaf:plan .

okns:foaf_publications a linkml:SlotDefinition ;
    dcterms:source foaf: ;
    dcterms:title "publications" ;
    skos:definition "A link to the publications of this person." ;
    skos:editorialNote "No occurrences of this slot in the graph." ;
    skos:inScheme okns:foaf ;
    skos:mappingRelation foaf:publications ;
    linkml:definition_uri okns:foaf_publications ;
    linkml:domain okns:FoafPerson ;
    linkml:inlined true ;
    linkml:owner okns:foaf_publications ;
    linkml:range okns:FoafDocument ;
    linkml:slot_uri foaf:publications .

okns:foaf_schoolHomepage a linkml:SlotDefinition ;
    dcterms:source foaf: ;
    dcterms:title "schoolHomepage" ;
    skos:definition "A homepage of a school attended by the person." ;
    skos:editorialNote "No occurrences of this slot in the graph." ;
    skos:inScheme okns:foaf ;
    skos:mappingRelation foaf:schoolHomepage ;
    linkml:definition_uri okns:foaf_schoolHomepage ;
    linkml:domain okns:FoafPerson ;
    linkml:inlined true ;
    linkml:owner okns:foaf_schoolHomepage ;
    linkml:range okns:FoafDocument ;
    linkml:slot_uri foaf:schoolHomepage .

okns:foaf_sha1 a linkml:SlotDefinition ;
    dcterms:source foaf: ;
    dcterms:title "sha1sum (hex)" ;
    skos:definition "A sha1sum hash, in hex." ;
    skos:editorialNote "No occurrences of this slot in the graph." ;
    skos:inScheme okns:foaf ;
    skos:mappingRelation foaf:sha1 ;
    linkml:definition_uri okns:foaf_sha1 ;
    linkml:domain okns:FoafDocument ;
    linkml:inlined true ;
    linkml:owner okns:foaf_sha1 ;
    linkml:range okns:Any ;
    linkml:slot_uri foaf:sha1 .

okns:foaf_skypeID a linkml:SlotDefinition ;
    dcterms:source foaf: ;
    dcterms:title "Skype ID" ;
    rdfs:subPropertyOf okns:foaf_nick ;
    skos:definition "A Skype ID" ;
    skos:editorialNote "No occurrences of this slot in the graph." ;
    skos:inScheme okns:foaf ;
    skos:mappingRelation foaf:skypeID ;
    linkml:definition_uri okns:foaf_skypeID ;
    linkml:domain okns:FoafAgent ;
    linkml:inlined true ;
    linkml:owner okns:foaf_skypeID ;
    linkml:range okns:RdfsLiteral ;
    linkml:slot_uri foaf:skypeID .

okns:foaf_status a linkml:SlotDefinition ;
    dcterms:source foaf: ;
    dcterms:title "status" ;
    skos:definition "A string expressing what the user is happy for the general public (normally) to know about their current activity." ;
    skos:editorialNote "No occurrences of this slot in the graph." ;
    skos:inScheme okns:foaf ;
    skos:mappingRelation foaf:status ;
    linkml:definition_uri okns:foaf_status ;
    linkml:domain okns:FoafAgent ;
    linkml:inlined true ;
    linkml:owner okns:foaf_status ;
    linkml:range okns:RdfsLiteral ;
    linkml:slot_uri foaf:status .

okns:foaf_surname a linkml:SlotDefinition ;
    dcterms:source foaf: ;
    dcterms:title "Surname" ;
    skos:definition "The surname of some person." ;
    skos:editorialNote "No occurrences of this slot in the graph." ;
    skos:inScheme okns:foaf ;
    skos:mappingRelation foaf:surname ;
    linkml:definition_uri okns:foaf_surname ;
    linkml:domain okns:FoafPerson ;
    linkml:inlined true ;
    linkml:owner okns:foaf_surname ;
    linkml:range okns:RdfsLiteral ;
    linkml:slot_uri foaf:surname .

okns:foaf_theme a linkml:SlotDefinition ;
    dcterms:source foaf: ;
    dcterms:title "theme" ;
    skos:definition "A theme." ;
    skos:editorialNote "No occurrences of this slot in the graph." ;
    skos:inScheme okns:foaf ;
    skos:mappingRelation foaf:theme ;
    linkml:definition_uri okns:foaf_theme ;
    linkml:domain okns:OwlThing ;
    linkml:inlined true ;
    linkml:owner okns:foaf_theme ;
    linkml:range okns:OwlThing ;
    linkml:slot_uri foaf:theme .

okns:foaf_thumbnail a linkml:SlotDefinition ;
    dcterms:source foaf: ;
    dcterms:title "thumbnail" ;
    skos:definition "A derived thumbnail image." ;
    skos:editorialNote "No occurrences of this slot in the graph." ;
    skos:inScheme okns:foaf ;
    skos:mappingRelation foaf:thumbnail ;
    linkml:definition_uri okns:foaf_thumbnail ;
    linkml:domain okns:FoafImage ;
    linkml:inlined true ;
    linkml:owner okns:foaf_thumbnail ;
    linkml:range okns:FoafImage ;
    linkml:slot_uri foaf:thumbnail .

okns:foaf_tipjar a linkml:SlotDefinition ;
    dcterms:source foaf: ;
    dcterms:title "tipjar" ;
    rdfs:subPropertyOf okns:foaf_page ;
    skos:definition "A tipjar document for this agent, describing means for payment and reward." ;
    skos:editorialNote "No occurrences of this slot in the graph." ;
    skos:inScheme okns:foaf ;
    skos:mappingRelation foaf:tipjar ;
    linkml:definition_uri okns:foaf_tipjar ;
    linkml:domain okns:FoafAgent ;
    linkml:inlined true ;
    linkml:owner okns:foaf_tipjar ;
    linkml:range okns:FoafDocument ;
    linkml:slot_uri foaf:tipjar .

okns:foaf_topic_interest a linkml:SlotDefinition ;
    dcterms:source foaf: ;
    dcterms:title "topic_interest" ;
    skos:definition "A thing of interest to this person." ;
    skos:editorialNote "No occurrences of this slot in the graph." ;
    skos:inScheme okns:foaf ;
    skos:mappingRelation foaf:topic_interest ;
    linkml:definition_uri okns:foaf_topic_interest ;
    linkml:domain okns:FoafAgent ;
    linkml:inlined true ;
    linkml:owner okns:foaf_topic_interest ;
    linkml:range okns:OwlThing ;
    linkml:slot_uri foaf:topic_interest .

okns:foaf_weblog a linkml:SlotDefinition ;
    dcterms:source foaf: ;
    dcterms:title "weblog" ;
    rdfs:subPropertyOf okns:foaf_page ;
    skos:definition "A weblog of some thing (whether person, group, company etc.)." ;
    skos:editorialNote "No occurrences of this slot in the graph." ;
    skos:inScheme okns:foaf ;
    skos:mappingRelation foaf:weblog ;
    linkml:definition_uri okns:foaf_weblog ;
    linkml:domain okns:FoafAgent ;
    linkml:inlined true ;
    linkml:owner okns:foaf_weblog ;
    linkml:range okns:FoafDocument ;
    linkml:slot_uri foaf:weblog .

okns:foaf_workInfoHomepage a linkml:SlotDefinition ;
    dcterms:source foaf: ;
    dcterms:title "work info homepage" ;
    skos:definition "A work info homepage of some person; a page about their work for some organization." ;
    skos:editorialNote "No occurrences of this slot in the graph." ;
    skos:inScheme okns:foaf ;
    skos:mappingRelation foaf:workInfoHomepage ;
    linkml:definition_uri okns:foaf_workInfoHomepage ;
    linkml:domain okns:FoafPerson ;
    linkml:inlined true ;
    linkml:owner okns:foaf_workInfoHomepage ;
    linkml:range okns:FoafDocument ;
    linkml:slot_uri foaf:workInfoHomepage .

okns:foaf_workplaceHomepage a linkml:SlotDefinition ;
    dcterms:source foaf: ;
    dcterms:title "workplace homepage" ;
    skos:definition "A workplace homepage of some person; the homepage of an organization they work for." ;
    skos:editorialNote "No occurrences of this slot in the graph." ;
    skos:inScheme okns:foaf ;
    skos:mappingRelation foaf:workplaceHomepage ;
    linkml:definition_uri okns:foaf_workplaceHomepage ;
    linkml:domain okns:FoafPerson ;
    linkml:inlined true ;
    linkml:owner okns:foaf_workplaceHomepage ;
    linkml:range okns:FoafDocument ;
    linkml:slot_uri foaf:workplaceHomepage .

okns:foaf_yahooChatID a linkml:SlotDefinition ;
    dcterms:source foaf: ;
    dcterms:title "Yahoo chat ID" ;
    rdfs:subPropertyOf okns:foaf_nick ;
    skos:definition "A Yahoo chat ID" ;
    skos:editorialNote "No occurrences of this slot in the graph." ;
    skos:inScheme okns:foaf ;
    skos:mappingRelation foaf:yahooChatID ;
    linkml:definition_uri okns:foaf_yahooChatID ;
    linkml:domain okns:FoafAgent ;
    linkml:inlined true ;
    linkml:owner okns:foaf_yahooChatID ;
    linkml:range okns:RdfsLiteral ;
    linkml:slot_uri foaf:yahooChatID .

okns:frbr_adaption a linkml:SlotDefinition ;
    dcterms:source frbr: ;
    dcterms:title "adaption" ;
    rdfs:subPropertyOf okns:frbr_relatedEndeavour ;
    owl:inverseOf okns:frbr_adaptionOf ;
    skos:definition "An adaption of a work or expression." ;
    skos:editorialNote "N06f3c0b5e1e747618c169ed2f1211d40",
        "N07f795a57c5c48eb94fd0ec121833b81",
        "Ncc9909c93d4a489a8f2298b3c451ea21",
        "No occurrences of this slot in the graph." ;
    skos:inScheme okns:frbr ;
    skos:mappingRelation frbr:adaption ;
    linkml:definition_uri okns:frbr_adaption ;
    linkml:domain okns:Any ;
    linkml:inlined true ;
    linkml:range okns:Any ;
    linkml:slot_uri frbr:adaption .

okns:frbr_adaptionOf a linkml:SlotDefinition ;
    dcterms:source frbr: ;
    dcterms:title "adaption of" ;
    rdfs:subPropertyOf okns:frbr_relatedEndeavour ;
    owl:inverseOf okns:frbr_adaption ;
    skos:definition "A work or expression that is adapted." ;
    skos:editorialNote "N0a95918a620045e5957be335ba7fea35",
        "N1b504a0124654f88bcd19341c16cf540",
        "N224ce65ca0004af6966c1bb46889b98b",
        "No occurrences of this slot in the graph." ;
    skos:inScheme okns:frbr ;
    skos:mappingRelation frbr:adaptionOf ;
    linkml:definition_uri okns:frbr_adaptionOf ;
    linkml:domain okns:Any ;
    linkml:inlined true ;
    linkml:range okns:Any ;
    linkml:slot_uri frbr:adaptionOf .

okns:frbr_complement a linkml:SlotDefinition ;
    dcterms:source frbr: ;
    dcterms:title "complement" ;
    rdfs:subPropertyOf okns:frbr_relatedEndeavour ;
    owl:inverseOf okns:frbr_complementOf ;
    skos:definition "A complement to a work or expression." ;
    skos:editorialNote "N3ed7ccbf34354511b4e3a2f7a3e410a1",
        "N5b1b0f4356d0438e85a957c660a066b0",
        "Ndd48068eb6f44cc0aff499065c11d801",
        "No occurrences of this slot in the graph." ;
    skos:inScheme okns:frbr ;
    skos:mappingRelation frbr:complement ;
    linkml:definition_uri okns:frbr_complement ;
    linkml:domain okns:Any ;
    linkml:inlined true ;
    linkml:range okns:Any ;
    linkml:slot_uri frbr:complement .

okns:frbr_complementOf a linkml:SlotDefinition ;
    dcterms:source frbr: ;
    dcterms:title "complement of" ;
    rdfs:subPropertyOf okns:frbr_relatedEndeavour ;
    owl:inverseOf okns:frbr_complement ;
    skos:definition "A work or expression that is complemented." ;
    skos:editorialNote "N4b351cb23ab14863b90379b8a22d29d2",
        "Nd643b473bf8f48178e4c4d35f06dd88b",
        "Ne9760d5499a24a76a7877416b873dbe0",
        "No occurrences of this slot in the graph." ;
    skos:inScheme okns:frbr ;
    skos:mappingRelation frbr:complementOf ;
    linkml:definition_uri okns:frbr_complementOf ;
    linkml:domain okns:Any ;
    linkml:inlined true ;
    linkml:range okns:Any ;
    linkml:slot_uri frbr:complementOf .

okns:frbr_imitation a linkml:SlotDefinition ;
    dcterms:source frbr: ;
    dcterms:title "imitation" ;
    rdfs:subPropertyOf okns:frbr_relatedEndeavour ;
    owl:inverseOf okns:frbr_imitationOf ;
    skos:definition "An imitation of a work or expression." ;
    skos:editorialNote "N1b30cb54c0514ec99dd992b00039fb6c",
        "N855b406439e1463b926760eacd02b46a",
        "Nd31eedc644e14373b54bf3496acaa372",
        "No occurrences of this slot in the graph." ;
    skos:inScheme okns:frbr ;
    skos:mappingRelation frbr:imitation ;
    linkml:definition_uri okns:frbr_imitation ;
    linkml:domain okns:Any ;
    linkml:inlined true ;
    linkml:range okns:Any ;
    linkml:slot_uri frbr:imitation .

okns:frbr_imitationOf a linkml:SlotDefinition ;
    dcterms:source frbr: ;
    dcterms:title "imitation of" ;
    rdfs:subPropertyOf okns:frbr_relatedEndeavour ;
    owl:inverseOf okns:frbr_imitation ;
    skos:definition "A work or expression that is imitated." ;
    skos:editorialNote "N211adae207fb469ea2b3f764e20a135c",
        "N3ce63f536113413996a42f480c47360b",
        "N4a4a5041f31f4c67b9d00b3f3f720a7e",
        "No occurrences of this slot in the graph." ;
    skos:inScheme okns:frbr ;
    skos:mappingRelation frbr:imitationOf ;
    linkml:definition_uri okns:frbr_imitationOf ;
    linkml:domain okns:Any ;
    linkml:inlined true ;
    linkml:range okns:Any ;
    linkml:slot_uri frbr:imitationOf .

okns:frbr_part a linkml:SlotDefinition ;
    dcterms:source frbr: ;
    dcterms:title "part" ;
    rdfs:subPropertyOf okns:frbr_relatedEndeavour ;
    owl:inverseOf okns:frbr_partOf ;
    skos:definition "A part of an endeavour." ;
    skos:editorialNote "N8898c09ad1614022a3dd18d67ef04aed",
        "Ne3a2b11c644940368feb5ae0b5133d80",
        "No occurrences of this slot in the graph." ;
    skos:inScheme okns:frbr ;
    skos:mappingRelation frbr:part ;
    linkml:definition_uri okns:frbr_part ;
    linkml:domain okns:Any ;
    linkml:inlined true ;
    linkml:range okns:Any ;
    linkml:slot_uri frbr:part .

okns:frbr_partOf a linkml:SlotDefinition ;
    dcterms:source frbr: ;
    dcterms:title "part of" ;
    rdfs:subPropertyOf okns:frbr_relatedEndeavour ;
    owl:inverseOf okns:frbr_part ;
    skos:definition "An endeavour incorporating an endeavour." ;
    skos:editorialNote "N7daed7b9dbe54472b639af93b9b1c350",
        "Ne3a3c80751314efaba5c3d97652284e3",
        "No occurrences of this slot in the graph." ;
    skos:inScheme okns:frbr ;
    skos:mappingRelation frbr:partOf ;
    linkml:definition_uri okns:frbr_partOf ;
    linkml:domain okns:Any ;
    linkml:inlined true ;
    linkml:range okns:Any ;
    linkml:slot_uri frbr:partOf .

okns:frbr_reproduction a linkml:SlotDefinition ;
    dcterms:source frbr: ;
    dcterms:title "reproduction" ;
    rdfs:subPropertyOf okns:frbr_relatedEndeavour ;
    owl:inverseOf okns:frbr_reproductionOf ;
    skos:definition "A reproduction of a manifestation or item." ;
    skos:editorialNote "N22039df0be3447c090bcb16e74c7d171",
        "N7c8202fc64f0479f876a33c62b133a3f",
        "Nda710445ec2546759d24678e0614c2e0",
        "No occurrences of this slot in the graph." ;
    skos:inScheme okns:frbr ;
    skos:mappingRelation frbr:reproduction ;
    linkml:definition_uri okns:frbr_reproduction ;
    linkml:domain okns:Any ;
    linkml:inlined true ;
    linkml:range okns:Any ;
    linkml:slot_uri frbr:reproduction .

okns:frbr_reproductionOf a linkml:SlotDefinition ;
    dcterms:source frbr: ;
    dcterms:title "reproduction of" ;
    rdfs:subPropertyOf okns:frbr_relatedEndeavour ;
    owl:inverseOf okns:frbr_reproduction ;
    skos:definition "A manifestation or item that is reproduced." ;
    skos:editorialNote "N072e529762ea45d6b167cd4a42b893dc",
        "N56fa8d17650644589c90842d38b6fb62",
        "Ndeae1dd6d7e54466837e7de11e757304",
        "No occurrences of this slot in the graph." ;
    skos:inScheme okns:frbr ;
    skos:mappingRelation frbr:reproductionOf ;
    linkml:definition_uri okns:frbr_reproductionOf ;
    linkml:domain okns:Any ;
    linkml:inlined true ;
    linkml:range okns:Any ;
    linkml:slot_uri frbr:reproductionOf .

okns:frbr_subject a linkml:SlotDefinition ;
    dcterms:source frbr: ;
    dcterms:title "subject" ;
    skos:definition "The subject of a work." ;
    skos:editorialNote "N27c0ba612d564c74a2ef599260626410",
        "N4c2054568144473f913b9242a7ece86b",
        "No occurrences of this slot in the graph." ;
    skos:inScheme okns:frbr ;
    skos:mappingRelation frbr:subject ;
    linkml:definition_uri okns:frbr_subject ;
    linkml:domain okns:FrbrWork ;
    linkml:inlined true ;
    linkml:owner okns:frbr_subject ;
    linkml:range okns:Any ;
    linkml:slot_uri frbr:subject .

okns:frbr_successor a linkml:SlotDefinition ;
    dcterms:source frbr: ;
    dcterms:title "successor" ;
    rdfs:subPropertyOf okns:frbr_relatedEndeavour ;
    owl:inverseOf okns:frbr_successorOf ;
    skos:definition "A successor to a work or expression." ;
    skos:editorialNote "N02dfcb9c24f64608995ed6331e7bd5ed",
        "N16764e93f5f04eadbc4ad37d1b5a1fc4",
        "N320f6cad1aa84382b1407bb9472ccc4a",
        "No occurrences of this slot in the graph." ;
    skos:inScheme okns:frbr ;
    skos:mappingRelation frbr:successor ;
    linkml:definition_uri okns:frbr_successor ;
    linkml:domain okns:Any ;
    linkml:inlined true ;
    linkml:range okns:Any ;
    linkml:slot_uri frbr:successor .

okns:frbr_successorOf a linkml:SlotDefinition ;
    dcterms:source frbr: ;
    dcterms:title "successor of" ;
    rdfs:subPropertyOf okns:frbr_relatedEndeavour ;
    owl:inverseOf okns:frbr_successor ;
    skos:definition "A work or expression that is succeeded." ;
    skos:editorialNote "N151e25f414824bd0ae86c258997c4832",
        "N89b9545e83af4b5890b7ba270bc051fe",
        "N9896ef30b041409ba12f2f5f5e04e010",
        "No occurrences of this slot in the graph." ;
    skos:inScheme okns:frbr ;
    skos:mappingRelation frbr:successorOf ;
    linkml:definition_uri okns:frbr_successorOf ;
    linkml:domain okns:Any ;
    linkml:inlined true ;
    linkml:range okns:Any ;
    linkml:slot_uri frbr:successorOf .

okns:frbr_summarization a linkml:SlotDefinition ;
    dcterms:source frbr: ;
    dcterms:title "summarization" ;
    rdfs:subPropertyOf okns:frbr_relatedEndeavour ;
    owl:inverseOf okns:frbr_summarizationOf ;
    skos:definition "A summarization of a work or expression." ;
    skos:editorialNote "N163e9185402445cc82859899c49e9743",
        "N67a8c0415a8d4135ae7d050c46a190b8",
        "N8a6f3f17fce94cd29fd3a0f20736670a",
        "No occurrences of this slot in the graph." ;
    skos:inScheme okns:frbr ;
    skos:mappingRelation frbr:summarization ;
    linkml:definition_uri okns:frbr_summarization ;
    linkml:domain okns:Any ;
    linkml:inlined true ;
    linkml:range okns:Any ;
    linkml:slot_uri frbr:summarization .

okns:frbr_summarizationOf a linkml:SlotDefinition ;
    dcterms:source frbr: ;
    dcterms:title "summarization of" ;
    rdfs:subPropertyOf okns:frbr_relatedEndeavour ;
    owl:inverseOf okns:frbr_summarization ;
    skos:definition "A work or expression that is summarized." ;
    skos:editorialNote "N0137cf1485d54b33b520a35ffac1c214",
        "N806a57b683b5484a984a7e449e07e27c",
        "N884c6e298a3a45a0aa0c80a7f2bbdc54",
        "No occurrences of this slot in the graph." ;
    skos:inScheme okns:frbr ;
    skos:mappingRelation frbr:summarizationOf ;
    linkml:definition_uri okns:frbr_summarizationOf ;
    linkml:domain okns:Any ;
    linkml:inlined true ;
    linkml:range okns:Any ;
    linkml:slot_uri frbr:summarizationOf .

okns:frbr_supplement a linkml:SlotDefinition ;
    dcterms:source frbr: ;
    dcterms:title "supplement" ;
    rdfs:subPropertyOf okns:frbr_relatedEndeavour ;
    owl:inverseOf okns:frbr_supplementOf ;
    skos:definition "A supplement to a work or expression." ;
    skos:editorialNote "N8236bf9a5ea64a2b9e3fc67fb12664c7",
        "Na4621fee86294594826fdc9c6e2b5061",
        "Nc7b0aa4a4cbe411396aaf25a3019dc74",
        "No occurrences of this slot in the graph." ;
    skos:inScheme okns:frbr ;
    skos:mappingRelation frbr:supplement ;
    linkml:definition_uri okns:frbr_supplement ;
    linkml:domain okns:Any ;
    linkml:inlined true ;
    linkml:range okns:Any ;
    linkml:slot_uri frbr:supplement .

okns:frbr_supplementOf a linkml:SlotDefinition ;
    dcterms:source frbr: ;
    dcterms:title "supplement of" ;
    rdfs:subPropertyOf okns:frbr_relatedEndeavour ;
    owl:inverseOf okns:frbr_supplement ;
    skos:definition "A work or expression that is supplemented." ;
    skos:editorialNote "N1471afc748a6483b8dacd914f97545d2",
        "Nce389cf2062d4bb19d3220dd4ea3a7fd",
        "Nd5603796fef541a992a9285f2c9d7976",
        "No occurrences of this slot in the graph." ;
    skos:inScheme okns:frbr ;
    skos:mappingRelation frbr:supplementOf ;
    linkml:definition_uri okns:frbr_supplementOf ;
    linkml:domain okns:Any ;
    linkml:inlined true ;
    linkml:range okns:Any ;
    linkml:slot_uri frbr:supplementOf .

okns:frbr_transformation a linkml:SlotDefinition ;
    dcterms:source frbr: ;
    dcterms:title "transformation" ;
    rdfs:subPropertyOf okns:frbr_relatedEndeavour ;
    owl:inverseOf okns:frbr_transformationOf ;
    skos:definition "A transformation of a work or expression." ;
    skos:editorialNote "N23bcc8d410d3437a9ddf4c13da330b6d",
        "N97dfee91d8fd45f3af23808af583c1f0",
        "Nef44ff607f8c40cd8598367e3cda4f32",
        "No occurrences of this slot in the graph." ;
    skos:inScheme okns:frbr ;
    skos:mappingRelation frbr:transformation ;
    linkml:definition_uri okns:frbr_transformation ;
    linkml:domain okns:Any ;
    linkml:inlined true ;
    linkml:range okns:Any ;
    linkml:slot_uri frbr:transformation .

okns:frbr_transformationOf a linkml:SlotDefinition ;
    dcterms:source frbr: ;
    dcterms:title "transformation of" ;
    rdfs:subPropertyOf okns:frbr_relatedEndeavour ;
    owl:inverseOf okns:frbr_transformation ;
    skos:definition "A work or expression that is transformed." ;
    skos:editorialNote "Nc6388a8e3aac4182ae11665763a67a8b",
        "Nd252db20c8034a6ba8637ccc5ff12bfc",
        "Ne566164d5a394f17ac1c42de9e70b780",
        "No occurrences of this slot in the graph." ;
    skos:inScheme okns:frbr ;
    skos:mappingRelation frbr:transformationOf ;
    linkml:definition_uri okns:frbr_transformationOf ;
    linkml:domain okns:Any ;
    linkml:inlined true ;
    linkml:range okns:Any ;
    linkml:slot_uri frbr:transformationOf .

okns:ical_completed a linkml:SlotDefinition ;
    dcterms:title "COMPLETED" ;
    skos:definition "This property defines the date and time that a to-do was actually completed." ;
    skos:editorialNote "No occurrences of this slot in the graph." ;
    skos:inScheme okns:ical ;
    skos:mappingRelation ical:completed ;
    skos:note "description: value type: DATE-TIME" ;
    linkml:definition_uri okns:ical_completed ;
    linkml:domain okns:IcalVtodo ;
    linkml:inlined true ;
    linkml:owner okns:ical_completed ;
    linkml:range okns:IcalValueDATE-TIME ;
    linkml:slot_uri ical:completed .

okns:ical_due a linkml:SlotDefinition ;
    dcterms:title "DUE" ;
    skos:definition "This property defines the date and time that a to-do is expected to be completed." ;
    skos:editorialNote "No occurrences of this slot in the graph." ;
    skos:inScheme okns:ical ;
    skos:mappingRelation ical:due ;
    skos:note "description: default value type: DATE-TIME" ;
    linkml:definition_uri okns:ical_due ;
    linkml:domain okns:IcalVtodo ;
    linkml:inlined true ;
    linkml:owner okns:ical_due ;
    linkml:range okns:Any ;
    linkml:slot_uri ical:due .

okns:ical_exdate a linkml:SlotDefinition ;
    dcterms:title "EXDATE" ;
    skos:definition "This property defines the list of date/time exceptions for a recurring calendar component." ;
    skos:editorialNote "No occurrences of this slot in the graph." ;
    skos:inScheme okns:ical ;
    skos:mappingRelation ical:exdate ;
    skos:note "description: default value type: DATE-TIME" ;
    linkml:definition_uri okns:ical_exdate ;
    linkml:domain okns:IcalDomainOfRrule ;
    linkml:inlined true ;
    linkml:owner okns:ical_exdate ;
    linkml:range okns:Any ;
    linkml:slot_uri ical:exdate .

okns:ical_percentComplete a linkml:SlotDefinition ;
    dcterms:title "PERCENT-COMPLETE" ;
    skos:definition "This property is used by an assignee or delegatee of a to-do to convey the percent completion of a to-do to the Organizer." ;
    skos:editorialNote "No occurrences of this slot in the graph." ;
    skos:inScheme okns:ical ;
    skos:mappingRelation ical:percentComplete ;
    skos:note "description: value type: INTEGER" ;
    linkml:definition_uri okns:ical_percentComplete ;
    linkml:domain okns:IcalVtodo ;
    linkml:owner okns:ical_percentComplete ;
    linkml:range okns:integer ;
    linkml:slot_uri ical:percentComplete .

okns:ical_recurrenceId a linkml:SlotDefinition ;
    dcterms:title "RECURRENCE-ID" ;
    skos:definition "This property is used in conjunction with the \"UID\" and \"SEQUENCE\" property to identify a specific instance of a recurring \"VEVENT\", \"VTODO\" or \"VJOURNAL\" calendar component. The property value is the effective value of the \"DTSTART\" property of the recurrence instance." ;
    skos:editorialNote "No occurrences of this slot in the graph." ;
    skos:inScheme okns:ical ;
    skos:mappingRelation ical:recurrenceId ;
    skos:note "description: default value type: DATE-TIME" ;
    linkml:definition_uri okns:ical_recurrenceId ;
    linkml:domain okns:IcalDomainOfRrule ;
    linkml:inlined true ;
    linkml:owner okns:ical_recurrenceId ;
    linkml:range okns:Any ;
    linkml:slot_uri ical:recurrenceId .

okns:ical_repeat a linkml:SlotDefinition ;
    dcterms:title "REPEAT" ;
    skos:definition "This property defines the number of time the alarm should be repeated, after the initial trigger." ;
    skos:editorialNote "No occurrences of this slot in the graph." ;
    skos:inScheme okns:ical ;
    skos:mappingRelation ical:repeat ;
    skos:note "description: value type: INTEGER" ;
    linkml:definition_uri okns:ical_repeat ;
    linkml:domain okns:IcalValarm ;
    linkml:owner okns:ical_repeat ;
    linkml:range okns:integer ;
    linkml:slot_uri ical:repeat .

okns:ical_transp a linkml:SlotDefinition ;
    dcterms:title "TRANSP" ;
    skos:definition "This property defines whether an event is transparent or not to busy time searches." ;
    skos:editorialNote "No occurrences of this slot in the graph." ;
    skos:inScheme okns:ical ;
    skos:mappingRelation ical:transp ;
    skos:note "description: value type: TEXT" ;
    linkml:definition_uri okns:ical_transp ;
    linkml:domain okns:IcalVevent ;
    linkml:owner okns:ical_transp ;
    linkml:range okns:string ;
    linkml:slot_uri ical:transp .

okns:ical_tzid a linkml:SlotDefinition ;
    dcterms:title "TZID" ;
    skos:definition "This property specifies the text value that uniquely identifies the \"VTIMEZONE\" calendar component." ;
    skos:editorialNote "No occurrences of this slot in the graph." ;
    skos:inScheme okns:ical ;
    skos:mappingRelation ical:tzid ;
    skos:note "description: value type: TEXT" ;
    linkml:definition_uri okns:ical_tzid ;
    linkml:domain okns:IcalVtimezone ;
    linkml:owner okns:ical_tzid ;
    linkml:range okns:string ;
    linkml:slot_uri ical:tzid .

okns:ical_tzname a linkml:SlotDefinition ;
    dcterms:title "TZNAME" ;
    skos:definition "This property specifies the customary designation for a time zone description." ;
    skos:editorialNote "No occurrences of this slot in the graph." ;
    skos:inScheme okns:ical ;
    skos:mappingRelation ical:tzname ;
    skos:note "description: value type: TEXT" ;
    linkml:definition_uri okns:ical_tzname ;
    linkml:domain okns:IcalVtimezone ;
    linkml:owner okns:ical_tzname ;
    linkml:range okns:string ;
    linkml:slot_uri ical:tzname .

okns:ical_tzoffsetto a linkml:SlotDefinition ;
    dcterms:title "TZOFFSETTO" ;
    skos:definition "This property specifies the offset which is in use in this time zone observance." ;
    skos:editorialNote "No occurrences of this slot in the graph." ;
    skos:inScheme okns:ical ;
    skos:mappingRelation ical:tzoffsetto ;
    skos:note "description: value type: UTC-OFFSET" ;
    linkml:definition_uri okns:ical_tzoffsetto ;
    linkml:domain okns:IcalVtimezone ;
    linkml:owner okns:ical_tzoffsetto ;
    linkml:range okns:string ;
    linkml:slot_uri ical:tzoffsetto .

okns:mo_activity a linkml:SlotDefinition ;
    dcterms:source <http://purl.org/ontology/mo/> ;
    dcterms:title "activity" ;
    skos:definition "Relates an artist to an activity period" ;
    skos:editorialNote "No occurrences of this slot in the graph." ;
    skos:inScheme okns:mo ;
    skos:mappingRelation <http://purl.org/ontology/mo/activity> ;
    linkml:definition_uri okns:mo_activity ;
    linkml:domain okns:MoMusicArtist ;
    linkml:inlined true ;
    linkml:owner okns:mo_activity ;
    linkml:range okns:MoActivity ;
    linkml:slot_uri <http://purl.org/ontology/mo/activity> .

okns:mo_activity_end a linkml:SlotDefinition ;
    dcterms:source <http://purl.org/ontology/mo/> ;
    dcterms:title "activity end" ;
    skos:definition "Relates an artist to a date at which its activity ended" ;
    skos:editorialNote "No occurrences of this slot in the graph." ;
    skos:inScheme okns:mo ;
    skos:mappingRelation <http://purl.org/ontology/mo/activity_end> ;
    linkml:definition_uri okns:mo_activity_end ;
    linkml:domain okns:MoMusicArtist ;
    linkml:owner okns:mo_activity_end ;
    linkml:range okns:date ;
    linkml:slot_uri <http://purl.org/ontology/mo/activity_end> .

okns:mo_activity_start a linkml:SlotDefinition ;
    dcterms:source <http://purl.org/ontology/mo/> ;
    dcterms:title "activity start" ;
    skos:definition "Relates an artist to a date at which its activity started" ;
    skos:editorialNote "No occurrences of this slot in the graph." ;
    skos:inScheme okns:mo ;
    skos:mappingRelation <http://purl.org/ontology/mo/activity_start> ;
    linkml:definition_uri okns:mo_activity_start ;
    linkml:domain okns:MoMusicArtist ;
    linkml:owner okns:mo_activity_start ;
    linkml:range okns:date ;
    linkml:slot_uri <http://purl.org/ontology/mo/activity_start> .

okns:mo_artist a linkml:SlotDefinition ;
    dcterms:source <http://purl.org/ontology/mo/> ;
    dcterms:title "artist" ;
    skos:definition "Relates a membership event with the corresponding artist" ;
    skos:editorialNote "No occurrences of this slot in the graph." ;
    skos:inScheme okns:mo ;
    skos:mappingRelation <http://purl.org/ontology/mo/artist> ;
    linkml:definition_uri okns:mo_artist ;
    linkml:domain okns:MoMembership ;
    linkml:inlined true ;
    linkml:owner okns:mo_artist ;
    linkml:range okns:FoafAgent ;
    linkml:slot_uri <http://purl.org/ontology/mo/artist> .

okns:mo_biography a linkml:SlotDefinition ;
    dcterms:source <http://purl.org/ontology/mo/> ;
    dcterms:title "biography" ;
    rdfs:subPropertyOf okns:foaf_isPrimaryTopicOf ;
    skos:definition "Used to link an artist to their online biography." ;
    skos:editorialNote "No occurrences of this slot in the graph." ;
    skos:inScheme okns:mo ;
    skos:mappingRelation <http://purl.org/ontology/mo/biography> ;
    linkml:definition_uri okns:mo_biography ;
    linkml:domain okns:MoMusicArtist ;
    linkml:inlined true ;
    linkml:owner okns:mo_biography ;
    linkml:range okns:FoafDocument ;
    linkml:slot_uri <http://purl.org/ontology/mo/biography> .

okns:mo_bitsPerSample a linkml:SlotDefinition ;
    dcterms:source <http://purl.org/ontology/mo/> ;
    skos:definition "Associates a digital signal to the number a bits used to encode one sample. Range is xsd:int." ;
    skos:editorialNote "No occurrences of this slot in the graph." ;
    skos:inScheme okns:mo ;
    skos:mappingRelation <http://purl.org/ontology/mo/bitsPerSample> ;
    skos:note "description: Associates a digital signal to the number a bits used to encode one sample. Range is xsd:int.",
        "source: http://purl.org/ontology/mo/" ;
    linkml:definition_uri okns:mo_bitsPerSample ;
    linkml:domain okns:MoDigitalSignal ;
    linkml:owner okns:mo_bitsPerSample ;
    linkml:range okns:int32 ;
    linkml:slot_uri <http://purl.org/ontology/mo/bitsPerSample> .

okns:mo_catalogue_number a linkml:SlotDefinition ;
    dcterms:source <http://purl.org/ontology/mo/> ;
    dcterms:title "catalogue number" ;
    rdfs:subPropertyOf okns:mo_uuid ;
    skos:definition "Links a release with the corresponding catalogue number" ;
    skos:editorialNote "No occurrences of this slot in the graph." ;
    skos:inScheme okns:mo ;
    skos:mappingRelation <http://purl.org/ontology/mo/catalogue_number> ;
    linkml:definition_uri okns:mo_catalogue_number ;
    linkml:domain okns:MoRelease ;
    linkml:owner okns:mo_catalogue_number ;
    linkml:range okns:string ;
    linkml:slot_uri <http://purl.org/ontology/mo/catalogue_number> .

okns:mo_channels a linkml:SlotDefinition ;
    dcterms:source <http://purl.org/ontology/mo/> ;
    skos:definition "Associates a signal to the number of channels it holds (mono --> 1, stereo --> 2). Range is xsd:int." ;
    skos:editorialNote "No occurrences of this slot in the graph." ;
    skos:inScheme okns:mo ;
    skos:mappingRelation <http://purl.org/ontology/mo/channels> ;
    skos:note "description: Associates a signal to the number of channels it holds (mono --> 1, stereo --> 2). Range is xsd:int.",
        "source: http://purl.org/ontology/mo/" ;
    linkml:definition_uri okns:mo_channels ;
    linkml:domain okns:MoSignal ;
    linkml:owner okns:mo_channels ;
    linkml:range okns:int32 ;
    linkml:slot_uri <http://purl.org/ontology/mo/channels> .

okns:mo_collaborated_with a linkml:SlotDefinition ;
    dcterms:source <http://purl.org/ontology/mo/> ;
    dcterms:title "collaborated_with" ;
    skos:definition "Used to relate two collaborating people on a work." ;
    skos:editorialNote "No occurrences of this slot in the graph." ;
    skos:inScheme okns:mo ;
    skos:mappingRelation <http://purl.org/ontology/mo/collaborated_with> ;
    linkml:definition_uri okns:mo_collaborated_with ;
    linkml:domain okns:FoafAgent ;
    linkml:inlined true ;
    linkml:owner okns:mo_collaborated_with ;
    linkml:range okns:FoafAgent ;
    linkml:slot_uri <http://purl.org/ontology/mo/collaborated_with> .

okns:mo_compilation_of a linkml:SlotDefinition ;
    dcterms:source <http://purl.org/ontology/mo/> ;
    dcterms:title "compilation_of" ;
    skos:definition "Indicates that a musical manifestation is a compilation of several Signals." ;
    skos:editorialNote "No occurrences of this slot in the graph." ;
    skos:inScheme okns:mo ;
    skos:mappingRelation <http://purl.org/ontology/mo/compilation_of> ;
    linkml:definition_uri okns:mo_compilation_of ;
    linkml:domain okns:MoMusicalManifestation ;
    linkml:inlined true ;
    linkml:owner okns:mo_compilation_of ;
    linkml:range okns:MoSignal ;
    linkml:slot_uri <http://purl.org/ontology/mo/compilation_of> .

okns:mo_composer a linkml:SlotDefinition ;
    dcterms:source <http://purl.org/ontology/mo/> ;
    dcterms:title "composer" ;
    rdfs:subPropertyOf okns:event_agent ;
    skos:definition "Associates a composition event to the actual composer. For example,␊        this property could link the event corresponding to the composition of the␊        Magic Flute in 1782 to Mozart himself (who obviously has a FOAF profile:-) )." ;
    skos:editorialNote "No occurrences of this slot in the graph." ;
    skos:inScheme okns:mo ;
    skos:mappingRelation <http://purl.org/ontology/mo/composer> ;
    linkml:definition_uri okns:mo_composer ;
    linkml:domain okns:MoComposition ;
    linkml:inlined true ;
    linkml:owner okns:mo_composer ;
    linkml:range okns:FoafAgent ;
    linkml:slot_uri <http://purl.org/ontology/mo/composer> .

okns:mo_discography a linkml:SlotDefinition ;
    dcterms:source <http://purl.org/ontology/mo/> ;
    dcterms:title "discography" ;
    rdfs:subPropertyOf okns:foaf_isPrimaryTopicOf ;
    skos:definition "Used to links an artist to an online discography of their musical works. The discography should provide a summary of each released musical work of the artist." ;
    skos:editorialNote "No occurrences of this slot in the graph." ;
    skos:inScheme okns:mo ;
    skos:mappingRelation <http://purl.org/ontology/mo/discography> ;
    linkml:definition_uri okns:mo_discography ;
    linkml:domain okns:MoMusicArtist ;
    linkml:inlined true ;
    linkml:owner okns:mo_discography ;
    linkml:range okns:FoafDocument ;
    linkml:slot_uri <http://purl.org/ontology/mo/discography> .

okns:mo_download a linkml:SlotDefinition ;
    dcterms:source <http://purl.org/ontology/mo/> ;
    dcterms:title "download" ;
    rdfs:subPropertyOf okns:foaf_isPrimaryTopicOf ;
    skos:definition "This property can be used to link from a person to the website where they make their works available, or from␊                a manifestation (a track or an album, for example) to a web page where it is available for␊                download.␊        ␊        It is better to use one of the three sub-properties instead of this one in order to specify wether the␊        content can be accessed for free (mo:freedownload), if it is just free preview material (mo:previewdownload), or␊        if it can be accessed for some money (mo:paiddownload) (this includes links to the Amazon store, for example).␊␊                This property MUST be used only if the content is just available through a web page (holding, for example␊                a Flash application) - it is better to link to actual content directly through the use of mo:available_as and␊                mo:Stream, mo:Torrent or mo:ED2K, etc. Therefore, Semantic Web user agents that don't know how to read HTML and even␊                less to rip streams from Flash applications can still access the audio content." ;
    skos:editorialNote "No occurrences of this slot in the graph." ;
    skos:inScheme okns:mo ;
    skos:mappingRelation <http://purl.org/ontology/mo/download> ;
    linkml:definition_uri okns:mo_download ;
    linkml:inlined true ;
    linkml:range okns:FoafDocument ;
    linkml:slot_uri <http://purl.org/ontology/mo/download> .

okns:mo_ean a linkml:SlotDefinition ;
    dcterms:source <http://purl.org/ontology/mo/> ;
    dcterms:title "ean" ;
    rdfs:subPropertyOf okns:mo_gtin ;
    skos:definition "The European Article Number (EAN) is a universal identifier for products, commonly printed in form of barcodes on them. The numbers represented by those codes can either be 8 or 13 digits long, with the 13-digit-version being most common. EANs form a superset of the North American Universal Product Code (UPC) as every UPC can be made an EAN by adding a leading zero to it. Additionally every EAN is also a Japanese Article Number (JAN). The identifiers were formerly assigned by EAN International which merged with Uniform Code Council (UCC, the guys behind the UPCs) and Electronic Commerce Council of Canada (ECCC) to become GS1." ;
    skos:editorialNote "No occurrences of this slot in the graph." ;
    skos:inScheme okns:mo ;
    skos:mappingRelation <http://purl.org/ontology/mo/ean> ;
    linkml:definition_uri okns:mo_ean ;
    linkml:domain okns:MoRelease ;
    linkml:owner okns:mo_ean ;
    linkml:range okns:string ;
    linkml:slot_uri <http://purl.org/ontology/mo/ean> .

okns:mo_encodes a linkml:SlotDefinition ;
    dcterms:source <http://purl.org/ontology/mo/> ;
    dcterms:title "encodes" ;
    skos:definition "Relates a MusicalItem (a track on a particular CD, an audio file, a stream somewhere) to the signal it encodes.␊␊        This is usually a lower-resolution version of the master signal (issued from a Recording event)." ;
    skos:editorialNote "No occurrences of this slot in the graph." ;
    skos:inScheme okns:mo ;
    skos:mappingRelation <http://purl.org/ontology/mo/encodes> ;
    linkml:definition_uri okns:mo_encodes ;
    linkml:domain okns:MoMusicalItem ;
    linkml:inlined true ;
    linkml:owner okns:mo_encodes ;
    linkml:range okns:MoSignal ;
    linkml:slot_uri <http://purl.org/ontology/mo/encodes> .

okns:mo_encoding a linkml:SlotDefinition ;
    dcterms:source <http://purl.org/ontology/mo/> ;
    dcterms:title "encoding" ;
    skos:definition "Method used to convert analog electronic signals into digital format such as \"MP3 CBR @ 128kbps\", \"OGG @ 160kbps\", \"FLAC\", etc." ;
    skos:editorialNote "No occurrences of this slot in the graph." ;
    skos:inScheme okns:mo ;
    skos:mappingRelation <http://purl.org/ontology/mo/encoding> ;
    linkml:definition_uri okns:mo_encoding ;
    linkml:domain okns:MoAudioFile ;
    linkml:inlined true ;
    linkml:owner okns:mo_encoding ;
    linkml:range okns:RdfsLiteral ;
    linkml:slot_uri <http://purl.org/ontology/mo/encoding> .

okns:mo_engineer a linkml:SlotDefinition ;
    dcterms:source <http://purl.org/ontology/mo/> ;
    rdfs:subPropertyOf okns:event_agent ;
    owl:inverseOf okns:mo_engineered ;
    skos:definition "Relates a performance or a recording to the engineer involved" ;
    skos:editorialNote "No occurrences of this slot in the graph." ;
    skos:inScheme okns:mo ;
    skos:mappingRelation <http://purl.org/ontology/mo/engineer> ;
    linkml:definition_uri okns:mo_engineer ;
    linkml:domain okns:Any ;
    linkml:inlined true ;
    linkml:range okns:FoafAgent ;
    linkml:slot_uri <http://purl.org/ontology/mo/engineer> .

okns:mo_event_homepage a linkml:SlotDefinition ;
    dcterms:source <http://purl.org/ontology/mo/> ;
    dcterms:title "event homepage" ;
    rdfs:subPropertyOf okns:foaf_isPrimaryTopicOf ;
    skos:definition "Links a particular event to a web page" ;
    skos:editorialNote "No occurrences of this slot in the graph." ;
    skos:inScheme okns:mo ;
    skos:mappingRelation <http://purl.org/ontology/mo/event_homepage> ;
    linkml:definition_uri okns:mo_event_homepage ;
    linkml:domain okns:EventEvent ;
    linkml:inlined true ;
    linkml:owner okns:mo_event_homepage ;
    linkml:range okns:FoafDocument ;
    linkml:slot_uri <http://purl.org/ontology/mo/event_homepage> .

okns:mo_exchange_item a linkml:SlotDefinition ;
    dcterms:source <http://purl.org/ontology/mo/> ;
    dcterms:title "exchange_item" ;
    skos:definition "A person, a group of person or an organization exchanging an exemplar of a single manifestation." ;
    skos:editorialNote "No occurrences of this slot in the graph." ;
    skos:inScheme okns:mo ;
    skos:mappingRelation <http://purl.org/ontology/mo/exchange_item> ;
    linkml:definition_uri okns:mo_exchange_item ;
    linkml:domain okns:FoafAgent ;
    linkml:inlined true ;
    linkml:owner okns:mo_exchange_item ;
    linkml:range okns:FrbrItem ;
    linkml:slot_uri <http://purl.org/ontology/mo/exchange_item> .

okns:mo_fanpage a linkml:SlotDefinition ;
    dcterms:source <http://purl.org/ontology/mo/> ;
    dcterms:title "fanpage" ;
    rdfs:subPropertyOf okns:foaf_isPrimaryTopicOf ;
    skos:definition "Used to link an artist to a fan-created webpage devoted to that artist." ;
    skos:editorialNote "No occurrences of this slot in the graph." ;
    skos:inScheme okns:mo ;
    skos:mappingRelation <http://purl.org/ontology/mo/fanpage> ;
    linkml:definition_uri okns:mo_fanpage ;
    linkml:domain okns:MoMusicArtist ;
    linkml:inlined true ;
    linkml:owner okns:mo_fanpage ;
    linkml:range okns:FoafDocument ;
    linkml:slot_uri <http://purl.org/ontology/mo/fanpage> .

okns:mo_grid a linkml:SlotDefinition ;
    dcterms:source <http://purl.org/ontology/mo/> ;
    dcterms:title "GRid" ;
    rdfs:subPropertyOf okns:mo_uuid ;
    skos:definition "The Global Release Identifier (GRid) is a system for uniquely identifying Releases of music over electronic networks (that is, online stores where you can buy music as digital files). As that it can be seen as the equivalent of the BarCode (or more correctly the GTIN) as found on physical releases of music. Like the ISRC (a code for identifying single recordings as found on releases) it was developed by the IFPI but it does not appear to be a standard of the ISO." ;
    skos:editorialNote "No occurrences of this slot in the graph." ;
    skos:inScheme okns:mo ;
    skos:mappingRelation <http://purl.org/ontology/mo/grid> ;
    linkml:definition_uri okns:mo_grid ;
    linkml:domain okns:MoRelease ;
    linkml:owner okns:mo_grid ;
    linkml:range okns:string ;
    linkml:slot_uri <http://purl.org/ontology/mo/grid> .

okns:mo_group a linkml:SlotDefinition ;
    dcterms:source <http://purl.org/ontology/mo/> ;
    dcterms:title "group" ;
    skos:definition "Relates a membership event with the corresponding group" ;
    skos:editorialNote "No occurrences of this slot in the graph." ;
    skos:inScheme okns:mo ;
    skos:mappingRelation <http://purl.org/ontology/mo/group> ;
    linkml:definition_uri okns:mo_group ;
    linkml:domain okns:MoMembership ;
    linkml:inlined true ;
    linkml:owner okns:mo_group ;
    linkml:range okns:FoafGroup ;
    linkml:slot_uri <http://purl.org/ontology/mo/group> .

okns:mo_instrument a linkml:SlotDefinition ;
    dcterms:source <http://purl.org/ontology/mo/> ;
    rdfs:subPropertyOf okns:event_factor ;
    skos:definition "Relates a performance to a musical instrument involved" ;
    skos:editorialNote "No occurrences of this slot in the graph." ;
    skos:inScheme okns:mo ;
    skos:mappingRelation <http://purl.org/ontology/mo/instrument> ;
    linkml:definition_uri okns:mo_instrument ;
    linkml:domain okns:MoPerformance ;
    linkml:inlined true ;
    linkml:owner okns:mo_instrument ;
    linkml:range okns:MoInstrument ;
    linkml:slot_uri <http://purl.org/ontology/mo/instrument> .

okns:mo_ipi a linkml:SlotDefinition ;
    dcterms:source <http://purl.org/ontology/mo/> ;
    dcterms:title "ipi" ;
    rdfs:subPropertyOf okns:mo_uuid ;
    skos:definition "The Interested Parties Information Code (IPI) is an ISO standard similar to ISBNs for identifying the people or groups with some involvement with a particular musical work / compositions." ;
    skos:editorialNote "No occurrences of this slot in the graph." ;
    skos:inScheme okns:mo ;
    skos:mappingRelation <http://purl.org/ontology/mo/ipi> ;
    linkml:definition_uri okns:mo_ipi ;
    linkml:domain okns:MoMusicArtist ;
    linkml:owner okns:mo_ipi ;
    linkml:range okns:string ;
    linkml:slot_uri <http://purl.org/ontology/mo/ipi> .

okns:mo_isrc a linkml:SlotDefinition ;
    dcterms:source <http://purl.org/ontology/mo/> ;
    dcterms:title "isrc" ;
    rdfs:subPropertyOf okns:mo_uuid ;
    skos:definition "The ISRC (International Standard Recording Code) is the international identification system for sound recordings and music videorecordings. ␊    Each ISRC is a unique and permanent identifier for a specific recording which can be permanently encoded into a product as its digital fingerprint. ␊    Encoded ISRC provide the means to automatically identify recordings for royalty payments." ;
    skos:editorialNote "No occurrences of this slot in the graph." ;
    skos:inScheme okns:mo ;
    skos:mappingRelation <http://purl.org/ontology/mo/isrc> ;
    linkml:definition_uri okns:mo_isrc ;
    linkml:domain okns:MoSignal ;
    linkml:owner okns:mo_isrc ;
    linkml:range okns:string ;
    linkml:slot_uri <http://purl.org/ontology/mo/isrc> .

okns:mo_iswc a linkml:SlotDefinition ;
    dcterms:source <http://purl.org/ontology/mo/> ;
    dcterms:title "iswc" ;
    rdfs:subPropertyOf okns:mo_uuid ;
    skos:definition "Links a musical work to the corresponding ISWC number" ;
    skos:editorialNote "No occurrences of this slot in the graph." ;
    skos:inScheme okns:mo ;
    skos:mappingRelation <http://purl.org/ontology/mo/iswc> ;
    linkml:definition_uri okns:mo_iswc ;
    linkml:domain okns:MoMusicalWork ;
    linkml:owner okns:mo_iswc ;
    linkml:range okns:string ;
    linkml:slot_uri <http://purl.org/ontology/mo/iswc> .

okns:mo_item a linkml:SlotDefinition ;
    dcterms:source <http://purl.org/ontology/mo/> ;
    rdfs:subPropertyOf okns:mo_available_as ;
    skos:definition "Relates a musical manifestation to a musical item (this album, and my particular cd) holding the␊                entire manifestation, and not just a part of it." ;
    skos:editorialNote "No occurrences of this slot in the graph." ;
    skos:inScheme okns:mo ;
    skos:mappingRelation <http://purl.org/ontology/mo/item> ;
    linkml:definition_uri okns:mo_item ;
    linkml:domain okns:MoMusicalManifestation ;
    linkml:inlined true ;
    linkml:owner okns:mo_item ;
    linkml:range okns:MoMusicalItem ;
    linkml:slot_uri <http://purl.org/ontology/mo/item> .

okns:mo_lc a linkml:SlotDefinition ;
    dcterms:source <http://purl.org/ontology/mo/> ;
    dcterms:title "lc" ;
    rdfs:subPropertyOf okns:mo_uuid ;
    skos:definition "The Label Code (LC) was introduced in 1977 by the IFPI (International Federation of Phonogram and Videogram Industries) in order to unmistakably identify the different record labels (see Introduction, Record labels) for rights purposes. The Label Code consists historically of 4 figures, presently being extended to 5 figures, preceded by LC and a dash (e.g. LC-0193 = Electrola; LC-0233 = His Master's Voice). Note that the number of countries using the LC is limited, and that the code given on the item is not always accurate." ;
    skos:editorialNote "No occurrences of this slot in the graph." ;
    skos:inScheme okns:mo ;
    skos:mappingRelation <http://purl.org/ontology/mo/lc> ;
    linkml:definition_uri okns:mo_lc ;
    linkml:domain okns:MoLabel ;
    linkml:owner okns:mo_lc ;
    linkml:range okns:string ;
    linkml:slot_uri <http://purl.org/ontology/mo/lc> .

okns:mo_lyrics a linkml:SlotDefinition ;
    dcterms:source <http://purl.org/ontology/mo/> ;
    dcterms:title "lyrics" ;
    skos:definition "Associates lyrics with a musical work" ;
    skos:editorialNote "No occurrences of this slot in the graph." ;
    skos:inScheme okns:mo ;
    skos:mappingRelation <http://purl.org/ontology/mo/lyrics> ;
    linkml:definition_uri okns:mo_lyrics ;
    linkml:domain okns:MoMusicalWork ;
    linkml:inlined true ;
    linkml:owner okns:mo_lyrics ;
    linkml:range okns:MoLyrics ;
    linkml:slot_uri <http://purl.org/ontology/mo/lyrics> .

okns:mo_media_type a linkml:SlotDefinition ;
    dcterms:source <http://purl.org/ontology/mo/> ;
    dcterms:title "has media type" ;
    rdfs:subPropertyOf okns:dct_format ;
    skos:definition "The mediatype (file format or MIME type, or physical medium) of a musical manifestation, e.g. a MP3, CD or vinyl." ;
    skos:editorialNote "No occurrences of this slot in the graph." ;
    skos:inScheme okns:mo ;
    skos:mappingRelation <http://purl.org/ontology/mo/media_type> ;
    linkml:definition_uri okns:mo_media_type ;
    linkml:domain okns:MoMusicalManifestation ;
    linkml:inlined true ;
    linkml:owner okns:mo_media_type ;
    linkml:range okns:DctMediaType ;
    linkml:slot_uri <http://purl.org/ontology/mo/media_type> .

okns:mo_member a linkml:SlotDefinition ;
    dcterms:source <http://purl.org/ontology/mo/> ;
    dcterms:title "member" ;
    rdfs:subPropertyOf okns:foaf_member ;
    skos:definition "Indicates a member of a musical group" ;
    skos:editorialNote "No occurrences of this slot in the graph." ;
    skos:inScheme okns:mo ;
    skos:mappingRelation <http://purl.org/ontology/mo/member> ;
    linkml:definition_uri okns:mo_member ;
    linkml:domain okns:MoMusicGroup ;
    linkml:inlined true ;
    linkml:owner okns:mo_member ;
    linkml:range okns:FoafAgent ;
    linkml:slot_uri <http://purl.org/ontology/mo/member> .

okns:mo_membership a linkml:SlotDefinition ;
    dcterms:source <http://purl.org/ontology/mo/> ;
    dcterms:title "membership" ;
    skos:definition "Relates an agent with related membership events" ;
    skos:editorialNote "No occurrences of this slot in the graph." ;
    skos:inScheme okns:mo ;
    skos:mappingRelation <http://purl.org/ontology/mo/membership> ;
    linkml:definition_uri okns:mo_membership ;
    linkml:domain okns:FoafAgent ;
    linkml:inlined true ;
    linkml:owner okns:mo_membership ;
    linkml:range okns:MoMembership ;
    linkml:slot_uri <http://purl.org/ontology/mo/membership> .

okns:mo_movement a linkml:SlotDefinition ;
    dcterms:source <http://purl.org/ontology/mo/> ;
    dcterms:title "has_movement" ;
    skos:definition "Indicates that a musical work has movements" ;
    skos:editorialNote "No occurrences of this slot in the graph." ;
    skos:inScheme okns:mo ;
    skos:mappingRelation <http://purl.org/ontology/mo/movement> ;
    linkml:definition_uri okns:mo_movement ;
    linkml:domain okns:MoMusicalWork ;
    linkml:inlined true ;
    linkml:owner okns:mo_movement ;
    linkml:range okns:MoMovement ;
    linkml:slot_uri <http://purl.org/ontology/mo/movement> .

okns:mo_movement_number a linkml:SlotDefinition ;
    dcterms:source <http://purl.org/ontology/mo/> ;
    dcterms:title "movement number" ;
    skos:definition "Indicates the position of a movement in a musical work." ;
    skos:editorialNote "No occurrences of this slot in the graph." ;
    skos:inScheme okns:mo ;
    skos:mappingRelation <http://purl.org/ontology/mo/movement_number> ;
    linkml:definition_uri okns:mo_movement_number ;
    linkml:domain okns:MoMovement ;
    linkml:owner okns:mo_movement_number ;
    linkml:range okns:int32 ;
    linkml:slot_uri <http://purl.org/ontology/mo/movement_number> .

okns:mo_myspace a linkml:SlotDefinition ;
    dcterms:source <http://purl.org/ontology/mo/> ;
    dcterms:title "myspace" ;
    rdfs:subPropertyOf okns:foaf_isPrimaryTopicOf ;
    skos:definition "Used to link a person to its corresponding MySpace page." ;
    skos:editorialNote "No occurrences of this slot in the graph." ;
    skos:inScheme okns:mo ;
    skos:mappingRelation <http://purl.org/ontology/mo/myspace> ;
    linkml:definition_uri okns:mo_myspace ;
    linkml:domain okns:FoafAgent ;
    linkml:inlined true ;
    linkml:owner okns:mo_myspace ;
    linkml:range okns:FoafDocument ;
    linkml:slot_uri <http://purl.org/ontology/mo/myspace> .

okns:mo_olga a linkml:SlotDefinition ;
    dcterms:source <http://purl.org/ontology/mo/> ;
    dcterms:title "olga" ;
    rdfs:subPropertyOf okns:foaf_isPrimaryTopicOf ;
    skos:definition "Used to link a track to a tabulature file for track in the On-Line Guitar Archive." ;
    skos:editorialNote "No occurrences of this slot in the graph." ;
    skos:inScheme okns:mo ;
    skos:mappingRelation <http://purl.org/ontology/mo/olga> ;
    linkml:definition_uri okns:mo_olga ;
    linkml:domain okns:MoTrack ;
    linkml:inlined true ;
    linkml:owner okns:mo_olga ;
    linkml:range okns:FoafDocument ;
    linkml:slot_uri <http://purl.org/ontology/mo/olga> .

okns:mo_onlinecommunity a linkml:SlotDefinition ;
    dcterms:source <http://purl.org/ontology/mo/> ;
    dcterms:title "onlinecommunity" ;
    rdfs:subPropertyOf okns:foaf_isPrimaryTopicOf ;
    skos:definition "Used to link a person with an online community web page like a blog, a wiki, a forum, a livejournal page, Etc." ;
    skos:editorialNote "No occurrences of this slot in the graph." ;
    skos:inScheme okns:mo ;
    skos:mappingRelation <http://purl.org/ontology/mo/onlinecommunity> ;
    linkml:definition_uri okns:mo_onlinecommunity ;
    linkml:domain okns:FoafAgent ;
    linkml:inlined true ;
    linkml:owner okns:mo_onlinecommunity ;
    linkml:range okns:FoafDocument ;
    linkml:slot_uri <http://purl.org/ontology/mo/onlinecommunity> .

okns:mo_opus a linkml:SlotDefinition ;
    dcterms:source <http://purl.org/ontology/mo/> ;
    dcterms:title "opus" ;
    skos:definition "Used to define a creative work, especially a musical composition numbered to designate the order of a composer's works." ;
    skos:editorialNote "No occurrences of this slot in the graph." ;
    skos:inScheme okns:mo ;
    skos:mappingRelation <http://purl.org/ontology/mo/opus> ;
    linkml:definition_uri okns:mo_opus ;
    linkml:domain okns:MoMusicalWork ;
    linkml:inlined true ;
    linkml:owner okns:mo_opus ;
    linkml:range okns:RdfsLiteral ;
    linkml:slot_uri <http://purl.org/ontology/mo/opus> .

okns:mo_origin a linkml:SlotDefinition ;
    dcterms:source <http://purl.org/ontology/mo/> ;
    dcterms:title "origin" ;
    skos:definition "Relates an artist to its geographic origin" ;
    skos:editorialNote "No occurrences of this slot in the graph." ;
    skos:inScheme okns:mo ;
    skos:mappingRelation <http://purl.org/ontology/mo/origin> ;
    linkml:definition_uri okns:mo_origin ;
    linkml:domain okns:MoMusicArtist ;
    linkml:inlined true ;
    linkml:owner okns:mo_origin ;
    linkml:range okns:WgsSpatialThing ;
    linkml:slot_uri <http://purl.org/ontology/mo/origin> .

okns:mo_other_release_of a linkml:SlotDefinition ;
    dcterms:source <http://purl.org/ontology/mo/> ;
    dcterms:title "other_release_of" ;
    skos:definition "Indicates that two musical manifestations are essentially the same." ;
    skos:editorialNote "No occurrences of this slot in the graph." ;
    skos:inScheme okns:mo ;
    skos:mappingRelation <http://purl.org/ontology/mo/other_release_of> ;
    linkml:definition_uri okns:mo_other_release_of ;
    linkml:domain okns:MoMusicalManifestation ;
    linkml:inlined true ;
    linkml:owner okns:mo_other_release_of ;
    linkml:range okns:MoMusicalManifestation ;
    linkml:slot_uri <http://purl.org/ontology/mo/other_release_of> .

okns:mo_performed_in a linkml:SlotDefinition ;
    dcterms:source <http://purl.org/ontology/mo/> ;
    dcterms:title "performed in" ;
    rdfs:subPropertyOf okns:event_isFactorOf ;
    owl:inverseOf okns:mo_performance_of ;
    skos:definition "Associates a Musical Work or an Score to Performances in which they were␊        a factor. For example, I might use this property in order to ␊        associate the Magic Flute to a particular performance at the Opera␊        Bastille last year." ;
    skos:editorialNote "No occurrences of this slot in the graph." ;
    skos:inScheme okns:mo ;
    skos:mappingRelation <http://purl.org/ontology/mo/performed_in> ;
    linkml:definition_uri okns:mo_performed_in ;
    linkml:domain okns:Any ;
    linkml:inlined true ;
    linkml:range okns:MoPerformance ;
    linkml:slot_uri <http://purl.org/ontology/mo/performed_in> .

okns:mo_possess_item a linkml:SlotDefinition ;
    dcterms:source <http://purl.org/ontology/mo/> ;
    dcterms:title "possess_item" ;
    skos:definition "A person, a group of person or an organization possessing an exemplar of a single manifestation." ;
    skos:editorialNote "No occurrences of this slot in the graph." ;
    skos:inScheme okns:mo ;
    skos:mappingRelation <http://purl.org/ontology/mo/possess_item> ;
    linkml:definition_uri okns:mo_possess_item ;
    linkml:domain okns:FoafAgent ;
    linkml:inlined true ;
    linkml:owner okns:mo_possess_item ;
    linkml:range okns:FrbrItem ;
    linkml:slot_uri <http://purl.org/ontology/mo/possess_item> .

okns:mo_preview a linkml:SlotDefinition ;
    dcterms:source <http://purl.org/ontology/mo/> ;
    rdfs:subPropertyOf okns:mo_available_as ;
    skos:definition "Relates a musical manifestation to a musical item (this album, and my particular cd), which holds␊                a preview of the manifestation (eg. one track for an album, or a snippet for a track)" ;
    skos:editorialNote "No occurrences of this slot in the graph." ;
    skos:inScheme okns:mo ;
    skos:mappingRelation <http://purl.org/ontology/mo/preview> ;
    linkml:definition_uri okns:mo_preview ;
    linkml:domain okns:MoMusicalManifestation ;
    linkml:inlined true ;
    linkml:owner okns:mo_preview ;
    linkml:range okns:MoMusicalItem ;
    linkml:slot_uri <http://purl.org/ontology/mo/preview> .

okns:mo_produced_signal a linkml:SlotDefinition ;
    dcterms:source <http://purl.org/ontology/mo/> ;
    dcterms:title "produced signal" ;
    rdfs:subPropertyOf okns:event_product ;
    skos:definition "Associates a Recording to the outputted signal." ;
    skos:editorialNote "No occurrences of this slot in the graph." ;
    skos:inScheme okns:mo ;
    skos:mappingRelation <http://purl.org/ontology/mo/produced_signal> ;
    linkml:definition_uri okns:mo_produced_signal ;
    linkml:domain okns:MoRecording ;
    linkml:inlined true ;
    linkml:owner okns:mo_produced_signal ;
    linkml:range okns:MoSignal ;
    linkml:slot_uri <http://purl.org/ontology/mo/produced_signal> .

okns:mo_produced_signal_group a linkml:SlotDefinition ;
    dcterms:source <http://purl.org/ontology/mo/> ;
    dcterms:title "produced signal group" ;
    rdfs:subPropertyOf okns:event_product ;
    skos:definition "Associates a recording session with a group of master signals produced by it." ;
    skos:editorialNote "No occurrences of this slot in the graph." ;
    skos:inScheme okns:mo ;
    skos:mappingRelation <http://purl.org/ontology/mo/produced_signal_group> ;
    linkml:definition_uri okns:mo_produced_signal_group ;
    linkml:domain okns:MoRecordingSession ;
    linkml:inlined true ;
    linkml:owner okns:mo_produced_signal_group ;
    linkml:range okns:MoSignalGroup ;
    linkml:slot_uri <http://purl.org/ontology/mo/produced_signal_group> .

okns:mo_produced_sound a linkml:SlotDefinition ;
    dcterms:source <http://purl.org/ontology/mo/> ;
    dcterms:title "produced sound" ;
    rdfs:subPropertyOf okns:event_product ;
    skos:definition "Associates a Performance to a physical Sound that is being produced by it." ;
    skos:editorialNote "No occurrences of this slot in the graph." ;
    skos:inScheme okns:mo ;
    skos:mappingRelation <http://purl.org/ontology/mo/produced_sound> ;
    linkml:definition_uri okns:mo_produced_sound ;
    linkml:domain okns:MoPerformance ;
    linkml:inlined true ;
    linkml:owner okns:mo_produced_sound ;
    linkml:range okns:MoSound ;
    linkml:slot_uri <http://purl.org/ontology/mo/produced_sound> .

okns:mo_publishing_location a linkml:SlotDefinition ;
    dcterms:source <http://purl.org/ontology/mo/> ;
    dcterms:title "publishingLocation" ;
    skos:definition "Relates a musical manifestation to its publication location." ;
    skos:editorialNote "No occurrences of this slot in the graph." ;
    skos:inScheme okns:mo ;
    skos:mappingRelation <http://purl.org/ontology/mo/publishing_location> ;
    linkml:definition_uri okns:mo_publishing_location ;
    linkml:domain okns:MoMusicalManifestation ;
    linkml:inlined true ;
    linkml:owner okns:mo_publishing_location ;
    linkml:range okns:WgsSpatialThing ;
    linkml:slot_uri <http://purl.org/ontology/mo/publishing_location> .

okns:mo_puid a linkml:SlotDefinition ;
    dcterms:source <http://purl.org/ontology/mo/> ;
    dcterms:title "puid" ;
    skos:definition "Link a signal to the PUIDs associated with it, that is, PUID computed from MusicalItems (mo:AudioFile) ␊        derived from this signal.␊        PUIDs (Portable Unique IDentifier) are the IDs used in the ␊        proprietary MusicDNS AudioFingerprinting system which is operated by MusicIP.␊␊        Using PUIDs, one (with some luck) can identify the Signal object associated with a particular audio file, therefore allowing␊        to access further information (on which release this track is featured? etc.). Using some more metadata one can identify␊        the particular Track corresponding to the audio file (a track on a particular release)." ;
    skos:editorialNote "No occurrences of this slot in the graph." ;
    skos:inScheme okns:mo ;
    skos:mappingRelation <http://purl.org/ontology/mo/puid> ;
    linkml:definition_uri okns:mo_puid ;
    linkml:domain okns:MoSignal ;
    linkml:owner okns:mo_puid ;
    linkml:range okns:string ;
    linkml:slot_uri <http://purl.org/ontology/mo/puid> .

okns:mo_record a linkml:SlotDefinition ;
    dcterms:source <http://purl.org/ontology/mo/> ;
    dcterms:title "released record" ;
    skos:definition "Associates a release with the records it contains. A single release can be associated with multiple records, for example for a multi-disc release." ;
    skos:editorialNote "No occurrences of this slot in the graph." ;
    skos:inScheme okns:mo ;
    skos:mappingRelation <http://purl.org/ontology/mo/record> ;
    linkml:definition_uri okns:mo_record ;
    linkml:domain okns:MoRelease ;
    linkml:inlined true ;
    linkml:owner okns:mo_record ;
    linkml:range okns:MoRecord ;
    linkml:slot_uri <http://purl.org/ontology/mo/record> .

okns:mo_record_count a linkml:SlotDefinition ;
    dcterms:source <http://purl.org/ontology/mo/> ;
    dcterms:title "record count" ;
    skos:definition "Associates a release with the number of records it contains, e.g. the number of discs it contains in the case of a multi-disc release." ;
    skos:editorialNote "No occurrences of this slot in the graph." ;
    skos:inScheme okns:mo ;
    skos:mappingRelation <http://purl.org/ontology/mo/record_count> ;
    linkml:definition_uri okns:mo_record_count ;
    linkml:domain okns:MoRelease ;
    linkml:owner okns:mo_record_count ;
    linkml:range okns:int32 ;
    linkml:slot_uri <http://purl.org/ontology/mo/record_count> .

okns:mo_record_number a linkml:SlotDefinition ;
    dcterms:source <http://purl.org/ontology/mo/> ;
    dcterms:title "has record number" ;
    skos:definition "Indicates the position of a record in a release (e.g. a 2xLP, etc.)." ;
    skos:editorialNote "No occurrences of this slot in the graph." ;
    skos:inScheme okns:mo ;
    skos:mappingRelation <http://purl.org/ontology/mo/record_number> ;
    linkml:definition_uri okns:mo_record_number ;
    linkml:domain okns:MoRecord ;
    linkml:owner okns:mo_record_number ;
    linkml:range okns:unsignedinteger ;
    linkml:slot_uri <http://purl.org/ontology/mo/record_number> .

okns:mo_record_side a linkml:SlotDefinition ;
    dcterms:source <http://purl.org/ontology/mo/> ;
    dcterms:title "has record side" ;
    skos:definition "Associates the side on a vinyl record, where a track is located, e.g. A, B, C, etc. This property can then also be used ␊in conjunction with mo:track_number, so that one can infer e.g. \"A1\", that means, track number 1 on side A." ;
    skos:editorialNote "No occurrences of this slot in the graph." ;
    skos:inScheme okns:mo ;
    skos:mappingRelation <http://purl.org/ontology/mo/record_side> ;
    linkml:definition_uri okns:mo_record_side ;
    linkml:domain okns:MoTrack ;
    linkml:owner okns:mo_record_side ;
    linkml:range okns:string ;
    linkml:slot_uri <http://purl.org/ontology/mo/record_side> .

okns:mo_recordedAs a linkml:SlotDefinition ;
    skos:editorialNote "No occurrences of this slot in the graph." ;
    skos:exactMatch <http://purl.org/ontology/mo/recorded_as> ;
    skos:inScheme okns:mo ;
    skos:mappingRelation <http://purl.org/ontology/mo/recordedAs> ;
    linkml:definition_uri okns:mo_recordedAs ;
    linkml:domain okns:MoPerformance ;
    linkml:inlined true ;
    linkml:owner okns:mo_recordedAs ;
    linkml:range okns:MoSignal ;
    linkml:slot_uri <http://purl.org/ontology/mo/recordedAs> .

okns:mo_release a linkml:SlotDefinition ;
    dcterms:source <http://purl.org/ontology/mo/> ;
    dcterms:title "release" ;
    rdfs:subPropertyOf okns:event_product ;
    skos:definition "Associates a release with the corresponding release event" ;
    skos:editorialNote "No occurrences of this slot in the graph." ;
    skos:inScheme okns:mo ;
    skos:mappingRelation <http://purl.org/ontology/mo/release> ;
    linkml:definition_uri okns:mo_release ;
    linkml:domain okns:MoReleaseEvent ;
    linkml:inlined true ;
    linkml:owner okns:mo_release ;
    linkml:range okns:MoRelease ;
    linkml:slot_uri <http://purl.org/ontology/mo/release> .

okns:mo_release_status a linkml:SlotDefinition ;
    dcterms:source <http://purl.org/ontology/mo/> ;
    skos:definition "Relates a musical manifestation to its release status (bootleg, ...)" ;
    skos:editorialNote "No occurrences of this slot in the graph." ;
    skos:inScheme okns:mo ;
    skos:mappingRelation <http://purl.org/ontology/mo/release_status> ;
    linkml:definition_uri okns:mo_release_status ;
    linkml:domain okns:MoMusicalManifestation ;
    linkml:inlined true ;
    linkml:owner okns:mo_release_status ;
    linkml:range okns:MoReleaseStatus ;
    linkml:slot_uri <http://purl.org/ontology/mo/release_status> .

okns:mo_release_type a linkml:SlotDefinition ;
    dcterms:source <http://purl.org/ontology/mo/> ;
    skos:definition "Relates a musical manifestation to its release type (interview, spoken word, album, ...)" ;
    skos:editorialNote "No occurrences of this slot in the graph." ;
    skos:inScheme okns:mo ;
    skos:mappingRelation <http://purl.org/ontology/mo/release_type> ;
    linkml:definition_uri okns:mo_release_type ;
    linkml:domain okns:MoMusicalManifestation ;
    linkml:inlined true ;
    linkml:owner okns:mo_release_type ;
    linkml:range okns:MoReleaseType ;
    linkml:slot_uri <http://purl.org/ontology/mo/release_type> .

okns:mo_remixer a linkml:SlotDefinition ;
    dcterms:source <http://purl.org/ontology/mo/> ;
    dcterms:title "remixer" ;
    rdfs:subPropertyOf okns:mo_interpreter ;
    owl:inverseOf okns:mo_remixed ;
    skos:definition "Used to relate a musical work or the expression of a musical work to an artist who remixed it. ␊    ␊This involves taking just one other musical work and using audio editing to make it sound like a significantly different, but usually still recognisable, song. It can be used to link an artist to a single song that they remixed, or, if they remixed an entire musical work." ;
    skos:editorialNote "No occurrences of this slot in the graph." ;
    skos:inScheme okns:mo ;
    skos:mappingRelation <http://purl.org/ontology/mo/remixer> ;
    linkml:definition_uri okns:mo_remixer ;
    linkml:domain okns:MoSignal ;
    linkml:inlined true ;
    linkml:range okns:Any ;
    linkml:slot_uri <http://purl.org/ontology/mo/remixer> .

okns:mo_sample_rate a linkml:SlotDefinition ;
    dcterms:source <http://purl.org/ontology/mo/> ;
    skos:definition "Associates a digital signal to its sample rate. It might be easier to express it this way instead of␊        defining a timeline map:-) Range is xsd:float." ;
    skos:editorialNote "No occurrences of this slot in the graph." ;
    skos:inScheme okns:mo ;
    skos:mappingRelation <http://purl.org/ontology/mo/sample_rate> ;
    skos:note """description: Associates a digital signal to its sample rate. It might be easier to express it this way instead of
        defining a timeline map:-) Range is xsd:float.""",
        "source: http://purl.org/ontology/mo/" ;
    linkml:definition_uri okns:mo_sample_rate ;
    linkml:domain okns:MoDigitalSignal ;
    linkml:owner okns:mo_sample_rate ;
    linkml:range okns:float ;
    linkml:slot_uri <http://purl.org/ontology/mo/sample_rate> .

okns:mo_sampler a linkml:SlotDefinition ;
    dcterms:source <http://purl.org/ontology/mo/> ;
    dcterms:title "sampler" ;
    rdfs:subPropertyOf okns:mo_interpreter ;
    owl:inverseOf okns:mo_sampled ;
    skos:definition "Used to relate the signal of a musical work to an artist who sampled it." ;
    skos:editorialNote "No occurrences of this slot in the graph." ;
    skos:inScheme okns:mo ;
    skos:mappingRelation <http://purl.org/ontology/mo/sampler> ;
    linkml:definition_uri okns:mo_sampler ;
    linkml:domain okns:MoSignal ;
    linkml:inlined true ;
    linkml:range okns:Any ;
    linkml:slot_uri <http://purl.org/ontology/mo/sampler> .

okns:mo_sell_item a linkml:SlotDefinition ;
    dcterms:source <http://purl.org/ontology/mo/> ;
    dcterms:title "sell_item" ;
    skos:definition "A person, a group of person or an organization selling an exemplar of a single manifestation." ;
    skos:editorialNote "No occurrences of this slot in the graph." ;
    skos:inScheme okns:mo ;
    skos:mappingRelation <http://purl.org/ontology/mo/sell_item> ;
    linkml:definition_uri okns:mo_sell_item ;
    linkml:domain okns:FoafAgent ;
    linkml:inlined true ;
    linkml:owner okns:mo_sell_item ;
    linkml:range okns:FrbrItem ;
    linkml:slot_uri <http://purl.org/ontology/mo/sell_item> .

okns:mo_signal a linkml:SlotDefinition ;
    dcterms:source <http://purl.org/ontology/mo/> ;
    dcterms:title "signal" ;
    skos:definition "Associates a group of signals with one of the signals it contains" ;
    skos:editorialNote "No occurrences of this slot in the graph." ;
    skos:inScheme okns:mo ;
    skos:mappingRelation <http://purl.org/ontology/mo/signal> ;
    linkml:definition_uri okns:mo_signal ;
    linkml:domain okns:MoSignalGroup ;
    linkml:inlined true ;
    linkml:owner okns:mo_signal ;
    linkml:range okns:MoSignal ;
    linkml:slot_uri <http://purl.org/ontology/mo/signal> .

okns:mo_singer a linkml:SlotDefinition ;
    dcterms:source <http://purl.org/ontology/mo/> ;
    rdfs:subPropertyOf okns:mo_performer ;
    skos:definition "Relates a performance to an involved singer" ;
    skos:editorialNote "No occurrences of this slot in the graph." ;
    skos:inScheme okns:mo ;
    skos:mappingRelation <http://purl.org/ontology/mo/singer> ;
    linkml:definition_uri okns:mo_singer ;
    linkml:domain okns:MoPerformance ;
    linkml:inlined true ;
    linkml:owner okns:mo_singer ;
    linkml:range okns:FoafAgent ;
    linkml:slot_uri <http://purl.org/ontology/mo/singer> .

okns:mo_supporting_musician a linkml:SlotDefinition ;
    dcterms:source <http://purl.org/ontology/mo/> ;
    dcterms:title "supporting_musician" ;
    skos:definition "Used to relate an artist doing long-time instrumental or vocal support for another artist." ;
    skos:editorialNote "No occurrences of this slot in the graph." ;
    skos:inScheme okns:mo ;
    skos:mappingRelation <http://purl.org/ontology/mo/supporting_musician> ;
    linkml:definition_uri okns:mo_supporting_musician ;
    linkml:domain okns:MoMusicArtist ;
    linkml:inlined true ;
    linkml:owner okns:mo_supporting_musician ;
    linkml:range okns:MoMusicArtist ;
    linkml:slot_uri <http://purl.org/ontology/mo/supporting_musician> .

okns:mo_text a linkml:SlotDefinition ;
    dcterms:source <http://purl.org/ontology/mo/> ;
    dcterms:title "text" ;
    skos:definition "Associates lyrics with their text." ;
    skos:editorialNote "No occurrences of this slot in the graph." ;
    skos:inScheme okns:mo ;
    skos:mappingRelation <http://purl.org/ontology/mo/text> ;
    linkml:definition_uri okns:mo_text ;
    linkml:domain okns:MoLyrics ;
    linkml:inlined true ;
    linkml:owner okns:mo_text ;
    linkml:range okns:Any ;
    linkml:slot_uri <http://purl.org/ontology/mo/text> .

okns:mo_time a linkml:SlotDefinition ;
    dcterms:source <http://purl.org/ontology/mo/> ;
    dcterms:title "time" ;
    skos:definition "Associates a Signal to a time object - its actual domain" ;
    skos:editorialNote "No occurrences of this slot in the graph." ;
    skos:inScheme okns:mo ;
    skos:mappingRelation <http://purl.org/ontology/mo/time> ;
    linkml:definition_uri okns:mo_time ;
    linkml:domain okns:MoSignal ;
    linkml:inlined true ;
    linkml:owner okns:mo_time ;
    linkml:range okns:TimeTemporalEntity ;
    linkml:slot_uri <http://purl.org/ontology/mo/time> .

okns:mo_track a linkml:SlotDefinition ;
    dcterms:source <http://purl.org/ontology/mo/> ;
    dcterms:title "track" ;
    skos:definition "Indicates a part of a musical manifestation - in this particular case, a track." ;
    skos:editorialNote "No occurrences of this slot in the graph." ;
    skos:inScheme okns:mo ;
    skos:mappingRelation <http://purl.org/ontology/mo/track> ;
    linkml:definition_uri okns:mo_track ;
    linkml:domain okns:MoRecord ;
    linkml:inlined true ;
    linkml:owner okns:mo_track ;
    linkml:range okns:MoTrack ;
    linkml:slot_uri <http://purl.org/ontology/mo/track> .

okns:mo_track_count a linkml:SlotDefinition ;
    dcterms:source <http://purl.org/ontology/mo/> ;
    dcterms:title "track count" ;
    skos:definition "The track count of a record" ;
    skos:editorialNote "No occurrences of this slot in the graph." ;
    skos:inScheme okns:mo ;
    skos:mappingRelation <http://purl.org/ontology/mo/track_count> ;
    linkml:definition_uri okns:mo_track_count ;
    linkml:domain okns:MoRecord ;
    linkml:owner okns:mo_track_count ;
    linkml:range okns:int32 ;
    linkml:slot_uri <http://purl.org/ontology/mo/track_count> .

okns:mo_track_number a linkml:SlotDefinition ;
    dcterms:source <http://purl.org/ontology/mo/> ;
    dcterms:title "track number" ;
    skos:definition "Indicates the position of a track on a record medium (a CD, etc.)." ;
    skos:editorialNote "No occurrences of this slot in the graph." ;
    skos:inScheme okns:mo ;
    skos:mappingRelation <http://purl.org/ontology/mo/track_number> ;
    linkml:definition_uri okns:mo_track_number ;
    linkml:domain okns:MoTrack ;
    linkml:owner okns:mo_track_number ;
    linkml:range okns:unsignedinteger ;
    linkml:slot_uri <http://purl.org/ontology/mo/track_number> .

okns:mo_translation_of a linkml:SlotDefinition ;
    dcterms:source <http://purl.org/ontology/mo/> ;
    dcterms:title "translation_of" ;
    skos:definition "Indicates that a work or the expression of a work has translated or transliterated into another expression of a work." ;
    skos:editorialNote "No occurrences of this slot in the graph." ;
    skos:inScheme okns:mo ;
    skos:mappingRelation <http://purl.org/ontology/mo/translation_of> ;
    linkml:definition_uri okns:mo_translation_of ;
    linkml:domain okns:FrbrExpression ;
    linkml:inlined true ;
    linkml:owner okns:mo_translation_of ;
    linkml:range okns:FrbrExpression ;
    linkml:slot_uri <http://purl.org/ontology/mo/translation_of> .

okns:mo_tribute_to a linkml:SlotDefinition ;
    dcterms:source <http://purl.org/ontology/mo/> ;
    dcterms:title "tribute_to" ;
    skos:definition "Indicates a musical work or the expression of a musical work that is a tribute to an artist - normally consisting of music being composed by the artist but performed by other artists." ;
    skos:editorialNote "No occurrences of this slot in the graph." ;
    skos:inScheme okns:mo ;
    skos:mappingRelation <http://purl.org/ontology/mo/tribute_to> ;
    linkml:definition_uri okns:mo_tribute_to ;
    linkml:domain okns:MoMusicalManifestation ;
    linkml:inlined true ;
    linkml:owner okns:mo_tribute_to ;
    linkml:range okns:MoMusicArtist ;
    linkml:slot_uri <http://purl.org/ontology/mo/tribute_to> .

okns:mo_trmid a linkml:SlotDefinition ;
    dcterms:source <http://purl.org/ontology/mo/> ;
    dcterms:title "trmid" ;
    skos:definition "Indicates the TRMID of a track.␊        TRM IDs are MusicBrainz' old AudioFingerprinting system. ␊        TRM (TRM Recognizes Music) IDs are (somewhat) unique ids that represent ␊        the audio signature of a musical piece (see AudioFingerprint)." ;
    skos:editorialNote "No occurrences of this slot in the graph." ;
    skos:inScheme okns:mo ;
    skos:mappingRelation <http://purl.org/ontology/mo/trmid> ;
    linkml:definition_uri okns:mo_trmid ;
    linkml:domain okns:MoSignal ;
    linkml:owner okns:mo_trmid ;
    linkml:range okns:string ;
    linkml:slot_uri <http://purl.org/ontology/mo/trmid> .

okns:mo_upc a linkml:SlotDefinition ;
    dcterms:source <http://purl.org/ontology/mo/> ;
    dcterms:title "upc" ;
    rdfs:subPropertyOf okns:mo_gtin ;
    skos:definition "UPC stands for \"Universal Product Code\", which was the original barcode used in the United States and Canada. The UPC (now officially EAN.UCC-12 is a numerical method of identifying products without redundancy worldwide for all types of products in the retail sector. The EAN is a superset of the original UPC increasing the digits to 13 with the prefix 0 reserved for UPC. As of 2005, manufacturers are only allowed to use the new 13-digit codes on their items, rather than having two separate numbers." ;
    skos:editorialNote "No occurrences of this slot in the graph." ;
    skos:inScheme okns:mo ;
    skos:mappingRelation <http://purl.org/ontology/mo/upc> ;
    linkml:definition_uri okns:mo_upc ;
    linkml:domain okns:MoRelease ;
    linkml:owner okns:mo_upc ;
    linkml:range okns:string ;
    linkml:slot_uri <http://purl.org/ontology/mo/upc> .

okns:mo_want_item a linkml:SlotDefinition ;
    dcterms:source <http://purl.org/ontology/mo/> ;
    dcterms:title "want_item" ;
    skos:definition "A person, a group of person or an organization wanting an exemplar of a single manifestation." ;
    skos:editorialNote "No occurrences of this slot in the graph." ;
    skos:inScheme okns:mo ;
    skos:mappingRelation <http://purl.org/ontology/mo/want_item> ;
    linkml:definition_uri okns:mo_want_item ;
    linkml:domain okns:FoafAgent ;
    linkml:inlined true ;
    linkml:owner okns:mo_want_item ;
    linkml:range okns:FrbrItem ;
    linkml:slot_uri <http://purl.org/ontology/mo/want_item> .

okns:owl_allValuesFrom a linkml:SlotDefinition ;
    dcterms:source owl: ;
    dcterms:title "allValuesFrom" ;
    skos:definition "The property that determines the class that a universal property restriction refers to." ;
    skos:editorialNote "No occurrences of this slot in the graph." ;
    skos:inScheme okns:owl-rdf-rdfs ;
    skos:mappingRelation owl:allValuesFrom ;
    linkml:definition_uri okns:owl_allValuesFrom ;
    linkml:domain okns:OwlRestriction ;
    linkml:inlined true ;
    linkml:owner okns:owl_allValuesFrom ;
    linkml:range okns:RdfsClass ;
    linkml:slot_uri owl:allValuesFrom .

okns:owl_annotatedProperty a linkml:SlotDefinition ;
    dcterms:source owl: ;
    dcterms:title "annotatedProperty" ;
    skos:definition "The property that determines the predicate of an annotated axiom or annotated annotation." ;
    skos:editorialNote "No occurrences of this slot in the graph." ;
    skos:inScheme okns:owl-rdf-rdfs ;
    skos:mappingRelation owl:annotatedProperty ;
    linkml:definition_uri okns:owl_annotatedProperty ;
    linkml:domain okns:RdfsResource ;
    linkml:inlined true ;
    linkml:owner okns:owl_annotatedProperty ;
    linkml:range okns:RdfsResource ;
    linkml:slot_uri owl:annotatedProperty .

okns:owl_annotatedSource a linkml:SlotDefinition ;
    dcterms:source owl: ;
    dcterms:title "annotatedSource" ;
    skos:definition "The property that determines the subject of an annotated axiom or annotated annotation." ;
    skos:editorialNote "No occurrences of this slot in the graph." ;
    skos:inScheme okns:owl-rdf-rdfs ;
    skos:mappingRelation owl:annotatedSource ;
    linkml:definition_uri okns:owl_annotatedSource ;
    linkml:domain okns:RdfsResource ;
    linkml:inlined true ;
    linkml:owner okns:owl_annotatedSource ;
    linkml:range okns:RdfsResource ;
    linkml:slot_uri owl:annotatedSource .

okns:owl_annotatedTarget a linkml:SlotDefinition ;
    dcterms:source owl: ;
    dcterms:title "annotatedTarget" ;
    skos:definition "The property that determines the object of an annotated axiom or annotated annotation." ;
    skos:editorialNote "No occurrences of this slot in the graph." ;
    skos:inScheme okns:owl-rdf-rdfs ;
    skos:mappingRelation owl:annotatedTarget ;
    linkml:definition_uri okns:owl_annotatedTarget ;
    linkml:domain okns:RdfsResource ;
    linkml:inlined true ;
    linkml:owner okns:owl_annotatedTarget ;
    linkml:range okns:RdfsResource ;
    linkml:slot_uri owl:annotatedTarget .

okns:owl_assertionProperty a linkml:SlotDefinition ;
    dcterms:source owl: ;
    dcterms:title "assertionProperty" ;
    skos:definition "The property that determines the predicate of a negative property assertion." ;
    skos:editorialNote "No occurrences of this slot in the graph." ;
    skos:inScheme okns:owl-rdf-rdfs ;
    skos:mappingRelation owl:assertionProperty ;
    linkml:definition_uri okns:owl_assertionProperty ;
    linkml:domain okns:OwlNegativePropertyAssertion ;
    linkml:inlined true ;
    linkml:owner okns:owl_assertionProperty ;
    linkml:range okns:RdfProperty ;
    linkml:slot_uri owl:assertionProperty .

okns:owl_backwardCompatibleWith a linkml:SlotDefinition ;
    dcterms:source owl: ;
    dcterms:title "backwardCompatibleWith" ;
    skos:definition "The annotation property that indicates that a given ontology is backward compatible with another ontology." ;
    skos:editorialNote "No occurrences of this slot in the graph." ;
    skos:inScheme okns:owl-rdf-rdfs ;
    skos:mappingRelation owl:backwardCompatibleWith ;
    linkml:definition_uri okns:owl_backwardCompatibleWith ;
    linkml:domain okns:OwlOntology ;
    linkml:inlined true ;
    linkml:owner okns:owl_backwardCompatibleWith ;
    linkml:range okns:OwlOntology ;
    linkml:slot_uri owl:backwardCompatibleWith .

okns:owl_bottomDataProperty a linkml:SlotDefinition ;
    dcterms:source owl: ;
    dcterms:title "bottomDataProperty" ;
    skos:definition "The data property that does not relate any individual to any data value." ;
    skos:editorialNote "No occurrences of this slot in the graph." ;
    skos:inScheme okns:owl-rdf-rdfs ;
    skos:mappingRelation owl:bottomDataProperty ;
    linkml:definition_uri okns:owl_bottomDataProperty ;
    linkml:domain okns:OwlThing ;
    linkml:inlined true ;
    linkml:owner okns:owl_bottomDataProperty ;
    linkml:range okns:RdfsLiteral ;
    linkml:slot_uri owl:bottomDataProperty .

okns:owl_bottomObjectProperty a linkml:SlotDefinition ;
    dcterms:source owl: ;
    dcterms:title "bottomObjectProperty" ;
    skos:definition "The object property that does not relate any two individuals." ;
    skos:editorialNote "No occurrences of this slot in the graph." ;
    skos:inScheme okns:owl-rdf-rdfs ;
    skos:mappingRelation owl:bottomObjectProperty ;
    linkml:definition_uri okns:owl_bottomObjectProperty ;
    linkml:domain okns:OwlThing ;
    linkml:inlined true ;
    linkml:owner okns:owl_bottomObjectProperty ;
    linkml:range okns:OwlThing ;
    linkml:slot_uri owl:bottomObjectProperty .

okns:owl_cardinality a linkml:SlotDefinition ;
    dcterms:source owl: ;
    dcterms:title "cardinality" ;
    skos:definition "The property that determines the cardinality of an exact cardinality restriction." ;
    skos:editorialNote "No occurrences of this slot in the graph." ;
    skos:inScheme okns:owl-rdf-rdfs ;
    skos:mappingRelation owl:cardinality ;
    linkml:definition_uri okns:owl_cardinality ;
    linkml:domain okns:OwlRestriction ;
    linkml:owner okns:owl_cardinality ;
    linkml:range okns:unsignedinteger ;
    linkml:slot_uri owl:cardinality .

okns:owl_complementOf a linkml:SlotDefinition ;
    dcterms:source owl: ;
    dcterms:title "complementOf" ;
    skos:definition "The property that determines that a given class is the complement of another class." ;
    skos:editorialNote "No occurrences of this slot in the graph." ;
    skos:inScheme okns:owl-rdf-rdfs ;
    skos:mappingRelation owl:complementOf ;
    linkml:definition_uri okns:owl_complementOf ;
    linkml:domain okns:OwlClass ;
    linkml:inlined true ;
    linkml:owner okns:owl_complementOf ;
    linkml:range okns:OwlClass ;
    linkml:slot_uri owl:complementOf .

okns:owl_datatypeComplementOf a linkml:SlotDefinition ;
    dcterms:source owl: ;
    dcterms:title "datatypeComplementOf" ;
    skos:definition "The property that determines that a given data range is the complement of another data range with respect to the data domain." ;
    skos:editorialNote "No occurrences of this slot in the graph." ;
    skos:inScheme okns:owl-rdf-rdfs ;
    skos:mappingRelation owl:datatypeComplementOf ;
    linkml:definition_uri okns:owl_datatypeComplementOf ;
    linkml:domain okns:RdfsDatatype ;
    linkml:inlined true ;
    linkml:owner okns:owl_datatypeComplementOf ;
    linkml:range okns:RdfsDatatype ;
    linkml:slot_uri owl:datatypeComplementOf .

okns:owl_deprecated a linkml:SlotDefinition ;
    dcterms:source owl: ;
    dcterms:title "deprecated" ;
    skos:definition "The annotation property that indicates that a given entity has been deprecated." ;
    skos:editorialNote "No occurrences of this slot in the graph." ;
    skos:inScheme okns:owl-rdf-rdfs ;
    skos:mappingRelation owl:deprecated ;
    linkml:definition_uri okns:owl_deprecated ;
    linkml:domain okns:RdfsResource ;
    linkml:inlined true ;
    linkml:owner okns:owl_deprecated ;
    linkml:range okns:RdfsResource ;
    linkml:slot_uri owl:deprecated .

okns:owl_differentFrom a linkml:SlotDefinition ;
    dcterms:source owl: ;
    dcterms:title "differentFrom" ;
    skos:definition "The property that determines that two given individuals are different." ;
    skos:editorialNote "No occurrences of this slot in the graph." ;
    skos:inScheme okns:owl-rdf-rdfs ;
    skos:mappingRelation owl:differentFrom ;
    linkml:definition_uri okns:owl_differentFrom ;
    linkml:domain okns:OwlThing ;
    linkml:inlined true ;
    linkml:owner okns:owl_differentFrom ;
    linkml:range okns:OwlThing ;
    linkml:slot_uri owl:differentFrom .

okns:owl_disjointUnionOf a linkml:SlotDefinition ;
    dcterms:source owl: ;
    dcterms:title "disjointUnionOf" ;
    skos:definition "The property that determines that a given class is equivalent to the disjoint union of a collection of other classes." ;
    skos:editorialNote "No occurrences of this slot in the graph." ;
    skos:inScheme okns:owl-rdf-rdfs ;
    skos:mappingRelation owl:disjointUnionOf ;
    linkml:definition_uri okns:owl_disjointUnionOf ;
    linkml:domain okns:OwlClass ;
    linkml:inlined true ;
    linkml:owner okns:owl_disjointUnionOf ;
    linkml:range okns:RdfList ;
    linkml:slot_uri owl:disjointUnionOf .

okns:owl_disjointWith a linkml:SlotDefinition ;
    dcterms:source owl: ;
    dcterms:title "disjointWith" ;
    skos:definition "The property that determines that two given classes are disjoint." ;
    skos:editorialNote "No occurrences of this slot in the graph." ;
    skos:inScheme okns:owl-rdf-rdfs ;
    skos:mappingRelation owl:disjointWith ;
    linkml:definition_uri okns:owl_disjointWith ;
    linkml:domain okns:OwlClass ;
    linkml:inlined true ;
    linkml:owner okns:owl_disjointWith ;
    linkml:range okns:OwlClass ;
    linkml:slot_uri owl:disjointWith .

okns:owl_distinctMembers a linkml:SlotDefinition ;
    dcterms:source owl: ;
    dcterms:title "distinctMembers" ;
    skos:definition "The property that determines the collection of pairwise different individuals in a owl:AllDifferent axiom." ;
    skos:editorialNote "No occurrences of this slot in the graph." ;
    skos:inScheme okns:owl-rdf-rdfs ;
    skos:mappingRelation owl:distinctMembers ;
    linkml:definition_uri okns:owl_distinctMembers ;
    linkml:domain okns:OwlAllDifferent ;
    linkml:inlined true ;
    linkml:owner okns:owl_distinctMembers ;
    linkml:range okns:RdfList ;
    linkml:slot_uri owl:distinctMembers .

okns:owl_equivalentClass a linkml:SlotDefinition ;
    dcterms:source owl: ;
    dcterms:title "equivalentClass" ;
    skos:definition "The property that determines that two given classes are equivalent, and that is used to specify datatype definitions." ;
    skos:editorialNote "No occurrences of this slot in the graph." ;
    skos:inScheme okns:owl-rdf-rdfs ;
    skos:mappingRelation owl:equivalentClass ;
    linkml:definition_uri okns:owl_equivalentClass ;
    linkml:domain okns:RdfsClass ;
    linkml:inlined true ;
    linkml:owner okns:owl_equivalentClass ;
    linkml:range okns:RdfsClass ;
    linkml:slot_uri owl:equivalentClass .

okns:owl_equivalentProperty a linkml:SlotDefinition ;
    dcterms:source owl: ;
    dcterms:title "equivalentProperty" ;
    skos:definition "The property that determines that two given properties are equivalent." ;
    skos:editorialNote "No occurrences of this slot in the graph." ;
    skos:inScheme okns:owl-rdf-rdfs ;
    skos:mappingRelation owl:equivalentProperty ;
    linkml:definition_uri okns:owl_equivalentProperty ;
    linkml:domain okns:RdfProperty ;
    linkml:inlined true ;
    linkml:owner okns:owl_equivalentProperty ;
    linkml:range okns:RdfProperty ;
    linkml:slot_uri owl:equivalentProperty .

okns:owl_hasKey a linkml:SlotDefinition ;
    dcterms:source owl: ;
    dcterms:title "hasKey" ;
    skos:definition "The property that determines the collection of properties that jointly build a key." ;
    skos:editorialNote "No occurrences of this slot in the graph." ;
    skos:inScheme okns:owl-rdf-rdfs ;
    skos:mappingRelation owl:hasKey ;
    linkml:definition_uri okns:owl_hasKey ;
    linkml:domain okns:OwlClass ;
    linkml:inlined true ;
    linkml:owner okns:owl_hasKey ;
    linkml:range okns:RdfList ;
    linkml:slot_uri owl:hasKey .

okns:owl_hasSelf a linkml:SlotDefinition ;
    dcterms:source owl: ;
    dcterms:title "hasSelf" ;
    skos:definition "The property that determines the property that a self restriction refers to." ;
    skos:editorialNote "No occurrences of this slot in the graph." ;
    skos:inScheme okns:owl-rdf-rdfs ;
    skos:mappingRelation owl:hasSelf ;
    linkml:definition_uri okns:owl_hasSelf ;
    linkml:domain okns:OwlRestriction ;
    linkml:inlined true ;
    linkml:owner okns:owl_hasSelf ;
    linkml:range okns:RdfsResource ;
    linkml:slot_uri owl:hasSelf .

okns:owl_hasValue a linkml:SlotDefinition ;
    dcterms:source owl: ;
    dcterms:title "hasValue" ;
    skos:definition "The property that determines the individual that a has-value restriction refers to." ;
    skos:editorialNote "No occurrences of this slot in the graph." ;
    skos:inScheme okns:owl-rdf-rdfs ;
    skos:mappingRelation owl:hasValue ;
    linkml:definition_uri okns:owl_hasValue ;
    linkml:domain okns:OwlRestriction ;
    linkml:inlined true ;
    linkml:owner okns:owl_hasValue ;
    linkml:range okns:RdfsResource ;
    linkml:slot_uri owl:hasValue .

okns:owl_imports a linkml:SlotDefinition ;
    dcterms:source owl: ;
    dcterms:title "imports" ;
    skos:definition "The property that is used for importing other ontologies into a given ontology." ;
    skos:editorialNote "No occurrences of this slot in the graph." ;
    skos:inScheme okns:owl-rdf-rdfs ;
    skos:mappingRelation owl:imports ;
    linkml:definition_uri okns:owl_imports ;
    linkml:domain okns:OwlOntology ;
    linkml:inlined true ;
    linkml:owner okns:owl_imports ;
    linkml:range okns:OwlOntology ;
    linkml:slot_uri owl:imports .

okns:owl_incompatibleWith a linkml:SlotDefinition ;
    dcterms:source owl: ;
    dcterms:title "incompatibleWith" ;
    skos:definition "The annotation property that indicates that a given ontology is incompatible with another ontology." ;
    skos:editorialNote "No occurrences of this slot in the graph." ;
    skos:inScheme okns:owl-rdf-rdfs ;
    skos:mappingRelation owl:incompatibleWith ;
    linkml:definition_uri okns:owl_incompatibleWith ;
    linkml:domain okns:OwlOntology ;
    linkml:inlined true ;
    linkml:owner okns:owl_incompatibleWith ;
    linkml:range okns:OwlOntology ;
    linkml:slot_uri owl:incompatibleWith .

okns:owl_intersectionOf a linkml:SlotDefinition ;
    dcterms:source owl: ;
    dcterms:title "intersectionOf" ;
    skos:definition "The property that determines the collection of classes or data ranges that build an intersection." ;
    skos:editorialNote "No occurrences of this slot in the graph." ;
    skos:inScheme okns:owl-rdf-rdfs ;
    skos:mappingRelation owl:intersectionOf ;
    linkml:definition_uri okns:owl_intersectionOf ;
    linkml:domain okns:RdfsClass ;
    linkml:inlined true ;
    linkml:owner okns:owl_intersectionOf ;
    linkml:range okns:RdfList ;
    linkml:slot_uri owl:intersectionOf .

okns:owl_inverseOf a linkml:SlotDefinition ;
    dcterms:source owl: ;
    dcterms:title "inverseOf" ;
    skos:definition "The property that determines that two given properties are inverse." ;
    skos:editorialNote "No occurrences of this slot in the graph." ;
    skos:inScheme okns:owl-rdf-rdfs ;
    skos:mappingRelation owl:inverseOf ;
    linkml:definition_uri okns:owl_inverseOf ;
    linkml:domain okns:OwlObjectProperty ;
    linkml:inlined true ;
    linkml:owner okns:owl_inverseOf ;
    linkml:range okns:OwlObjectProperty ;
    linkml:slot_uri owl:inverseOf .

okns:owl_maxCardinality a linkml:SlotDefinition ;
    dcterms:source owl: ;
    dcterms:title "maxCardinality" ;
    skos:definition "The property that determines the cardinality of a maximum cardinality restriction." ;
    skos:editorialNote "No occurrences of this slot in the graph." ;
    skos:inScheme okns:owl-rdf-rdfs ;
    skos:mappingRelation owl:maxCardinality ;
    linkml:definition_uri okns:owl_maxCardinality ;
    linkml:domain okns:OwlRestriction ;
    linkml:owner okns:owl_maxCardinality ;
    linkml:range okns:unsignedinteger ;
    linkml:slot_uri owl:maxCardinality .

okns:owl_maxQualifiedCardinality a linkml:SlotDefinition ;
    dcterms:source owl: ;
    dcterms:title "maxQualifiedCardinality" ;
    skos:definition "The property that determines the cardinality of a maximum qualified cardinality restriction." ;
    skos:editorialNote "No occurrences of this slot in the graph." ;
    skos:inScheme okns:owl-rdf-rdfs ;
    skos:mappingRelation owl:maxQualifiedCardinality ;
    linkml:definition_uri okns:owl_maxQualifiedCardinality ;
    linkml:domain okns:OwlRestriction ;
    linkml:owner okns:owl_maxQualifiedCardinality ;
    linkml:range okns:unsignedinteger ;
    linkml:slot_uri owl:maxQualifiedCardinality .

okns:owl_members a linkml:SlotDefinition ;
    dcterms:source owl: ;
    dcterms:title "members" ;
    skos:definition "The property that determines the collection of members in either a owl:AllDifferent, owl:AllDisjointClasses or owl:AllDisjointProperties axiom." ;
    skos:editorialNote "No occurrences of this slot in the graph." ;
    skos:inScheme okns:owl-rdf-rdfs ;
    skos:mappingRelation owl:members ;
    linkml:definition_uri okns:owl_members ;
    linkml:domain okns:RdfsResource ;
    linkml:inlined true ;
    linkml:owner okns:owl_members ;
    linkml:range okns:RdfList ;
    linkml:slot_uri owl:members .

okns:owl_minCardinality a linkml:SlotDefinition ;
    dcterms:source owl: ;
    dcterms:title "minCardinality" ;
    skos:definition "The property that determines the cardinality of a minimum cardinality restriction." ;
    skos:editorialNote "No occurrences of this slot in the graph." ;
    skos:inScheme okns:owl-rdf-rdfs ;
    skos:mappingRelation owl:minCardinality ;
    linkml:definition_uri okns:owl_minCardinality ;
    linkml:domain okns:OwlRestriction ;
    linkml:owner okns:owl_minCardinality ;
    linkml:range okns:unsignedinteger ;
    linkml:slot_uri owl:minCardinality .

okns:owl_minQualifiedCardinality a linkml:SlotDefinition ;
    dcterms:source owl: ;
    dcterms:title "minQualifiedCardinality" ;
    skos:definition "The property that determines the cardinality of a minimum qualified cardinality restriction." ;
    skos:editorialNote "No occurrences of this slot in the graph." ;
    skos:inScheme okns:owl-rdf-rdfs ;
    skos:mappingRelation owl:minQualifiedCardinality ;
    linkml:definition_uri okns:owl_minQualifiedCardinality ;
    linkml:domain okns:OwlRestriction ;
    linkml:owner okns:owl_minQualifiedCardinality ;
    linkml:range okns:unsignedinteger ;
    linkml:slot_uri owl:minQualifiedCardinality .

okns:owl_onClass a linkml:SlotDefinition ;
    dcterms:source owl: ;
    dcterms:title "onClass" ;
    skos:definition "The property that determines the class that a qualified object cardinality restriction refers to." ;
    skos:editorialNote "No occurrences of this slot in the graph." ;
    skos:inScheme okns:owl-rdf-rdfs ;
    skos:mappingRelation owl:onClass ;
    linkml:definition_uri okns:owl_onClass ;
    linkml:domain okns:OwlRestriction ;
    linkml:inlined true ;
    linkml:owner okns:owl_onClass ;
    linkml:range okns:OwlClass ;
    linkml:slot_uri owl:onClass .

okns:owl_onDataRange a linkml:SlotDefinition ;
    dcterms:source owl: ;
    dcterms:title "onDataRange" ;
    skos:definition "The property that determines the data range that a qualified data cardinality restriction refers to." ;
    skos:editorialNote "No occurrences of this slot in the graph." ;
    skos:inScheme okns:owl-rdf-rdfs ;
    skos:mappingRelation owl:onDataRange ;
    linkml:definition_uri okns:owl_onDataRange ;
    linkml:domain okns:OwlRestriction ;
    linkml:inlined true ;
    linkml:owner okns:owl_onDataRange ;
    linkml:range okns:RdfsDatatype ;
    linkml:slot_uri owl:onDataRange .

okns:owl_onDatatype a linkml:SlotDefinition ;
    dcterms:source owl: ;
    dcterms:title "onDatatype" ;
    skos:definition "The property that determines the datatype that a datatype restriction refers to." ;
    skos:editorialNote "No occurrences of this slot in the graph." ;
    skos:inScheme okns:owl-rdf-rdfs ;
    skos:mappingRelation owl:onDatatype ;
    linkml:definition_uri okns:owl_onDatatype ;
    linkml:domain okns:RdfsDatatype ;
    linkml:inlined true ;
    linkml:owner okns:owl_onDatatype ;
    linkml:range okns:RdfsDatatype ;
    linkml:slot_uri owl:onDatatype .

okns:owl_onProperties a linkml:SlotDefinition ;
    dcterms:source owl: ;
    dcterms:title "onProperties" ;
    skos:definition "The property that determines the n-tuple of properties that a property restriction on an n-ary data range refers to." ;
    skos:editorialNote "No occurrences of this slot in the graph." ;
    skos:inScheme okns:owl-rdf-rdfs ;
    skos:mappingRelation owl:onProperties ;
    linkml:definition_uri okns:owl_onProperties ;
    linkml:domain okns:OwlRestriction ;
    linkml:inlined true ;
    linkml:owner okns:owl_onProperties ;
    linkml:range okns:RdfList ;
    linkml:slot_uri owl:onProperties .

okns:owl_onProperty a linkml:SlotDefinition ;
    dcterms:source owl: ;
    dcterms:title "onProperty" ;
    skos:definition "The property that determines the property that a property restriction refers to." ;
    skos:editorialNote "No occurrences of this slot in the graph." ;
    skos:inScheme okns:owl-rdf-rdfs ;
    skos:mappingRelation owl:onProperty ;
    linkml:definition_uri okns:owl_onProperty ;
    linkml:domain okns:OwlRestriction ;
    linkml:inlined true ;
    linkml:owner okns:owl_onProperty ;
    linkml:range okns:RdfProperty ;
    linkml:slot_uri owl:onProperty .

okns:owl_oneOf a linkml:SlotDefinition ;
    dcterms:source owl: ;
    dcterms:title "oneOf" ;
    skos:definition "The property that determines the collection of individuals or data values that build an enumeration." ;
    skos:editorialNote "No occurrences of this slot in the graph." ;
    skos:inScheme okns:owl-rdf-rdfs ;
    skos:mappingRelation owl:oneOf ;
    linkml:definition_uri okns:owl_oneOf ;
    linkml:domain okns:RdfsClass ;
    linkml:inlined true ;
    linkml:owner okns:owl_oneOf ;
    linkml:range okns:RdfList ;
    linkml:slot_uri owl:oneOf .

okns:owl_priorVersion a linkml:SlotDefinition ;
    dcterms:source owl: ;
    dcterms:title "priorVersion" ;
    skos:definition "The annotation property that indicates the predecessor ontology of a given ontology." ;
    skos:editorialNote "No occurrences of this slot in the graph." ;
    skos:inScheme okns:owl-rdf-rdfs ;
    skos:mappingRelation owl:priorVersion ;
    linkml:definition_uri okns:owl_priorVersion ;
    linkml:domain okns:OwlOntology ;
    linkml:inlined true ;
    linkml:owner okns:owl_priorVersion ;
    linkml:range okns:OwlOntology ;
    linkml:slot_uri owl:priorVersion .

okns:owl_propertyChainAxiom a linkml:SlotDefinition ;
    dcterms:source owl: ;
    dcterms:title "propertyChainAxiom" ;
    skos:definition "The property that determines the n-tuple of properties that build a sub property chain of a given property." ;
    skos:editorialNote "No occurrences of this slot in the graph." ;
    skos:inScheme okns:owl-rdf-rdfs ;
    skos:mappingRelation owl:propertyChainAxiom ;
    linkml:definition_uri okns:owl_propertyChainAxiom ;
    linkml:domain okns:OwlObjectProperty ;
    linkml:inlined true ;
    linkml:owner okns:owl_propertyChainAxiom ;
    linkml:range okns:RdfList ;
    linkml:slot_uri owl:propertyChainAxiom .

okns:owl_propertyDisjointWith a linkml:SlotDefinition ;
    dcterms:source owl: ;
    dcterms:title "propertyDisjointWith" ;
    skos:definition "The property that determines that two given properties are disjoint." ;
    skos:editorialNote "No occurrences of this slot in the graph." ;
    skos:inScheme okns:owl-rdf-rdfs ;
    skos:mappingRelation owl:propertyDisjointWith ;
    linkml:definition_uri okns:owl_propertyDisjointWith ;
    linkml:domain okns:RdfProperty ;
    linkml:inlined true ;
    linkml:owner okns:owl_propertyDisjointWith ;
    linkml:range okns:RdfProperty ;
    linkml:slot_uri owl:propertyDisjointWith .

okns:owl_qualifiedCardinality a linkml:SlotDefinition ;
    dcterms:source owl: ;
    dcterms:title "qualifiedCardinality" ;
    skos:definition "The property that determines the cardinality of an exact qualified cardinality restriction." ;
    skos:editorialNote "No occurrences of this slot in the graph." ;
    skos:inScheme okns:owl-rdf-rdfs ;
    skos:mappingRelation owl:qualifiedCardinality ;
    linkml:definition_uri okns:owl_qualifiedCardinality ;
    linkml:domain okns:OwlRestriction ;
    linkml:owner okns:owl_qualifiedCardinality ;
    linkml:range okns:unsignedinteger ;
    linkml:slot_uri owl:qualifiedCardinality .

okns:owl_sameAs a linkml:SlotDefinition ;
    dcterms:source owl: ;
    dcterms:title "sameAs" ;
    skos:definition "The property that determines that two given individuals are equal." ;
    skos:editorialNote "No occurrences of this slot in the graph." ;
    skos:inScheme okns:owl-rdf-rdfs ;
    skos:mappingRelation owl:sameAs ;
    linkml:definition_uri okns:owl_sameAs ;
    linkml:domain okns:OwlThing ;
    linkml:inlined true ;
    linkml:owner okns:owl_sameAs ;
    linkml:range okns:OwlThing ;
    linkml:slot_uri owl:sameAs .

okns:owl_someValuesFrom a linkml:SlotDefinition ;
    dcterms:source owl: ;
    dcterms:title "someValuesFrom" ;
    skos:definition "The property that determines the class that an existential property restriction refers to." ;
    skos:editorialNote "No occurrences of this slot in the graph." ;
    skos:inScheme okns:owl-rdf-rdfs ;
    skos:mappingRelation owl:someValuesFrom ;
    linkml:definition_uri okns:owl_someValuesFrom ;
    linkml:domain okns:OwlRestriction ;
    linkml:inlined true ;
    linkml:owner okns:owl_someValuesFrom ;
    linkml:range okns:RdfsClass ;
    linkml:slot_uri owl:someValuesFrom .

okns:owl_sourceIndividual a linkml:SlotDefinition ;
    dcterms:source owl: ;
    dcterms:title "sourceIndividual" ;
    skos:definition "The property that determines the subject of a negative property assertion." ;
    skos:editorialNote "No occurrences of this slot in the graph." ;
    skos:inScheme okns:owl-rdf-rdfs ;
    skos:mappingRelation owl:sourceIndividual ;
    linkml:definition_uri okns:owl_sourceIndividual ;
    linkml:domain okns:OwlNegativePropertyAssertion ;
    linkml:inlined true ;
    linkml:owner okns:owl_sourceIndividual ;
    linkml:range okns:OwlThing ;
    linkml:slot_uri owl:sourceIndividual .

okns:owl_targetIndividual a linkml:SlotDefinition ;
    dcterms:source owl: ;
    dcterms:title "targetIndividual" ;
    skos:definition "The property that determines the object of a negative object property assertion." ;
    skos:editorialNote "No occurrences of this slot in the graph." ;
    skos:inScheme okns:owl-rdf-rdfs ;
    skos:mappingRelation owl:targetIndividual ;
    linkml:definition_uri okns:owl_targetIndividual ;
    linkml:domain okns:OwlNegativePropertyAssertion ;
    linkml:inlined true ;
    linkml:owner okns:owl_targetIndividual ;
    linkml:range okns:OwlThing ;
    linkml:slot_uri owl:targetIndividual .

okns:owl_targetValue a linkml:SlotDefinition ;
    dcterms:source owl: ;
    dcterms:title "targetValue" ;
    skos:definition "The property that determines the value of a negative data property assertion." ;
    skos:editorialNote "No occurrences of this slot in the graph." ;
    skos:inScheme okns:owl-rdf-rdfs ;
    skos:mappingRelation owl:targetValue ;
    linkml:definition_uri okns:owl_targetValue ;
    linkml:domain okns:OwlNegativePropertyAssertion ;
    linkml:inlined true ;
    linkml:owner okns:owl_targetValue ;
    linkml:range okns:RdfsLiteral ;
    linkml:slot_uri owl:targetValue .

okns:owl_topDataProperty a linkml:SlotDefinition ;
    dcterms:source owl: ;
    dcterms:title "topDataProperty" ;
    skos:definition "The data property that relates every individual to every data value." ;
    skos:editorialNote "No occurrences of this slot in the graph." ;
    skos:inScheme okns:owl-rdf-rdfs ;
    skos:mappingRelation owl:topDataProperty ;
    linkml:definition_uri okns:owl_topDataProperty ;
    linkml:domain okns:OwlThing ;
    linkml:inlined true ;
    linkml:owner okns:owl_topDataProperty ;
    linkml:range okns:RdfsLiteral ;
    linkml:slot_uri owl:topDataProperty .

okns:owl_topObjectProperty a linkml:SlotDefinition ;
    dcterms:source owl: ;
    dcterms:title "topObjectProperty" ;
    skos:definition "The object property that relates every two individuals." ;
    skos:editorialNote "No occurrences of this slot in the graph." ;
    skos:inScheme okns:owl-rdf-rdfs ;
    skos:mappingRelation owl:topObjectProperty ;
    linkml:definition_uri okns:owl_topObjectProperty ;
    linkml:domain okns:OwlThing ;
    linkml:inlined true ;
    linkml:owner okns:owl_topObjectProperty ;
    linkml:range okns:OwlThing ;
    linkml:slot_uri owl:topObjectProperty .

okns:owl_unionOf a linkml:SlotDefinition ;
    dcterms:source owl: ;
    dcterms:title "unionOf" ;
    skos:definition "The property that determines the collection of classes or data ranges that build a union." ;
    skos:editorialNote "No occurrences of this slot in the graph." ;
    skos:inScheme okns:owl-rdf-rdfs ;
    skos:mappingRelation owl:unionOf ;
    linkml:definition_uri okns:owl_unionOf ;
    linkml:domain okns:RdfsClass ;
    linkml:inlined true ;
    linkml:owner okns:owl_unionOf ;
    linkml:range okns:RdfList ;
    linkml:slot_uri owl:unionOf .

okns:owl_versionIRI a linkml:SlotDefinition ;
    dcterms:source owl: ;
    dcterms:title "versionIRI" ;
    skos:definition "The property that identifies the version IRI of an ontology." ;
    skos:editorialNote "No occurrences of this slot in the graph." ;
    skos:inScheme okns:owl-rdf-rdfs ;
    skos:mappingRelation owl:versionIRI ;
    linkml:definition_uri okns:owl_versionIRI ;
    linkml:domain okns:OwlOntology ;
    linkml:inlined true ;
    linkml:owner okns:owl_versionIRI ;
    linkml:range okns:OwlOntology ;
    linkml:slot_uri owl:versionIRI .

okns:owl_versionInfo a linkml:SlotDefinition ;
    dcterms:source owl: ;
    dcterms:title "versionInfo" ;
    skos:definition "The annotation property that provides version information for an ontology or another OWL construct." ;
    skos:editorialNote "No occurrences of this slot in the graph." ;
    skos:inScheme okns:owl-rdf-rdfs ;
    skos:mappingRelation owl:versionInfo ;
    linkml:definition_uri okns:owl_versionInfo ;
    linkml:domain okns:RdfsResource ;
    linkml:inlined true ;
    linkml:owner okns:owl_versionInfo ;
    linkml:range okns:RdfsResource ;
    linkml:slot_uri owl:versionInfo .

okns:owl_withRestrictions a linkml:SlotDefinition ;
    dcterms:source owl: ;
    dcterms:title "withRestrictions" ;
    skos:definition "The property that determines the collection of facet-value pairs that define a datatype restriction." ;
    skos:editorialNote "No occurrences of this slot in the graph." ;
    skos:inScheme okns:owl-rdf-rdfs ;
    skos:mappingRelation owl:withRestrictions ;
    linkml:definition_uri okns:owl_withRestrictions ;
    linkml:domain okns:RdfsDatatype ;
    linkml:inlined true ;
    linkml:owner okns:owl_withRestrictions ;
    linkml:range okns:RdfList ;
    linkml:slot_uri owl:withRestrictions .

okns:rdf_direction a linkml:SlotDefinition ;
    dcterms:source rdf: ;
    dcterms:title "direction" ;
    rdfs:seeAlso <https://www.w3.org/TR/json-ld11/#the-rdf-compoundliteral-class-and-the-rdf-language-and-rdf-direction-properties> ;
    skos:definition "The base direction component of a CompoundLiteral." ;
    skos:editorialNote "No occurrences of this slot in the graph." ;
    skos:inScheme okns:owl-rdf-rdfs ;
    skos:mappingRelation rdf:direction ;
    linkml:definition_uri okns:rdf_direction ;
    linkml:domain okns:RdfCompoundLiteral ;
    linkml:inlined true ;
    linkml:owner okns:rdf_direction ;
    linkml:range okns:Any ;
    linkml:slot_uri rdf:direction .

okns:rdf_first a linkml:SlotDefinition ;
    dcterms:source rdf: ;
    dcterms:title "first" ;
    skos:definition "The first item in the subject RDF list." ;
    skos:editorialNote "No occurrences of this slot in the graph." ;
    skos:inScheme okns:owl-rdf-rdfs ;
    skos:mappingRelation rdf:first ;
    linkml:definition_uri okns:rdf_first ;
    linkml:domain okns:RdfList ;
    linkml:inlined true ;
    linkml:owner okns:rdf_first ;
    linkml:range okns:RdfsResource ;
    linkml:slot_uri rdf:first .

okns:rdf_language a linkml:SlotDefinition ;
    dcterms:source rdf: ;
    dcterms:title "language" ;
    rdfs:seeAlso <https://www.w3.org/TR/json-ld11/#the-rdf-compoundliteral-class-and-the-rdf-language-and-rdf-direction-properties> ;
    skos:definition "The language component of a CompoundLiteral." ;
    skos:editorialNote "No occurrences of this slot in the graph." ;
    skos:inScheme okns:owl-rdf-rdfs ;
    skos:mappingRelation rdf:language ;
    linkml:definition_uri okns:rdf_language ;
    linkml:domain okns:RdfCompoundLiteral ;
    linkml:inlined true ;
    linkml:owner okns:rdf_language ;
    linkml:range okns:Any ;
    linkml:slot_uri rdf:language .

okns:rdf_object a linkml:SlotDefinition ;
    dcterms:source rdf: ;
    dcterms:title "object" ;
    skos:definition "The object of the subject RDF statement." ;
    skos:editorialNote "No occurrences of this slot in the graph." ;
    skos:inScheme okns:owl-rdf-rdfs ;
    skos:mappingRelation rdf:object ;
    linkml:definition_uri okns:rdf_object ;
    linkml:domain okns:RdfStatement ;
    linkml:inlined true ;
    linkml:owner okns:rdf_object ;
    linkml:range okns:RdfsResource ;
    linkml:slot_uri rdf:object .

okns:rdf_predicate a linkml:SlotDefinition ;
    dcterms:source rdf: ;
    dcterms:title "predicate" ;
    skos:definition "The predicate of the subject RDF statement." ;
    skos:editorialNote "No occurrences of this slot in the graph." ;
    skos:inScheme okns:owl-rdf-rdfs ;
    skos:mappingRelation rdf:predicate ;
    linkml:definition_uri okns:rdf_predicate ;
    linkml:domain okns:RdfStatement ;
    linkml:inlined true ;
    linkml:owner okns:rdf_predicate ;
    linkml:range okns:RdfsResource ;
    linkml:slot_uri rdf:predicate .

okns:rdf_rest a linkml:SlotDefinition ;
    dcterms:source rdf: ;
    dcterms:title "rest" ;
    skos:definition "The rest of the subject RDF list after the first item." ;
    skos:editorialNote "No occurrences of this slot in the graph." ;
    skos:inScheme okns:owl-rdf-rdfs ;
    skos:mappingRelation rdf:rest ;
    linkml:definition_uri okns:rdf_rest ;
    linkml:domain okns:RdfList ;
    linkml:inlined true ;
    linkml:owner okns:rdf_rest ;
    linkml:range okns:RdfList ;
    linkml:slot_uri rdf:rest .

okns:rdf_subject a linkml:SlotDefinition ;
    dcterms:source rdf: ;
    dcterms:title "subject" ;
    skos:definition "The subject of the subject RDF statement." ;
    skos:editorialNote "No occurrences of this slot in the graph." ;
    skos:inScheme okns:owl-rdf-rdfs ;
    skos:mappingRelation rdf:subject ;
    linkml:definition_uri okns:rdf_subject ;
    linkml:domain okns:RdfStatement ;
    linkml:inlined true ;
    linkml:owner okns:rdf_subject ;
    linkml:range okns:RdfsResource ;
    linkml:slot_uri rdf:subject .

okns:rdf_type a linkml:SlotDefinition ;
    dcterms:source rdf: ;
    dcterms:title "type" ;
    skos:definition "The subject is an instance of a class." ;
    skos:editorialNote "No occurrences of this slot in the graph." ;
    skos:inScheme okns:owl-rdf-rdfs ;
    skos:mappingRelation rdf:type ;
    linkml:definition_uri okns:rdf_type ;
    linkml:domain okns:RdfsResource ;
    linkml:inlined true ;
    linkml:owner okns:rdf_type ;
    linkml:range okns:RdfsClass ;
    linkml:slot_uri rdf:type .

okns:rdfs_member a linkml:SlotDefinition ;
    dcterms:source rdfs: ;
    dcterms:title "member" ;
    skos:definition "A member of the subject resource." ;
    skos:editorialNote "No occurrences of this slot in the graph." ;
    skos:inScheme okns:owl-rdf-rdfs ;
    skos:mappingRelation rdfs:member ;
    linkml:definition_uri okns:rdfs_member ;
    linkml:domain okns:RdfsResource ;
    linkml:inlined true ;
    linkml:owner okns:rdfs_member ;
    linkml:range okns:RdfsResource ;
    linkml:slot_uri rdfs:member .

okns:rev_hasComment a linkml:SlotDefinition ;
    dcterms:source rev: ;
    dcterms:title "hasComment" ;
    skos:definition "Used to associate a review with a comment on the review" ;
    skos:editorialNote "No occurrences of this slot in the graph." ;
    skos:inScheme okns:rev ;
    skos:mappingRelation rev:hasComment ;
    linkml:definition_uri okns:rev_hasComment ;
    linkml:domain okns:RevReview ;
    linkml:inlined true ;
    linkml:owner okns:rev_hasComment ;
    linkml:range okns:RevComment ;
    linkml:slot_uri rev:hasComment .

okns:rev_hasFeedback a linkml:SlotDefinition ;
    dcterms:source rev: ;
    dcterms:title "hasFeedback" ;
    skos:definition "Associates a review with a feedback on the review" ;
    skos:editorialNote "No occurrences of this slot in the graph." ;
    skos:inScheme okns:rev ;
    skos:mappingRelation rev:hasFeedback ;
    linkml:definition_uri okns:rev_hasFeedback ;
    linkml:domain okns:RevReview ;
    linkml:inlined true ;
    linkml:owner okns:rev_hasFeedback ;
    linkml:range okns:RevFeedback ;
    linkml:slot_uri rev:hasFeedback .

okns:rev_hasReview a linkml:SlotDefinition ;
    dcterms:source rev: ;
    dcterms:title "has Review" ;
    skos:definition "Associates a work with a a review" ;
    skos:editorialNote "No occurrences of this slot in the graph." ;
    skos:inScheme okns:rev ;
    skos:mappingRelation rev:hasReview ;
    linkml:definition_uri okns:rev_hasReview ;
    linkml:domain okns:RdfsResource ;
    linkml:inlined true ;
    linkml:owner okns:rev_hasReview ;
    linkml:range okns:RevReview ;
    linkml:slot_uri rev:hasReview .

okns:rev_positiveVotes a linkml:SlotDefinition ;
    dcterms:source rev: ;
    dcterms:title "positiveVotes" ;
    skos:definition "Number of positive usefulness votes (integer)" ;
    skos:editorialNote "No occurrences of this slot in the graph." ;
    skos:inScheme okns:rev ;
    skos:mappingRelation rev:positiveVotes ;
    linkml:definition_uri okns:rev_positiveVotes ;
    linkml:domain okns:RevReview ;
    linkml:inlined true ;
    linkml:owner okns:rev_positiveVotes ;
    linkml:range okns:RdfsLiteral ;
    linkml:slot_uri rev:positiveVotes .

okns:rev_reviewer a linkml:SlotDefinition ;
    dcterms:source rev: ;
    dcterms:title "reviewer" ;
    skos:definition "The person that has written the review" ;
    skos:editorialNote "No occurrences of this slot in the graph." ;
    skos:inScheme okns:rev ;
    skos:mappingRelation rev:reviewer ;
    linkml:definition_uri okns:rev_reviewer ;
    linkml:domain okns:RevReview ;
    linkml:inlined true ;
    linkml:owner okns:rev_reviewer ;
    linkml:range okns:FoafPerson ;
    linkml:slot_uri rev:reviewer .

okns:rev_title a linkml:SlotDefinition ;
    dcterms:source rev: ;
    dcterms:title "title" ;
    rdfs:subPropertyOf okns:dc_title ;
    skos:definition "The title of the review" ;
    skos:editorialNote "No occurrences of this slot in the graph." ;
    skos:inScheme okns:rev ;
    skos:mappingRelation rev:title ;
    linkml:definition_uri okns:rev_title ;
    linkml:domain okns:RevReview ;
    linkml:inlined true ;
    linkml:owner okns:rev_title ;
    linkml:range okns:RdfsLiteral ;
    linkml:slot_uri rev:title .

okns:rev_totalVotes a linkml:SlotDefinition ;
    dcterms:source rev: ;
    dcterms:title "totalVotes" ;
    skos:definition "Number of usefulness votes (integer)" ;
    skos:editorialNote "No occurrences of this slot in the graph." ;
    skos:inScheme okns:rev ;
    skos:mappingRelation rev:totalVotes ;
    linkml:definition_uri okns:rev_totalVotes ;
    linkml:domain okns:RevReview ;
    linkml:inlined true ;
    linkml:owner okns:rev_totalVotes ;
    linkml:range okns:RdfsLiteral ;
    linkml:slot_uri rev:totalVotes .

okns:sim_association a linkml:SlotDefinition ;
    dcterms:source sim: ;
    dcterms:title "association" ;
    skos:definition "Binds a sim:Association to an arbitrary thing." ;
    skos:editorialNote "No occurrences of this slot in the graph." ;
    skos:inScheme okns:sim ;
    skos:mappingRelation sim:association ;
    linkml:definition_uri okns:sim_association ;
    linkml:domain okns:OwlThing ;
    linkml:inlined true ;
    linkml:owner okns:sim_association ;
    linkml:range okns:SimAssociation ;
    linkml:slot_uri sim:association .

okns:sim_description a linkml:SlotDefinition ;
    dcterms:source sim: ;
    dcterms:title "description" ;
    skos:definition "Specifies some description that discloses the process or set of processes used to derive association statements for the given <code>AssociationMethod</code>.  This property is depricated in favor of the more appropriately named <code>sim:workflow</code> property." ;
    skos:editorialNote "No occurrences of this slot in the graph." ;
    skos:exactMatch sim:workflow ;
    skos:inScheme okns:sim ;
    skos:mappingRelation sim:description ;
    linkml:definition_uri okns:sim_description ;
    linkml:domain okns:SimAssociationMethod ;
    linkml:inlined true ;
    linkml:owner okns:sim_description ;
    linkml:range okns:Any ;
    linkml:slot_uri sim:description .

okns:sim_distance a linkml:SlotDefinition ;
    dcterms:source sim: ;
    dcterms:title "distance" ;
    skos:definition "A weighting value for an Association where a value of 0 implies two elements are the same individual." ;
    skos:editorialNote "No occurrences of this slot in the graph." ;
    skos:inScheme okns:sim ;
    skos:mappingRelation sim:distance ;
    linkml:definition_uri okns:sim_distance ;
    linkml:domain okns:SimAssociation ;
    linkml:inlined true ;
    linkml:owner okns:sim_distance ;
    linkml:range okns:Any ;
    linkml:slot_uri sim:distance .

okns:sim_domain a linkml:SlotDefinition ;
    dcterms:source sim: ;
    dcterms:title "domain" ;
    skos:definition "Specifies appropriate object types for the <code>sim:subject</code> predicate for <code>sim:Association</code>s bound to the given <code>sim:AssociationMethod</code>.  The presence of this predicate implies the given <code>sim:AssociationMethod</code> begets <i>directed</i> associations." ;
    skos:editorialNote "No occurrences of this slot in the graph." ;
    skos:inScheme okns:sim ;
    skos:mappingRelation sim:domain ;
    linkml:definition_uri okns:sim_domain ;
    linkml:domain okns:SimAssociationMethod ;
    linkml:inlined true ;
    linkml:owner okns:sim_domain ;
    linkml:range okns:OwlThing ;
    linkml:slot_uri sim:domain .

okns:sim_edge a linkml:SlotDefinition ;
    dcterms:source sim: ;
    dcterms:title "edge" ;
    skos:definition "Specifies an edge in a <code>sim:Network</code>" ;
    skos:editorialNote "No occurrences of this slot in the graph." ;
    skos:inScheme okns:sim ;
    skos:mappingRelation sim:edge ;
    linkml:definition_uri okns:sim_edge ;
    linkml:domain okns:SimNetwork ;
    linkml:inlined true ;
    linkml:owner okns:sim_edge ;
    linkml:range okns:SimAssociation ;
    linkml:slot_uri sim:edge .

okns:sim_grounding a linkml:SlotDefinition ;
    dcterms:source sim: ;
    dcterms:title "grounding" ;
    skos:definition "Binds an <code>sim:Association</code> statement directly instantiated N3-Tr formulae or some other workflow graph which enabled the association derivation." ;
    skos:editorialNote "No occurrences of this slot in the graph." ;
    skos:inScheme okns:sim ;
    skos:mappingRelation sim:grounding ;
    linkml:definition_uri okns:sim_grounding ;
    linkml:domain okns:SimAssociation ;
    linkml:inlined true ;
    linkml:owner okns:sim_grounding ;
    linkml:range okns:Any ;
    linkml:slot_uri sim:grounding .

okns:sim_method a linkml:SlotDefinition ;
    dcterms:source sim: ;
    dcterms:title "method" ;
    skos:definition "Specifies the <code>sim:AssociationMethod</code> used to derive a particular Association statement.  This should be used when the process for deriving association statements can be described further." ;
    skos:editorialNote "No occurrences of this slot in the graph." ;
    skos:inScheme okns:sim ;
    skos:mappingRelation sim:method ;
    linkml:definition_uri okns:sim_method ;
    linkml:domain okns:SimAssociation ;
    linkml:inlined true ;
    linkml:owner okns:sim_method ;
    linkml:range okns:SimAssociationMethod ;
    linkml:slot_uri sim:method .

okns:sim_object a linkml:SlotDefinition ;
    dcterms:source sim: ;
    dcterms:title "object" ;
    rdfs:subPropertyOf okns:sim_element ;
    skos:definition "Specifies the object of a <code>sim:Association</code> implying a directed association where \"subject is associated to object\" but the reverse association does not necessarily exist, and if it does exist, it is not an equivalent association." ;
    skos:editorialNote "No occurrences of this slot in the graph." ;
    skos:inScheme okns:sim ;
    skos:mappingRelation sim:object ;
    linkml:definition_uri okns:sim_object ;
    linkml:domain okns:SimAssociation ;
    linkml:inlined true ;
    linkml:owner okns:sim_object ;
    linkml:range okns:Any ;
    linkml:slot_uri sim:object .

okns:sim_range a linkml:SlotDefinition ;
    dcterms:source sim: ;
    dcterms:title "domain" ;
    skos:definition "Specifies appropriate object types for the <code>sim:object</code> predicate for <code>sim:Association</code>s bound to the given <code>sim:AssociationMethod</code>.  The presence of this predicate implies the given <code>sim:AssociationMethod</code> begets <i>directed</i> associations." ;
    skos:editorialNote "No occurrences of this slot in the graph." ;
    skos:inScheme okns:sim ;
    skos:mappingRelation sim:range ;
    linkml:definition_uri okns:sim_range ;
    linkml:domain okns:SimAssociationMethod ;
    linkml:inlined true ;
    linkml:owner okns:sim_range ;
    linkml:range okns:OwlThing ;
    linkml:slot_uri sim:range .

okns:sim_scope a linkml:SlotDefinition ;
    dcterms:source sim: ;
    dcterms:title "domain" ;
    skos:definition "Specifies appropriate object types for the <code>sim:element</code> predicate for <code>sim:Association</code>s bound to the given <code>sim:AssociationMethod</code>.  The presence of this predicate implies the given <code>sim:AssociationMethod</code> begets <i>undirected</i> associations." ;
    skos:editorialNote "No occurrences of this slot in the graph." ;
    skos:inScheme okns:sim ;
    skos:mappingRelation sim:scope ;
    linkml:definition_uri okns:sim_scope ;
    linkml:domain okns:SimAssociationMethod ;
    linkml:inlined true ;
    linkml:owner okns:sim_scope ;
    linkml:range okns:OwlThing ;
    linkml:slot_uri sim:scope .

okns:sim_subject a linkml:SlotDefinition ;
    dcterms:source sim: ;
    dcterms:title "subject" ;
    rdfs:subPropertyOf okns:sim_element ;
    skos:definition "Specifies the subject of an <code>sim:Association</code> implying a directed association where \"subject is associated to object\" but the reverse association does not necessarily exist, and if it does exist, it is not an equivalent association." ;
    skos:editorialNote "No occurrences of this slot in the graph." ;
    skos:inScheme okns:sim ;
    skos:mappingRelation sim:subject ;
    linkml:definition_uri okns:sim_subject ;
    linkml:domain okns:SimAssociation ;
    linkml:inlined true ;
    linkml:owner okns:sim_subject ;
    linkml:range okns:Any ;
    linkml:slot_uri sim:subject .

okns:sim_weight a linkml:SlotDefinition ;
    dcterms:source sim: ;
    dcterms:title "weight" ;
    skos:definition "A weighting value bound to a <code>sim:Association</code> where a value of 0 implies two elements are not at all associated and a higher value implies a closer association." ;
    skos:editorialNote "No occurrences of this slot in the graph." ;
    skos:inScheme okns:sim ;
    skos:mappingRelation sim:weight ;
    linkml:definition_uri okns:sim_weight ;
    linkml:domain okns:SimAssociation ;
    linkml:inlined true ;
    linkml:owner okns:sim_weight ;
    linkml:range okns:Any ;
    linkml:slot_uri sim:weight .

okns:sim_workflow a linkml:SlotDefinition ;
    dcterms:source sim: ;
    dcterms:title "workflow" ;
    skos:definition "Specifies a workflow that discloses the process or set of processes used to derive association statements for the given <code>sim:AssociationMethod</code>" ;
    skos:editorialNote "No occurrences of this slot in the graph." ;
    skos:inScheme okns:sim ;
    skos:mappingRelation sim:workflow ;
    linkml:definition_uri okns:sim_workflow ;
    linkml:domain okns:SimAssociationMethod ;
    linkml:inlined true ;
    linkml:owner okns:sim_workflow ;
    linkml:range okns:Any ;
    linkml:slot_uri sim:workflow .

okns:skos_broadMatch a linkml:SlotDefinition ;
    dcterms:source <http://www.w3.org/2004/02/skos/core> ;
    dcterms:title "has broader match" ;
    rdfs:subPropertyOf okns:skos_broader ;
    owl:inverseOf okns:skos_narrowMatch ;
    skos:definition "skos:broadMatch is used to state a hierarchical mapping link between two conceptual resources in different concept schemes." ;
    skos:editorialNote "No occurrences of this slot in the graph." ;
    skos:inScheme okns:skos ;
    skos:mappingRelation skos:broadMatch ;
    linkml:definition_uri okns:skos_broadMatch ;
    linkml:domain okns:Any ;
    linkml:inlined true ;
    linkml:range okns:Any ;
    linkml:slot_uri skos:broadMatch .

okns:skos_closeMatch a linkml:SlotDefinition ;
    dcterms:source <http://www.w3.org/2004/02/skos/core> ;
    dcterms:title "has close match" ;
    rdfs:subPropertyOf okns:skos_mappingRelation ;
    skos:definition "skos:closeMatch is used to link two concepts that are sufficiently similar that they can be used interchangeably in some information retrieval applications. In order to avoid the possibility of \"compound errors\" when combining mappings across more than two concept schemes, skos:closeMatch is not declared to be a transitive property." ;
    skos:editorialNote "No occurrences of this slot in the graph." ;
    skos:inScheme okns:skos ;
    skos:mappingRelation skos:closeMatch ;
    linkml:definition_uri okns:skos_closeMatch ;
    linkml:inlined true ;
    linkml:range okns:Any ;
    linkml:slot_uri skos:closeMatch .

okns:skos_inScheme a linkml:SlotDefinition ;
    dcterms:source <http://www.w3.org/2004/02/skos/core> ;
    dcterms:title "is in scheme" ;
    skos:definition "Relates a resource (for example a concept) to a concept scheme in which it is included." ;
    skos:editorialNote "A concept may be a member of more than one concept scheme.",
        "No occurrences of this slot in the graph." ;
    skos:inScheme okns:skos ;
    skos:mappingRelation skos:inScheme ;
    linkml:definition_uri okns:skos_inScheme ;
    linkml:inlined true ;
    linkml:range okns:SkosConceptScheme ;
    linkml:slot_uri skos:inScheme .

okns:skos_mappingRelation a linkml:SlotDefinition ;
    dcterms:source <http://www.w3.org/2004/02/skos/core> ;
    dcterms:title "is in mapping relation with" ;
    rdfs:subPropertyOf okns:skos_semanticRelation ;
    skos:definition "Relates two concepts coming, by convention, from different schemes, and that have comparable meanings" ;
    skos:editorialNote "No occurrences of this slot in the graph." ;
    skos:inScheme okns:skos ;
    skos:mappingRelation skos:mappingRelation ;
    skos:note "description: These concept mapping relations mirror semantic relations, and the data model defined below is similar (with the exception of skos:exactMatch) to the data model defined for semantic relations. A distinct vocabulary is provided for concept mapping relations, to provide a convenient way to differentiate links within a concept scheme from links between concept schemes. However, this pattern of usage is not a formal requirement of the SKOS data model, and relies on informal definitions of best practice." ;
    linkml:definition_uri okns:skos_mappingRelation ;
    linkml:inlined true ;
    linkml:range okns:Any ;
    linkml:slot_uri skos:mappingRelation .

okns:skos_member a linkml:SlotDefinition ;
    dcterms:source <http://www.w3.org/2004/02/skos/core> ;
    dcterms:title "has member" ;
    skos:definition "Relates a collection to one of its members." ;
    skos:editorialNote "No occurrences of this slot in the graph." ;
    skos:inScheme okns:skos ;
    skos:mappingRelation skos:member ;
    linkml:definition_uri okns:skos_member ;
    linkml:domain okns:SkosCollection ;
    linkml:inlined true ;
    linkml:owner okns:skos_member ;
    linkml:range okns:Any ;
    linkml:slot_uri skos:member .

okns:skos_memberList a linkml:SlotDefinition ;
    dcterms:source <http://www.w3.org/2004/02/skos/core> ;
    dcterms:title "has member list" ;
    skos:definition "Relates an ordered collection to the RDF list containing its members." ;
    skos:editorialNote "No occurrences of this slot in the graph." ;
    skos:inScheme okns:skos ;
    skos:mappingRelation skos:memberList ;
    skos:note """description: For any resource, every item in the list given as the value of the
      skos:memberList property is also a value of the skos:member property.""" ;
    linkml:definition_uri okns:skos_memberList ;
    linkml:domain okns:SkosOrderedCollection ;
    linkml:inlined true ;
    linkml:owner okns:skos_memberList ;
    linkml:range okns:RdfList ;
    linkml:slot_uri skos:memberList .

okns:skos_narrowMatch a linkml:SlotDefinition ;
    dcterms:source <http://www.w3.org/2004/02/skos/core> ;
    dcterms:title "has narrower match" ;
    rdfs:subPropertyOf okns:skos_narrower ;
    owl:inverseOf okns:skos_broadMatch ;
    skos:definition "skos:narrowMatch is used to state a hierarchical mapping link between two conceptual resources in different concept schemes." ;
    skos:editorialNote "No occurrences of this slot in the graph." ;
    skos:inScheme okns:skos ;
    skos:mappingRelation skos:narrowMatch ;
    linkml:definition_uri okns:skos_narrowMatch ;
    linkml:domain okns:Any ;
    linkml:inlined true ;
    linkml:range okns:Any ;
    linkml:slot_uri skos:narrowMatch .

okns:skos_related a linkml:SlotDefinition ;
    dcterms:source <http://www.w3.org/2004/02/skos/core> ;
    dcterms:title "has related" ;
    rdfs:subPropertyOf okns:skos_semanticRelation ;
    skos:definition "Relates a concept to a concept with which there is an associative semantic relationship." ;
    skos:editorialNote "No occurrences of this slot in the graph." ;
    skos:inScheme okns:skos ;
    skos:mappingRelation skos:related ;
    skos:note "description: skos:related is disjoint with skos:broaderTransitive" ;
    linkml:definition_uri okns:skos_related ;
    linkml:inlined true ;
    linkml:range okns:Any ;
    linkml:slot_uri skos:related .

okns:time_day a linkml:SlotDefinition ;
    dcterms:title "day" ;
    skos:definition "Day position in a calendar-clock system.␊␊The range of this property is not specified, so can be replaced by any specific representation of a calendar day from any calendar." ;
    skos:editorialNote "No occurrences of this slot in the graph." ;
    skos:inScheme okns:time ;
    skos:mappingRelation time:day ;
    skos:note """description: Day position in a calendar-clock system.

The range of this property is not specified, so can be replaced by any specific representation of a calendar day from any calendar.""",
        "description: Posición de día en un sistema calendario-reloj.",
        """description: Posición de día en un sistema calendario-reloj.

El rango de esta propiedad no está especificado, por tanto, se puede reemplazar por una representación específica de un día de calendario de cualquier calendario.""",
        "title: día" ;
    linkml:definition_uri okns:time_day ;
    linkml:domain okns:TimeGeneralDateTimeDescription ;
    linkml:inlined true ;
    linkml:owner okns:time_day ;
    linkml:range okns:Any ;
    linkml:slot_uri time:day .

okns:time_dayOfWeek a linkml:SlotDefinition ;
    dcterms:title "day of week" ;
    skos:definition "The day of week, whose value is a member of the class time:DayOfWeek" ;
    skos:editorialNote "No occurrences of this slot in the graph." ;
    skos:inScheme okns:time ;
    skos:mappingRelation time:dayOfWeek ;
    skos:note "description: El día de la semana, cuyo valor es un miembro de la clase 'día de la semana'.",
        "description: The day of week, whose value is a member of the class time:DayOfWeek",
        "title: día de la semana" ;
    linkml:definition_uri okns:time_dayOfWeek ;
    linkml:domain okns:TimeGeneralDateTimeDescription ;
    linkml:inlined true ;
    linkml:owner okns:time_dayOfWeek ;
    linkml:range okns:TimeDayOfWeek ;
    linkml:slot_uri time:dayOfWeek .

okns:time_dayOfYear a linkml:SlotDefinition ;
    dcterms:title "day of year" ;
    skos:definition "The number of the day within the year" ;
    skos:editorialNote "No occurrences of this slot in the graph." ;
    skos:inScheme okns:time ;
    skos:mappingRelation time:dayOfYear ;
    skos:note "description: El número de día en el año.",
        "description: The number of the day within the year",
        "title: día del año" ;
    linkml:definition_uri okns:time_dayOfYear ;
    linkml:domain okns:TimeGeneralDateTimeDescription ;
    linkml:owner okns:time_dayOfYear ;
    linkml:range okns:unsignedinteger ;
    linkml:slot_uri time:dayOfYear .

okns:time_entry_after a linkml:SlotDefinition ;
    owl:inverseOf okns:time_entry_before ;
    skos:editorialNote "No occurrences of this slot in the graph." ;
    skos:inScheme okns:daml ;
    skos:mappingRelation time-entry:after ;
    linkml:definition_uri okns:time_entry_after ;
    linkml:domain okns:Time-entryTemporalThing ;
    linkml:inlined true ;
    linkml:range okns:Any ;
    linkml:slot_uri time-entry:after .

okns:time_entry_begins a linkml:SlotDefinition ;
    skos:editorialNote "No occurrences of this slot in the graph." ;
    skos:inScheme okns:daml ;
    skos:mappingRelation time-entry:begins ;
    linkml:definition_uri okns:time_entry_begins ;
    linkml:domain okns:Time-entryTemporalThing ;
    linkml:inlined true ;
    linkml:owner okns:time_entry_begins ;
    linkml:range okns:Time-entryInstantThing ;
    linkml:slot_uri time-entry:begins .

okns:time_entry_calendarClockDescriptionDataType a linkml:SlotDefinition ;
    skos:editorialNote "No occurrences of this slot in the graph." ;
    skos:inScheme okns:daml ;
    skos:mappingRelation time-entry:calendarClockDescriptionDataType ;
    linkml:definition_uri okns:time_entry_calendarClockDescriptionDataType ;
    linkml:domain okns:Time-entryCalendarClockInterval ;
    linkml:owner okns:time_entry_calendarClockDescriptionDataType ;
    linkml:range okns:datetime ;
    linkml:slot_uri time-entry:calendarClockDescriptionDataType .

okns:time_entry_calendarClockDescriptionOf a linkml:SlotDefinition ;
    skos:editorialNote "No occurrences of this slot in the graph." ;
    skos:inScheme okns:daml ;
    skos:mappingRelation time-entry:calendarClockDescriptionOf ;
    linkml:definition_uri okns:time_entry_calendarClockDescriptionOf ;
    linkml:domain okns:Time-entryCalendarClockInterval ;
    linkml:inlined true ;
    linkml:owner okns:time_entry_calendarClockDescriptionOf ;
    linkml:range okns:Time-entryCalendarClockDescription ;
    linkml:slot_uri time-entry:calendarClockDescriptionOf .

okns:time_entry_day a linkml:SlotDefinition ;
    skos:editorialNote "No occurrences of this slot in the graph." ;
    skos:inScheme okns:daml ;
    skos:mappingRelation time-entry:day ;
    linkml:definition_uri okns:time_entry_day ;
    linkml:domain okns:Time-entryCalendarClockDescription ;
    linkml:inlined true ;
    linkml:owner okns:time_entry_day ;
    linkml:range okns:XsdGDay ;
    linkml:slot_uri time-entry:day .

okns:time_entry_dayOfWeekField a linkml:SlotDefinition ;
    skos:editorialNote "No occurrences of this slot in the graph." ;
    skos:inScheme okns:daml ;
    skos:mappingRelation time-entry:dayOfWeekField ;
    linkml:definition_uri okns:time_entry_dayOfWeekField ;
    linkml:domain okns:Time-entryCalendarClockDescription ;
    linkml:owner okns:time_entry_dayOfWeekField ;
    linkml:range okns:unsignedinteger ;
    linkml:slot_uri time-entry:dayOfWeekField .

okns:time_entry_dayOfYearField a linkml:SlotDefinition ;
    skos:editorialNote "No occurrences of this slot in the graph." ;
    skos:inScheme okns:daml ;
    skos:mappingRelation time-entry:dayOfYearField ;
    linkml:definition_uri okns:time_entry_dayOfYearField ;
    linkml:domain okns:Time-entryCalendarClockDescription ;
    linkml:owner okns:time_entry_dayOfYearField ;
    linkml:range okns:unsignedinteger ;
    linkml:slot_uri time-entry:dayOfYearField .

okns:time_entry_days a linkml:SlotDefinition ;
    skos:editorialNote "No occurrences of this slot in the graph." ;
    skos:inScheme okns:daml ;
    skos:mappingRelation time-entry:days ;
    linkml:definition_uri okns:time_entry_days ;
    linkml:domain okns:Time-entryDurationDescription ;
    linkml:owner okns:time_entry_days ;
    linkml:range okns:decimal ;
    linkml:slot_uri time-entry:days .

okns:time_entry_durationDescriptionDataType a linkml:SlotDefinition ;
    skos:editorialNote "No occurrences of this slot in the graph." ;
    skos:inScheme okns:daml ;
    skos:mappingRelation time-entry:durationDescriptionDataType ;
    linkml:definition_uri okns:time_entry_durationDescriptionDataType ;
    linkml:domain okns:Time-entryTemporalThing ;
    linkml:inlined true ;
    linkml:owner okns:time_entry_durationDescriptionDataType ;
    linkml:range okns:XsdDuration ;
    linkml:slot_uri time-entry:durationDescriptionDataType .

okns:time_entry_durationDescriptionOf a linkml:SlotDefinition ;
    skos:editorialNote "No occurrences of this slot in the graph." ;
    skos:inScheme okns:daml ;
    skos:mappingRelation time-entry:durationDescriptionOf ;
    linkml:definition_uri okns:time_entry_durationDescriptionOf ;
    linkml:domain okns:Time-entryTemporalThing ;
    linkml:inlined true ;
    linkml:owner okns:time_entry_durationDescriptionOf ;
    linkml:range okns:Time-entryDurationDescription ;
    linkml:slot_uri time-entry:durationDescriptionOf .

okns:time_entry_ends a linkml:SlotDefinition ;
    skos:editorialNote "No occurrences of this slot in the graph." ;
    skos:inScheme okns:daml ;
    skos:mappingRelation time-entry:ends ;
    linkml:definition_uri okns:time_entry_ends ;
    linkml:domain okns:Time-entryTemporalThing ;
    linkml:inlined true ;
    linkml:owner okns:time_entry_ends ;
    linkml:range okns:Time-entryInstantThing ;
    linkml:slot_uri time-entry:ends .

okns:time_entry_firstInstantThing a linkml:SlotDefinition ;
    skos:editorialNote "No occurrences of this slot in the graph." ;
    skos:inScheme okns:daml ;
    skos:mappingRelation time-entry:firstInstantThing ;
    linkml:definition_uri okns:time_entry_firstInstantThing ;
    linkml:domain okns:Time-entryInstantThingPair ;
    linkml:inlined true ;
    linkml:owner okns:time_entry_firstInstantThing ;
    linkml:range okns:Time-entryInstantThing ;
    linkml:slot_uri time-entry:firstInstantThing .

okns:time_entry_hour a linkml:SlotDefinition ;
    skos:editorialNote "No occurrences of this slot in the graph." ;
    skos:inScheme okns:daml ;
    skos:mappingRelation time-entry:hour ;
    linkml:definition_uri okns:time_entry_hour ;
    linkml:domain okns:Time-entryCalendarClockDescription ;
    linkml:owner okns:time_entry_hour ;
    linkml:range okns:unsignedinteger ;
    linkml:slot_uri time-entry:hour .

okns:time_entry_hours a linkml:SlotDefinition ;
    skos:editorialNote "No occurrences of this slot in the graph." ;
    skos:inScheme okns:daml ;
    skos:mappingRelation time-entry:hours ;
    linkml:definition_uri okns:time_entry_hours ;
    linkml:domain okns:Time-entryDurationDescription ;
    linkml:owner okns:time_entry_hours ;
    linkml:range okns:decimal ;
    linkml:slot_uri time-entry:hours .

okns:time_entry_inCalendarClock a linkml:SlotDefinition ;
    skos:editorialNote "No occurrences of this slot in the graph." ;
    skos:inScheme okns:daml ;
    skos:mappingRelation time-entry:inCalendarClock ;
    linkml:definition_uri okns:time_entry_inCalendarClock ;
    linkml:domain okns:Time-entryInstantThing ;
    linkml:inlined true ;
    linkml:owner okns:time_entry_inCalendarClock ;
    linkml:range okns:Time-entryCalendarClockDescription ;
    linkml:slot_uri time-entry:inCalendarClock .

okns:time_entry_inCalendarClockDataType a linkml:SlotDefinition ;
    skos:editorialNote "No occurrences of this slot in the graph." ;
    skos:inScheme okns:daml ;
    skos:mappingRelation time-entry:inCalendarClockDataType ;
    linkml:definition_uri okns:time_entry_inCalendarClockDataType ;
    linkml:domain okns:Time-entryInstantThing ;
    linkml:owner okns:time_entry_inCalendarClockDataType ;
    linkml:range okns:datetime ;
    linkml:slot_uri time-entry:inCalendarClockDataType .

okns:time_entry_inside a linkml:SlotDefinition ;
    skos:editorialNote "No occurrences of this slot in the graph." ;
    skos:inScheme okns:daml ;
    skos:mappingRelation time-entry:inside ;
    linkml:definition_uri okns:time_entry_inside ;
    linkml:domain okns:Time-entryIntervalThing ;
    linkml:inlined true ;
    linkml:owner okns:time_entry_inside ;
    linkml:range okns:Time-entryInstantThing ;
    linkml:slot_uri time-entry:inside .

okns:time_entry_instantPairDurationDescriptionDataType a linkml:SlotDefinition ;
    skos:editorialNote "No occurrences of this slot in the graph." ;
    skos:inScheme okns:daml ;
    skos:mappingRelation time-entry:instantPairDurationDescriptionDataType ;
    linkml:definition_uri okns:time_entry_instantPairDurationDescriptionDataType ;
    linkml:domain okns:Time-entryInstantThingPair ;
    linkml:inlined true ;
    linkml:owner okns:time_entry_instantPairDurationDescriptionDataType ;
    linkml:range okns:XsdDuration ;
    linkml:slot_uri time-entry:instantPairDurationDescriptionDataType .

okns:time_entry_instantPairDurationDescriptionOf a linkml:SlotDefinition ;
    skos:editorialNote "No occurrences of this slot in the graph." ;
    skos:inScheme okns:daml ;
    skos:mappingRelation time-entry:instantPairDurationDescriptionOf ;
    linkml:definition_uri okns:time_entry_instantPairDurationDescriptionOf ;
    linkml:domain okns:Time-entryInstantThingPair ;
    linkml:inlined true ;
    linkml:owner okns:time_entry_instantPairDurationDescriptionOf ;
    linkml:range okns:Time-entryDurationDescription ;
    linkml:slot_uri time-entry:instantPairDurationDescriptionOf .

okns:time_entry_intAfter a linkml:SlotDefinition ;
    rdfs:subPropertyOf okns:time_entry_nonoverlap ;
    owl:inverseOf okns:time_entry_intBefore ;
    skos:editorialNote "No occurrences of this slot in the graph." ;
    skos:inScheme okns:daml ;
    skos:mappingRelation time-entry:intAfter ;
    linkml:definition_uri okns:time_entry_intAfter ;
    linkml:domain okns:Time-entryProperIntervalThing ;
    linkml:inlined true ;
    linkml:range okns:Any ;
    linkml:slot_uri time-entry:intAfter .

okns:time_entry_intContains a linkml:SlotDefinition ;
    owl:inverseOf okns:time_entry_intDuring ;
    skos:editorialNote "No occurrences of this slot in the graph." ;
    skos:inScheme okns:daml ;
    skos:mappingRelation time-entry:intContains ;
    linkml:definition_uri okns:time_entry_intContains ;
    linkml:domain okns:Time-entryProperIntervalThing ;
    linkml:inlined true ;
    linkml:range okns:Any ;
    linkml:slot_uri time-entry:intContains .

okns:time_entry_intEquals a linkml:SlotDefinition ;
    skos:editorialNote "No occurrences of this slot in the graph." ;
    skos:inScheme okns:daml ;
    skos:mappingRelation time-entry:intEquals ;
    linkml:definition_uri okns:time_entry_intEquals ;
    linkml:domain okns:Time-entryProperIntervalThing ;
    linkml:inlined true ;
    linkml:owner okns:time_entry_intEquals ;
    linkml:range okns:Time-entryProperIntervalThing ;
    linkml:slot_uri time-entry:intEquals .

okns:time_entry_intFinishedBy a linkml:SlotDefinition ;
    owl:inverseOf okns:time_entry_intFinishes ;
    skos:editorialNote "No occurrences of this slot in the graph." ;
    skos:inScheme okns:daml ;
    skos:mappingRelation time-entry:intFinishedBy ;
    linkml:definition_uri okns:time_entry_intFinishedBy ;
    linkml:domain okns:Time-entryProperIntervalThing ;
    linkml:inlined true ;
    linkml:range okns:Any ;
    linkml:slot_uri time-entry:intFinishedBy .

okns:time_entry_intMetBy a linkml:SlotDefinition ;
    rdfs:subPropertyOf okns:time_entry_nonoverlap ;
    owl:inverseOf okns:time_entry_intMeets ;
    skos:editorialNote "No occurrences of this slot in the graph." ;
    skos:inScheme okns:daml ;
    skos:mappingRelation time-entry:intMetBy ;
    linkml:definition_uri okns:time_entry_intMetBy ;
    linkml:domain okns:Time-entryProperIntervalThing ;
    linkml:inlined true ;
    linkml:range okns:Any ;
    linkml:slot_uri time-entry:intMetBy .

okns:time_entry_intOverlappedBy a linkml:SlotDefinition ;
    owl:inverseOf okns:time_entry_intOverlaps ;
    skos:editorialNote "No occurrences of this slot in the graph." ;
    skos:inScheme okns:daml ;
    skos:mappingRelation time-entry:intOverlappedBy ;
    linkml:definition_uri okns:time_entry_intOverlappedBy ;
    linkml:domain okns:Time-entryProperIntervalThing ;
    linkml:inlined true ;
    linkml:range okns:Any ;
    linkml:slot_uri time-entry:intOverlappedBy .

okns:time_entry_intStartedBy a linkml:SlotDefinition ;
    owl:inverseOf okns:time_entry_intStarts ;
    skos:editorialNote "No occurrences of this slot in the graph." ;
    skos:inScheme okns:daml ;
    skos:mappingRelation time-entry:intStartedBy ;
    linkml:definition_uri okns:time_entry_intStartedBy ;
    linkml:domain okns:Time-entryProperIntervalThing ;
    linkml:inlined true ;
    linkml:range okns:Any ;
    linkml:slot_uri time-entry:intStartedBy .

okns:time_entry_minute a linkml:SlotDefinition ;
    skos:editorialNote "No occurrences of this slot in the graph." ;
    skos:inScheme okns:daml ;
    skos:mappingRelation time-entry:minute ;
    linkml:definition_uri okns:time_entry_minute ;
    linkml:domain okns:Time-entryCalendarClockDescription ;
    linkml:owner okns:time_entry_minute ;
    linkml:range okns:unsignedinteger ;
    linkml:slot_uri time-entry:minute .

okns:time_entry_minutes a linkml:SlotDefinition ;
    skos:editorialNote "No occurrences of this slot in the graph." ;
    skos:inScheme okns:daml ;
    skos:mappingRelation time-entry:minutes ;
    linkml:definition_uri okns:time_entry_minutes ;
    linkml:domain okns:Time-entryDurationDescription ;
    linkml:owner okns:time_entry_minutes ;
    linkml:range okns:decimal ;
    linkml:slot_uri time-entry:minutes .

okns:time_entry_month a linkml:SlotDefinition ;
    skos:editorialNote "No occurrences of this slot in the graph." ;
    skos:inScheme okns:daml ;
    skos:mappingRelation time-entry:month ;
    linkml:definition_uri okns:time_entry_month ;
    linkml:domain okns:Time-entryCalendarClockDescription ;
    linkml:inlined true ;
    linkml:owner okns:time_entry_month ;
    linkml:range okns:XsdGMonth ;
    linkml:slot_uri time-entry:month .

okns:time_entry_months a linkml:SlotDefinition ;
    skos:editorialNote "No occurrences of this slot in the graph." ;
    skos:inScheme okns:daml ;
    skos:mappingRelation time-entry:months ;
    linkml:definition_uri okns:time_entry_months ;
    linkml:domain okns:Time-entryDurationDescription ;
    linkml:owner okns:time_entry_months ;
    linkml:range okns:decimal ;
    linkml:slot_uri time-entry:months .

okns:time_entry_second a linkml:SlotDefinition ;
    skos:editorialNote "No occurrences of this slot in the graph." ;
    skos:inScheme okns:daml ;
    skos:mappingRelation time-entry:second ;
    linkml:definition_uri okns:time_entry_second ;
    linkml:domain okns:Time-entryCalendarClockDescription ;
    linkml:owner okns:time_entry_second ;
    linkml:range okns:decimal ;
    linkml:slot_uri time-entry:second .

okns:time_entry_secondInstantThing a linkml:SlotDefinition ;
    skos:editorialNote "No occurrences of this slot in the graph." ;
    skos:inScheme okns:daml ;
    skos:mappingRelation time-entry:secondInstantThing ;
    linkml:definition_uri okns:time_entry_secondInstantThing ;
    linkml:domain okns:Time-entryInstantThingPair ;
    linkml:inlined true ;
    linkml:owner okns:time_entry_secondInstantThing ;
    linkml:range okns:Time-entryInstantThing ;
    linkml:slot_uri time-entry:secondInstantThing .

okns:time_entry_seconds a linkml:SlotDefinition ;
    skos:editorialNote "No occurrences of this slot in the graph." ;
    skos:inScheme okns:daml ;
    skos:mappingRelation time-entry:seconds ;
    linkml:definition_uri okns:time_entry_seconds ;
    linkml:domain okns:Time-entryDurationDescription ;
    linkml:owner okns:time_entry_seconds ;
    linkml:range okns:decimal ;
    linkml:slot_uri time-entry:seconds .

okns:time_entry_timeZone a linkml:SlotDefinition ;
    skos:editorialNote "No occurrences of this slot in the graph." ;
    skos:inScheme okns:daml ;
    skos:mappingRelation time-entry:timeZone ;
    linkml:definition_uri okns:time_entry_timeZone ;
    linkml:domain okns:Time-entryCalendarClockDescription ;
    linkml:inlined true ;
    linkml:owner okns:time_entry_timeZone ;
    linkml:range okns:TzontTimeZone ;
    linkml:slot_uri time-entry:timeZone .

okns:time_entry_unitType a linkml:SlotDefinition ;
    skos:editorialNote "No occurrences of this slot in the graph." ;
    skos:inScheme okns:daml ;
    skos:mappingRelation time-entry:unitType ;
    linkml:definition_uri okns:time_entry_unitType ;
    linkml:domain okns:Time-entryCalendarClockDescription ;
    linkml:inlined true ;
    linkml:owner okns:time_entry_unitType ;
    linkml:range okns:Time-entryTemporalUnit ;
    linkml:slot_uri time-entry:unitType .

okns:time_entry_week a linkml:SlotDefinition ;
    skos:editorialNote "No occurrences of this slot in the graph." ;
    skos:inScheme okns:daml ;
    skos:mappingRelation time-entry:week ;
    linkml:definition_uri okns:time_entry_week ;
    linkml:domain okns:Time-entryCalendarClockDescription ;
    linkml:owner okns:time_entry_week ;
    linkml:range okns:unsignedinteger ;
    linkml:slot_uri time-entry:week .

okns:time_entry_weeks a linkml:SlotDefinition ;
    skos:editorialNote "No occurrences of this slot in the graph." ;
    skos:inScheme okns:daml ;
    skos:mappingRelation time-entry:weeks ;
    linkml:definition_uri okns:time_entry_weeks ;
    linkml:domain okns:Time-entryDurationDescription ;
    linkml:owner okns:time_entry_weeks ;
    linkml:range okns:decimal ;
    linkml:slot_uri time-entry:weeks .

okns:time_entry_year a linkml:SlotDefinition ;
    skos:editorialNote "No occurrences of this slot in the graph." ;
    skos:inScheme okns:daml ;
    skos:mappingRelation time-entry:year ;
    linkml:definition_uri okns:time_entry_year ;
    linkml:domain okns:Time-entryCalendarClockDescription ;
    linkml:inlined true ;
    linkml:owner okns:time_entry_year ;
    linkml:range okns:XsdGYear ;
    linkml:slot_uri time-entry:year .

okns:time_entry_years a linkml:SlotDefinition ;
    skos:editorialNote "No occurrences of this slot in the graph." ;
    skos:inScheme okns:daml ;
    skos:mappingRelation time-entry:years ;
    linkml:definition_uri okns:time_entry_years ;
    linkml:domain okns:Time-entryDurationDescription ;
    linkml:owner okns:time_entry_years ;
    linkml:range okns:decimal ;
    linkml:slot_uri time-entry:years .

okns:time_hasBeginning a linkml:SlotDefinition ;
    dcterms:title "has beginning" ;
    rdfs:subPropertyOf okns:time_hasTime ;
    skos:definition "Beginning of a temporal entity" ;
    skos:editorialNote "No occurrences of this slot in the graph." ;
    skos:inScheme okns:time ;
    skos:mappingRelation time:hasBeginning ;
    skos:note "description: Beginning of a temporal entity.",
        "description: Comienzo de una entidad temporal.",
        "title: tiene principio" ;
    linkml:definition_uri okns:time_hasBeginning ;
    linkml:domain okns:TimeTemporalEntity ;
    linkml:inlined true ;
    linkml:owner okns:time_hasBeginning ;
    linkml:range okns:TimeInstant ;
    linkml:slot_uri time:hasBeginning .

okns:time_hasDateTimeDescription a linkml:SlotDefinition ;
    dcterms:title "has Date-Time description" ;
    skos:definition "Value of DateTimeInterval expressed as a structured value. The beginning and end of the interval coincide with the limits of the shortest element in the description." ;
    skos:editorialNote "No occurrences of this slot in the graph." ;
    skos:inScheme okns:time ;
    skos:mappingRelation time:hasDateTimeDescription ;
    skos:note "description: Valor de intervalo de fecha-hora expresado como un valor estructurado. El principio y el final del intervalo coincide con los límites del elemento más corto en la descripción.",
        "description: Value of DateTimeInterval expressed as a structured value. The beginning and end of the interval coincide with the limits of the shortest element in the description.",
        "title: tiene descripción fecha-hora" ;
    linkml:definition_uri okns:time_hasDateTimeDescription ;
    linkml:domain okns:TimeDateTimeInterval ;
    linkml:inlined true ;
    linkml:owner okns:time_hasDateTimeDescription ;
    linkml:range okns:TimeGeneralDateTimeDescription ;
    linkml:slot_uri time:hasDateTimeDescription .

okns:time_hasEnd a linkml:SlotDefinition ;
    dcterms:title "has end" ;
    rdfs:subPropertyOf okns:time_hasTime ;
    skos:definition "End of a temporal entity." ;
    skos:editorialNote "No occurrences of this slot in the graph." ;
    skos:inScheme okns:time ;
    skos:mappingRelation time:hasEnd ;
    skos:note "description: End of a temporal entity.",
        "description: Final de una entidad temporal.",
        "title: tiene fin" ;
    linkml:definition_uri okns:time_hasEnd ;
    linkml:domain okns:TimeTemporalEntity ;
    linkml:inlined true ;
    linkml:owner okns:time_hasEnd ;
    linkml:range okns:TimeInstant ;
    linkml:slot_uri time:hasEnd .

okns:time_hasXSDDuration a linkml:SlotDefinition ;
    dcterms:title "has XSD duration" ;
    skos:definition "Extent of a temporal entity, expressed using xsd:duration" ;
    skos:editorialNote "Característica arriesgada - añadida en la revisión de 2017, y todavía no ampliamente utilizada.",
        "Feature at risk - added in 2017 revision, and not yet widely used. ",
        "No occurrences of this slot in the graph." ;
    skos:inScheme okns:time ;
    skos:mappingRelation time:hasXSDDuration ;
    skos:note "description: Extensión de una entidad temporal, expresada utilizando xsd:duration.",
        "description: Extent of a temporal entity, expressed using xsd:duration",
        "title: tiene duración XSD" ;
    linkml:definition_uri okns:time_hasXSDDuration ;
    linkml:domain okns:TimeTemporalEntity ;
    linkml:inlined true ;
    linkml:owner okns:time_hasXSDDuration ;
    linkml:range okns:XsdDuration ;
    linkml:slot_uri time:hasXSDDuration .

okns:time_hour a linkml:SlotDefinition ;
    dcterms:title "hour" ;
    skos:definition "Hour position in a calendar-clock system." ;
    skos:editorialNote "No occurrences of this slot in the graph." ;
    skos:inScheme okns:time ;
    skos:mappingRelation time:hour ;
    skos:note "description: Hour position in a calendar-clock system.",
        "description: Posición de hora en un sistema calendario-reloj.",
        "title: hora" ;
    linkml:definition_uri okns:time_hour ;
    linkml:domain okns:TimeGeneralDateTimeDescription ;
    linkml:owner okns:time_hour ;
    linkml:range okns:unsignedinteger ;
    linkml:slot_uri time:hour .

okns:time_inDateTime a linkml:SlotDefinition ;
    dcterms:title "in date-time description" ;
    rdfs:subPropertyOf okns:time_inTemporalPosition ;
    skos:definition "Position of an instant, expressed using a structured description" ;
    skos:editorialNote "No occurrences of this slot in the graph." ;
    skos:inScheme okns:time ;
    skos:mappingRelation time:inDateTime ;
    skos:note "description: Posición de un instante, expresada utilizando una descripción estructurada.",
        "description: Position of an instant, expressed using a structured description",
        "title: en descripción de fecha-hora" ;
    linkml:definition_uri okns:time_inDateTime ;
    linkml:domain okns:TimeInstant ;
    linkml:inlined true ;
    linkml:owner okns:time_inDateTime ;
    linkml:range okns:TimeGeneralDateTimeDescription ;
    linkml:slot_uri time:inDateTime .

okns:time_inTimePosition a linkml:SlotDefinition ;
    dcterms:title "Time position" ;
    rdfs:subPropertyOf okns:time_inTemporalPosition ;
    skos:definition "Position of an instant, expressed as a temporal coordinate or nominal value" ;
    skos:editorialNote "No occurrences of this slot in the graph." ;
    skos:inScheme okns:time ;
    skos:mappingRelation time:inTimePosition ;
    skos:note "description: Posición de un instante, expresada como una coordenada temporal o un valor nominal.",
        "description: Position of a time instant expressed as a TimePosition",
        "title: posición de tiempo" ;
    linkml:definition_uri okns:time_inTimePosition ;
    linkml:domain okns:TimeInstant ;
    linkml:inlined true ;
    linkml:owner okns:time_inTimePosition ;
    linkml:range okns:TimeTimePosition ;
    linkml:slot_uri time:inTimePosition .

okns:time_inXSDDate a linkml:SlotDefinition ;
    dcterms:title "in XSD date" ;
    skos:definition "Position of an instant, expressed using xsd:date" ;
    skos:editorialNote "No occurrences of this slot in the graph." ;
    skos:inScheme okns:time ;
    skos:mappingRelation time:inXSDDate ;
    skos:note "description: Posición de un instante, expresado utilizando xsd:date.",
        "description: Position of an instant, expressed using xsd:date",
        "title: en fecha XSD" ;
    linkml:definition_uri okns:time_inXSDDate ;
    linkml:domain okns:TimeInstant ;
    linkml:owner okns:time_inXSDDate ;
    linkml:range okns:date ;
    linkml:slot_uri time:inXSDDate .

okns:time_inXSDDateTime a linkml:SlotDefinition ;
    dcterms:title "in XSD Date-Time" ;
    skos:definition "Position of an instant, expressed using xsd:dateTime" ;
    skos:editorialNote "La propiedad 'en fecha-hora XSD' ha sido reemplazada por 'en fecha-sello de tiempo XSD' que hace obligatorio el campo 'huso horario'.",
        "No occurrences of this slot in the graph.",
        "The property :inXSDDateTime is replaced by :inXSDDateTimeStamp which makes the time-zone field mandatory." ;
    skos:inScheme okns:time ;
    skos:mappingRelation time:inXSDDateTime ;
    skos:note "description: Posición de un instante, expresado utilizando xsd:dateTime.",
        "description: Position of an instant, expressed using xsd:dateTime",
        "title: en fecha-tiempo XSD" ;
    linkml:deprecated "true" ;
    linkml:definition_uri okns:time_inXSDDateTime ;
    linkml:domain okns:TimeInstant ;
    linkml:owner okns:time_inXSDDateTime ;
    linkml:range okns:datetime ;
    linkml:slot_uri time:inXSDDateTime .

okns:time_inXSDDateTimeStamp a linkml:SlotDefinition ;
    dcterms:title "in XSD Date-Time-Stamp" ;
    skos:definition "Position of an instant, expressed using xsd:dateTimeStamp" ;
    skos:editorialNote "No occurrences of this slot in the graph." ;
    skos:inScheme okns:time ;
    skos:mappingRelation time:inXSDDateTimeStamp ;
    skos:note "description: Posición de un instante, expresado utilizando xsd:dateTimeStamp.",
        "description: Position of an instant, expressed using xsd:dateTimeStamp",
        "title: en fecha-sello de tiempo XSD" ;
    linkml:definition_uri okns:time_inXSDDateTimeStamp ;
    linkml:domain okns:TimeInstant ;
    linkml:inlined true ;
    linkml:owner okns:time_inXSDDateTimeStamp ;
    linkml:range okns:XsdDateTimeStamp ;
    linkml:slot_uri time:inXSDDateTimeStamp .

okns:time_inXSDgYear a linkml:SlotDefinition ;
    dcterms:title "in XSD g-Year" ;
    skos:definition "Position of an instant, expressed using xsd:gYear" ;
    skos:editorialNote "No occurrences of this slot in the graph." ;
    skos:inScheme okns:time ;
    skos:mappingRelation time:inXSDgYear ;
    skos:note "description: Posición de un instante, expresado utilizando xsd:gYear.",
        "description: Position of an instant, expressed using xsd:gYear",
        "title: en año gregoriano XSD" ;
    linkml:definition_uri okns:time_inXSDgYear ;
    linkml:domain okns:TimeInstant ;
    linkml:inlined true ;
    linkml:owner okns:time_inXSDgYear ;
    linkml:range okns:XsdGYear ;
    linkml:slot_uri time:inXSDgYear .

okns:time_inXSDgYearMonth a linkml:SlotDefinition ;
    dcterms:title "in XSD g-YearMonth" ;
    skos:definition "Position of an instant, expressed using xsd:gYearMonth" ;
    skos:editorialNote "No occurrences of this slot in the graph." ;
    skos:inScheme okns:time ;
    skos:mappingRelation time:inXSDgYearMonth ;
    skos:note "description: Posición de un instante, expresado utilizando xsd:gYearMonth.",
        "description: Position of an instant, expressed using xsd:gYearMonth",
        "title: en año-mes gregoriano XSD" ;
    linkml:definition_uri okns:time_inXSDgYearMonth ;
    linkml:domain okns:TimeInstant ;
    linkml:inlined true ;
    linkml:owner okns:time_inXSDgYearMonth ;
    linkml:range okns:XsdGYearMonth ;
    linkml:slot_uri time:inXSDgYearMonth .

okns:time_inside a linkml:SlotDefinition ;
    dcterms:title "has time instant inside" ;
    skos:definition "An instant that falls inside the interval. It is not intended to include beginnings and ends of intervals." ;
    skos:editorialNote "No occurrences of this slot in the graph." ;
    skos:inScheme okns:time ;
    skos:mappingRelation time:inside ;
    skos:note "description: An instant that falls inside the interval. It is not intended to include beginnings and ends of intervals.",
        "description: Un instante que cae dentro del intervalo. Se asume que no es ni el principio ni el final de ningún intervalo.",
        "title: tiene instante de tiempo dentro" ;
    linkml:definition_uri okns:time_inside ;
    linkml:domain okns:TimeInterval ;
    linkml:inlined true ;
    linkml:owner okns:time_inside ;
    linkml:range okns:TimeInstant ;
    linkml:slot_uri time:inside .

okns:time_intervalEquals a linkml:SlotDefinition ;
    dcterms:title "interval equals" ;
    skos:definition "If a proper interval T1 is intervalEquals another proper interval T2, then the beginning of T1 is coincident with the beginning of T2, and the end of T1 is coincident with the end of T2." ;
    skos:editorialNote "No occurrences of this slot in the graph." ;
    skos:inScheme okns:time ;
    skos:mappingRelation time:intervalEquals ;
    skos:note "description: If a proper interval T1 is intervalEquals another proper interval T2, then the beginning of T1 is coincident with the beginning of T2, and the end of T1 is coincident with the end of T2.",
        "description: Si un intervalo propio T1 es igual a otro intervalo propio T2, entonces el principio de T1 coincide con el principio de T2, y el final de T1 coincide con el final de T2.",
        "title: intervalo igual" ;
    linkml:definition_uri okns:time_intervalEquals ;
    linkml:domain okns:TimeProperInterval ;
    linkml:inlined true ;
    linkml:owner okns:time_intervalEquals ;
    linkml:range okns:TimeProperInterval ;
    linkml:slot_uri time:intervalEquals .

okns:time_minute a linkml:SlotDefinition ;
    dcterms:title "minute" ;
    skos:definition "Minute position in a calendar-clock system." ;
    skos:editorialNote "No occurrences of this slot in the graph." ;
    skos:inScheme okns:time ;
    skos:mappingRelation time:minute ;
    skos:note "description: Minute position in a calendar-clock system.",
        "description: Posición de minuto en un sistema calendario-reloj.",
        "title: minuto" ;
    linkml:definition_uri okns:time_minute ;
    linkml:domain okns:TimeGeneralDateTimeDescription ;
    linkml:owner okns:time_minute ;
    linkml:range okns:unsignedinteger ;
    linkml:slot_uri time:minute .

okns:time_month a linkml:SlotDefinition ;
    dcterms:title "month" ;
    skos:definition "Month position in a calendar-clock system.␊␊The range of this property is not specified, so can be replaced by any specific representation of a calendar month from any calendar." ;
    skos:editorialNote "No occurrences of this slot in the graph." ;
    skos:inScheme okns:time ;
    skos:mappingRelation time:month ;
    skos:note """description: Month position in a calendar-clock system.

The range of this property is not specified, so can be replaced by any specific representation of a calendar month from any calendar.""",
        """description: Posición de mes en un sistema calendario-reloj.
            El rango de esta propiedad no está especificado, por tanto, se puede reemplazar por cualquier representación específica de un mes de calendario de un calendario cualquiera.""",
        """description: Posición de mes en un sistema calendario-reloj.
    El rango de esta propiedad no está especificado, por tanto, se puede reemplazar por cualquier representación específica de un mes de calendario de un calendario cualquiera.""",
        "title: mes" ;
    linkml:definition_uri okns:time_month ;
    linkml:domain okns:TimeGeneralDateTimeDescription ;
    linkml:inlined true ;
    linkml:owner okns:time_month ;
    linkml:range okns:Any ;
    linkml:slot_uri time:month .

okns:time_monthOfYear a linkml:SlotDefinition ;
    dcterms:title "month of year" ;
    skos:definition "The month of the year, whose value is a member of the class time:MonthOfYear" ;
    skos:editorialNote "Característica arriesgada - añadida en la revisión de 2017, y todavía no ampliamente utilizada.",
        "Feature at risk - added in 2017 revision, and not yet widely used. ",
        "No occurrences of this slot in the graph." ;
    skos:inScheme okns:time ;
    skos:mappingRelation time:monthOfYear ;
    skos:note "description: El mes del año, cuyo valor es un miembro de la clase 'mes del año'.",
        "description: The month of the year, whose value is a member of the class time:MonthOfYear",
        "title: mes del año" ;
    linkml:definition_uri okns:time_monthOfYear ;
    linkml:domain okns:TimeGeneralDateTimeDescription ;
    linkml:inlined true ;
    linkml:owner okns:time_monthOfYear ;
    linkml:range okns:TimeMonthOfYear ;
    linkml:slot_uri time:monthOfYear .

okns:time_nominalPosition a linkml:SlotDefinition ;
    dcterms:title "Name of temporal position" ;
    skos:definition "The (nominal) value indicating temporal position in an ordinal reference system" ;
    skos:editorialNote "No occurrences of this slot in the graph." ;
    skos:inScheme okns:time ;
    skos:mappingRelation time:nominalPosition ;
    skos:note "description: El valor (nominal) que indica posición temporal en un sistema de referencia ordinal.",
        "description: The (nominal) value indicating temporal position in an ordinal reference system",
        "title: nombre de posición temporal" ;
    linkml:definition_uri okns:time_nominalPosition ;
    linkml:domain okns:TimeTimePosition ;
    linkml:owner okns:time_nominalPosition ;
    linkml:range okns:string ;
    linkml:slot_uri time:nominalPosition .

okns:time_numericDuration a linkml:SlotDefinition ;
    dcterms:title "Numeric value of temporal duration" ;
    skos:definition "Value of a temporal extent expressed as a decimal number scaled by a temporal unit" ;
    skos:editorialNote "No occurrences of this slot in the graph." ;
    skos:inScheme okns:time ;
    skos:mappingRelation time:numericDuration ;
    skos:note "description: Valor de una extensión temporal expresada como un número decimal escalado por una unidad de tiempo.",
        "description: Value of a temporal extent expressed as a decimal number scaled by a temporal unit",
        "title: valor numérico de duración temporal" ;
    linkml:definition_uri okns:time_numericDuration ;
    linkml:domain okns:TimeDuration ;
    linkml:owner okns:time_numericDuration ;
    linkml:range okns:decimal ;
    linkml:slot_uri time:numericDuration .

okns:time_numericPosition a linkml:SlotDefinition ;
    dcterms:title "Numeric value of temporal position" ;
    skos:definition "The (numeric) value indicating position within a temporal coordinate system" ;
    skos:editorialNote "No occurrences of this slot in the graph." ;
    skos:inScheme okns:time ;
    skos:mappingRelation time:numericPosition ;
    skos:note "description: El valor (numérico) que indica posición temporal en un sistema de referencia ordinal.",
        "description: The (numeric) value indicating position within a temporal coordinate system",
        "title: valor numérico de posición temporal" ;
    linkml:definition_uri okns:time_numericPosition ;
    linkml:domain okns:TimeTimePosition ;
    linkml:owner okns:time_numericPosition ;
    linkml:range okns:decimal ;
    linkml:slot_uri time:numericPosition .

okns:time_second a linkml:SlotDefinition ;
    dcterms:title "second" ;
    skos:definition "Second position in a calendar-clock system." ;
    skos:editorialNote "No occurrences of this slot in the graph." ;
    skos:inScheme okns:time ;
    skos:mappingRelation time:second ;
    skos:note "description: Posición de segundo en un sistema calendario-reloj.",
        "title: segundo" ;
    linkml:definition_uri okns:time_second ;
    linkml:domain okns:TimeGeneralDateTimeDescription ;
    linkml:owner okns:time_second ;
    linkml:range okns:decimal ;
    linkml:slot_uri time:second .

okns:time_timeZone a linkml:SlotDefinition ;
    dcterms:title "in time zone" ;
    skos:definition "The time zone for clock elements in the temporal position" ;
    skos:editorialNote """En la versión original de OWL-Time de 2006, el rango de 'en huso horario' se definió en un espacio de nombres diferente "http://www.w3.org/2006/timezone#".
            Un axioma de alineación permite que los datos codificados de acuerdo con la versión anterior sean consistentes con la ontología actualizada.""",
        """IANA maintains a database of timezones. These are well maintained and generally considered authoritative, but individual items are not available at individual URIs, so cannot be used directly in data expressed using OWL-Time.

DBPedia provides a set of resources corresponding to the IANA timezones, with a URI for each (e.g. http://dbpedia.org/resource/Australia/Eucla). The World Clock service also provides a list of time zones with the description of each available as an individual webpage with a convenient individual URI (e.g. https://www.timeanddate.com/time/zones/acwst). These or other, similar, resources might be used as a value of the time:timeZone property.""",
        """IANA mantiene una base de datos de husos horarios. Éstas están bien mantenidas y generalmente se consideran autorizadas, pero los ítems individuales no están disponibles en URIs individuales, por tanto, no se pueden utilizar directamente en datos expresados utilizando OWL-Time.
            La BDPedia proporciona un conjunto de recursos correspondientes a los husos horarios de IANA, con una URI para cada uno (por ejemplo, http://dbpedia.org/resource/Australia/Eucla). El Servicio de Reloj Mundial también proporciona una lista de husos horarios con la descripción de cada uno de los disponibles como una página Web individual con una URI adecuada individual (por ejemplo, https://www.timeanddate.com/time/zones/acwst). Éstos, y otros recursos similares, se puden usar como un valor de la propiedad 'huso horario'.""",
        """In the original 2006 version of OWL-Time, the range of time:timeZone was a TimeZone class in a separate namespace "http://www.w3.org/2006/timezone#". 
An alignment axiom 
	tzont:TimeZone rdfs:subClassOf time:TimeZone . 
allows data encoded according to the previous version to be consistent with the updated ontology. """,
        "No occurrences of this slot in the graph." ;
    skos:inScheme okns:time ;
    skos:mappingRelation time:timeZone ;
    skos:note "title: en huso horario" ;
    linkml:definition_uri okns:time_timeZone ;
    linkml:domain okns:TimeGeneralDateTimeDescription ;
    linkml:inlined true ;
    linkml:owner okns:time_timeZone ;
    linkml:range okns:TimeTimeZone ;
    linkml:slot_uri time:timeZone .

okns:time_week a linkml:SlotDefinition ;
    dcterms:title "week" ;
    skos:definition "Week number within the year." ;
    skos:editorialNote "Las semanas están numeradas de forma diferente dependiendo del calendario en uso y de las convenciones lingüísticas y culturales locales (locale en inglés). El ISO-8601 especifica que la primera semana del año incluye al menos cuatro días, y que el lunes es el primer día de la semana. En ese sistema, la semana 1 es la semana que contiene el primer jueves del año.",
        "No occurrences of this slot in the graph.",
        "Weeks are numbered differently depending on the calendar in use and the local language or cultural conventions (locale). ISO-8601 specifies that the first week of the year includes at least four days, and that Monday is the first day of the week. In that system, week 1 is the week that contains the first Thursday in the year." ;
    skos:inScheme okns:time ;
    skos:mappingRelation time:week ;
    skos:note "description: Número de semana en el año.",
        "title: semana" ;
    linkml:definition_uri okns:time_week ;
    linkml:domain okns:TimeGeneralDateTimeDescription ;
    linkml:owner okns:time_week ;
    linkml:range okns:unsignedinteger ;
    linkml:slot_uri time:week .

okns:time_xsdDateTime a linkml:SlotDefinition ;
    dcterms:title "has XSD date-time" ;
    skos:definition "Value of DateTimeInterval expressed as a compact value." ;
    skos:editorialNote "No occurrences of this slot in the graph.",
        "Using xsd:dateTime in this place means that the duration of the interval is implicit: it corresponds to the length of the smallest non-zero element of the date-time literal. However, this rule cannot be used for intervals whose duration is more than one rank smaller than the starting time - e.g. the first minute or second of a day, the first hour of a month, or the first day of a year. In these cases the desired interval cannot be distinguished from the interval corresponding to the next rank up. Because of this essential ambiguity, use of this property is not recommended and it is deprecated.",
        "Utilizando xsd:dateTime en este lugar significa que la duración del intervalo está implícita: se corresponde con la longitud del elemento más pequeño distinto de cero del literal fecha-hora. Sin embargo, esta regla no se puede utilizar para intervalos cuya duración es mayor que un rango más pequeño que el tiempo de comienzo - p.ej. el primer minuto o segundo del día, la primera hora del mes, o el primer día del año. En estos casos el intervalo deseado no se puede distinguir del intervalo correspondiente al próximo rango más alto. Debido a esta ambigüedad esencial, no se recomienda el uso de esta propiedad y está desaprobada." ;
    skos:inScheme okns:time ;
    skos:mappingRelation time:xsdDateTime ;
    skos:note "description: Valor de 'intervalo de fecha-hora' expresado como un valor compacto.",
        "title: tiene fecha-hora XSD" ;
    linkml:deprecated "true" ;
    linkml:definition_uri okns:time_xsdDateTime ;
    linkml:domain okns:TimeDateTimeInterval ;
    linkml:owner okns:time_xsdDateTime ;
    linkml:range okns:datetime ;
    linkml:slot_uri time:xsdDateTime .

okns:time_year a linkml:SlotDefinition ;
    dcterms:title "year" ;
    skos:definition "Year position in a calendar-clock system.␊␊The range of this property is not specified, so can be replaced by any specific representation of a calendar year from any calendar." ;
    skos:editorialNote "No occurrences of this slot in the graph." ;
    skos:inScheme okns:time ;
    skos:mappingRelation time:year ;
    skos:note """description: Posición de año en un sistema calendario-reloj.

l rango de esta propiedad no está especificado, por tanto, se puede reemplazar por cualquier representación específica de un año de calendario de un calendario cualquiera.""" ;
    linkml:definition_uri okns:time_year ;
    linkml:domain okns:TimeGeneralDateTimeDescription ;
    linkml:inlined true ;
    linkml:owner okns:time_year ;
    linkml:range okns:Any ;
    linkml:slot_uri time:year .

okns:tzont_GMToffset a linkml:SlotDefinition ;
    skos:editorialNote "No occurrences of this slot in the graph." ;
    skos:inScheme okns:daml ;
    skos:mappingRelation tzont:GMToffset ;
    linkml:definition_uri okns:tzont_GMToffset ;
    linkml:domain okns:TzontTimeZone ;
    linkml:inlined true ;
    linkml:owner okns:tzont_GMToffset ;
    linkml:range okns:XsdDuration ;
    linkml:slot_uri tzont:GMToffset .

okns:tzont_exceptionalRegion a linkml:SlotDefinition ;
    skos:editorialNote "No occurrences of this slot in the graph." ;
    skos:inScheme okns:daml ;
    skos:mappingRelation tzont:exceptionalRegion ;
    linkml:definition_uri okns:tzont_exceptionalRegion ;
    linkml:domain okns:TzontRegion ;
    linkml:inlined true ;
    linkml:owner okns:tzont_exceptionalRegion ;
    linkml:range okns:TzontRegion ;
    linkml:slot_uri tzont:exceptionalRegion .

okns:tzont_hasDaylightSavingsPolicy a linkml:SlotDefinition ;
    skos:editorialNote "No occurrences of this slot in the graph." ;
    skos:inScheme okns:daml ;
    skos:mappingRelation tzont:hasDaylightSavingsPolicy ;
    linkml:definition_uri okns:tzont_hasDaylightSavingsPolicy ;
    linkml:domain okns:TzontRegion ;
    linkml:inlined true ;
    linkml:owner okns:tzont_hasDaylightSavingsPolicy ;
    linkml:range okns:TzontDaylightSavingsPolicy ;
    linkml:slot_uri tzont:hasDaylightSavingsPolicy .

okns:tzont_hasTimeZone a linkml:SlotDefinition ;
    skos:editorialNote "No occurrences of this slot in the graph." ;
    skos:inScheme okns:daml ;
    skos:mappingRelation tzont:hasTimeZone ;
    linkml:definition_uri okns:tzont_hasTimeZone ;
    linkml:domain okns:TzontRegion ;
    linkml:inlined true ;
    linkml:owner okns:tzont_hasTimeZone ;
    linkml:range okns:TzontTimeZone ;
    linkml:slot_uri tzont:hasTimeZone .

okns:tzont_observesDaylightSavingsTime a linkml:SlotDefinition ;
    skos:editorialNote "No occurrences of this slot in the graph." ;
    skos:inScheme okns:daml ;
    skos:mappingRelation tzont:observesDaylightSavingsTime ;
    linkml:definition_uri okns:tzont_observesDaylightSavingsTime ;
    linkml:domain okns:TzontRegion ;
    linkml:owner okns:tzont_observesDaylightSavingsTime ;
    linkml:range okns:boolean ;
    linkml:slot_uri tzont:observesDaylightSavingsTime .

okns:tzont_timeZonePart a linkml:SlotDefinition ;
    skos:editorialNote "No occurrences of this slot in the graph." ;
    skos:inScheme okns:daml ;
    skos:mappingRelation tzont:timeZonePart ;
    linkml:definition_uri okns:tzont_timeZonePart ;
    linkml:domain okns:TzontRegion ;
    linkml:inlined true ;
    linkml:owner okns:tzont_timeZonePart ;
    linkml:range okns:TzontRegion ;
    linkml:slot_uri tzont:timeZonePart .

okns:wgs_alt a linkml:SlotDefinition ;
    dcterms:title "altitude" ;
    skos:definition "The WGS84 altitude of a SpatialThing (decimal meters ␊above the local reference ellipsoid)." ;
    skos:editorialNote "No occurrences of this slot in the graph." ;
    skos:inScheme okns:wgs ;
    skos:mappingRelation wgs1:alt ;
    linkml:definition_uri okns:wgs_alt ;
    linkml:domain okns:WgsSpatialThing ;
    linkml:inlined true ;
    linkml:owner okns:wgs_alt ;
    linkml:range okns:Any ;
    linkml:slot_uri wgs1:alt .

okns:wgs_lat a linkml:SlotDefinition ;
    dcterms:title "latitude" ;
    skos:definition "The WGS84 latitude of a SpatialThing (decimal degrees)." ;
    skos:editorialNote "No occurrences of this slot in the graph." ;
    skos:inScheme okns:wgs ;
    skos:mappingRelation wgs1:lat ;
    linkml:definition_uri okns:wgs_lat ;
    linkml:domain okns:WgsSpatialThing ;
    linkml:inlined true ;
    linkml:owner okns:wgs_lat ;
    linkml:range okns:Any ;
    linkml:slot_uri wgs1:lat .

okns:wgs_long a linkml:SlotDefinition ;
    dcterms:title "longitude" ;
    skos:definition "The WGS84 longitude of a SpatialThing (decimal degrees)." ;
    skos:editorialNote "No occurrences of this slot in the graph." ;
    skos:inScheme okns:wgs ;
    skos:mappingRelation wgs1:long ;
    linkml:definition_uri okns:wgs_long ;
    linkml:domain okns:WgsSpatialThing ;
    linkml:inlined true ;
    linkml:owner okns:wgs_long ;
    linkml:range okns:Any ;
    linkml:slot_uri wgs1:long .

okns:wot_assurance a linkml:SlotDefinition ;
    dcterms:source wot: ;
    dcterms:title "Assurance" ;
    skos:definition "A property linking a document to an endorsement resource containing a detached ascii signature." ;
    skos:editorialNote "No occurrences of this slot in the graph." ;
    skos:inScheme okns:wot ;
    skos:mappingRelation wot:assurance ;
    linkml:definition_uri okns:wot_assurance ;
    linkml:domain okns:FoafDocument ;
    linkml:inlined true ;
    linkml:owner okns:wot_assurance ;
    linkml:range okns:WotEndorsement ;
    linkml:slot_uri wot:assurance .

okns:wot_encryptedTo a linkml:SlotDefinition ;
    dcterms:source wot: ;
    dcterms:title "Encrypted to" ;
    skos:definition "A property linking an encrypted document to a recipient." ;
    skos:editorialNote "No occurrences of this slot in the graph." ;
    skos:inScheme okns:wot ;
    skos:mappingRelation wot:encryptedTo ;
    linkml:definition_uri okns:wot_encryptedTo ;
    linkml:domain okns:WotEncryptedDocument ;
    linkml:inlined true ;
    linkml:owner okns:wot_encryptedTo ;
    linkml:range okns:WotPubKey ;
    linkml:slot_uri wot:encryptedTo .

okns:wot_encrypter a linkml:SlotDefinition ;
    dcterms:source wot: ;
    dcterms:title "Encrypted by" ;
    skos:definition "A property linking an encrypted document to the public key that was used to encrypt it." ;
    skos:editorialNote "No occurrences of this slot in the graph." ;
    skos:inScheme okns:wot ;
    skos:mappingRelation wot:encrypter ;
    linkml:definition_uri okns:wot_encrypter ;
    linkml:domain okns:WotEncryptedDocument ;
    linkml:inlined true ;
    linkml:owner okns:wot_encrypter ;
    linkml:range okns:WotPubKey ;
    linkml:slot_uri wot:encrypter .

okns:wot_fingerprint a linkml:SlotDefinition ;
    dcterms:source wot: ;
    dcterms:title "Fingerprint" ;
    skos:definition "A public key hex fingerprint string (40 digits, white space insignificant)." ;
    skos:editorialNote "No occurrences of this slot in the graph." ;
    skos:inScheme okns:wot ;
    skos:mappingRelation wot:fingerprint ;
    linkml:definition_uri okns:wot_fingerprint ;
    linkml:domain okns:WotPubKey ;
    linkml:owner okns:wot_fingerprint ;
    linkml:range okns:string ;
    linkml:slot_uri wot:fingerprint .

okns:wot_hex_id a linkml:SlotDefinition ;
    dcterms:source wot: ;
    dcterms:title "Hex identifier" ;
    skos:definition "A public key hex identifier string (8 digits)." ;
    skos:editorialNote "No occurrences of this slot in the graph." ;
    skos:inScheme okns:wot ;
    skos:mappingRelation wot:hex_id ;
    linkml:definition_uri okns:wot_hex_id ;
    linkml:domain okns:WotPubKey ;
    linkml:owner okns:wot_hex_id ;
    linkml:range okns:string ;
    linkml:slot_uri wot:hex_id .

okns:wot_length a linkml:SlotDefinition ;
    dcterms:source wot: ;
    dcterms:title "Length" ;
    skos:definition "A numeric string representing the length, in bytes, of a public key." ;
    skos:editorialNote "No occurrences of this slot in the graph." ;
    skos:inScheme okns:wot ;
    skos:mappingRelation wot:length ;
    linkml:definition_uri okns:wot_length ;
    linkml:domain okns:WotPubKey ;
    linkml:owner okns:wot_length ;
    linkml:range okns:integer ;
    linkml:slot_uri wot:length .

okns:wot_pubkeyAddress a linkml:SlotDefinition ;
    dcterms:source wot: ;
    dcterms:title "Address" ;
    skos:definition "The location of an ascii version of a public key." ;
    skos:editorialNote "No occurrences of this slot in the graph." ;
    skos:inScheme okns:wot ;
    skos:mappingRelation wot:pubkeyAddress ;
    linkml:definition_uri okns:wot_pubkeyAddress ;
    linkml:domain okns:WotPubKey ;
    linkml:inlined true ;
    linkml:owner okns:wot_pubkeyAddress ;
    linkml:range okns:FoafDocument ;
    linkml:slot_uri wot:pubkeyAddress .

okns:wot_sigdate a linkml:SlotDefinition ;
    dcterms:source wot: ;
    dcterms:title "Signature date" ;
    skos:definition "The date of a public key signature event." ;
    skos:editorialNote "No occurrences of this slot in the graph." ;
    skos:inScheme okns:wot ;
    skos:mappingRelation wot:sigdate ;
    linkml:definition_uri okns:wot_sigdate ;
    linkml:domain okns:WotSigEvent ;
    linkml:owner okns:wot_sigdate ;
    linkml:range okns:date ;
    linkml:slot_uri wot:sigdate .

okns:wot_signed a linkml:SlotDefinition ;
    dcterms:source wot: ;
    dcterms:title "Signed" ;
    skos:definition "A property linking a public key to a public key signature event." ;
    skos:editorialNote "No occurrences of this slot in the graph." ;
    skos:inScheme okns:wot ;
    skos:mappingRelation wot:signed ;
    linkml:definition_uri okns:wot_signed ;
    linkml:domain okns:WotPubKey ;
    linkml:inlined true ;
    linkml:owner okns:wot_signed ;
    linkml:range okns:WotSigEvent ;
    linkml:slot_uri wot:signed .

okns:wot_signer a linkml:SlotDefinition ;
    dcterms:source wot: ;
    dcterms:title "Signer" ;
    skos:definition "A property linking a public key signature event to the public key that was used to sign." ;
    skos:editorialNote "No occurrences of this slot in the graph." ;
    skos:inScheme okns:wot ;
    skos:mappingRelation wot:signer ;
    linkml:definition_uri okns:wot_signer ;
    linkml:domain okns:WotSigEvent ;
    linkml:inlined true ;
    linkml:owner okns:wot_signer ;
    linkml:range okns:WotPubKey ;
    linkml:slot_uri wot:signer .

okns:wot_sigtime a linkml:SlotDefinition ;
    dcterms:source wot: ;
    dcterms:title "Signature time" ;
    skos:definition "The time (of day) of a public key signature event." ;
    skos:editorialNote "No occurrences of this slot in the graph." ;
    skos:inScheme okns:wot ;
    skos:mappingRelation wot:sigtime ;
    linkml:definition_uri okns:wot_sigtime ;
    linkml:domain okns:WotSigEvent ;
    linkml:owner okns:wot_sigtime ;
    linkml:range okns:time ;
    linkml:slot_uri wot:sigtime .

okns:Daml-oilDatatypeProperty a linkml:ClassDefinition ;
    dcterms:title "DatatypeProperty" ;
    skos:definition "if P is a DatatypeProperty, and P(x, y), then y is a data value." ;
    skos:inScheme okns:daml ;
    skos:mappingRelation daml-oil:DatatypeProperty ;
    linkml:class_uri daml-oil:DatatypeProperty ;
    linkml:definition_uri okns:Daml-oilDatatypeProperty ;
    linkml:is_a okns:RdfProperty ;
    linkml:slot_usage [ ] ;
    linkml:slots okns:daml_oil_domain,
        okns:daml_oil_range .

okns:Daml-oilProperty a linkml:ClassDefinition ;
    skos:inScheme okns:daml ;
    skos:mappingRelation daml-oil:Property ;
    linkml:class_uri daml-oil:Property ;
    linkml:definition_uri okns:Daml-oilProperty ;
    linkml:slot_usage [ ] ;
    linkml:slots okns:daml_oil_domain,
        okns:daml_oil_range .

okns:Daml-usregionstateUSRegion a linkml:ClassDefinition ;
    dcterms:title "USRegion" ;
    skos:definition "Information about the US regions." ;
    skos:inScheme okns:daml ;
    skos:mappingRelation daml-usregionstate:USRegion ;
    linkml:class_uri daml-usregionstate:USRegion ;
    linkml:definition_uri okns:Daml-usregionstateUSRegion ;
    linkml:is_a okns:Daml-oilThing ;
    linkml:slot_usage [ ] .

okns:Daml-usregionstateUSState a linkml:ClassDefinition ;
    dcterms:title "USState" ;
    skos:definition "Information about one of the US states." ;
    skos:inScheme okns:daml ;
    skos:mappingRelation daml-usregionstate:USState ;
    linkml:class_uri daml-usregionstate:USState ;
    linkml:definition_uri okns:Daml-usregionstateUSState ;
    linkml:is_a okns:Daml-stateState ;
    linkml:slot_usage [ ] .

okns:DcmitypeImage a linkml:ClassDefinition ;
    dcterms:source dcmitype: ;
    dcterms:title "Image" ;
    skos:definition "Examples include images and photographs of physical objects, paintings, prints, drawings, other images and graphics, animations and moving pictures, film, diagrams, maps, musical notation.  Note that Image may include both electronic and physical representations." ;
    skos:inScheme okns:dc ;
    skos:mappingRelation dcmitype:Image ;
    skos:note "description: A visual representation other than text." ;
    linkml:class_uri dcmitype:Image ;
    linkml:definition_uri okns:DcmitypeImage ;
    linkml:slot_usage [ ] .

okns:DctIMT a linkml:ClassDefinition ;
    skos:inScheme okns:frbr ;
    skos:mappingRelation dcterms:IMT ;
    linkml:class_uri dcterms:IMT ;
    linkml:definition_uri okns:DctIMT ;
    linkml:slot_usage [ ] ;
    linkml:slots okns:rdf_value,
        okns:rdfs_label .

okns:DctMediaTypeOrExtent a linkml:ClassDefinition ;
    dcterms:source dcterms: ;
    dcterms:title "Media Type or Extent" ;
    skos:definition "A media type or extent." ;
    skos:inScheme okns:dc ;
    skos:mappingRelation dcterms:MediaTypeOrExtent ;
    linkml:class_uri dcterms:MediaTypeOrExtent ;
    linkml:definition_uri okns:DctMediaTypeOrExtent ;
    linkml:slot_usage [ ] .

okns:IcalDomainOfRrule a linkml:ClassDefinition ;
    skos:inScheme okns:ical ;
    skos:mappingRelation ical:DomainOf_rrule ;
    linkml:class_uri ical:DomainOf_rrule ;
    linkml:definition_uri okns:IcalDomainOfRrule ;
    linkml:slot_usage [ ] .

okns:IcalValueCAL-ADDRESS a linkml:ClassDefinition ;
    skos:inScheme okns:ical ;
    skos:mappingRelation ical:Value_CAL-ADDRESS ;
    linkml:class_uri ical:Value_CAL-ADDRESS ;
    linkml:definition_uri okns:IcalValueCAL-ADDRESS ;
    linkml:slot_usage [ ] .

okns:IcalValueRECUR a linkml:ClassDefinition ;
    skos:inScheme okns:ical ;
    skos:mappingRelation ical:Value_RECUR ;
    linkml:class_uri ical:Value_RECUR ;
    linkml:definition_uri okns:IcalValueRECUR ;
    linkml:slot_usage [ ] .

okns:MoAnalogSignal a linkml:ClassDefinition ;
    dcterms:source <http://purl.org/ontology/mo/> ;
    dcterms:title "analogue signal" ;
    skos:definition "An analog signal." ;
    skos:inScheme okns:mo ;
    skos:mappingRelation ns1:AnalogSignal ;
    linkml:class_uri <http://purl.org/ontology/mo/AnalogSignal> ;
    linkml:definition_uri okns:MoAnalogSignal ;
    linkml:is_a okns:MoSignal ;
    linkml:slot_usage [ ] .

okns:MoInstrument a linkml:ClassDefinition ;
    dcterms:source <http://purl.org/ontology/mo/> ;
    dcterms:title "Instrument" ;
    rdfs:seeAlso <http://purl.org/ontology/mo/mit#> ;
    skos:definition "Any of various devices or contrivances that can be used to produce musical tones or sound.␊        ␊        Any taxonomy can be used to subsume this concept. The default one is one extracted by Ivan Herman␊        from the Musicbrainz instrument taxonomy, conforming to SKOS. This concept holds a seeAlso link ␊        towards this taxonomy." ;
    skos:inScheme okns:mo ;
    skos:mappingRelation ns1:Instrument ;
    linkml:class_uri <http://purl.org/ontology/mo/Instrument> ;
    linkml:definition_uri okns:MoInstrument ;
    linkml:slot_usage [ ] .

okns:MoLabel a linkml:ClassDefinition ;
    dcterms:source <http://purl.org/ontology/mo/> ;
    dcterms:title "label" ;
    skos:definition "Trade name of a company that produces musical works or expression of musical works." ;
    skos:inScheme okns:mo ;
    skos:mappingRelation ns1:Label ;
    linkml:class_uri <http://purl.org/ontology/mo/Label> ;
    linkml:definition_uri okns:MoLabel ;
    linkml:is_a okns:MoCorporateBody ;
    linkml:slot_usage [ ] .

okns:MoLyrics a linkml:ClassDefinition ;
    dcterms:source <http://purl.org/ontology/mo/> ;
    dcterms:title "lyrics" ;
    skos:definition "Lyrics" ;
    skos:inScheme okns:mo ;
    skos:mappingRelation ns1:Lyrics ;
    linkml:class_uri <http://purl.org/ontology/mo/Lyrics> ;
    linkml:definition_uri okns:MoLyrics ;
    linkml:is_a okns:MoMusicalExpression ;
    linkml:slot_usage [ ] .

okns:MoMovement a linkml:ClassDefinition ;
    dcterms:source <http://purl.org/ontology/mo/> ;
    dcterms:title "movement" ;
    skos:definition "A movement is a self-contained part of a musical work. While individual or selected movements from a composition are sometimes performed separately, a performance of the complete work requires all the movements to be performed in succession.␊␊Often a composer attempts to interrelate the movements thematically, or sometimes in more subtle ways, in order that the individual␊movements exert a cumulative effect. In some forms, composers sometimes link the movements, or ask for them to be played without a␊pause between them." ;
    skos:inScheme okns:mo ;
    skos:mappingRelation ns1:Movement ;
    linkml:class_uri <http://purl.org/ontology/mo/Movement> ;
    linkml:definition_uri okns:MoMovement ;
    linkml:is_a okns:MoMusicalWork ;
    linkml:slot_usage [ ] .

okns:MoSignalGroup a linkml:ClassDefinition ;
    dcterms:source <http://purl.org/ontology/mo/> ;
    dcterms:title "signal group" ;
    skos:definition "A musical expression representing a group of signals, for example a set of masters resulting from a whole recording/mastering session." ;
    skos:inScheme okns:mo ;
    skos:mappingRelation ns1:SignalGroup ;
    linkml:class_uri <http://purl.org/ontology/mo/SignalGroup> ;
    linkml:definition_uri okns:MoSignalGroup ;
    linkml:is_a okns:MoMusicalExpression ;
    linkml:slot_usage [ ] .

okns:RdfCompoundLiteral a linkml:ClassDefinition ;
    dcterms:source rdf: ;
    dcterms:title "CompoundLiteral" ;
    rdfs:seeAlso <https://www.w3.org/TR/json-ld11/#the-rdf-compoundliteral-class-and-the-rdf-language-and-rdf-direction-properties> ;
    skos:definition "A class representing a compound literal." ;
    skos:inScheme okns:owl-rdf-rdfs ;
    skos:mappingRelation rdf:CompoundLiteral ;
    linkml:class_uri rdf:CompoundLiteral ;
    linkml:definition_uri okns:RdfCompoundLiteral ;
    linkml:is_a okns:RdfsResource ;
    linkml:slot_usage [ ] .

okns:SkosCollection a linkml:ClassDefinition ;
    dcterms:source <http://www.w3.org/2004/02/skos/core> ;
    dcterms:title "Collection" ;
    skos:definition "A meaningful collection of concepts." ;
    skos:editorialNote "Labelled collections can be used where you would like a set of concepts to be displayed under a 'node label' in the hierarchy." ;
    skos:inScheme okns:skos ;
    skos:mappingRelation skos:Collection ;
    linkml:class_uri skos:Collection ;
    linkml:definition_uri okns:SkosCollection ;
    linkml:slot_usage [ ] .

okns:Time-entryCalendarClockInterval a linkml:ClassDefinition ;
    skos:inScheme okns:daml ;
    skos:mappingRelation time-entry:CalendarClockInterval ;
    linkml:class_uri time-entry:CalendarClockInterval ;
    linkml:definition_uri okns:Time-entryCalendarClockInterval ;
    linkml:is_a okns:Time-entryProperInterval ;
    linkml:slot_usage [ ] .

okns:TimeDateTimeDescription a linkml:ClassDefinition ;
    dcterms:title "Date-Time description" ;
    skos:definition "Description of date and time structured with separate values for the various elements of a calendar-clock system. The temporal reference system is fixed to Gregorian Calendar, and the range of year, month, day properties restricted to corresponding XML Schema types xsd:gYear, xsd:gMonth and xsd:gDay, respectively." ;
    skos:inScheme okns:time ;
    skos:mappingRelation time:DateTimeDescription ;
    skos:note "description: Descripción de fecha y tiempo estructurada con valores separados para los diferentes elementos de un sistema calendario-reloj. El sistema de referencia temporal está fijado al calendario gregoriano, y el rango de las propiedades año, mes, día restringidas a los correspondientes tipos del XML Schema xsd:gYear, xsd:gMonth y xsd:gDay respectivamente.",
        "description: Description of date and time structured with separate values for the various elements of a calendar-clock system. The temporal reference system is fixed to Gregorian Calendar, and the range of year, month, day properties restricted to corresponding XML Schema types xsd:gYear, xsd:gMonth and xsd:gDay, respectively.",
        "title: descripción de fecha-tiempo" ;
    linkml:class_uri time:DateTimeDescription ;
    linkml:definition_uri okns:TimeDateTimeDescription ;
    linkml:is_a okns:TimeGeneralDateTimeDescription ;
    linkml:slot_usage [ ] .

okns:TimeDateTimeInterval a linkml:ClassDefinition ;
    dcterms:title "Date-time interval" ;
    skos:definition "DateTimeInterval is a subclass of ProperInterval, defined using the multi-element DateTimeDescription." ;
    skos:editorialNote "'intervalo de fecha-hora' se puede utilizar sólo para un intervalo cuyos límites coinciden con un elemento de fecha-hora alineados con el calendario y la zona horaria indicados. Por ejemplo, aunque ambos tienen una duración de un día, el intervalo de 24 horas que empieza en la media noche del comienzo del 8 mayo en Europa Central se puede expresar como un 'intervalo de fecha-hora', el intervalo de 24 horas que empieza a las 1:30pm no.",
        ":DateTimeInterval can only be used for an interval whose limits coincide with a date-time element aligned to the calendar and timezone indicated. For example, while both have a duration of one day, the 24-hour interval beginning at midnight at the beginning of 8 May in Central Europe can be expressed as a :DateTimeInterval, but the 24-hour interval starting at 1:30pm cannot." ;
    skos:inScheme okns:time ;
    skos:mappingRelation time:DateTimeInterval ;
    skos:note "description: 'intervalo de fecha-hora' es una subclase de 'intervalo propio', definida utilizando el multi-elemento 'descripción de fecha-hora'.",
        "description: DateTimeInterval is a subclass of ProperInterval, defined using the multi-element DateTimeDescription.",
        "title: intervalo de fecha-hora" ;
    linkml:class_uri time:DateTimeInterval ;
    linkml:definition_uri okns:TimeDateTimeInterval ;
    linkml:is_a okns:TimeProperInterval ;
    linkml:slot_usage [ ] .

okns:TimeDuration a linkml:ClassDefinition ;
    dcterms:title "Time duration" ;
    skos:definition "Duration of a temporal extent expressed as a number scaled by a temporal unit" ;
    skos:editorialNote "Alternativa a 'descripción de tiempo' para proporcionar descripción soporte a una duración temporal diferente a utilizar un sistema de calendario/reloj.",
        "Alternative to time:DurationDescription to support description of a temporal duration other than using a calendar/clock system." ;
    skos:inScheme okns:time ;
    skos:mappingRelation time:Duration ;
    skos:note "description: Duración de una extensión temporal expresada como un número escalado por una unidad temporal.",
        "description: Duration of a temporal extent expressed as a number scaled by a temporal unit",
        "title: duración de tiempo" ;
    linkml:class_uri time:Duration ;
    linkml:definition_uri okns:TimeDuration ;
    linkml:is_a okns:TimeTemporalDuration ;
    linkml:slot_usage [ ] .

okns:TimeInterval a linkml:ClassDefinition ;
    dcterms:title "Time interval" ;
    skos:definition "A temporal entity with an extent or duration" ;
    skos:inScheme okns:time ;
    skos:mappingRelation time:Interval ;
    skos:note "description: A temporal entity with an extent or duration",
        "description: Una entidad temporal con una extensión o duración.",
        "title: intervalo de tiempo" ;
    linkml:class_uri time:Interval ;
    linkml:definition_uri okns:TimeInterval ;
    linkml:is_a okns:TimeTemporalEntity ;
    linkml:slot_usage [ ] .

okns:TzontDaylightSavingsPolicy a linkml:ClassDefinition ;
    skos:inScheme okns:daml ;
    skos:mappingRelation tzont:DaylightSavingsPolicy ;
    linkml:class_uri tzont:DaylightSavingsPolicy ;
    linkml:definition_uri okns:TzontDaylightSavingsPolicy ;
    linkml:slot_usage [ ] .

okns:Wn16Endorsement-4 a linkml:ClassDefinition ;
    dcterms:title "No class (entity type) name specified -- this class is noted as a superclass of another class in this graph but has not itself been defined." ;
    skos:inScheme okns:wot ;
    skos:mappingRelation wn16:Endorsement-4 ;
    linkml:class_uri wn16:Endorsement-4 ;
    linkml:definition_uri okns:Wn16Endorsement-4 ;
    linkml:slot_usage [ ] .

okns:WotEncryptedDocument a linkml:ClassDefinition ;
    dcterms:source wot: ;
    dcterms:title "Encrypted Document" ;
    skos:definition "An encrypted document intended for a set of recipients." ;
    skos:inScheme okns:wot ;
    skos:mappingRelation wot:EncryptedDocument ;
    linkml:class_uri wot:EncryptedDocument ;
    linkml:definition_uri okns:WotEncryptedDocument ;
    linkml:is_a okns:Wn16Endorsement-4 ;
    linkml:slot_usage [ ] .

okns:WotUser a linkml:ClassDefinition ;
    dcterms:source wot: ;
    dcterms:title "Key User" ;
    skos:definition "A user (agent, person, group or organization) of a PGP/GPG public key." ;
    skos:inScheme okns:wot ;
    skos:mappingRelation wot:User ;
    linkml:class_uri wot:User ;
    linkml:definition_uri okns:WotUser ;
    linkml:is_a okns:FoafAgent ;
    linkml:slot_usage [ ] .

okns:XsdGYear a linkml:ClassDefinition ;
    dcterms:title "No class (entity type) name specified -- this class is noted as being in the domain or range of a slot in this graph but has not itself been defined." ;
    skos:inScheme okns:time ;
    skos:mappingRelation xsd:gYear ;
    linkml:class_uri xsd:gYear ;
    linkml:definition_uri okns:XsdGYear ;
    linkml:slot_usage [ ] .

okns:ao_genre a linkml:SlotDefinition ;
    dcterms:source ao: ;
    dcterms:title "has genre" ;
    rdfs:subPropertyOf okns:dct_subject ;
    skos:definition "An genre of something." ;
    skos:editorialNote "No occurrences of this slot in the graph." ;
    skos:inScheme okns:ao ;
    skos:mappingRelation ao:genre ;
    linkml:definition_uri okns:ao_genre ;
    linkml:domain okns:OwlThing ;
    linkml:inlined true ;
    linkml:owner okns:ao_genre ;
    linkml:range okns:Any ;
    linkml:slot_uri ao:genre .

okns:daml_comment a linkml:SlotDefinition ;
    skos:inScheme okns:daml ;
    skos:mappingRelation daml:comment ;
    linkml:definition_uri okns:daml_comment ;
    linkml:domain_of okns:DamlClass,
        okns:DamlProperty ;
    linkml:owner okns:DamlProperty ;
    linkml:range okns:string ;
    linkml:slot_uri daml:comment .

okns:daml_label a linkml:SlotDefinition ;
    skos:inScheme okns:daml ;
    skos:mappingRelation daml:label ;
    linkml:definition_uri okns:daml_label ;
    linkml:domain_of okns:DamlClass,
        okns:DamlProperty ;
    linkml:owner okns:DamlProperty ;
    linkml:range okns:string ;
    linkml:slot_uri daml:label .

okns:daml_oil_label a linkml:SlotDefinition ;
    skos:inScheme okns:daml ;
    skos:mappingRelation daml-oil:label ;
    linkml:definition_uri okns:daml_oil_label ;
    linkml:domain_of okns:Daml-oilClass ;
    linkml:owner okns:Daml-oilClass ;
    linkml:range okns:string ;
    linkml:slot_uri daml-oil:label .

okns:daml_oil_subClassOf a linkml:SlotDefinition ;
    skos:inScheme okns:daml ;
    skos:mappingRelation daml-oil:subClassOf ;
    linkml:any_of [ a okns:AnonymousSlotExpression ;
            linkml:range okns:Daml-oilClass ],
        [ a okns:AnonymousSlotExpression ;
            linkml:range okns:uri ],
        [ a okns:AnonymousSlotExpression ;
            linkml:range okns:Daml-2001Class ] ;
    linkml:definition_uri okns:daml_oil_subClassOf ;
    linkml:domain_of okns:Daml-oilClass ;
    linkml:inlined true ;
    linkml:owner okns:Daml-oilClass ;
    linkml:range okns:Any ;
    linkml:slot_uri daml-oil:subClassOf .

okns:daml_ont_name a linkml:SlotDefinition ;
    skos:inScheme okns:daml ;
    skos:mappingRelation daml-ont:name ;
    linkml:definition_uri okns:daml_ont_name ;
    linkml:domain_of okns:Daml-ontCountry,
        okns:Daml-ontUSState ;
    linkml:owner okns:Daml-ontUSState ;
    linkml:range okns:string ;
    linkml:slot_uri daml-ont:name .

okns:daml_sameClassAs a linkml:SlotDefinition ;
    skos:inScheme okns:daml ;
    skos:mappingRelation daml:sameClassAs ;
    linkml:any_of [ a okns:AnonymousSlotExpression ;
            linkml:range okns:Daml-ontCountry ],
        [ a okns:AnonymousSlotExpression ;
            linkml:range okns:uri ] ;
    linkml:definition_uri okns:daml_sameClassAs ;
    linkml:domain_of okns:Daml-ontCountry,
        okns:DamlClass ;
    linkml:inlined true ;
    linkml:owner okns:DamlClass ;
    linkml:range okns:Any ;
    linkml:slot_uri daml:sameClassAs .

okns:dct_audience a linkml:SlotDefinition ;
    dcterms:source dcterms: ;
    dcterms:title "Audience" ;
    skos:definition "Recommended practice is to use this property with non-literal values from a vocabulary of audience types." ;
    skos:editorialNote "No occurrences of this slot in the graph." ;
    skos:inScheme okns:dc ;
    skos:mappingRelation dcterms:audience ;
    skos:note "description: A class of agents for whom the resource is intended or useful." ;
    linkml:definition_uri okns:dct_audience ;
    linkml:inlined true ;
    linkml:range okns:Any ;
    linkml:slot_uri dcterms:audience .

okns:dct_coverage a linkml:SlotDefinition ;
    dcterms:source dcterms: ;
    dcterms:title "Coverage" ;
    rdfs:subPropertyOf okns:dc_coverage ;
    skos:definition "Spatial topic and spatial applicability may be a named place or a location specified by its geographic coordinates. Temporal topic may be a named period, date, or date range. A jurisdiction may be a named administrative entity or a geographic place to which the resource applies. Recommended practice is to use a controlled vocabulary such as the Getty Thesaurus of Geographic Names [[TGN](https://www.getty.edu/research/tools/vocabulary/tgn/index.html)]. Where appropriate, named places or time periods may be used in preference to numeric identifiers such as sets of coordinates or date ranges.  Because coverage is so broadly defined, it is preferable to use the more specific subproperties Temporal Coverage and Spatial Coverage." ;
    skos:editorialNote "No occurrences of this slot in the graph." ;
    skos:inScheme okns:dc ;
    skos:mappingRelation dcterms:coverage ;
    skos:note "description: The spatial or temporal topic of the resource, spatial applicability of the resource, or jurisdiction under which the resource is relevant." ;
    linkml:definition_uri okns:dct_coverage ;
    linkml:inlined true ;
    linkml:range okns:Any ;
    linkml:slot_uri dcterms:coverage .

okns:dct_description a linkml:SlotDefinition ;
    dcterms:source dcterms: ;
    dcterms:title "Description" ;
    rdfs:subPropertyOf okns:dc_description ;
    skos:definition "Description may include but is not limited to: an abstract, a table of contents, a graphical representation, or a free-text account of the resource." ;
    skos:inScheme okns:dc ;
    skos:mappingRelation dcterms:description ;
    skos:note "description: An account of the resource." ;
    linkml:definition_uri okns:dct_description ;
    linkml:range okns:string ;
    linkml:slot_uri dcterms:description .

okns:dct_identifier a linkml:SlotDefinition ;
    dcterms:source dcterms: ;
    dcterms:title "Identifier" ;
    rdfs:subPropertyOf okns:dc_identifier ;
    skos:definition "Recommended practice is to identify the resource by means of a string conforming to an identification system. Examples include International Standard Book Number (ISBN), Digital Object Identifier (DOI), and Uniform Resource Name (URN).  Persistent identifiers should be provided as HTTP URIs." ;
    skos:editorialNote "No occurrences of this slot in the graph." ;
    skos:inScheme okns:dc ;
    skos:mappingRelation dcterms:identifier ;
    skos:note "description: An unambiguous reference to the resource within a given context." ;
    linkml:definition_uri okns:dct_identifier ;
    linkml:inlined true ;
    linkml:range okns:RdfsLiteral ;
    linkml:slot_uri dcterms:identifier .

okns:dct_issued a linkml:SlotDefinition ;
    dcterms:source dcterms: ;
    dcterms:title "Date Issued" ;
    rdfs:subPropertyOf okns:dct_date ;
    skos:definition "Recommended practice is to describe the date, date/time, or period of time as recommended for the property Date, of which this is a subproperty." ;
    skos:inScheme okns:dc ;
    skos:mappingRelation dcterms:issued ;
    skos:note "description: Date of formal issuance of the resource." ;
    linkml:any_of [ a okns:AnonymousSlotExpression ;
            linkml:range okns:RdfsLiteral ],
        [ a okns:AnonymousSlotExpression ;
            linkml:range okns:date ] ;
    linkml:definition_uri okns:dct_issued ;
    linkml:domain_of okns:DcamVocabularyEncodingScheme,
        okns:DctAgentClass ;
    linkml:inlined true ;
    linkml:owner okns:DctAgentClass ;
    linkml:range okns:Any ;
    linkml:slot_uri dcterms:issued .

okns:dct_rights a linkml:SlotDefinition ;
    dcterms:source dcterms: ;
    dcterms:title "Rights" ;
    rdfs:subPropertyOf okns:dc_rights ;
    skos:definition "Typically, rights information includes a statement about various property rights associated with the resource, including intellectual property rights.  Recommended practice is to refer to a rights statement with a URI.  If this is not possible or feasible, a literal value (name, label, or short text) may be provided." ;
    skos:editorialNote "No occurrences of this slot in the graph." ;
    skos:inScheme okns:dc ;
    skos:mappingRelation dcterms:rights ;
    skos:note "description: Information about rights held in and over the resource." ;
    linkml:definition_uri okns:dct_rights ;
    linkml:inlined true ;
    linkml:range okns:Any ;
    linkml:slot_uri dcterms:rights .

okns:foaf_depicts a linkml:SlotDefinition ;
    dcterms:source foaf: ;
    dcterms:title "depicts" ;
    owl:inverseOf okns:foaf_depiction ;
    skos:definition "A thing depicted in this representation." ;
    skos:editorialNote "No occurrences of this slot in the graph." ;
    skos:inScheme okns:foaf ;
    skos:mappingRelation foaf:depicts ;
    linkml:definition_uri okns:foaf_depicts ;
    linkml:domain okns:FoafImage ;
    linkml:inlined true ;
    linkml:owner okns:foaf_depicts ;
    linkml:range okns:OwlThing ;
    linkml:slot_uri foaf:depicts .

okns:foaf_made a linkml:SlotDefinition ;
    dcterms:source foaf: ;
    dcterms:title "made" ;
    owl:inverseOf okns:foaf_maker ;
    skos:definition "Something that was made by this agent." ;
    skos:editorialNote "No occurrences of this slot in the graph." ;
    skos:inScheme okns:foaf ;
    skos:mappingRelation foaf:made ;
    linkml:definition_uri okns:foaf_made ;
    linkml:domain okns:FoafAgent ;
    linkml:inlined true ;
    linkml:owner okns:foaf_made ;
    linkml:range okns:OwlThing ;
    linkml:slot_uri foaf:made .

okns:foaf_maker a linkml:SlotDefinition ;
    dcterms:source foaf: ;
    dcterms:title "maker" ;
    owl:inverseOf okns:foaf_made ;
    skos:definition "An agent that  made this thing." ;
    skos:editorialNote "No occurrences of this slot in the graph." ;
    skos:exactMatch dcterms:creator ;
    skos:inScheme okns:foaf ;
    skos:mappingRelation foaf:maker ;
    linkml:definition_uri okns:foaf_maker ;
    linkml:domain okns:OwlThing ;
    linkml:inlined true ;
    linkml:owner okns:foaf_maker ;
    linkml:range okns:FoafAgent ;
    linkml:slot_uri foaf:maker .

okns:foaf_primaryTopic a linkml:SlotDefinition ;
    dcterms:source foaf: ;
    dcterms:title "primary topic" ;
    owl:inverseOf okns:foaf_isPrimaryTopicOf ;
    skos:definition "The primary topic of some page or document." ;
    skos:editorialNote "No occurrences of this slot in the graph." ;
    skos:inScheme okns:foaf ;
    skos:mappingRelation foaf:primaryTopic ;
    linkml:definition_uri okns:foaf_primaryTopic ;
    linkml:domain okns:FoafDocument ;
    linkml:inlined true ;
    linkml:owner okns:foaf_primaryTopic ;
    linkml:range okns:OwlThing ;
    linkml:slot_uri foaf:primaryTopic .

okns:foaf_topic a linkml:SlotDefinition ;
    dcterms:source foaf: ;
    dcterms:title "topic" ;
    owl:inverseOf okns:foaf_page ;
    skos:definition "A topic of some page or document." ;
    skos:editorialNote "No occurrences of this slot in the graph." ;
    skos:inScheme okns:foaf ;
    skos:mappingRelation foaf:topic ;
    linkml:definition_uri okns:foaf_topic ;
    linkml:domain okns:FoafDocument ;
    linkml:inlined true ;
    linkml:owner okns:foaf_topic ;
    linkml:range okns:OwlThing ;
    linkml:slot_uri foaf:topic .

okns:frbr_abridgement a linkml:SlotDefinition ;
    dcterms:source frbr: ;
    dcterms:title "abridgement" ;
    rdfs:subPropertyOf okns:frbr_relatedEndeavour ;
    owl:inverseOf okns:frbr_abridgementOf ;
    skos:definition "An abridgment of an expression." ;
    skos:editorialNote "N53f44b1328b8426f8afa5f29c31ea02b",
        "N9075c196f3f54eb9ad7fe60038d0b116",
        "Nf05e5a3f0dbe4e31ba6fb825fd2724db",
        "No occurrences of this slot in the graph." ;
    skos:inScheme okns:frbr ;
    skos:mappingRelation frbr:abridgement ;
    linkml:definition_uri okns:frbr_abridgement ;
    linkml:domain okns:FrbrExpression ;
    linkml:inlined true ;
    linkml:owner okns:frbr_abridgement ;
    linkml:range okns:FrbrExpression ;
    linkml:slot_uri frbr:abridgement .

okns:frbr_abridgementOf a linkml:SlotDefinition ;
    dcterms:source frbr: ;
    dcterms:title "abridgement of" ;
    rdfs:subPropertyOf okns:frbr_relatedEndeavour ;
    owl:inverseOf okns:frbr_abridgement ;
    skos:definition "An expression that is abridged." ;
    skos:editorialNote "Na1d6cf78ceb64de6b50c8932c6ddcb34",
        "Nb8e0e48d0fc341c3ab525b3ebb30e26d",
        "Ndb7f22c6d95a47c49ae1f77a33f8058b",
        "No occurrences of this slot in the graph." ;
    skos:inScheme okns:frbr ;
    skos:mappingRelation frbr:abridgementOf ;
    linkml:definition_uri okns:frbr_abridgementOf ;
    linkml:domain okns:FrbrExpression ;
    linkml:inlined true ;
    linkml:owner okns:frbr_abridgementOf ;
    linkml:range okns:FrbrExpression ;
    linkml:slot_uri frbr:abridgementOf .

okns:frbr_alternate a linkml:SlotDefinition ;
    dcterms:source frbr: ;
    dcterms:title "alternate" ;
    rdfs:subPropertyOf okns:frbr_relatedEndeavour ;
    owl:inverseOf okns:frbr_alternateOf ;
    skos:definition "An alternative to a manifestation." ;
    skos:editorialNote "No occurrences of this slot in the graph." ;
    skos:inScheme okns:frbr ;
    skos:mappingRelation frbr:alternate ;
    linkml:definition_uri okns:frbr_alternate ;
    linkml:domain okns:FrbrManifestation ;
    linkml:inlined true ;
    linkml:owner okns:frbr_alternate ;
    linkml:range okns:FrbrManifestation ;
    linkml:slot_uri frbr:alternate .

okns:frbr_alternateOf a linkml:SlotDefinition ;
    dcterms:source frbr: ;
    dcterms:title "alternate of" ;
    rdfs:subPropertyOf okns:frbr_relatedEndeavour ;
    owl:inverseOf okns:frbr_alternate ;
    skos:definition "A manifestation that is alternated." ;
    skos:editorialNote "No occurrences of this slot in the graph." ;
    skos:inScheme okns:frbr ;
    skos:mappingRelation frbr:alternateOf ;
    linkml:definition_uri okns:frbr_alternateOf ;
    linkml:domain okns:FrbrManifestation ;
    linkml:inlined true ;
    linkml:owner okns:frbr_alternateOf ;
    linkml:range okns:FrbrManifestation ;
    linkml:slot_uri frbr:alternateOf .

okns:frbr_arrangement a linkml:SlotDefinition ;
    dcterms:source frbr: ;
    dcterms:title "arrangement" ;
    rdfs:subPropertyOf okns:frbr_relatedEndeavour ;
    owl:inverseOf okns:frbr_arrangementOf ;
    skos:definition "An arrangement of an expression." ;
    skos:editorialNote "N04eea93a51674a5d89551c9bce5f5271",
        "N79ec4ebb8a6f481f90c16626db4dca8a",
        "Nd9d92d5819104cc79dc66c30184eb10e",
        "No occurrences of this slot in the graph." ;
    skos:inScheme okns:frbr ;
    skos:mappingRelation frbr:arrangement ;
    linkml:definition_uri okns:frbr_arrangement ;
    linkml:domain okns:FrbrExpression ;
    linkml:inlined true ;
    linkml:owner okns:frbr_arrangement ;
    linkml:range okns:FrbrExpression ;
    linkml:slot_uri frbr:arrangement .

okns:frbr_arrangementOf a linkml:SlotDefinition ;
    dcterms:source frbr: ;
    dcterms:title "arrangement of" ;
    rdfs:subPropertyOf okns:frbr_relatedEndeavour ;
    owl:inverseOf okns:frbr_arrangement ;
    skos:definition "An expression that is arranged." ;
    skos:editorialNote "N58f803ac9893451d88563e99735c848c",
        "N63442c6cdfc74b28b529d97e6950b213",
        "Nda5514c3154b488e89acb931e3408378",
        "No occurrences of this slot in the graph." ;
    skos:inScheme okns:frbr ;
    skos:mappingRelation frbr:arrangementOf ;
    linkml:definition_uri okns:frbr_arrangementOf ;
    linkml:domain okns:FrbrExpression ;
    linkml:inlined true ;
    linkml:owner okns:frbr_arrangementOf ;
    linkml:range okns:FrbrExpression ;
    linkml:slot_uri frbr:arrangementOf .

okns:frbr_creator a linkml:SlotDefinition ;
    dcterms:source frbr: ;
    dcterms:title "creator" ;
    rdfs:subPropertyOf okns:frbr_responsibleEntity ;
    owl:inverseOf okns:frbr_creatorOf ;
    skos:definition "An entity in some way responsible for the creation of a work." ;
    skos:editorialNote "N624e2cd580484e779d37e0fbb8576652",
        "Ndaf6654e70474a57bfaeea242d91cc7d",
        "No occurrences of this slot in the graph." ;
    skos:inScheme okns:frbr ;
    skos:mappingRelation frbr:creator ;
    linkml:definition_uri okns:frbr_creator ;
    linkml:domain okns:FrbrWork ;
    linkml:inlined true ;
    linkml:owner okns:frbr_creator ;
    linkml:range okns:FrbrResponsibleEntity ;
    linkml:slot_uri frbr:creator .

okns:frbr_creatorOf a linkml:SlotDefinition ;
    dcterms:source frbr: ;
    dcterms:title "creator of" ;
    rdfs:subPropertyOf okns:frbr_responsibleEntityOf ;
    owl:inverseOf okns:frbr_creator ;
    skos:definition "A work that was in some way created by of an entity." ;
    skos:editorialNote "N7e9edf2b784c4b1fb73616381ec76d1a",
        "Nbe9b10a808684d6a80c9fbccca1bef89",
        "No occurrences of this slot in the graph." ;
    skos:inScheme okns:frbr ;
    skos:mappingRelation frbr:creatorOf ;
    linkml:definition_uri okns:frbr_creatorOf ;
    linkml:domain okns:FrbrResponsibleEntity ;
    linkml:inlined true ;
    linkml:owner okns:frbr_creatorOf ;
    linkml:range okns:FrbrWork ;
    linkml:slot_uri frbr:creatorOf .

okns:frbr_embodimentOf a linkml:SlotDefinition ;
    dcterms:source frbr: ;
    dcterms:title "embodiment of" ;
    rdfs:subPropertyOf okns:frbr_relatedEndeavour ;
    owl:inverseOf okns:frbr_embodiment ;
    skos:definition "An expression that is embodied by a manifestation." ;
    skos:editorialNote "N7703209c64c443548cfe0b2b35a83604",
        "Nefee085fa0ff45648834b29e38dcf322",
        "No occurrences of this slot in the graph." ;
    skos:inScheme okns:frbr ;
    skos:mappingRelation frbr:embodimentOf ;
    linkml:definition_uri okns:frbr_embodimentOf ;
    linkml:domain okns:FrbrManifestation ;
    linkml:inlined true ;
    linkml:owner okns:frbr_embodimentOf ;
    linkml:range okns:FrbrExpression ;
    linkml:slot_uri frbr:embodimentOf .

okns:frbr_exemplarOf a linkml:SlotDefinition ;
    dcterms:source frbr: ;
    dcterms:title "exemplar of" ;
    rdfs:subPropertyOf okns:frbr_relatedEndeavour ;
    owl:inverseOf okns:frbr_exemplar ;
    skos:definition "The manifestation that is exemplified by a item." ;
    skos:editorialNote "N13c2217aa96743c6a63dea80eb4d6ba9",
        "Nf821047dcf594e86a7464933e8472db1",
        "No occurrences of this slot in the graph." ;
    skos:inScheme okns:frbr ;
    skos:mappingRelation frbr:exemplarOf ;
    linkml:definition_uri okns:frbr_exemplarOf ;
    linkml:domain okns:FrbrItem ;
    linkml:inlined true ;
    linkml:owner okns:frbr_exemplarOf ;
    linkml:range okns:FrbrManifestation ;
    linkml:slot_uri frbr:exemplarOf .

okns:frbr_owner a linkml:SlotDefinition ;
    dcterms:source frbr: ;
    dcterms:title "owner" ;
    rdfs:subPropertyOf okns:frbr_responsibleEntity ;
    owl:inverseOf okns:frbr_ownerOf ;
    skos:definition "An entity that owns an item." ;
    skos:editorialNote "N2adb586b387442a1a1452d3de443d3fb",
        "N67b26f2782bc4a5c9cecedb66605fa9e",
        "No occurrences of this slot in the graph." ;
    skos:inScheme okns:frbr ;
    skos:mappingRelation frbr:owner ;
    linkml:definition_uri okns:frbr_owner ;
    linkml:domain okns:FrbrItem ;
    linkml:inlined true ;
    linkml:owner okns:frbr_owner ;
    linkml:range okns:FrbrResponsibleEntity ;
    linkml:slot_uri frbr:owner .

okns:frbr_ownerOf a linkml:SlotDefinition ;
    dcterms:source frbr: ;
    dcterms:title "owner of" ;
    rdfs:subPropertyOf okns:frbr_responsibleEntityOf ;
    owl:inverseOf okns:frbr_owner ;
    skos:definition "An item that is in some way owned an entity." ;
    skos:editorialNote "N0ce2b4c9f3194c29bd86af95b2e97805",
        "N8ed1a33ea09b4e3a8d4dc62a24f16ba1",
        "No occurrences of this slot in the graph." ;
    skos:inScheme okns:frbr ;
    skos:mappingRelation frbr:ownerOf ;
    linkml:definition_uri okns:frbr_ownerOf ;
    linkml:domain okns:FrbrResponsibleEntity ;
    linkml:inlined true ;
    linkml:owner okns:frbr_ownerOf ;
    linkml:range okns:FrbrItem ;
    linkml:slot_uri frbr:ownerOf .

okns:frbr_producer a linkml:SlotDefinition ;
    dcterms:source frbr: ;
    dcterms:title "producer" ;
    rdfs:subPropertyOf okns:frbr_responsibleEntity ;
    owl:inverseOf okns:frbr_producerOf ;
    skos:definition "An entity in some way responsible for producing a manifestation." ;
    skos:editorialNote "N09c1942d42504c92be517d01f682a6ed",
        "Nbb3138354a9947cbb92bb80b7e207698",
        "No occurrences of this slot in the graph." ;
    skos:inScheme okns:frbr ;
    skos:mappingRelation frbr:producer ;
    linkml:definition_uri okns:frbr_producer ;
    linkml:domain okns:FrbrManifestation ;
    linkml:inlined true ;
    linkml:owner okns:frbr_producer ;
    linkml:range okns:FrbrResponsibleEntity ;
    linkml:slot_uri frbr:producer .

okns:frbr_producerOf a linkml:SlotDefinition ;
    dcterms:source frbr: ;
    dcterms:title "producer of" ;
    rdfs:subPropertyOf okns:frbr_responsibleEntityOf ;
    owl:inverseOf okns:frbr_producer ;
    skos:definition "A manifestation that was in some way produced an entity." ;
    skos:editorialNote "N1c3846fb8dae4bc6b3b2a499cf78e0dc",
        "Ne418147c07b649589d8ac08f1f733bcc",
        "No occurrences of this slot in the graph." ;
    skos:inScheme okns:frbr ;
    skos:mappingRelation frbr:producerOf ;
    linkml:definition_uri okns:frbr_producerOf ;
    linkml:domain okns:FrbrResponsibleEntity ;
    linkml:inlined true ;
    linkml:owner okns:frbr_producerOf ;
    linkml:range okns:FrbrManifestation ;
    linkml:slot_uri frbr:producerOf .

okns:frbr_realization a linkml:SlotDefinition ;
    dcterms:source frbr: ;
    dcterms:title "realization" ;
    rdfs:subPropertyOf okns:frbr_relatedEndeavour ;
    owl:inverseOf okns:frbr_realizationOf ;
    skos:definition "An expression that is an intellectual or artistic realization of a work." ;
    skos:editorialNote "N5c62a4f58b63498ba3c322206e0d1109",
        "N64f0edca05c043858980ef4d9a97e5e8",
        "No occurrences of this slot in the graph." ;
    skos:inScheme okns:frbr ;
    skos:mappingRelation frbr:realization ;
    linkml:definition_uri okns:frbr_realization ;
    linkml:domain okns:FrbrWork ;
    linkml:inlined true ;
    linkml:owner okns:frbr_realization ;
    linkml:range okns:FrbrExpression ;
    linkml:slot_uri frbr:realization .

okns:frbr_realizationOf a linkml:SlotDefinition ;
    dcterms:source frbr: ;
    dcterms:title "realization of" ;
    rdfs:subPropertyOf okns:frbr_relatedEndeavour ;
    owl:inverseOf okns:frbr_realization ;
    skos:definition "The work that has been realized by an expression." ;
    skos:editorialNote "Nc9581f7fe6ce441495bfc1faed879cb8",
        "Ne90922840f2a4814ae079a3460bbd457",
        "No occurrences of this slot in the graph." ;
    skos:inScheme okns:frbr ;
    skos:mappingRelation frbr:realizationOf ;
    linkml:definition_uri okns:frbr_realizationOf ;
    linkml:domain okns:FrbrExpression ;
    linkml:inlined true ;
    linkml:owner okns:frbr_realizationOf ;
    linkml:range okns:FrbrWork ;
    linkml:slot_uri frbr:realizationOf .

okns:frbr_realizer a linkml:SlotDefinition ;
    dcterms:source frbr: ;
    dcterms:title "realizer" ;
    rdfs:subPropertyOf okns:frbr_responsibleEntity ;
    owl:inverseOf okns:frbr_realizerOf ;
    skos:definition "An entity in some way responsible for realizing an expression." ;
    skos:editorialNote "N25977bf53f1a46b1a8fa0b25a0a4d387",
        "N81e543c93181451cb459ac8243386e19",
        "No occurrences of this slot in the graph." ;
    skos:inScheme okns:frbr ;
    skos:mappingRelation frbr:realizer ;
    linkml:definition_uri okns:frbr_realizer ;
    linkml:domain okns:FrbrExpression ;
    linkml:inlined true ;
    linkml:owner okns:frbr_realizer ;
    linkml:range okns:FrbrResponsibleEntity ;
    linkml:slot_uri frbr:realizer .

okns:frbr_realizerOf a linkml:SlotDefinition ;
    dcterms:source frbr: ;
    dcterms:title "realizer of" ;
    rdfs:subPropertyOf okns:frbr_responsibleEntityOf ;
    owl:inverseOf okns:frbr_realizer ;
    skos:definition "An expression that was in some way realized by an entity." ;
    skos:editorialNote "N9d1c53fdbba04ef9bad2aba7e81a103f",
        "Nd861ec19934349f3b628990def34a6b7",
        "No occurrences of this slot in the graph." ;
    skos:inScheme okns:frbr ;
    skos:mappingRelation frbr:realizerOf ;
    linkml:definition_uri okns:frbr_realizerOf ;
    linkml:domain okns:FrbrResponsibleEntity ;
    linkml:inlined true ;
    linkml:owner okns:frbr_realizerOf ;
    linkml:range okns:FrbrExpression ;
    linkml:slot_uri frbr:realizerOf .

okns:frbr_reconfiguration a linkml:SlotDefinition ;
    dcterms:source frbr: ;
    dcterms:title "reconfiguration" ;
    rdfs:subPropertyOf okns:frbr_relatedEndeavour ;
    owl:inverseOf okns:frbr_reconfigurationOf ;
    skos:definition "A recongifuration of an item." ;
    skos:editorialNote "No occurrences of this slot in the graph." ;
    skos:inScheme okns:frbr ;
    skos:mappingRelation frbr:reconfiguration ;
    linkml:definition_uri okns:frbr_reconfiguration ;
    linkml:domain okns:FrbrItem ;
    linkml:inlined true ;
    linkml:owner okns:frbr_reconfiguration ;
    linkml:range okns:FrbrItem ;
    linkml:slot_uri frbr:reconfiguration .

okns:frbr_reconfigurationOf a linkml:SlotDefinition ;
    dcterms:source frbr: ;
    dcterms:title "reconfiguration of" ;
    rdfs:subPropertyOf okns:frbr_relatedEndeavour ;
    owl:inverseOf okns:frbr_reconfiguration ;
    skos:definition "An item that is reconfigured." ;
    skos:editorialNote "No occurrences of this slot in the graph." ;
    skos:inScheme okns:frbr ;
    skos:mappingRelation frbr:reconfigurationOf ;
    linkml:definition_uri okns:frbr_reconfigurationOf ;
    linkml:domain okns:FrbrItem ;
    linkml:inlined true ;
    linkml:owner okns:frbr_reconfigurationOf ;
    linkml:range okns:FrbrItem ;
    linkml:slot_uri frbr:reconfigurationOf .

okns:frbr_revision a linkml:SlotDefinition ;
    dcterms:source frbr: ;
    dcterms:title "revision" ;
    rdfs:subPropertyOf okns:frbr_relatedEndeavour ;
    owl:inverseOf okns:frbr_revisionOf ;
    skos:definition "A revision of an expression." ;
    skos:editorialNote "N56326931a116444d89263d5a466edcc6",
        "N5e24eca6157c48a3bb3872cb12c30537",
        "Nf1860089f8054b2c8f26dba23f2ae1af",
        "No occurrences of this slot in the graph." ;
    skos:inScheme okns:frbr ;
    skos:mappingRelation frbr:revision ;
    linkml:definition_uri okns:frbr_revision ;
    linkml:domain okns:FrbrExpression ;
    linkml:inlined true ;
    linkml:owner okns:frbr_revision ;
    linkml:range okns:FrbrExpression ;
    linkml:slot_uri frbr:revision .

okns:frbr_revisionOf a linkml:SlotDefinition ;
    dcterms:source frbr: ;
    dcterms:title "revision of" ;
    rdfs:subPropertyOf okns:frbr_relatedEndeavour ;
    owl:inverseOf okns:frbr_revision ;
    skos:definition "An expression that is revised." ;
    skos:editorialNote "N4917721ec671477f91fa80da716216f2",
        "N85bfe5c8ea9843d48811433c04987d20",
        "N934f199deb924d27b6656663c3397b27",
        "No occurrences of this slot in the graph." ;
    skos:inScheme okns:frbr ;
    skos:mappingRelation frbr:revisionOf ;
    linkml:definition_uri okns:frbr_revisionOf ;
    linkml:domain okns:FrbrExpression ;
    linkml:inlined true ;
    linkml:owner okns:frbr_revisionOf ;
    linkml:range okns:FrbrExpression ;
    linkml:slot_uri frbr:revisionOf .

okns:frbr_translation a linkml:SlotDefinition ;
    dcterms:source frbr: ;
    dcterms:title "translation" ;
    rdfs:subPropertyOf okns:frbr_relatedEndeavour ;
    owl:inverseOf okns:frbr_translationOf ;
    skos:definition "A translation of an expression." ;
    skos:editorialNote "N813c423bb86c433384a649c8927d0a8f",
        "Nc787de18329044c58347d68028cc6666",
        "Nde612754755547d78cd578318ffbad8a",
        "No occurrences of this slot in the graph." ;
    skos:inScheme okns:frbr ;
    skos:mappingRelation frbr:translation ;
    linkml:definition_uri okns:frbr_translation ;
    linkml:domain okns:FrbrExpression ;
    linkml:inlined true ;
    linkml:owner okns:frbr_translation ;
    linkml:range okns:FrbrExpression ;
    linkml:slot_uri frbr:translation .

okns:frbr_translationOf a linkml:SlotDefinition ;
    dcterms:source frbr: ;
    dcterms:title "translation of" ;
    rdfs:subPropertyOf okns:frbr_relatedEndeavour ;
    owl:inverseOf okns:frbr_translation ;
    skos:definition "An expression that is translated." ;
    skos:editorialNote "N5718bd90898b489285a4b9f2addcf13e",
        "N73a5120b039f40a9be70584431acfbbc",
        "Nfb13e668960c49cfa63d6d32a4c60113",
        "No occurrences of this slot in the graph." ;
    skos:inScheme okns:frbr ;
    skos:mappingRelation frbr:translationOf ;
    linkml:definition_uri okns:frbr_translationOf ;
    linkml:domain okns:FrbrExpression ;
    linkml:inlined true ;
    linkml:owner okns:frbr_translationOf ;
    linkml:range okns:FrbrExpression ;
    linkml:slot_uri frbr:translationOf .

okns:mo_arranged_in a linkml:SlotDefinition ;
    dcterms:source <http://purl.org/ontology/mo/> ;
    dcterms:title "arranged in" ;
    rdfs:subPropertyOf okns:event_isFactorOf ;
    owl:inverseOf okns:mo_arrangement_of ;
    skos:definition "Associates a work to an arrangement event where it was arranged" ;
    skos:editorialNote "No occurrences of this slot in the graph." ;
    skos:inScheme okns:mo ;
    skos:mappingRelation <http://purl.org/ontology/mo/arranged_in> ;
    linkml:definition_uri okns:mo_arranged_in ;
    linkml:domain okns:MoMusicalWork ;
    linkml:inlined true ;
    linkml:owner okns:mo_arranged_in ;
    linkml:range okns:MoArrangement ;
    linkml:slot_uri <http://purl.org/ontology/mo/arranged_in> .

okns:mo_arrangement_of a linkml:SlotDefinition ;
    dcterms:source <http://purl.org/ontology/mo/> ;
    dcterms:title "arrangement of" ;
    rdfs:subPropertyOf okns:event_factor ;
    owl:inverseOf okns:mo_arranged_in ;
    skos:definition "Associates an arrangement event to a work" ;
    skos:editorialNote "No occurrences of this slot in the graph." ;
    skos:inScheme okns:mo ;
    skos:mappingRelation <http://purl.org/ontology/mo/arrangement_of> ;
    linkml:definition_uri okns:mo_arrangement_of ;
    linkml:domain okns:MoArrangement ;
    linkml:inlined true ;
    linkml:owner okns:mo_arrangement_of ;
    linkml:range okns:MoMusicalWork ;
    linkml:slot_uri <http://purl.org/ontology/mo/arrangement_of> .

okns:mo_compiled a linkml:SlotDefinition ;
    dcterms:source <http://purl.org/ontology/mo/> ;
    dcterms:title "compiled" ;
    owl:inverseOf okns:mo_compiler ;
    skos:definition "Used to relate an person or a group of person who compiled the manifestation of a musical work." ;
    skos:editorialNote "No occurrences of this slot in the graph." ;
    skos:inScheme okns:mo ;
    skos:mappingRelation <http://purl.org/ontology/mo/compiled> ;
    linkml:definition_uri okns:mo_compiled ;
    linkml:domain okns:MoMusicArtist ;
    linkml:inlined true ;
    linkml:owner okns:mo_compiled ;
    linkml:range okns:MoMusicalManifestation ;
    linkml:slot_uri <http://purl.org/ontology/mo/compiled> .

okns:mo_compiler a linkml:SlotDefinition ;
    dcterms:source <http://purl.org/ontology/mo/> ;
    dcterms:title "compiler" ;
    owl:inverseOf okns:mo_compiled ;
    skos:definition "Used to relate the manifestation of a musical work to a person or a group of person who compiled it." ;
    skos:editorialNote "No occurrences of this slot in the graph." ;
    skos:inScheme okns:mo ;
    skos:mappingRelation <http://purl.org/ontology/mo/compiler> ;
    linkml:definition_uri okns:mo_compiler ;
    linkml:domain okns:MoMusicalManifestation ;
    linkml:inlined true ;
    linkml:owner okns:mo_compiler ;
    linkml:range okns:MoMusicArtist ;
    linkml:slot_uri <http://purl.org/ontology/mo/compiler> .

okns:mo_composed_in a linkml:SlotDefinition ;
    dcterms:source <http://purl.org/ontology/mo/> ;
    dcterms:title "composed in" ;
    rdfs:subPropertyOf okns:event_producedIn ;
    owl:inverseOf okns:mo_produced_work ;
    skos:definition "Associates a MusicalWork to the Composition event pertaining␊        to its creation. For example, I might use this property to associate␊        the Magic Flute to its composition event, occuring during 1782 and having as␊        a mo:composer Mozart." ;
    skos:editorialNote "No occurrences of this slot in the graph." ;
    skos:inScheme okns:mo ;
    skos:mappingRelation <http://purl.org/ontology/mo/composed_in> ;
    linkml:definition_uri okns:mo_composed_in ;
    linkml:domain okns:MoMusicalWork ;
    linkml:inlined true ;
    linkml:owner okns:mo_composed_in ;
    linkml:range okns:MoComposition ;
    linkml:slot_uri <http://purl.org/ontology/mo/composed_in> .

okns:mo_conducted a linkml:SlotDefinition ;
    dcterms:source <http://purl.org/ontology/mo/> ;
    dcterms:title "conducted" ;
    rdfs:subPropertyOf okns:event_isAgentIn ;
    owl:inverseOf okns:mo_conductor ;
    skos:definition "Relates agents to the performances they were conducting" ;
    skos:editorialNote "No occurrences of this slot in the graph." ;
    skos:inScheme okns:mo ;
    skos:mappingRelation <http://purl.org/ontology/mo/conducted> ;
    linkml:definition_uri okns:mo_conducted ;
    linkml:domain okns:FoafAgent ;
    linkml:inlined true ;
    linkml:owner okns:mo_conducted ;
    linkml:range okns:MoPerformance ;
    linkml:slot_uri <http://purl.org/ontology/mo/conducted> .

okns:mo_conductor a linkml:SlotDefinition ;
    dcterms:source <http://purl.org/ontology/mo/> ;
    rdfs:subPropertyOf okns:event_agent ;
    owl:inverseOf okns:mo_conducted ;
    skos:definition "Relates a performance to the conductor involved" ;
    skos:editorialNote "No occurrences of this slot in the graph." ;
    skos:inScheme okns:mo ;
    skos:mappingRelation <http://purl.org/ontology/mo/conductor> ;
    linkml:definition_uri okns:mo_conductor ;
    linkml:domain okns:MoPerformance ;
    linkml:inlined true ;
    linkml:owner okns:mo_conductor ;
    linkml:range okns:FoafAgent ;
    linkml:slot_uri <http://purl.org/ontology/mo/conductor> .

okns:mo_djmixed a linkml:SlotDefinition ;
    dcterms:source <http://purl.org/ontology/mo/> ;
    dcterms:title "djmixed" ;
    owl:inverseOf okns:mo_djmixed_by ;
    skos:definition "Used to relate an artist who djmixed a musical work or the expression of a musical work. ␊    ␊The artist usually selected the tracks, chose their sequence, and slightly changed them by fading (so that one track blends in smoothly with the other) or pitching (so that the tempo of one track matches the tempo of the following track). This applies to a 'Mixtape' in which all tracks were DJ-mixed together into one single long track." ;
    skos:editorialNote "No occurrences of this slot in the graph." ;
    skos:inScheme okns:mo ;
    skos:mappingRelation <http://purl.org/ontology/mo/djmixed> ;
    linkml:definition_uri okns:mo_djmixed ;
    linkml:domain okns:MoMusicArtist ;
    linkml:inlined true ;
    linkml:owner okns:mo_djmixed ;
    linkml:range okns:MoSignal ;
    linkml:slot_uri <http://purl.org/ontology/mo/djmixed> .

okns:mo_djmixed_by a linkml:SlotDefinition ;
    dcterms:source <http://purl.org/ontology/mo/> ;
    dcterms:title "djmixed_by" ;
    owl:inverseOf okns:mo_djmixed ;
    skos:definition "Used to relate a work or the expression of a work to an artist who djmixed it. ␊    ␊The artist usually selected the tracks, chose their sequence, and slightly changed them by fading (so that one track blends in smoothly with the other) or pitching (so that the tempo of one track matches the tempo of the following track). This applies to a 'Mixtape' in which all tracks were DJ-mixed together into one single long track." ;
    skos:editorialNote "No occurrences of this slot in the graph." ;
    skos:inScheme okns:mo ;
    skos:mappingRelation <http://purl.org/ontology/mo/djmixed_by> ;
    linkml:definition_uri okns:mo_djmixed_by ;
    linkml:domain okns:MoSignal ;
    linkml:inlined true ;
    linkml:owner okns:mo_djmixed_by ;
    linkml:range okns:MoMusicArtist ;
    linkml:slot_uri <http://purl.org/ontology/mo/djmixed_by> .

okns:mo_engineered a linkml:SlotDefinition ;
    dcterms:source <http://purl.org/ontology/mo/> ;
    dcterms:title "engineered" ;
    rdfs:subPropertyOf okns:event_isAgentIn ;
    owl:inverseOf okns:mo_engineer ;
    skos:definition "Relates agents to the performances/recordings they were engineering in" ;
    skos:editorialNote "No occurrences of this slot in the graph." ;
    skos:inScheme okns:mo ;
    skos:mappingRelation <http://purl.org/ontology/mo/engineered> ;
    linkml:definition_uri okns:mo_engineered ;
    linkml:domain okns:FoafAgent ;
    linkml:inlined true ;
    linkml:owner okns:mo_engineered ;
    linkml:range okns:Any ;
    linkml:slot_uri <http://purl.org/ontology/mo/engineered> .

okns:mo_level a linkml:SlotDefinition ;
    dcterms:source <http://purl.org/ontology/mo/> ;
    dcterms:title "level" ;
    skos:definition "This annotation property associates to a particular Music Ontology term the corresponding␊        expressiveness level. These levels can be:␊␊            - 1: Only editorial/Musicbrainz type information␊            - 2: Workflow information␊            - 3: Even decomposition␊        ␊        This property is mainly used for specification generation." ;
    skos:inScheme okns:mo ;
    skos:mappingRelation <http://purl.org/ontology/mo/level> ;
    linkml:definition_uri okns:mo_level ;
    linkml:domain_of okns:MoReleaseStatus,
        okns:MoReleaseType ;
    linkml:owner okns:MoReleaseType ;
    linkml:range okns:string ;
    linkml:slot_uri <http://purl.org/ontology/mo/level> .

okns:mo_listened a linkml:SlotDefinition ;
    dcterms:source <http://purl.org/ontology/mo/> ;
    dcterms:title "listened" ;
    rdfs:subPropertyOf okns:event_isAgentIn ;
    owl:inverseOf okns:mo_listener ;
    skos:definition "Relates agents to the performances they were listening in" ;
    skos:editorialNote "No occurrences of this slot in the graph." ;
    skos:inScheme okns:mo ;
    skos:mappingRelation <http://purl.org/ontology/mo/listened> ;
    linkml:definition_uri okns:mo_listened ;
    linkml:domain okns:FoafAgent ;
    linkml:inlined true ;
    linkml:owner okns:mo_listened ;
    linkml:range okns:MoPerformance ;
    linkml:slot_uri <http://purl.org/ontology/mo/listened> .

okns:mo_listener a linkml:SlotDefinition ;
    dcterms:source <http://purl.org/ontology/mo/> ;
    rdfs:subPropertyOf okns:event_agent ;
    owl:inverseOf okns:mo_listened ;
    skos:definition "Relates a performance to the listener involved" ;
    skos:editorialNote "No occurrences of this slot in the graph." ;
    skos:inScheme okns:mo ;
    skos:mappingRelation <http://purl.org/ontology/mo/listener> ;
    linkml:definition_uri okns:mo_listener ;
    linkml:domain okns:MoPerformance ;
    linkml:inlined true ;
    linkml:owner okns:mo_listener ;
    linkml:range okns:FoafAgent ;
    linkml:slot_uri <http://purl.org/ontology/mo/listener> .

okns:mo_member_of a linkml:SlotDefinition ;
    dcterms:source <http://purl.org/ontology/mo/> ;
    dcterms:title "member_of" ;
    owl:inverseOf okns:foaf_member ;
    skos:definition "Inverse of the foaf:member property" ;
    skos:editorialNote "No occurrences of this slot in the graph." ;
    skos:inScheme okns:mo ;
    skos:mappingRelation <http://purl.org/ontology/mo/member_of> ;
    linkml:definition_uri okns:mo_member_of ;
    linkml:domain okns:FoafAgent ;
    linkml:inlined true ;
    linkml:owner okns:mo_member_of ;
    linkml:range okns:FoafGroup ;
    linkml:slot_uri <http://purl.org/ontology/mo/member_of> .

okns:mo_performance_of a linkml:SlotDefinition ;
    dcterms:source <http://purl.org/ontology/mo/> ;
    dcterms:title "performance of" ;
    rdfs:subPropertyOf okns:event_factor ;
    owl:inverseOf okns:mo_performed_in ;
    skos:definition "Associates a Performance to a musical work or an arrangement that is being used as a factor in it.␊        For example, I might use this property to attach the Magic Flute musical work to ␊        a particular Performance." ;
    skos:editorialNote "No occurrences of this slot in the graph." ;
    skos:inScheme okns:mo ;
    skos:mappingRelation <http://purl.org/ontology/mo/performance_of> ;
    linkml:definition_uri okns:mo_performance_of ;
    linkml:domain okns:MoPerformance ;
    linkml:inlined true ;
    linkml:owner okns:mo_performance_of ;
    linkml:range okns:Any ;
    linkml:slot_uri <http://purl.org/ontology/mo/performance_of> .

okns:mo_performed a linkml:SlotDefinition ;
    dcterms:source <http://purl.org/ontology/mo/> ;
    dcterms:title "performed" ;
    rdfs:subPropertyOf okns:event_isAgentIn ;
    owl:inverseOf okns:mo_performer ;
    skos:definition "Relates agents to the performances they were performing in" ;
    skos:editorialNote "No occurrences of this slot in the graph." ;
    skos:inScheme okns:mo ;
    skos:mappingRelation <http://purl.org/ontology/mo/performed> ;
    linkml:definition_uri okns:mo_performed ;
    linkml:domain okns:FoafAgent ;
    linkml:inlined true ;
    linkml:owner okns:mo_performed ;
    linkml:range okns:MoPerformance ;
    linkml:slot_uri <http://purl.org/ontology/mo/performed> .

okns:mo_produced a linkml:SlotDefinition ;
    dcterms:source <http://purl.org/ontology/mo/> ;
    dcterms:title "produced" ;
    owl:inverseOf okns:mo_producer ;
    skos:definition "Used to relate an person or a group of person who produced the manifestation of a work." ;
    skos:editorialNote "No occurrences of this slot in the graph." ;
    skos:inScheme okns:mo ;
    skos:mappingRelation <http://purl.org/ontology/mo/produced> ;
    linkml:definition_uri okns:mo_produced ;
    linkml:domain okns:FoafAgent ;
    linkml:inlined true ;
    linkml:owner okns:mo_produced ;
    linkml:range okns:MoMusicalManifestation ;
    linkml:slot_uri <http://purl.org/ontology/mo/produced> .

okns:mo_produced_work a linkml:SlotDefinition ;
    dcterms:source <http://purl.org/ontology/mo/> ;
    dcterms:title "produced work" ;
    rdfs:subPropertyOf okns:event_product ;
    owl:inverseOf okns:mo_composed_in ;
    skos:definition "Associates a composition event to the produced MusicalWork. For example,␊                this property could link the event corresponding to the composition of the␊                Magic Flute in 1782 to the Magic Flute musical work itself. This musical work␊                can then be used in particular performances." ;
    skos:editorialNote "No occurrences of this slot in the graph." ;
    skos:inScheme okns:mo ;
    skos:mappingRelation <http://purl.org/ontology/mo/produced_work> ;
    linkml:definition_uri okns:mo_produced_work ;
    linkml:domain okns:MoComposition ;
    linkml:inlined true ;
    linkml:owner okns:mo_produced_work ;
    linkml:range okns:MoMusicalWork ;
    linkml:slot_uri <http://purl.org/ontology/mo/produced_work> .

okns:mo_producer a linkml:SlotDefinition ;
    dcterms:source <http://purl.org/ontology/mo/> ;
    dcterms:title "producer" ;
    owl:inverseOf okns:mo_produced ;
    skos:definition "Used to relate the manifestation of a work to a person or a group of person who produced it." ;
    skos:editorialNote "No occurrences of this slot in the graph." ;
    skos:inScheme okns:mo ;
    skos:mappingRelation <http://purl.org/ontology/mo/producer> ;
    linkml:definition_uri okns:mo_producer ;
    linkml:domain okns:MoMusicalManifestation ;
    linkml:inlined true ;
    linkml:owner okns:mo_producer ;
    linkml:range okns:FoafAgent ;
    linkml:slot_uri <http://purl.org/ontology/mo/producer> .

okns:mo_publication_of a linkml:SlotDefinition ;
    dcterms:source <http://purl.org/ontology/mo/> ;
    dcterms:title "publication of" ;
    owl:inverseOf okns:mo_published_as ;
    skos:definition "Link a particular manifestation to the related signal, score, libretto, or lyrics" ;
    skos:editorialNote "No occurrences of this slot in the graph." ;
    skos:inScheme okns:mo ;
    skos:mappingRelation <http://purl.org/ontology/mo/publication_of> ;
    linkml:definition_uri okns:mo_publication_of ;
    linkml:domain okns:MoMusicalManifestation ;
    linkml:inlined true ;
    linkml:owner okns:mo_publication_of ;
    linkml:range okns:MoMusicalExpression ;
    linkml:slot_uri <http://purl.org/ontology/mo/publication_of> .

okns:mo_published a linkml:SlotDefinition ;
    dcterms:source <http://purl.org/ontology/mo/> ;
    dcterms:title "published" ;
    owl:inverseOf okns:mo_publisher ;
    skos:definition "Used to relate an person or a group of person who published the manifestation of a work." ;
    skos:editorialNote "No occurrences of this slot in the graph." ;
    skos:inScheme okns:mo ;
    skos:mappingRelation <http://purl.org/ontology/mo/published> ;
    linkml:definition_uri okns:mo_published ;
    linkml:domain okns:FoafAgent ;
    linkml:inlined true ;
    linkml:owner okns:mo_published ;
    linkml:range okns:MoMusicalManifestation ;
    linkml:slot_uri <http://purl.org/ontology/mo/published> .

okns:mo_published_as a linkml:SlotDefinition ;
    dcterms:source <http://purl.org/ontology/mo/> ;
    dcterms:title "published as" ;
    rdfs:subPropertyOf okns:frbr_embodiment ;
    owl:inverseOf okns:mo_publication_of ;
    skos:definition "Links a musical expression (e.g. a signal or a score) to one of its manifestations (e.g. a track on a particular record or a published score)." ;
    skos:editorialNote "No occurrences of this slot in the graph." ;
    skos:inScheme okns:mo ;
    skos:mappingRelation <http://purl.org/ontology/mo/published_as> ;
    linkml:definition_uri okns:mo_published_as ;
    linkml:domain okns:MoMusicalExpression ;
    linkml:inlined true ;
    linkml:owner okns:mo_published_as ;
    linkml:range okns:MoMusicalManifestation ;
    linkml:slot_uri <http://purl.org/ontology/mo/published_as> .

okns:mo_publisher a linkml:SlotDefinition ;
    dcterms:source <http://purl.org/ontology/mo/> ;
    dcterms:title "publisher" ;
    owl:inverseOf okns:mo_published ;
    skos:definition "Used to relate a musical manifestation to a person or a group of person who published it." ;
    skos:editorialNote "No occurrences of this slot in the graph." ;
    skos:inScheme okns:mo ;
    skos:mappingRelation <http://purl.org/ontology/mo/publisher> ;
    linkml:definition_uri okns:mo_publisher ;
    linkml:domain okns:MoMusicalManifestation ;
    linkml:inlined true ;
    linkml:owner okns:mo_publisher ;
    linkml:range okns:FoafAgent ;
    linkml:slot_uri <http://purl.org/ontology/mo/publisher> .

okns:mo_recorded_as a linkml:SlotDefinition ;
    dcterms:source <http://purl.org/ontology/mo/> ;
    dcterms:title "recorded as" ;
    owl:inverseOf okns:mo_records ;
    skos:definition "This is a shortcut property, allowing to bypass all the Sound/Recording steps. This property␊        allows to directly link a Performance to the recorded Signal. This is recommended for \"normal\"␊        users. However, advanced users wanting to express things such as the location of the microphone will␊        have to create this shortcut as well as the whole workflow, in order to let the \"normal\" users access␊        simply the, well, simple information:-) ." ;
    skos:editorialNote "No occurrences of this slot in the graph." ;
    skos:inScheme okns:mo ;
    skos:mappingRelation <http://purl.org/ontology/mo/recorded_as> ;
    linkml:definition_uri okns:mo_recorded_as ;
    linkml:domain okns:MoPerformance ;
    linkml:inlined true ;
    linkml:owner okns:mo_recorded_as ;
    linkml:range okns:MoSignal ;
    linkml:slot_uri <http://purl.org/ontology/mo/recorded_as> .

okns:mo_recorded_in a linkml:SlotDefinition ;
    dcterms:source <http://purl.org/ontology/mo/> ;
    dcterms:title "recorded in" ;
    rdfs:subPropertyOf okns:event_isFactorOf ;
    owl:inverseOf okns:mo_recording_of ;
    skos:definition "Associates a physical Sound to a Recording event where it is being used ␊        in order to produce a signal. For example, I might use this property to ␊        associate the sound produced by a particular performance of the magic flute␊        to a given recording, done using my cell-phone." ;
    skos:editorialNote "No occurrences of this slot in the graph." ;
    skos:inScheme okns:mo ;
    skos:mappingRelation <http://purl.org/ontology/mo/recorded_in> ;
    linkml:definition_uri okns:mo_recorded_in ;
    linkml:domain okns:MoSound ;
    linkml:inlined true ;
    linkml:owner okns:mo_recorded_in ;
    linkml:range okns:MoRecording ;
    linkml:slot_uri <http://purl.org/ontology/mo/recorded_in> .

okns:mo_recording_of a linkml:SlotDefinition ;
    dcterms:source <http://purl.org/ontology/mo/> ;
    dcterms:title "recorded sound" ;
    rdfs:subPropertyOf okns:event_factor ;
    owl:inverseOf okns:mo_recorded_in ;
    skos:definition "Associates a Recording event to a physical Sound being recorded.␊                For example, I might use this property to␊                associate a given recording, done using my cell phone, to the ␊        sound produced by a particular performance of the magic flute." ;
    skos:editorialNote "No occurrences of this slot in the graph." ;
    skos:inScheme okns:mo ;
    skos:mappingRelation <http://purl.org/ontology/mo/recording_of> ;
    linkml:definition_uri okns:mo_recording_of ;
    linkml:domain okns:MoRecording ;
    linkml:inlined true ;
    linkml:owner okns:mo_recording_of ;
    linkml:range okns:MoSound ;
    linkml:slot_uri <http://purl.org/ontology/mo/recording_of> .

okns:mo_records a linkml:SlotDefinition ;
    dcterms:source <http://purl.org/ontology/mo/> ;
    dcterms:title "records" ;
    owl:inverseOf okns:mo_recorded_as ;
    skos:definition "This is the inverse of the shortcut property recordedAs, allowing to relate directly a performance␊        to a signal." ;
    skos:editorialNote "No occurrences of this slot in the graph." ;
    skos:inScheme okns:mo ;
    skos:mappingRelation <http://purl.org/ontology/mo/records> ;
    linkml:definition_uri okns:mo_records ;
    linkml:domain okns:MoSignal ;
    linkml:inlined true ;
    linkml:owner okns:mo_records ;
    linkml:range okns:MoPerformance ;
    linkml:slot_uri <http://purl.org/ontology/mo/records> .

okns:mo_remixed a linkml:SlotDefinition ;
    dcterms:source <http://purl.org/ontology/mo/> ;
    dcterms:title "remixed" ;
    owl:inverseOf okns:mo_remixer ;
    skos:definition "Used to relate an artist who remixed a musical work or the expression of a musical work. ␊    ␊This involves taking just one other musical work and using audio editing to make it sound like a significantly different, but usually still recognisable, song. It can be used to link an artist to a single song that they remixed, or, if they remixed an entire musical work." ;
    skos:editorialNote "No occurrences of this slot in the graph." ;
    skos:inScheme okns:mo ;
    skos:mappingRelation <http://purl.org/ontology/mo/remixed> ;
    linkml:definition_uri okns:mo_remixed ;
    linkml:domain okns:MoMusicArtist ;
    linkml:inlined true ;
    linkml:owner okns:mo_remixed ;
    linkml:range okns:MoSignal ;
    linkml:slot_uri <http://purl.org/ontology/mo/remixed> .

okns:mo_sampled a linkml:SlotDefinition ;
    dcterms:source <http://purl.org/ontology/mo/> ;
    dcterms:title "sampled" ;
    owl:inverseOf okns:mo_sampler ;
    skos:definition "Used to relate an artist who sampled a Signal." ;
    skos:editorialNote "No occurrences of this slot in the graph." ;
    skos:inScheme okns:mo ;
    skos:mappingRelation <http://purl.org/ontology/mo/sampled> ;
    linkml:definition_uri okns:mo_sampled ;
    linkml:domain okns:MoMusicArtist ;
    linkml:inlined true ;
    linkml:owner okns:mo_sampled ;
    linkml:range okns:MoSignal ;
    linkml:slot_uri <http://purl.org/ontology/mo/sampled> .

okns:mo_sampled_version a linkml:SlotDefinition ;
    dcterms:source <http://purl.org/ontology/mo/> ;
    dcterms:title "sampled version" ;
    owl:inverseOf okns:mo_sampled_version_of ;
    skos:definition "Associates an analog signal with a sampled version of it" ;
    skos:editorialNote "No occurrences of this slot in the graph." ;
    skos:inScheme okns:mo ;
    skos:mappingRelation <http://purl.org/ontology/mo/sampled_version> ;
    linkml:definition_uri okns:mo_sampled_version ;
    linkml:domain okns:MoAnalogSignal ;
    linkml:inlined true ;
    linkml:owner okns:mo_sampled_version ;
    linkml:range okns:MoDigitalSignal ;
    linkml:slot_uri <http://purl.org/ontology/mo/sampled_version> .

okns:mo_sampled_version_of a linkml:SlotDefinition ;
    dcterms:source <http://purl.org/ontology/mo/> ;
    dcterms:title "sampled version of" ;
    rdfs:subPropertyOf okns:mo_derived_from ;
    owl:inverseOf okns:mo_sampled_version ;
    skos:definition "Associates a digital signal with the analog version of it" ;
    skos:editorialNote "No occurrences of this slot in the graph." ;
    skos:inScheme okns:mo ;
    skos:mappingRelation <http://purl.org/ontology/mo/sampled_version_of> ;
    linkml:definition_uri okns:mo_sampled_version_of ;
    linkml:domain okns:MoDigitalSignal ;
    linkml:inlined true ;
    linkml:owner okns:mo_sampled_version_of ;
    linkml:range okns:MoAnalogSignal ;
    linkml:slot_uri <http://purl.org/ontology/mo/sampled_version_of> .

okns:rdf_value a linkml:SlotDefinition ;
    dcterms:source rdf: ;
    dcterms:title "value" ;
    skos:definition "Idiomatic property used for structured values." ;
    skos:editorialNote "No occurrences of this slot in the graph." ;
    skos:inScheme okns:owl-rdf-rdfs ;
    skos:mappingRelation rdf:value ;
    linkml:definition_uri okns:rdf_value ;
    linkml:domain okns:RdfsResource ;
    linkml:domain_of okns:DctIMT ;
    linkml:inlined true ;
    linkml:owner okns:rdf_value ;
    linkml:range okns:RdfsResource ;
    linkml:slot_uri rdf:value .

okns:rdfs_domain a linkml:SlotDefinition ;
    dcterms:source rdfs: ;
    dcterms:title "domain" ;
    skos:definition "A domain of the subject property." ;
    skos:editorialNote "No occurrences of this slot in the graph." ;
    skos:inScheme okns:owl-rdf-rdfs ;
    skos:mappingRelation rdfs:domain ;
    linkml:definition_uri okns:rdfs_domain ;
    linkml:domain okns:RdfProperty ;
    linkml:domain_of okns:Daml-2001Property ;
    linkml:inlined true ;
    linkml:owner okns:rdfs_domain ;
    linkml:range okns:RdfsClass ;
    linkml:slot_uri rdfs:domain .

okns:rdfs_range a linkml:SlotDefinition ;
    dcterms:source rdfs: ;
    dcterms:title "range" ;
    skos:definition "A range of the subject property." ;
    skos:editorialNote "No occurrences of this slot in the graph." ;
    skos:inScheme okns:owl-rdf-rdfs ;
    skos:mappingRelation rdfs:range ;
    linkml:definition_uri okns:rdfs_range ;
    linkml:domain okns:RdfProperty ;
    linkml:domain_of okns:Daml-2001Property ;
    linkml:inlined true ;
    linkml:owner okns:rdfs_range ;
    linkml:range okns:RdfsClass ;
    linkml:slot_uri rdfs:range .

okns:rdfs_subPropertyOf a linkml:SlotDefinition ;
    dcterms:source rdfs: ;
    dcterms:title "subPropertyOf" ;
    skos:definition "The subject is a subproperty of a property." ;
    skos:editorialNote "No occurrences of this slot in the graph." ;
    skos:inScheme okns:owl-rdf-rdfs ;
    skos:mappingRelation rdfs:subPropertyOf ;
    linkml:definition_uri okns:rdfs_subPropertyOf ;
    linkml:domain okns:RdfProperty ;
    linkml:domain_of okns:Daml-2001Property ;
    linkml:inlined true ;
    linkml:owner okns:rdfs_subPropertyOf ;
    linkml:range okns:RdfProperty ;
    linkml:slot_uri rdfs:subPropertyOf .

okns:skos_broader a linkml:SlotDefinition ;
    dcterms:source <http://www.w3.org/2004/02/skos/core> ;
    dcterms:title "has broader" ;
    rdfs:subPropertyOf okns:skos_broaderTransitive ;
    owl:inverseOf okns:skos_narrower ;
    skos:definition "Relates a concept to a concept that is more general in meaning." ;
    skos:editorialNote "By convention, skos:broader is only used to assert an immediate (i.e. direct) hierarchical link between two conceptual resources.",
        "No occurrences of this slot in the graph." ;
    skos:inScheme okns:skos ;
    skos:mappingRelation skos:broader ;
    skos:note "description: Broader concepts are typically rendered as parents in a concept hierarchy (tree)." ;
    linkml:definition_uri okns:skos_broader ;
    linkml:domain okns:Any ;
    linkml:inlined true ;
    linkml:range okns:Any ;
    linkml:slot_uri skos:broader .

okns:skos_broaderTransitive a linkml:SlotDefinition ;
    dcterms:source <http://www.w3.org/2004/02/skos/core> ;
    dcterms:title "has broader transitive" ;
    rdfs:subPropertyOf okns:skos_semanticRelation ;
    owl:inverseOf okns:skos_narrowerTransitive ;
    skos:definition "skos:broaderTransitive is a transitive superproperty of skos:broader." ;
    skos:editorialNote "By convention, skos:broaderTransitive is not used to make assertions. Rather, the properties can be used to draw inferences about the transitive closure of the hierarchical relation, which is useful e.g. when implementing a simple query expansion algorithm in a search application.",
        "No occurrences of this slot in the graph." ;
    skos:inScheme okns:skos ;
    skos:mappingRelation skos:broaderTransitive ;
    linkml:definition_uri okns:skos_broaderTransitive ;
    linkml:domain okns:Any ;
    linkml:inlined true ;
    linkml:range okns:Any ;
    linkml:slot_uri skos:broaderTransitive .

okns:skos_hasTopConcept a linkml:SlotDefinition ;
    dcterms:source <http://www.w3.org/2004/02/skos/core> ;
    dcterms:title "has top concept" ;
    owl:inverseOf okns:skos_topConceptOf ;
    skos:definition "Relates, by convention, a concept scheme to a concept which is topmost in the broader/narrower concept hierarchies for that scheme, providing an entry point to these hierarchies." ;
    skos:editorialNote "No occurrences of this slot in the graph." ;
    skos:inScheme okns:skos ;
    skos:mappingRelation skos:hasTopConcept ;
    linkml:definition_uri okns:skos_hasTopConcept ;
    linkml:domain okns:SkosConceptScheme ;
    linkml:inlined true ;
    linkml:owner okns:skos_hasTopConcept ;
    linkml:range okns:SkosConcept ;
    linkml:slot_uri skos:hasTopConcept .

okns:skos_narrower a linkml:SlotDefinition ;
    dcterms:source <http://www.w3.org/2004/02/skos/core> ;
    dcterms:title "has narrower" ;
    rdfs:subPropertyOf okns:skos_narrowerTransitive ;
    owl:inverseOf okns:skos_broader ;
    skos:definition "Relates a concept to a concept that is more specific in meaning." ;
    skos:editorialNote "By convention, skos:broader is only used to assert an immediate (i.e. direct) hierarchical link between two conceptual resources.",
        "No occurrences of this slot in the graph." ;
    skos:inScheme okns:skos ;
    skos:mappingRelation skos:narrower ;
    skos:note "description: Narrower concepts are typically rendered as children in a concept hierarchy (tree)." ;
    linkml:definition_uri okns:skos_narrower ;
    linkml:domain okns:Any ;
    linkml:inlined true ;
    linkml:range okns:Any ;
    linkml:slot_uri skos:narrower .

okns:skos_narrowerTransitive a linkml:SlotDefinition ;
    dcterms:source <http://www.w3.org/2004/02/skos/core> ;
    dcterms:title "has narrower transitive" ;
    rdfs:subPropertyOf okns:skos_semanticRelation ;
    owl:inverseOf okns:skos_broaderTransitive ;
    skos:definition "skos:narrowerTransitive is a transitive superproperty of skos:narrower." ;
    skos:editorialNote "By convention, skos:narrowerTransitive is not used to make assertions. Rather, the properties can be used to draw inferences about the transitive closure of the hierarchical relation, which is useful e.g. when implementing a simple query expansion algorithm in a search application.",
        "No occurrences of this slot in the graph." ;
    skos:inScheme okns:skos ;
    skos:mappingRelation skos:narrowerTransitive ;
    linkml:definition_uri okns:skos_narrowerTransitive ;
    linkml:domain okns:Any ;
    linkml:inlined true ;
    linkml:range okns:Any ;
    linkml:slot_uri skos:narrowerTransitive .

okns:skos_prefLabel a linkml:SlotDefinition ;
    dcterms:source <http://www.w3.org/2004/02/skos/core> ;
    dcterms:title "preferred label" ;
    rdfs:subPropertyOf okns:rdfs_label ;
    skos:definition "The preferred lexical label for a resource, in a given language." ;
    skos:editorialNote "No occurrences of this slot in the graph." ;
    skos:inScheme okns:skos ;
    skos:mappingRelation skos:prefLabel ;
    skos:note "description: A resource has no more than one value of skos:prefLabel per language tag, and no more than one value of skos:prefLabel without language tag.",
        "description: The range of skos:prefLabel is the class of RDF plain literals.",
        """description: skos:prefLabel, skos:altLabel and skos:hiddenLabel are pairwise
      disjoint properties.""" ;
    linkml:definition_uri okns:skos_prefLabel ;
    linkml:domain_of okns:TimeDayOfWeek,
        okns:TimeTemporalUnit ;
    linkml:inlined true ;
    linkml:owner okns:TimeTemporalUnit ;
    linkml:range okns:Any ;
    linkml:slot_uri skos:prefLabel .

okns:skos_topConceptOf a linkml:SlotDefinition ;
    dcterms:source <http://www.w3.org/2004/02/skos/core> ;
    dcterms:title "is top concept in scheme" ;
    rdfs:subPropertyOf okns:skos_inScheme ;
    owl:inverseOf okns:skos_hasTopConcept ;
    skos:definition "Relates a concept to the concept scheme that it is a top level concept of." ;
    skos:editorialNote "No occurrences of this slot in the graph." ;
    skos:inScheme okns:skos ;
    skos:mappingRelation skos:topConceptOf ;
    linkml:definition_uri okns:skos_topConceptOf ;
    linkml:domain okns:SkosConcept ;
    linkml:inlined true ;
    linkml:owner okns:skos_topConceptOf ;
    linkml:range okns:SkosConceptScheme ;
    linkml:slot_uri skos:topConceptOf .

okns:time_after a linkml:SlotDefinition ;
    dcterms:title "after" ;
    owl:inverseOf okns:time_before ;
    skos:definition "Gives directionality to time. If a temporal entity T1 is after another temporal entity T2, then the beginning of T1 is after the end of T2." ;
    skos:editorialNote "No occurrences of this slot in the graph." ;
    skos:inScheme okns:time ;
    skos:mappingRelation time:after ;
    skos:note "description: Asume una dirección en el tiempo. Si una entidad temporal T1 está después de otra entidad temporal T2, entonces el principio de T1 está después del final de T2.",
        "description: Gives directionality to time. If a temporal entity T1 is after another temporal entity T2, then the beginning of T1 is after the end of T2.",
        "title: después" ;
    linkml:definition_uri okns:time_after ;
    linkml:domain okns:TimeTemporalEntity ;
    linkml:inlined true ;
    linkml:owner okns:time_after ;
    linkml:range okns:TimeTemporalEntity ;
    linkml:slot_uri time:after .

okns:time_before a linkml:SlotDefinition ;
    dcterms:title "before" ;
    owl:inverseOf okns:time_after ;
    skos:definition "Gives directionality to time. If a temporal entity T1 is before another temporal entity T2, then the end of T1 is before the beginning of T2. Thus, \"before\" can be considered to be basic to instants and derived for intervals." ;
    skos:editorialNote "No occurrences of this slot in the graph." ;
    skos:inScheme okns:time ;
    skos:mappingRelation time:before ;
    skos:note "description: Asume una dirección en el tiempo. Si una entidad temporal T1 está antes que otra entidad temporal T2, entonces el final de T1 está antes que el principio de T2. Así, \"antes\" se puede considerar básica para instantes y derivada para intervalos.",
        "description: Gives directionality to time. If a temporal entity T1 is before another temporal entity T2, then the end of T1 is before the beginning of T2. Thus, \"before\" can be considered to be basic to instants and derived for intervals.",
        "title: antes" ;
    linkml:definition_uri okns:time_before ;
    linkml:domain okns:TimeTemporalEntity ;
    linkml:inlined true ;
    linkml:owner okns:time_before ;
    linkml:range okns:TimeTemporalEntity ;
    linkml:slot_uri time:before .

okns:time_days a linkml:SlotDefinition ;
    dcterms:title "days duration" ;
    skos:definition "length of, or element of the length of, a temporal extent expressed in days" ;
    skos:inScheme okns:time ;
    skos:mappingRelation time:days ;
    skos:note "description: Longitud de, o elemento de la longitud de, una extensión temporal expresada en días.",
        "description: length of, or element of the length of, a temporal extent expressed in days",
        "title: duración en días" ;
    linkml:definition_uri okns:time_days ;
    linkml:domain okns:TimeGeneralDurationDescription ;
    linkml:domain_of okns:TimeTemporalUnit ;
    linkml:owner okns:time_days ;
    linkml:range okns:decimal ;
    linkml:slot_uri time:days .

okns:time_entry_before a linkml:SlotDefinition ;
    owl:inverseOf okns:time_entry_after ;
    skos:editorialNote "No occurrences of this slot in the graph." ;
    skos:inScheme okns:daml ;
    skos:mappingRelation time-entry:before ;
    linkml:definition_uri okns:time_entry_before ;
    linkml:domain okns:Time-entryTemporalThing ;
    linkml:inlined true ;
    linkml:owner okns:time_entry_before ;
    linkml:range okns:Time-entryTemporalThing ;
    linkml:slot_uri time-entry:before ;
    linkml:transitive true .

okns:time_entry_intBefore a linkml:SlotDefinition ;
    rdfs:subPropertyOf okns:time_entry_nonoverlap ;
    owl:inverseOf okns:time_entry_intAfter ;
    skos:editorialNote "No occurrences of this slot in the graph." ;
    skos:inScheme okns:daml ;
    skos:mappingRelation time-entry:intBefore ;
    linkml:definition_uri okns:time_entry_intBefore ;
    linkml:domain okns:Time-entryProperIntervalThing ;
    linkml:inlined true ;
    linkml:owner okns:time_entry_intBefore ;
    linkml:range okns:Time-entryProperIntervalThing ;
    linkml:slot_uri time-entry:intBefore .

okns:time_entry_intDuring a linkml:SlotDefinition ;
    rdfs:subPropertyOf okns:time_entry_startsOrDuring ;
    owl:inverseOf okns:time_entry_intContains ;
    skos:editorialNote "No occurrences of this slot in the graph." ;
    skos:inScheme okns:daml ;
    skos:mappingRelation time-entry:intDuring ;
    linkml:definition_uri okns:time_entry_intDuring ;
    linkml:domain okns:Time-entryProperIntervalThing ;
    linkml:inlined true ;
    linkml:owner okns:time_entry_intDuring ;
    linkml:range okns:Time-entryProperIntervalThing ;
    linkml:slot_uri time-entry:intDuring .

okns:time_entry_intFinishes a linkml:SlotDefinition ;
    owl:inverseOf okns:time_entry_intFinishedBy ;
    skos:editorialNote "No occurrences of this slot in the graph." ;
    skos:inScheme okns:daml ;
    skos:mappingRelation time-entry:intFinishes ;
    linkml:definition_uri okns:time_entry_intFinishes ;
    linkml:domain okns:Time-entryProperIntervalThing ;
    linkml:inlined true ;
    linkml:owner okns:time_entry_intFinishes ;
    linkml:range okns:Time-entryProperIntervalThing ;
    linkml:slot_uri time-entry:intFinishes .

okns:time_entry_intMeets a linkml:SlotDefinition ;
    rdfs:subPropertyOf okns:time_entry_nonoverlap ;
    owl:inverseOf okns:time_entry_intMetBy ;
    skos:editorialNote "No occurrences of this slot in the graph." ;
    skos:inScheme okns:daml ;
    skos:mappingRelation time-entry:intMeets ;
    linkml:definition_uri okns:time_entry_intMeets ;
    linkml:domain okns:Time-entryProperIntervalThing ;
    linkml:inlined true ;
    linkml:owner okns:time_entry_intMeets ;
    linkml:range okns:Time-entryProperIntervalThing ;
    linkml:slot_uri time-entry:intMeets .

okns:time_entry_intOverlaps a linkml:SlotDefinition ;
    owl:inverseOf okns:time_entry_intOverlappedBy ;
    skos:editorialNote "No occurrences of this slot in the graph." ;
    skos:inScheme okns:daml ;
    skos:mappingRelation time-entry:intOverlaps ;
    linkml:definition_uri okns:time_entry_intOverlaps ;
    linkml:domain okns:Time-entryProperIntervalThing ;
    linkml:inlined true ;
    linkml:owner okns:time_entry_intOverlaps ;
    linkml:range okns:Time-entryProperIntervalThing ;
    linkml:slot_uri time-entry:intOverlaps .

okns:time_entry_intStarts a linkml:SlotDefinition ;
    rdfs:subPropertyOf okns:time_entry_startsOrDuring ;
    owl:inverseOf okns:time_entry_intStartedBy ;
    skos:editorialNote "No occurrences of this slot in the graph." ;
    skos:inScheme okns:daml ;
    skos:mappingRelation time-entry:intStarts ;
    linkml:definition_uri okns:time_entry_intStarts ;
    linkml:domain okns:Time-entryProperIntervalThing ;
    linkml:inlined true ;
    linkml:owner okns:time_entry_intStarts ;
    linkml:range okns:Time-entryProperIntervalThing ;
    linkml:slot_uri time-entry:intStarts .

okns:time_hasTime a linkml:SlotDefinition ;
    dcterms:title "has time" ;
    skos:definition "Supports the association of a temporal entity (instant or interval) to any thing" ;
    skos:editorialNote "Característica arriesgada -añadida en la revisión del 2017 que no ha sido todavía utilizada de forma amplia.",
        "Feature at risk - added in 2017 revision, and not yet widely used. ",
        "No occurrences of this slot in the graph." ;
    skos:inScheme okns:time ;
    skos:mappingRelation time:hasTime ;
    skos:note "description: Proporciona soporte a la asociación de una entidad temporal (instante o intervalo) a cualquier cosa.",
        "description: Supports the association of a temporal entity (instant or interval) to any thing",
        "title: tiene tiempo" ;
    linkml:definition_uri okns:time_hasTime ;
    linkml:inlined true ;
    linkml:range okns:TimeTemporalEntity ;
    linkml:slot_uri time:hasTime .

okns:time_hours a linkml:SlotDefinition ;
    dcterms:title "hours duration" ;
    skos:definition "length of, or element of the length of, a temporal extent expressed in hours" ;
    skos:inScheme okns:time ;
    skos:mappingRelation time:hours ;
    skos:note "description: Longitud de, o elemento de la longitud de, una extensión temporal expresada en horas.",
        "description: length of, or element of the length of, a temporal extent expressed in hours",
        "title: duración en horas" ;
    linkml:definition_uri okns:time_hours ;
    linkml:domain okns:TimeGeneralDurationDescription ;
    linkml:domain_of okns:TimeTemporalUnit ;
    linkml:owner okns:time_hours ;
    linkml:range okns:decimal ;
    linkml:slot_uri time:hours .

okns:time_intervalAfter a linkml:SlotDefinition ;
    dcterms:title "interval after" ;
    rdfs:subPropertyOf okns:time_intervalDisjoint ;
    owl:inverseOf okns:time_intervalBefore ;
    skos:definition "If a proper interval T1 is intervalAfter another proper interval T2, then the beginning of T1 is after the end of T2." ;
    skos:editorialNote "No occurrences of this slot in the graph." ;
    skos:inScheme okns:time ;
    skos:mappingRelation time:intervalAfter ;
    skos:note "description: If a proper interval T1 is intervalAfter another proper interval T2, then the beginning of T1 is after the end of T2.",
        "description: Si un intervalo propio T1 es posterior a otro intervalo propio T2, entonces el principio de T1 está después que el final de T2.",
        "title: intervalo posterior" ;
    linkml:definition_uri okns:time_intervalAfter ;
    linkml:domain okns:TimeProperInterval ;
    linkml:inlined true ;
    linkml:owner okns:time_intervalAfter ;
    linkml:range okns:TimeProperInterval ;
    linkml:slot_uri time:intervalAfter .

okns:time_intervalBefore a linkml:SlotDefinition ;
    dcterms:title "interval before" ;
    rdfs:subPropertyOf okns:time_intervalDisjoint ;
    owl:inverseOf okns:time_intervalAfter ;
    skos:definition "If a proper interval T1 is intervalBefore another proper interval T2, then the end of T1 is before the beginning of T2." ;
    skos:editorialNote "No occurrences of this slot in the graph." ;
    skos:inScheme okns:time ;
    skos:mappingRelation time:intervalBefore ;
    skos:note "description: If a proper interval T1 is intervalBefore another proper interval T2, then the end of T1 is before the beginning of T2.",
        "description: Si un intervalo propio T1 está antes que otro intervalo propio T2, entonces el final de T1 está antes que el principio de T2.",
        "title: intervalo anterior" ;
    linkml:definition_uri okns:time_intervalBefore ;
    linkml:domain okns:TimeProperInterval ;
    linkml:inlined true ;
    linkml:owner okns:time_intervalBefore ;
    linkml:range okns:TimeProperInterval ;
    linkml:slot_uri time:intervalBefore .

okns:time_intervalContains a linkml:SlotDefinition ;
    dcterms:title "interval contains" ;
    owl:inverseOf okns:time_intervalDuring ;
    skos:definition "If a proper interval T1 is intervalContains another proper interval T2, then the beginning of T1 is before the beginning of T2, and the end of T1 is after the end of T2." ;
    skos:editorialNote "No occurrences of this slot in the graph." ;
    skos:inScheme okns:time ;
    skos:mappingRelation time:intervalContains ;
    skos:note "description: If a proper interval T1 is intervalContains another proper interval T2, then the beginning of T1 is before the beginning of T2, and the end of T1 is after the end of T2.",
        "description: Si un intervalo propio T1 contiene otro intervalo propio T2, entonces el principio de T1 está antes que el principio de T2, y el final de T1 está después del final de T2.",
        "title: intervalo contiene" ;
    linkml:definition_uri okns:time_intervalContains ;
    linkml:domain okns:TimeProperInterval ;
    linkml:inlined true ;
    linkml:owner okns:time_intervalContains ;
    linkml:range okns:TimeProperInterval ;
    linkml:slot_uri time:intervalContains .

okns:time_intervalDuring a linkml:SlotDefinition ;
    dcterms:title "interval during" ;
    rdfs:subPropertyOf okns:time_intervalIn ;
    owl:inverseOf okns:time_intervalContains ;
    skos:definition "If a proper interval T1 is intervalDuring another proper interval T2, then the beginning of T1 is after the beginning of T2, and the end of T1 is before the end of T2." ;
    skos:editorialNote "No occurrences of this slot in the graph." ;
    skos:inScheme okns:time ;
    skos:mappingRelation time:intervalDuring ;
    skos:note "description: If a proper interval T1 is intervalDuring another proper interval T2, then the beginning of T1 is after the beginning of T2, and the end of T1 is before the end of T2.",
        "description: Si un intervalo propio T1 está durante otro intervalo propio T2, entonces del principio de T1 está después del principio de T2, y el final de T1 está antes que el final de T2.",
        "title: intervalo durante" ;
    linkml:definition_uri okns:time_intervalDuring ;
    linkml:domain okns:TimeProperInterval ;
    linkml:inlined true ;
    linkml:owner okns:time_intervalDuring ;
    linkml:range okns:TimeProperInterval ;
    linkml:slot_uri time:intervalDuring .

okns:time_intervalFinishedBy a linkml:SlotDefinition ;
    dcterms:title "interval finished by" ;
    owl:inverseOf okns:time_intervalFinishes ;
    skos:definition "If a proper interval T1 is intervalFinishedBy another proper interval T2, then the beginning of T1 is before the beginning of T2, and the end of T1 is coincident with the end of T2." ;
    skos:editorialNote "No occurrences of this slot in the graph." ;
    skos:inScheme okns:time ;
    skos:mappingRelation time:intervalFinishedBy ;
    skos:note "description: If a proper interval T1 is intervalFinishedBy another proper interval T2, then the beginning of T1 is before the beginning of T2, and the end of T1 is coincident with the end of T2.",
        "description: Si un intervalo propio T1 está terminado por otro intervalo propio T2, entonces el principio de T1 está antes que el principio de T2, y el final de T1 coincide con el final de T2.",
        "title: intervalo terminado por" ;
    linkml:definition_uri okns:time_intervalFinishedBy ;
    linkml:domain okns:TimeProperInterval ;
    linkml:inlined true ;
    linkml:owner okns:time_intervalFinishedBy ;
    linkml:range okns:TimeProperInterval ;
    linkml:slot_uri time:intervalFinishedBy .

okns:time_intervalFinishes a linkml:SlotDefinition ;
    dcterms:title "interval finishes" ;
    rdfs:subPropertyOf okns:time_intervalIn ;
    owl:inverseOf okns:time_intervalFinishedBy ;
    skos:definition "If a proper interval T1 is intervalFinishes another proper interval T2, then the beginning of T1 is after the beginning of T2, and the end of T1 is coincident with the end of T2." ;
    skos:editorialNote "No occurrences of this slot in the graph." ;
    skos:inScheme okns:time ;
    skos:mappingRelation time:intervalFinishes ;
    skos:note "description: If a proper interval T1 is intervalFinishes another proper interval T2, then the beginning of T1 is after the beginning of T2, and the end of T1 is coincident with the end of T2.",
        "description: Si un intervalo propio T1 termina otro intervalo propio T2, entonces del principio de T1 está después del principio de T2, y el final de T1 coincide con el final de T2.",
        "title: intervalo termina" ;
    linkml:definition_uri okns:time_intervalFinishes ;
    linkml:domain okns:TimeProperInterval ;
    linkml:inlined true ;
    linkml:owner okns:time_intervalFinishes ;
    linkml:range okns:TimeProperInterval ;
    linkml:slot_uri time:intervalFinishes .

okns:time_intervalMeets a linkml:SlotDefinition ;
    dcterms:title "interval meets" ;
    owl:inverseOf okns:time_intervalMetBy ;
    skos:definition "If a proper interval T1 is intervalMeets another proper interval T2, then the end of T1 is coincident with the beginning of T2." ;
    skos:editorialNote "No occurrences of this slot in the graph." ;
    skos:inScheme okns:time ;
    skos:mappingRelation time:intervalMeets ;
    skos:note "description: If a proper interval T1 is intervalMeets another proper interval T2, then the end of T1 is coincident with the beginning of T2.",
        "description: Si un intervalo propio T1 se encuentra con otro intervalo propio T2, entonces el final de T1 coincide con el principio de T2.",
        "title: intervalo se encuentra" ;
    linkml:definition_uri okns:time_intervalMeets ;
    linkml:domain okns:TimeProperInterval ;
    linkml:inlined true ;
    linkml:owner okns:time_intervalMeets ;
    linkml:range okns:TimeProperInterval ;
    linkml:slot_uri time:intervalMeets .

okns:time_intervalMetBy a linkml:SlotDefinition ;
    dcterms:title "interval met by" ;
    owl:inverseOf okns:time_intervalMeets ;
    skos:definition "If a proper interval T1 is intervalMetBy another proper interval T2, then the beginning of T1 is coincident with the end of T2." ;
    skos:editorialNote "No occurrences of this slot in the graph." ;
    skos:inScheme okns:time ;
    skos:mappingRelation time:intervalMetBy ;
    skos:note "description: If a proper interval T1 is intervalMetBy another proper interval T2, then the beginning of T1 is coincident with the end of T2.",
        "description: Si un intervalo propio T1 es 'intervalo encontrado por' otro intervalo propio T2, entonces el principio de T1 coincide con el final de T2.",
        "title: intervalo encontrado por" ;
    linkml:definition_uri okns:time_intervalMetBy ;
    linkml:domain okns:TimeProperInterval ;
    linkml:inlined true ;
    linkml:owner okns:time_intervalMetBy ;
    linkml:range okns:TimeProperInterval ;
    linkml:slot_uri time:intervalMetBy .

okns:time_intervalOverlappedBy a linkml:SlotDefinition ;
    dcterms:title "interval overlapped by" ;
    owl:inverseOf okns:time_intervalOverlaps ;
    skos:definition "If a proper interval T1 is intervalOverlappedBy another proper interval T2, then the beginning of T1 is after the beginning of T2, the beginning of T1 is before the end of T2, and the end of T1 is after the end of T2." ;
    skos:editorialNote "No occurrences of this slot in the graph." ;
    skos:inScheme okns:time ;
    skos:mappingRelation time:intervalOverlappedBy ;
    skos:note "description: If a proper interval T1 is intervalOverlappedBy another proper interval T2, then the beginning of T1 is after the beginning of T2, the beginning of T1 is before the end of T2, and the end of T1 is after the end of T2.",
        "description: Si un intervalo propio T1 es 'intervalo solapado por' otro intervalo propio T2, entonces el principio de T1 es posterior al principio de T2, y el principio de T1 es anterior al final de T2, y el final de T1 es posterior al final de T2.",
        "title: intervalo solapado por" ;
    linkml:definition_uri okns:time_intervalOverlappedBy ;
    linkml:domain okns:TimeProperInterval ;
    linkml:inlined true ;
    linkml:owner okns:time_intervalOverlappedBy ;
    linkml:range okns:TimeProperInterval ;
    linkml:slot_uri time:intervalOverlappedBy .

okns:time_intervalOverlaps a linkml:SlotDefinition ;
    dcterms:title "interval overlaps" ;
    owl:inverseOf okns:time_intervalOverlappedBy ;
    skos:definition "If a proper interval T1 is intervalOverlaps another proper interval T2, then the beginning of T1 is before the beginning of T2, the end of T1 is after the beginning of T2, and the end of T1 is before the end of T2." ;
    skos:editorialNote "No occurrences of this slot in the graph." ;
    skos:inScheme okns:time ;
    skos:mappingRelation time:intervalOverlaps ;
    skos:note "description: Asume una dirección en el tiempo. Si una entidad temporal T1 está después de otra entidad temporal T2, entonces el principio de T1 está después del final de T2.",
        "description: If a proper interval T1 is intervalOverlaps another proper interval T2, then the beginning of T1 is before the beginning of T2, the end of T1 is after the beginning of T2, and the end of T1 is before the end of T2.",
        "description: Si un intervalo propio T1 se solapa con otro intervalo propio T2, entonces el principio de T1 es anterior al principio de T2, el final de T1 es posterior al principio de T2, y el final de T1 es anterior al final de T2.",
        "title: intervalo se solapa" ;
    linkml:definition_uri okns:time_intervalOverlaps ;
    linkml:domain okns:TimeProperInterval ;
    linkml:inlined true ;
    linkml:owner okns:time_intervalOverlaps ;
    linkml:range okns:TimeProperInterval ;
    linkml:slot_uri time:intervalOverlaps .

okns:time_intervalStartedBy a linkml:SlotDefinition ;
    dcterms:title "interval started by" ;
    owl:inverseOf okns:time_intervalStarts ;
    skos:definition "If a proper interval T1 is intervalStarted another proper interval T2, then the beginning of T1 is coincident with the beginning of T2, and the end of T1 is after the end of T2." ;
    skos:editorialNote "No occurrences of this slot in the graph." ;
    skos:inScheme okns:time ;
    skos:mappingRelation time:intervalStartedBy ;
    skos:note "description: If a proper interval T1 is intervalStarted another proper interval T2, then the beginning of T1 is coincident with the beginning of T2, and the end of T1 is after the end of T2.",
        "description: Si un intervalo propio T1 es empezado por otro intervalo propio T2, entonces el principio de T1 coincide con el principio de T2, y el final de T1 es posterior al final de T2." ;
    linkml:definition_uri okns:time_intervalStartedBy ;
    linkml:domain okns:TimeProperInterval ;
    linkml:inlined true ;
    linkml:owner okns:time_intervalStartedBy ;
    linkml:range okns:TimeProperInterval ;
    linkml:slot_uri time:intervalStartedBy .

okns:time_intervalStarts a linkml:SlotDefinition ;
    dcterms:title "interval starts" ;
    rdfs:subPropertyOf okns:time_intervalIn ;
    owl:inverseOf okns:time_intervalStartedBy ;
    skos:definition "If a proper interval T1 is intervalStarts another proper interval T2, then the beginning of T1 is coincident with the beginning of T2, and the end of T1 is before the end of T2." ;
    skos:editorialNote "No occurrences of this slot in the graph." ;
    skos:inScheme okns:time ;
    skos:mappingRelation time:intervalStarts ;
    skos:note "description: If a proper interval T1 is intervalStarts another proper interval T2, then the beginning of T1 is coincident with the beginning of T2, and the end of T1 is before the end of T2.",
        "description: Si un intervalo propio T1 empieza otro intervalo propio T2, entonces del principio de T1 con el final de T2, y el final de T1 es anterior al final de T2.",
        "description: Si un intervalo propio T1 empieza otro intervalo propio T2, entonces del principio de T1 con el principio de T2, y el final de T1 es anterior al final de T2.",
        "title: intervalo empieza" ;
    linkml:definition_uri okns:time_intervalStarts ;
    linkml:domain okns:TimeProperInterval ;
    linkml:inlined true ;
    linkml:owner okns:time_intervalStarts ;
    linkml:range okns:TimeProperInterval ;
    linkml:slot_uri time:intervalStarts .

okns:time_minutes a linkml:SlotDefinition ;
    dcterms:title "minutes" ;
    skos:definition "length, or element of, a temporal extent expressed in minutes" ;
    skos:inScheme okns:time ;
    skos:mappingRelation time:minutes ;
    skos:note "description: Longitud de, o elemento de la longitud de, una extensión temporal expresada en minutos.",
        "description: length, or element of, a temporal extent expressed in minutes",
        "title: minutos" ;
    linkml:definition_uri okns:time_minutes ;
    linkml:domain okns:TimeGeneralDurationDescription ;
    linkml:domain_of okns:TimeTemporalUnit ;
    linkml:owner okns:time_minutes ;
    linkml:range okns:decimal ;
    linkml:slot_uri time:minutes .

okns:time_months a linkml:SlotDefinition ;
    dcterms:title "months duration" ;
    skos:definition "length of, or element of the length of, a temporal extent expressed in months" ;
    skos:inScheme okns:time ;
    skos:mappingRelation time:months ;
    skos:note "description: Longitud de, o elemento de la longitud de, una extensión temporal expresada en meses.",
        "description: length of, or element of the length of, a temporal extent expressed in months",
        "title: duración en meses" ;
    linkml:definition_uri okns:time_months ;
    linkml:domain okns:TimeGeneralDurationDescription ;
    linkml:domain_of okns:TimeTemporalUnit ;
    linkml:owner okns:time_months ;
    linkml:range okns:decimal ;
    linkml:slot_uri time:months .

okns:time_seconds a linkml:SlotDefinition ;
    dcterms:title "seconds duration" ;
    rdfs:seeAlso <http://www.bipm.org/en/publications/si-brochure/second.html> ;
    skos:definition "length of, or element of the length of, a temporal extent expressed in seconds" ;
    skos:inScheme okns:time ;
    skos:mappingRelation time:seconds ;
    skos:note "description: Longitud de, o elemento de la longitud de, una extensión temporal expresada en segundos.",
        "title: duración en segundos" ;
    linkml:definition_uri okns:time_seconds ;
    linkml:domain okns:TimeGeneralDurationDescription ;
    linkml:domain_of okns:TimeTemporalUnit ;
    linkml:owner okns:time_seconds ;
    linkml:range okns:decimal ;
    linkml:slot_uri time:seconds .

okns:time_weeks a linkml:SlotDefinition ;
    dcterms:title "weeks duration" ;
    skos:definition "length of, or element of the length of, a temporal extent expressed in weeks" ;
    skos:inScheme okns:time ;
    skos:mappingRelation time:weeks ;
    skos:note "description: Longitud de, o elemento de la longitud de, una extensión temporal expresada en semanas.",
        "title: duración en semanas" ;
    linkml:definition_uri okns:time_weeks ;
    linkml:domain okns:TimeGeneralDurationDescription ;
    linkml:domain_of okns:TimeTemporalUnit ;
    linkml:owner okns:time_weeks ;
    linkml:range okns:decimal ;
    linkml:slot_uri time:weeks .

okns:time_years a linkml:SlotDefinition ;
    dcterms:title "years duration" ;
    skos:definition "length of, or element of the length of, a temporal extent expressed in years" ;
    skos:inScheme okns:time ;
    skos:mappingRelation time:years ;
    skos:note "description: Longitud de, o elemento de la longitud de, una extensión temporal expresada en años.",
        "title: duración en años" ;
    linkml:definition_uri okns:time_years ;
    linkml:domain okns:TimeGeneralDurationDescription ;
    linkml:domain_of okns:TimeTemporalUnit ;
    linkml:owner okns:time_years ;
    linkml:range okns:decimal ;
    linkml:slot_uri time:years .

okns:token a linkml:TypeDefinition ;
    skos:definition "Tokenized string, one that does not contain the carriage return (#xD), line feed (#xA) nor tab (#x9) characters, that has no leading or trailing spaces (#x20) and that has no internal sequences of two or more spaces." ;
    skos:inScheme okns:extended_types ;
    skos:note "added by Mahir Morshed <mmorshed@scripps.edu>" ;
    linkml:base "str" ;
    linkml:definition_uri linkml:Token ;
    linkml:typeof okns:normalizedstring ;
    linkml:uri xsd:token .

okns:tzont_hasAncestorRegion a linkml:SlotDefinition ;
    skos:editorialNote "No occurrences of this slot in the graph." ;
    skos:inScheme okns:daml ;
    skos:mappingRelation tzont:hasAncestorRegion ;
    linkml:definition_uri okns:tzont_hasAncestorRegion ;
    linkml:domain okns:TzontRegion ;
    linkml:inlined true ;
    linkml:owner okns:tzont_hasAncestorRegion ;
    linkml:range okns:TzontRegion ;
    linkml:slot_uri tzont:hasAncestorRegion ;
    linkml:transitive true .

okns:tzont_hasParentRegion a linkml:SlotDefinition ;
    rdfs:subPropertyOf okns:tzont_hasAncestorRegion ;
    skos:editorialNote "No occurrences of this slot in the graph." ;
    skos:inScheme okns:daml ;
    skos:mappingRelation tzont:hasParentRegion ;
    linkml:definition_uri okns:tzont_hasParentRegion ;
    linkml:inlined true ;
    linkml:range okns:Any ;
    linkml:slot_uri tzont:hasParentRegion .

okns:wot_hasKey a linkml:SlotDefinition ;
    dcterms:source wot: ;
    dcterms:title "has Key" ;
    owl:inverseOf okns:wot_identity ;
    skos:definition "A property to link a PubKey from a User" ;
    skos:editorialNote "No occurrences of this slot in the graph." ;
    skos:inScheme okns:wot ;
    skos:mappingRelation wot:hasKey ;
    linkml:definition_uri okns:wot_hasKey ;
    linkml:domain okns:WotUser ;
    linkml:inlined true ;
    linkml:owner okns:wot_hasKey ;
    linkml:range okns:WotPubKey ;
    linkml:slot_uri wot:hasKey .

okns:wot_identity a linkml:SlotDefinition ;
    dcterms:source wot: ;
    dcterms:title "Identity" ;
    owl:inverseOf okns:wot_hasKey ;
    skos:definition "A property linking a public key to the user of the key." ;
    skos:editorialNote "No occurrences of this slot in the graph." ;
    skos:inScheme okns:wot ;
    skos:mappingRelation wot:identity ;
    linkml:definition_uri okns:wot_identity ;
    linkml:domain okns:WotPubKey ;
    linkml:inlined true ;
    linkml:owner okns:wot_identity ;
    linkml:range okns:WotUser ;
    linkml:slot_uri wot:identity .

okns:CcPermission a linkml:ClassDefinition ;
    dcterms:title "permission" ;
    skos:definition "an action that may or may not be allowed or desired" ;
    skos:inScheme okns:cc ;
    skos:mappingRelation cc:Permission ;
    linkml:class_uri cc:Permission ;
    linkml:definition_uri okns:CcPermission ;
    linkml:slot_usage [ ] ;
    linkml:slots okns:dc_description,
        okns:dc_title .

okns:CcProhibition a linkml:ClassDefinition ;
    dcterms:title "prohibition" ;
    skos:definition "something you may be asked not to do" ;
    skos:inScheme okns:cc ;
    skos:mappingRelation cc:Prohibition ;
    linkml:class_uri cc:Prohibition ;
    linkml:definition_uri okns:CcProhibition ;
    linkml:slot_usage [ ] ;
    linkml:slots okns:dc_description,
        okns:dc_title .

okns:CcWork a linkml:ClassDefinition ;
    dcterms:title "work" ;
    rdfs:seeAlso <http://www.w3.org/2000/10/swap/pim/doc#Work> ;
    skos:definition "a potentially copyrightable work" ;
    skos:inScheme okns:cc ;
    skos:mappingRelation cc:Work ;
    linkml:class_uri cc:Work ;
    linkml:definition_uri okns:CcWork ;
    linkml:slot_usage [ ] .

okns:Daml-cityCity a linkml:ClassDefinition ;
    dcterms:title "City" ;
    skos:definition "High level city concept." ;
    skos:inScheme okns:daml ;
    skos:mappingRelation daml-city:City ;
    linkml:class_uri daml-city:City ;
    linkml:definition_uri okns:Daml-cityCity ;
    linkml:is_a okns:Daml-oilThing ;
    linkml:slot_usage [ ] .

okns:Daml-oilThing a linkml:ClassDefinition ;
    dcterms:title "No class (entity type) name specified -- this class is noted as a superclass of another class in this graph but has not itself been defined." ;
    skos:inScheme okns:daml ;
    skos:mappingRelation daml-oil:Thing ;
    linkml:class_uri daml-oil:Thing ;
    linkml:definition_uri okns:Daml-oilThing ;
    linkml:slot_usage [ ] .

okns:DcmitypeCollection a linkml:ClassDefinition ;
    dcterms:source dcmitype: ;
    dcterms:title "Collection" ;
    skos:definition "A collection is described as a group; its parts may also be separately described." ;
    skos:inScheme okns:dc ;
    skos:mappingRelation dcmitype:Collection ;
    skos:note "description: An aggregation of resources." ;
    linkml:class_uri dcmitype:Collection ;
    linkml:definition_uri okns:DcmitypeCollection ;
    linkml:slot_usage [ ] .

okns:DctLocationPeriodOrJurisdiction a linkml:ClassDefinition ;
    dcterms:source dcterms: ;
    dcterms:title "Location, Period, or Jurisdiction" ;
    skos:definition "A location, period of time, or jurisdiction." ;
    skos:inScheme okns:dc ;
    skos:mappingRelation dcterms:LocationPeriodOrJurisdiction ;
    linkml:class_uri dcterms:LocationPeriodOrJurisdiction ;
    linkml:definition_uri okns:DctLocationPeriodOrJurisdiction ;
    linkml:slot_usage [ ] .

okns:DctMediaType a linkml:ClassDefinition ;
    dcterms:source dcterms: ;
    dcterms:title "Media Type" ;
    skos:definition "A file format or physical medium." ;
    skos:inScheme okns:dc ;
    skos:mappingRelation dcterms:MediaType ;
    linkml:class_uri dcterms:MediaType ;
    linkml:definition_uri okns:DctMediaType ;
    linkml:is_a okns:DctMediaTypeOrExtent ;
    linkml:slot_usage [ ] .

okns:FoafGroup a linkml:ClassDefinition ;
    dcterms:title "Group" ;
    skos:definition "A class of Agents." ;
    skos:inScheme okns:foaf ;
    skos:mappingRelation foaf:Group ;
    linkml:class_uri foaf:Group ;
    linkml:definition_uri okns:FoafGroup ;
    linkml:is_a okns:FoafAgent ;
    linkml:slot_usage [ ] .

okns:IcalVtimezone a linkml:ClassDefinition ;
    dcterms:title "VTIMEZONE" ;
    skos:definition "Provide a grouping of component properties that defines a time zone." ;
    skos:inScheme okns:ical ;
    skos:mappingRelation ical:Vtimezone ;
    linkml:class_uri ical:Vtimezone ;
    linkml:definition_uri okns:IcalVtimezone ;
    linkml:slot_usage [ ] .

okns:IcalVtodo a linkml:ClassDefinition ;
    dcterms:title "VTODO" ;
    skos:definition "Provide a grouping of calendar properties that describe a to-do." ;
    skos:inScheme okns:ical ;
    skos:mappingRelation ical:Vtodo ;
    linkml:class_uri ical:Vtodo ;
    linkml:definition_uri okns:IcalVtodo ;
    linkml:slot_usage [ ] .

okns:MoComposition a linkml:ClassDefinition ;
    dcterms:source <http://purl.org/ontology/mo/> ;
    dcterms:title "composition" ;
    skos:definition "A composition event.␊        Takes as agent the composer himself.␊        It produces a MusicalWork, or a MusicalExpression (when the initial \"product\" is a score, for example), or both..." ;
    skos:inScheme okns:mo ;
    skos:mappingRelation ns1:Composition ;
    linkml:class_uri <http://purl.org/ontology/mo/Composition> ;
    linkml:definition_uri okns:MoComposition ;
    linkml:is_a okns:EventEvent ;
    linkml:slot_usage [ ] .

okns:MoMembership a linkml:ClassDefinition ;
    dcterms:source <http://purl.org/ontology/mo/> ;
    dcterms:title "membership" ;
    skos:definition "A membership event, where one or several people belongs to a group during a particular time period." ;
    skos:inScheme okns:mo ;
    skos:mappingRelation ns1:Membership ;
    linkml:class_uri <http://purl.org/ontology/mo/Membership> ;
    linkml:definition_uri okns:MoMembership ;
    linkml:is_a okns:EventEvent ;
    linkml:slot_usage [ ] .

okns:MoRecording a linkml:ClassDefinition ;
    dcterms:source <http://purl.org/ontology/mo/> ;
    dcterms:title "recording" ;
    skos:definition "A recording event.␊        Takes a sound as a factor to produce a signal (analog or digital).␊        The location of such events (if any) is the actual location of the corresponding␊        microphone or the \"recording device\"." ;
    skos:inScheme okns:mo ;
    skos:mappingRelation ns1:Recording ;
    linkml:class_uri <http://purl.org/ontology/mo/Recording> ;
    linkml:definition_uri okns:MoRecording ;
    linkml:is_a okns:EventEvent ;
    linkml:slot_usage [ ] .

okns:MoSound a linkml:ClassDefinition ;
    dcterms:source <http://purl.org/ontology/mo/> ;
    dcterms:title "sound" ;
    skos:definition "A subclass of MusicalExpression, representing a sound. Realisation of a MusicalWork during a musical Performance." ;
    skos:inScheme okns:mo ;
    skos:mappingRelation ns1:Sound ;
    linkml:class_uri <http://purl.org/ontology/mo/Sound> ;
    linkml:definition_uri okns:MoSound ;
    linkml:is_a okns:MoMusicalExpression ;
    linkml:slot_usage [ ] .

okns:RdfStatement a linkml:ClassDefinition ;
    dcterms:source rdf: ;
    dcterms:title "Statement" ;
    skos:definition "The class of RDF statements." ;
    skos:inScheme okns:owl-rdf-rdfs ;
    skos:mappingRelation rdf:Statement ;
    linkml:class_uri rdf:Statement ;
    linkml:definition_uri okns:RdfStatement ;
    linkml:is_a okns:RdfsResource ;
    linkml:slot_usage [ ] .

okns:RdfsContainer a linkml:ClassDefinition ;
    dcterms:source rdfs: ;
    dcterms:title "Container" ;
    skos:definition "The class of RDF containers." ;
    skos:inScheme okns:owl-rdf-rdfs ;
    skos:mappingRelation rdfs:Container ;
    linkml:class_uri rdfs:Container ;
    linkml:definition_uri okns:RdfsContainer ;
    linkml:is_a okns:RdfsResource ;
    linkml:slot_usage [ ] .

okns:SkosConceptScheme a linkml:ClassDefinition ;
    dcterms:source <http://www.w3.org/2004/02/skos/core> ;
    dcterms:title "Concept Scheme" ;
    skos:definition "A set of concepts, optionally including statements about semantic relationships between those concepts." ;
    skos:editorialNote "A concept scheme may be defined to include concepts from different sources." ;
    skos:inScheme okns:skos ;
    skos:mappingRelation skos:ConceptScheme ;
    linkml:class_uri skos:ConceptScheme ;
    linkml:definition_uri okns:SkosConceptScheme ;
    linkml:slot_usage [ ] .

okns:Time-entryEvent a linkml:ClassDefinition ;
    dcterms:title "No class (entity type) name specified -- this class is noted as a superclass of another class in this graph but has not itself been defined." ;
    skos:inScheme okns:daml ;
    skos:mappingRelation time-entry:Event ;
    linkml:class_uri time-entry:Event ;
    linkml:definition_uri okns:Time-entryEvent ;
    linkml:is_a okns:Time-entryTemporalThing ;
    linkml:slot_usage [ ] .

okns:Time-entryIntervalThing a linkml:ClassDefinition ;
    dcterms:title "No class (entity type) name specified -- this class is noted as a superclass of another class in this graph but has not itself been defined." ;
    skos:inScheme okns:daml ;
    skos:mappingRelation time-entry:IntervalThing ;
    linkml:class_uri time-entry:IntervalThing ;
    linkml:definition_uri okns:Time-entryIntervalThing ;
    linkml:is_a okns:Time-entryTemporalThing ;
    linkml:slot_usage [ ] .

okns:TimeDayOfWeek a linkml:ClassDefinition ;
    dcterms:title "Day of week" ;
    skos:definition "The day of week" ;
    skos:editorialNote "La pertenencia a la clase 'día de la semana' está abierta, para permitir longitudes de semana alternativas y diferentes nombres de días.",
        "Membership of the class :DayOfWeek is open, to allow for alternative week lengths and different day names.",
        """Remove enumeration from definition, in order to allow other days to be used when required in other calendars. 
NOTE: existing days are still present as members of the class, but the class membership is now open. 

In the original OWL-Time the following constraint appeared: 
  owl:oneOf (
      time:Monday
      time:Tuesday
      time:Wednesday
      time:Thursday
      time:Friday
      time:Saturday
      time:Sunday
    ) ;""" ;
    skos:inScheme okns:time ;
    skos:mappingRelation time:DayOfWeek ;
    skos:note "description: El día de la semana",
        "description: The day of week",
        "title: día de la semana" ;
    linkml:class_uri time:DayOfWeek ;
    linkml:definition_uri okns:TimeDayOfWeek ;
    linkml:is_a okns:OwlThing ;
    linkml:slot_usage [ ] ;
    linkml:slots okns:rdfs_label,
        okns:skos_prefLabel .

okns:TimeTemporalPosition a linkml:ClassDefinition ;
    dcterms:title "Temporal position" ;
    skos:definition "A position on a time-line" ;
    skos:inScheme okns:time ;
    skos:mappingRelation time:TemporalPosition ;
    skos:note "description: A position on a time-line",
        "description: Una posición sobre una línea de tiempo.",
        "title: posición temporal" ;
    linkml:class_uri time:TemporalPosition ;
    linkml:definition_uri okns:TimeTemporalPosition ;
    linkml:slot_usage [ ] .

okns:TimeTimePosition a linkml:ClassDefinition ;
    dcterms:title "Time position" ;
    skos:definition "A temporal position described using either a (nominal) value from an ordinal reference system, or a (numeric) value in a temporal coordinate system." ;
    skos:inScheme okns:time ;
    skos:mappingRelation time:TimePosition ;
    skos:note "description: A temporal position described using either a (nominal) value from an ordinal reference system, or a (numeric) value in a temporal coordinate system.",
        "description: Una posición temporal descrita utilizando bien un valor (nominal) de un sistema de referencia ordinal, o un valor (numérico) en un sistema de coordenadas temporales.",
        "title: posición de tiempo" ;
    linkml:class_uri time:TimePosition ;
    linkml:definition_uri okns:TimeTimePosition ;
    linkml:is_a okns:TimeTemporalPosition ;
    linkml:slot_usage [ ] .

okns:TzontTimeZone a linkml:ClassDefinition ;
    skos:inScheme okns:daml ;
    skos:mappingRelation tzont:TimeZone ;
    linkml:class_uri tzont:TimeZone ;
    linkml:definition_uri okns:TzontTimeZone ;
    linkml:slot_usage [ ] .

okns:daml_oil_comment a linkml:SlotDefinition ;
    skos:inScheme okns:daml ;
    skos:mappingRelation daml-oil:comment ;
    linkml:definition_uri okns:daml_oil_comment ;
    linkml:domain_of okns:Daml-oilClass,
        okns:Daml-oilOntology ;
    linkml:owner okns:Daml-oilOntology ;
    linkml:range okns:string ;
    linkml:slot_uri daml-oil:comment .

okns:daml_oil_subPropertyOf a linkml:SlotDefinition ;
    skos:inScheme okns:daml ;
    skos:mappingRelation daml-oil:subPropertyOf ;
    linkml:definition_uri okns:daml_oil_subPropertyOf ;
    linkml:domain_of okns:Daml-oilObjectProperty ;
    linkml:inlined true ;
    linkml:owner okns:Daml-oilObjectProperty ;
    linkml:range okns:Daml-oilObjectProperty ;
    linkml:slot_uri daml-oil:subPropertyOf .

okns:datetime a linkml:TypeDefinition ;
    skos:definition "The combination of a date and time" ;
    skos:editorialNote "If you are authoring schemas in LinkML YAML, the type is referenced with the lower case \"datetime\"." ;
    skos:exactMatch schema1:DateTime ;
    skos:inScheme linkml:types ;
    linkml:base "XSDDateTime" ;
    linkml:imported_from "linkml:types" ;
    linkml:repr "str" ;
    linkml:definition_uri linkml:Datetime ;
    linkml:uri xsd:dateTime .

okns:dct_format a linkml:SlotDefinition ;
    dcterms:source dcterms: ;
    dcterms:title "Format" ;
    rdfs:subPropertyOf okns:dc_format ;
    skos:definition "Recommended practice is to use a controlled vocabulary where available. For example, for file formats one could use the list of Internet Media Types [[MIME](https://www.iana.org/assignments/media-types/media-types.xhtml)].  Examples of dimensions include size and duration." ;
    skos:editorialNote "No occurrences of this slot in the graph." ;
    skos:inScheme okns:dc ;
    skos:mappingRelation dcterms:format ;
    skos:note "description: The file format, physical medium, or dimensions of the resource." ;
    linkml:definition_uri okns:dct_format ;
    linkml:inlined true ;
    linkml:range okns:Any ;
    linkml:slot_uri dcterms:format .

okns:dct_subject a linkml:SlotDefinition ;
    dcterms:source dcterms: ;
    dcterms:title "Subject" ;
    rdfs:subPropertyOf okns:dc_subject ;
    skos:definition "Recommended practice is to refer to the subject with a URI. If this is not possible or feasible, a literal value that identifies the subject may be provided. Both should preferably refer to a subject in a controlled vocabulary." ;
    skos:editorialNote "No occurrences of this slot in the graph." ;
    skos:inScheme okns:dc ;
    skos:mappingRelation dcterms:subject ;
    skos:note "description: A topic of the resource." ;
    linkml:definition_uri okns:dct_subject ;
    linkml:inlined true ;
    linkml:range okns:Any ;
    linkml:slot_uri dcterms:subject .

okns:event_isFactorOf a linkml:SlotDefinition ;
    dcterms:title "factor of" ;
    skos:editorialNote "No occurrences of this slot in the graph." ;
    skos:exactMatch event:factor_of ;
    skos:inScheme okns:event ;
    skos:mappingRelation event:isFactorOf ;
    linkml:definition_uri okns:event_isFactorOf ;
    linkml:inlined true ;
    linkml:range okns:Any ;
    linkml:slot_uri event:isFactorOf .

okns:foaf_member a linkml:SlotDefinition ;
    dcterms:source foaf: ;
    dcterms:title "member" ;
    owl:inverseOf okns:mo_member_of ;
    skos:definition "Indicates a member of a Group" ;
    skos:editorialNote "No occurrences of this slot in the graph." ;
    skos:inScheme okns:foaf ;
    skos:mappingRelation foaf:member ;
    linkml:definition_uri okns:foaf_member ;
    linkml:domain okns:FoafGroup ;
    linkml:inlined true ;
    linkml:owner okns:foaf_member ;
    linkml:range okns:FoafAgent ;
    linkml:slot_uri foaf:member .

okns:frbr_embodiment a linkml:SlotDefinition ;
    dcterms:source frbr: ;
    dcterms:title "embodiment" ;
    rdfs:subPropertyOf okns:frbr_relatedEndeavour ;
    owl:inverseOf okns:frbr_embodimentOf ;
    skos:definition "A manifestation that embodies an expression." ;
    skos:editorialNote "N02934a353f4645ce943310f1bfdd28cf",
        "N3559b6651b5047c4a35f453761bb06b0",
        "No occurrences of this slot in the graph." ;
    skos:inScheme okns:frbr ;
    skos:mappingRelation frbr:embodiment ;
    linkml:definition_uri okns:frbr_embodiment ;
    linkml:domain okns:FrbrExpression ;
    linkml:inlined true ;
    linkml:owner okns:frbr_embodiment ;
    linkml:range okns:FrbrManifestation ;
    linkml:slot_uri frbr:embodiment .

okns:frbr_exemplar a linkml:SlotDefinition ;
    dcterms:source frbr: ;
    dcterms:title "exemplar" ;
    rdfs:subPropertyOf okns:frbr_relatedEndeavour ;
    owl:inverseOf okns:frbr_exemplarOf ;
    skos:definition "An item that is an exemplar of a manifestation." ;
    skos:editorialNote "N055be709e2d14472969b55ee355d2119",
        "N958e21883c704c89b174428a0cf5d31b",
        "No occurrences of this slot in the graph." ;
    skos:inScheme okns:frbr ;
    skos:mappingRelation frbr:exemplar ;
    linkml:definition_uri okns:frbr_exemplar ;
    linkml:domain okns:FrbrManifestation ;
    linkml:inlined true ;
    linkml:owner okns:frbr_exemplar ;
    linkml:range okns:FrbrItem ;
    linkml:slot_uri frbr:exemplar .

okns:mo_available_as a linkml:SlotDefinition ;
    dcterms:source <http://purl.org/ontology/mo/> ;
    rdfs:subPropertyOf okns:frbr_exemplar ;
    skos:definition "Relates a musical manifestation to a musical item (this album, and my particular cd). By using␊        this property, there is no assumption on wether the full content is available on the linked item.␊        To be explicit about this, you can use a sub-property, such as mo:item (the full manifestation␊        is available on that item) or mo:preview (only a part of the manifestation is available on␊        that item).␊␊        This is a subproperty of frbr:examplar." ;
    skos:editorialNote "No occurrences of this slot in the graph." ;
    skos:inScheme okns:mo ;
    skos:mappingRelation <http://purl.org/ontology/mo/available_as> ;
    linkml:definition_uri okns:mo_available_as ;
    linkml:domain okns:MoMusicalManifestation ;
    linkml:inlined true ;
    linkml:owner okns:mo_available_as ;
    linkml:range okns:MoMusicalItem ;
    linkml:slot_uri <http://purl.org/ontology/mo/available_as> .

okns:mo_gtin a linkml:SlotDefinition ;
    dcterms:source <http://purl.org/ontology/mo/> ;
    dcterms:title "gtin" ;
    skos:definition "GTIN is a grouping term for EANs and UPCs. In common speech those are called barcodes although the barcodes are just a representation of those identifying numbers." ;
    skos:editorialNote "No occurrences of this slot in the graph." ;
    skos:inScheme okns:mo ;
    skos:mappingRelation <http://purl.org/ontology/mo/gtin> ;
    linkml:definition_uri okns:mo_gtin ;
    linkml:domain okns:MoRelease ;
    linkml:owner okns:mo_gtin ;
    linkml:range okns:string ;
    linkml:slot_uri <http://purl.org/ontology/mo/gtin> .

okns:mo_interpreter a linkml:SlotDefinition ;
    dcterms:source <http://purl.org/ontology/mo/> ;
    dcterms:title "has interpeter" ;
    skos:definition "Adds an involved music artist, who interpreted, remixed, or otherwise modified an existing signal, which resulted in the signal that is here the subject of this relation." ;
    skos:editorialNote "No occurrences of this slot in the graph." ;
    skos:inScheme okns:mo ;
    skos:mappingRelation <http://purl.org/ontology/mo/interpreter> ;
    linkml:definition_uri okns:mo_interpreter ;
    linkml:domain okns:MoSignal ;
    linkml:inlined true ;
    linkml:owner okns:mo_interpreter ;
    linkml:range okns:MoMusicArtist ;
    linkml:slot_uri <http://purl.org/ontology/mo/interpreter> .

okns:rdfs_subClassOf a linkml:SlotDefinition ;
    dcterms:source rdfs: ;
    dcterms:title "subClassOf" ;
    skos:definition "The subject is a subclass of a class." ;
    skos:inScheme okns:owl-rdf-rdfs ;
    skos:mappingRelation rdfs:subClassOf ;
    linkml:definition_uri okns:rdfs_subClassOf ;
    linkml:domain okns:RdfsClass ;
    linkml:domain_of okns:RdfsDatatype ;
    linkml:inlined true ;
    linkml:owner okns:rdfs_subClassOf ;
    linkml:range okns:RdfsClass ;
    linkml:slot_uri rdfs:subClassOf .

okns:signedinteger a linkml:TypeDefinition ;
    rdfs:seeAlso <https://numpy.org/doc/stable/reference/arrays.scalars.html#numpy.signedinteger> ;
    skos:definition "An integer that may be negative" ;
    skos:inScheme okns:extended_types ;
    linkml:base "int" ;
    linkml:definition_uri linkml:Signedinteger ;
    linkml:typeof okns:integer ;
    linkml:uri xsd:integer .

okns:sim_element a linkml:SlotDefinition ;
    dcterms:source sim: ;
    dcterms:title "element" ;
    skos:definition "Specifies an entity involved in the given <code>sim:Association</code> and implies the given association is undirected." ;
    skos:editorialNote "No occurrences of this slot in the graph." ;
    skos:inScheme okns:sim ;
    skos:mappingRelation sim:element ;
    linkml:definition_uri okns:sim_element ;
    linkml:domain okns:SimAssociation ;
    linkml:inlined true ;
    linkml:owner okns:sim_element ;
    linkml:range okns:Any ;
    linkml:slot_uri sim:element .

okns:time_entry_startsOrDuring a linkml:SlotDefinition ;
    dcterms:title "No slot (predicate) name specified -- this slot is noted as a subproperty of another slot in this graph but has not itself been defined." ;
    skos:editorialNote "No occurrences of this slot in the graph." ;
    skos:inScheme okns:daml ;
    skos:mappingRelation time-entry:startsOrDuring ;
    linkml:definition_uri okns:time_entry_startsOrDuring ;
    linkml:domain okns:Time-entryProperIntervalThing ;
    linkml:inlined true ;
    linkml:owner okns:time_entry_startsOrDuring ;
    linkml:range okns:Time-entryProperIntervalThing ;
    linkml:slot_uri time-entry:startsOrDuring .

okns:time_hasTemporalDuration a linkml:SlotDefinition ;
    dcterms:title "has temporal duration" ;
    skos:definition "Duration of a temporal entity." ;
    skos:editorialNote "No occurrences of this slot in the graph." ;
    skos:inScheme okns:time ;
    skos:mappingRelation time:hasTemporalDuration ;
    skos:note "description: Duración de una entidad temporal.",
        "description: Duration of a temporal entity.",
        "title: tiene duración temporal" ;
    linkml:definition_uri okns:time_hasTemporalDuration ;
    linkml:domain okns:TimeTemporalEntity ;
    linkml:inlined true ;
    linkml:owner okns:time_hasTemporalDuration ;
    linkml:range okns:TimeTemporalDuration ;
    linkml:slot_uri time:hasTemporalDuration .

okns:time_inTemporalPosition a linkml:SlotDefinition ;
    dcterms:title "Temporal position" ;
    skos:definition "Position of a time instant" ;
    skos:editorialNote "No occurrences of this slot in the graph." ;
    skos:inScheme okns:time ;
    skos:mappingRelation time:inTemporalPosition ;
    skos:note "description: Posición de un instante de tiempo.",
        "description: Position of a time instant",
        "title: posición temporal" ;
    linkml:definition_uri okns:time_inTemporalPosition ;
    linkml:domain okns:TimeInstant ;
    linkml:inlined true ;
    linkml:owner okns:time_inTemporalPosition ;
    linkml:range okns:TimeTemporalPosition ;
    linkml:slot_uri time:inTemporalPosition .

okns:time_intervalDisjoint a linkml:SlotDefinition ;
    dcterms:title "interval disjoint" ;
    skos:definition "If a proper interval T1 is intervalDisjoint another proper interval T2, then the beginning of T1 is after the end of T2, or the end of T1 is before the beginning of T2, i.e. the intervals do not overlap in any way, but their ordering relationship is not known." ;
    skos:editorialNote "Esta relación entre intervalos no estaba incluida en las 13 relaciones básicas definidas por Allen (1984), pero está definida en T.3 como la unión de 'intervalo anterior' con 'intervalo posterior'. Sin embargo, esto está fuera de la expresividad de OWL2, por tanto, está implementado como una propiedad explícita, con 'intervalo anterior' e 'intervalo posterior' como sub-propiedades.",
        "No occurrences of this slot in the graph.",
        "This interval relation is not included in the 13 basic relationships defined in Allen (1984), but is defined in (T.3) as the union of :intervalBefore v :intervalAfter . However, that is outside OWL2 expressivity, so is implemented as an explicit property, with :intervalBefore , :intervalAfter as sub-properties" ;
    skos:inScheme okns:time ;
    skos:mappingRelation time:intervalDisjoint ;
    skos:note "description: If a proper interval T1 is intervalDisjoint another proper interval T2, then the beginning of T1 is after the end of T2, or the end of T1 is before the beginning of T2, i.e. the intervals do not overlap in any way, but their ordering relationship is not known.",
        "description: Si un intervalo propio T1 es disjunto con otro intervalo propio T2, entonces el principio de T1 está después del final de T2, o el final de T1 está antes que el principio de T2, es decir, los intervalos no se solapan de ninguna forma, aunque su relación de orden no se conozca.",
        "title: intervalo disjunto" ;
    linkml:definition_uri okns:time_intervalDisjoint ;
    linkml:domain okns:TimeProperInterval ;
    linkml:inlined true ;
    linkml:owner okns:time_intervalDisjoint ;
    linkml:range okns:TimeProperInterval ;
    linkml:slot_uri time:intervalDisjoint .

okns:Daml-countryCountry a linkml:ClassDefinition ;
    dcterms:title "Country" ;
    skos:definition "High level country concept." ;
    skos:inScheme okns:daml ;
    skos:mappingRelation daml-country:Country ;
    linkml:class_uri daml-country:Country ;
    linkml:definition_uri okns:Daml-countryCountry ;
    linkml:is_a okns:Daml-profileLocation ;
    linkml:slot_usage [ ] .

okns:Daml-iso3166Country a linkml:ClassDefinition ;
    skos:inScheme okns:daml ;
    skos:mappingRelation daml-iso3166:Country ;
    linkml:class_uri daml-iso3166:Country ;
    linkml:definition_uri okns:Daml-iso3166Country ;
    linkml:is_a okns:Daml-country-ontCountry ;
    linkml:slot_usage [ ] ;
    linkml:slots okns:daml_iso3166_code,
        okns:daml_iso3166_name .

okns:Daml-oilUniqueProperty a linkml:ClassDefinition ;
    dcterms:title "UniqueProperty" ;
    skos:definition "compare with maxCardinality=1; e.g. integer successor: if P is a UniqueProperty, then if P(x, y) and P(x, z) then y=z. cf OIL FunctionalProperty." ;
    skos:inScheme okns:daml ;
    skos:mappingRelation daml-oil:UniqueProperty ;
    linkml:class_uri daml-oil:UniqueProperty ;
    linkml:definition_uri okns:Daml-oilUniqueProperty ;
    linkml:is_a okns:RdfProperty ;
    linkml:slot_usage [ ] ;
    linkml:slots okns:daml_oil_domain,
        okns:daml_oil_range .

okns:Daml-ontUSRegion a linkml:ClassDefinition ;
    skos:inScheme okns:daml ;
    skos:mappingRelation daml-ont:USRegion ;
    linkml:class_uri daml-ont:USRegion ;
    linkml:definition_uri okns:Daml-ontUSRegion ;
    linkml:slot_usage [ ] ;
    linkml:slots okns:daml_ont_memberstate,
        okns:rdfs_label .

okns:IcalValueDATE-TIME a linkml:ClassDefinition ;
    skos:inScheme okns:ical ;
    skos:mappingRelation ical:Value_DATE-TIME ;
    linkml:class_uri ical:Value_DATE-TIME ;
    linkml:definition_uri okns:IcalValueDATE-TIME ;
    linkml:slot_usage [ ] .

okns:MoArrangement a linkml:ClassDefinition ;
    dcterms:source <http://purl.org/ontology/mo/> ;
    dcterms:title "arrangement" ;
    skos:definition "An arrangement event.␊        Takes as agent the arranger, and produces a score (informational object, not the actually published score)." ;
    skos:inScheme okns:mo ;
    skos:mappingRelation ns1:Arrangement ;
    linkml:class_uri <http://purl.org/ontology/mo/Arrangement> ;
    linkml:definition_uri okns:MoArrangement ;
    linkml:is_a okns:EventEvent ;
    linkml:slot_usage [ ] .

okns:MoDigitalSignal a linkml:ClassDefinition ;
    dcterms:source <http://purl.org/ontology/mo/> ;
    dcterms:title "digital signal" ;
    skos:definition "A digital signal" ;
    skos:inScheme okns:mo ;
    skos:mappingRelation ns1:DigitalSignal ;
    linkml:class_uri <http://purl.org/ontology/mo/DigitalSignal> ;
    linkml:definition_uri okns:MoDigitalSignal ;
    linkml:is_a okns:MoSignal ;
    linkml:slot_usage [ ] .

okns:MoRecord a linkml:ClassDefinition ;
    dcterms:source <http://purl.org/ontology/mo/> ;
    dcterms:title "record" ;
    skos:definition "A published record (manifestation which first aim is to render the product of a recording)" ;
    skos:inScheme okns:mo ;
    skos:mappingRelation ns1:Record ;
    linkml:class_uri <http://purl.org/ontology/mo/Record> ;
    linkml:definition_uri okns:MoRecord ;
    linkml:is_a okns:MoMusicalManifestation ;
    linkml:slot_usage [ ] .

okns:MoTrack a linkml:ClassDefinition ;
    dcterms:source <http://purl.org/ontology/mo/> ;
    dcterms:title "track" ;
    skos:definition "A track on a particular record" ;
    skos:inScheme okns:mo ;
    skos:mappingRelation ns1:Track ;
    linkml:class_uri <http://purl.org/ontology/mo/Track> ;
    linkml:definition_uri okns:MoTrack ;
    linkml:is_a okns:MoMusicalManifestation ;
    linkml:slot_usage [ ] .

okns:OwlNegativePropertyAssertion a linkml:ClassDefinition ;
    dcterms:source owl: ;
    dcterms:title "NegativePropertyAssertion" ;
    skos:definition "The class of negative property assertions." ;
    skos:inScheme okns:owl-rdf-rdfs ;
    skos:mappingRelation owl:NegativePropertyAssertion ;
    linkml:class_uri owl:NegativePropertyAssertion ;
    linkml:definition_uri okns:OwlNegativePropertyAssertion ;
    linkml:is_a okns:RdfsResource ;
    linkml:slot_usage [ ] .

okns:Time-entryInstantThingPair a linkml:ClassDefinition ;
    skos:inScheme okns:daml ;
    skos:mappingRelation time-entry:InstantThingPair ;
    linkml:class_uri time-entry:InstantThingPair ;
    linkml:definition_uri okns:Time-entryInstantThingPair ;
    linkml:slot_usage [ ] .

okns:TimeTemporalDuration a linkml:ClassDefinition ;
    dcterms:title "Temporal duration" ;
    skos:definition "Time extent; duration of a time interval separate from its particular start position" ;
    skos:inScheme okns:time ;
    skos:mappingRelation time:TemporalDuration ;
    skos:note "description: Extensión de tiempo; duración de un intervalo de tiempo independiente de su posición de inicio particular.",
        "description: Time extent; duration of a time interval separate from its particular start position",
        "title: duración temporal" ;
    linkml:class_uri time:TemporalDuration ;
    linkml:definition_uri okns:TimeTemporalDuration ;
    linkml:slot_usage [ ] .

okns:WotSigEvent a linkml:ClassDefinition ;
    dcterms:source wot: ;
    dcterms:title "Key Signing Event" ;
    skos:definition "An event describing the action of a public key being signed by some other public key." ;
    skos:inScheme okns:wot ;
    skos:mappingRelation wot:SigEvent ;
    linkml:class_uri wot:SigEvent ;
    linkml:definition_uri okns:WotSigEvent ;
    linkml:is_a okns:Wn16Event ;
    linkml:slot_usage [ ] .

okns:XsdDuration a linkml:ClassDefinition ;
    dcterms:title "No class (entity type) name specified -- this class is noted as being in the domain or range of a slot in this graph but has not itself been defined." ;
    skos:inScheme okns:time ;
    skos:mappingRelation xsd:duration ;
    linkml:class_uri xsd:duration ;
    linkml:definition_uri okns:XsdDuration ;
    linkml:slot_usage [ ] .

okns:event_isAgentIn a linkml:SlotDefinition ;
    dcterms:title "agent in" ;
    skos:editorialNote "No occurrences of this slot in the graph." ;
    skos:exactMatch event:agent_in ;
    skos:inScheme okns:event ;
    skos:mappingRelation event:isAgentIn ;
    linkml:definition_uri okns:event_isAgentIn ;
    linkml:inlined true ;
    linkml:range okns:Any ;
    linkml:slot_uri event:isAgentIn .

okns:foaf_depiction a linkml:SlotDefinition ;
    dcterms:source foaf: ;
    dcterms:title "depiction" ;
    owl:inverseOf okns:foaf_depicts ;
    skos:definition "A depiction of some thing." ;
    skos:editorialNote "No occurrences of this slot in the graph." ;
    skos:inScheme okns:foaf ;
    skos:mappingRelation foaf:depiction ;
    linkml:definition_uri okns:foaf_depiction ;
    linkml:domain okns:OwlThing ;
    linkml:inlined true ;
    linkml:owner okns:foaf_depiction ;
    linkml:range okns:FoafImage ;
    linkml:slot_uri foaf:depiction .

okns:int32 a linkml:TypeDefinition ;
    rdfs:seeAlso <https://numpy.org/doc/stable/reference/arrays.scalars.html#numpy.intc> ;
    skos:altLabel "i",
        "intc" ;
    skos:definition "A 32-bit signed integer" ;
    skos:inScheme okns:extended_types ;
    skos:note "uri added by Mahir Morshed <mmorshed@scripps.edu>" ;
    linkml:base "int" ;
    linkml:definition_uri linkml:Int32 ;
    linkml:maximum_value "2147483647"^^<https://purl.org/okn/schema/@id> ;
    linkml:minimum_value "-2147483648"^^<https://purl.org/okn/schema/@id> ;
    linkml:typeof okns:signedinteger ;
    linkml:uri xsd:int .

okns:mo_performer a linkml:SlotDefinition ;
    dcterms:source <http://purl.org/ontology/mo/> ;
    dcterms:title "No slot (predicate) name specified -- this slot is noted as a subproperty of another slot in this graph but has not itself been defined." ;
    rdfs:subPropertyOf okns:event_agent ;
    owl:inverseOf okns:mo_performed ;
    skos:definition "Relates a performance to the performers involved" ;
    skos:editorialNote "No occurrences of this slot in the graph." ;
    skos:inScheme okns:mo ;
    skos:mappingRelation <http://purl.org/ontology/mo/performer> ;
    linkml:definition_uri okns:mo_performer ;
    linkml:domain okns:MoPerformance ;
    linkml:inlined true ;
    linkml:owner okns:mo_performer ;
    linkml:range okns:FoafAgent ;
    linkml:slot_uri <http://purl.org/ontology/mo/performer> .

okns:time_intervalIn a linkml:SlotDefinition ;
    dcterms:title "interval in" ;
    skos:definition "If a proper interval T1 is intervalIn another proper interval T2, then the beginning of T1 is after the beginning of T2 or is coincident with the beginning of T2, and the end of T1 is before the end of T2, or is coincident with the end of T2, except that end of T1 may not be coincident with the end of T2 if the beginning of T1 is coincident with the beginning of T2." ;
    skos:editorialNote "Esta relación entre intervalos no estaba incluida en las 13 relaciones básicas definidas por Allen (1984), pero se hace referencia a ella como \"una relación importante\" en Allen y Ferguson (1997). Es la unión disjunta de 'intervalo empieza', 'intervalo durante' y con 'intervalo termina'. Sin embargo, esto está fuera de la expresividad de OWL2, por tanto, se implementa como una propiedad explícita, con 'intervalo empieza', 'intervalo durante' e 'intervalo termina' como sub-propiedades.",
        "No occurrences of this slot in the graph.",
        "This interval relation is not included in the 13 basic relationships defined in Allen (1984), but is referred to as 'an important relationship' in Allen and Ferguson (1997). It is the disjoint union of :intervalStarts v :intervalDuring v :intervalFinishes . However, that is outside OWL2 expressivity, so is implemented as an explicit property, with :intervalStarts , :intervalDuring , :intervalFinishes as sub-properties" ;
    skos:inScheme okns:time ;
    skos:mappingRelation time:intervalIn ;
    skos:note "description: If a proper interval T1 is intervalIn another proper interval T2, then the beginning of T1 is after the beginning of T2 or is coincident with the beginning of T2, and the end of T1 is before the end of T2, or is coincident with the end of T2, except that end of T1 may not be coincident with the end of T2 if the beginning of T1 is coincident with the beginning of T2.",
        "description: Si un intervalo propio T1 es un intervalo interior a otro intervalo propio T2, entonces el principio de T1 está después del principio de T2 o coincide con el principio de T2, y el final de T1 está antes que el final de T2, o coincide con el final de T2, excepto que el final de T1 puede no coincidir con el final de T2 si el principio de T1 coincide con el principio de T2.",
        "title: intervalo interior" ;
    linkml:definition_uri okns:time_intervalIn ;
    linkml:domain okns:TimeProperInterval ;
    linkml:inlined true ;
    linkml:owner okns:time_intervalIn ;
    linkml:range okns:TimeProperInterval ;
    linkml:slot_uri time:intervalIn .

okns:CcRequirement a linkml:ClassDefinition ;
    dcterms:title "requirement" ;
    skos:definition "an action that may or may not be requested of you" ;
    skos:inScheme okns:cc ;
    skos:mappingRelation cc:Requirement ;
    linkml:class_uri cc:Requirement ;
    linkml:definition_uri okns:CcRequirement ;
    linkml:slot_usage [ ] ;
    linkml:slots okns:dc_description,
        okns:dc_title .

okns:Daml-ontCountry a linkml:ClassDefinition ;
    skos:inScheme okns:daml ;
    skos:mappingRelation daml-ont:Country ;
    linkml:class_uri daml-ont:Country ;
    linkml:definition_uri okns:Daml-ontCountry ;
    linkml:slot_usage [ ] ;
    linkml:slots okns:daml_ont_cia,
        okns:daml_ont_name,
        okns:daml_sameClassAs .

okns:DctAgentClass a linkml:ClassDefinition ;
    dcterms:source dcterms: ;
    dcterms:title "Agent Class" ;
    skos:definition "A group of agents." ;
    skos:inScheme okns:dc ;
    skos:mappingRelation dcterms:AgentClass ;
    linkml:class_uri dcterms:AgentClass ;
    linkml:definition_uri okns:DctAgentClass ;
    linkml:is_a okns:RdfsClass ;
    linkml:slot_usage [ ] ;
    linkml:slots okns:dct_issued,
        okns:rdfs_comment,
        okns:rdfs_isDefinedBy,
        okns:rdfs_label .

okns:MoMusicalItem a linkml:ClassDefinition ;
    dcterms:source <http://purl.org/ontology/mo/> ;
    dcterms:title "MusicalItem" ;
    skos:definition "A single exemplar of a musical expression.␊    ␊For example, it could be a single exemplar of a CD. This is normally an single object (a CD) possessed by somebody.␊␊From the FRBR final report: The entity defined as item is a concrete entity. It is in many instances a single physical object (e.g., a copy of a one-volume monograph, a single audio cassette, etc.). There are instances, however, where the entity defined as item comprises more than one physical object (e.g., a monograph issued as two separately bound volumes, a recording issued on three separate compact discs, etc.).␊␊In terms of intellectual content and physical form, an item exemplifying a manifestation is normally the same as the manifestation itself. However, variations may occur from one item to another, even when the items exemplify the same manifestation, where those variations are the result of actions external to the intent of the producer of the manifestation (e.g., damage occurring after the item was produced, binding performed by a library, etc.)." ;
    skos:inScheme okns:mo ;
    skos:mappingRelation ns1:MusicalItem ;
    linkml:class_uri <http://purl.org/ontology/mo/MusicalItem> ;
    linkml:definition_uri okns:MoMusicalItem ;
    linkml:slot_usage [ ] .

okns:MoReleaseStatus a linkml:ClassDefinition ;
    dcterms:source <http://purl.org/ontology/mo/> ;
    dcterms:title "release status" ;
    skos:definition "Musical manifestation release status." ;
    skos:inScheme okns:mo ;
    skos:mappingRelation ns1:ReleaseStatus ;
    linkml:class_uri <http://purl.org/ontology/mo/ReleaseStatus> ;
    linkml:definition_uri okns:MoReleaseStatus ;
    linkml:slot_usage [ ] ;
    linkml:slots okns:dc_description,
        okns:dc_title,
        okns:mo_level,
        okns:rdfs_isDefinedBy .

okns:TzontPoliticalRegion a linkml:ClassDefinition ;
    skos:inScheme okns:daml ;
    skos:mappingRelation tzont:PoliticalRegion ;
    linkml:class_uri tzont:PoliticalRegion ;
    linkml:definition_uri okns:TzontPoliticalRegion ;
    linkml:is_a okns:TzontRegion ;
    linkml:slot_usage [ ] .

okns:float a linkml:TypeDefinition ;
    skos:definition "A real number that conforms to the xsd:float specification" ;
    skos:editorialNote "If you are authoring schemas in LinkML YAML, the type is referenced with the lower case \"float\"." ;
    skos:exactMatch schema1:Float ;
    skos:inScheme linkml:types ;
    linkml:base "float" ;
    linkml:imported_from "linkml:types" ;
    linkml:definition_uri linkml:Float ;
    linkml:uri xsd:float .

okns:foaf_nick a linkml:SlotDefinition ;
    dcterms:source foaf: ;
    dcterms:title "nickname" ;
    skos:definition "A short informal nickname characterising an agent (includes login identifiers, IRC and other chat nicknames)." ;
    skos:editorialNote "No occurrences of this slot in the graph." ;
    skos:inScheme okns:foaf ;
    skos:mappingRelation foaf:nick ;
    linkml:definition_uri okns:foaf_nick ;
    linkml:inlined true ;
    linkml:range okns:Any ;
    linkml:slot_uri foaf:nick .

okns:foaf_page a linkml:SlotDefinition ;
    dcterms:source foaf: ;
    dcterms:title "page" ;
    owl:inverseOf okns:foaf_topic ;
    skos:definition "A page or document about this thing." ;
    skos:editorialNote "No occurrences of this slot in the graph." ;
    skos:inScheme okns:foaf ;
    skos:mappingRelation foaf:page ;
    linkml:definition_uri okns:foaf_page ;
    linkml:domain okns:OwlThing ;
    linkml:inlined true ;
    linkml:owner okns:foaf_page ;
    linkml:range okns:FoafDocument ;
    linkml:slot_uri foaf:page .

okns:rdfs_seeAlso a linkml:SlotDefinition ;
    dcterms:source rdfs: ;
    dcterms:title "seeAlso" ;
    skos:definition "Further information about the subject resource." ;
    skos:inScheme okns:owl-rdf-rdfs ;
    skos:mappingRelation rdfs:seeAlso ;
    linkml:any_of [ a okns:AnonymousSlotExpression ;
            linkml:range okns:RdfsResource ],
        [ a okns:AnonymousSlotExpression ;
            linkml:range okns:uri ] ;
    linkml:definition_uri okns:rdfs_seeAlso ;
    linkml:domain okns:RdfsResource ;
    linkml:domain_of okns:DcamVocabularyEncodingScheme,
        okns:RdfsDatatype ;
    linkml:inlined true ;
    linkml:owner okns:rdfs_seeAlso ;
    linkml:range okns:Any ;
    linkml:slot_uri rdfs:seeAlso .

okns:skos_semanticRelation a linkml:SlotDefinition ;
    dcterms:source <http://www.w3.org/2004/02/skos/core> ;
    dcterms:title "is in semantic relation with" ;
    skos:definition "Links a concept to a concept related by meaning." ;
    skos:editorialNote "No occurrences of this slot in the graph.",
        "This property should not be used directly, but as a super-property for all properties denoting a relationship of meaning between concepts." ;
    skos:inScheme okns:skos ;
    skos:mappingRelation skos:semanticRelation ;
    linkml:definition_uri okns:skos_semanticRelation ;
    linkml:domain okns:SkosConcept ;
    linkml:inlined true ;
    linkml:owner okns:skos_semanticRelation ;
    linkml:range okns:SkosConcept ;
    linkml:slot_uri skos:semanticRelation .

okns:time_entry_nonoverlap a linkml:SlotDefinition ;
    dcterms:title "No slot (predicate) name specified -- this slot is noted as a subproperty of another slot in this graph but has not itself been defined." ;
    skos:editorialNote "No occurrences of this slot in the graph." ;
    skos:inScheme okns:daml ;
    skos:mappingRelation time-entry:nonoverlap ;
    linkml:definition_uri okns:time_entry_nonoverlap ;
    linkml:domain okns:Time-entryProperIntervalThing ;
    linkml:inlined true ;
    linkml:owner okns:time_entry_nonoverlap ;
    linkml:range okns:Time-entryProperIntervalThing ;
    linkml:slot_uri time-entry:nonoverlap .

okns:Daml-2001Ontology a linkml:ClassDefinition ;
    skos:inScheme okns:daml ;
    skos:mappingRelation daml-2001:Ontology ;
    linkml:class_uri daml-2001:Ontology ;
    linkml:definition_uri okns:Daml-2001Ontology ;
    linkml:slot_usage [ ] ;
    linkml:slots okns:daml_2001_imports,
        okns:daml_2001_versionInfo .

okns:Daml-oilOntology a linkml:ClassDefinition ;
    dcterms:title "Ontology" ;
    skos:definition "An Ontology is a document that describes a vocabulary of terms for communication between (human and) automated agents." ;
    skos:inScheme okns:daml ;
    skos:mappingRelation daml-oil:Ontology ;
    linkml:class_uri daml-oil:Ontology ;
    linkml:definition_uri okns:Daml-oilOntology ;
    linkml:slot_usage [ ] ;
    linkml:slots okns:daml_oil_comment,
        okns:daml_oil_imports,
        okns:daml_oil_versionInfo .

okns:DamlOntology a linkml:ClassDefinition ;
    skos:inScheme okns:daml ;
    skos:mappingRelation daml:Ontology ;
    linkml:class_uri daml:Ontology ;
    linkml:definition_uri okns:DamlOntology ;
    linkml:slot_usage [ ] ;
    linkml:slots okns:daml_imports,
        okns:daml_versionInfo,
        okns:rdfs_comment .

okns:DcamVocabularyEncodingScheme a linkml:ClassDefinition ;
    dcterms:source dcam: ;
    dcterms:title "Vocabulary Encoding Scheme" ;
    rdfs:seeAlso <https://www.dublincore.org/specifications/dublin-core/2007/06/04/abstract-model/> ;
    skos:definition "An enumerated set of resources." ;
    skos:inScheme okns:dc ;
    skos:mappingRelation dcam:VocabularyEncodingScheme ;
    linkml:class_uri dcam:VocabularyEncodingScheme ;
    linkml:definition_uri okns:DcamVocabularyEncodingScheme ;
    linkml:slot_usage [ ] ;
    linkml:slots okns:dct_issued,
        okns:rdfs_comment,
        okns:rdfs_isDefinedBy,
        okns:rdfs_label,
        okns:rdfs_seeAlso .

okns:FoafImage a linkml:ClassDefinition ;
    dcterms:source foaf: ;
    dcterms:title "Image" ;
    skos:definition "An image." ;
    skos:inScheme okns:foaf ;
    skos:mappingRelation foaf:Image ;
    linkml:class_uri foaf:Image ;
    linkml:definition_uri okns:FoafImage ;
    linkml:is_a okns:FoafDocument ;
    linkml:slot_usage [ ] .

okns:FrbrWork a linkml:ClassDefinition ;
    dcterms:source frbr: ;
    dcterms:title "work" ;
    skos:definition "An abstract notion of an artistic or intellectual creation." ;
    skos:editorialNote "N7e49ec98377c446d93042554eed74edb",
        "N8f74280acd0d446682229c09b9af1b16",
        "Nd7448abd61bb479c859fd8287b17d96e",
        "Ndf107e4b600e4f2991ce940e0790130b" ;
    skos:inScheme okns:frbr ;
    skos:mappingRelation frbr:Work ;
    skos:note "description: This class corresponds to the FRBR group one entity 'Work'." ;
    linkml:class_uri frbr:Work ;
    linkml:definition_uri okns:FrbrWork ;
    linkml:is_a <https://purl.org/okn/schema/Wn16Work~2> ;
    linkml:slot_usage [ ] .

okns:MoReleaseType a linkml:ClassDefinition ;
    dcterms:source <http://purl.org/ontology/mo/> ;
    dcterms:title "Release type" ;
    skos:definition "Release type of a particular manifestation, such as \"album\" or \"interview\"..." ;
    skos:inScheme okns:mo ;
    skos:mappingRelation ns1:ReleaseType ;
    linkml:class_uri <http://purl.org/ontology/mo/ReleaseType> ;
    linkml:definition_uri okns:MoReleaseType ;
    linkml:slot_usage [ ] ;
    linkml:slots okns:dc_description,
        okns:dc_title,
        okns:mo_level,
        okns:rdfs_isDefinedBy .

okns:SimAssociationMethod a linkml:ClassDefinition ;
    dcterms:source sim: ;
    dcterms:title "Association Method" ;
    skos:definition "A concept for representing the method used to derive association or similarity statements." ;
    skos:inScheme okns:sim ;
    skos:mappingRelation sim:AssociationMethod ;
    linkml:class_uri sim:AssociationMethod ;
    linkml:definition_uri okns:SimAssociationMethod ;
    linkml:is_a okns:OwlThing ;
    linkml:slot_usage [ ] .

okns:SkosConcept a linkml:ClassDefinition ;
    dcterms:source <http://www.w3.org/2004/02/skos/core> ;
    dcterms:title "Concept" ;
    skos:definition "An idea or notion; a unit of thought." ;
    skos:inScheme okns:skos ;
    skos:mappingRelation skos:Concept ;
    linkml:class_uri skos:Concept ;
    linkml:definition_uri okns:SkosConcept ;
    linkml:slot_usage [ ] .

okns:Xsd2000NonNegativeInteger a linkml:ClassDefinition ;
    dcterms:title "No class (entity type) name specified -- this class is noted as being in the domain or range of a slot in this graph but has not itself been defined." ;
    skos:inScheme okns:daml ;
    skos:mappingRelation xsd2000:nonNegativeInteger ;
    linkml:class_uri xsd2000:nonNegativeInteger ;
    linkml:definition_uri okns:Xsd2000NonNegativeInteger ;
    linkml:slot_usage [ ] .

okns:ao_context a linkml:SlotDefinition ;
    dcterms:source ao: ;
    dcterms:title "has context" ;
    skos:definition "A property to associate any environmental context to an individual, e.g. a location, a time or an activity. Hence, this property is intended that sub properties should be created from it." ;
    skos:editorialNote "No occurrences of this slot in the graph." ;
    skos:inScheme okns:ao ;
    skos:mappingRelation ao:context ;
    linkml:definition_uri okns:ao_context ;
    linkml:domain okns:OwlThing ;
    linkml:inlined true ;
    linkml:owner okns:ao_context ;
    linkml:range okns:Any ;
    linkml:slot_uri ao:context .

okns:daml_oil_domain a linkml:SlotDefinition ;
    skos:inScheme okns:daml ;
    skos:mappingRelation daml-oil:domain ;
    linkml:any_of [ a okns:AnonymousSlotExpression ;
            linkml:range okns:uri ],
        [ a okns:AnonymousSlotExpression ;
            linkml:range okns:Daml-oilClass ] ;
    linkml:definition_uri okns:daml_oil_domain ;
    linkml:domain_of okns:Daml-oilDatatypeProperty,
        okns:Daml-oilObjectProperty,
        okns:Daml-oilProperty,
        okns:Daml-oilUniqueProperty ;
    linkml:inlined true ;
    linkml:owner okns:Daml-oilUniqueProperty ;
    linkml:range okns:Any ;
    linkml:slot_uri daml-oil:domain .

okns:daml_oil_range a linkml:SlotDefinition ;
    skos:inScheme okns:daml ;
    skos:mappingRelation daml-oil:range ;
    linkml:any_of [ a okns:AnonymousSlotExpression ;
            linkml:range okns:Daml-2001Class ],
        [ a okns:AnonymousSlotExpression ;
            linkml:range okns:Daml-oilClass ],
        [ a okns:AnonymousSlotExpression ;
            linkml:range okns:RdfsClass ],
        [ a okns:AnonymousSlotExpression ;
            linkml:range okns:uri ] ;
    linkml:definition_uri okns:daml_oil_range ;
    linkml:domain_of okns:Daml-oilDatatypeProperty,
        okns:Daml-oilObjectProperty,
        okns:Daml-oilProperty,
        okns:Daml-oilUniqueProperty ;
    linkml:inlined true ;
    linkml:owner okns:Daml-oilUniqueProperty ;
    linkml:range okns:Any ;
    linkml:slot_uri daml-oil:range .

okns:event_factor a linkml:SlotDefinition ;
    dcterms:title "factor" ;
    owl:inverseOf okns:event_factor_of ;
    skos:definition "Relates an event to a passive factor (a tool, an instrument, an abstract cause...)" ;
    skos:editorialNote "No occurrences of this slot in the graph." ;
    skos:exactMatch event:hasFactor ;
    skos:inScheme okns:event ;
    skos:mappingRelation event:factor ;
    linkml:definition_uri okns:event_factor ;
    linkml:domain okns:EventEvent ;
    linkml:inlined true ;
    linkml:owner okns:event_factor ;
    linkml:range okns:Any ;
    linkml:slot_uri event:factor .

okns:frbr_responsibleEntity a linkml:SlotDefinition ;
    dcterms:source frbr: ;
    dcterms:title "responsible entity" ;
    owl:inverseOf okns:frbr_responsibleEntityOf ;
    skos:definition "An entity in some way responsible for an endeavour." ;
    skos:editorialNote "Ncec984f0def64ac981f73592bf1c4802",
        "Nfff80747af3d4aa89f6030a61ed76949",
        "No occurrences of this slot in the graph." ;
    skos:inScheme okns:frbr ;
    skos:mappingRelation frbr:responsibleEntity ;
    linkml:definition_uri okns:frbr_responsibleEntity ;
    linkml:domain okns:FrbrEndeavour ;
    linkml:inlined true ;
    linkml:owner okns:frbr_responsibleEntity ;
    linkml:range okns:FrbrResponsibleEntity ;
    linkml:slot_uri frbr:responsibleEntity .

okns:frbr_responsibleEntityOf a linkml:SlotDefinition ;
    dcterms:source frbr: ;
    dcterms:title "responsible entity of" ;
    owl:inverseOf okns:frbr_responsibleEntity ;
    skos:definition "An endeavour that is the responsibility of an entity." ;
    skos:editorialNote "N82257a5f524c424b9a99dd15e38f52c5",
        "Ncd498d5bd69546f4a0e3819069a5d05e",
        "No occurrences of this slot in the graph." ;
    skos:inScheme okns:frbr ;
    skos:mappingRelation frbr:responsibleEntityOf ;
    linkml:definition_uri okns:frbr_responsibleEntityOf ;
    linkml:domain okns:FrbrResponsibleEntity ;
    linkml:inlined true ;
    linkml:owner okns:frbr_responsibleEntityOf ;
    linkml:range okns:FrbrEndeavour ;
    linkml:slot_uri frbr:responsibleEntityOf .

okns:skos_note a linkml:SlotDefinition ;
    dcterms:source <http://www.w3.org/2004/02/skos/core> ;
    dcterms:title "note" ;
    skos:definition "A general note, for any purpose." ;
    skos:editorialNote "No occurrences of this slot in the graph.",
        "This property may be used directly, or as a super-property for more specific note types." ;
    skos:inScheme okns:skos ;
    skos:mappingRelation skos:note ;
    linkml:definition_uri okns:skos_note ;
    linkml:inlined true ;
    linkml:range okns:Any ;
    linkml:slot_uri skos:note .

okns:CcLicense a linkml:ClassDefinition ;
    dcterms:title "license" ;
    skos:definition "a set of requests/permissions to users of a Work, e.g. a copyright license, the public domain, information for distributors" ;
    skos:inScheme okns:cc ;
    skos:mappingRelation cc:License ;
    linkml:class_uri cc:License ;
    linkml:definition_uri okns:CcLicense ;
    linkml:slot_usage [ ] ;
    linkml:slots okns:dc_description,
        okns:dc_title .

okns:Daml-2001Property a linkml:ClassDefinition ;
    skos:inScheme okns:daml ;
    skos:mappingRelation daml-2001:Property ;
    linkml:class_uri daml-2001:Property ;
    linkml:definition_uri okns:Daml-2001Property ;
    linkml:slot_usage [ ] ;
    linkml:slots okns:daml_2001_comment,
        okns:rdfs_comment,
        okns:rdfs_domain,
        okns:rdfs_label,
        okns:rdfs_range,
        okns:rdfs_subPropertyOf .

okns:Daml-stateState a linkml:ClassDefinition ;
    dcterms:title "State" ;
    skos:definition "Information about some geographic region, such as a US state." ;
    skos:inScheme okns:daml ;
    skos:mappingRelation daml-state:State ;
    linkml:class_uri daml-state:State ;
    linkml:definition_uri okns:Daml-stateState ;
    linkml:is_a okns:Daml-oilThing ;
    linkml:slot_usage [ ] .

okns:FoafOnlineAccount a linkml:ClassDefinition ;
    dcterms:source foaf: ;
    dcterms:title "Online Account" ;
    skos:definition "An online account." ;
    skos:inScheme okns:foaf ;
    skos:mappingRelation foaf:OnlineAccount ;
    linkml:class_uri foaf:OnlineAccount ;
    linkml:definition_uri okns:FoafOnlineAccount ;
    linkml:is_a okns:OwlThing ;
    linkml:slot_usage [ ] .

okns:FrbrEndeavour a linkml:ClassDefinition ;
    dcterms:source frbr: ;
    dcterms:title "endeavour" ;
    skos:definition "Any of the products of artistic or creative endeavour." ;
    skos:editorialNote "N8dd72b6b9eff45c298d4dc53e52e655c",
        "Nbe61b733e4e64a7e9324081b37b42673",
        "Nff7df09854724fa98fbdb2752d248d03" ;
    skos:inScheme okns:frbr ;
    skos:mappingRelation frbr:Endeavour ;
    skos:note "description: This class represents any one of the FRBR group one entities." ;
    linkml:class_uri frbr:Endeavour ;
    linkml:definition_uri okns:FrbrEndeavour ;
    linkml:slot_usage [ ] .

okns:date a linkml:TypeDefinition ;
    skos:definition "a date (year, month and day) in an idealized calendar" ;
    skos:editorialNote "If you are authoring schemas in LinkML YAML, the type is referenced with the lower case \"date\".",
        "URI is dateTime because OWL reasoners don't work with straight date or time" ;
    skos:exactMatch schema1:Date ;
    skos:inScheme linkml:types ;
    linkml:base "XSDDate" ;
    linkml:imported_from "linkml:types" ;
    linkml:repr "str" ;
    linkml:definition_uri linkml:Date ;
    linkml:uri xsd:date .

okns:dc_description a linkml:SlotDefinition ;
    dcterms:source dc: ;
    dcterms:title "Description" ;
    skos:definition "Description may include but is not limited to: an abstract, a table of contents, a graphical representation, or a free-text account of the resource." ;
    skos:editorialNote "A [second property](/specifications/dublin-core/dcmi-terms/#http://purl.org/dc/terms/description) with the same name as this property has been declared in the [dcterms: namespace](http://purl.org/dc/terms/).  See the Introduction to the document [DCMI Metadata Terms](/specifications/dublin-core/dcmi-terms/) for an explanation.",
        "No occurrences of this slot in the graph." ;
    skos:inScheme okns:dc ;
    skos:mappingRelation dc:description ;
    skos:note "description: An account of the resource." ;
    linkml:definition_uri okns:dc_description ;
    linkml:domain_of okns:CcLicense,
        okns:CcPermission,
        okns:CcProhibition,
        okns:CcRequirement,
        okns:MoReleaseStatus,
        okns:MoReleaseType ;
    linkml:inlined true ;
    linkml:owner okns:CcRequirement ;
    linkml:range okns:Any ;
    linkml:slot_uri dc:description .

okns:event_agent a linkml:SlotDefinition ;
    dcterms:title "agent" ;
    owl:inverseOf okns:event_agent_in ;
    skos:definition "Relates an event to an active agent (a person, a computer, ... :-) )" ;
    skos:editorialNote "No occurrences of this slot in the graph." ;
    skos:exactMatch event:hasAgent ;
    skos:inScheme okns:event ;
    skos:mappingRelation event:agent ;
    linkml:definition_uri okns:event_agent ;
    linkml:domain okns:EventEvent ;
    linkml:inlined true ;
    linkml:owner okns:event_agent ;
    linkml:range okns:FoafAgent ;
    linkml:slot_uri event:agent .

okns:Daml-oilList a linkml:ClassDefinition ;
    skos:inScheme okns:daml ;
    skos:mappingRelation daml-oil:List ;
    linkml:class_uri daml-oil:List ;
    linkml:definition_uri okns:Daml-oilList ;
    linkml:is_a okns:RdfSeq ;
    linkml:slot_usage [ ] .

okns:MoMusicalExpression a linkml:ClassDefinition ;
    dcterms:source <http://purl.org/ontology/mo/> ;
    dcterms:title "musical expression" ;
    skos:definition "The intellectual or artistic realization of a work in the form of alpha-numeric, musical, or choreographic notation, sound, etc., or any combination of such forms.    ␊␊␊For example:␊␊Work #1 Franz Schubert's Trout quintet␊␊    * Expression #1 the composer's score␊    * Expression #2 sound issued from the performance by the Amadeus Quartet and Hephzibah Menuhin on piano␊    * Expression #3 sound issued from the performance by the Cleveland Quartet and Yo-Yo Ma on the cello␊    * . . . . ␊␊The Music Ontology defines the following sub-concepts of a MusicalExpression, which should be used instead of MusicalExpression itself: Score (the␊result of an arrangement), Sound (produced during a performance), Signal. However, it is possible to stick to FRBR and bypass the worflow␊mechanism this ontology defines by using the core FRBR properties on such objects. But it is often better to use events to interconnect such ␊expressions (allowing to go deeply into the production process - `this performer was playing this particular instrument at that␊particular time')." ;
    skos:inScheme okns:mo ;
    skos:mappingRelation ns1:MusicalExpression ;
    linkml:class_uri <http://purl.org/ontology/mo/MusicalExpression> ;
    linkml:definition_uri okns:MoMusicalExpression ;
    linkml:is_a okns:FrbrExpression ;
    linkml:slot_usage [ ] .

okns:MoRelease a linkml:ClassDefinition ;
    dcterms:source <http://purl.org/ontology/mo/> ;
    dcterms:title "release" ;
    skos:definition "A specific release, with barcode, box, liner notes, cover art, and a number of records" ;
    skos:inScheme okns:mo ;
    skos:mappingRelation ns1:Release ;
    linkml:class_uri <http://purl.org/ontology/mo/Release> ;
    linkml:definition_uri okns:MoRelease ;
    linkml:is_a okns:MoMusicalManifestation ;
    linkml:slot_usage [ ] .

okns:OwlClass a linkml:ClassDefinition ;
    dcterms:source owl: ;
    dcterms:title "Class" ;
    skos:definition "The class of OWL classes." ;
    skos:inScheme okns:owl-rdf-rdfs ;
    skos:mappingRelation owl:Class ;
    linkml:class_uri owl:Class ;
    linkml:definition_uri okns:OwlClass ;
    linkml:is_a okns:RdfsClass ;
    linkml:slot_usage [ ] .

okns:RevReview a linkml:ClassDefinition ;
    dcterms:source rev: ;
    dcterms:title "Review" ;
    skos:definition "A review of an work" ;
    skos:inScheme okns:rev ;
    skos:mappingRelation rev:Review ;
    linkml:class_uri rev:Review ;
    linkml:definition_uri okns:RevReview ;
    linkml:slot_usage [ ] .

okns:Time-entryInstantThing a linkml:ClassDefinition ;
    dcterms:title "No class (entity type) name specified -- this class is noted as a superclass of another class in this graph but has not itself been defined." ;
    skos:inScheme okns:daml ;
    skos:mappingRelation time-entry:InstantThing ;
    linkml:class_uri time-entry:InstantThing ;
    linkml:definition_uri okns:Time-entryInstantThing ;
    linkml:is_a okns:Time-entryTemporalThing ;
    linkml:slot_usage [ ] .

okns:dc_title a linkml:SlotDefinition ;
    dcterms:source dc: ;
    dcterms:title "Title" ;
    skos:definition "A name given to the resource." ;
    skos:editorialNote "A [second property](/specifications/dublin-core/dcmi-terms/#http://purl.org/dc/terms/title) with the same name as this property has been declared in the [dcterms: namespace](http://purl.org/dc/terms/).  See the Introduction to the document [DCMI Metadata Terms](/specifications/dublin-core/dcmi-terms/) for an explanation.",
        "No occurrences of this slot in the graph." ;
    skos:inScheme okns:dc ;
    skos:mappingRelation dc:title ;
    linkml:definition_uri okns:dc_title ;
    linkml:domain_of okns:CcLicense,
        okns:CcPermission,
        okns:CcProhibition,
        okns:CcRequirement,
        okns:MoReleaseStatus,
        okns:MoReleaseType ;
    linkml:inlined true ;
    linkml:owner okns:CcRequirement ;
    linkml:range okns:Any ;
    linkml:slot_uri dc:title .

okns:dct_date a linkml:SlotDefinition ;
    dcterms:source dcterms: ;
    dcterms:title "Date" ;
    rdfs:subPropertyOf okns:dc_date ;
    skos:definition "Date may be used to express temporal information at any level of granularity.  Recommended practice is to express the date, date/time, or period of time according to ISO 8601-1 [[ISO 8601-1](https://www.iso.org/iso-8601-date-and-time-format.html)] or a published profile of the ISO standard, such as the W3C Note on Date and Time Formats [[W3CDTF](https://www.w3.org/TR/NOTE-datetime)] or the Extended Date/Time Format Specification [[EDTF](http://www.loc.gov/standards/datetime/)].  If the full date is unknown, month and year (YYYY-MM) or just year (YYYY) may be used. Date ranges may be specified using ISO 8601 period of time specification in which start and end dates are separated by a '/' (slash) character.  Either the start or end date may be missing." ;
    skos:editorialNote "No occurrences of this slot in the graph." ;
    skos:inScheme okns:dc ;
    skos:mappingRelation dcterms:date ;
    skos:note "description: A point or period of time associated with an event in the lifecycle of the resource." ;
    linkml:definition_uri okns:dct_date ;
    linkml:inlined true ;
    linkml:range okns:RdfsLiteral ;
    linkml:slot_uri dcterms:date .

okns:event_product a linkml:SlotDefinition ;
    dcterms:title "product" ;
    owl:inverseOf okns:event_produced_in ;
    skos:definition "Relates an event to something produced during the event---a sound, a pie, whatever..." ;
    skos:editorialNote "No occurrences of this slot in the graph." ;
    skos:exactMatch event:hasProduct ;
    skos:inScheme okns:event ;
    skos:mappingRelation event:product ;
    linkml:definition_uri okns:event_product ;
    linkml:domain okns:EventEvent ;
    linkml:inlined true ;
    linkml:owner okns:event_product ;
    linkml:range okns:Any ;
    linkml:slot_uri event:product .

okns:mo_derived_from a linkml:SlotDefinition ;
    dcterms:source <http://purl.org/ontology/mo/> ;
    dcterms:title "derived from" ;
    rdfs:subPropertyOf okns:dct_source ;
    skos:definition "A related signal from which the described signal is derived." ;
    skos:editorialNote "No occurrences of this slot in the graph." ;
    skos:inScheme okns:mo ;
    skos:mappingRelation <http://purl.org/ontology/mo/derived_from> ;
    linkml:definition_uri okns:mo_derived_from ;
    linkml:domain okns:MoSignal ;
    linkml:inlined true ;
    linkml:owner okns:mo_derived_from ;
    linkml:range okns:MoSignal ;
    linkml:slot_uri <http://purl.org/ontology/mo/derived_from> .

okns:rdfs_isDefinedBy a linkml:SlotDefinition ;
    dcterms:source rdfs: ;
    dcterms:title "isDefinedBy" ;
    rdfs:subPropertyOf okns:rdfs_seeAlso ;
    skos:definition "The definition of the subject resource." ;
    skos:inScheme okns:owl-rdf-rdfs ;
    skos:mappingRelation rdfs:isDefinedBy ;
    linkml:any_of [ a okns:AnonymousSlotExpression ;
            linkml:range okns:OwlOntology ],
        [ a okns:AnonymousSlotExpression ;
            linkml:range okns:RdfsResource ] ;
    linkml:definition_uri okns:rdfs_isDefinedBy ;
    linkml:domain okns:RdfsResource ;
    linkml:domain_of okns:DcamVocabularyEncodingScheme,
        okns:DctAgentClass,
        okns:MoReleaseStatus,
        okns:MoReleaseType,
        okns:RdfList,
        okns:RdfsDatatype ;
    linkml:inlined true ;
    linkml:owner okns:rdfs_isDefinedBy ;
    linkml:range okns:Any ;
    linkml:slot_uri rdfs:isDefinedBy .

okns:Daml-2001Class a linkml:ClassDefinition ;
    skos:inScheme okns:daml ;
    skos:mappingRelation daml-2001:Class ;
    linkml:class_uri daml-2001:Class ;
    linkml:definition_uri okns:Daml-2001Class ;
    linkml:slot_usage [ ] ;
    linkml:slots okns:daml_2001_complementOf,
        okns:daml_2001_unionOf,
        okns:rdfs_comment,
        okns:rdfs_label .

okns:Daml-oilObjectProperty a linkml:ClassDefinition ;
    dcterms:title "ObjectProperty" ;
    skos:definition "if P is an ObjectProperty, and P(x, y), then y is an object." ;
    skos:inScheme okns:daml ;
    skos:mappingRelation daml-oil:ObjectProperty ;
    linkml:class_uri daml-oil:ObjectProperty ;
    linkml:definition_uri okns:Daml-oilObjectProperty ;
    linkml:is_a okns:RdfProperty ;
    linkml:slot_usage [ ] ;
    linkml:slots okns:daml_oil_domain,
        okns:daml_oil_range,
        okns:daml_oil_subPropertyOf .

okns:MoMusicalWork a linkml:ClassDefinition ;
    dcterms:source <http://purl.org/ontology/mo/> ;
    dcterms:title "musical work" ;
    skos:definition "Distinct intellectual or artistic musical creation.␊    ␊From the FRBR final report: A work is an abstract entity; there is no single material object one can point to as the work. We recognize the work through individual realizations or expressions of the work, but the work itself exists only in the commonality of␊content between and among the various expressions of the work. When we speak of Homer's Iliad as a work, our point of reference is not a particular recitation or text of the work, but the intellectual creation that lies behind all the various expressions of the work.     ␊␊For example:␊␊work #1 J. S. Bach's The art of the fugue" ;
    skos:inScheme okns:mo ;
    skos:mappingRelation ns1:MusicalWork ;
    linkml:class_uri <http://purl.org/ontology/mo/MusicalWork> ;
    linkml:definition_uri okns:MoMusicalWork ;
    linkml:is_a okns:FrbrWork ;
    linkml:slot_usage [ ] .

okns:OwlObjectProperty a linkml:ClassDefinition ;
    dcterms:source owl: ;
    dcterms:title "ObjectProperty" ;
    skos:definition "The class of object properties." ;
    skos:inScheme okns:owl-rdf-rdfs ;
    skos:mappingRelation owl:ObjectProperty ;
    linkml:class_uri owl:ObjectProperty ;
    linkml:definition_uri okns:OwlObjectProperty ;
    linkml:is_a okns:RdfProperty ;
    linkml:slot_usage [ ] .

okns:Time-entryDurationDescription a linkml:ClassDefinition ;
    skos:inScheme okns:daml ;
    skos:mappingRelation time-entry:DurationDescription ;
    linkml:class_uri time-entry:DurationDescription ;
    linkml:definition_uri okns:Time-entryDurationDescription ;
    linkml:slot_usage [ ] .

okns:TimeGeneralDurationDescription a linkml:ClassDefinition ;
    dcterms:title "Generalized duration description" ;
    skos:definition "Description of temporal extent structured with separate values for the various elements of a calendar-clock system." ;
    skos:editorialNote "La extensión de una duración de tiempo expresada como una 'descripción de duración general' depende del Sistema de Referencia Temporal. En algunos calendarios la longitud de la semana o del mes no es constante a lo largo del año. Por tanto, un valor como \"25 meses\" puede no ser necesariamente ser comparado con un duración similar expresada en términos de semanas o días. Cuando se consideran calendarios que no están basados en el movimiento de la Tierra, se deben tomar incluso más precauciones en la comparación de duraciones.",
        "The extent of a time duration expressed as a GeneralDurationDescription depends on the Temporal Reference System. In some calendars the length of the week or month is not constant within the year. Therefore, a value like \"2.5 months\" may not necessarily be exactly compared with a similar duration expressed in terms of weeks or days. When non-earth-based calendars are considered even more care must be taken in comparing durations." ;
    skos:inScheme okns:time ;
    skos:mappingRelation time:GeneralDurationDescription ;
    skos:note "description: Descripción de extensión temporal estructurada con valores separados para los distintos elementos de un sistema de horario-calendario.",
        "description: Description of temporal extent structured with separate values for the various elements of a calendar-clock system.",
        "title: descripción de duración generalizada" ;
    linkml:class_uri time:GeneralDurationDescription ;
    linkml:definition_uri okns:TimeGeneralDurationDescription ;
    linkml:is_a okns:TimeTemporalDuration ;
    linkml:slot_usage [ ] .

okns:integer a linkml:TypeDefinition ;
    skos:definition "An integer" ;
    skos:editorialNote "If you are authoring schemas in LinkML YAML, the type is referenced with the lower case \"integer\"." ;
    skos:exactMatch schema1:Integer ;
    skos:inScheme linkml:types ;
    linkml:base "int" ;
    linkml:imported_from "linkml:types" ;
    linkml:definition_uri linkml:Integer ;
    linkml:uri xsd:integer .

okns:mo_uuid a linkml:SlotDefinition ;
    dcterms:title "universally unique identifier" ;
    rdfs:subPropertyOf okns:dct_identifier ;
    skos:definition "Links an object to an universally unique identifier for it." ;
    skos:editorialNote "No occurrences of this slot in the graph." ;
    skos:inScheme okns:mo ;
    skos:mappingRelation <http://purl.org/ontology/mo/uuid> ;
    linkml:definition_uri okns:mo_uuid ;
    linkml:domain okns:OwlThing ;
    linkml:inlined true ;
    linkml:owner okns:mo_uuid ;
    linkml:range okns:Any ;
    linkml:slot_uri <http://purl.org/ontology/mo/uuid> .

okns:TzontRegion a linkml:ClassDefinition ;
    skos:inScheme okns:daml ;
    skos:mappingRelation tzont:Region ;
    linkml:class_uri tzont:Region ;
    linkml:definition_uri okns:TzontRegion ;
    linkml:slot_usage [ ] .

okns:WotPubKey a linkml:ClassDefinition ;
    dcterms:source wot: ;
    dcterms:title "Public Key" ;
    skos:definition "A class used to represent a PGP/GPG public key for a user (an agent, person, group or organization)." ;
    skos:inScheme okns:wot ;
    skos:mappingRelation wot:PubKey ;
    linkml:class_uri wot:PubKey ;
    linkml:definition_uri okns:WotPubKey ;
    linkml:is_a okns:Wn16Credential ;
    linkml:slot_usage [ ] .

okns:Daml-oilRestriction a linkml:ClassDefinition ;
    dcterms:title "Restriction" ;
    skos:definition "something is in the class R if it satisfies the attached restrictions, and vice versa." ;
    skos:inScheme okns:daml ;
    skos:mappingRelation daml-oil:Restriction ;
    linkml:class_uri daml-oil:Restriction ;
    linkml:definition_uri okns:Daml-oilRestriction ;
    linkml:is_a okns:Daml-oilClass ;
    linkml:slot_usage [ ] ;
    linkml:slots okns:daml_oil_comment,
        okns:daml_oil_label,
        okns:daml_oil_subClassOf .

okns:FrbrManifestation a linkml:ClassDefinition ;
    dcterms:source frbr: ;
    dcterms:title "manifestation" ;
    skos:definition "The physical embodiment of one or more expressions." ;
    skos:editorialNote "N38f57c70af3a4cafa7d361b87333fde8",
        "N6446c020e94942fb85596d8d9e02451a",
        "Ne9807fb980274ede8d37a38c54c8908d" ;
    skos:inScheme okns:frbr ;
    skos:mappingRelation frbr:Manifestation ;
    skos:note "description: This class corresponds to the FRBR group one entity 'Manifestation'." ;
    linkml:class_uri frbr:Manifestation ;
    linkml:definition_uri okns:FrbrManifestation ;
    linkml:is_a okns:FrbrEndeavour ;
    linkml:slot_usage [ ] .

okns:FrbrResponsibleEntity a linkml:ClassDefinition ;
    dcterms:source frbr: ;
    dcterms:title "responsible entity" ;
    skos:definition "One responsible for the creation, production, distribution or maintenance of artistic or creative content." ;
    skos:editorialNote "N644b3d0b35fb4665a54047db49029c16",
        "N68ac490f3d254485be1cb53a65eed590",
        "Na5b3a1774293400d97841b2bb007e167" ;
    skos:inScheme okns:frbr ;
    skos:mappingRelation frbr:ResponsibleEntity ;
    skos:note "description: This class represents any of the FRBR group two entities." ;
    linkml:class_uri frbr:ResponsibleEntity ;
    linkml:definition_uri okns:FrbrResponsibleEntity ;
    linkml:slot_usage [ ] .

okns:MoMedium a linkml:ClassDefinition ;
    dcterms:source <http://purl.org/ontology/mo/> ;
    dcterms:title "Medium" ;
    skos:definition "A means or instrumentality for storing or communicating musical manifestation." ;
    skos:inScheme okns:mo ;
    skos:mappingRelation ns1:Medium ;
    linkml:class_uri <http://purl.org/ontology/mo/Medium> ;
    linkml:definition_uri okns:MoMedium ;
    linkml:is_a okns:MoMusicalItem ;
    linkml:slot_usage [ ] .

okns:OwlOntology a linkml:ClassDefinition ;
    dcterms:source owl: ;
    dcterms:title "Ontology" ;
    skos:definition "The class of ontologies." ;
    skos:inScheme okns:owl-rdf-rdfs ;
    skos:mappingRelation owl:Ontology ;
    linkml:class_uri owl:Ontology ;
    linkml:definition_uri okns:OwlOntology ;
    linkml:is_a okns:RdfsResource ;
    linkml:slot_usage [ ] .

okns:Time-entryTemporalThing a linkml:ClassDefinition ;
    dcterms:title "No class (entity type) name specified -- this class is noted as a superclass of another class in this graph but has not itself been defined." ;
    skos:inScheme okns:daml ;
    skos:mappingRelation time-entry:TemporalThing ;
    linkml:class_uri time-entry:TemporalThing ;
    linkml:definition_uri okns:Time-entryTemporalThing ;
    linkml:slot_usage [ ] .

okns:TimeInstant a linkml:ClassDefinition ;
    dcterms:title "Time instant" ;
    skos:definition "A temporal entity with zero extent or duration" ;
    skos:inScheme okns:time ;
    skos:mappingRelation time:Instant ;
    skos:note "description: A temporal entity with zero extent or duration",
        "description: Una entidad temporal con una extensión o duración cero.",
        "title: instante de tiempo." ;
    linkml:class_uri time:Instant ;
    linkml:definition_uri okns:TimeInstant ;
    linkml:is_a okns:TimeTemporalEntity ;
    linkml:slot_usage [ ] .

okns:TimeTemporalUnit a linkml:ClassDefinition ;
    dcterms:title "Temporal unit" ;
    skos:definition "A standard duration, which provides a scale factor for a time extent, or the granularity or precision for a time position." ;
    skos:editorialNote "La pertenencia de la clase 'unidad de tiempo' está abierta, para permitir otras unidades de tiempo utilizadas en algunas aplicaciones técnicas (por ejemplo, millones de años o el mes Baha'i).",
        "Membership of the class TemporalUnit is open, to allow for other temporal units used in some technical applications (e.g. millions of years, Baha'i month).",
        """Remove enumeration from definition, in order to allow other units to be used when required in other coordinate systems. 
NOTE: existing units are still present as members of the class, but the class membership is now open. 

In the original OWL-Time the following constraint appeared: 
  owl:oneOf (
      time:unitSecond
      time:unitMinute
      time:unitHour
      time:unitDay
      time:unitWeek
      time:unitMonth
      time:unitYear
    ) ;""" ;
    skos:inScheme okns:time ;
    skos:mappingRelation time:TemporalUnit ;
    skos:note "description: A standard duration, which provides a scale factor for a time extent, or the granularity or precision for a time position.",
        "description: Una duración estándar, que proporciona un factor de escala para una extensión de tiempo, o la granularidad o precisión para una posición de tiempo.",
        "title: unidad de tiempo" ;
    linkml:class_uri time:TemporalUnit ;
    linkml:definition_uri okns:TimeTemporalUnit ;
    linkml:is_a okns:TimeTemporalDuration ;
    linkml:slot_usage [ ] ;
    linkml:slots okns:rdfs_label,
        okns:skos_prefLabel,
        okns:time_days,
        okns:time_hours,
        okns:time_minutes,
        okns:time_months,
        okns:time_seconds,
        okns:time_weeks,
        okns:time_years .

okns:WgsSpatialThing a linkml:ClassDefinition ;
    dcterms:title "SpatialThing" ;
    skos:definition "Anything with spatial extent, i.e. size, shape, or position.␊ e.g. people, places, bowling balls, as well as abstract areas like cubes." ;
    skos:inScheme okns:wgs ;
    skos:mappingRelation wgs1:SpatialThing ;
    linkml:class_uri wgs1:SpatialThing ;
    linkml:definition_uri okns:WgsSpatialThing ;
    linkml:slot_usage [ ] .

okns:rdfs_comment a linkml:SlotDefinition ;
    dcterms:source rdfs: ;
    dcterms:title "comment" ;
    skos:definition "A description of the subject resource." ;
    skos:inScheme okns:owl-rdf-rdfs ;
    skos:mappingRelation rdfs:comment ;
    linkml:any_of [ a okns:AnonymousSlotExpression ;
            linkml:range okns:RdfsLiteral ],
        [ a okns:AnonymousSlotExpression ;
            linkml:range okns:string ] ;
    linkml:definition_uri okns:rdfs_comment ;
    linkml:domain okns:RdfsResource ;
    linkml:domain_of okns:Daml-2001Class,
        okns:Daml-2001List,
        okns:Daml-2001Property,
        okns:Daml-ontUSState,
        okns:DamlOntology,
        okns:DcamVocabularyEncodingScheme,
        okns:DctAgentClass,
        okns:RdfList,
        okns:RdfsDatatype ;
    linkml:inlined true ;
    linkml:owner okns:rdfs_comment ;
    linkml:range okns:Any ;
    linkml:slot_uri rdfs:comment .

okns:FrbrItem a linkml:ClassDefinition ;
    dcterms:source frbr: ;
    dcterms:title "item" ;
    skos:definition "An exemplar of a single manifestation." ;
    skos:editorialNote "N042043e7d60c4a3d99c212ac711f06c0",
        "N4408d3925a9745a188c3b2c300e9bfab",
        "N4787cfb2c21649eda3977ea1eaa4892d",
        "N695d2786b3984954aa9201f353175a77",
        "Nbc61d1e9ad66430bb3e3072d119a07c9" ;
    skos:inScheme okns:frbr ;
    skos:mappingRelation frbr:Item ;
    skos:note "description: This class corresponds to the FRBR group one entity 'Item'." ;
    linkml:class_uri frbr:Item ;
    linkml:definition_uri okns:FrbrItem ;
    linkml:is_a okns:FrbrEndeavour ;
    linkml:slot_usage [ ] .

okns:RdfsDatatype a linkml:ClassDefinition ;
    dcterms:source rdfs: ;
    dcterms:title "Datatype" ;
    skos:definition "The class of RDF datatypes." ;
    skos:inScheme okns:owl-rdf-rdfs ;
    skos:mappingRelation rdfs:Datatype ;
    linkml:class_uri rdfs:Datatype ;
    linkml:definition_uri okns:RdfsDatatype ;
    linkml:is_a okns:RdfsClass ;
    linkml:slot_usage [ ] ;
    linkml:slots okns:rdfs_comment,
        okns:rdfs_isDefinedBy,
        okns:rdfs_label,
        okns:rdfs_seeAlso,
        okns:rdfs_subClassOf .

okns:Daml-ontUSState a linkml:ClassDefinition ;
    skos:inScheme okns:daml ;
    skos:mappingRelation daml-ont:USState ;
    linkml:class_uri daml-ont:USState ;
    linkml:definition_uri okns:Daml-ontUSState ;
    linkml:slot_usage [ ] ;
    linkml:slots okns:daml_ont_borderstate,
        okns:daml_ont_capital,
        okns:daml_ont_code,
        okns:daml_ont_name,
        okns:daml_ont_region,
        okns:rdfs_comment .

okns:DamlProperty a linkml:ClassDefinition ;
    skos:inScheme okns:daml ;
    skos:mappingRelation daml:Property ;
    linkml:class_uri daml:Property ;
    linkml:definition_uri okns:DamlProperty ;
    linkml:slot_usage [ ] ;
    linkml:slots okns:daml_comment,
        okns:daml_domain,
        okns:daml_label,
        okns:daml_range,
        okns:daml_samePropertyAs,
        okns:daml_subPropertyOf .

okns:Time-entryCalendarClockDescription a linkml:ClassDefinition ;
    skos:inScheme okns:daml ;
    skos:mappingRelation time-entry:CalendarClockDescription ;
    linkml:class_uri time-entry:CalendarClockDescription ;
    linkml:definition_uri okns:Time-entryCalendarClockDescription ;
    linkml:slot_usage [ ] .

okns:TimeTemporalEntity a linkml:ClassDefinition ;
    dcterms:title "Temporal entity" ;
    skos:definition "A temporal interval or instant." ;
    skos:inScheme okns:time ;
    skos:mappingRelation time:TemporalEntity ;
    skos:note "description: A temporal interval or instant.",
        "description: Un intervalo temporal o un instante.",
        "title: entidad temporal" ;
    linkml:class_uri time:TemporalEntity ;
    linkml:definition_uri okns:TimeTemporalEntity ;
    linkml:is_a okns:OwlThing ;
    linkml:slot_usage [ ] .

okns:MoPerformance a linkml:ClassDefinition ;
    dcterms:source <http://purl.org/ontology/mo/> ;
    dcterms:title "performance" ;
    skos:definition "A performance event. ␊        It might include as agents performers, engineers, conductors, or even listeners.␊        It might include as factors a score, a MusicalWork, musical instruments. ␊        It might produce a sound:-)" ;
    skos:inScheme okns:mo ;
    skos:mappingRelation ns1:Performance ;
    linkml:class_uri <http://purl.org/ontology/mo/Performance> ;
    linkml:definition_uri okns:MoPerformance ;
    linkml:is_a okns:EventEvent ;
    linkml:slot_usage [ ] .

okns:OwlRestriction a linkml:ClassDefinition ;
    dcterms:source owl: ;
    dcterms:title "Restriction" ;
    skos:definition "The class of property restrictions." ;
    skos:inScheme okns:owl-rdf-rdfs ;
    skos:mappingRelation owl:Restriction ;
    linkml:class_uri owl:Restriction ;
    linkml:definition_uri okns:OwlRestriction ;
    linkml:is_a okns:OwlClass ;
    linkml:slot_usage [ ] .

okns:SimAssociation a linkml:ClassDefinition ;
    dcterms:source sim: ;
    dcterms:title "Association" ;
    skos:definition "An abstract class to define some association between things.  Entities share an association if they are somehow inter-connected.  Generally a <b>directed association</b> should have at lease one <code>sim:subject</code> property and one <code>sim:object</code> property <b>or</b> an <b>undirected association</b> should have at least two <code>sim:element</code> properties, however this is not a requirement and intentionally left out of the model." ;
    skos:inScheme okns:sim ;
    skos:mappingRelation sim:Association ;
    linkml:class_uri sim:Association ;
    linkml:definition_uri okns:SimAssociation ;
    linkml:is_a okns:OwlThing ;
    linkml:slot_usage [ ] .

okns:TimeGeneralDateTimeDescription a linkml:ClassDefinition ;
    dcterms:title "Generalized date-time description" ;
    skos:definition "Description of date and time structured with separate values for the various elements of a calendar-clock system" ;
    skos:editorialNote "Algunas combinaciones de propiedades son redundantes - por ejemplo, dentro de un 'año' especificado si se proporciona 'día del año' entonces 'día' y 'mes' se pueden computar, y viceversa. Los valores individuales deberían ser consistentes entre ellos y con el calendario, indicado a través del valor de la propiedad 'tiene TRS'.",
        "Some combinations of properties are redundant - for example, within a specified :year if :dayOfYear is provided then :day and :month can be computed, and vice versa. Individual values should be consistent with each other and the calendar, indicated through the value of the :hasTRS property." ;
    skos:inScheme okns:time ;
    skos:mappingRelation time:GeneralDateTimeDescription ;
    skos:note "description: Descripción de fecha y hora estructurada con valores separados para los distintos elementos de un sistema calendario-reloj.",
        "description: Description of date and time structured with separate values for the various elements of a calendar-clock system",
        "title: descripción de fecha-hora generalizada" ;
    linkml:class_uri time:GeneralDateTimeDescription ;
    linkml:definition_uri okns:TimeGeneralDateTimeDescription ;
    linkml:is_a okns:TimeTemporalPosition ;
    linkml:slot_usage [ ] .

okns:dct_relation a linkml:SlotDefinition ;
    dcterms:source dcterms: ;
    dcterms:title "Relation" ;
    rdfs:subPropertyOf okns:dc_relation ;
    skos:definition "Recommended practice is to identify the related resource by means of a URI.  If this is not possible or feasible, a string conforming to a formal identification system may be provided." ;
    skos:editorialNote "No occurrences of this slot in the graph." ;
    skos:inScheme okns:dc ;
    skos:mappingRelation dcterms:relation ;
    skos:note "description: A related resource." ;
    linkml:definition_uri okns:dct_relation ;
    linkml:inlined true ;
    linkml:range okns:Any ;
    linkml:slot_uri dcterms:relation .

okns:DamlClass a linkml:ClassDefinition ;
    skos:inScheme okns:daml ;
    skos:mappingRelation daml:Class ;
    linkml:class_uri daml:Class ;
    linkml:definition_uri okns:DamlClass ;
    linkml:slot_usage [ ] ;
    linkml:slots okns:daml_asClass,
        okns:daml_comment,
        okns:daml_complementOf,
        okns:daml_label,
        okns:daml_sameClassAs,
        okns:daml_subClassOf .

okns:uri a linkml:TypeDefinition ;
    dcterms:conformsTo "https://www.ietf.org/rfc/rfc3987.txt" ;
    skos:closeMatch schema1:URL ;
    skos:definition "a complete URI" ;
    skos:editorialNote "If you are authoring schemas in LinkML YAML, the type is referenced with the lower case \"uri\"." ;
    skos:inScheme linkml:types ;
    skos:note "in RDF serializations a slot with range of uri is treated as a literal or type xsd:anyURI unless it is an identifier or a reference to an identifier, in which case it is translated directly to a node" ;
    linkml:base "URI" ;
    linkml:imported_from "linkml:types" ;
    linkml:repr "str" ;
    linkml:definition_uri linkml:Uri ;
    linkml:uri xsd:anyURI .

okns:rdfs_label a linkml:SlotDefinition ;
    dcterms:source rdfs: ;
    dcterms:title "label" ;
    skos:definition "A human-readable name for the subject." ;
    skos:inScheme okns:owl-rdf-rdfs ;
    skos:mappingRelation rdfs:label ;
    linkml:any_of [ a okns:AnonymousSlotExpression ;
            linkml:range okns:RdfsLiteral ],
        [ a okns:AnonymousSlotExpression ;
            linkml:range okns:string ] ;
    linkml:definition_uri okns:rdfs_label ;
    linkml:domain okns:RdfsResource ;
    linkml:domain_of okns:Daml-2001Class,
        okns:Daml-2001Property,
        okns:Daml-ontUSRegion,
        okns:DcamVocabularyEncodingScheme,
        okns:DctAgentClass,
        okns:DctIMT,
        okns:RdfList,
        okns:RdfsDatatype,
        okns:TimeDayOfWeek,
        okns:TimeTemporalUnit ;
    linkml:inlined true ;
    linkml:owner okns:rdfs_label ;
    linkml:range okns:Any ;
    linkml:slot_uri rdfs:label .

okns:Daml-oilClass a linkml:ClassDefinition ;
    dcterms:title "Class" ;
    skos:definition "The class of all \"object\" classes" ;
    skos:inScheme okns:daml ;
    skos:mappingRelation daml-oil:Class ;
    linkml:class_uri daml-oil:Class ;
    linkml:definition_uri okns:Daml-oilClass ;
    linkml:is_a okns:RdfsClass ;
    linkml:slot_usage [ ] ;
    linkml:slots okns:daml_oil_comment,
        okns:daml_oil_label,
        okns:daml_oil_subClassOf .

okns:RdfList a linkml:ClassDefinition ;
    dcterms:source rdf: ;
    dcterms:title "List" ;
    skos:definition "The class of RDF Lists." ;
    skos:inScheme okns:owl-rdf-rdfs ;
    skos:mappingRelation rdf:List ;
    linkml:class_uri rdf:List ;
    linkml:definition_uri okns:RdfList ;
    linkml:is_a okns:RdfsResource ;
    linkml:slot_usage [ ] ;
    linkml:slots okns:rdfs_comment,
        okns:rdfs_isDefinedBy,
        okns:rdfs_label .

okns:FoafPerson a linkml:ClassDefinition ;
    dcterms:source foaf: ;
    dcterms:title "Person" ;
    skos:definition "A person." ;
    skos:inScheme okns:foaf ;
    skos:mappingRelation foaf:Person ;
    linkml:class_uri foaf:Person ;
    linkml:definition_uri okns:FoafPerson ;
    linkml:is_a okns:WgsSpatialThing ;
    linkml:slot_usage [ ] .

okns:decimal a linkml:TypeDefinition ;
    skos:broadMatch schema1:Number ;
    skos:definition "A real number with arbitrary precision that conforms to the xsd:decimal specification" ;
    skos:editorialNote "If you are authoring schemas in LinkML YAML, the type is referenced with the lower case \"decimal\"." ;
    skos:inScheme linkml:types ;
    linkml:base "Decimal" ;
    linkml:imported_from "linkml:types" ;
    linkml:definition_uri linkml:Decimal ;
    linkml:uri xsd:decimal .

okns:EventEvent a linkml:ClassDefinition ;
    dcterms:title "Event" ;
    skos:definition "An arbitrary classification of a space/time region, by a ␊		cognitive agent. An event may have actively participating agents,␊		passive factors, products, and a location in space/time." ;
    skos:inScheme okns:event ;
    skos:mappingRelation event:Event ;
    linkml:class_uri event:Event ;
    linkml:definition_uri okns:EventEvent ;
    linkml:slot_usage [ ] .

okns:MoMusicArtist a linkml:ClassDefinition ;
    dcterms:source <http://purl.org/ontology/mo/> ;
    dcterms:title "music artist" ;
    skos:definition "A person or a group of people (or a computer :-) ), whose musical ␊        creative work shows sensitivity and imagination" ;
    skos:inScheme okns:mo ;
    skos:mappingRelation ns1:MusicArtist ;
    linkml:class_uri <http://purl.org/ontology/mo/MusicArtist> ;
    linkml:definition_uri okns:MoMusicArtist ;
    linkml:is_a okns:FoafAgent ;
    linkml:slot_usage [ ] .

okns:unsignedinteger a linkml:TypeDefinition ;
    rdfs:seeAlso <https://numpy.org/doc/stable/reference/arrays.scalars.html#numpy.unsignedinteger>,
        <https://www.w3.org/TR/xmlschema-2/#nonNegativeInteger> ;
    skos:definition "An integer that is non-negative" ;
    skos:inScheme okns:extended_types ;
    linkml:base "int" ;
    linkml:definition_uri linkml:Unsignedinteger ;
    linkml:minimum_value "0"^^<https://purl.org/okn/schema/@id> ;
    linkml:typeof okns:integer ;
    linkml:uri xsd:unsignedInt .

okns:RdfProperty a linkml:ClassDefinition ;
    dcterms:source rdf: ;
    dcterms:title "Property" ;
    skos:definition "The class of RDF properties." ;
    skos:inScheme okns:owl-rdf-rdfs ;
    skos:mappingRelation rdf:Property ;
    linkml:class_uri rdf:Property ;
    linkml:definition_uri okns:RdfProperty ;
    linkml:is_a okns:RdfsResource ;
    linkml:slot_usage [ ] .

okns:RdfsClass a linkml:ClassDefinition ;
    dcterms:source rdfs: ;
    dcterms:title "Class" ;
    skos:definition "The class of classes." ;
    skos:inScheme okns:owl-rdf-rdfs ;
    skos:mappingRelation rdfs:Class ;
    linkml:class_uri rdfs:Class ;
    linkml:definition_uri okns:RdfsClass ;
    linkml:is_a okns:RdfsResource ;
    linkml:slot_usage [ ] .

okns:MoSignal a linkml:ClassDefinition ;
    dcterms:source <http://purl.org/ontology/mo/> ;
    dcterms:title "signal" ;
    skos:definition "A subclass of MusicalExpression, representing a signal, for example a master signal produced by a performance and a recording." ;
    skos:inScheme okns:mo ;
    skos:mappingRelation ns1:Signal ;
    linkml:class_uri <http://purl.org/ontology/mo/Signal> ;
    linkml:definition_uri okns:MoSignal ;
    linkml:is_a okns:MoMusicalExpression ;
    linkml:slot_usage [ ] .

okns:foaf_isPrimaryTopicOf a linkml:SlotDefinition ;
    dcterms:source foaf: ;
    dcterms:title "is primary topic of" ;
    rdfs:subPropertyOf okns:foaf_page ;
    owl:inverseOf okns:foaf_primaryTopic ;
    skos:definition "A document that this thing is the primary topic of." ;
    skos:editorialNote "No occurrences of this slot in the graph." ;
    skos:inScheme okns:foaf ;
    skos:mappingRelation foaf:isPrimaryTopicOf ;
    linkml:definition_uri okns:foaf_isPrimaryTopicOf ;
    linkml:domain okns:OwlThing ;
    linkml:inlined true ;
    linkml:owner okns:foaf_isPrimaryTopicOf ;
    linkml:range okns:FoafDocument ;
    linkml:slot_uri foaf:isPrimaryTopicOf .

okns:FrbrExpression a linkml:ClassDefinition ;
    dcterms:source frbr: ;
    dcterms:title "expression" ;
    skos:definition "A realization of a single work usually in a physical form." ;
    skos:editorialNote "N3bd4139074924d3882e40967dd357662",
        "N450c285c097b4781a1ffeb7e70e1ca13",
        "N748d92d042344fcf8e49a2a8ab79c87d" ;
    skos:inScheme okns:frbr ;
    skos:mappingRelation frbr:Expression ;
    skos:note "description: This class corresponds to the FRBR group one entity 'Expression'." ;
    linkml:class_uri frbr:Expression ;
    linkml:definition_uri okns:FrbrExpression ;
    linkml:is_a okns:FrbrEndeavour ;
    linkml:slot_usage [ ] .

okns:MoMusicalManifestation a linkml:ClassDefinition ;
    dcterms:source <http://purl.org/ontology/mo/> ;
    dcterms:title "musical manifestation" ;
    skos:definition "This entity is related to the edition/production/publication of a musical expression (musical manifestation are closely related with the music industry (their terms, concepts, definitions, methods (production, publication, etc.), etc.)␊    ␊From the FRBR final report: The entity defined as manifestation encompasses a wide range of materials, including manuscripts, books, periodicals, maps, posters, sound recordings, films, video recordings, CD-ROMs, multimedia kits, etc. As an entity, manifestation represents all the physical objects that bear the same characteristics, in respect to both intellectual content and physical form.␊␊␊Work #1 J. S. Bach's Six suites for unaccompanied cello␊␊    * Expression #1 sound issued during the performance by Janos Starker recorded in 1963 and 1965␊          o Manifestation #1 recordings released on 33 1/3 rpm sound discs in 1965 by Mercury␊          o Manifestation #2 recordings re-released on compact disc in 1991 by Mercury ␊    * Expression #2 sound issued during the performances by Yo-Yo Ma recorded in 1983␊          o Manifestation #1 recordings released on 33 1/3 rpm sound discs in 1983 by CBS Records␊          o Manifestation #2 recordings re-released on compact disc in 1992 by CBS Records ␊␊          ␊Changes that occur deliberately or even inadvertently in the production process that affect the copies result, strictly speaking, in a new manifestation. A manifestation resulting from such a change may be identified as a particular \"state\" or \"issue\" of the publication.␊␊Changes that occur to an individual copy after the production process is complete (e.g., the loss of a page, rebinding, etc.) are not considered to result in a new manifestation. That copy is simply considered to be an exemplar (or item) of the manifestation that deviates from the copy as produced.␊␊With the entity defined as manifestation we can describe the physical characteristics of a set of items and the characteristics associated with the production and distribution of that set of items that may be important factors in enabling users to choose a manifestation appropriate to their physical needs and constraints, and to identify and acquire a copy of that manifestation.␊␊Defining manifestation as an entity also enables us to draw relationships between specific manifestations of a work. We can use the relationships between manifestations to identify, for example, the specific publication that was used to create a microreproduction." ;
    skos:inScheme okns:mo ;
    skos:mappingRelation ns1:MusicalManifestation ;
    linkml:class_uri <http://purl.org/ontology/mo/MusicalManifestation> ;
    linkml:definition_uri okns:MoMusicalManifestation ;
    linkml:is_a okns:FrbrManifestation ;
    linkml:slot_usage [ ] .

okns:Time-entryProperIntervalThing a linkml:ClassDefinition ;
    dcterms:title "No class (entity type) name specified -- this class is noted as a superclass of another class in this graph but has not itself been defined." ;
    skos:inScheme okns:daml ;
    skos:mappingRelation time-entry:ProperIntervalThing ;
    linkml:class_uri time-entry:ProperIntervalThing ;
    linkml:definition_uri okns:Time-entryProperIntervalThing ;
    linkml:is_a okns:Time-entryIntervalThing ;
    linkml:slot_usage [ ] .

okns:TimeProperInterval a linkml:ClassDefinition ;
    dcterms:title "Proper interval" ;
    skos:definition "A temporal entity with non-zero extent or duration, i.e. for which the value of the beginning and end are different" ;
    skos:inScheme okns:time ;
    skos:mappingRelation time:ProperInterval ;
    skos:note "description: A temporal entity with non-zero extent or duration, i.e. for which the value of the beginning and end are different",
        "description: Una entidad temporal con extensión o duración distinta de cero, es decir, para la cual los valores de principio y fin del intervalo son diferentes.",
        "title: intervalo propio" ;
    linkml:class_uri time:ProperInterval ;
    linkml:definition_uri okns:TimeProperInterval ;
    linkml:is_a okns:TimeInterval ;
    linkml:slot_usage [ ] .

okns:frbr_relatedEndeavour a linkml:SlotDefinition ;
    dcterms:source frbr: ;
    dcterms:title "related endeavour" ;
    skos:definition "Another endeavour that is related in some way to an endeavour." ;
    skos:editorialNote "N15c6bc1db7f345b1973823d079ba3054",
        "Nbe7b8cbc2f62455aba816b6bd60221fd",
        "No occurrences of this slot in the graph." ;
    skos:inScheme okns:frbr ;
    skos:mappingRelation frbr:relatedEndeavour ;
    linkml:definition_uri okns:frbr_relatedEndeavour ;
    linkml:domain okns:FrbrEndeavour ;
    linkml:inlined true ;
    linkml:owner okns:frbr_relatedEndeavour ;
    linkml:range okns:FrbrEndeavour ;
    linkml:slot_uri frbr:relatedEndeavour .

okns:FoafDocument a linkml:ClassDefinition ;
    dcterms:title "No class (entity type) name specified -- this class is noted as a superclass of another class in this graph but has not itself been defined." ;
    skos:inScheme okns:wot ;
    skos:mappingRelation foaf:Document ;
    linkml:class_uri foaf:Document ;
    linkml:definition_uri okns:FoafDocument ;
    linkml:slot_usage [ ] .

okns:RdfsResource a linkml:ClassDefinition ;
    dcterms:source rdfs: ;
    dcterms:title "Resource" ;
    skos:definition "The class resource, everything." ;
    skos:inScheme okns:owl-rdf-rdfs ;
    skos:mappingRelation rdfs:Resource ;
    linkml:class_uri rdfs:Resource ;
    linkml:definition_uri okns:RdfsResource ;
    linkml:slot_usage [ ] .

okns:RdfsLiteral a linkml:ClassDefinition ;
    dcterms:source rdfs: ;
    dcterms:title "No (data)type name specified -- this type is noted as a supertype of another type in this graph but has not itself been defined." ;
    skos:definition "The class of literal values, eg. textual strings and integers." ;
    skos:inScheme okns:owl-rdf-rdfs ;
    skos:mappingRelation rdfs:Literal ;
    linkml:class_uri rdfs:Literal ;
    linkml:definition_uri okns:RdfsLiteral ;
    linkml:is_a okns:RdfsResource ;
    linkml:slot_usage [ ] .

okns:OwlThing a linkml:ClassDefinition ;
    dcterms:source owl: ;
    dcterms:title "Thing" ;
    skos:definition "The class of OWL individuals." ;
    skos:inScheme okns:owl-rdf-rdfs ;
    skos:mappingRelation owl:Thing ;
    linkml:class_uri owl:Thing ;
    linkml:definition_uri okns:OwlThing ;
    linkml:slot_usage [ ] .

okns:FoafAgent a linkml:ClassDefinition ;
    dcterms:title "No class (entity type) name specified -- this class is noted as a superclass of another class in this graph but has not itself been defined." ;
    skos:inScheme okns:wot ;
    skos:mappingRelation foaf:Agent ;
    linkml:class_uri foaf:Agent ;
    linkml:definition_uri okns:FoafAgent ;
    linkml:slot_usage [ ] .

okns:time a linkml:TypeDefinition ;
    skos:definition "A time object represents a (local) time of day, independent of any particular day" ;
    skos:editorialNote "If you are authoring schemas in LinkML YAML, the type is referenced with the lower case \"time\".",
        "URI is dateTime because OWL reasoners do not work with straight date or time" ;
    skos:exactMatch schema1:Time ;
    skos:inScheme linkml:types ;
    linkml:base "XSDTime" ;
    linkml:imported_from "linkml:types" ;
    linkml:repr "str" ;
    linkml:definition_uri linkml:Time ;
    linkml:uri xsd:time .

okns:string a linkml:TypeDefinition ;
    skos:definition "A character string" ;
    skos:editorialNote "In RDF serializations, a slot with range of string is treated as a literal or type xsd:string.   If you are authoring schemas in LinkML YAML, the type is referenced with the lower case \"string\"." ;
    skos:exactMatch schema1:Text ;
    skos:inScheme linkml:types ;
    linkml:base "str" ;
    linkml:imported_from "linkml:types" ;
    linkml:definition_uri linkml:String ;
    linkml:uri xsd:string .

okns:mo a linkml:SchemaDefinition ;
    dcterms:license "https://creativecommons.org/publicdomain/zero/1.0/" ;
    pav:createdOn "2025-09-03T11:22:55.066790"^^xsd:dateTime ;
    pav:lastUpdatedOn "2025-09-03T11:22:55.066790"^^xsd:dateTime ;
    skos:definition "␊        The Music Ontology Specification provides main concepts and ␊        properties fo describing music (i.e. artists, albums and tracks) ␊        on the Semantic Web. ␊" ;
    skos:note "last_updated_on: 2013/07/22 16:54:19",
        "title: The Music Ontology" ;
    sh:declare [ sh:namespace owl: ;
            sh:prefix "owl" ],
        [ sh:namespace event: ;
            sh:prefix "event" ],
        [ sh:namespace dcterms: ;
            sh:prefix "dct" ],
        [ sh:namespace swvs: ;
            sh:prefix "swvs" ],
        [ sh:namespace <http://purl.org/ontology/mo/> ;
            sh:prefix "mo" ],
        [ sh:namespace okns: ;
            sh:prefix "okns" ],
        [ sh:namespace frbr: ;
            sh:prefix "frbr" ],
        [ sh:namespace time: ;
            sh:prefix "time" ],
        [ sh:namespace xsd: ;
            sh:prefix "xsd" ],
        [ sh:namespace wgs1: ;
            sh:prefix "wgs" ],
        [ sh:namespace ao: ;
            sh:prefix "ao" ],
        [ sh:namespace rdfs: ;
            sh:prefix "rdfs" ],
        [ sh:namespace foaf: ;
            sh:prefix "foaf" ],
        [ sh:namespace rdf: ;
            sh:prefix "rdf" ],
        [ sh:namespace cc: ;
            sh:prefix "cc" ],
        [ sh:namespace okn: ;
            sh:prefix "okn" ],
        [ sh:namespace dc: ;
            sh:prefix "dc" ],
        [ sh:namespace linkml: ;
            sh:prefix "linkml" ] ;
    linkml:default_prefix "okns" ;
    linkml:metamodel_version "1.7.0" ;
    linkml:source_file "mo.yaml" ;
    linkml:annotations [ skos:example [ okns:pairs [ skos:example [ dc:description [ skos:example [ ns1:ReleaseStatus [ skos:example [ okns:string [ skos:example 3 ;
                                                                            linkml:tag okns:string ] ] ;
                                                            linkml:tag ns1:ReleaseStatus ] ;
                                                    ns1:ReleaseType [ skos:example [ okns:string [ skos:example 10 ;
                                                                            linkml:tag okns:string ] ] ;
                                                            linkml:tag ns1:ReleaseType ] ] ;
                                            linkml:tag dc:description ] ;
                                    dc:title [ skos:example [ ns1:ReleaseStatus [ skos:example [ okns:string [ skos:example 3 ;
                                                                            linkml:tag okns:string ] ] ;
                                                            linkml:tag ns1:ReleaseStatus ] ;
                                                    ns1:ReleaseType [ skos:example [ okns:string [ skos:example 10 ;
                                                                            linkml:tag okns:string ] ] ;
                                                            linkml:tag ns1:ReleaseType ] ] ;
                                            linkml:tag dc:title ] ;
                                    rdfs:isDefinedBy [ skos:example [ ns1:ReleaseStatus [ skos:example [ owl:Ontology [ skos:example 3 ;
                                                                            linkml:tag owl:Ontology ] ] ;
                                                            linkml:tag ns1:ReleaseStatus ] ;
                                                    ns1:ReleaseType [ skos:example [ owl:Ontology [ skos:example 10 ;
                                                                            linkml:tag owl:Ontology ] ] ;
                                                            linkml:tag ns1:ReleaseType ] ] ;
                                            linkml:tag rdfs:isDefinedBy ] ;
                                    foaf:homepage [ skos:example [ okns:untyped [ skos:example [ linkml:uri [ skos:example 6 ;
                                                                            linkml:tag okns:uri ] ] ;
                                                            linkml:tag okns:untyped ] ] ;
                                            linkml:tag foaf:homepage ] ;
                                    foaf:name [ skos:example [ okns:untyped [ skos:example [ okns:string [ skos:example 7 ;
                                                                            linkml:tag okns:string ] ] ;
                                                            linkml:tag okns:untyped ] ] ;
                                            linkml:tag foaf:name ] ;
                                    ns1:level [ skos:example [ ns1:ReleaseStatus [ skos:example [ okns:string [ skos:example 3 ;
                                                                            linkml:tag okns:string ] ] ;
                                                            linkml:tag ns1:ReleaseStatus ] ;
                                                    ns1:ReleaseType [ skos:example [ okns:string [ skos:example 10 ;
                                                                            linkml:tag okns:string ] ] ;
                                                            linkml:tag ns1:ReleaseType ] ] ;
                                            linkml:tag ns1:level ] ] ;
                            linkml:tag okns:pairs ] ;
                    linkml:classes [ skos:example [ ns1:ReleaseStatus [ skos:example 3 ;
                                            linkml:tag ns1:ReleaseStatus ] ;
                                    ns1:ReleaseType [ skos:example 10 ;
                                            linkml:tag ns1:ReleaseType ] ] ;
                            linkml:tag okns:classes ] ;
                    linkml:slots [ skos:example [ dc:description [ skos:example 13 ;
                                            linkml:tag dc:description ] ;
                                    dc:title [ skos:example 13 ;
                                            linkml:tag dc:title ] ;
                                    rdfs:isDefinedBy [ skos:example 13 ;
                                            linkml:tag rdfs:isDefinedBy ] ;
                                    foaf:homepage [ skos:example 6 ;
                                            linkml:tag foaf:homepage ] ;
                                    foaf:name [ skos:example 7 ;
                                            linkml:tag foaf:name ] ;
                                    ns1:level [ skos:example 13 ;
                                            linkml:tag ns1:level ] ] ;
                            linkml:tag okns:slots ] ] ;
            linkml:tag okns:counts ],
        [ skos:example [ okns:pairs [ skos:example [ dc:description [ skos:example [ ns1:ReleaseStatus [ skos:example [ okns:string [ skos:example [ rdf:predicate [ skos:example "dc:description" ;
                                                                                            linkml:tag okns:predicate ] ;
                                                                                    linkml:subject [ skos:example "mo:promotion" ;
                                                                                            linkml:tag okns:subject ] ;
                                                                                    linkml:object [ skos:example "A giveaway musical work or the expression of a musical work intended to promote an upcoming official musical work or the expression of a musical work." ;
                                                                                            linkml:tag okns:object ] ] ;
                                                                            linkml:tag okns:string ] ] ;
                                                            linkml:tag ns1:ReleaseStatus ] ;
                                                    ns1:ReleaseType [ skos:example [ okns:string [ skos:example [ rdf:predicate [ skos:example "dc:description" ;
                                                                                            linkml:tag okns:predicate ] ;
                                                                                    linkml:subject [ skos:example "mo:live" ;
                                                                                            linkml:tag okns:subject ] ;
                                                                                    linkml:object [ skos:example """
        A musical manifestation that was recorded live.
        This is a type of MusicalManifestation defined by the musical industry.""" ;
                                                                                            linkml:tag okns:object ] ] ;
                                                                            linkml:tag okns:string ] ] ;
                                                            linkml:tag ns1:ReleaseType ] ] ;
                                            linkml:tag dc:description ] ;
                                    dc:title [ skos:example [ ns1:ReleaseStatus [ skos:example [ okns:string [ skos:example [ rdf:predicate [ skos:example "dc:title" ;
                                                                                            linkml:tag okns:predicate ] ;
                                                                                    linkml:subject [ skos:example "mo:promotion" ;
                                                                                            linkml:tag okns:subject ] ;
                                                                                    linkml:object [ skos:example "promotion" ;
                                                                                            linkml:tag okns:object ] ] ;
                                                                            linkml:tag okns:string ] ] ;
                                                            linkml:tag ns1:ReleaseStatus ] ;
                                                    ns1:ReleaseType [ skos:example [ okns:string [ skos:example [ rdf:predicate [ skos:example "dc:title" ;
                                                                                            linkml:tag okns:predicate ] ;
                                                                                    linkml:subject [ skos:example "mo:live" ;
                                                                                            linkml:tag okns:subject ] ;
                                                                                    linkml:object [ skos:example "live" ;
                                                                                            linkml:tag okns:object ] ] ;
                                                                            linkml:tag okns:string ] ] ;
                                                            linkml:tag ns1:ReleaseType ] ] ;
                                            linkml:tag dc:title ] ;
                                    rdfs:isDefinedBy [ skos:example [ ns1:ReleaseStatus [ skos:example [ owl:Ontology [ skos:example [ rdf:predicate [ skos:example "rdfs:isDefinedBy" ;
                                                                                            linkml:tag okns:predicate ] ;
                                                                                    linkml:subject [ skos:example "mo:promotion" ;
                                                                                            linkml:tag okns:subject ] ;
                                                                                    linkml:object [ skos:example "mo:" ;
                                                                                            linkml:tag okns:object ] ] ;
                                                                            linkml:tag owl:Ontology ] ] ;
                                                            linkml:tag ns1:ReleaseStatus ] ;
                                                    ns1:ReleaseType [ skos:example [ owl:Ontology [ skos:example [ rdf:predicate [ skos:example "rdfs:isDefinedBy" ;
                                                                                            linkml:tag okns:predicate ] ;
                                                                                    linkml:subject [ skos:example "mo:live" ;
                                                                                            linkml:tag okns:subject ] ;
                                                                                    linkml:object [ skos:example "mo:" ;
                                                                                            linkml:tag okns:object ] ] ;
                                                                            linkml:tag owl:Ontology ] ] ;
                                                            linkml:tag ns1:ReleaseType ] ] ;
                                            linkml:tag rdfs:isDefinedBy ] ;
                                    foaf:homepage [ skos:example [ okns:untyped [ skos:example [ linkml:uri [ skos:example [ rdf:predicate [ skos:example "foaf:homepage" ;
                                                                                            linkml:tag okns:predicate ] ;
                                                                                    linkml:subject [ skos:example "nd0063b47b65f4a2f9b9bc638f1814a84b2" ;
                                                                                            linkml:tag okns:subject ] ;
                                                                                    linkml:object [ skos:example "http://simon-reinhardt.de/" ;
                                                                                            linkml:tag okns:object ] ] ;
                                                                            linkml:tag okns:uri ] ] ;
                                                            linkml:tag okns:untyped ] ] ;
                                            linkml:tag foaf:homepage ] ;
                                    foaf:name [ skos:example [ okns:untyped [ skos:example [ okns:string [ skos:example [ rdf:predicate [ skos:example "foaf:name" ;
                                                                                            linkml:tag okns:predicate ] ;
                                                                                    linkml:subject [ skos:example "nd0063b47b65f4a2f9b9bc638f1814a84b2" ;
                                                                                            linkml:tag okns:subject ] ;
                                                                                    linkml:object [ skos:example "Simon Reinhardt" ;
                                                                                            linkml:tag okns:object ] ] ;
                                                                            linkml:tag okns:string ] ] ;
                                                            linkml:tag okns:untyped ] ] ;
                                            linkml:tag foaf:name ] ;
                                    ns1:level [ skos:example [ ns1:ReleaseStatus [ skos:example [ okns:string [ skos:example [ rdf:predicate [ skos:example "mo:level" ;
                                                                                            linkml:tag okns:predicate ] ;
                                                                                    linkml:subject [ skos:example "mo:promotion" ;
                                                                                            linkml:tag okns:subject ] ;
                                                                                    linkml:object [ skos:example "1" ;
                                                                                            linkml:tag okns:object ] ] ;
                                                                            linkml:tag okns:string ] ] ;
                                                            linkml:tag ns1:ReleaseStatus ] ;
                                                    ns1:ReleaseType [ skos:example [ okns:string [ skos:example [ rdf:predicate [ skos:example "mo:level" ;
                                                                                            linkml:tag okns:predicate ] ;
                                                                                    linkml:subject [ skos:example "mo:live" ;
                                                                                            linkml:tag okns:subject ] ;
                                                                                    linkml:object [ skos:example "1" ;
                                                                                            linkml:tag okns:object ] ] ;
                                                                            linkml:tag okns:string ] ] ;
                                                            linkml:tag ns1:ReleaseType ] ] ;
                                            linkml:tag ns1:level ] ] ;
                            linkml:tag okns:pairs ] ;
                    linkml:classes [ skos:example [ ns1:ReleaseStatus [ skos:example "mo:official" ;
                                            linkml:tag ns1:ReleaseStatus ] ;
                                    ns1:ReleaseType [ skos:example "mo:interview" ;
                                            linkml:tag ns1:ReleaseType ] ] ;
                            linkml:tag okns:classes ] ] ;
            linkml:tag okns:examples ] ;
    linkml:classes okns:Any,
        okns:AoLikeableAssociation,
        okns:CcAgent,
        okns:CcLicense,
        okns:CcPermission,
        okns:CcProhibition,
        okns:CcRequirement,
        okns:CcWork,
        okns:Daml-2001Class,
        okns:Daml-2001List,
        okns:Daml-2001Ontology,
        okns:Daml-2001Property,
        okns:Daml-cityCity,
        okns:Daml-country-ontCountry,
        okns:Daml-countryCountry,
        okns:Daml-countryUNITED-STATES,
        okns:Daml-iso3166Country,
        okns:Daml-oilClass,
        okns:Daml-oilDatatype,
        okns:Daml-oilDatatypeProperty,
        okns:Daml-oilList,
        okns:Daml-oilLiteral,
        okns:Daml-oilObjectProperty,
        okns:Daml-oilOntology,
        okns:Daml-oilProperty,
        okns:Daml-oilRestriction,
        okns:Daml-oilThing,
        okns:Daml-oilTransitiveProperty,
        okns:Daml-oilUnambiguousProperty,
        okns:Daml-oilUniqueProperty,
        okns:Daml-ontCountry,
        okns:Daml-ontUSRegion,
        okns:Daml-ontUSState,
        okns:Daml-profileLocation,
        okns:Daml-stateState,
        okns:Daml-usregionstateUSRegion,
        okns:Daml-usregionstateUSState,
        okns:DamlClass,
        okns:DamlOntology,
        okns:DamlProperty,
        okns:DcamVocabularyEncodingScheme,
        okns:DcmitypeCollection,
        okns:DcmitypeDataset,
        okns:DcmitypeEvent,
        okns:DcmitypeImage,
        okns:DcmitypeInteractiveResource,
        okns:DcmitypeMovingImage,
        okns:DcmitypePhysicalObject,
        okns:DcmitypeService,
        okns:DcmitypeSoftware,
        okns:DcmitypeSound,
        okns:DcmitypeStillImage,
        okns:DcmitypeText,
        okns:DctAgent,
        okns:DctAgentClass,
        okns:DctBibliographicResource,
        okns:DctFileFormat,
        okns:DctFrequency,
        okns:DctIMT,
        okns:DctJurisdiction,
        okns:DctLicenseDocument,
        okns:DctLinguisticSystem,
        okns:DctLocation,
        okns:DctLocationPeriodOrJurisdiction,
        okns:DctMediaType,
        okns:DctMediaTypeOrExtent,
        okns:DctMethodOfAccrual,
        okns:DctMethodOfInstruction,
        okns:DctPeriodOfTime,
        okns:DctPhysicalMedium,
        okns:DctPhysicalResource,
        okns:DctPolicy,
        okns:DctProvenanceStatement,
        okns:DctRightsStatement,
        okns:DctSizeOrDuration,
        okns:DctStandard,
        okns:EventEvent,
        okns:EventFactor,
        okns:EventProduct,
        okns:FoafAgent,
        okns:FoafDocument,
        okns:FoafGroup,
        okns:FoafImage,
        okns:FoafLabelProperty,
        okns:FoafOnlineAccount,
        okns:FoafOnlineChatAccount,
        okns:FoafOnlineEcommerceAccount,
        okns:FoafOnlineGamingAccount,
        okns:FoafOrganization,
        okns:FoafPerson,
        okns:FoafPersonalProfileDocument,
        okns:FoafProject,
        okns:FrbrConcept,
        okns:FrbrCorporateBody,
        okns:FrbrEndeavour,
        okns:FrbrEvent,
        okns:FrbrExpression,
        okns:FrbrItem,
        okns:FrbrManifestation,
        okns:FrbrObject,
        okns:FrbrPerson,
        okns:FrbrPlace,
        okns:FrbrResponsibleEntity,
        okns:FrbrSubject,
        okns:FrbrWork,
        <https://purl.org/okn/schema/HttpPurl.orgNETC4dmKeys.owl#Key>,
        okns:IcalDomainOfRrule,
        okns:IcalListOfFloat,
        okns:IcalValarm,
        okns:IcalValueCAL-ADDRESS,
        okns:IcalValueDATE,
        okns:IcalValueDATE-TIME,
        okns:IcalValueDURATION,
        okns:IcalValuePERIOD,
        okns:IcalValueRECUR,
        okns:IcalVevent,
        okns:IcalVfreebusy,
        okns:IcalVjournal,
        okns:IcalVtimezone,
        okns:IcalVtodo,
        okns:MoActivity,
        okns:MoAnalogSignal,
        okns:MoArrangement,
        okns:MoArranger,
        okns:MoAudioFile,
        okns:MoCD,
        okns:MoComposer,
        okns:MoComposition,
        okns:MoConductor,
        okns:MoCorporateBody,
        okns:MoDAT,
        okns:MoDCC,
        okns:MoDVDA,
        okns:MoDigitalSignal,
        okns:MoED2K,
        okns:MoFestival,
        okns:MoGenre,
        okns:MoInstrument,
        okns:MoInstrumentation,
        okns:MoLabel,
        okns:MoLibretto,
        okns:MoListener,
        okns:MoLyrics,
        okns:MoMD,
        okns:MoMagneticTape,
        okns:MoMedium,
        okns:MoMembership,
        okns:MoMovement,
        okns:MoMusicArtist,
        okns:MoMusicGroup,
        okns:MoMusicalExpression,
        okns:MoMusicalItem,
        okns:MoMusicalManifestation,
        okns:MoMusicalWork,
        okns:MoOrchestration,
        okns:MoPerformance,
        okns:MoPerformer,
        okns:MoPublishedLibretto,
        okns:MoPublishedLyrics,
        okns:MoPublishedScore,
        okns:MoRecord,
        okns:MoRecording,
        okns:MoRecordingSession,
        okns:MoRelease,
        okns:MoReleaseEvent,
        okns:MoReleaseStatus,
        okns:MoReleaseType,
        okns:MoSACD,
        okns:MoScore,
        okns:MoShow,
        okns:MoSignal,
        okns:MoSignalGroup,
        okns:MoSoloMusicArtist,
        okns:MoSound,
        okns:MoSoundEngineer,
        okns:MoStream,
        okns:MoTorrent,
        okns:MoTrack,
        okns:MoTranscription,
        okns:MoVinyl,
        okns:OwlAllDifferent,
        okns:OwlAllDisjointClasses,
        okns:OwlAllDisjointProperties,
        okns:OwlAnnotation,
        okns:OwlAnnotationProperty,
        okns:OwlAsymmetricProperty,
        okns:OwlAxiom,
        okns:OwlClass,
        okns:OwlDataRange,
        okns:OwlDatatypeProperty,
        okns:OwlDeprecatedClass,
        okns:OwlDeprecatedProperty,
        okns:OwlFunctionalProperty,
        okns:OwlInverseFunctionalProperty,
        okns:OwlIrreflexiveProperty,
        okns:OwlNamedIndividual,
        okns:OwlNegativePropertyAssertion,
        okns:OwlNothing,
        okns:OwlObjectProperty,
        okns:OwlOntology,
        okns:OwlOntologyProperty,
        okns:OwlReflexiveProperty,
        okns:OwlRestriction,
        okns:OwlSymmetricProperty,
        okns:OwlThing,
        okns:OwlTransitiveProperty,
        okns:RdfAlt,
        okns:RdfBag,
        okns:RdfCompoundLiteral,
        okns:RdfList,
        okns:RdfProperty,
        okns:RdfSeq,
        okns:RdfStatement,
        okns:RdfsClass,
        okns:RdfsContainer,
        okns:RdfsContainerMembershipProperty,
        okns:RdfsDatatype,
        okns:RdfsLiteral,
        okns:RdfsResource,
        okns:RevComment,
        okns:RevFeedback,
        okns:RevReview,
        okns:SimAssociation,
        okns:SimAssociationMethod,
        okns:SimInfluence,
        okns:SimNetwork,
        okns:SimSimilarity,
        okns:SkosCollection,
        okns:SkosConcept,
        okns:SkosConceptScheme,
        okns:SkosOrderedCollection,
        okns:Time-entryCalendarClockDescription,
        okns:Time-entryCalendarClockInterval,
        okns:Time-entryDurationDescription,
        okns:Time-entryEvent,
        okns:Time-entryInstant,
        okns:Time-entryInstantEvent,
        okns:Time-entryInstantThing,
        okns:Time-entryInstantThingPair,
        okns:Time-entryInterval,
        okns:Time-entryIntervalEvent,
        okns:Time-entryIntervalThing,
        okns:Time-entryProperInterval,
        okns:Time-entryProperIntervalThing,
        okns:Time-entryTemporalEntity,
        okns:Time-entryTemporalThing,
        okns:Time-entryTemporalUnit,
        okns:TimeDateTimeDescription,
        okns:TimeDateTimeInterval,
        okns:TimeDayOfWeek,
        okns:TimeDuration,
        okns:TimeDurationDescription,
        okns:TimeGeneralDateTimeDescription,
        okns:TimeGeneralDurationDescription,
        okns:TimeInstant,
        okns:TimeInterval,
        okns:TimeJanuary,
        okns:TimeMonthOfYear,
        okns:TimeProperInterval,
        okns:TimeTRS,
        okns:TimeTemporalDuration,
        okns:TimeTemporalEntity,
        okns:TimeTemporalPosition,
        okns:TimeTemporalUnit,
        okns:TimeTimePosition,
        okns:TimeTimeZone,
        okns:TimeYear,
        okns:TzontCity,
        okns:TzontCountry,
        okns:TzontCounty,
        okns:TzontDaylightSavingsPolicy,
        okns:TzontEnumeratedDaylightSavingsPolicy,
        okns:TzontPoliticalRegion,
        okns:TzontRegion,
        okns:TzontReservation,
        okns:TzontState,
        okns:TzontTimeZone,
        okns:WfbGEOREF,
        okns:WgsPoint,
        okns:WgsSpatialThing,
        okns:Wn16Credential,
        okns:Wn16Endorsement-4,
        okns:Wn16Event,
        <https://purl.org/okn/schema/Wn16Work~2>,
        okns:WotEncryptedDocument,
        okns:WotEndorsement,
        okns:WotPubKey,
        okns:WotSigEvent,
        okns:WotUser,
        okns:Xsd2000NonNegativeInteger,
        okns:XsdDateTimeStamp,
        okns:XsdDuration,
        okns:XsdGDay,
        okns:XsdGMonth,
        okns:XsdGYear,
        okns:XsdGYearMonth ;
    linkml:default_range okns:string ;
    linkml:generation_date "2025-09-04T07:34:44"^^xsd:dateTime ;
    linkml:id okns:mo ;
    linkml:imports okns:ao,
        okns:cc,
        okns:daml,
        okns:dc,
        okns:event,
        okns:extended_types,
        okns:foaf,
        okns:frbr,
        okns:ical,
        okns:owl-rdf-rdfs,
        okns:rev,
        okns:sim,
        okns:skos,
        okns:time,
        okns:wgs,
        okns:wot,
        linkml:types ;
    linkml:slots okns:ao_activity,
        okns:ao_application,
        okns:ao_context,
        okns:ao_device,
        okns:ao_genre,
        okns:ao_included_association,
        okns:ao_likeminded,
        okns:ao_location,
        okns:ao_mood,
        okns:ao_occasion,
        okns:ao_time,
        okns:ao_used_application,
        okns:ao_used_device,
        okns:cc_derivativeWork,
        okns:cc_license,
        okns:cc_permits,
        okns:cc_prohibits,
        okns:cc_requires,
        okns:daml_2001_comment,
        okns:daml_2001_complementOf,
        okns:daml_2001_imports,
        okns:daml_2001_unionOf,
        okns:daml_2001_versionInfo,
        okns:daml_asClass,
        okns:daml_city_country,
        okns:daml_city_name,
        okns:daml_comment,
        okns:daml_complementOf,
        okns:daml_country_cia,
        okns:daml_country_name,
        okns:daml_domain,
        okns:daml_imports,
        okns:daml_iso3166_code,
        okns:daml_iso3166_name,
        okns:daml_label,
        okns:daml_oil_cardinality,
        okns:daml_oil_cardinalityQ,
        okns:daml_oil_comment,
        okns:daml_oil_complementOf,
        okns:daml_oil_disjointUnionOf,
        okns:daml_oil_disjointWith,
        okns:daml_oil_domain,
        okns:daml_oil_first,
        okns:daml_oil_hasClass,
        okns:daml_oil_hasClassQ,
        okns:daml_oil_hasValue,
        okns:daml_oil_imports,
        okns:daml_oil_intersectionOf,
        okns:daml_oil_inverseOf,
        okns:daml_oil_isDefinedBy,
        okns:daml_oil_item,
        okns:daml_oil_label,
        okns:daml_oil_maxCardinality,
        okns:daml_oil_maxCardinalityQ,
        okns:daml_oil_minCardinality,
        okns:daml_oil_minCardinalityQ,
        okns:daml_oil_onProperty,
        okns:daml_oil_oneOf,
        okns:daml_oil_range,
        okns:daml_oil_rest,
        okns:daml_oil_seeAlso,
        okns:daml_oil_subClassOf,
        okns:daml_oil_subPropertyOf,
        okns:daml_oil_toClass,
        okns:daml_oil_type,
        okns:daml_oil_unionOf,
        okns:daml_oil_value,
        okns:daml_oil_versionInfo,
        okns:daml_ont_borderstate,
        okns:daml_ont_capital,
        okns:daml_ont_cia,
        okns:daml_ont_code,
        okns:daml_ont_memberstate,
        okns:daml_ont_name,
        okns:daml_ont_region,
        okns:daml_range,
        okns:daml_sameClassAs,
        okns:daml_samePropertyAs,
        okns:daml_state_borderstate,
        okns:daml_state_capital,
        okns:daml_state_code,
        okns:daml_state_country,
        okns:daml_state_name,
        okns:daml_subClassOf,
        okns:daml_subPropertyOf,
        okns:daml_usregionstate_memberstate,
        okns:daml_usregionstate_region,
        okns:daml_versionInfo,
        okns:dc_contributor,
        okns:dc_coverage,
        okns:dc_creator,
        okns:dc_date,
        okns:dc_description,
        okns:dc_format,
        okns:dc_identifier,
        okns:dc_language,
        okns:dc_publisher,
        okns:dc_relation,
        okns:dc_rights,
        okns:dc_source,
        okns:dc_subject,
        okns:dc_title,
        okns:dc_type,
        okns:dcam_domainIncludes,
        okns:dcam_memberOf,
        okns:dcam_rangeIncludes,
        okns:dct_abstract,
        okns:dct_accessRights,
        okns:dct_accrualMethod,
        okns:dct_accrualPeriodicity,
        okns:dct_accrualPolicy,
        okns:dct_alternative,
        okns:dct_audience,
        okns:dct_available,
        okns:dct_bibliographicCitation,
        okns:dct_conformsTo,
        okns:dct_contributor,
        okns:dct_coverage,
        okns:dct_created,
        okns:dct_creator,
        okns:dct_date,
        okns:dct_dateAccepted,
        okns:dct_dateCopyrighted,
        okns:dct_dateSubmitted,
        okns:dct_description,
        okns:dct_educationLevel,
        okns:dct_extent,
        okns:dct_format,
        okns:dct_hasFormat,
        okns:dct_hasPart,
        okns:dct_hasVersion,
        okns:dct_identifier,
        okns:dct_instructionalMethod,
        okns:dct_isFormatOf,
        okns:dct_isPartOf,
        okns:dct_isReferencedBy,
        okns:dct_isReplacedBy,
        okns:dct_isRequiredBy,
        okns:dct_isVersionOf,
        okns:dct_issued,
        okns:dct_language,
        okns:dct_license,
        okns:dct_mediator,
        okns:dct_medium,
        okns:dct_modified,
        okns:dct_provenance,
        okns:dct_publisher,
        okns:dct_references,
        okns:dct_relation,
        okns:dct_replaces,
        okns:dct_requires,
        okns:dct_rights,
        okns:dct_rightsHolder,
        okns:dct_source,
        okns:dct_spatial,
        okns:dct_subject,
        okns:dct_tableOfContents,
        okns:dct_temporal,
        okns:dct_title,
        okns:dct_type,
        okns:dct_valid,
        okns:event_agent,
        okns:event_agent_in,
        okns:event_factor,
        okns:event_factor_of,
        okns:event_hasAgent,
        okns:event_hasFactor,
        okns:event_hasLiteralFactor,
        okns:event_hasProduct,
        okns:event_hasSubEvent,
        okns:event_isAgentIn,
        okns:event_isFactorOf,
        okns:event_literal_factor,
        okns:event_place,
        okns:event_producedIn,
        okns:event_produced_in,
        okns:event_product,
        okns:event_sub_event,
        okns:event_time,
        okns:foaf_account,
        okns:foaf_accountName,
        okns:foaf_accountServiceHomepage,
        okns:foaf_age,
        okns:foaf_aimChatID,
        okns:foaf_based_near,
        okns:foaf_birthday,
        okns:foaf_currentProject,
        okns:foaf_depiction,
        okns:foaf_depicts,
        okns:foaf_dnaChecksum,
        okns:foaf_familyName,
        okns:foaf_family_name,
        okns:foaf_firstName,
        okns:foaf_focus,
        okns:foaf_fundedBy,
        okns:foaf_geekcode,
        okns:foaf_gender,
        okns:foaf_givenName,
        okns:foaf_givenname,
        okns:foaf_holdsAccount,
        okns:foaf_homepage,
        okns:foaf_icqChatID,
        okns:foaf_img,
        okns:foaf_interest,
        okns:foaf_isPrimaryTopicOf,
        okns:foaf_jabberID,
        okns:foaf_knows,
        okns:foaf_lastName,
        okns:foaf_logo,
        okns:foaf_made,
        okns:foaf_maker,
        okns:foaf_mbox,
        okns:foaf_mbox_sha1sum,
        okns:foaf_member,
        okns:foaf_membershipClass,
        okns:foaf_msnChatID,
        okns:foaf_myersBriggs,
        okns:foaf_name,
        okns:foaf_nick,
        okns:foaf_openid,
        okns:foaf_page,
        okns:foaf_pastProject,
        okns:foaf_phone,
        okns:foaf_plan,
        okns:foaf_primaryTopic,
        okns:foaf_publications,
        okns:foaf_schoolHomepage,
        okns:foaf_sha1,
        okns:foaf_skypeID,
        okns:foaf_status,
        okns:foaf_surname,
        okns:foaf_theme,
        okns:foaf_thumbnail,
        okns:foaf_tipjar,
        okns:foaf_title,
        okns:foaf_topic,
        okns:foaf_topic_interest,
        okns:foaf_weblog,
        okns:foaf_workInfoHomepage,
        okns:foaf_workplaceHomepage,
        okns:foaf_yahooChatID,
        okns:frbr_abridgement,
        okns:frbr_abridgementOf,
        okns:frbr_adaption,
        okns:frbr_adaptionOf,
        okns:frbr_alternate,
        okns:frbr_alternateOf,
        okns:frbr_arrangement,
        okns:frbr_arrangementOf,
        okns:frbr_complement,
        okns:frbr_complementOf,
        okns:frbr_creator,
        okns:frbr_creatorOf,
        okns:frbr_embodiment,
        okns:frbr_embodimentOf,
        okns:frbr_exemplar,
        okns:frbr_exemplarOf,
        okns:frbr_imitation,
        okns:frbr_imitationOf,
        okns:frbr_owner,
        okns:frbr_ownerOf,
        okns:frbr_part,
        okns:frbr_partOf,
        okns:frbr_producer,
        okns:frbr_producerOf,
        okns:frbr_realization,
        okns:frbr_realizationOf,
        okns:frbr_realizer,
        okns:frbr_realizerOf,
        okns:frbr_reconfiguration,
        okns:frbr_reconfigurationOf,
        okns:frbr_relatedEndeavour,
        okns:frbr_reproduction,
        okns:frbr_reproductionOf,
        okns:frbr_responsibleEntity,
        okns:frbr_responsibleEntityOf,
        okns:frbr_revision,
        okns:frbr_revisionOf,
        okns:frbr_subject,
        okns:frbr_successor,
        okns:frbr_successorOf,
        okns:frbr_summarization,
        okns:frbr_summarizationOf,
        okns:frbr_supplement,
        okns:frbr_supplementOf,
        okns:frbr_transformation,
        okns:frbr_transformationOf,
        okns:frbr_translation,
        okns:frbr_translationOf,
        okns:http___purl.org_vocab_bio_0.1_event,
        okns:ical_X_,
        okns:ical_action,
        okns:ical_attach,
        okns:ical_attendee,
        okns:ical_calscale,
        okns:ical_categories,
        okns:ical_class,
        okns:ical_comment,
        okns:ical_completed,
        okns:ical_contact,
        okns:ical_created,
        okns:ical_description,
        okns:ical_dtend,
        okns:ical_dtstamp,
        okns:ical_dtstart,
        okns:ical_due,
        okns:ical_duration,
        okns:ical_exdate,
        okns:ical_exrule,
        okns:ical_freebusy,
        okns:ical_geo,
        okns:ical_lastModified,
        okns:ical_location,
        okns:ical_method,
        okns:ical_organizer,
        okns:ical_percentComplete,
        okns:ical_priority,
        okns:ical_prodid,
        okns:ical_rdate,
        okns:ical_recurrenceId,
        okns:ical_relatedTo,
        okns:ical_repeat,
        okns:ical_requestStatus,
        okns:ical_resources,
        okns:ical_rrule,
        okns:ical_sequence,
        okns:ical_status,
        okns:ical_summary,
        okns:ical_transp,
        okns:ical_trigger,
        okns:ical_tzid,
        okns:ical_tzname,
        okns:ical_tzoffsetfrom,
        okns:ical_tzoffsetto,
        okns:ical_tzurl,
        okns:ical_uid,
        okns:ical_url,
        okns:ical_version,
        okns:icalspec_valueListType,
        okns:icalspec_valueType,
        okns:langrange,
        okns:length,
        okns:maxexclusive,
        okns:maxlength,
        okns:minexclusive,
        okns:minlength,
        okns:mo_activity,
        okns:mo_activity_end,
        okns:mo_activity_start,
        okns:mo_amazon_asin,
        okns:mo_arranged_in,
        okns:mo_arrangement_of,
        okns:mo_artist,
        okns:mo_availableAs,
        okns:mo_available_as,
        okns:mo_biography,
        okns:mo_bitsPerSample,
        okns:mo_bpm,
        okns:mo_catalogue_number,
        okns:mo_channels,
        okns:mo_collaborated_with,
        okns:mo_compilation_of,
        okns:mo_compiled,
        okns:mo_compiler,
        okns:mo_composed_in,
        okns:mo_composer,
        okns:mo_conducted,
        okns:mo_conductor,
        okns:mo_contains_sample_from,
        okns:mo_derived_from,
        okns:mo_discography,
        okns:mo_discogs,
        okns:mo_djmix_of,
        okns:mo_djmixed,
        okns:mo_djmixed_by,
        okns:mo_download,
        okns:mo_duration,
        okns:mo_ean,
        okns:mo_encodes,
        okns:mo_encoding,
        okns:mo_engineer,
        okns:mo_engineered,
        okns:mo_eventHomePage,
        okns:mo_event_homepage,
        okns:mo_exchange_item,
        okns:mo_fanpage,
        okns:mo_free_download,
        okns:mo_freedownload,
        okns:mo_genre,
        okns:mo_grid,
        okns:mo_group,
        okns:mo_gtin,
        okns:mo_has_track,
        okns:mo_headliner,
        okns:mo_homepage,
        okns:mo_image,
        okns:mo_imdb,
        okns:mo_instrument,
        okns:mo_interpreter,
        okns:mo_ipi,
        okns:mo_ismn,
        okns:mo_isrc,
        okns:mo_iswc,
        okns:mo_item,
        okns:mo_key,
        okns:mo_label,
        okns:mo_lc,
        okns:mo_level,
        okns:mo_licence,
        okns:mo_listened,
        okns:mo_listener,
        okns:mo_lyrics,
        okns:mo_mailorder,
        okns:mo_mashup_of,
        okns:mo_media_type,
        okns:mo_medley_of,
        okns:mo_member,
        okns:mo_member_of,
        okns:mo_membership,
        okns:mo_meter,
        okns:mo_movement,
        okns:mo_movementNum,
        okns:mo_movement_number,
        okns:mo_musicbrainz,
        okns:mo_musicbrainz_guid,
        okns:mo_musicmoz,
        okns:mo_myspace,
        okns:mo_olga,
        okns:mo_onlinecommunity,
        okns:mo_opus,
        okns:mo_origin,
        okns:mo_other_release_of,
        okns:mo_paid_download,
        okns:mo_paiddownload,
        okns:mo_performance_of,
        okns:mo_performed,
        okns:mo_performed_in,
        okns:mo_performer,
        okns:mo_possess_item,
        okns:mo_preview,
        okns:mo_preview_download,
        okns:mo_primary_instrument,
        okns:mo_produced,
        okns:mo_produced_score,
        okns:mo_produced_signal,
        okns:mo_produced_signal_group,
        okns:mo_produced_sound,
        okns:mo_produced_work,
        okns:mo_producer,
        okns:mo_producesSignal,
        okns:mo_producesSound,
        okns:mo_producesWork,
        okns:mo_productOfComposition,
        okns:mo_publicationOf,
        okns:mo_publication_of,
        okns:mo_published,
        okns:mo_publishedAs,
        okns:mo_published_as,
        okns:mo_publisher,
        okns:mo_publishingLocation,
        okns:mo_publishing_location,
        okns:mo_puid,
        okns:mo_record,
        okns:mo_record_count,
        okns:mo_record_number,
        okns:mo_record_side,
        okns:mo_recordedAs,
        okns:mo_recorded_as,
        okns:mo_recorded_in,
        okns:mo_recording_of,
        okns:mo_records,
        okns:mo_release,
        okns:mo_releaseStatus,
        okns:mo_releaseType,
        okns:mo_release_status,
        okns:mo_release_type,
        okns:mo_remaster_of,
        okns:mo_remix_of,
        okns:mo_remixed,
        okns:mo_remixer,
        okns:mo_review,
        okns:mo_sampleRate,
        okns:mo_sample_rate,
        okns:mo_sampled,
        okns:mo_sampledVersionOf,
        okns:mo_sampled_version,
        okns:mo_sampled_version_of,
        okns:mo_sampler,
        okns:mo_sell_item,
        okns:mo_signal,
        okns:mo_signalTime,
        okns:mo_similar_to,
        okns:mo_singer,
        okns:mo_supporting_musician,
        okns:mo_tempo,
        okns:mo_text,
        okns:mo_time,
        okns:mo_track,
        okns:mo_trackNum,
        okns:mo_track_count,
        okns:mo_track_number,
        okns:mo_translation_of,
        okns:mo_tribute_to,
        okns:mo_trmid,
        okns:mo_upc,
        okns:mo_usedInPerformance,
        okns:mo_usedInRecording,
        okns:mo_usesSound,
        okns:mo_usesWork,
        okns:mo_uuid,
        okns:mo_want_item,
        okns:mo_wikipedia,
        okns:owl_allValuesFrom,
        okns:owl_annotatedProperty,
        okns:owl_annotatedSource,
        okns:owl_annotatedTarget,
        okns:owl_assertionProperty,
        okns:owl_backwardCompatibleWith,
        okns:owl_bottomDataProperty,
        okns:owl_bottomObjectProperty,
        okns:owl_cardinality,
        okns:owl_complementOf,
        okns:owl_datatypeComplementOf,
        okns:owl_deprecated,
        okns:owl_differentFrom,
        okns:owl_disjointUnionOf,
        okns:owl_disjointWith,
        okns:owl_distinctMembers,
        okns:owl_equivalentClass,
        okns:owl_equivalentProperty,
        okns:owl_hasKey,
        okns:owl_hasSelf,
        okns:owl_hasValue,
        okns:owl_imports,
        okns:owl_incompatibleWith,
        okns:owl_intersectionOf,
        okns:owl_inverseOf,
        okns:owl_maxCardinality,
        okns:owl_maxQualifiedCardinality,
        okns:owl_members,
        okns:owl_minCardinality,
        okns:owl_minQualifiedCardinality,
        okns:owl_onClass,
        okns:owl_onDataRange,
        okns:owl_onDatatype,
        okns:owl_onProperties,
        okns:owl_onProperty,
        okns:owl_oneOf,
        okns:owl_priorVersion,
        okns:owl_propertyChainAxiom,
        okns:owl_propertyDisjointWith,
        okns:owl_qualifiedCardinality,
        okns:owl_sameAs,
        okns:owl_someValuesFrom,
        okns:owl_sourceIndividual,
        okns:owl_targetIndividual,
        okns:owl_targetValue,
        okns:owl_topDataProperty,
        okns:owl_topObjectProperty,
        okns:owl_unionOf,
        okns:owl_versionIRI,
        okns:owl_versionInfo,
        okns:owl_withRestrictions,
        okns:rdf_direction,
        okns:rdf_first,
        okns:rdf_language,
        okns:rdf_object,
        okns:rdf_predicate,
        okns:rdf_rest,
        okns:rdf_subject,
        okns:rdf_type,
        okns:rdf_value,
        okns:rdfs_comment,
        okns:rdfs_domain,
        okns:rdfs_isDefinedBy,
        okns:rdfs_label,
        okns:rdfs_member,
        okns:rdfs_range,
        okns:rdfs_seeAlso,
        okns:rdfs_subClassOf,
        okns:rdfs_subPropertyOf,
        okns:rev_commenter,
        okns:rev_hasComment,
        okns:rev_hasFeedback,
        okns:rev_hasReview,
        okns:rev_maxRating,
        okns:rev_minRating,
        okns:rev_positiveVotes,
        okns:rev_rating,
        okns:rev_reviewer,
        okns:rev_text,
        okns:rev_title,
        okns:rev_totalVotes,
        okns:rev_type,
        okns:sim_association,
        okns:sim_description,
        okns:sim_distance,
        okns:sim_domain,
        okns:sim_edge,
        okns:sim_element,
        okns:sim_grounding,
        okns:sim_method,
        okns:sim_object,
        okns:sim_range,
        okns:sim_scope,
        okns:sim_subject,
        okns:sim_weight,
        okns:sim_workflow,
        okns:skos_altLabel,
        okns:skos_broadMatch,
        okns:skos_broader,
        okns:skos_broaderTransitive,
        okns:skos_changeNote,
        okns:skos_closeMatch,
        okns:skos_definition,
        okns:skos_editorialNote,
        okns:skos_exactMatch,
        okns:skos_example,
        okns:skos_hasTopConcept,
        okns:skos_hiddenLabel,
        okns:skos_historyNote,
        okns:skos_inScheme,
        okns:skos_mappingRelation,
        okns:skos_member,
        okns:skos_memberList,
        okns:skos_narrowMatch,
        okns:skos_narrower,
        okns:skos_narrowerTransitive,
        okns:skos_notation,
        okns:skos_note,
        okns:skos_prefLabel,
        okns:skos_related,
        okns:skos_relatedMatch,
        okns:skos_scopeNote,
        okns:skos_semanticRelation,
        okns:skos_topConceptOf,
        okns:time_after,
        okns:time_before,
        okns:time_day,
        okns:time_dayOfWeek,
        okns:time_dayOfYear,
        okns:time_days,
        okns:time_entry_after,
        okns:time_entry_before,
        okns:time_entry_begins,
        okns:time_entry_calendarClockDescriptionDataType,
        okns:time_entry_calendarClockDescriptionOf,
        okns:time_entry_day,
        okns:time_entry_dayOfWeekField,
        okns:time_entry_dayOfYearField,
        okns:time_entry_days,
        okns:time_entry_durationDescriptionDataType,
        okns:time_entry_durationDescriptionOf,
        okns:time_entry_ends,
        okns:time_entry_firstInstantThing,
        okns:time_entry_hour,
        okns:time_entry_hours,
        okns:time_entry_inCalendarClock,
        okns:time_entry_inCalendarClockDataType,
        okns:time_entry_inside,
        okns:time_entry_instantPairDurationDescriptionDataType,
        okns:time_entry_instantPairDurationDescriptionOf,
        okns:time_entry_intAfter,
        okns:time_entry_intBefore,
        okns:time_entry_intContains,
        okns:time_entry_intDuring,
        okns:time_entry_intEquals,
        okns:time_entry_intFinishedBy,
        okns:time_entry_intFinishes,
        okns:time_entry_intMeets,
        okns:time_entry_intMetBy,
        okns:time_entry_intOverlappedBy,
        okns:time_entry_intOverlaps,
        okns:time_entry_intStartedBy,
        okns:time_entry_intStarts,
        okns:time_entry_minute,
        okns:time_entry_minutes,
        okns:time_entry_month,
        okns:time_entry_months,
        okns:time_entry_nonoverlap,
        okns:time_entry_second,
        okns:time_entry_secondInstantThing,
        okns:time_entry_seconds,
        okns:time_entry_startsOrDuring,
        okns:time_entry_timeZone,
        okns:time_entry_unitType,
        okns:time_entry_week,
        okns:time_entry_weeks,
        okns:time_entry_year,
        okns:time_entry_years,
        okns:time_hasBeginning,
        okns:time_hasDateTimeDescription,
        okns:time_hasDuration,
        okns:time_hasDurationDescription,
        okns:time_hasEnd,
        okns:time_hasTRS,
        okns:time_hasTemporalDuration,
        okns:time_hasTime,
        okns:time_hasXSDDuration,
        okns:time_hour,
        okns:time_hours,
        okns:time_inDateTime,
        okns:time_inTemporalPosition,
        okns:time_inTimePosition,
        okns:time_inXSDDate,
        okns:time_inXSDDateTime,
        okns:time_inXSDDateTimeStamp,
        okns:time_inXSDgYear,
        okns:time_inXSDgYearMonth,
        okns:time_inside,
        okns:time_intervalAfter,
        okns:time_intervalBefore,
        okns:time_intervalContains,
        okns:time_intervalDisjoint,
        okns:time_intervalDuring,
        okns:time_intervalEquals,
        okns:time_intervalFinishedBy,
        okns:time_intervalFinishes,
        okns:time_intervalIn,
        okns:time_intervalMeets,
        okns:time_intervalMetBy,
        okns:time_intervalOverlappedBy,
        okns:time_intervalOverlaps,
        okns:time_intervalStartedBy,
        okns:time_intervalStarts,
        okns:time_minute,
        okns:time_minutes,
        okns:time_month,
        okns:time_monthOfYear,
        okns:time_months,
        okns:time_nominalPosition,
        okns:time_numericDuration,
        okns:time_numericPosition,
        okns:time_second,
        okns:time_seconds,
        okns:time_timeZone,
        okns:time_unitType,
        okns:time_week,
        okns:time_weeks,
        okns:time_xsdDateTime,
        okns:time_year,
        okns:time_years,
        okns:tzont_DLSendDate,
        okns:tzont_DLSstartDate,
        okns:tzont_GMToffset,
        okns:tzont_countryOf,
        okns:tzont_exceptionalRegion,
        okns:tzont_hasAncestorRegion,
        okns:tzont_hasDaylightSavingsPolicy,
        okns:tzont_hasParentRegion,
        okns:tzont_hasTimeZone,
        okns:tzont_name,
        okns:tzont_observesDaylightSavingsTime,
        okns:tzont_stateOf,
        okns:tzont_timeZonePart,
        okns:vann_changes,
        okns:vann_preferredNamespacePrefix,
        okns:vann_preferredNamespaceUri,
        okns:wgs_alt,
        okns:wgs_lat,
        okns:wgs_lat_long,
        okns:wgs_location,
        okns:wgs_long,
        okns:wot_assurance,
        okns:wot_encryptedTo,
        okns:wot_encrypter,
        okns:wot_fingerprint,
        okns:wot_hasKey,
        okns:wot_hex_id,
        okns:wot_identity,
        okns:wot_length,
        okns:wot_pubkeyAddress,
        okns:wot_sigdate,
        okns:wot_signed,
        okns:wot_signer,
        okns:wot_sigtime,
        okns:wot_src_assurance,
        okns:xsd_pattern ;
    linkml:source_file_date "2025-09-03T11:22:55"^^xsd:dateTime ;
    linkml:source_file_size 105358 ;
    linkml:types okns:base64binary,
        okns:boolean,
        okns:curie,
        okns:date,
        okns:date_or_datetime,
        okns:datetime,
        okns:dct_Box,
        okns:dct_ISO3166,
        okns:dct_ISO639_2,
        okns:dct_ISO639_3,
        okns:dct_Period,
        okns:dct_Point,
        okns:dct_RFC1766,
        okns:dct_RFC3066,
        okns:dct_RFC4646,
        okns:dct_RFC5646,
        okns:dct_URI,
        okns:dct_W3CDTF,
        okns:decimal,
        okns:double,
        okns:float,
        okns:float16,
        okns:float32,
        okns:float64,
        okns:hexbinary,
        okns:int16,
        okns:int32,
        okns:int64,
        okns:int8,
        okns:integer,
        okns:jsonpath,
        okns:jsonpointer,
        okns:language,
        okns:name,
        okns:ncname,
        okns:negativeinteger,
        okns:nmtoken,
        okns:nodeidentifier,
        okns:nonpositiveinteger,
        okns:normalizedstring,
        okns:objectidentifier,
        okns:positiveinteger,
        okns:rational,
        okns:rdf_HTML,
        okns:rdf_JSON,
        okns:rdf_PlainLiteral,
        okns:rdf_XMLLiteral,
        okns:rdf_langString,
        okns:real,
        okns:signedinteger,
        okns:sparqlpath,
        okns:string,
        okns:time,
        okns:time_generalDay,
        okns:time_generalMonth,
        okns:time_generalYear,
        okns:token,
        okns:uint16,
        okns:uint32,
        okns:uint64,
        okns:uint8,
        okns:unsignedinteger,
        okns:uri,
        okns:uriorcurie .

okns:Any a linkml:ClassDefinition ;
    skos:definition "An unconstrained type or object" ;
    skos:inScheme okns:extended_types ;
    skos:mappingRelation linkml:Any ;
    linkml:class_uri linkml:Any ;
    linkml:definition_uri linkml:Any ;
    linkml:slot_usage [ ] .


