@prefix dcterms: <http://purl.org/dc/terms/> .
@prefix linkml: <https://w3id.org/linkml/> .
@prefix ns1: <xhv:> .
@prefix okn: <https://purl.org/okn/> .
@prefix okns: <https://purl.org/okn/schema/> .
@prefix owl: <http://www.w3.org/2002/07/owl#> .
@prefix pav: <http://purl.org/pav/> .
@prefix rdf: <http://www.w3.org/1999/02/22-rdf-syntax-ns#> .
@prefix rdfs: <http://www.w3.org/2000/01/rdf-schema#> .
@prefix schema1: <http://schema.org/> .
@prefix sh: <http://www.w3.org/ns/shacl#> .
@prefix shex: <http://www.w3.org/ns/shex#> .
@prefix skos: <http://www.w3.org/2004/02/skos/core#> .
@prefix xsd: <http://www.w3.org/2001/XMLSchema#> .

okns:base64binary a linkml:TypeDefinition ;
    skos:definition "Arbitrary Base64-encoded binary data." ;
    skos:inScheme okns:extended_types ;
    skos:note "added by Mahir Morshed <mmorshed@scripps.edu>",
        "used 'string' as base type since no 'binary' base type exists" ;
    linkml:base "string" ;
    linkml:definition_uri linkml:Base64binary ;
    linkml:uri xsd:hexBinary .

okns:boolean a linkml:TypeDefinition ;
    skos:definition "A binary (true or false) value" ;
    skos:editorialNote "If you are authoring schemas in LinkML YAML, the type is referenced with the lower case \"boolean\"." ;
    skos:exactMatch schema1:Boolean ;
    skos:inScheme linkml:types ;
    linkml:base "Bool" ;
    linkml:definition_uri linkml:Boolean ;
    linkml:imported_from "linkml:types" ;
    linkml:repr "bool" ;
    linkml:uri xsd:boolean .

okns:curie a linkml:TypeDefinition ;
    dcterms:conformsTo "https://www.w3.org/TR/curie/" ;
    skos:definition "a compact URI" ;
    skos:editorialNote "If you are authoring schemas in LinkML YAML, the type is referenced with the lower case \"curie\"." ;
    skos:inScheme linkml:types ;
    skos:note "in RDF serializations this MUST be expanded to a URI",
        "in non-RDF serializations MAY be serialized as the compact representation" ;
    linkml:base "Curie" ;
    linkml:definition_uri linkml:Curie ;
    linkml:imported_from "linkml:types" ;
    linkml:repr "str" ;
    linkml:uri xsd:string .

okns:date a linkml:TypeDefinition ;
    skos:definition "a date (year, month and day) in an idealized calendar" ;
    skos:editorialNote "If you are authoring schemas in LinkML YAML, the type is referenced with the lower case \"date\".",
        "URI is dateTime because OWL reasoners don't work with straight date or time" ;
    skos:exactMatch schema1:Date ;
    skos:inScheme linkml:types ;
    linkml:base "XSDDate" ;
    linkml:definition_uri linkml:Date ;
    linkml:imported_from "linkml:types" ;
    linkml:repr "str" ;
    linkml:uri xsd:date .

okns:date_or_datetime a linkml:TypeDefinition ;
    skos:definition "Either a date or a datetime" ;
    skos:editorialNote "If you are authoring schemas in LinkML YAML, the type is referenced with the lower case \"date_or_datetime\"." ;
    skos:inScheme linkml:types ;
    linkml:base "str" ;
    linkml:definition_uri linkml:DateOrDatetime ;
    linkml:imported_from "linkml:types" ;
    linkml:repr "str" ;
    linkml:uri linkml:DateOrDatetime .

okns:datetime a linkml:TypeDefinition ;
    skos:definition "The combination of a date and time" ;
    skos:editorialNote "If you are authoring schemas in LinkML YAML, the type is referenced with the lower case \"datetime\"." ;
    skos:exactMatch schema1:DateTime ;
    skos:inScheme linkml:types ;
    linkml:base "XSDDateTime" ;
    linkml:definition_uri linkml:Datetime ;
    linkml:imported_from "linkml:types" ;
    linkml:repr "str" ;
    linkml:uri xsd:dateTime .

okns:double a linkml:TypeDefinition ;
    skos:closeMatch schema1:Float ;
    skos:definition "A real number that conforms to the xsd:double specification" ;
    skos:editorialNote "If you are authoring schemas in LinkML YAML, the type is referenced with the lower case \"double\"." ;
    skos:inScheme linkml:types ;
    linkml:base "float" ;
    linkml:definition_uri linkml:Double ;
    linkml:imported_from "linkml:types" ;
    linkml:uri xsd:double .

okns:float16 a linkml:TypeDefinition ;
    rdfs:seeAlso <https://numpy.org/doc/stable/reference/arrays.scalars.html#numpy.half> ;
    skos:altLabel "e",
        "half" ;
    skos:definition "A 16-bit floating point number" ;
    skos:inScheme okns:extended_types ;
    linkml:base "float" ;
    linkml:definition_uri linkml:Float16 ;
    linkml:typeof okns:float ;
    linkml:uri xsd:float .

okns:float32 a linkml:TypeDefinition ;
    rdfs:seeAlso <https://numpy.org/doc/stable/reference/arrays.scalars.html#numpy.float32> ;
    skos:altLabel "f" ;
    skos:definition "A 32-bit floating point number" ;
    skos:inScheme okns:extended_types ;
    linkml:base "float" ;
    linkml:definition_uri linkml:Float32 ;
    linkml:typeof okns:float ;
    linkml:uri xsd:float .

okns:float64 a linkml:TypeDefinition ;
    rdfs:seeAlso <https://numpy.org/doc/stable/reference/arrays.scalars.html#numpy.float64> ;
    skos:altLabel "d" ;
    skos:definition "A 64-bit floating point number" ;
    skos:inScheme okns:extended_types ;
    linkml:base "float" ;
    linkml:definition_uri linkml:Float64 ;
    linkml:typeof okns:float ;
    linkml:uri xsd:float .

okns:hexbinary a linkml:TypeDefinition ;
    skos:definition "Arbitrary hex-encoded binary data." ;
    skos:inScheme okns:extended_types ;
    skos:note "added by Mahir Morshed <mmorshed@scripps.edu>",
        "used 'string' as base type since no 'binary' base type exists" ;
    linkml:base "string" ;
    linkml:definition_uri linkml:Hexbinary ;
    linkml:uri xsd:hexBinary .

okns:int16 a linkml:TypeDefinition ;
    rdfs:seeAlso <https://numpy.org/doc/stable/reference/arrays.scalars.html#numpy.short> ;
    skos:altLabel "h",
        "short" ;
    skos:definition "A 16-bit signed integer" ;
    skos:inScheme okns:extended_types ;
    skos:note "uri added by Mahir Morshed <mmorshed@scripps.edu>" ;
    linkml:base "int" ;
    linkml:definition_uri linkml:Int16 ;
    linkml:maximum_value "32767"^^<https://w3id.org/linkml/@id> ;
    linkml:minimum_value "-32768"^^<https://w3id.org/linkml/@id> ;
    linkml:typeof okns:signedinteger ;
    linkml:uri xsd:short .

okns:int32 a linkml:TypeDefinition ;
    rdfs:seeAlso <https://numpy.org/doc/stable/reference/arrays.scalars.html#numpy.intc> ;
    skos:altLabel "i",
        "intc" ;
    skos:definition "A 32-bit signed integer" ;
    skos:inScheme okns:extended_types ;
    skos:note "uri added by Mahir Morshed <mmorshed@scripps.edu>" ;
    linkml:base "int" ;
    linkml:definition_uri linkml:Int32 ;
    linkml:maximum_value "2147483647"^^<https://w3id.org/linkml/@id> ;
    linkml:minimum_value "-2147483648"^^<https://w3id.org/linkml/@id> ;
    linkml:typeof okns:signedinteger ;
    linkml:uri xsd:int .

okns:int64 a linkml:TypeDefinition ;
    rdfs:seeAlso <https://numpy.org/doc/stable/reference/arrays.scalars.html#numpy.int_> ;
    skos:altLabel "int_",
        "l",
        "long" ;
    skos:definition "A 64-bit signed integer" ;
    skos:inScheme okns:extended_types ;
    skos:note "uri added by Mahir Morshed <mmorshed@scripps.edu>" ;
    linkml:base "int" ;
    linkml:definition_uri linkml:Int64 ;
    linkml:maximum_value "9223372036854775807"^^<https://w3id.org/linkml/@id> ;
    linkml:minimum_value "-9223372036854775808"^^<https://w3id.org/linkml/@id> ;
    linkml:typeof okns:signedinteger ;
    linkml:uri xsd:long .

okns:int8 a linkml:TypeDefinition ;
    rdfs:seeAlso <https://numpy.org/doc/stable/reference/arrays.scalars.html#numpy.byte> ;
    skos:altLabel "b",
        "byte" ;
    skos:definition "An 8-bit signed integer" ;
    skos:inScheme okns:extended_types ;
    skos:note "uri added by Mahir Morshed <mmorshed@scripps.edu>" ;
    linkml:base "int" ;
    linkml:definition_uri linkml:Int8 ;
    linkml:maximum_value "127"^^<https://w3id.org/linkml/@id> ;
    linkml:minimum_value "-128"^^<https://w3id.org/linkml/@id> ;
    linkml:typeof okns:signedinteger ;
    linkml:uri xsd:byte .

okns:jsonpath a linkml:TypeDefinition ;
    dcterms:conformsTo "https://www.ietf.org/archive/id/draft-goessner-dispatch-jsonpath-00.html" ;
    skos:definition "A string encoding a JSON Path. The value of the string MUST conform to JSON Point syntax and SHOULD dereference to zero or more valid objects within the current instance document when encoded in tree form." ;
    skos:editorialNote "If you are authoring schemas in LinkML YAML, the type is referenced with the lower case \"jsonpath\"." ;
    skos:inScheme linkml:types ;
    linkml:base "str" ;
    linkml:definition_uri linkml:Jsonpath ;
    linkml:imported_from "linkml:types" ;
    linkml:repr "str" ;
    linkml:uri xsd:string .

okns:jsonpointer a linkml:TypeDefinition ;
    dcterms:conformsTo "https://datatracker.ietf.org/doc/html/rfc6901" ;
    skos:definition "A string encoding a JSON Pointer. The value of the string MUST conform to JSON Point syntax and SHOULD dereference to a valid object within the current instance document when encoded in tree form." ;
    skos:editorialNote "If you are authoring schemas in LinkML YAML, the type is referenced with the lower case \"jsonpointer\"." ;
    skos:inScheme linkml:types ;
    linkml:base "str" ;
    linkml:definition_uri linkml:Jsonpointer ;
    linkml:imported_from "linkml:types" ;
    linkml:repr "str" ;
    linkml:uri xsd:string .

okns:langrange a linkml:SlotDefinition ;
    skos:definition "Used to refer to a subset of strings containing a particular language tag." ;
    skos:inScheme okns:extended_types ;
    skos:mappingRelation rdf:langRange ;
    skos:note "added by Mahir Morshed <mmorshed@scripps.edu>" ;
    linkml:definition_uri linkml:langrange ;
    linkml:range okns:string ;
    linkml:slot_uri rdf:langRange .

okns:language a linkml:TypeDefinition ;
    skos:definition "Formal natural language identifier, as defined by [BCP 47] (currently represented by [RFC 4646] and [RFC 4647]) or its successor(s)." ;
    skos:inScheme okns:extended_types ;
    skos:note "added by Mahir Morshed <mmorshed@scripps.edu>" ;
    linkml:base "str" ;
    linkml:definition_uri linkml:Language ;
    linkml:typeof okns:token ;
    linkml:uri xsd:language .

okns:length a linkml:SlotDefinition ;
    skos:definition "Number of units of length, where units of length varies depending on the type that is being derived from." ;
    skos:inScheme okns:extended_types ;
    skos:mappingRelation xsd:length ;
    skos:note "added by Mahir Morshed <mmorshed@scripps.edu>" ;
    linkml:definition_uri linkml:length ;
    linkml:range okns:string ;
    linkml:slot_uri xsd:length .

okns:maxexclusive a linkml:SlotDefinition ;
    skos:definition "Exclusive upper bound of the ·value space· for a datatype with the ordered property." ;
    skos:inScheme okns:extended_types ;
    skos:mappingRelation xsd:maxExclusive ;
    skos:note "added by Mahir Morshed <mmorshed@scripps.edu>" ;
    linkml:definition_uri linkml:maxexclusive ;
    linkml:range okns:string ;
    linkml:slot_uri xsd:maxExclusive .

okns:maxlength a linkml:SlotDefinition ;
    skos:definition "Maximum number of units of length, where units of length varies depending on the type that is being derived from." ;
    skos:inScheme okns:extended_types ;
    skos:mappingRelation xsd:maxLength ;
    skos:note "added by Mahir Morshed <mmorshed@scripps.edu>" ;
    linkml:definition_uri linkml:maxlength ;
    linkml:range okns:string ;
    linkml:slot_uri xsd:maxLength .

okns:minexclusive a linkml:SlotDefinition ;
    skos:definition "Exclusive lower bound of the ·value space· for a datatype with the ordered property." ;
    skos:inScheme okns:extended_types ;
    skos:mappingRelation xsd:minExclusive ;
    skos:note "added by Mahir Morshed <mmorshed@scripps.edu>" ;
    linkml:definition_uri linkml:minexclusive ;
    linkml:range okns:string ;
    linkml:slot_uri xsd:minExclusive .

okns:minlength a linkml:SlotDefinition ;
    skos:definition "Minimum number of units of length, where units of length varies depending on the type that is being derived from." ;
    skos:inScheme okns:extended_types ;
    skos:mappingRelation xsd:minLength ;
    skos:note "added by Mahir Morshed <mmorshed@scripps.edu>" ;
    linkml:definition_uri linkml:minlength ;
    linkml:range okns:string ;
    linkml:slot_uri xsd:minLength .

okns:name a linkml:TypeDefinition ;
    skos:definition "XML Name." ;
    skos:inScheme okns:extended_types ;
    skos:note "added by Mahir Morshed <mmorshed@scripps.edu>" ;
    linkml:base "str" ;
    linkml:definition_uri linkml:Name ;
    linkml:typeof okns:token ;
    linkml:uri xsd:Name .

okns:ncname a linkml:TypeDefinition ;
    skos:definition "Prefix part of CURIE" ;
    skos:editorialNote "If you are authoring schemas in LinkML YAML, the type is referenced with the lower case \"ncname\"." ;
    skos:inScheme linkml:types ;
    linkml:base "NCName" ;
    linkml:definition_uri linkml:Ncname ;
    linkml:imported_from "linkml:types" ;
    linkml:repr "str" ;
    linkml:uri xsd:string .

okns:negativeinteger a linkml:TypeDefinition ;
    skos:definition "An integer that is negative" ;
    skos:inScheme okns:extended_types ;
    skos:note "added by Mahir Morshed <mmorshed@scripps.edu>" ;
    linkml:base "int" ;
    linkml:definition_uri linkml:Negativeinteger ;
    linkml:maximum_value "-1"^^<https://w3id.org/linkml/@id> ;
    linkml:typeof okns:integer ;
    linkml:uri xsd:negativeInteger .

okns:nmtoken a linkml:TypeDefinition ;
    skos:definition "NMTOKEN attribute type from [XML]." ;
    skos:inScheme okns:extended_types ;
    skos:note "added by Mahir Morshed <mmorshed@scripps.edu>" ;
    linkml:base "str" ;
    linkml:definition_uri linkml:Nmtoken ;
    linkml:typeof okns:token ;
    linkml:uri xsd:NMTOKEN .

okns:nodeidentifier a linkml:TypeDefinition ;
    skos:definition "A URI, CURIE or BNODE that represents a node in a model." ;
    skos:editorialNote "If you are authoring schemas in LinkML YAML, the type is referenced with the lower case \"nodeidentifier\"." ;
    skos:inScheme linkml:types ;
    linkml:base "NodeIdentifier" ;
    linkml:definition_uri linkml:Nodeidentifier ;
    linkml:imported_from "linkml:types" ;
    linkml:repr "str" ;
    linkml:uri shex:nonLiteral .

okns:nonpositiveinteger a linkml:TypeDefinition ;
    skos:definition "An integer that is not positive" ;
    skos:inScheme okns:extended_types ;
    skos:note "added by Mahir Morshed <mmorshed@scripps.edu>" ;
    linkml:base "int" ;
    linkml:definition_uri linkml:Nonpositiveinteger ;
    linkml:maximum_value "0"^^<https://w3id.org/linkml/@id> ;
    linkml:typeof okns:integer ;
    linkml:uri xsd:nonPositiveInteger .

okns:objectidentifier a linkml:TypeDefinition ;
    skos:definition "A URI or CURIE that represents an object in the model." ;
    skos:editorialNote "If you are authoring schemas in LinkML YAML, the type is referenced with the lower case \"objectidentifier\"." ;
    skos:inScheme linkml:types ;
    skos:note "Used for inheritance and type checking" ;
    linkml:base "ElementIdentifier" ;
    linkml:definition_uri linkml:Objectidentifier ;
    linkml:imported_from "linkml:types" ;
    linkml:repr "str" ;
    linkml:uri shex:iri .

okns:positiveinteger a linkml:TypeDefinition ;
    skos:definition "An integer that is positive" ;
    skos:inScheme okns:extended_types ;
    skos:note "added by Mahir Morshed <mmorshed@scripps.edu>" ;
    linkml:base "int" ;
    linkml:definition_uri linkml:Positiveinteger ;
    linkml:minimum_value "1"^^<https://w3id.org/linkml/@id> ;
    linkml:typeof okns:integer ;
    linkml:uri xsd:positiveInteger .

okns:rational a linkml:TypeDefinition ;
    skos:definition "Rational number." ;
    skos:inScheme okns:extended_types ;
    skos:note "added by Mahir Morshed <mmorshed@scripps.edu>" ;
    linkml:base "Decimal" ;
    linkml:definition_uri linkml:Rational ;
    linkml:typeof okns:decimal ;
    linkml:uri owl:rational .

okns:rdf_HTML a linkml:TypeDefinition ;
    dcterms:source rdf: ;
    dcterms:title "HTML" ;
    rdfs:seeAlso <http://www.w3.org/TR/rdf11-concepts/#section-html> ;
    skos:definition "The datatype of RDF literals storing fragments of HTML content" ;
    skos:inScheme okns:owl-rdf-rdfs ;
    linkml:base "str" ;
    linkml:definition_uri okns:RdfHTML ;
    linkml:typeof okns:string ;
    linkml:uri rdf:HTML .

okns:rdf_JSON a linkml:TypeDefinition ;
    dcterms:source rdf: ;
    dcterms:title "JSON" ;
    rdfs:seeAlso <https://www.w3.org/TR/json-ld11/#the-rdf-json-datatype> ;
    skos:definition "The datatype of RDF literals storing JSON content." ;
    skos:inScheme okns:owl-rdf-rdfs ;
    linkml:base "str" ;
    linkml:definition_uri okns:RdfJSON ;
    linkml:typeof okns:string ;
    linkml:uri rdf:JSON .

okns:rdf_PlainLiteral a linkml:TypeDefinition ;
    dcterms:source rdf: ;
    dcterms:title "PlainLiteral" ;
    rdfs:seeAlso <http://www.w3.org/TR/rdf-plain-literal/> ;
    skos:definition "The class of plain (i.e. untyped) literal values, as used in RIF and OWL 2" ;
    skos:inScheme okns:owl-rdf-rdfs ;
    linkml:base "str" ;
    linkml:definition_uri okns:RdfPlainLiteral ;
    linkml:typeof okns:string ;
    linkml:uri rdf:PlainLiteral .

okns:rdf_XMLLiteral a linkml:TypeDefinition ;
    dcterms:source rdf: ;
    dcterms:title "XMLLiteral" ;
    skos:definition "The datatype of XML literal values." ;
    skos:inScheme okns:owl-rdf-rdfs ;
    linkml:base "str" ;
    linkml:definition_uri okns:RdfXMLLiteral ;
    linkml:typeof okns:string ;
    linkml:uri rdf:XMLLiteral .

okns:rdf_langString a linkml:TypeDefinition ;
    dcterms:source rdf: ;
    dcterms:title "langString" ;
    rdfs:seeAlso <http://www.w3.org/TR/rdf11-concepts/#section-Graph-Literal> ;
    skos:definition "The datatype of language-tagged string values" ;
    skos:inScheme okns:owl-rdf-rdfs ;
    linkml:base "str" ;
    linkml:definition_uri okns:RdfLangString ;
    linkml:typeof okns:string ;
    linkml:uri rdf:langString .

okns:real a linkml:TypeDefinition ;
    skos:definition "Real number." ;
    skos:inScheme okns:extended_types ;
    skos:note "added by Mahir Morshed <mmorshed@scripps.edu>" ;
    linkml:base "Decimal" ;
    linkml:definition_uri linkml:Real ;
    linkml:typeof okns:decimal ;
    linkml:uri owl:real .

okns:sparqlpath a linkml:TypeDefinition ;
    dcterms:conformsTo "https://www.w3.org/TR/sparql11-query/#propertypaths" ;
    skos:definition "A string encoding a SPARQL Property Path. The value of the string MUST conform to SPARQL syntax and SHOULD dereference to zero or more valid objects within the current instance document when encoded as RDF." ;
    skos:editorialNote "If you are authoring schemas in LinkML YAML, the type is referenced with the lower case \"sparqlpath\"." ;
    skos:inScheme linkml:types ;
    linkml:base "str" ;
    linkml:definition_uri linkml:Sparqlpath ;
    linkml:imported_from "linkml:types" ;
    linkml:repr "str" ;
    linkml:uri xsd:string .

okns:time a linkml:TypeDefinition ;
    skos:definition "A time object represents a (local) time of day, independent of any particular day" ;
    skos:editorialNote "If you are authoring schemas in LinkML YAML, the type is referenced with the lower case \"time\".",
        "URI is dateTime because OWL reasoners do not work with straight date or time" ;
    skos:exactMatch schema1:Time ;
    skos:inScheme linkml:types ;
    linkml:base "XSDTime" ;
    linkml:definition_uri linkml:Time ;
    linkml:imported_from "linkml:types" ;
    linkml:repr "str" ;
    linkml:uri xsd:time .

okns:uint16 a linkml:TypeDefinition ;
    skos:altLabel "H",
        "ushort" ;
    skos:definition "A 16-bit unsigned integer" ;
    skos:inScheme okns:extended_types ;
    skos:note "uri added by Mahir Morshed <mmorshed@scripps.edu>" ;
    linkml:base "int" ;
    linkml:definition_uri linkml:Uint16 ;
    linkml:maximum_value "65535"^^<https://w3id.org/linkml/@id> ;
    linkml:minimum_value "0"^^<https://w3id.org/linkml/@id> ;
    linkml:typeof okns:unsignedinteger ;
    linkml:uri xsd:unsignedShort .

okns:uint32 a linkml:TypeDefinition ;
    skos:altLabel "I",
        "uintc" ;
    skos:definition "A 32-bit unsigned integer" ;
    skos:inScheme okns:extended_types ;
    skos:note "uri added by Mahir Morshed <mmorshed@scripps.edu>" ;
    linkml:base "int" ;
    linkml:definition_uri linkml:Uint32 ;
    linkml:maximum_value "4294967295"^^<https://w3id.org/linkml/@id> ;
    linkml:minimum_value "0"^^<https://w3id.org/linkml/@id> ;
    linkml:typeof okns:unsignedinteger ;
    linkml:uri xsd:unsignedInt .

okns:uint64 a linkml:TypeDefinition ;
    skos:altLabel "L",
        "uint_",
        "ulong" ;
    skos:definition "A 64-bit unsigned integer" ;
    skos:inScheme okns:extended_types ;
    skos:note "uri added by Mahir Morshed <mmorshed@scripps.edu>" ;
    linkml:base "int" ;
    linkml:definition_uri linkml:Uint64 ;
    linkml:maximum_value "18446744073709551615"^^<https://w3id.org/linkml/@id> ;
    linkml:minimum_value "0"^^<https://w3id.org/linkml/@id> ;
    linkml:typeof okns:unsignedinteger ;
    linkml:uri xsd:unsignedLong .

okns:uint8 a linkml:TypeDefinition ;
    rdfs:seeAlso <https://numpy.org/doc/stable/reference/arrays.scalars.html#numpy.uint8> ;
    skos:altLabel "B",
        "ubyte" ;
    skos:definition "An 8-bit unsigned integer" ;
    skos:inScheme okns:extended_types ;
    skos:note "uri added by Mahir Morshed <mmorshed@scripps.edu>" ;
    linkml:base "int" ;
    linkml:definition_uri linkml:Uint8 ;
    linkml:maximum_value "255"^^<https://w3id.org/linkml/@id> ;
    linkml:minimum_value "0"^^<https://w3id.org/linkml/@id> ;
    linkml:typeof okns:unsignedinteger ;
    linkml:uri xsd:unsignedByte .

okns:uriorcurie a linkml:TypeDefinition ;
    skos:definition "a URI or a CURIE" ;
    skos:editorialNote "If you are authoring schemas in LinkML YAML, the type is referenced with the lower case \"uriorcurie\"." ;
    skos:inScheme linkml:types ;
    linkml:base "URIorCURIE" ;
    linkml:definition_uri linkml:Uriorcurie ;
    linkml:imported_from "linkml:types" ;
    linkml:repr "str" ;
    linkml:uri xsd:anyURI .

okns:OwlAllDisjointClasses a linkml:ClassDefinition ;
    dcterms:source owl: ;
    dcterms:title "AllDisjointClasses" ;
    skos:definition "The class of collections of pairwise disjoint classes." ;
    skos:inScheme okns:owl-rdf-rdfs ;
    skos:mappingRelation owl:AllDisjointClasses ;
    linkml:class_uri owl:AllDisjointClasses ;
    linkml:definition_uri okns:OwlAllDisjointClasses ;
    linkml:is_a okns:RdfsResource ;
    linkml:slot_usage [ ] .

okns:OwlAllDisjointProperties a linkml:ClassDefinition ;
    dcterms:source owl: ;
    dcterms:title "AllDisjointProperties" ;
    skos:definition "The class of collections of pairwise disjoint properties." ;
    skos:inScheme okns:owl-rdf-rdfs ;
    skos:mappingRelation owl:AllDisjointProperties ;
    linkml:class_uri owl:AllDisjointProperties ;
    linkml:definition_uri okns:OwlAllDisjointProperties ;
    linkml:is_a okns:RdfsResource ;
    linkml:slot_usage [ ] .

okns:OwlAnnotation a linkml:ClassDefinition ;
    dcterms:source owl: ;
    dcterms:title "Annotation" ;
    skos:definition "The class of annotated annotations for which the RDF serialization consists of an annotated subject, predicate and object." ;
    skos:inScheme okns:owl-rdf-rdfs ;
    skos:mappingRelation owl:Annotation ;
    linkml:class_uri owl:Annotation ;
    linkml:definition_uri okns:OwlAnnotation ;
    linkml:is_a okns:RdfsResource ;
    linkml:slot_usage [ ] .

okns:OwlAnnotationProperty a linkml:ClassDefinition ;
    dcterms:source owl: ;
    dcterms:title "AnnotationProperty" ;
    skos:definition "The class of annotation properties." ;
    skos:inScheme okns:owl-rdf-rdfs ;
    skos:mappingRelation owl:AnnotationProperty ;
    linkml:class_uri owl:AnnotationProperty ;
    linkml:definition_uri okns:OwlAnnotationProperty ;
    linkml:is_a okns:RdfProperty ;
    linkml:slot_usage [ ] .

okns:OwlAsymmetricProperty a linkml:ClassDefinition ;
    dcterms:source owl: ;
    dcterms:title "AsymmetricProperty" ;
    skos:definition "The class of asymmetric properties." ;
    skos:inScheme okns:owl-rdf-rdfs ;
    skos:mappingRelation owl:AsymmetricProperty ;
    linkml:class_uri owl:AsymmetricProperty ;
    linkml:definition_uri okns:OwlAsymmetricProperty ;
    linkml:is_a okns:OwlObjectProperty ;
    linkml:slot_usage [ ] .

okns:OwlAxiom a linkml:ClassDefinition ;
    dcterms:source owl: ;
    dcterms:title "Axiom" ;
    skos:definition "The class of annotated axioms for which the RDF serialization consists of an annotated subject, predicate and object." ;
    skos:inScheme okns:owl-rdf-rdfs ;
    skos:mappingRelation owl:Axiom ;
    linkml:class_uri owl:Axiom ;
    linkml:definition_uri okns:OwlAxiom ;
    linkml:is_a okns:RdfsResource ;
    linkml:slot_usage [ ] .

okns:OwlDataRange a linkml:ClassDefinition ;
    dcterms:source owl: ;
    dcterms:title "DataRange" ;
    skos:definition "The class of OWL data ranges, which are special kinds of datatypes. Note: The use of the IRI owl:DataRange has been deprecated as of OWL 2. The IRI rdfs:Datatype SHOULD be used instead." ;
    skos:inScheme okns:owl-rdf-rdfs ;
    skos:mappingRelation owl:DataRange ;
    linkml:class_uri owl:DataRange ;
    linkml:definition_uri okns:OwlDataRange ;
    linkml:is_a okns:RdfsDatatype ;
    linkml:slot_usage [ ] ;
    linkml:slots okns:rdfs_comment,
        okns:rdfs_isDefinedBy,
        okns:rdfs_label,
        okns:rdfs_seeAlso,
        okns:rdfs_subClassOf .

okns:OwlDatatypeProperty a linkml:ClassDefinition ;
    dcterms:source owl: ;
    dcterms:title "DatatypeProperty" ;
    skos:definition "The class of data properties." ;
    skos:inScheme okns:owl-rdf-rdfs ;
    skos:mappingRelation owl:DatatypeProperty ;
    linkml:class_uri owl:DatatypeProperty ;
    linkml:definition_uri okns:OwlDatatypeProperty ;
    linkml:is_a okns:RdfProperty ;
    linkml:slot_usage [ ] .

okns:OwlDeprecatedClass a linkml:ClassDefinition ;
    dcterms:source owl: ;
    dcterms:title "DeprecatedClass" ;
    skos:definition "The class of deprecated classes." ;
    skos:inScheme okns:owl-rdf-rdfs ;
    skos:mappingRelation owl:DeprecatedClass ;
    linkml:class_uri owl:DeprecatedClass ;
    linkml:definition_uri okns:OwlDeprecatedClass ;
    linkml:is_a okns:RdfsClass ;
    linkml:slot_usage [ ] .

okns:OwlDeprecatedProperty a linkml:ClassDefinition ;
    dcterms:source owl: ;
    dcterms:title "DeprecatedProperty" ;
    skos:definition "The class of deprecated properties." ;
    skos:inScheme okns:owl-rdf-rdfs ;
    skos:mappingRelation owl:DeprecatedProperty ;
    linkml:class_uri owl:DeprecatedProperty ;
    linkml:definition_uri okns:OwlDeprecatedProperty ;
    linkml:is_a okns:RdfProperty ;
    linkml:slot_usage [ ] .

okns:OwlFunctionalProperty a linkml:ClassDefinition ;
    dcterms:source owl: ;
    dcterms:title "FunctionalProperty" ;
    skos:definition "The class of functional properties." ;
    skos:inScheme okns:owl-rdf-rdfs ;
    skos:mappingRelation owl:FunctionalProperty ;
    linkml:class_uri owl:FunctionalProperty ;
    linkml:definition_uri okns:OwlFunctionalProperty ;
    linkml:is_a okns:RdfProperty ;
    linkml:slot_usage [ ] .

okns:OwlInverseFunctionalProperty a linkml:ClassDefinition ;
    dcterms:source owl: ;
    dcterms:title "InverseFunctionalProperty" ;
    skos:definition "The class of inverse-functional properties." ;
    skos:inScheme okns:owl-rdf-rdfs ;
    skos:mappingRelation owl:InverseFunctionalProperty ;
    linkml:class_uri owl:InverseFunctionalProperty ;
    linkml:definition_uri okns:OwlInverseFunctionalProperty ;
    linkml:is_a okns:OwlObjectProperty ;
    linkml:slot_usage [ ] .

okns:OwlIrreflexiveProperty a linkml:ClassDefinition ;
    dcterms:source owl: ;
    dcterms:title "IrreflexiveProperty" ;
    skos:definition "The class of irreflexive properties." ;
    skos:inScheme okns:owl-rdf-rdfs ;
    skos:mappingRelation owl:IrreflexiveProperty ;
    linkml:class_uri owl:IrreflexiveProperty ;
    linkml:definition_uri okns:OwlIrreflexiveProperty ;
    linkml:is_a okns:OwlObjectProperty ;
    linkml:slot_usage [ ] .

okns:OwlNamedIndividual a linkml:ClassDefinition ;
    dcterms:source owl: ;
    dcterms:title "NamedIndividual" ;
    skos:definition "The class of named individuals." ;
    skos:inScheme okns:owl-rdf-rdfs ;
    skos:mappingRelation owl:NamedIndividual ;
    linkml:class_uri owl:NamedIndividual ;
    linkml:definition_uri okns:OwlNamedIndividual ;
    linkml:is_a okns:OwlThing ;
    linkml:slot_usage [ ] .

okns:OwlNothing a linkml:ClassDefinition ;
    dcterms:source owl: ;
    dcterms:title "Nothing" ;
    skos:definition "This is the empty class." ;
    skos:inScheme okns:owl-rdf-rdfs ;
    skos:mappingRelation owl:Nothing ;
    linkml:class_uri owl:Nothing ;
    linkml:definition_uri okns:OwlNothing ;
    linkml:is_a okns:OwlThing ;
    linkml:slot_usage [ ] .

okns:OwlOntologyProperty a linkml:ClassDefinition ;
    dcterms:source owl: ;
    dcterms:title "OntologyProperty" ;
    skos:definition "The class of ontology properties." ;
    skos:inScheme okns:owl-rdf-rdfs ;
    skos:mappingRelation owl:OntologyProperty ;
    linkml:class_uri owl:OntologyProperty ;
    linkml:definition_uri okns:OwlOntologyProperty ;
    linkml:is_a okns:RdfProperty ;
    linkml:slot_usage [ ] .

okns:OwlReflexiveProperty a linkml:ClassDefinition ;
    dcterms:source owl: ;
    dcterms:title "ReflexiveProperty" ;
    skos:definition "The class of reflexive properties." ;
    skos:inScheme okns:owl-rdf-rdfs ;
    skos:mappingRelation owl:ReflexiveProperty ;
    linkml:class_uri owl:ReflexiveProperty ;
    linkml:definition_uri okns:OwlReflexiveProperty ;
    linkml:is_a okns:OwlObjectProperty ;
    linkml:slot_usage [ ] .

okns:OwlSymmetricProperty a linkml:ClassDefinition ;
    dcterms:source owl: ;
    dcterms:title "SymmetricProperty" ;
    skos:definition "The class of symmetric properties." ;
    skos:inScheme okns:owl-rdf-rdfs ;
    skos:mappingRelation owl:SymmetricProperty ;
    linkml:class_uri owl:SymmetricProperty ;
    linkml:definition_uri okns:OwlSymmetricProperty ;
    linkml:is_a okns:OwlObjectProperty ;
    linkml:slot_usage [ ] .

okns:OwlTransitiveProperty a linkml:ClassDefinition ;
    dcterms:source owl: ;
    dcterms:title "TransitiveProperty" ;
    skos:definition "The class of transitive properties." ;
    skos:inScheme okns:owl-rdf-rdfs ;
    skos:mappingRelation owl:TransitiveProperty ;
    linkml:class_uri owl:TransitiveProperty ;
    linkml:definition_uri okns:OwlTransitiveProperty ;
    linkml:is_a okns:OwlObjectProperty ;
    linkml:slot_usage [ ] .

okns:RdfAlt a linkml:ClassDefinition ;
    dcterms:source rdf: ;
    dcterms:title "Alt" ;
    skos:definition "The class of containers of alternatives." ;
    skos:inScheme okns:owl-rdf-rdfs ;
    skos:mappingRelation rdf:Alt ;
    linkml:class_uri rdf:Alt ;
    linkml:definition_uri okns:RdfAlt ;
    linkml:is_a okns:RdfsContainer ;
    linkml:slot_usage [ ] .

okns:RdfBag a linkml:ClassDefinition ;
    dcterms:source rdf: ;
    dcterms:title "Bag" ;
    skos:definition "The class of unordered containers." ;
    skos:inScheme okns:owl-rdf-rdfs ;
    skos:mappingRelation rdf:Bag ;
    linkml:class_uri rdf:Bag ;
    linkml:definition_uri okns:RdfBag ;
    linkml:is_a okns:RdfsContainer ;
    linkml:slot_usage [ ] .

okns:RdfSeq a linkml:ClassDefinition ;
    dcterms:source rdf: ;
    dcterms:title "Seq" ;
    skos:definition "The class of ordered containers." ;
    skos:inScheme okns:owl-rdf-rdfs ;
    skos:mappingRelation rdf:Seq ;
    linkml:class_uri rdf:Seq ;
    linkml:definition_uri okns:RdfSeq ;
    linkml:is_a okns:RdfsContainer ;
    linkml:slot_usage [ ] .

okns:RdfsContainerMembershipProperty a linkml:ClassDefinition ;
    dcterms:source rdfs: ;
    dcterms:title "ContainerMembershipProperty" ;
    skos:definition "The class of container membership properties, rdf:_1, rdf:_2, ..., all of which are sub-properties of 'member'." ;
    skos:inScheme okns:owl-rdf-rdfs ;
    skos:mappingRelation rdfs:ContainerMembershipProperty ;
    linkml:class_uri rdfs:ContainerMembershipProperty ;
    linkml:definition_uri okns:RdfsContainerMembershipProperty ;
    linkml:is_a okns:RdfProperty ;
    linkml:slot_usage [ ] .

okns:normalizedstring a linkml:TypeDefinition ;
    skos:definition "Normalized string, one that does not contain the carriage return (#xD), line feed (#xA) nor tab (#x9) characters." ;
    skos:inScheme okns:extended_types ;
    skos:note "added by Mahir Morshed <mmorshed@scripps.edu>" ;
    linkml:base "str" ;
    linkml:definition_uri linkml:Normalizedstring ;
    linkml:typeof okns:string ;
    linkml:uri xsd:normalizedString .

okns:xhv_alert a linkml:SlotDefinition ;
    skos:definition "A message␊      with important, and usually time-sensitive, information. Also see alertdialog␊      and status." ;
    skos:editorialNote "No occurrences of this slot in the graph." ;
    skos:inScheme okns:xhv ;
    skos:mappingRelation <http://www.w3.org/1999/xhtml/vocab#alert> ;
    linkml:definition_uri okns:xhv_alert ;
    linkml:inlined true ;
    linkml:range okns:Any ;
    linkml:slot_uri <http://www.w3.org/1999/xhtml/vocab#alert> .

okns:xhv_alertdialog a linkml:SlotDefinition ;
    skos:definition "A␊      type of dialog that contains an alert message, where initial focus goes␊      an element within the dialog. Also see alert and dialog." ;
    skos:editorialNote "No occurrences of this slot in the graph." ;
    skos:inScheme okns:xhv ;
    skos:mappingRelation <http://www.w3.org/1999/xhtml/vocab#alertdialog> ;
    linkml:definition_uri okns:xhv_alertdialog ;
    linkml:inlined true ;
    linkml:range okns:Any ;
    linkml:slot_uri <http://www.w3.org/1999/xhtml/vocab#alertdialog> .

okns:xhv_alternate a linkml:SlotDefinition ;
    skos:definition "alternate ␊    designates alternate versions for a resource." ;
    skos:editorialNote "No occurrences of this slot in the graph." ;
    skos:inScheme okns:xhv ;
    skos:mappingRelation <http://www.w3.org/1999/xhtml/vocab#alternate> ;
    linkml:definition_uri okns:xhv_alternate ;
    linkml:inlined true ;
    linkml:range okns:Any ;
    linkml:slot_uri <http://www.w3.org/1999/xhtml/vocab#alternate> .

okns:xhv_appendix a linkml:SlotDefinition ;
    skos:definition "appendix refers to a resource serving␊      as an appendix in a collection." ;
    skos:editorialNote "No occurrences of this slot in the graph." ;
    skos:inScheme okns:xhv ;
    skos:mappingRelation <http://www.w3.org/1999/xhtml/vocab#appendix> ;
    linkml:definition_uri okns:xhv_appendix ;
    linkml:inlined true ;
    linkml:range okns:Any ;
    linkml:slot_uri <http://www.w3.org/1999/xhtml/vocab#appendix> .

okns:xhv_application a linkml:SlotDefinition ;
    skos:definition "A␊      region declared as a web application, as opposed to a web document." ;
    skos:editorialNote "No occurrences of this slot in the graph." ;
    skos:inScheme okns:xhv ;
    skos:mappingRelation <http://www.w3.org/1999/xhtml/vocab#application> ;
    linkml:definition_uri okns:xhv_application ;
    linkml:inlined true ;
    linkml:range okns:Any ;
    linkml:slot_uri <http://www.w3.org/1999/xhtml/vocab#application> .

okns:xhv_article a linkml:SlotDefinition ;
    skos:definition "A section␊      of a page that consists of a composition that forms an independent part␊      of a document, page, or site." ;
    skos:editorialNote "No occurrences of this slot in the graph." ;
    skos:inScheme okns:xhv ;
    skos:mappingRelation <http://www.w3.org/1999/xhtml/vocab#article> ;
    linkml:definition_uri okns:xhv_article ;
    linkml:inlined true ;
    linkml:range okns:Any ;
    linkml:slot_uri <http://www.w3.org/1999/xhtml/vocab#article> .

okns:xhv_banner a linkml:SlotDefinition ;
    skos:definition "contains␊      the prime heading or internal title of a page." ;
    skos:editorialNote "No occurrences of this slot in the graph." ;
    skos:inScheme okns:xhv ;
    skos:mappingRelation <http://www.w3.org/1999/xhtml/vocab#banner> ;
    linkml:definition_uri okns:xhv_banner ;
    linkml:inlined true ;
    linkml:range okns:Any ;
    linkml:slot_uri <http://www.w3.org/1999/xhtml/vocab#banner> .

okns:xhv_bookmark a linkml:SlotDefinition ;
    skos:definition "bookmark refers to a bookmark - a link␊      to a key entry point within an extended document." ;
    skos:editorialNote "No occurrences of this slot in the graph." ;
    skos:inScheme okns:xhv ;
    skos:mappingRelation <http://www.w3.org/1999/xhtml/vocab#bookmark> ;
    linkml:definition_uri okns:xhv_bookmark ;
    linkml:inlined true ;
    linkml:range okns:Any ;
    linkml:slot_uri <http://www.w3.org/1999/xhtml/vocab#bookmark> .

okns:xhv_button a linkml:SlotDefinition ;
    skos:definition "An input␊      that allows for user-triggered actions when clicked or pressed. Also see␊      link." ;
    skos:editorialNote "No occurrences of this slot in the graph." ;
    skos:inScheme okns:xhv ;
    skos:mappingRelation <http://www.w3.org/1999/xhtml/vocab#button> ;
    linkml:definition_uri okns:xhv_button ;
    linkml:inlined true ;
    linkml:range okns:Any ;
    linkml:slot_uri <http://www.w3.org/1999/xhtml/vocab#button> .

okns:xhv_chapter a linkml:SlotDefinition ;
    skos:definition "chapter refers to a resource serving␊      as a chapter in a collection." ;
    skos:editorialNote "No occurrences of this slot in the graph." ;
    skos:inScheme okns:xhv ;
    skos:mappingRelation <http://www.w3.org/1999/xhtml/vocab#chapter> ;
    linkml:definition_uri okns:xhv_chapter ;
    linkml:inlined true ;
    linkml:range okns:Any ;
    linkml:slot_uri <http://www.w3.org/1999/xhtml/vocab#chapter> .

okns:xhv_checkbox a linkml:SlotDefinition ;
    skos:definition "A checkable␊      input that has three possible values: true, false, or mixed." ;
    skos:editorialNote "No occurrences of this slot in the graph." ;
    skos:inScheme okns:xhv ;
    skos:mappingRelation <http://www.w3.org/1999/xhtml/vocab#checkbox> ;
    linkml:definition_uri okns:xhv_checkbox ;
    linkml:inlined true ;
    linkml:range okns:Any ;
    linkml:slot_uri <http://www.w3.org/1999/xhtml/vocab#checkbox> .

okns:xhv_cite a linkml:SlotDefinition ;
    skos:definition "cite refers to a resource that defines␊      a citation." ;
    skos:editorialNote "No occurrences of this slot in the graph." ;
    skos:inScheme okns:xhv ;
    skos:mappingRelation <http://www.w3.org/1999/xhtml/vocab#cite> ;
    linkml:definition_uri okns:xhv_cite ;
    linkml:inlined true ;
    linkml:range okns:Any ;
    linkml:slot_uri <http://www.w3.org/1999/xhtml/vocab#cite> .

okns:xhv_columnheader a linkml:SlotDefinition ;
    skos:definition "A␊      cell containing header information for a column." ;
    skos:editorialNote "No occurrences of this slot in the graph." ;
    skos:inScheme okns:xhv ;
    skos:mappingRelation <http://www.w3.org/1999/xhtml/vocab#columnheader> ;
    linkml:definition_uri okns:xhv_columnheader ;
    linkml:inlined true ;
    linkml:range okns:Any ;
    linkml:slot_uri <http://www.w3.org/1999/xhtml/vocab#columnheader> .

okns:xhv_combobox a linkml:SlotDefinition ;
    skos:definition "A presentation␊      of a select; usually similar to a textbox where users can type ahead to␊      select an option, or type to enter arbitrary text as a new item in the␊      list. Also see listbox." ;
    skos:editorialNote "No occurrences of this slot in the graph." ;
    skos:inScheme okns:xhv ;
    skos:mappingRelation <http://www.w3.org/1999/xhtml/vocab#combobox> ;
    linkml:definition_uri okns:xhv_combobox ;
    linkml:inlined true ;
    linkml:range okns:Any ;
    linkml:slot_uri <http://www.w3.org/1999/xhtml/vocab#combobox> .

okns:xhv_complementary a linkml:SlotDefinition ;
    skos:definition "indicates that the section supports but is␊      separable from the main content of resource." ;
    skos:editorialNote "No occurrences of this slot in the graph." ;
    skos:inScheme okns:xhv ;
    skos:mappingRelation <http://www.w3.org/1999/xhtml/vocab#complementary> ;
    linkml:definition_uri okns:xhv_complementary ;
    linkml:inlined true ;
    linkml:range okns:Any ;
    linkml:slot_uri <http://www.w3.org/1999/xhtml/vocab#complementary> .

okns:xhv_contentinfo a linkml:SlotDefinition ;
    skos:definition "contains meta information about the␊      content on the page or the page as a whole." ;
    skos:editorialNote "No occurrences of this slot in the graph." ;
    skos:inScheme okns:xhv ;
    skos:mappingRelation <http://www.w3.org/1999/xhtml/vocab#contentinfo> ;
    linkml:definition_uri okns:xhv_contentinfo ;
    linkml:inlined true ;
    linkml:range okns:Any ;
    linkml:slot_uri <http://www.w3.org/1999/xhtml/vocab#contentinfo> .

okns:xhv_contents a linkml:SlotDefinition ;
    skos:definition "contents refers to a resource serving␊      as a table of contents." ;
    skos:editorialNote "No occurrences of this slot in the graph." ;
    skos:inScheme okns:xhv ;
    skos:mappingRelation <http://www.w3.org/1999/xhtml/vocab#contents> ;
    linkml:definition_uri okns:xhv_contents ;
    linkml:inlined true ;
    linkml:range okns:Any ;
    linkml:slot_uri <http://www.w3.org/1999/xhtml/vocab#contents> .

okns:xhv_copyright a linkml:SlotDefinition ;
    skos:definition "copyright refers to a copyright␊      statement for the resource." ;
    skos:editorialNote "No occurrences of this slot in the graph." ;
    skos:inScheme okns:xhv ;
    skos:mappingRelation <http://www.w3.org/1999/xhtml/vocab#copyright> ;
    linkml:definition_uri okns:xhv_copyright ;
    linkml:inlined true ;
    linkml:range okns:Any ;
    linkml:slot_uri <http://www.w3.org/1999/xhtml/vocab#copyright> .

okns:xhv_definition a linkml:SlotDefinition ;
    skos:definition "indicates the definition of a term or concept." ;
    skos:editorialNote "No occurrences of this slot in the graph." ;
    skos:inScheme okns:xhv ;
    skos:mappingRelation <http://www.w3.org/1999/xhtml/vocab#definition> ;
    linkml:definition_uri okns:xhv_definition ;
    linkml:inlined true ;
    linkml:range okns:Any ;
    linkml:slot_uri <http://www.w3.org/1999/xhtml/vocab#definition> .

okns:xhv_dialog a linkml:SlotDefinition ;
    skos:definition "A dialog␊      is an application window that is designed to interrupt the current processing␊      of an application in order to prompt the user to enter information or require␊      a response. Also see alertdialog." ;
    skos:editorialNote "No occurrences of this slot in the graph." ;
    skos:inScheme okns:xhv ;
    skos:mappingRelation <http://www.w3.org/1999/xhtml/vocab#dialog> ;
    linkml:definition_uri okns:xhv_dialog ;
    linkml:inlined true ;
    linkml:range okns:Any ;
    linkml:slot_uri <http://www.w3.org/1999/xhtml/vocab#dialog> .

okns:xhv_directory a linkml:SlotDefinition ;
    skos:definition "A list␊      of references to members of a group, such as a static table of contents." ;
    skos:editorialNote "No occurrences of this slot in the graph." ;
    skos:inScheme okns:xhv ;
    skos:mappingRelation <http://www.w3.org/1999/xhtml/vocab#directory> ;
    linkml:definition_uri okns:xhv_directory ;
    linkml:inlined true ;
    linkml:range okns:Any ;
    linkml:slot_uri <http://www.w3.org/1999/xhtml/vocab#directory> .

okns:xhv_document a linkml:SlotDefinition ;
    skos:definition "A region␊      containing related information that is declared as document content, as␊      opposed to a web application." ;
    skos:editorialNote "No occurrences of this slot in the graph." ;
    skos:inScheme okns:xhv ;
    skos:mappingRelation <http://www.w3.org/1999/xhtml/vocab#document> ;
    linkml:definition_uri okns:xhv_document ;
    linkml:inlined true ;
    linkml:range okns:Any ;
    linkml:slot_uri <http://www.w3.org/1999/xhtml/vocab#document> .

okns:xhv_first a linkml:SlotDefinition ;
    skos:definition "first refers the first item in a␊      collection (see also start and top)." ;
    skos:editorialNote "No occurrences of this slot in the graph." ;
    skos:inScheme okns:xhv ;
    skos:mappingRelation <http://www.w3.org/1999/xhtml/vocab#first> ;
    linkml:definition_uri okns:xhv_first ;
    linkml:inlined true ;
    linkml:range okns:Any ;
    linkml:slot_uri <http://www.w3.org/1999/xhtml/vocab#first> .

okns:xhv_form a linkml:SlotDefinition ;
    skos:definition "A landmark␊      region that contains a collection of items and objects that, as a whole,␊      combine to create a form. Also see search." ;
    skos:editorialNote "No occurrences of this slot in the graph." ;
    skos:inScheme okns:xhv ;
    skos:mappingRelation <http://www.w3.org/1999/xhtml/vocab#form> ;
    linkml:definition_uri okns:xhv_form ;
    linkml:inlined true ;
    linkml:range okns:Any ;
    linkml:slot_uri <http://www.w3.org/1999/xhtml/vocab#form> .

okns:xhv_glossary a linkml:SlotDefinition ;
    skos:definition "glossary refers to a resource␊      providing a glossary of terms." ;
    skos:editorialNote "No occurrences of this slot in the graph." ;
    skos:inScheme okns:xhv ;
    skos:mappingRelation <http://www.w3.org/1999/xhtml/vocab#glossary> ;
    linkml:definition_uri okns:xhv_glossary ;
    linkml:inlined true ;
    linkml:range okns:Any ;
    linkml:slot_uri <http://www.w3.org/1999/xhtml/vocab#glossary> .

okns:xhv_grid a linkml:SlotDefinition ;
    skos:definition "A grid is␊      an interactive control which contains cells of tabular data arranged in␊      rows and columns, like a table." ;
    skos:editorialNote "No occurrences of this slot in the graph." ;
    skos:inScheme okns:xhv ;
    skos:mappingRelation <http://www.w3.org/1999/xhtml/vocab#grid> ;
    linkml:definition_uri okns:xhv_grid ;
    linkml:inlined true ;
    linkml:range okns:Any ;
    linkml:slot_uri <http://www.w3.org/1999/xhtml/vocab#grid> .

okns:xhv_gridcell a linkml:SlotDefinition ;
    skos:definition "A cell␊      in a grid or treegrid." ;
    skos:editorialNote "No occurrences of this slot in the graph." ;
    skos:inScheme okns:xhv ;
    skos:mappingRelation <http://www.w3.org/1999/xhtml/vocab#gridcell> ;
    linkml:definition_uri okns:xhv_gridcell ;
    linkml:inlined true ;
    linkml:range okns:Any ;
    linkml:slot_uri <http://www.w3.org/1999/xhtml/vocab#gridcell> .

okns:xhv_group a linkml:SlotDefinition ;
    skos:definition "A set of␊      user interface objects which are not intended to be included in a page␊      summary or table of contents by assistive technologies." ;
    skos:editorialNote "No occurrences of this slot in the graph." ;
    skos:inScheme okns:xhv ;
    skos:mappingRelation <http://www.w3.org/1999/xhtml/vocab#group> ;
    linkml:definition_uri okns:xhv_group ;
    linkml:inlined true ;
    linkml:range okns:Any ;
    linkml:slot_uri <http://www.w3.org/1999/xhtml/vocab#group> .

okns:xhv_heading a linkml:SlotDefinition ;
    skos:definition "A heading␊      for a section of the page." ;
    skos:editorialNote "No occurrences of this slot in the graph." ;
    skos:inScheme okns:xhv ;
    skos:mappingRelation <http://www.w3.org/1999/xhtml/vocab#heading> ;
    linkml:definition_uri okns:xhv_heading ;
    linkml:inlined true ;
    linkml:range okns:Any ;
    linkml:slot_uri <http://www.w3.org/1999/xhtml/vocab#heading> .

okns:xhv_help a linkml:SlotDefinition ;
    skos:definition "help refers to a resource offering␊      help." ;
    skos:editorialNote "No occurrences of this slot in the graph." ;
    skos:inScheme okns:xhv ;
    skos:mappingRelation <http://www.w3.org/1999/xhtml/vocab#help> ;
    linkml:definition_uri okns:xhv_help ;
    linkml:inlined true ;
    linkml:range okns:Any ;
    linkml:slot_uri <http://www.w3.org/1999/xhtml/vocab#help> .

okns:xhv_icon a linkml:SlotDefinition ;
    skos:definition "icon refers to a resource that␊      represents an icon." ;
    skos:editorialNote "No occurrences of this slot in the graph." ;
    skos:inScheme okns:xhv ;
    skos:mappingRelation <http://www.w3.org/1999/xhtml/vocab#icon> ;
    linkml:definition_uri okns:xhv_icon ;
    linkml:inlined true ;
    linkml:range okns:Any ;
    linkml:slot_uri <http://www.w3.org/1999/xhtml/vocab#icon> .

okns:xhv_img a linkml:SlotDefinition ;
    skos:definition "A container␊      for a collection of elements that form an image." ;
    skos:editorialNote "No occurrences of this slot in the graph." ;
    skos:inScheme okns:xhv ;
    skos:mappingRelation <http://www.w3.org/1999/xhtml/vocab#img> ;
    linkml:definition_uri okns:xhv_img ;
    linkml:inlined true ;
    linkml:range okns:Any ;
    linkml:slot_uri <http://www.w3.org/1999/xhtml/vocab#img> .

okns:xhv_index a linkml:SlotDefinition ;
    skos:definition "index refers to a resource providing␊      an index." ;
    skos:editorialNote "No occurrences of this slot in the graph." ;
    skos:inScheme okns:xhv ;
    skos:mappingRelation <http://www.w3.org/1999/xhtml/vocab#index> ;
    linkml:definition_uri okns:xhv_index ;
    linkml:inlined true ;
    linkml:range okns:Any ;
    linkml:slot_uri <http://www.w3.org/1999/xhtml/vocab#index> .

okns:xhv_itsRules a linkml:SlotDefinition ;
    skos:definition "itsRules indicates that the designated␊      resource is an [ITS] rule set." ;
    skos:editorialNote "No occurrences of this slot in the graph." ;
    skos:inScheme okns:xhv ;
    skos:mappingRelation <http://www.w3.org/1999/xhtml/vocab#itsRules> ;
    linkml:definition_uri okns:xhv_itsRules ;
    linkml:inlined true ;
    linkml:range okns:Any ;
    linkml:slot_uri <http://www.w3.org/1999/xhtml/vocab#itsRules> .

okns:xhv_last a linkml:SlotDefinition ;
    skos:definition "last refers to the last resource in a␊      collection of resources." ;
    skos:editorialNote "No occurrences of this slot in the graph." ;
    skos:inScheme okns:xhv ;
    skos:mappingRelation <http://www.w3.org/1999/xhtml/vocab#last> ;
    linkml:definition_uri okns:xhv_last ;
    linkml:inlined true ;
    linkml:range okns:Any ;
    linkml:slot_uri <http://www.w3.org/1999/xhtml/vocab#last> .

okns:xhv_license a linkml:SlotDefinition ;
    skos:definition "license refers to a resource that␊      defines the associated license." ;
    skos:editorialNote "No occurrences of this slot in the graph." ;
    skos:inScheme okns:xhv ;
    skos:mappingRelation <http://www.w3.org/1999/xhtml/vocab#license> ;
    linkml:definition_uri okns:xhv_license ;
    linkml:inlined true ;
    linkml:range okns:Any ;
    linkml:slot_uri <http://www.w3.org/1999/xhtml/vocab#license> .

okns:xhv_link a linkml:SlotDefinition ;
    skos:definition "An interactive␊      reference to an internal or external resource that, when activated, causes␊      the user agent to navigate to that resource. Also see button." ;
    skos:editorialNote "No occurrences of this slot in the graph." ;
    skos:inScheme okns:xhv ;
    skos:mappingRelation <http://www.w3.org/1999/xhtml/vocab#link> ;
    linkml:definition_uri okns:xhv_link ;
    linkml:inlined true ;
    linkml:range okns:Any ;
    linkml:slot_uri <http://www.w3.org/1999/xhtml/vocab#link> .

okns:xhv_list a linkml:SlotDefinition ;
    skos:definition "A group of␊      non-interactive list items. Also see listbox." ;
    skos:editorialNote "No occurrences of this slot in the graph." ;
    skos:inScheme okns:xhv ;
    skos:mappingRelation <http://www.w3.org/1999/xhtml/vocab#list> ;
    linkml:definition_uri okns:xhv_list ;
    linkml:inlined true ;
    linkml:range okns:Any ;
    linkml:slot_uri <http://www.w3.org/1999/xhtml/vocab#list> .

okns:xhv_listbox a linkml:SlotDefinition ;
    skos:definition "A widget␊      that allows the user to select one or more items from a list of choices.␊      Also see combobox and list." ;
    skos:editorialNote "No occurrences of this slot in the graph." ;
    skos:inScheme okns:xhv ;
    skos:mappingRelation <http://www.w3.org/1999/xhtml/vocab#listbox> ;
    linkml:definition_uri okns:xhv_listbox ;
    linkml:inlined true ;
    linkml:range okns:Any ;
    linkml:slot_uri <http://www.w3.org/1999/xhtml/vocab#listbox> .

okns:xhv_listitem a linkml:SlotDefinition ;
    skos:definition "A single␊      item in a list or directory." ;
    skos:editorialNote "No occurrences of this slot in the graph." ;
    skos:inScheme okns:xhv ;
    skos:mappingRelation <http://www.w3.org/1999/xhtml/vocab#listitem> ;
    linkml:definition_uri okns:xhv_listitem ;
    linkml:inlined true ;
    linkml:range okns:Any ;
    linkml:slot_uri <http://www.w3.org/1999/xhtml/vocab#listitem> .

okns:xhv_log a linkml:SlotDefinition ;
    skos:definition "A type of␊      live region where new information is added in meaningful order and old␊      information may disappear. Also see marquee." ;
    skos:editorialNote "No occurrences of this slot in the graph." ;
    skos:inScheme okns:xhv ;
    skos:mappingRelation <http://www.w3.org/1999/xhtml/vocab#log> ;
    linkml:definition_uri okns:xhv_log ;
    linkml:inlined true ;
    linkml:range okns:Any ;
    linkml:slot_uri <http://www.w3.org/1999/xhtml/vocab#log> .

okns:xhv_main a linkml:SlotDefinition ;
    skos:definition "acts as the␊      main content of the document." ;
    skos:editorialNote "No occurrences of this slot in the graph." ;
    skos:inScheme okns:xhv ;
    skos:mappingRelation <http://www.w3.org/1999/xhtml/vocab#main> ;
    linkml:definition_uri okns:xhv_main ;
    linkml:inlined true ;
    linkml:range okns:Any ;
    linkml:slot_uri <http://www.w3.org/1999/xhtml/vocab#main> .

okns:xhv_marquee a linkml:SlotDefinition ;
    skos:definition "A type␊      of live region where non-essential information changes frequently. Also␊      see log." ;
    skos:editorialNote "No occurrences of this slot in the graph." ;
    skos:inScheme okns:xhv ;
    skos:mappingRelation <http://www.w3.org/1999/xhtml/vocab#marquee> ;
    linkml:definition_uri okns:xhv_marquee ;
    linkml:inlined true ;
    linkml:range okns:Any ;
    linkml:slot_uri <http://www.w3.org/1999/xhtml/vocab#marquee> .

okns:xhv_math a linkml:SlotDefinition ;
    skos:definition "Content that␊      represents a mathematical expression." ;
    skos:editorialNote "No occurrences of this slot in the graph." ;
    skos:inScheme okns:xhv ;
    skos:mappingRelation <http://www.w3.org/1999/xhtml/vocab#math> ;
    linkml:definition_uri okns:xhv_math ;
    linkml:inlined true ;
    linkml:range okns:Any ;
    linkml:slot_uri <http://www.w3.org/1999/xhtml/vocab#math> .

okns:xhv_menu a linkml:SlotDefinition ;
    skos:definition "A type of␊      widget that offers a list of choices to the user." ;
    skos:editorialNote "No occurrences of this slot in the graph." ;
    skos:inScheme okns:xhv ;
    skos:mappingRelation <http://www.w3.org/1999/xhtml/vocab#menu> ;
    linkml:definition_uri okns:xhv_menu ;
    linkml:inlined true ;
    linkml:range okns:Any ;
    linkml:slot_uri <http://www.w3.org/1999/xhtml/vocab#menu> .

okns:xhv_menubar a linkml:SlotDefinition ;
    skos:definition "A presentation␊      of menu that usually remains visible and is usually presented horizontally." ;
    skos:editorialNote "No occurrences of this slot in the graph." ;
    skos:inScheme okns:xhv ;
    skos:mappingRelation <http://www.w3.org/1999/xhtml/vocab#menubar> ;
    linkml:definition_uri okns:xhv_menubar ;
    linkml:inlined true ;
    linkml:range okns:Any ;
    linkml:slot_uri <http://www.w3.org/1999/xhtml/vocab#menubar> .

okns:xhv_menuitem a linkml:SlotDefinition ;
    skos:definition "An option␊      in a group of choices contained by a menu or menubar." ;
    skos:editorialNote "No occurrences of this slot in the graph." ;
    skos:inScheme okns:xhv ;
    skos:mappingRelation <http://www.w3.org/1999/xhtml/vocab#menuitem> ;
    linkml:definition_uri okns:xhv_menuitem ;
    linkml:inlined true ;
    linkml:range okns:Any ;
    linkml:slot_uri <http://www.w3.org/1999/xhtml/vocab#menuitem> .

okns:xhv_menuitemcheckbox a linkml:SlotDefinition ;
    skos:definition "A␊      checkable menuitem that has three possible values: true, false, or mixed." ;
    skos:editorialNote "No occurrences of this slot in the graph." ;
    skos:inScheme okns:xhv ;
    skos:mappingRelation <http://www.w3.org/1999/xhtml/vocab#menuitemcheckbox> ;
    linkml:definition_uri okns:xhv_menuitemcheckbox ;
    linkml:inlined true ;
    linkml:range okns:Any ;
    linkml:slot_uri <http://www.w3.org/1999/xhtml/vocab#menuitemcheckbox> .

okns:xhv_menuitemradio a linkml:SlotDefinition ;
    skos:definition "A␊      checkable menuitem in a group of menuitemradio roles, only one of which␊      can be checked at a time." ;
    skos:editorialNote "No occurrences of this slot in the graph." ;
    skos:inScheme okns:xhv ;
    skos:mappingRelation <http://www.w3.org/1999/xhtml/vocab#menuitemradio> ;
    linkml:definition_uri okns:xhv_menuitemradio ;
    linkml:inlined true ;
    linkml:range okns:Any ;
    linkml:slot_uri <http://www.w3.org/1999/xhtml/vocab#menuitemradio> .

okns:xhv_meta a linkml:SlotDefinition ;
    skos:definition "meta refers to a resource that␊      provides metadata." ;
    skos:editorialNote "No occurrences of this slot in the graph." ;
    skos:inScheme okns:xhv ;
    skos:mappingRelation <http://www.w3.org/1999/xhtml/vocab#meta> ;
    linkml:definition_uri okns:xhv_meta ;
    linkml:inlined true ;
    linkml:range okns:Any ;
    linkml:slot_uri <http://www.w3.org/1999/xhtml/vocab#meta> .

okns:xhv_navigation a linkml:SlotDefinition ;
    skos:definition "indicates a collection of items suitable for␊      navigating the document or related documents." ;
    skos:editorialNote "No occurrences of this slot in the graph." ;
    skos:inScheme okns:xhv ;
    skos:mappingRelation <http://www.w3.org/1999/xhtml/vocab#navigation> ;
    linkml:definition_uri okns:xhv_navigation ;
    linkml:inlined true ;
    linkml:range okns:Any ;
    linkml:slot_uri <http://www.w3.org/1999/xhtml/vocab#navigation> .

okns:xhv_next a linkml:SlotDefinition ;
    skos:definition "next refers to the next resource␊      (after the current one) in an ordered collection of resources." ;
    skos:editorialNote "No occurrences of this slot in the graph." ;
    skos:inScheme okns:xhv ;
    skos:mappingRelation <http://www.w3.org/1999/xhtml/vocab#next> ;
    linkml:definition_uri okns:xhv_next ;
    linkml:inlined true ;
    linkml:range okns:Any ;
    linkml:slot_uri <http://www.w3.org/1999/xhtml/vocab#next> .

okns:xhv_note a linkml:SlotDefinition ;
    skos:definition "indicates␊      the content is parenthetic or ancillary to the main content of the␊      resource." ;
    skos:editorialNote "No occurrences of this slot in the graph." ;
    skos:inScheme okns:xhv ;
    skos:mappingRelation <http://www.w3.org/1999/xhtml/vocab#note> ;
    linkml:definition_uri okns:xhv_note ;
    linkml:inlined true ;
    linkml:range okns:Any ;
    linkml:slot_uri <http://www.w3.org/1999/xhtml/vocab#note> .

okns:xhv_option a linkml:SlotDefinition ;
    skos:definition "A selectable␊      item in a select list." ;
    skos:editorialNote "No occurrences of this slot in the graph." ;
    skos:inScheme okns:xhv ;
    skos:mappingRelation <http://www.w3.org/1999/xhtml/vocab#option> ;
    linkml:definition_uri okns:xhv_option ;
    linkml:inlined true ;
    linkml:range okns:Any ;
    linkml:slot_uri <http://www.w3.org/1999/xhtml/vocab#option> .

okns:xhv_p3pv1 a linkml:SlotDefinition ;
    skos:definition "p3pv1 refers to a P3P Policy Reference␊      File [P3P]." ;
    skos:editorialNote "No occurrences of this slot in the graph." ;
    skos:inScheme okns:xhv ;
    skos:mappingRelation <http://www.w3.org/1999/xhtml/vocab#p3pv1> ;
    linkml:definition_uri okns:xhv_p3pv1 ;
    linkml:inlined true ;
    linkml:range okns:Any ;
    linkml:slot_uri <http://www.w3.org/1999/xhtml/vocab#p3pv1> .

okns:xhv_presentation a linkml:SlotDefinition ;
    skos:definition "An␊      element whose implicit native role semantics will not be mapped to the␊      accessibility API." ;
    skos:editorialNote "No occurrences of this slot in the graph." ;
    skos:inScheme okns:xhv ;
    skos:mappingRelation <http://www.w3.org/1999/xhtml/vocab#presentation> ;
    linkml:definition_uri okns:xhv_presentation ;
    linkml:inlined true ;
    linkml:range okns:Any ;
    linkml:slot_uri <http://www.w3.org/1999/xhtml/vocab#presentation> .

okns:xhv_prev a linkml:SlotDefinition ;
    skos:definition "prev refers to a previous resource␊      (before the current one) in an ordered collection of resources." ;
    skos:editorialNote "No occurrences of this slot in the graph." ;
    skos:inScheme okns:xhv ;
    skos:mappingRelation <http://www.w3.org/1999/xhtml/vocab#prev> ;
    linkml:definition_uri okns:xhv_prev ;
    linkml:inlined true ;
    linkml:range okns:Any ;
    linkml:slot_uri <http://www.w3.org/1999/xhtml/vocab#prev> .

okns:xhv_progressbar a linkml:SlotDefinition ;
    skos:definition "An␊      element that displays the progress status for tasks that take a long time." ;
    skos:editorialNote "No occurrences of this slot in the graph." ;
    skos:inScheme okns:xhv ;
    skos:mappingRelation <http://www.w3.org/1999/xhtml/vocab#progressbar> ;
    linkml:definition_uri okns:xhv_progressbar ;
    linkml:inlined true ;
    linkml:range okns:Any ;
    linkml:slot_uri <http://www.w3.org/1999/xhtml/vocab#progressbar> .

okns:xhv_radio a linkml:SlotDefinition ;
    skos:definition "A checkable␊      input in a group of radio roles, only one of which can be checked at a␊      time." ;
    skos:editorialNote "No occurrences of this slot in the graph." ;
    skos:inScheme okns:xhv ;
    skos:mappingRelation <http://www.w3.org/1999/xhtml/vocab#radio> ;
    linkml:definition_uri okns:xhv_radio ;
    linkml:inlined true ;
    linkml:range okns:Any ;
    linkml:slot_uri <http://www.w3.org/1999/xhtml/vocab#radio> .

okns:xhv_radiogroup a linkml:SlotDefinition ;
    skos:definition "A group␊      of radio buttons." ;
    skos:editorialNote "No occurrences of this slot in the graph." ;
    skos:inScheme okns:xhv ;
    skos:mappingRelation <http://www.w3.org/1999/xhtml/vocab#radiogroup> ;
    linkml:definition_uri okns:xhv_radiogroup ;
    linkml:inlined true ;
    linkml:range okns:Any ;
    linkml:slot_uri <http://www.w3.org/1999/xhtml/vocab#radiogroup> .

okns:xhv_region a linkml:SlotDefinition ;
    skos:definition "A large␊      perceivable section of a web page or document, that the author feels is␊      important enough to be included in a page summary or table of contents,␊      for example, an area of the page containing live sporting event statistics." ;
    skos:editorialNote "No occurrences of this slot in the graph." ;
    skos:inScheme okns:xhv ;
    skos:mappingRelation <http://www.w3.org/1999/xhtml/vocab#region> ;
    linkml:definition_uri okns:xhv_region ;
    linkml:inlined true ;
    linkml:range okns:Any ;
    linkml:slot_uri <http://www.w3.org/1999/xhtml/vocab#region> .

okns:xhv_role a linkml:SlotDefinition ;
    skos:definition "role indicates the purpose of the␊      resource. See the XHTML Role␊      Vocabulary for roles in this vocabulary space, and XHTMLROLE for information on extending the␊      collection of roles." ;
    skos:editorialNote "No occurrences of this slot in the graph." ;
    skos:inScheme okns:xhv ;
    skos:mappingRelation <http://www.w3.org/1999/xhtml/vocab#role> ;
    linkml:definition_uri okns:xhv_role ;
    linkml:inlined true ;
    linkml:range okns:Any ;
    linkml:slot_uri <http://www.w3.org/1999/xhtml/vocab#role> .

okns:xhv_row a linkml:SlotDefinition ;
    skos:definition "A row of cells␊      in a grid." ;
    skos:editorialNote "No occurrences of this slot in the graph." ;
    skos:inScheme okns:xhv ;
    skos:mappingRelation <http://www.w3.org/1999/xhtml/vocab#row> ;
    linkml:definition_uri okns:xhv_row ;
    linkml:inlined true ;
    linkml:range okns:Any ;
    linkml:slot_uri <http://www.w3.org/1999/xhtml/vocab#row> .

okns:xhv_rowgroup a linkml:SlotDefinition ;
    skos:definition "A group␊      containing one or more row elements in a grid." ;
    skos:editorialNote "No occurrences of this slot in the graph." ;
    skos:inScheme okns:xhv ;
    skos:mappingRelation <http://www.w3.org/1999/xhtml/vocab#rowgroup> ;
    linkml:definition_uri okns:xhv_rowgroup ;
    linkml:inlined true ;
    linkml:range okns:Any ;
    linkml:slot_uri <http://www.w3.org/1999/xhtml/vocab#rowgroup> .

okns:xhv_rowheader a linkml:SlotDefinition ;
    skos:definition "A cell␊      containing header information for a row in a grid." ;
    skos:editorialNote "No occurrences of this slot in the graph." ;
    skos:inScheme okns:xhv ;
    skos:mappingRelation <http://www.w3.org/1999/xhtml/vocab#rowheader> ;
    linkml:definition_uri okns:xhv_rowheader ;
    linkml:inlined true ;
    linkml:range okns:Any ;
    linkml:slot_uri <http://www.w3.org/1999/xhtml/vocab#rowheader> .

okns:xhv_scrollbar a linkml:SlotDefinition ;
    skos:definition "A graphical␊      object that controls the scrolling of content within a viewing area, regardless␊      of whether the content is fully displayed within the viewing area." ;
    skos:editorialNote "No occurrences of this slot in the graph." ;
    skos:inScheme okns:xhv ;
    skos:mappingRelation <http://www.w3.org/1999/xhtml/vocab#scrollbar> ;
    linkml:definition_uri okns:xhv_scrollbar ;
    linkml:inlined true ;
    linkml:range okns:Any ;
    linkml:slot_uri <http://www.w3.org/1999/xhtml/vocab#scrollbar> .

okns:xhv_search a linkml:SlotDefinition ;
    skos:definition "indicates␊      that the section provides a search facility." ;
    skos:editorialNote "No occurrences of this slot in the graph." ;
    skos:inScheme okns:xhv ;
    skos:mappingRelation <http://www.w3.org/1999/xhtml/vocab#search> ;
    linkml:definition_uri okns:xhv_search ;
    linkml:inlined true ;
    linkml:range okns:Any ;
    linkml:slot_uri <http://www.w3.org/1999/xhtml/vocab#search> .

okns:xhv_section a linkml:SlotDefinition ;
    skos:definition "section refers to a resource serving␊      as a section in a collection." ;
    skos:editorialNote "No occurrences of this slot in the graph." ;
    skos:inScheme okns:xhv ;
    skos:mappingRelation <http://www.w3.org/1999/xhtml/vocab#section> ;
    linkml:definition_uri okns:xhv_section ;
    linkml:inlined true ;
    linkml:range okns:Any ;
    linkml:slot_uri <http://www.w3.org/1999/xhtml/vocab#section> .

okns:xhv_separator a linkml:SlotDefinition ;
    skos:definition "A divider␊      that separates and distinguishes sections of content or groups of menuitems." ;
    skos:editorialNote "No occurrences of this slot in the graph." ;
    skos:inScheme okns:xhv ;
    skos:mappingRelation <http://www.w3.org/1999/xhtml/vocab#separator> ;
    linkml:definition_uri okns:xhv_separator ;
    linkml:inlined true ;
    linkml:range okns:Any ;
    linkml:slot_uri <http://www.w3.org/1999/xhtml/vocab#separator> .

okns:xhv_slider a linkml:SlotDefinition ;
    skos:definition "A user␊      input where the user selects a value from within a given range." ;
    skos:editorialNote "No occurrences of this slot in the graph." ;
    skos:inScheme okns:xhv ;
    skos:mappingRelation <http://www.w3.org/1999/xhtml/vocab#slider> ;
    linkml:definition_uri okns:xhv_slider ;
    linkml:inlined true ;
    linkml:range okns:Any ;
    linkml:slot_uri <http://www.w3.org/1999/xhtml/vocab#slider> .

okns:xhv_spinbutton a linkml:SlotDefinition ;
    skos:definition "A form␊      of range that expects a user to select from amongst discrete choices." ;
    skos:editorialNote "No occurrences of this slot in the graph." ;
    skos:inScheme okns:xhv ;
    skos:mappingRelation <http://www.w3.org/1999/xhtml/vocab#spinbutton> ;
    linkml:definition_uri okns:xhv_spinbutton ;
    linkml:inlined true ;
    linkml:range okns:Any ;
    linkml:slot_uri <http://www.w3.org/1999/xhtml/vocab#spinbutton> .

okns:xhv_start a linkml:SlotDefinition ;
    skos:definition "start refers to the first resource in␊      a collection of resources." ;
    skos:editorialNote "No occurrences of this slot in the graph." ;
    skos:inScheme okns:xhv ;
    skos:mappingRelation <http://www.w3.org/1999/xhtml/vocab#start> ;
    linkml:definition_uri okns:xhv_start ;
    linkml:inlined true ;
    linkml:range okns:Any ;
    linkml:slot_uri <http://www.w3.org/1999/xhtml/vocab#start> .

okns:xhv_status a linkml:SlotDefinition ;
    skos:definition "A container␊      whose content is advisory information for the user but is not important␊      enough to justify an alert. Also see alert." ;
    skos:editorialNote "No occurrences of this slot in the graph." ;
    skos:inScheme okns:xhv ;
    skos:mappingRelation <http://www.w3.org/1999/xhtml/vocab#status> ;
    linkml:definition_uri okns:xhv_status ;
    linkml:inlined true ;
    linkml:range okns:Any ;
    linkml:slot_uri <http://www.w3.org/1999/xhtml/vocab#status> .

okns:xhv_stylesheet a linkml:SlotDefinition ;
    skos:definition "stylesheet refers to a resource␊      serving as a stylesheet for a resource." ;
    skos:inScheme okns:xhv ;
    skos:mappingRelation <http://www.w3.org/1999/xhtml/vocab#stylesheet> ;
    linkml:definition_uri okns:xhv_stylesheet ;
    linkml:range okns:uri ;
    linkml:slot_uri <http://www.w3.org/1999/xhtml/vocab#stylesheet> .

okns:xhv_subsection a linkml:SlotDefinition ;
    skos:definition "subsection refers to a resource␊      serving as a subsection in a collection." ;
    skos:editorialNote "No occurrences of this slot in the graph." ;
    skos:inScheme okns:xhv ;
    skos:mappingRelation <http://www.w3.org/1999/xhtml/vocab#subsection> ;
    linkml:definition_uri okns:xhv_subsection ;
    linkml:inlined true ;
    linkml:range okns:Any ;
    linkml:slot_uri <http://www.w3.org/1999/xhtml/vocab#subsection> .

okns:xhv_tab a linkml:SlotDefinition ;
    skos:definition "A grouping␊      label providing a mechanism for selecting the tab content that is to be␊      rendered to the user." ;
    skos:editorialNote "No occurrences of this slot in the graph." ;
    skos:inScheme okns:xhv ;
    skos:mappingRelation <http://www.w3.org/1999/xhtml/vocab#tab> ;
    linkml:definition_uri okns:xhv_tab ;
    linkml:inlined true ;
    linkml:range okns:Any ;
    linkml:slot_uri <http://www.w3.org/1999/xhtml/vocab#tab> .

okns:xhv_tablist a linkml:SlotDefinition ;
    skos:definition "A list␊      of tab elements, which are references to tabpanel elements." ;
    skos:editorialNote "No occurrences of this slot in the graph." ;
    skos:inScheme okns:xhv ;
    skos:mappingRelation <http://www.w3.org/1999/xhtml/vocab#tablist> ;
    linkml:definition_uri okns:xhv_tablist ;
    linkml:inlined true ;
    linkml:range okns:Any ;
    linkml:slot_uri <http://www.w3.org/1999/xhtml/vocab#tablist> .

okns:xhv_tabpanel a linkml:SlotDefinition ;
    skos:definition "A container␊      for the resources associated with a tab, where each tab is contained in␊      a tablist." ;
    skos:editorialNote "No occurrences of this slot in the graph." ;
    skos:inScheme okns:xhv ;
    skos:mappingRelation <http://www.w3.org/1999/xhtml/vocab#tabpanel> ;
    linkml:definition_uri okns:xhv_tabpanel ;
    linkml:inlined true ;
    linkml:range okns:Any ;
    linkml:slot_uri <http://www.w3.org/1999/xhtml/vocab#tabpanel> .

okns:xhv_textbox a linkml:SlotDefinition ;
    skos:definition "Input␊      that allows free-form text as its value." ;
    skos:editorialNote "No occurrences of this slot in the graph." ;
    skos:inScheme okns:xhv ;
    skos:mappingRelation <http://www.w3.org/1999/xhtml/vocab#textbox> ;
    linkml:definition_uri okns:xhv_textbox ;
    linkml:inlined true ;
    linkml:range okns:Any ;
    linkml:slot_uri <http://www.w3.org/1999/xhtml/vocab#textbox> .

okns:xhv_timer a linkml:SlotDefinition ;
    skos:definition "A type of␊      live region containing a numerical counter which indicates an amount of␊      elapsed time from a start point, or the time remaining until an end point." ;
    skos:editorialNote "No occurrences of this slot in the graph." ;
    skos:inScheme okns:xhv ;
    skos:mappingRelation <http://www.w3.org/1999/xhtml/vocab#timer> ;
    linkml:definition_uri okns:xhv_timer ;
    linkml:inlined true ;
    linkml:range okns:Any ;
    linkml:slot_uri <http://www.w3.org/1999/xhtml/vocab#timer> .

okns:xhv_toolbar a linkml:SlotDefinition ;
    skos:definition "A collection␊      of commonly used function buttons represented in compact visual form." ;
    skos:editorialNote "No occurrences of this slot in the graph." ;
    skos:inScheme okns:xhv ;
    skos:mappingRelation <http://www.w3.org/1999/xhtml/vocab#toolbar> ;
    linkml:definition_uri okns:xhv_toolbar ;
    linkml:inlined true ;
    linkml:range okns:Any ;
    linkml:slot_uri <http://www.w3.org/1999/xhtml/vocab#toolbar> .

okns:xhv_tooltip a linkml:SlotDefinition ;
    skos:definition "A contextual␊      popup that displays a description for an element." ;
    skos:editorialNote "No occurrences of this slot in the graph." ;
    skos:inScheme okns:xhv ;
    skos:mappingRelation <http://www.w3.org/1999/xhtml/vocab#tooltip> ;
    linkml:definition_uri okns:xhv_tooltip ;
    linkml:inlined true ;
    linkml:range okns:Any ;
    linkml:slot_uri <http://www.w3.org/1999/xhtml/vocab#tooltip> .

okns:xhv_top a linkml:SlotDefinition ;
    skos:definition "top is a synonym for start." ;
    skos:editorialNote "No occurrences of this slot in the graph." ;
    skos:inScheme okns:xhv ;
    skos:mappingRelation <http://www.w3.org/1999/xhtml/vocab#top> ;
    linkml:definition_uri okns:xhv_top ;
    linkml:inlined true ;
    linkml:range okns:Any ;
    linkml:slot_uri <http://www.w3.org/1999/xhtml/vocab#top> .

okns:xhv_tree a linkml:SlotDefinition ;
    skos:definition "A type of␊      list that may contain sub-level nested groups that can be collapsed and␊      expanded." ;
    skos:editorialNote "No occurrences of this slot in the graph." ;
    skos:inScheme okns:xhv ;
    skos:mappingRelation <http://www.w3.org/1999/xhtml/vocab#tree> ;
    linkml:definition_uri okns:xhv_tree ;
    linkml:inlined true ;
    linkml:range okns:Any ;
    linkml:slot_uri <http://www.w3.org/1999/xhtml/vocab#tree> .

okns:xhv_treegrid a linkml:SlotDefinition ;
    skos:definition "A grid␊      whose rows can be expanded and collapsed in the same manner as for a tree." ;
    skos:editorialNote "No occurrences of this slot in the graph." ;
    skos:inScheme okns:xhv ;
    skos:mappingRelation <http://www.w3.org/1999/xhtml/vocab#treegrid> ;
    linkml:definition_uri okns:xhv_treegrid ;
    linkml:inlined true ;
    linkml:range okns:Any ;
    linkml:slot_uri <http://www.w3.org/1999/xhtml/vocab#treegrid> .

okns:xhv_treeitem a linkml:SlotDefinition ;
    skos:definition "An option␊      item of a tree. This is an element within a tree that may be expanded or␊      collapsed if it contains a sub-level group of treeitems." ;
    skos:editorialNote "No occurrences of this slot in the graph." ;
    skos:inScheme okns:xhv ;
    skos:mappingRelation <http://www.w3.org/1999/xhtml/vocab#treeitem> ;
    linkml:definition_uri okns:xhv_treeitem ;
    linkml:inlined true ;
    linkml:range okns:Any ;
    linkml:slot_uri <http://www.w3.org/1999/xhtml/vocab#treeitem> .

okns:xhv_up a linkml:SlotDefinition ;
    skos:definition "up refers to a resource \"above\" in a␊      hierarchically structured set." ;
    skos:editorialNote "No occurrences of this slot in the graph." ;
    skos:inScheme okns:xhv ;
    skos:mappingRelation <http://www.w3.org/1999/xhtml/vocab#up> ;
    linkml:definition_uri okns:xhv_up ;
    linkml:inlined true ;
    linkml:range okns:Any ;
    linkml:slot_uri <http://www.w3.org/1999/xhtml/vocab#up> .

okns:OwlAllDifferent a linkml:ClassDefinition ;
    dcterms:source owl: ;
    dcterms:title "AllDifferent" ;
    skos:definition "The class of collections of pairwise different individuals." ;
    skos:inScheme okns:owl-rdf-rdfs ;
    skos:mappingRelation owl:AllDifferent ;
    linkml:class_uri owl:AllDifferent ;
    linkml:definition_uri okns:OwlAllDifferent ;
    linkml:is_a okns:RdfsResource ;
    linkml:slot_usage [ ] .

okns:decimal a linkml:TypeDefinition ;
    skos:broadMatch schema1:Number ;
    skos:definition "A real number with arbitrary precision that conforms to the xsd:decimal specification" ;
    skos:editorialNote "If you are authoring schemas in LinkML YAML, the type is referenced with the lower case \"decimal\"." ;
    skos:inScheme linkml:types ;
    linkml:base "Decimal" ;
    linkml:definition_uri linkml:Decimal ;
    linkml:imported_from "linkml:types" ;
    linkml:uri xsd:decimal .

okns:owl_allValuesFrom a linkml:SlotDefinition ;
    dcterms:source owl: ;
    dcterms:title "allValuesFrom" ;
    skos:definition "The property that determines the class that a universal property restriction refers to." ;
    skos:editorialNote "No occurrences of this slot in the graph." ;
    skos:inScheme okns:owl-rdf-rdfs ;
    skos:mappingRelation owl:allValuesFrom ;
    linkml:definition_uri okns:owl_allValuesFrom ;
    linkml:domain okns:OwlRestriction ;
    linkml:inlined true ;
    linkml:owner okns:owl_allValuesFrom ;
    linkml:range okns:RdfsClass ;
    linkml:slot_uri owl:allValuesFrom .

okns:owl_annotatedProperty a linkml:SlotDefinition ;
    dcterms:source owl: ;
    dcterms:title "annotatedProperty" ;
    skos:definition "The property that determines the predicate of an annotated axiom or annotated annotation." ;
    skos:editorialNote "No occurrences of this slot in the graph." ;
    skos:inScheme okns:owl-rdf-rdfs ;
    skos:mappingRelation owl:annotatedProperty ;
    linkml:definition_uri okns:owl_annotatedProperty ;
    linkml:domain okns:RdfsResource ;
    linkml:inlined true ;
    linkml:owner okns:owl_annotatedProperty ;
    linkml:range okns:RdfsResource ;
    linkml:slot_uri owl:annotatedProperty .

okns:owl_annotatedSource a linkml:SlotDefinition ;
    dcterms:source owl: ;
    dcterms:title "annotatedSource" ;
    skos:definition "The property that determines the subject of an annotated axiom or annotated annotation." ;
    skos:editorialNote "No occurrences of this slot in the graph." ;
    skos:inScheme okns:owl-rdf-rdfs ;
    skos:mappingRelation owl:annotatedSource ;
    linkml:definition_uri okns:owl_annotatedSource ;
    linkml:domain okns:RdfsResource ;
    linkml:inlined true ;
    linkml:owner okns:owl_annotatedSource ;
    linkml:range okns:RdfsResource ;
    linkml:slot_uri owl:annotatedSource .

okns:owl_annotatedTarget a linkml:SlotDefinition ;
    dcterms:source owl: ;
    dcterms:title "annotatedTarget" ;
    skos:definition "The property that determines the object of an annotated axiom or annotated annotation." ;
    skos:editorialNote "No occurrences of this slot in the graph." ;
    skos:inScheme okns:owl-rdf-rdfs ;
    skos:mappingRelation owl:annotatedTarget ;
    linkml:definition_uri okns:owl_annotatedTarget ;
    linkml:domain okns:RdfsResource ;
    linkml:inlined true ;
    linkml:owner okns:owl_annotatedTarget ;
    linkml:range okns:RdfsResource ;
    linkml:slot_uri owl:annotatedTarget .

okns:owl_assertionProperty a linkml:SlotDefinition ;
    dcterms:source owl: ;
    dcterms:title "assertionProperty" ;
    skos:definition "The property that determines the predicate of a negative property assertion." ;
    skos:editorialNote "No occurrences of this slot in the graph." ;
    skos:inScheme okns:owl-rdf-rdfs ;
    skos:mappingRelation owl:assertionProperty ;
    linkml:definition_uri okns:owl_assertionProperty ;
    linkml:domain okns:OwlNegativePropertyAssertion ;
    linkml:inlined true ;
    linkml:owner okns:owl_assertionProperty ;
    linkml:range okns:RdfProperty ;
    linkml:slot_uri owl:assertionProperty .

okns:owl_backwardCompatibleWith a linkml:SlotDefinition ;
    dcterms:source owl: ;
    dcterms:title "backwardCompatibleWith" ;
    skos:definition "The annotation property that indicates that a given ontology is backward compatible with another ontology." ;
    skos:editorialNote "No occurrences of this slot in the graph." ;
    skos:inScheme okns:owl-rdf-rdfs ;
    skos:mappingRelation owl:backwardCompatibleWith ;
    linkml:definition_uri okns:owl_backwardCompatibleWith ;
    linkml:domain okns:OwlOntology ;
    linkml:inlined true ;
    linkml:owner okns:owl_backwardCompatibleWith ;
    linkml:range okns:OwlOntology ;
    linkml:slot_uri owl:backwardCompatibleWith .

okns:owl_bottomDataProperty a linkml:SlotDefinition ;
    dcterms:source owl: ;
    dcterms:title "bottomDataProperty" ;
    skos:definition "The data property that does not relate any individual to any data value." ;
    skos:editorialNote "No occurrences of this slot in the graph." ;
    skos:inScheme okns:owl-rdf-rdfs ;
    skos:mappingRelation owl:bottomDataProperty ;
    linkml:definition_uri okns:owl_bottomDataProperty ;
    linkml:domain okns:OwlThing ;
    linkml:inlined true ;
    linkml:owner okns:owl_bottomDataProperty ;
    linkml:range okns:RdfsLiteral ;
    linkml:slot_uri owl:bottomDataProperty .

okns:owl_bottomObjectProperty a linkml:SlotDefinition ;
    dcterms:source owl: ;
    dcterms:title "bottomObjectProperty" ;
    skos:definition "The object property that does not relate any two individuals." ;
    skos:editorialNote "No occurrences of this slot in the graph." ;
    skos:inScheme okns:owl-rdf-rdfs ;
    skos:mappingRelation owl:bottomObjectProperty ;
    linkml:definition_uri okns:owl_bottomObjectProperty ;
    linkml:domain okns:OwlThing ;
    linkml:inlined true ;
    linkml:owner okns:owl_bottomObjectProperty ;
    linkml:range okns:OwlThing ;
    linkml:slot_uri owl:bottomObjectProperty .

okns:owl_cardinality a linkml:SlotDefinition ;
    dcterms:source owl: ;
    dcterms:title "cardinality" ;
    skos:definition "The property that determines the cardinality of an exact cardinality restriction." ;
    skos:editorialNote "No occurrences of this slot in the graph." ;
    skos:inScheme okns:owl-rdf-rdfs ;
    skos:mappingRelation owl:cardinality ;
    linkml:definition_uri okns:owl_cardinality ;
    linkml:domain okns:OwlRestriction ;
    linkml:owner okns:owl_cardinality ;
    linkml:range okns:unsignedinteger ;
    linkml:slot_uri owl:cardinality .

okns:owl_complementOf a linkml:SlotDefinition ;
    dcterms:source owl: ;
    dcterms:title "complementOf" ;
    skos:definition "The property that determines that a given class is the complement of another class." ;
    skos:editorialNote "No occurrences of this slot in the graph." ;
    skos:inScheme okns:owl-rdf-rdfs ;
    skos:mappingRelation owl:complementOf ;
    linkml:definition_uri okns:owl_complementOf ;
    linkml:domain okns:OwlClass ;
    linkml:inlined true ;
    linkml:owner okns:owl_complementOf ;
    linkml:range okns:OwlClass ;
    linkml:slot_uri owl:complementOf .

okns:owl_datatypeComplementOf a linkml:SlotDefinition ;
    dcterms:source owl: ;
    dcterms:title "datatypeComplementOf" ;
    skos:definition "The property that determines that a given data range is the complement of another data range with respect to the data domain." ;
    skos:editorialNote "No occurrences of this slot in the graph." ;
    skos:inScheme okns:owl-rdf-rdfs ;
    skos:mappingRelation owl:datatypeComplementOf ;
    linkml:definition_uri okns:owl_datatypeComplementOf ;
    linkml:domain okns:RdfsDatatype ;
    linkml:inlined true ;
    linkml:owner okns:owl_datatypeComplementOf ;
    linkml:range okns:RdfsDatatype ;
    linkml:slot_uri owl:datatypeComplementOf .

okns:owl_deprecated a linkml:SlotDefinition ;
    dcterms:source owl: ;
    dcterms:title "deprecated" ;
    skos:definition "The annotation property that indicates that a given entity has been deprecated." ;
    skos:editorialNote "No occurrences of this slot in the graph." ;
    skos:inScheme okns:owl-rdf-rdfs ;
    skos:mappingRelation owl:deprecated ;
    linkml:definition_uri okns:owl_deprecated ;
    linkml:domain okns:RdfsResource ;
    linkml:inlined true ;
    linkml:owner okns:owl_deprecated ;
    linkml:range okns:RdfsResource ;
    linkml:slot_uri owl:deprecated .

okns:owl_differentFrom a linkml:SlotDefinition ;
    dcterms:source owl: ;
    dcterms:title "differentFrom" ;
    skos:definition "The property that determines that two given individuals are different." ;
    skos:editorialNote "No occurrences of this slot in the graph." ;
    skos:inScheme okns:owl-rdf-rdfs ;
    skos:mappingRelation owl:differentFrom ;
    linkml:definition_uri okns:owl_differentFrom ;
    linkml:domain okns:OwlThing ;
    linkml:inlined true ;
    linkml:owner okns:owl_differentFrom ;
    linkml:range okns:OwlThing ;
    linkml:slot_uri owl:differentFrom .

okns:owl_disjointUnionOf a linkml:SlotDefinition ;
    dcterms:source owl: ;
    dcterms:title "disjointUnionOf" ;
    skos:definition "The property that determines that a given class is equivalent to the disjoint union of a collection of other classes." ;
    skos:editorialNote "No occurrences of this slot in the graph." ;
    skos:inScheme okns:owl-rdf-rdfs ;
    skos:mappingRelation owl:disjointUnionOf ;
    linkml:definition_uri okns:owl_disjointUnionOf ;
    linkml:domain okns:OwlClass ;
    linkml:inlined true ;
    linkml:owner okns:owl_disjointUnionOf ;
    linkml:range okns:RdfList ;
    linkml:slot_uri owl:disjointUnionOf .

okns:owl_disjointWith a linkml:SlotDefinition ;
    dcterms:source owl: ;
    dcterms:title "disjointWith" ;
    skos:definition "The property that determines that two given classes are disjoint." ;
    skos:editorialNote "No occurrences of this slot in the graph." ;
    skos:inScheme okns:owl-rdf-rdfs ;
    skos:mappingRelation owl:disjointWith ;
    linkml:definition_uri okns:owl_disjointWith ;
    linkml:domain okns:OwlClass ;
    linkml:inlined true ;
    linkml:owner okns:owl_disjointWith ;
    linkml:range okns:OwlClass ;
    linkml:slot_uri owl:disjointWith .

okns:owl_distinctMembers a linkml:SlotDefinition ;
    dcterms:source owl: ;
    dcterms:title "distinctMembers" ;
    skos:definition "The property that determines the collection of pairwise different individuals in a owl:AllDifferent axiom." ;
    skos:editorialNote "No occurrences of this slot in the graph." ;
    skos:inScheme okns:owl-rdf-rdfs ;
    skos:mappingRelation owl:distinctMembers ;
    linkml:definition_uri okns:owl_distinctMembers ;
    linkml:domain okns:OwlAllDifferent ;
    linkml:inlined true ;
    linkml:owner okns:owl_distinctMembers ;
    linkml:range okns:RdfList ;
    linkml:slot_uri owl:distinctMembers .

okns:owl_equivalentClass a linkml:SlotDefinition ;
    dcterms:source owl: ;
    dcterms:title "equivalentClass" ;
    skos:definition "The property that determines that two given classes are equivalent, and that is used to specify datatype definitions." ;
    skos:editorialNote "No occurrences of this slot in the graph." ;
    skos:inScheme okns:owl-rdf-rdfs ;
    skos:mappingRelation owl:equivalentClass ;
    linkml:definition_uri okns:owl_equivalentClass ;
    linkml:domain okns:RdfsClass ;
    linkml:inlined true ;
    linkml:owner okns:owl_equivalentClass ;
    linkml:range okns:RdfsClass ;
    linkml:slot_uri owl:equivalentClass .

okns:owl_equivalentProperty a linkml:SlotDefinition ;
    dcterms:source owl: ;
    dcterms:title "equivalentProperty" ;
    skos:definition "The property that determines that two given properties are equivalent." ;
    skos:editorialNote "No occurrences of this slot in the graph." ;
    skos:inScheme okns:owl-rdf-rdfs ;
    skos:mappingRelation owl:equivalentProperty ;
    linkml:definition_uri okns:owl_equivalentProperty ;
    linkml:domain okns:RdfProperty ;
    linkml:inlined true ;
    linkml:owner okns:owl_equivalentProperty ;
    linkml:range okns:RdfProperty ;
    linkml:slot_uri owl:equivalentProperty .

okns:owl_hasKey a linkml:SlotDefinition ;
    dcterms:source owl: ;
    dcterms:title "hasKey" ;
    skos:definition "The property that determines the collection of properties that jointly build a key." ;
    skos:editorialNote "No occurrences of this slot in the graph." ;
    skos:inScheme okns:owl-rdf-rdfs ;
    skos:mappingRelation owl:hasKey ;
    linkml:definition_uri okns:owl_hasKey ;
    linkml:domain okns:OwlClass ;
    linkml:inlined true ;
    linkml:owner okns:owl_hasKey ;
    linkml:range okns:RdfList ;
    linkml:slot_uri owl:hasKey .

okns:owl_hasSelf a linkml:SlotDefinition ;
    dcterms:source owl: ;
    dcterms:title "hasSelf" ;
    skos:definition "The property that determines the property that a self restriction refers to." ;
    skos:editorialNote "No occurrences of this slot in the graph." ;
    skos:inScheme okns:owl-rdf-rdfs ;
    skos:mappingRelation owl:hasSelf ;
    linkml:definition_uri okns:owl_hasSelf ;
    linkml:domain okns:OwlRestriction ;
    linkml:inlined true ;
    linkml:owner okns:owl_hasSelf ;
    linkml:range okns:RdfsResource ;
    linkml:slot_uri owl:hasSelf .

okns:owl_hasValue a linkml:SlotDefinition ;
    dcterms:source owl: ;
    dcterms:title "hasValue" ;
    skos:definition "The property that determines the individual that a has-value restriction refers to." ;
    skos:editorialNote "No occurrences of this slot in the graph." ;
    skos:inScheme okns:owl-rdf-rdfs ;
    skos:mappingRelation owl:hasValue ;
    linkml:definition_uri okns:owl_hasValue ;
    linkml:domain okns:OwlRestriction ;
    linkml:inlined true ;
    linkml:owner okns:owl_hasValue ;
    linkml:range okns:RdfsResource ;
    linkml:slot_uri owl:hasValue .

okns:owl_imports a linkml:SlotDefinition ;
    dcterms:source owl: ;
    dcterms:title "imports" ;
    skos:definition "The property that is used for importing other ontologies into a given ontology." ;
    skos:editorialNote "No occurrences of this slot in the graph." ;
    skos:inScheme okns:owl-rdf-rdfs ;
    skos:mappingRelation owl:imports ;
    linkml:definition_uri okns:owl_imports ;
    linkml:domain okns:OwlOntology ;
    linkml:inlined true ;
    linkml:owner okns:owl_imports ;
    linkml:range okns:OwlOntology ;
    linkml:slot_uri owl:imports .

okns:owl_incompatibleWith a linkml:SlotDefinition ;
    dcterms:source owl: ;
    dcterms:title "incompatibleWith" ;
    skos:definition "The annotation property that indicates that a given ontology is incompatible with another ontology." ;
    skos:editorialNote "No occurrences of this slot in the graph." ;
    skos:inScheme okns:owl-rdf-rdfs ;
    skos:mappingRelation owl:incompatibleWith ;
    linkml:definition_uri okns:owl_incompatibleWith ;
    linkml:domain okns:OwlOntology ;
    linkml:inlined true ;
    linkml:owner okns:owl_incompatibleWith ;
    linkml:range okns:OwlOntology ;
    linkml:slot_uri owl:incompatibleWith .

okns:owl_intersectionOf a linkml:SlotDefinition ;
    dcterms:source owl: ;
    dcterms:title "intersectionOf" ;
    skos:definition "The property that determines the collection of classes or data ranges that build an intersection." ;
    skos:editorialNote "No occurrences of this slot in the graph." ;
    skos:inScheme okns:owl-rdf-rdfs ;
    skos:mappingRelation owl:intersectionOf ;
    linkml:definition_uri okns:owl_intersectionOf ;
    linkml:domain okns:RdfsClass ;
    linkml:inlined true ;
    linkml:owner okns:owl_intersectionOf ;
    linkml:range okns:RdfList ;
    linkml:slot_uri owl:intersectionOf .

okns:owl_inverseOf a linkml:SlotDefinition ;
    dcterms:source owl: ;
    dcterms:title "inverseOf" ;
    skos:definition "The property that determines that two given properties are inverse." ;
    skos:editorialNote "No occurrences of this slot in the graph." ;
    skos:inScheme okns:owl-rdf-rdfs ;
    skos:mappingRelation owl:inverseOf ;
    linkml:definition_uri okns:owl_inverseOf ;
    linkml:domain okns:OwlObjectProperty ;
    linkml:inlined true ;
    linkml:owner okns:owl_inverseOf ;
    linkml:range okns:OwlObjectProperty ;
    linkml:slot_uri owl:inverseOf .

okns:owl_maxCardinality a linkml:SlotDefinition ;
    dcterms:source owl: ;
    dcterms:title "maxCardinality" ;
    skos:definition "The property that determines the cardinality of a maximum cardinality restriction." ;
    skos:editorialNote "No occurrences of this slot in the graph." ;
    skos:inScheme okns:owl-rdf-rdfs ;
    skos:mappingRelation owl:maxCardinality ;
    linkml:definition_uri okns:owl_maxCardinality ;
    linkml:domain okns:OwlRestriction ;
    linkml:owner okns:owl_maxCardinality ;
    linkml:range okns:unsignedinteger ;
    linkml:slot_uri owl:maxCardinality .

okns:owl_maxQualifiedCardinality a linkml:SlotDefinition ;
    dcterms:source owl: ;
    dcterms:title "maxQualifiedCardinality" ;
    skos:definition "The property that determines the cardinality of a maximum qualified cardinality restriction." ;
    skos:editorialNote "No occurrences of this slot in the graph." ;
    skos:inScheme okns:owl-rdf-rdfs ;
    skos:mappingRelation owl:maxQualifiedCardinality ;
    linkml:definition_uri okns:owl_maxQualifiedCardinality ;
    linkml:domain okns:OwlRestriction ;
    linkml:owner okns:owl_maxQualifiedCardinality ;
    linkml:range okns:unsignedinteger ;
    linkml:slot_uri owl:maxQualifiedCardinality .

okns:owl_members a linkml:SlotDefinition ;
    dcterms:source owl: ;
    dcterms:title "members" ;
    skos:definition "The property that determines the collection of members in either a owl:AllDifferent, owl:AllDisjointClasses or owl:AllDisjointProperties axiom." ;
    skos:editorialNote "No occurrences of this slot in the graph." ;
    skos:inScheme okns:owl-rdf-rdfs ;
    skos:mappingRelation owl:members ;
    linkml:definition_uri okns:owl_members ;
    linkml:domain okns:RdfsResource ;
    linkml:inlined true ;
    linkml:owner okns:owl_members ;
    linkml:range okns:RdfList ;
    linkml:slot_uri owl:members .

okns:owl_minCardinality a linkml:SlotDefinition ;
    dcterms:source owl: ;
    dcterms:title "minCardinality" ;
    skos:definition "The property that determines the cardinality of a minimum cardinality restriction." ;
    skos:editorialNote "No occurrences of this slot in the graph." ;
    skos:inScheme okns:owl-rdf-rdfs ;
    skos:mappingRelation owl:minCardinality ;
    linkml:definition_uri okns:owl_minCardinality ;
    linkml:domain okns:OwlRestriction ;
    linkml:owner okns:owl_minCardinality ;
    linkml:range okns:unsignedinteger ;
    linkml:slot_uri owl:minCardinality .

okns:owl_minQualifiedCardinality a linkml:SlotDefinition ;
    dcterms:source owl: ;
    dcterms:title "minQualifiedCardinality" ;
    skos:definition "The property that determines the cardinality of a minimum qualified cardinality restriction." ;
    skos:editorialNote "No occurrences of this slot in the graph." ;
    skos:inScheme okns:owl-rdf-rdfs ;
    skos:mappingRelation owl:minQualifiedCardinality ;
    linkml:definition_uri okns:owl_minQualifiedCardinality ;
    linkml:domain okns:OwlRestriction ;
    linkml:owner okns:owl_minQualifiedCardinality ;
    linkml:range okns:unsignedinteger ;
    linkml:slot_uri owl:minQualifiedCardinality .

okns:owl_onClass a linkml:SlotDefinition ;
    dcterms:source owl: ;
    dcterms:title "onClass" ;
    skos:definition "The property that determines the class that a qualified object cardinality restriction refers to." ;
    skos:editorialNote "No occurrences of this slot in the graph." ;
    skos:inScheme okns:owl-rdf-rdfs ;
    skos:mappingRelation owl:onClass ;
    linkml:definition_uri okns:owl_onClass ;
    linkml:domain okns:OwlRestriction ;
    linkml:inlined true ;
    linkml:owner okns:owl_onClass ;
    linkml:range okns:OwlClass ;
    linkml:slot_uri owl:onClass .

okns:owl_onDataRange a linkml:SlotDefinition ;
    dcterms:source owl: ;
    dcterms:title "onDataRange" ;
    skos:definition "The property that determines the data range that a qualified data cardinality restriction refers to." ;
    skos:editorialNote "No occurrences of this slot in the graph." ;
    skos:inScheme okns:owl-rdf-rdfs ;
    skos:mappingRelation owl:onDataRange ;
    linkml:definition_uri okns:owl_onDataRange ;
    linkml:domain okns:OwlRestriction ;
    linkml:inlined true ;
    linkml:owner okns:owl_onDataRange ;
    linkml:range okns:RdfsDatatype ;
    linkml:slot_uri owl:onDataRange .

okns:owl_onDatatype a linkml:SlotDefinition ;
    dcterms:source owl: ;
    dcterms:title "onDatatype" ;
    skos:definition "The property that determines the datatype that a datatype restriction refers to." ;
    skos:editorialNote "No occurrences of this slot in the graph." ;
    skos:inScheme okns:owl-rdf-rdfs ;
    skos:mappingRelation owl:onDatatype ;
    linkml:definition_uri okns:owl_onDatatype ;
    linkml:domain okns:RdfsDatatype ;
    linkml:inlined true ;
    linkml:owner okns:owl_onDatatype ;
    linkml:range okns:RdfsDatatype ;
    linkml:slot_uri owl:onDatatype .

okns:owl_onProperties a linkml:SlotDefinition ;
    dcterms:source owl: ;
    dcterms:title "onProperties" ;
    skos:definition "The property that determines the n-tuple of properties that a property restriction on an n-ary data range refers to." ;
    skos:editorialNote "No occurrences of this slot in the graph." ;
    skos:inScheme okns:owl-rdf-rdfs ;
    skos:mappingRelation owl:onProperties ;
    linkml:definition_uri okns:owl_onProperties ;
    linkml:domain okns:OwlRestriction ;
    linkml:inlined true ;
    linkml:owner okns:owl_onProperties ;
    linkml:range okns:RdfList ;
    linkml:slot_uri owl:onProperties .

okns:owl_onProperty a linkml:SlotDefinition ;
    dcterms:source owl: ;
    dcterms:title "onProperty" ;
    skos:definition "The property that determines the property that a property restriction refers to." ;
    skos:editorialNote "No occurrences of this slot in the graph." ;
    skos:inScheme okns:owl-rdf-rdfs ;
    skos:mappingRelation owl:onProperty ;
    linkml:definition_uri okns:owl_onProperty ;
    linkml:domain okns:OwlRestriction ;
    linkml:inlined true ;
    linkml:owner okns:owl_onProperty ;
    linkml:range okns:RdfProperty ;
    linkml:slot_uri owl:onProperty .

okns:owl_oneOf a linkml:SlotDefinition ;
    dcterms:source owl: ;
    dcterms:title "oneOf" ;
    skos:definition "The property that determines the collection of individuals or data values that build an enumeration." ;
    skos:editorialNote "No occurrences of this slot in the graph." ;
    skos:inScheme okns:owl-rdf-rdfs ;
    skos:mappingRelation owl:oneOf ;
    linkml:definition_uri okns:owl_oneOf ;
    linkml:domain okns:RdfsClass ;
    linkml:inlined true ;
    linkml:owner okns:owl_oneOf ;
    linkml:range okns:RdfList ;
    linkml:slot_uri owl:oneOf .

okns:owl_priorVersion a linkml:SlotDefinition ;
    dcterms:source owl: ;
    dcterms:title "priorVersion" ;
    skos:definition "The annotation property that indicates the predecessor ontology of a given ontology." ;
    skos:editorialNote "No occurrences of this slot in the graph." ;
    skos:inScheme okns:owl-rdf-rdfs ;
    skos:mappingRelation owl:priorVersion ;
    linkml:definition_uri okns:owl_priorVersion ;
    linkml:domain okns:OwlOntology ;
    linkml:inlined true ;
    linkml:owner okns:owl_priorVersion ;
    linkml:range okns:OwlOntology ;
    linkml:slot_uri owl:priorVersion .

okns:owl_propertyChainAxiom a linkml:SlotDefinition ;
    dcterms:source owl: ;
    dcterms:title "propertyChainAxiom" ;
    skos:definition "The property that determines the n-tuple of properties that build a sub property chain of a given property." ;
    skos:editorialNote "No occurrences of this slot in the graph." ;
    skos:inScheme okns:owl-rdf-rdfs ;
    skos:mappingRelation owl:propertyChainAxiom ;
    linkml:definition_uri okns:owl_propertyChainAxiom ;
    linkml:domain okns:OwlObjectProperty ;
    linkml:inlined true ;
    linkml:owner okns:owl_propertyChainAxiom ;
    linkml:range okns:RdfList ;
    linkml:slot_uri owl:propertyChainAxiom .

okns:owl_propertyDisjointWith a linkml:SlotDefinition ;
    dcterms:source owl: ;
    dcterms:title "propertyDisjointWith" ;
    skos:definition "The property that determines that two given properties are disjoint." ;
    skos:editorialNote "No occurrences of this slot in the graph." ;
    skos:inScheme okns:owl-rdf-rdfs ;
    skos:mappingRelation owl:propertyDisjointWith ;
    linkml:definition_uri okns:owl_propertyDisjointWith ;
    linkml:domain okns:RdfProperty ;
    linkml:inlined true ;
    linkml:owner okns:owl_propertyDisjointWith ;
    linkml:range okns:RdfProperty ;
    linkml:slot_uri owl:propertyDisjointWith .

okns:owl_qualifiedCardinality a linkml:SlotDefinition ;
    dcterms:source owl: ;
    dcterms:title "qualifiedCardinality" ;
    skos:definition "The property that determines the cardinality of an exact qualified cardinality restriction." ;
    skos:editorialNote "No occurrences of this slot in the graph." ;
    skos:inScheme okns:owl-rdf-rdfs ;
    skos:mappingRelation owl:qualifiedCardinality ;
    linkml:definition_uri okns:owl_qualifiedCardinality ;
    linkml:domain okns:OwlRestriction ;
    linkml:owner okns:owl_qualifiedCardinality ;
    linkml:range okns:unsignedinteger ;
    linkml:slot_uri owl:qualifiedCardinality .

okns:owl_sameAs a linkml:SlotDefinition ;
    dcterms:source owl: ;
    dcterms:title "sameAs" ;
    skos:definition "The property that determines that two given individuals are equal." ;
    skos:editorialNote "No occurrences of this slot in the graph." ;
    skos:inScheme okns:owl-rdf-rdfs ;
    skos:mappingRelation owl:sameAs ;
    linkml:definition_uri okns:owl_sameAs ;
    linkml:domain okns:OwlThing ;
    linkml:inlined true ;
    linkml:owner okns:owl_sameAs ;
    linkml:range okns:OwlThing ;
    linkml:slot_uri owl:sameAs .

okns:owl_someValuesFrom a linkml:SlotDefinition ;
    dcterms:source owl: ;
    dcterms:title "someValuesFrom" ;
    skos:definition "The property that determines the class that an existential property restriction refers to." ;
    skos:editorialNote "No occurrences of this slot in the graph." ;
    skos:inScheme okns:owl-rdf-rdfs ;
    skos:mappingRelation owl:someValuesFrom ;
    linkml:definition_uri okns:owl_someValuesFrom ;
    linkml:domain okns:OwlRestriction ;
    linkml:inlined true ;
    linkml:owner okns:owl_someValuesFrom ;
    linkml:range okns:RdfsClass ;
    linkml:slot_uri owl:someValuesFrom .

okns:owl_sourceIndividual a linkml:SlotDefinition ;
    dcterms:source owl: ;
    dcterms:title "sourceIndividual" ;
    skos:definition "The property that determines the subject of a negative property assertion." ;
    skos:editorialNote "No occurrences of this slot in the graph." ;
    skos:inScheme okns:owl-rdf-rdfs ;
    skos:mappingRelation owl:sourceIndividual ;
    linkml:definition_uri okns:owl_sourceIndividual ;
    linkml:domain okns:OwlNegativePropertyAssertion ;
    linkml:inlined true ;
    linkml:owner okns:owl_sourceIndividual ;
    linkml:range okns:OwlThing ;
    linkml:slot_uri owl:sourceIndividual .

okns:owl_targetIndividual a linkml:SlotDefinition ;
    dcterms:source owl: ;
    dcterms:title "targetIndividual" ;
    skos:definition "The property that determines the object of a negative object property assertion." ;
    skos:editorialNote "No occurrences of this slot in the graph." ;
    skos:inScheme okns:owl-rdf-rdfs ;
    skos:mappingRelation owl:targetIndividual ;
    linkml:definition_uri okns:owl_targetIndividual ;
    linkml:domain okns:OwlNegativePropertyAssertion ;
    linkml:inlined true ;
    linkml:owner okns:owl_targetIndividual ;
    linkml:range okns:OwlThing ;
    linkml:slot_uri owl:targetIndividual .

okns:owl_targetValue a linkml:SlotDefinition ;
    dcterms:source owl: ;
    dcterms:title "targetValue" ;
    skos:definition "The property that determines the value of a negative data property assertion." ;
    skos:editorialNote "No occurrences of this slot in the graph." ;
    skos:inScheme okns:owl-rdf-rdfs ;
    skos:mappingRelation owl:targetValue ;
    linkml:definition_uri okns:owl_targetValue ;
    linkml:domain okns:OwlNegativePropertyAssertion ;
    linkml:inlined true ;
    linkml:owner okns:owl_targetValue ;
    linkml:range okns:RdfsLiteral ;
    linkml:slot_uri owl:targetValue .

okns:owl_topDataProperty a linkml:SlotDefinition ;
    dcterms:source owl: ;
    dcterms:title "topDataProperty" ;
    skos:definition "The data property that relates every individual to every data value." ;
    skos:editorialNote "No occurrences of this slot in the graph." ;
    skos:inScheme okns:owl-rdf-rdfs ;
    skos:mappingRelation owl:topDataProperty ;
    linkml:definition_uri okns:owl_topDataProperty ;
    linkml:domain okns:OwlThing ;
    linkml:inlined true ;
    linkml:owner okns:owl_topDataProperty ;
    linkml:range okns:RdfsLiteral ;
    linkml:slot_uri owl:topDataProperty .

okns:owl_topObjectProperty a linkml:SlotDefinition ;
    dcterms:source owl: ;
    dcterms:title "topObjectProperty" ;
    skos:definition "The object property that relates every two individuals." ;
    skos:editorialNote "No occurrences of this slot in the graph." ;
    skos:inScheme okns:owl-rdf-rdfs ;
    skos:mappingRelation owl:topObjectProperty ;
    linkml:definition_uri okns:owl_topObjectProperty ;
    linkml:domain okns:OwlThing ;
    linkml:inlined true ;
    linkml:owner okns:owl_topObjectProperty ;
    linkml:range okns:OwlThing ;
    linkml:slot_uri owl:topObjectProperty .

okns:owl_unionOf a linkml:SlotDefinition ;
    dcterms:source owl: ;
    dcterms:title "unionOf" ;
    skos:definition "The property that determines the collection of classes or data ranges that build a union." ;
    skos:editorialNote "No occurrences of this slot in the graph." ;
    skos:inScheme okns:owl-rdf-rdfs ;
    skos:mappingRelation owl:unionOf ;
    linkml:definition_uri okns:owl_unionOf ;
    linkml:domain okns:RdfsClass ;
    linkml:inlined true ;
    linkml:owner okns:owl_unionOf ;
    linkml:range okns:RdfList ;
    linkml:slot_uri owl:unionOf .

okns:owl_versionIRI a linkml:SlotDefinition ;
    dcterms:source owl: ;
    dcterms:title "versionIRI" ;
    skos:definition "The property that identifies the version IRI of an ontology." ;
    skos:editorialNote "No occurrences of this slot in the graph." ;
    skos:inScheme okns:owl-rdf-rdfs ;
    skos:mappingRelation owl:versionIRI ;
    linkml:definition_uri okns:owl_versionIRI ;
    linkml:domain okns:OwlOntology ;
    linkml:inlined true ;
    linkml:owner okns:owl_versionIRI ;
    linkml:range okns:OwlOntology ;
    linkml:slot_uri owl:versionIRI .

okns:owl_versionInfo a linkml:SlotDefinition ;
    dcterms:source owl: ;
    dcterms:title "versionInfo" ;
    skos:definition "The annotation property that provides version information for an ontology or another OWL construct." ;
    skos:editorialNote "No occurrences of this slot in the graph." ;
    skos:inScheme okns:owl-rdf-rdfs ;
    skos:mappingRelation owl:versionInfo ;
    linkml:definition_uri okns:owl_versionInfo ;
    linkml:domain okns:RdfsResource ;
    linkml:inlined true ;
    linkml:owner okns:owl_versionInfo ;
    linkml:range okns:RdfsResource ;
    linkml:slot_uri owl:versionInfo .

okns:owl_withRestrictions a linkml:SlotDefinition ;
    dcterms:source owl: ;
    dcterms:title "withRestrictions" ;
    skos:definition "The property that determines the collection of facet-value pairs that define a datatype restriction." ;
    skos:editorialNote "No occurrences of this slot in the graph." ;
    skos:inScheme okns:owl-rdf-rdfs ;
    skos:mappingRelation owl:withRestrictions ;
    linkml:definition_uri okns:owl_withRestrictions ;
    linkml:domain okns:RdfsDatatype ;
    linkml:inlined true ;
    linkml:owner okns:owl_withRestrictions ;
    linkml:range okns:RdfList ;
    linkml:slot_uri owl:withRestrictions .

okns:rdf_direction a linkml:SlotDefinition ;
    dcterms:source rdf: ;
    dcterms:title "direction" ;
    rdfs:seeAlso <https://www.w3.org/TR/json-ld11/#the-rdf-compoundliteral-class-and-the-rdf-language-and-rdf-direction-properties> ;
    skos:definition "The base direction component of a CompoundLiteral." ;
    skos:editorialNote "No occurrences of this slot in the graph." ;
    skos:inScheme okns:owl-rdf-rdfs ;
    skos:mappingRelation rdf:direction ;
    linkml:definition_uri okns:rdf_direction ;
    linkml:domain okns:RdfCompoundLiteral ;
    linkml:inlined true ;
    linkml:owner okns:rdf_direction ;
    linkml:range okns:Any ;
    linkml:slot_uri rdf:direction .

okns:rdf_first a linkml:SlotDefinition ;
    dcterms:source rdf: ;
    dcterms:title "first" ;
    skos:definition "The first item in the subject RDF list." ;
    skos:editorialNote "No occurrences of this slot in the graph." ;
    skos:inScheme okns:owl-rdf-rdfs ;
    skos:mappingRelation rdf:first ;
    linkml:definition_uri okns:rdf_first ;
    linkml:domain okns:RdfList ;
    linkml:inlined true ;
    linkml:owner okns:rdf_first ;
    linkml:range okns:RdfsResource ;
    linkml:slot_uri rdf:first .

okns:rdf_language a linkml:SlotDefinition ;
    dcterms:source rdf: ;
    dcterms:title "language" ;
    rdfs:seeAlso <https://www.w3.org/TR/json-ld11/#the-rdf-compoundliteral-class-and-the-rdf-language-and-rdf-direction-properties> ;
    skos:definition "The language component of a CompoundLiteral." ;
    skos:editorialNote "No occurrences of this slot in the graph." ;
    skos:inScheme okns:owl-rdf-rdfs ;
    skos:mappingRelation rdf:language ;
    linkml:definition_uri okns:rdf_language ;
    linkml:domain okns:RdfCompoundLiteral ;
    linkml:inlined true ;
    linkml:owner okns:rdf_language ;
    linkml:range okns:Any ;
    linkml:slot_uri rdf:language .

okns:rdf_object a linkml:SlotDefinition ;
    dcterms:source rdf: ;
    dcterms:title "object" ;
    skos:definition "The object of the subject RDF statement." ;
    skos:editorialNote "No occurrences of this slot in the graph." ;
    skos:inScheme okns:owl-rdf-rdfs ;
    skos:mappingRelation rdf:object ;
    linkml:definition_uri okns:rdf_object ;
    linkml:domain okns:RdfStatement ;
    linkml:inlined true ;
    linkml:owner okns:rdf_object ;
    linkml:range okns:RdfsResource ;
    linkml:slot_uri rdf:object .

okns:rdf_predicate a linkml:SlotDefinition ;
    dcterms:source rdf: ;
    dcterms:title "predicate" ;
    skos:definition "The predicate of the subject RDF statement." ;
    skos:editorialNote "No occurrences of this slot in the graph." ;
    skos:inScheme okns:owl-rdf-rdfs ;
    skos:mappingRelation rdf:predicate ;
    linkml:definition_uri okns:rdf_predicate ;
    linkml:domain okns:RdfStatement ;
    linkml:inlined true ;
    linkml:owner okns:rdf_predicate ;
    linkml:range okns:RdfsResource ;
    linkml:slot_uri rdf:predicate .

okns:rdf_rest a linkml:SlotDefinition ;
    dcterms:source rdf: ;
    dcterms:title "rest" ;
    skos:definition "The rest of the subject RDF list after the first item." ;
    skos:editorialNote "No occurrences of this slot in the graph." ;
    skos:inScheme okns:owl-rdf-rdfs ;
    skos:mappingRelation rdf:rest ;
    linkml:definition_uri okns:rdf_rest ;
    linkml:domain okns:RdfList ;
    linkml:inlined true ;
    linkml:owner okns:rdf_rest ;
    linkml:range okns:RdfList ;
    linkml:slot_uri rdf:rest .

okns:rdf_subject a linkml:SlotDefinition ;
    dcterms:source rdf: ;
    dcterms:title "subject" ;
    skos:definition "The subject of the subject RDF statement." ;
    skos:editorialNote "No occurrences of this slot in the graph." ;
    skos:inScheme okns:owl-rdf-rdfs ;
    skos:mappingRelation rdf:subject ;
    linkml:definition_uri okns:rdf_subject ;
    linkml:domain okns:RdfStatement ;
    linkml:inlined true ;
    linkml:owner okns:rdf_subject ;
    linkml:range okns:RdfsResource ;
    linkml:slot_uri rdf:subject .

okns:rdf_type a linkml:SlotDefinition ;
    dcterms:source rdf: ;
    dcterms:title "type" ;
    skos:definition "The subject is an instance of a class." ;
    skos:editorialNote "No occurrences of this slot in the graph." ;
    skos:inScheme okns:owl-rdf-rdfs ;
    skos:mappingRelation rdf:type ;
    linkml:definition_uri okns:rdf_type ;
    linkml:domain okns:RdfsResource ;
    linkml:inlined true ;
    linkml:owner okns:rdf_type ;
    linkml:range okns:RdfsClass ;
    linkml:slot_uri rdf:type .

okns:rdf_value a linkml:SlotDefinition ;
    dcterms:source rdf: ;
    dcterms:title "value" ;
    skos:definition "Idiomatic property used for structured values." ;
    skos:editorialNote "No occurrences of this slot in the graph." ;
    skos:inScheme okns:owl-rdf-rdfs ;
    skos:mappingRelation rdf:value ;
    linkml:definition_uri okns:rdf_value ;
    linkml:domain okns:RdfsResource ;
    linkml:inlined true ;
    linkml:owner okns:rdf_value ;
    linkml:range okns:RdfsResource ;
    linkml:slot_uri rdf:value .

okns:rdfs_domain a linkml:SlotDefinition ;
    dcterms:source rdfs: ;
    dcterms:title "domain" ;
    skos:definition "A domain of the subject property." ;
    skos:editorialNote "No occurrences of this slot in the graph." ;
    skos:inScheme okns:owl-rdf-rdfs ;
    skos:mappingRelation rdfs:domain ;
    linkml:definition_uri okns:rdfs_domain ;
    linkml:domain okns:RdfProperty ;
    linkml:inlined true ;
    linkml:owner okns:rdfs_domain ;
    linkml:range okns:RdfsClass ;
    linkml:slot_uri rdfs:domain .

okns:rdfs_member a linkml:SlotDefinition ;
    dcterms:source rdfs: ;
    dcterms:title "member" ;
    skos:definition "A member of the subject resource." ;
    skos:editorialNote "No occurrences of this slot in the graph." ;
    skos:inScheme okns:owl-rdf-rdfs ;
    skos:mappingRelation rdfs:member ;
    linkml:definition_uri okns:rdfs_member ;
    linkml:domain okns:RdfsResource ;
    linkml:inlined true ;
    linkml:owner okns:rdfs_member ;
    linkml:range okns:RdfsResource ;
    linkml:slot_uri rdfs:member .

okns:rdfs_range a linkml:SlotDefinition ;
    dcterms:source rdfs: ;
    dcterms:title "range" ;
    skos:definition "A range of the subject property." ;
    skos:editorialNote "No occurrences of this slot in the graph." ;
    skos:inScheme okns:owl-rdf-rdfs ;
    skos:mappingRelation rdfs:range ;
    linkml:definition_uri okns:rdfs_range ;
    linkml:domain okns:RdfProperty ;
    linkml:inlined true ;
    linkml:owner okns:rdfs_range ;
    linkml:range okns:RdfsClass ;
    linkml:slot_uri rdfs:range .

okns:rdfs_subPropertyOf a linkml:SlotDefinition ;
    dcterms:source rdfs: ;
    dcterms:title "subPropertyOf" ;
    skos:definition "The subject is a subproperty of a property." ;
    skos:editorialNote "No occurrences of this slot in the graph." ;
    skos:inScheme okns:owl-rdf-rdfs ;
    skos:mappingRelation rdfs:subPropertyOf ;
    linkml:definition_uri okns:rdfs_subPropertyOf ;
    linkml:domain okns:RdfProperty ;
    linkml:inlined true ;
    linkml:owner okns:rdfs_subPropertyOf ;
    linkml:range okns:RdfProperty ;
    linkml:slot_uri rdfs:subPropertyOf .

okns:RdfCompoundLiteral a linkml:ClassDefinition ;
    dcterms:source rdf: ;
    dcterms:title "CompoundLiteral" ;
    rdfs:seeAlso <https://www.w3.org/TR/json-ld11/#the-rdf-compoundliteral-class-and-the-rdf-language-and-rdf-direction-properties> ;
    skos:definition "A class representing a compound literal." ;
    skos:inScheme okns:owl-rdf-rdfs ;
    skos:mappingRelation rdf:CompoundLiteral ;
    linkml:class_uri rdf:CompoundLiteral ;
    linkml:definition_uri okns:RdfCompoundLiteral ;
    linkml:is_a okns:RdfsResource ;
    linkml:slot_usage [ ] .

okns:float a linkml:TypeDefinition ;
    skos:definition "A real number that conforms to the xsd:float specification" ;
    skos:editorialNote "If you are authoring schemas in LinkML YAML, the type is referenced with the lower case \"float\"." ;
    skos:exactMatch schema1:Float ;
    skos:inScheme linkml:types ;
    linkml:base "float" ;
    linkml:definition_uri linkml:Float ;
    linkml:imported_from "linkml:types" ;
    linkml:uri xsd:float .

okns:token a linkml:TypeDefinition ;
    skos:definition "Tokenized string, one that does not contain the carriage return (#xD), line feed (#xA) nor tab (#x9) characters, that has no leading or trailing spaces (#x20) and that has no internal sequences of two or more spaces." ;
    skos:inScheme okns:extended_types ;
    skos:note "added by Mahir Morshed <mmorshed@scripps.edu>" ;
    linkml:base "str" ;
    linkml:definition_uri linkml:Token ;
    linkml:typeof okns:normalizedstring ;
    linkml:uri xsd:token .

okns:RdfStatement a linkml:ClassDefinition ;
    dcterms:source rdf: ;
    dcterms:title "Statement" ;
    skos:definition "The class of RDF statements." ;
    skos:inScheme okns:owl-rdf-rdfs ;
    skos:mappingRelation rdf:Statement ;
    linkml:class_uri rdf:Statement ;
    linkml:definition_uri okns:RdfStatement ;
    linkml:is_a okns:RdfsResource ;
    linkml:slot_usage [ ] .

okns:RdfsContainer a linkml:ClassDefinition ;
    dcterms:source rdfs: ;
    dcterms:title "Container" ;
    skos:definition "The class of RDF containers." ;
    skos:inScheme okns:owl-rdf-rdfs ;
    skos:mappingRelation rdfs:Container ;
    linkml:class_uri rdfs:Container ;
    linkml:definition_uri okns:RdfsContainer ;
    linkml:is_a okns:RdfsResource ;
    linkml:slot_usage [ ] .

okns:rdfs_subClassOf a linkml:SlotDefinition ;
    dcterms:source rdfs: ;
    dcterms:title "subClassOf" ;
    skos:definition "The subject is a subclass of a class." ;
    skos:inScheme okns:owl-rdf-rdfs ;
    skos:mappingRelation rdfs:subClassOf ;
    linkml:definition_uri okns:rdfs_subClassOf ;
    linkml:domain okns:RdfsClass ;
    linkml:domain_of okns:RdfsDatatype ;
    linkml:inlined true ;
    linkml:owner okns:rdfs_subClassOf ;
    linkml:range okns:RdfsClass ;
    linkml:slot_uri rdfs:subClassOf .

okns:signedinteger a linkml:TypeDefinition ;
    rdfs:seeAlso <https://numpy.org/doc/stable/reference/arrays.scalars.html#numpy.signedinteger> ;
    skos:definition "An integer that may be negative" ;
    skos:inScheme okns:extended_types ;
    linkml:base "int" ;
    linkml:definition_uri linkml:Signedinteger ;
    linkml:typeof okns:integer ;
    linkml:uri xsd:integer .

okns:uri a linkml:TypeDefinition ;
    dcterms:conformsTo "https://www.ietf.org/rfc/rfc3987.txt" ;
    skos:closeMatch schema1:URL ;
    skos:definition "a complete URI" ;
    skos:editorialNote "If you are authoring schemas in LinkML YAML, the type is referenced with the lower case \"uri\"." ;
    skos:inScheme linkml:types ;
    skos:note "in RDF serializations a slot with range of uri is treated as a literal or type xsd:anyURI unless it is an identifier or a reference to an identifier, in which case it is translated directly to a node" ;
    linkml:base "URI" ;
    linkml:definition_uri linkml:Uri ;
    linkml:imported_from "linkml:types" ;
    linkml:repr "str" ;
    linkml:uri xsd:anyURI .

okns:OwlNegativePropertyAssertion a linkml:ClassDefinition ;
    dcterms:source owl: ;
    dcterms:title "NegativePropertyAssertion" ;
    skos:definition "The class of negative property assertions." ;
    skos:inScheme okns:owl-rdf-rdfs ;
    skos:mappingRelation owl:NegativePropertyAssertion ;
    linkml:class_uri owl:NegativePropertyAssertion ;
    linkml:definition_uri okns:OwlNegativePropertyAssertion ;
    linkml:is_a okns:RdfsResource ;
    linkml:slot_usage [ ] .

okns:integer a linkml:TypeDefinition ;
    skos:definition "An integer" ;
    skos:editorialNote "If you are authoring schemas in LinkML YAML, the type is referenced with the lower case \"integer\"." ;
    skos:exactMatch schema1:Integer ;
    skos:inScheme linkml:types ;
    linkml:base "int" ;
    linkml:definition_uri linkml:Integer ;
    linkml:imported_from "linkml:types" ;
    linkml:uri xsd:integer .

okns:rdfs_comment a linkml:SlotDefinition ;
    dcterms:source rdfs: ;
    dcterms:title "comment" ;
    skos:definition "A description of the subject resource." ;
    skos:inScheme okns:owl-rdf-rdfs ;
    skos:mappingRelation rdfs:comment ;
    linkml:any_of [ a linkml:AnonymousSlotExpression ;
            linkml:range okns:RdfsLiteral ],
        [ a linkml:AnonymousSlotExpression ;
            linkml:range okns:string ] ;
    linkml:definition_uri okns:rdfs_comment ;
    linkml:domain okns:RdfsResource ;
    linkml:domain_of okns:RdfList,
        okns:RdfsDatatype ;
    linkml:inlined true ;
    linkml:owner okns:rdfs_comment ;
    linkml:range okns:Any ;
    linkml:slot_uri rdfs:comment .

okns:rdfs_isDefinedBy a linkml:SlotDefinition ;
    dcterms:source rdfs: ;
    dcterms:title "isDefinedBy" ;
    rdfs:subPropertyOf okns:rdfs_seeAlso ;
    skos:definition "The definition of the subject resource." ;
    skos:inScheme okns:owl-rdf-rdfs ;
    skos:mappingRelation rdfs:isDefinedBy ;
    linkml:any_of [ a linkml:AnonymousSlotExpression ;
            linkml:range okns:OwlOntology ],
        [ a linkml:AnonymousSlotExpression ;
            linkml:range okns:RdfsResource ] ;
    linkml:definition_uri okns:rdfs_isDefinedBy ;
    linkml:domain okns:RdfsResource ;
    linkml:domain_of okns:RdfList,
        okns:RdfsDatatype ;
    linkml:inlined true ;
    linkml:owner okns:rdfs_isDefinedBy ;
    linkml:range okns:Any ;
    linkml:slot_uri rdfs:isDefinedBy .

okns:rdfs_label a linkml:SlotDefinition ;
    dcterms:source rdfs: ;
    dcterms:title "label" ;
    skos:definition "A human-readable name for the subject." ;
    skos:inScheme okns:owl-rdf-rdfs ;
    skos:mappingRelation rdfs:label ;
    linkml:any_of [ a linkml:AnonymousSlotExpression ;
            linkml:range okns:RdfsLiteral ],
        [ a linkml:AnonymousSlotExpression ;
            linkml:range okns:string ] ;
    linkml:definition_uri okns:rdfs_label ;
    linkml:domain okns:RdfsResource ;
    linkml:domain_of okns:RdfList,
        okns:RdfsDatatype ;
    linkml:inlined true ;
    linkml:owner okns:rdfs_label ;
    linkml:range okns:Any ;
    linkml:slot_uri rdfs:label .

okns:rdfs_seeAlso a linkml:SlotDefinition ;
    dcterms:source rdfs: ;
    dcterms:title "seeAlso" ;
    skos:definition "Further information about the subject resource." ;
    skos:inScheme okns:owl-rdf-rdfs ;
    skos:mappingRelation rdfs:seeAlso ;
    linkml:any_of [ a linkml:AnonymousSlotExpression ;
            linkml:range okns:RdfsResource ],
        [ a linkml:AnonymousSlotExpression ;
            linkml:range okns:uri ] ;
    linkml:definition_uri okns:rdfs_seeAlso ;
    linkml:domain okns:RdfsResource ;
    linkml:domain_of okns:RdfsDatatype ;
    linkml:inlined true ;
    linkml:owner okns:rdfs_seeAlso ;
    linkml:range okns:Any ;
    linkml:slot_uri rdfs:seeAlso .

okns:RdfsLiteral a linkml:ClassDefinition ;
    dcterms:source rdfs: ;
    dcterms:title "No (data)type name specified -- this type is noted as a supertype of another type in this graph but has not itself been defined." ;
    skos:definition "The class of literal values, eg. textual strings and integers." ;
    skos:inScheme okns:owl-rdf-rdfs ;
    skos:mappingRelation rdfs:Literal ;
    linkml:class_uri rdfs:Literal ;
    linkml:definition_uri okns:RdfsLiteral ;
    linkml:is_a okns:RdfsResource ;
    linkml:slot_usage [ ] .

okns:OwlClass a linkml:ClassDefinition ;
    dcterms:source owl: ;
    dcterms:title "Class" ;
    skos:definition "The class of OWL classes." ;
    skos:inScheme okns:owl-rdf-rdfs ;
    skos:mappingRelation owl:Class ;
    linkml:class_uri owl:Class ;
    linkml:definition_uri okns:OwlClass ;
    linkml:is_a okns:RdfsClass ;
    linkml:slot_usage [ ] .

okns:OwlObjectProperty a linkml:ClassDefinition ;
    dcterms:source owl: ;
    dcterms:title "ObjectProperty" ;
    skos:definition "The class of object properties." ;
    skos:inScheme okns:owl-rdf-rdfs ;
    skos:mappingRelation owl:ObjectProperty ;
    linkml:class_uri owl:ObjectProperty ;
    linkml:definition_uri okns:OwlObjectProperty ;
    linkml:is_a okns:RdfProperty ;
    linkml:slot_usage [ ] .

okns:unsignedinteger a linkml:TypeDefinition ;
    rdfs:seeAlso <https://numpy.org/doc/stable/reference/arrays.scalars.html#numpy.unsignedinteger>,
        <https://www.w3.org/TR/xmlschema-2/#nonNegativeInteger> ;
    skos:definition "An integer that is non-negative" ;
    skos:inScheme okns:extended_types ;
    linkml:base "int" ;
    linkml:definition_uri linkml:Unsignedinteger ;
    linkml:minimum_value "0"^^<https://w3id.org/linkml/@id> ;
    linkml:typeof okns:integer ;
    linkml:uri xsd:unsignedInt .

okns:OwlOntology a linkml:ClassDefinition ;
    dcterms:source owl: ;
    dcterms:title "Ontology" ;
    skos:definition "The class of ontologies." ;
    skos:inScheme okns:owl-rdf-rdfs ;
    skos:mappingRelation owl:Ontology ;
    linkml:class_uri owl:Ontology ;
    linkml:definition_uri okns:OwlOntology ;
    linkml:is_a okns:RdfsResource ;
    linkml:slot_usage [ ] .

okns:RdfsDatatype a linkml:ClassDefinition ;
    dcterms:source rdfs: ;
    dcterms:title "Datatype" ;
    skos:definition "The class of RDF datatypes." ;
    skos:inScheme okns:owl-rdf-rdfs ;
    skos:mappingRelation rdfs:Datatype ;
    linkml:class_uri rdfs:Datatype ;
    linkml:definition_uri okns:RdfsDatatype ;
    linkml:is_a okns:RdfsClass ;
    linkml:slot_usage [ ] ;
    linkml:slots okns:rdfs_comment,
        okns:rdfs_isDefinedBy,
        okns:rdfs_label,
        okns:rdfs_seeAlso,
        okns:rdfs_subClassOf .

okns:OwlRestriction a linkml:ClassDefinition ;
    dcterms:source owl: ;
    dcterms:title "Restriction" ;
    skos:definition "The class of property restrictions." ;
    skos:inScheme okns:owl-rdf-rdfs ;
    skos:mappingRelation owl:Restriction ;
    linkml:class_uri owl:Restriction ;
    linkml:definition_uri okns:OwlRestriction ;
    linkml:is_a okns:OwlClass ;
    linkml:slot_usage [ ] .

okns:OwlThing a linkml:ClassDefinition ;
    dcterms:source owl: ;
    dcterms:title "Thing" ;
    skos:definition "The class of OWL individuals." ;
    skos:inScheme okns:owl-rdf-rdfs ;
    skos:mappingRelation owl:Thing ;
    linkml:class_uri owl:Thing ;
    linkml:definition_uri okns:OwlThing ;
    linkml:slot_usage [ ] .

okns:string a linkml:TypeDefinition ;
    skos:definition "A character string" ;
    skos:editorialNote "In RDF serializations, a slot with range of string is treated as a literal or type xsd:string.   If you are authoring schemas in LinkML YAML, the type is referenced with the lower case \"string\"." ;
    skos:exactMatch schema1:Text ;
    skos:inScheme linkml:types ;
    linkml:base "str" ;
    linkml:definition_uri linkml:String ;
    linkml:imported_from "linkml:types" ;
    linkml:uri xsd:string .

okns:RdfsClass a linkml:ClassDefinition ;
    dcterms:source rdfs: ;
    dcterms:title "Class" ;
    skos:definition "The class of classes." ;
    skos:inScheme okns:owl-rdf-rdfs ;
    skos:mappingRelation rdfs:Class ;
    linkml:class_uri rdfs:Class ;
    linkml:definition_uri okns:RdfsClass ;
    linkml:is_a okns:RdfsResource ;
    linkml:slot_usage [ ] .

okns:RdfList a linkml:ClassDefinition ;
    dcterms:source rdf: ;
    dcterms:title "List" ;
    skos:definition "The class of RDF Lists." ;
    skos:inScheme okns:owl-rdf-rdfs ;
    skos:mappingRelation rdf:List ;
    linkml:class_uri rdf:List ;
    linkml:definition_uri okns:RdfList ;
    linkml:is_a okns:RdfsResource ;
    linkml:slot_usage [ ] ;
    linkml:slots okns:rdfs_comment,
        okns:rdfs_isDefinedBy,
        okns:rdfs_label .

okns:RdfProperty a linkml:ClassDefinition ;
    dcterms:source rdf: ;
    dcterms:title "Property" ;
    skos:definition "The class of RDF properties." ;
    skos:inScheme okns:owl-rdf-rdfs ;
    skos:mappingRelation rdf:Property ;
    linkml:class_uri rdf:Property ;
    linkml:definition_uri okns:RdfProperty ;
    linkml:is_a okns:RdfsResource ;
    linkml:slot_usage [ ] .

okns:RdfsResource a linkml:ClassDefinition ;
    dcterms:source rdfs: ;
    dcterms:title "Resource" ;
    skos:definition "The class resource, everything." ;
    skos:inScheme okns:owl-rdf-rdfs ;
    skos:mappingRelation rdfs:Resource ;
    linkml:class_uri rdfs:Resource ;
    linkml:definition_uri okns:RdfsResource ;
    linkml:slot_usage [ ] .

okns:xhv a linkml:SchemaDefinition ;
    dcterms:license "https://creativecommons.org/publicdomain/zero/1.0/" ;
    pav:createdOn "2025-09-03T11:21:48.287307"^^xsd:dateTime ;
    pav:lastUpdatedOn "2025-09-03T11:21:48.287307"^^xsd:dateTime ;
    sh:declare [ sh:namespace rdfs: ;
            sh:prefix "rdfs" ],
        [ sh:namespace okn: ;
            sh:prefix "okn" ],
        [ sh:namespace okns: ;
            sh:prefix "okns" ],
        [ sh:namespace rdf: ;
            sh:prefix "rdf" ],
        [ sh:namespace linkml: ;
            sh:prefix "linkml" ],
        [ sh:namespace <http://www.w3.org/1999/xhtml/vocab#> ;
            sh:prefix "xhv" ] ;
    linkml:annotations [ skos:example [ linkml:classes [ skos:example [ rdf:Bag [ skos:example 2 ;
                                            linkml:tag rdf:Bag ] ] ;
                            linkml:tag okns:classes ] ;
                    linkml:pairs [ skos:example [ rdfs:member [ skos:example [ rdf:Bag [ skos:example [ rdf:Bag [ skos:example 1 ;
                                                                            linkml:tag rdf:Bag ] ] ;
                                                            linkml:tag rdf:Bag ] ] ;
                                            linkml:tag rdfs:member ] ;
                                    ns1:stylesheet [ skos:example [ linkml:untyped [ skos:example [ linkml:uri [ skos:example 1 ;
                                                                            linkml:tag okns:uri ] ] ;
                                                            linkml:tag okns:untyped ] ] ;
                                            linkml:tag ns1:stylesheet ] ] ;
                            linkml:tag okns:pairs ] ;
                    linkml:slots [ skos:example [ rdfs:member [ skos:example 1 ;
                                            linkml:tag rdfs:member ] ;
                                    ns1:stylesheet [ skos:example 1 ;
                                            linkml:tag ns1:stylesheet ] ] ;
                            linkml:tag okns:slots ] ] ;
            linkml:tag okns:counts ],
        [ skos:example [ linkml:classes [ skos:example [ rdf:Bag [ skos:example "xhv:role-properties" ;
                                            linkml:tag rdf:Bag ] ] ;
                            linkml:tag okns:classes ] ;
                    linkml:pairs [ skos:example [ rdfs:member [ skos:example [ rdf:Bag [ skos:example [ rdf:Bag [ skos:example [ rdf:predicate [ skos:example "rdfs:member" ;
                                                                                            linkml:tag okns:predicate ] ;
                                                                                    linkml:object [ skos:example "xhv:role-properties" ;
                                                                                            linkml:tag okns:object ] ;
                                                                                    linkml:subject [ skos:example "xhv:relrev-properties" ;
                                                                                            linkml:tag okns:subject ] ] ;
                                                                            linkml:tag rdf:Bag ] ] ;
                                                            linkml:tag rdf:Bag ] ] ;
                                            linkml:tag rdfs:member ] ;
                                    ns1:stylesheet [ skos:example [ linkml:untyped [ skos:example [ linkml:uri [ skos:example [ rdf:predicate [ skos:example "xhv:stylesheet" ;
                                                                                            linkml:tag okns:predicate ] ;
                                                                                    linkml:object [ skos:example "http://www.w3.org/StyleSheets/TR/base.css" ;
                                                                                            linkml:tag okns:object ] ;
                                                                                    linkml:subject [ skos:example "http://www.w3.org/1999/xhtml/vocab" ;
                                                                                            linkml:tag okns:subject ] ] ;
                                                                            linkml:tag okns:uri ] ] ;
                                                            linkml:tag okns:untyped ] ] ;
                                            linkml:tag ns1:stylesheet ] ] ;
                            linkml:tag okns:pairs ] ] ;
            linkml:tag okns:examples ] ;
    linkml:classes okns:Any,
        okns:OwlAllDifferent,
        okns:OwlAllDisjointClasses,
        okns:OwlAllDisjointProperties,
        okns:OwlAnnotation,
        okns:OwlAnnotationProperty,
        okns:OwlAsymmetricProperty,
        okns:OwlAxiom,
        okns:OwlClass,
        okns:OwlDataRange,
        okns:OwlDatatypeProperty,
        okns:OwlDeprecatedClass,
        okns:OwlDeprecatedProperty,
        okns:OwlFunctionalProperty,
        okns:OwlInverseFunctionalProperty,
        okns:OwlIrreflexiveProperty,
        okns:OwlNamedIndividual,
        okns:OwlNegativePropertyAssertion,
        okns:OwlNothing,
        okns:OwlObjectProperty,
        okns:OwlOntology,
        okns:OwlOntologyProperty,
        okns:OwlReflexiveProperty,
        okns:OwlRestriction,
        okns:OwlSymmetricProperty,
        okns:OwlThing,
        okns:OwlTransitiveProperty,
        okns:RdfAlt,
        okns:RdfBag,
        okns:RdfCompoundLiteral,
        okns:RdfList,
        okns:RdfProperty,
        okns:RdfSeq,
        okns:RdfStatement,
        okns:RdfsClass,
        okns:RdfsContainer,
        okns:RdfsContainerMembershipProperty,
        okns:RdfsDatatype,
        okns:RdfsLiteral,
        okns:RdfsResource ;
    linkml:default_prefix "okns" ;
    linkml:default_range okns:string ;
    linkml:generation_date "2025-09-04T07:22:59"^^xsd:dateTime ;
    linkml:id okns:xhv ;
    linkml:imports okns:extended_types,
        okns:owl-rdf-rdfs,
        linkml:types ;
    linkml:metamodel_version "1.7.0" ;
    linkml:slots okns:langrange,
        okns:length,
        okns:maxexclusive,
        okns:maxlength,
        okns:minexclusive,
        okns:minlength,
        okns:owl_allValuesFrom,
        okns:owl_annotatedProperty,
        okns:owl_annotatedSource,
        okns:owl_annotatedTarget,
        okns:owl_assertionProperty,
        okns:owl_backwardCompatibleWith,
        okns:owl_bottomDataProperty,
        okns:owl_bottomObjectProperty,
        okns:owl_cardinality,
        okns:owl_complementOf,
        okns:owl_datatypeComplementOf,
        okns:owl_deprecated,
        okns:owl_differentFrom,
        okns:owl_disjointUnionOf,
        okns:owl_disjointWith,
        okns:owl_distinctMembers,
        okns:owl_equivalentClass,
        okns:owl_equivalentProperty,
        okns:owl_hasKey,
        okns:owl_hasSelf,
        okns:owl_hasValue,
        okns:owl_imports,
        okns:owl_incompatibleWith,
        okns:owl_intersectionOf,
        okns:owl_inverseOf,
        okns:owl_maxCardinality,
        okns:owl_maxQualifiedCardinality,
        okns:owl_members,
        okns:owl_minCardinality,
        okns:owl_minQualifiedCardinality,
        okns:owl_onClass,
        okns:owl_onDataRange,
        okns:owl_onDatatype,
        okns:owl_onProperties,
        okns:owl_onProperty,
        okns:owl_oneOf,
        okns:owl_priorVersion,
        okns:owl_propertyChainAxiom,
        okns:owl_propertyDisjointWith,
        okns:owl_qualifiedCardinality,
        okns:owl_sameAs,
        okns:owl_someValuesFrom,
        okns:owl_sourceIndividual,
        okns:owl_targetIndividual,
        okns:owl_targetValue,
        okns:owl_topDataProperty,
        okns:owl_topObjectProperty,
        okns:owl_unionOf,
        okns:owl_versionIRI,
        okns:owl_versionInfo,
        okns:owl_withRestrictions,
        okns:rdf_direction,
        okns:rdf_first,
        okns:rdf_language,
        okns:rdf_object,
        okns:rdf_predicate,
        okns:rdf_rest,
        okns:rdf_subject,
        okns:rdf_type,
        okns:rdf_value,
        okns:rdfs_comment,
        okns:rdfs_domain,
        okns:rdfs_isDefinedBy,
        okns:rdfs_label,
        okns:rdfs_member,
        okns:rdfs_range,
        okns:rdfs_seeAlso,
        okns:rdfs_subClassOf,
        okns:rdfs_subPropertyOf,
        okns:xhv_alert,
        okns:xhv_alertdialog,
        okns:xhv_alternate,
        okns:xhv_appendix,
        okns:xhv_application,
        okns:xhv_article,
        okns:xhv_banner,
        okns:xhv_bookmark,
        okns:xhv_button,
        okns:xhv_chapter,
        okns:xhv_checkbox,
        okns:xhv_cite,
        okns:xhv_columnheader,
        okns:xhv_combobox,
        okns:xhv_complementary,
        okns:xhv_contentinfo,
        okns:xhv_contents,
        okns:xhv_copyright,
        okns:xhv_definition,
        okns:xhv_dialog,
        okns:xhv_directory,
        okns:xhv_document,
        okns:xhv_first,
        okns:xhv_form,
        okns:xhv_glossary,
        okns:xhv_grid,
        okns:xhv_gridcell,
        okns:xhv_group,
        okns:xhv_heading,
        okns:xhv_help,
        okns:xhv_icon,
        okns:xhv_img,
        okns:xhv_index,
        okns:xhv_itsRules,
        okns:xhv_last,
        okns:xhv_license,
        okns:xhv_link,
        okns:xhv_list,
        okns:xhv_listbox,
        okns:xhv_listitem,
        okns:xhv_log,
        okns:xhv_main,
        okns:xhv_marquee,
        okns:xhv_math,
        okns:xhv_menu,
        okns:xhv_menubar,
        okns:xhv_menuitem,
        okns:xhv_menuitemcheckbox,
        okns:xhv_menuitemradio,
        okns:xhv_meta,
        okns:xhv_navigation,
        okns:xhv_next,
        okns:xhv_note,
        okns:xhv_option,
        okns:xhv_p3pv1,
        okns:xhv_presentation,
        okns:xhv_prev,
        okns:xhv_progressbar,
        okns:xhv_radio,
        okns:xhv_radiogroup,
        okns:xhv_region,
        okns:xhv_role,
        okns:xhv_row,
        okns:xhv_rowgroup,
        okns:xhv_rowheader,
        okns:xhv_scrollbar,
        okns:xhv_search,
        okns:xhv_section,
        okns:xhv_separator,
        okns:xhv_slider,
        okns:xhv_spinbutton,
        okns:xhv_start,
        okns:xhv_status,
        okns:xhv_stylesheet,
        okns:xhv_subsection,
        okns:xhv_tab,
        okns:xhv_tablist,
        okns:xhv_tabpanel,
        okns:xhv_textbox,
        okns:xhv_timer,
        okns:xhv_toolbar,
        okns:xhv_tooltip,
        okns:xhv_top,
        okns:xhv_tree,
        okns:xhv_treegrid,
        okns:xhv_treeitem,
        okns:xhv_up ;
    linkml:source_file "xhv.yaml" ;
    linkml:source_file_date "2025-09-03T11:21:48"^^xsd:dateTime ;
    linkml:source_file_size 25388 ;
    linkml:types okns:base64binary,
        okns:boolean,
        okns:curie,
        okns:date,
        okns:date_or_datetime,
        okns:datetime,
        okns:decimal,
        okns:double,
        okns:float,
        okns:float16,
        okns:float32,
        okns:float64,
        okns:hexbinary,
        okns:int16,
        okns:int32,
        okns:int64,
        okns:int8,
        okns:integer,
        okns:jsonpath,
        okns:jsonpointer,
        okns:language,
        okns:name,
        okns:ncname,
        okns:negativeinteger,
        okns:nmtoken,
        okns:nodeidentifier,
        okns:nonpositiveinteger,
        okns:normalizedstring,
        okns:objectidentifier,
        okns:positiveinteger,
        okns:rational,
        okns:rdf_HTML,
        okns:rdf_JSON,
        okns:rdf_PlainLiteral,
        okns:rdf_XMLLiteral,
        okns:rdf_langString,
        okns:real,
        okns:signedinteger,
        okns:sparqlpath,
        okns:string,
        okns:time,
        okns:token,
        okns:uint16,
        okns:uint32,
        okns:uint64,
        okns:uint8,
        okns:unsignedinteger,
        okns:uri,
        okns:uriorcurie .

okns:Any a linkml:ClassDefinition ;
    skos:definition "An unconstrained type or object" ;
    skos:inScheme okns:extended_types ;
    skos:mappingRelation linkml:Any ;
    linkml:class_uri linkml:Any ;
    linkml:definition_uri linkml:Any ;
    linkml:slot_usage [ ] .


